<?xml version="1.0" encoding="UTF-8"?><?xml-stylesheet href="/VocabV2/skosrdf2html.xsl" type="text/xsl" media="screen"?><rdf:RDF xmlns:rdf="http://www.w3.org/1999/02/22-rdf-syntax-ns#" xmlns:skos="http://www.w3.org/2004/02/skos/core#" xmlns:dc="http://purl.org/dc/terms/" xmlns:dce="http://purl.org/dc/elements/1.1/" xmlns:rdfs="http://www.w3.org/2000/01/rdf-schema#" xmlns:grg="http://www.isotc211.org/schemas/grg/" xmlns:owl="http://www.w3.org/2002/07/owl#" xmlns:void="http://rdfs.org/ns/void#">
<skos:Collection rdf:about="http://vocab.nerc.ac.uk/collection/L08/current/">
<skos:prefLabel>SeaDataNet Data Access Restriction Policies</skos:prefLabel>
<dc:title>SeaDataNet Data Access Restriction Policies</dc:title>
<skos:altLabel>SeaDataNet Data Access Policies</skos:altLabel>
<dc:alternative>SeaDataNet Data Access Policies</dc:alternative>
<dc:description>Terms used to represent and classify data access policies in operation in the SeaDataNet project.</dc:description>
<dc:date>2012-05-17 02:00:03.0</dc:date>
<owl:versionInfo>3</owl:versionInfo>
<grg:RE_RegisterManager>British Oceanographic Data Centre</grg:RE_RegisterManager>
<dc:publisher>Natural Environment Research Council</dc:publisher>
<dc:creator>SeaDataNet</dc:creator>
<grg:RE_RegisterOwner>SeaDataNet</grg:RE_RegisterOwner>
<rdfs:comment>Governance for vocabularies used in the EU SeaDataNet project implemented as consultation between BODC and the members of the SeaDataNet Technical Task Team</rdfs:comment>
<skos:member>
<skos:Concept rdf:about="http://vocab.nerc.ac.uk/collection/L08/current/LS/">
<dc:identifier>SDN:L08::LS</dc:identifier>
<dce:identifier>SDN:L08::LS</dce:identifier>
<skos:notation>SDN:L08::LS</skos:notation>
<skos:prefLabel xml:lang="en">SeaDataNet licence</skos:prefLabel>
<skos:altLabel>SDN_licence</skos:altLabel>
<skos:definition xml:lang="en">Access to the data and usage are as specified in the SeaDataNet data policy and licence agreement</skos:definition>
<owl:versionInfo>1</owl:versionInfo>
<dc:date>2008-09-25 09:31:26.0</dc:date>
<skos:note xml:lang="en">accepted</skos:note>
<owl:deprecated>false</owl:deprecated>
<void:inDataset rdf:resource="http://vocab.nerc.ac.uk/.well-known/void"/>
</skos:Concept>
</skos:member>
<skos:member>
<skos:Concept rdf:about="http://vocab.nerc.ac.uk/collection/L08/current/SR/">
<dc:identifier>SDN:L08::SR</dc:identifier>
<dce:identifier>SDN:L08::SR</dce:identifier>
<skos:notation>SDN:L08::SR</skos:notation>
<skos:prefLabel xml:lang="en">academic</skos:prefLabel>
<skos:altLabel>academic</skos:altLabel>
<skos:definition xml:lang="en">The data are freely available for research and education purposes.  Usage acknowledgement is usually expected.</skos:definition>
<owl:versionInfo>1</owl:versionInfo>
<dc:date>2006-12-05 16:18:33.0</dc:date>
<skos:note xml:lang="en">accepted</skos:note>
<owl:deprecated>false</owl:deprecated>
<void:inDataset rdf:resource="http://vocab.nerc.ac.uk/.well-known/void"/>
</skos:Concept>
</skos:member>
<skos:member>
<skos:Concept rdf:about="http://vocab.nerc.ac.uk/collection/L08/current/RS/">
<dc:identifier>SDN:L08::RS</dc:identifier>
<dce:identifier>SDN:L08::RS</dce:identifier>
<skos:notation>SDN:L08::RS</skos:notation>
<skos:prefLabel xml:lang="en">by negotiation</skos:prefLabel>
<skos:altLabel>restricted</skos:altLabel>
<skos:definition xml:lang="en">The data are witheld from general circulation and disclosure but access may be obtained on a case-by-case basis through negotiation.</skos:definition>
<owl:versionInfo>2</owl:versionInfo>
<dc:date>2012-05-16 08:24:54.0</dc:date>
<skos:note xml:lang="en">accepted</skos:note>
<owl:deprecated>false</owl:deprecated>
<void:inDataset rdf:resource="http://vocab.nerc.ac.uk/.well-known/void"/>
</skos:Concept>
</skos:member>
<skos:member>
<skos:Concept rdf:about="http://vocab.nerc.ac.uk/collection/L08/current/CC/">
<dc:identifier>SDN:L08::CC</dc:identifier>
<dce:identifier>SDN:L08::CC</dce:identifier>
<skos:notation>SDN:L08::CC</skos:notation>
<skos:prefLabel xml:lang="en">collection cost charge</skos:prefLabel>
<skos:altLabel>collection_charge</skos:altLabel>
<skos:definition xml:lang="en">A charge is made related to the cost of collecting the data.</skos:definition>
<owl:versionInfo>1</owl:versionInfo>
<dc:date>2006-12-05 16:18:33.0</dc:date>
<skos:note xml:lang="en">accepted</skos:note>
<owl:deprecated>false</owl:deprecated>
<void:inDataset rdf:resource="http://vocab.nerc.ac.uk/.well-known/void"/>
</skos:Concept>
</skos:member>
<skos:member>
<skos:Concept rdf:about="http://vocab.nerc.ac.uk/collection/L08/current/FE/">
<dc:identifier>SDN:L08::FE</dc:identifier>
<dce:identifier>SDN:L08::FE</dce:identifier>
<skos:notation>SDN:L08::FE</skos:notation>
<skos:prefLabel xml:lang="en">commercial charge</skos:prefLabel>
<skos:altLabel>commercial_charge</skos:altLabel>
<skos:definition xml:lang="en">A charge significantly exceeding the cost of data collection and delivery is made for usage of the data.</skos:definition>
<owl:versionInfo>1</owl:versionInfo>
<dc:date>2006-12-05 16:18:33.0</dc:date>
<skos:note xml:lang="en">accepted</skos:note>
<owl:deprecated>false</owl:deprecated>
<void:inDataset rdf:resource="http://vocab.nerc.ac.uk/.well-known/void"/>
</skos:Concept>
</skos:member>
<skos:member>
<skos:Concept rdf:about="http://vocab.nerc.ac.uk/collection/L08/current/NC/">
<dc:identifier>SDN:L08::NC</dc:identifier>
<dce:identifier>SDN:L08::NC</dce:identifier>
<skos:notation>SDN:L08::NC</skos:notation>
<skos:prefLabel xml:lang="en">distribution cost charge</skos:prefLabel>
<skos:altLabel>distribution_charge</skos:altLabel>
<skos:definition xml:lang="en">A charge is made to cover the costs of delivering data to the user.</skos:definition>
<owl:versionInfo>1</owl:versionInfo>
<dc:date>2006-12-05 16:18:33.0</dc:date>
<skos:note xml:lang="en">accepted</skos:note>
<owl:deprecated>false</owl:deprecated>
<void:inDataset rdf:resource="http://vocab.nerc.ac.uk/.well-known/void"/>
</skos:Concept>
</skos:member>
<skos:member>
<skos:Concept rdf:about="http://vocab.nerc.ac.uk/collection/L08/current/LI/">
<dc:identifier>SDN:L08::LI</dc:identifier>
<dce:identifier>SDN:L08::LI</dce:identifier>
<skos:notation>SDN:L08::LI</skos:notation>
<skos:prefLabel xml:lang="en">licence</skos:prefLabel>
<skos:altLabel>licence</skos:altLabel>
<skos:definition xml:lang="en">Conditions of supply and usage of the data are specified in a formal agreement.</skos:definition>
<owl:versionInfo>1</owl:versionInfo>
<dc:date>2006-12-05 16:18:33.0</dc:date>
<skos:note xml:lang="en">accepted</skos:note>
<owl:deprecated>false</owl:deprecated>
<void:inDataset rdf:resource="http://vocab.nerc.ac.uk/.well-known/void"/>
</skos:Concept>
</skos:member>
<skos:member>
<skos:Concept rdf:about="http://vocab.nerc.ac.uk/collection/L08/current/MO/">
<dc:identifier>SDN:L08::MO</dc:identifier>
<dce:identifier>SDN:L08::MO</dce:identifier>
<skos:notation>SDN:L08::MO</skos:notation>
<skos:prefLabel xml:lang="en">moratorium</skos:prefLabel>
<skos:altLabel>moratorium</skos:altLabel>
<skos:definition xml:lang="en">Data are initially restricted, but the access condition relaxes to academic or unrestricted once a specified period of time after an event (such as collection, publication, completion of QC procedures or project cessation) has elapsed.</skos:definition>
<owl:versionInfo>1</owl:versionInfo>
<dc:date>2006-12-05 16:18:33.0</dc:date>
<skos:note xml:lang="en">accepted</skos:note>
<owl:deprecated>false</owl:deprecated>
<void:inDataset rdf:resource="http://vocab.nerc.ac.uk/.well-known/void"/>
</skos:Concept>
</skos:member>
<skos:member>
<skos:Concept rdf:about="http://vocab.nerc.ac.uk/collection/L08/current/NA/">
<dc:identifier>SDN:L08::NA</dc:identifier>
<dce:identifier>SDN:L08::NA</dce:identifier>
<skos:notation>SDN:L08::NA</skos:notation>
<skos:prefLabel xml:lang="en">no access</skos:prefLabel>
<skos:altLabel>none</skos:altLabel>
<skos:definition xml:lang="en">Access to the data cannot be negotiated.</skos:definition>
<owl:versionInfo>1</owl:versionInfo>
<dc:date>2006-12-05 16:18:33.0</dc:date>
<skos:note xml:lang="en">accepted</skos:note>
<owl:deprecated>false</owl:deprecated>
<void:inDataset rdf:resource="http://vocab.nerc.ac.uk/.well-known/void"/>
</skos:Concept>
</skos:member>
<skos:member>
<skos:Concept rdf:about="http://vocab.nerc.ac.uk/collection/L08/current/OG/">
<dc:identifier>SDN:L08::OG</dc:identifier>
<dce:identifier>SDN:L08::OG</dce:identifier>
<skos:notation>SDN:L08::OG</skos:notation>
<skos:prefLabel xml:lang="en">organisation</skos:prefLabel>
<skos:altLabel>organisation</skos:altLabel>
<skos:definition xml:lang="en">The data are unrestricted to members of an organisation or a virtual organisation (such as project or cruise participants) but restricted to anybody else.</skos:definition>
<owl:versionInfo>1</owl:versionInfo>
<dc:date>2006-12-05 16:18:33.0</dc:date>
<skos:note xml:lang="en">accepted</skos:note>
<owl:deprecated>false</owl:deprecated>
<void:inDataset rdf:resource="http://vocab.nerc.ac.uk/.well-known/void"/>
</skos:Concept>
</skos:member>
<skos:member>
<skos:Concept rdf:about="http://vocab.nerc.ac.uk/collection/L08/current/UK/">
<dc:identifier>SDN:L08::UK</dc:identifier>
<dce:identifier>SDN:L08::UK</dce:identifier>
<skos:notation>SDN:L08::UK</skos:notation>
<skos:prefLabel xml:lang="en">unknown</skos:prefLabel>
<skos:altLabel>unknown</skos:altLabel>
<skos:definition xml:lang="en">The correct value is not known to and not computable by the creator of this information. However a correct value probably exists.</skos:definition>
<owl:versionInfo>1</owl:versionInfo>
<dc:date>2006-12-05 16:18:33.0</dc:date>
<skos:note xml:lang="en">accepted</skos:note>
<owl:deprecated>false</owl:deprecated>
<void:inDataset rdf:resource="http://vocab.nerc.ac.uk/.well-known/void"/>
</skos:Concept>
</skos:member>
<skos:member>
<skos:Concept rdf:about="http://vocab.nerc.ac.uk/collection/L08/current/UN/">
<dc:identifier>SDN:L08::UN</dc:identifier>
<dce:identifier>SDN:L08::UN</dce:identifier>
<skos:notation>SDN:L08::UN</skos:notation>
<skos:prefLabel xml:lang="en">unrestricted</skos:prefLabel>
<skos:altLabel>unrestricted</skos:altLabel>
<skos:definition xml:lang="en">The data are freely available to anybody and may be used for any purpose. Usage acknowledgement may be required.</skos:definition>
<owl:versionInfo>1</owl:versionInfo>
<dc:date>2006-12-05 16:18:33.0</dc:date>
<skos:note xml:lang="en">accepted</skos:note>
<owl:deprecated>false</owl:deprecated>
<void:inDataset rdf:resource="http://vocab.nerc.ac.uk/.well-known/void"/>
</skos:Concept>
</skos:member>
</skos:Collection>
</rdf:RDF>
