<?xml version="1.0" encoding="UTF-8"?>
<rdf:RDF xmlns:rdf="http://www.w3.org/1999/02/22-rdf-syntax-ns#">
  <skos:ConceptScheme xmlns:skos="http://www.w3.org/2004/02/skos/core#" rdf:about="http://inspire.ec.europa.eu/theme">
    <dc:title xmlns:dc="http://purl.org/dc/elements/1.1/">GEMET - INSPIRE themes, version 1.0</dc:title>
    <dcterms:issued xmlns:dcterms="http://purl.org/dc/terms/">2008-06-01</dcterms:issued>
    <dcterms:modified xmlns:dcterms="http://purl.org/dc/terms/">2008-06-01</dcterms:modified>
  </skos:ConceptScheme>
  <skos:Concept xmlns:skos="http://www.w3.org/2004/02/skos/core#" rdf:about="http://inspire.ec.europa.eu/theme/ad">
    <skos:prefLabel xml:lang="en">Addresses</skos:prefLabel>
    <skos:scopeNote xml:lang="en">Location of properties based on address identifiers, usually by road name, house number, postal code.</skos:scopeNote>
    <skos:prefLabel xml:lang="bg">Адреси</skos:prefLabel>
    <skos:scopeNote xml:lang="bg">Местонахождение на имоти, обозначено чрез адресни данни, обичайно чрез наименование на улица, номер на сграда и пощенски код.</skos:scopeNote>
    <skos:prefLabel xml:lang="cs">Adresy</skos:prefLabel>
    <skos:scopeNote xml:lang="cs">Poloha nemovitostí podle adresních identifikátorů, obvykle pomocí názvu ulice, čísla domu, poštovního směrovacího čísla.</skos:scopeNote>
    <skos:prefLabel xml:lang="hr">Adrese</skos:prefLabel>
    <skos:scopeNote xml:lang="hr">Položaj nekretnina koji se temelji na identifikatoru adresa, najčešće s imenom ulice, kućnim brojem i poštanskim brojem.</skos:scopeNote>
    <skos:prefLabel xml:lang="da">Adresser</skos:prefLabel>
    <skos:scopeNote xml:lang="da">Lokalisering af ejendomme på grundlag af adresseidenter, normalt ved hjælp af vejnavn, husnummer og postnummer.</skos:scopeNote>
    <skos:prefLabel xml:lang="de">Adressen</skos:prefLabel>
    <skos:scopeNote xml:lang="de">Lokalisierung von Grundstücken anhand von Adressdaten, in der Regel Straßenname, Hausnummer und Postleitzahl.</skos:scopeNote>
    <skos:prefLabel xml:lang="el">Διευθύνσεις</skos:prefLabel>
    <skos:scopeNote xml:lang="el">Θέση ακινήτων με βάση τη διεύθυνση, συνήθως με όνομα οδού, αριθμό οικίας και ταχυδρομικό κώδικα.</skos:scopeNote>
    <skos:prefLabel xml:lang="es">Direcciones</skos:prefLabel>
    <skos:scopeNote xml:lang="es">Localización de las propiedades, basada en identificadores de direcciones, por ejemplo, el nombre de la vía pública, el número de la finca, el código postal.</skos:scopeNote>
    <skos:prefLabel xml:lang="et">Aadressid</skos:prefLabel>
    <skos:scopeNote xml:lang="et">Maavalduste asukoht aadressi elementide, tavaliselt tee või tänava nime, majanumbri ja postiindeksi järgi.</skos:scopeNote>
    <skos:prefLabel xml:lang="fi">Osoitteet</skos:prefLabel>
    <skos:scopeNote xml:lang="fi">Kiinteistöjen sijainti, joka perustuu osoitetietoon, jossa tavallisesti kadunnimi, talon numero ja postinumero.</skos:scopeNote>
    <skos:prefLabel xml:lang="fr">Adresses</skos:prefLabel>
    <skos:scopeNote xml:lang="fr">Localisation des propriétés fondée sur les identifiants des adresses, habituellement le nom de la rue, le numéro de la maison et le code postal.</skos:scopeNote>
    <skos:prefLabel xml:lang="hu">Címek</skos:prefLabel>
    <skos:scopeNote xml:lang="hu">Az ingatlanok helye címazonosítók – rendszerint utcanév, házszám, irányítószám – alapján.</skos:scopeNote>
    <skos:prefLabel xml:lang="it">Indirizzi</skos:prefLabel>
    <skos:scopeNote xml:lang="it">Localizzazione delle proprietà basata su identificatori di indirizzo, in genere nome della via, numero civico, codice postale.</skos:scopeNote>
    <skos:prefLabel xml:lang="lt">Adresai</skos:prefLabel>
    <skos:scopeNote xml:lang="lt">Nuosavybės vieta pagal adreso duomenis, paprastai gatvės pavadinimą, namo numerį, pašto kodą.</skos:scopeNote>
    <skos:prefLabel xml:lang="lv">Adreses</skos:prefLabel>
    <skos:scopeNote xml:lang="lv">Īpašumu ģeogrāfiskā atrašanās vieta, pamatojoties uz adreses identifikatoriem; parasti tie ir ceļu nosaukumi, māju numuri, pasta indeksi.</skos:scopeNote>
    <skos:prefLabel xml:lang="mt">Indirizzi</skos:prefLabel>
    <skos:scopeNote xml:lang="mt">Pożizzjoni ta' proprjetajiet ibbażata fuq identifikaturi ta' l-indirizzi, normalment bl-isem tat-triq, in-numru tad-dar, il-kodiċi postali.</skos:scopeNote>
    <skos:prefLabel xml:lang="nl">Adressen</skos:prefLabel>
    <skos:scopeNote xml:lang="nl">Locatie van onroerende zaken, gebaseerd op adresaanduidingen, gewoonlijk aan de hand van de straatnaam, het huisnummer en de postcode.</skos:scopeNote>
    <skos:prefLabel xml:lang="pl">Adresy</skos:prefLabel>
    <skos:scopeNote xml:lang="pl">Lokalizacja nieruchomości na podstawie danych adresowych, zazwyczaj nazwy ulicy, numeru budynku, kodu pocztowego.</skos:scopeNote>
    <skos:prefLabel xml:lang="pt">Endereços</skos:prefLabel>
    <skos:scopeNote xml:lang="pt">Localização de propriedades com base em identificadores de endereço, em regra, o nome da rua, o número da porta e o código postal.</skos:scopeNote>
    <skos:prefLabel xml:lang="ro">Adrese</skos:prefLabel>
    <skos:scopeNote xml:lang="ro">Localizare a proprietăților, bazată pe identificatori de adresă, de obicei numele străzii, numărul casei și codul poștal.</skos:scopeNote>
    <skos:prefLabel xml:lang="sk">Adresy</skos:prefLabel>
    <skos:scopeNote xml:lang="sk">Poloha nehnuteľností založená na identifikátoroch obsiahnutých v adrese, obyčajne podľa názvu ulice, čísla domu, poštového smerovacieho čísla.</skos:scopeNote>
    <skos:prefLabel xml:lang="sl">Naslovi</skos:prefLabel>
    <skos:scopeNote xml:lang="sl">Lokacija nepremičnin, ki temelji na identifikatorjih naslova, običajno z imenom ulice, hišno številko, poštno številko.</skos:scopeNote>
    <skos:prefLabel xml:lang="sv">Adresser</skos:prefLabel>
    <skos:scopeNote xml:lang="sv">Läge för fastigheter på grundval av adressuppgifter, vanligen i form av gatunamn, gatunummer och postnummer.</skos:scopeNote>
    <skos:altLabel>ad</skos:altLabel>
    <skos:inScheme rdf:resource="http://inspire.ec.europa.eu/theme" />
  </skos:Concept>
  <skos:Concept xmlns:skos="http://www.w3.org/2004/02/skos/core#" rdf:about="http://inspire.ec.europa.eu/theme/au">
    <skos:prefLabel xml:lang="en">Administrative units</skos:prefLabel>
    <skos:scopeNote xml:lang="en">Units of administration, dividing areas where Member States have and/or exercise jurisdictional rights, for local, regional and national governance, separated by administrative boundaries.</skos:scopeNote>
    <skos:prefLabel xml:lang="bg">Административни единици</skos:prefLabel>
    <skos:scopeNote xml:lang="bg">Административни единици, отделени с административни граници и отграничаващи райони, върху които държавите- членки имат и/или упражняват юридически правомощия, за целите на местното, регионалното и националното управление.</skos:scopeNote>
    <skos:prefLabel xml:lang="cs">Správní jednotky</skos:prefLabel>
    <skos:scopeNote xml:lang="cs">Správní jednotky rozdělující území, ve kterém členské státy mají nebo vykonávají svrchovaná práva, pro účely místní, regionální a státní správy, oddělené správními hranicemi.</skos:scopeNote>
    <skos:prefLabel xml:lang="hr">Administrativne jedinice</skos:prefLabel>
    <skos:scopeNote xml:lang="hr">Upravne jedinice za lokalnu, regionalnu ili državnu upravu, koje razdjeljuju područja na kojima države članice imaju i/ili primjenjuju jurisdikcijska prava i koje su razdvojene administrativnim granicama.</skos:scopeNote>
    <skos:prefLabel xml:lang="da">Administrative enheder</skos:prefLabel>
    <skos:scopeNote xml:lang="da">Forvaltningsenheder, der inddeler områder, hvor medlemsstaterne har og/eller udøver jurisdiktionelle rettigheder på lokalt, regionalt og nationalt plan, adskilt af administrative grænser.</skos:scopeNote>
    <skos:prefLabel xml:lang="de">Verwaltungseinheiten</skos:prefLabel>
    <skos:scopeNote xml:lang="de">Lokale, regionale und nationale Verwaltungseinheiten, die die Gebiete abgrenzen, in denen die Mitgliedstaaten Hoheitsbefugnisse haben und/oder ausüben und die durch Verwaltungsgrenzen voneinander getrennt sind.</skos:scopeNote>
    <skos:prefLabel xml:lang="el">Διοικητικές ενότητες</skos:prefLabel>
    <skos:scopeNote xml:lang="el">Διοικητικές ενότητες που χωρίζουν περιοχές επί των οποίων κράτη μέλη έχουν ή/και ασκούν δικαιοδοτικά δικαιώματα σε τοπικό, περιφερειακό και εθνικό επίπεδο, χωρίζονται από διοικητικά όρια.</skos:scopeNote>
    <skos:prefLabel xml:lang="es">Unidades administrativas</skos:prefLabel>
    <skos:scopeNote xml:lang="es">Unidades administrativas en que se dividan las áreas en las que los Estados miembros tienen y/o ejercen derechos jurisdiccionales, a efectos de administración local, regional y nacional, separadas por límites administrativos.</skos:scopeNote>
    <skos:prefLabel xml:lang="et">Haldusüksused</skos:prefLabel>
    <skos:scopeNote xml:lang="et">Halduspiiridega eraldatud haldusüksused, mis jagavad liikmesriikide jurisdiktsiooni all olevad alad kohaliku, piirkondliku ja riikliku juhtimise eesmärgil.</skos:scopeNote>
    <skos:prefLabel xml:lang="fi">Hallinnolliset yksiköt</skos:prefLabel>
    <skos:scopeNote xml:lang="fi">Hallinnolliset yksiköt, jotka jakavat alueen, jolla jäsenvaltioilla on tai jolla ne käyttävät lainkäyttöoikeuksia, paikalliseen, alueelliseen ja valtakunnalliseen hallintoon ja jotka erotetaan toisistaan hallinnollisin rajoin.</skos:scopeNote>
    <skos:prefLabel xml:lang="fr">Unités administratives</skos:prefLabel>
    <skos:scopeNote xml:lang="fr">Unités d'administration séparées par des limites administratives et délimitant les zones dans lesquelles les États membres détiennent et/ou exercent leurs compétences, aux fins de l'administration locale, régionale et nationale.</skos:scopeNote>
    <skos:prefLabel xml:lang="hu">Közigazgatási egységek</skos:prefLabel>
    <skos:scopeNote xml:lang="hu">Az olyan nemzeti területeket, amelyeken a tagállamok joghatósággal rendelkeznek és/vagy joghatóságot gyakorolnak, helyi, regionális és országos egységekre osztó, közigazgatási határvonalakkal elválasztott igazgatási egységek.</skos:scopeNote>
    <skos:prefLabel xml:lang="it">Unità amministrative</skos:prefLabel>
    <skos:scopeNote xml:lang="it">Unità amministrative di suddivisione delle zone su cui gli Stati membri hanno e/o esercitano la loro giurisdizione a livello locale, regionale e nazionale, delimitate da confini amministrativi.</skos:scopeNote>
    <skos:prefLabel xml:lang="lt">Administraciniai vienetai</skos:prefLabel>
    <skos:scopeNote xml:lang="lt">Administracinėmis ribomis atskirti vietos, regionų ir nacionalinės valdžios administraciniai vienetai, į kuriuos padalijamos teritorijos, kurios priklauso valstybės narės jurisdikcijai ir (arba) kuriose ji vykdo jurisdikciją.</skos:scopeNote>
    <skos:prefLabel xml:lang="lv">Administratīvas vienības</skos:prefLabel>
    <skos:scopeNote xml:lang="lv">Administratīvas vienības, kas sadala apgabalus, kuros dalībvalstīm ir jurisdikcija un/vai kurā tās to īsteno, pašvaldību, reģionu un valsts pārvaldes nolūkā, kas sadalītas ar administratīvo robežu palīdzību.</skos:scopeNote>
    <skos:prefLabel xml:lang="mt">Unitajiet amministrattivi</skos:prefLabel>
    <skos:scopeNote xml:lang="mt">Unitajiet ta' amministrazzjoni, li jaqsmu żoni fejn Stati Membri għandhom u/jew jeżerċitaw drittijiet ġurisdizzjonali, għal governanza reġjonali, lokali u nazzjonali, separati minn konfini amministrattivi.</skos:scopeNote>
    <skos:prefLabel xml:lang="nl">Administratieve eenheden</skos:prefLabel>
    <skos:scopeNote xml:lang="nl">Door administratieve grenzen gescheiden lokale, regionale en nationale bestuurlijke eenheden die deel uitmaken van gebieden waarover de lidstaten rechtsbevoegdheid hebben en/of uitoefenen.</skos:scopeNote>
    <skos:prefLabel xml:lang="pl">Jednostki administracyjne</skos:prefLabel>
    <skos:scopeNote xml:lang="pl">Jednostki administracyjne, dzielące obszary, na których państwa członkowskie mają lub wykonują uprawnienia jurysdykcyjne, dla celów sprawowania władzy na poziomie lokalnym, regionalnym i krajowym, oddzielone granicami administracyjnymi.</skos:scopeNote>
    <skos:prefLabel xml:lang="pt">Unidades administrativas</skos:prefLabel>
    <skos:scopeNote xml:lang="pt">Unidades administrativas, zonas de divisão sobre as quais os Estados-Membros possuam e/ou exerçam direitos jurisdicionais, para efeitos de governação local, regional e nacional, separadas por fronteiras administrativas.</skos:scopeNote>
    <skos:prefLabel xml:lang="ro">Unități administrative</skos:prefLabel>
    <skos:scopeNote xml:lang="ro">Unități de administrare, de delimitare a zonelor în care statele membre dețin și/sau își exercită competența, la nivel local, regional și național, separate prin limite administrative.</skos:scopeNote>
    <skos:prefLabel xml:lang="sk">Správne jednotky</skos:prefLabel>
    <skos:scopeNote xml:lang="sk">Správne jednotky rozdeľujúce oblasti, v ktorých členské štáty majú právomoc rozhodovať a/alebo vykonávajú túto právomoc na účely miestneho, regionálneho a celoštátneho riadenia, oddelené správnymi hranicami.</skos:scopeNote>
    <skos:prefLabel xml:lang="sl">Upravne enote</skos:prefLabel>
    <skos:scopeNote xml:lang="sl">Upravne enote za lokalno, regionalno in nacionalno upravo, ki razdeljujejo območja, na katerih države članice imajo in/ali izvajajo jurisdikcijo, ločene z upravnimi mejami.</skos:scopeNote>
    <skos:prefLabel xml:lang="sv">Administrativa enheter</skos:prefLabel>
    <skos:scopeNote xml:lang="sv">Administrativa enheters, som delar upp områden där medlemsstater har och/eller utövar jurisdiktion, på lokal, regional och nationell nivå, åtskilda av administrativa gränser.</skos:scopeNote>
    <skos:altLabel>au</skos:altLabel>
    <skos:inScheme rdf:resource="http://inspire.ec.europa.eu/theme" />
  </skos:Concept>
  <skos:Concept xmlns:skos="http://www.w3.org/2004/02/skos/core#" rdf:about="http://inspire.ec.europa.eu/theme/rs">
    <skos:prefLabel xml:lang="en">Coordinate reference systems</skos:prefLabel>
    <skos:scopeNote xml:lang="en">Systems for uniquely referencing spatial information in space as a set of coordinates (x, y, z) and/or latitude and longitude and height, based on a geodetic horizontal and vertical datum.</skos:scopeNote>
    <skos:prefLabel xml:lang="bg">Координатни справочни системи</skos:prefLabel>
    <skos:scopeNote xml:lang="bg">Системи за пространствена информация, предназначена изключително за справочни цели, представена в пространството с координати (x, y, z) и/или ширина, дължина и височина, на базата на геодезични хоризонтални и вертикални данни.</skos:scopeNote>
    <skos:prefLabel xml:lang="cs">Souřadnicové referenční systémy</skos:prefLabel>
    <skos:scopeNote xml:lang="cs">Systémy umožňující jednoznačné přiřazení polohy prostorovým informacím pomocí souboru souřadnic (x, y, z) nebo zeměpisné šířky, zeměpisné délky a výšky, vycházející z údajů polohových a výškových geodetických systémů.</skos:scopeNote>
    <skos:prefLabel xml:lang="hr">Referentni koordinatni sustavi</skos:prefLabel>
    <skos:scopeNote xml:lang="hr">Sustavi za jednoznačno lociranje prostornih informacija u prostoru u obliku koordinata (x,y,z), i/ili širine, dužine i visine, koji se temelje na horizontalnom i vertikalnom geodetskom datumu.</skos:scopeNote>
    <skos:prefLabel xml:lang="da">Koordinatsystemer</skos:prefLabel>
    <skos:scopeNote xml:lang="da">Systemer for entydig rumlig stedfæstelse af geografiske informationer ved hjælp af et sæt koordinater (x, y, z) og/eller længde, bredde og højde, baseret på et horisontalt og vertikalt geodætisk datum.</skos:scopeNote>
    <skos:prefLabel xml:lang="de">Koordinatenreferenzsysteme</skos:prefLabel>
    <skos:scopeNote xml:lang="de">Systeme zur eindeutigen räumlichen Referenzierung von Geodaten anhand eines Koordinatensatzes (x, y, z) und/oder Angaben zu Breite, Länge und Höhe auf der Grundlage eines geodätischen horizontalen und vertikalen Datums.</skos:scopeNote>
    <skos:prefLabel xml:lang="el">Συστήματα συντεταγμένων</skos:prefLabel>
    <skos:scopeNote xml:lang="el">Συστήματα για μονοσήμαντη αναφορά χωρικών πληροφοριών στον χώρο, ως σύνολο συντεταγμένων (x,y,z) ή/και γεωγραφικό πλάτος και μήκος και ύψος, με βάση γεωδαιτικό οριζόντιο και κατακόρυφο σύστημα αναφοράς (datum).</skos:scopeNote>
    <skos:prefLabel xml:lang="es">Sistemas de coordenadas de referencia</skos:prefLabel>
    <skos:scopeNote xml:lang="es">Sistemas para referenciar de forma unívoca la información espacial en el espacio como una serie de coordenadas (x, y, z) y/o latitud y longitud y altura, basándose en un punto de referencia geodésico horizontal y vertical.</skos:scopeNote>
    <skos:prefLabel xml:lang="et">Koordinaatsüsteemid</skos:prefLabel>
    <skos:scopeNote xml:lang="et">Süsteemid, milles ruumiandmete asukoht ruumis määratakse üheselt koordinaatide hulgaga (x, y, z) ja/või geodeetilisel referents- ja kõrgussüsteemil põhineva laiuse, pikkuse ja kõrgusega.</skos:scopeNote>
    <skos:prefLabel xml:lang="fi">Koordinaattijärjestelmät</skos:prefLabel>
    <skos:scopeNote xml:lang="fi">Järjestelmät, joissa paikkatietoihin liittyvä sijainti esitetään yksikäsitteisesti koordinaattien (x, y, z) ja/tai maantieteellisten pituus- ja leveysasteiden sekä korkeuden avulla ja jotka perustuvat horisontaalisiin ja vertikaalisiin geodeettisiin vertausjärjestelmiin.</skos:scopeNote>
    <skos:prefLabel xml:lang="fr">Référentiels de coordonnées</skos:prefLabel>
    <skos:scopeNote xml:lang="fr">Systèmes de référencement unique des informations géographiques dans l'espace sous forme d'une série de coordonnées (x, y, z) et/ou la latitude et la longitude et l'altitude, en se fondant sur un point géodésique horizontal et vertical.</skos:scopeNote>
    <skos:prefLabel xml:lang="hu">Koordinátarendszerek</skos:prefLabel>
    <skos:scopeNote xml:lang="hu">Olyan rendszerek, amelyek a térinformáció térbeli helyzetét koordinátákkal (x, y, z) és/vagy vízszintes és függőleges geodéziai adatokon alapuló földrajzi szélességgel, hosszúsággal és magassággal adják meg.</skos:scopeNote>
    <skos:prefLabel xml:lang="it">Sistemi di coordinate</skos:prefLabel>
    <skos:scopeNote xml:lang="it">Sistemi per referenziare in maniera univoca le informazioni territoriali nello spazio mediante un sistema di coordinate (x, y, z) e/o latitudine e longitudine e quota, sulla base di un dato geodetico orizzontale e verticale.</skos:scopeNote>
    <skos:prefLabel xml:lang="lt">Koordinačių atskaitos sistemos</skos:prefLabel>
    <skos:scopeNote xml:lang="lt">Vienareikšmio erdvinės informacijos nurodymo erdvėje naudojant koordinačių (x, y, z) derinį ir (arba) platumą, ilgumą bei aukštį sistemos, pagrįstos geodezinės horizontaliosios ir vertikaliosios atskaitos duomenimis.</skos:scopeNote>
    <skos:prefLabel xml:lang="lv">Koordinātu atskaites sistēmas</skos:prefLabel>
    <skos:scopeNote xml:lang="lv">Sistēmas viennozīmīgai telpiskās informācijas atskaišu norādīšanai telpā ar koordinātu kopu (x, y, z) un/vai platumu, garumu un augstumu, izmantojot ģeodēziskos horizontālos un vertikālos datus.</skos:scopeNote>
    <skos:prefLabel xml:lang="mt">Sistemi ta' referenza ta' koordinati</skos:prefLabel>
    <skos:scopeNote xml:lang="mt">Sistemi biex issir referenza unika ta' informazzjoni ġeografika fl-ispazju bħala sett ta' koordinati (x,y,z) u/jew latitudni u lonġitudni u altitudni, ibbażati fuq datum ġeodetiku orizzontali u vertikali.</skos:scopeNote>
    <skos:prefLabel xml:lang="nl">Systemen voor verwijzing door middel van coördinaten</skos:prefLabel>
    <skos:scopeNote xml:lang="nl">Systemen om aan ruimtelijke informatie een unieke reeks coördinaten (x, y,z) en/of breedte, lengte en hoogte toe te kennen, gebaseerd op een horizontaal en verticaal geodetische datum.</skos:scopeNote>
    <skos:prefLabel xml:lang="pl">Systemy odniesienia za pomocą współrzędnych</skos:prefLabel>
    <skos:scopeNote xml:lang="pl">Systemy dla jednoznacznego przestrzennego odnoszenia informacji przestrzennej za pomocą współrzędnych x, y,z lub za pomocą szerokości, długości lub wysokości na podstawie geodezyjnego poziomego i pionowego układu odniesienia.</skos:scopeNote>
    <skos:prefLabel xml:lang="pt">Sistemas de referencia</skos:prefLabel>
    <skos:scopeNote xml:lang="pt">Sistemas para referenciar de forma única a informação geográfica no espaço sob a forma de um conjunto de coordenadas (x, y, z) e/ou latitude e longitude e altitude, com base num datum geodésico horizontal e vertical.</skos:scopeNote>
    <skos:prefLabel xml:lang="ro">Sisteme de coordonate de referință</skos:prefLabel>
    <skos:scopeNote xml:lang="ro">Sisteme de referință unică în spațiu a informațiilor spațiale, alcătuite dintr-un set de coordonate (x, y, z) și/sau latitudine și longitudine și altitudine, bazate pe un datum orizontal și pe unul vertical.</skos:scopeNote>
    <skos:prefLabel xml:lang="sk">Súradnicové referenčné systémy</skos:prefLabel>
    <skos:scopeNote xml:lang="sk">Systémy pre jednotne referenčné priestorové informácie v priestore v podobe množiny súradníc (x, y, z) a/alebo zemepisnej šírky, dĺžky a výšky založených na geodetickom horizontálnom a vertikálnom východzom bode.</skos:scopeNote>
    <skos:prefLabel xml:lang="sl">Referenčni koordinatni sistemi</skos:prefLabel>
    <skos:scopeNote xml:lang="sl">Sistemi za izključno navajanje prostorskih informacij v prostoru v obliki niza koordinat (x, y, z) in/ali širine in dolžine ter višine, ki temeljijo na horizontalnem in vertikalnem geodetskem podatku.</skos:scopeNote>
    <skos:prefLabel xml:lang="sv">Referenskoordinatsystem</skos:prefLabel>
    <skos:scopeNote xml:lang="sv">System för att entydigt lägesbestämma rumslig information i rummet som en uppsättning koordinater (x, y, z) och/eller som latitud, longitud och höjd, på grundval av ett geodetiskt horisontellt och vertikalt datum.</skos:scopeNote>
    <skos:altLabel>rs</skos:altLabel>
    <skos:inScheme rdf:resource="http://inspire.ec.europa.eu/theme" />
  </skos:Concept>
  <skos:Concept xmlns:skos="http://www.w3.org/2004/02/skos/core#" rdf:about="http://inspire.ec.europa.eu/theme/gg">
    <skos:prefLabel xml:lang="en">Geographical grid systems</skos:prefLabel>
    <skos:scopeNote xml:lang="en">Harmonised multi-resolution grid with a common point of origin and standardised location and size of grid cells.</skos:scopeNote>
    <skos:prefLabel xml:lang="bg">Географски координатни системи</skos:prefLabel>
    <skos:scopeNote xml:lang="bg">Хармонизирана сложна координатна система с обща начална точка и стандартизирано разположение и размер на квадрантите на координатната система.</skos:scopeNote>
    <skos:prefLabel xml:lang="cs">Zeměpisné soustavy souřadnicových sítí</skos:prefLabel>
    <skos:scopeNote xml:lang="cs">Harmonizovaná souřadnicová síť s víceúrovňovým rozlišením, normalizovanou polohou a velikostí buněk souřadnicové sítě, a společným vztažným bodem.</skos:scopeNote>
    <skos:prefLabel xml:lang="hr">Sustavi geografske mreže</skos:prefLabel>
    <skos:scopeNote xml:lang="hr">Usklađena mreža višestruke razlučivosti sa zajedničkom početnom točkom i standardiziranim položajem i veličinom mrežnih polja.</skos:scopeNote>
    <skos:prefLabel xml:lang="da">Geografiske kvadratnetsystemer</skos:prefLabel>
    <skos:scopeNote xml:lang="da">Et harmoniseret kvadratnet med flere cellestørrelser samt fælles nulpunkt og standardiseret cellelokalisering og -størrelse.</skos:scopeNote>
    <skos:prefLabel xml:lang="de">Geografische Gittersysteme</skos:prefLabel>
    <skos:scopeNote xml:lang="de">Harmonisiertes Gittersystem mit Mehrfachauflösung, gemeinsamem Ursprungspunkt und standardisierter Lokalisierung und Größe der Gitterzellen.</skos:scopeNote>
    <skos:prefLabel xml:lang="el">Συστήματα γεωγραφικού καννάβου</skos:prefLabel>
    <skos:scopeNote xml:lang="el">Εναρμονισμένος κάνναβος πολλαπλής ανάλυσης με ενιαίο σημείο αφετηρίας και τυποποιημένη θέση και μέγεθος των φατνίων του καννάβου.</skos:scopeNote>
    <skos:prefLabel xml:lang="es">Sistema de cuadrículas geográficas</skos:prefLabel>
    <skos:scopeNote xml:lang="es">Cuadrículas armonizadas multirresolución con un punto de origen común y con ubicación y tamaños de cuadrícula normalizados.</skos:scopeNote>
    <skos:prefLabel xml:lang="et">Geograafilised ruutvõrgud</skos:prefLabel>
    <skos:scopeNote xml:lang="et">Ühtlustatud, ühise lähtepunktiga ning võrguruutude standardse paigutuse ja suurusega mitmetasandiline ruutvõrk.</skos:scopeNote>
    <skos:prefLabel xml:lang="fi">Paikannusruudustot</skos:prefLabel>
    <skos:scopeNote xml:lang="fi">Yhdenmukaistettu monitasoinen ruudukko, jossa on yhteinen lähtöpiste ja standardoitu yksittäisen ruudun sijainti ja koko.</skos:scopeNote>
    <skos:prefLabel xml:lang="fr">Systèmes de maillage géographique</skos:prefLabel>
    <skos:scopeNote xml:lang="fr">Grille multi-résolution harmonisée avec un point d'origine commun et une localisation ainsi qu'une taille des cellules harmonisées.</skos:scopeNote>
    <skos:prefLabel xml:lang="hu">Földrajzi rácsrendszerek</skos:prefLabel>
    <skos:scopeNote xml:lang="hu">Harmonizált több felbontású rács közös kiindulóponttal és egységesített rácscella-helymeghatározással és -mérettel.</skos:scopeNote>
    <skos:prefLabel xml:lang="it">Sistemi di griglie geografiche</skos:prefLabel>
    <skos:scopeNote xml:lang="it">Griglia multi-risoluzione armonizzata con un punto di origine comune e un posizionamento e una dimensione standard delle celle.</skos:scopeNote>
    <skos:prefLabel xml:lang="lt">Geografinio tinklelio sistemos</skos:prefLabel>
    <skos:scopeNote xml:lang="lt">Suderintas kintamos skiriamosios gebos tinklelis su bendru atskaitos tašku ir standartizuota tinklelio langelių lokacija bei dydžiu.</skos:scopeNote>
    <skos:prefLabel xml:lang="lv">Ģeogrāfisko koordinātu tīklu sistēmas</skos:prefLabel>
    <skos:scopeNote xml:lang="lv">Saskaņots daudzpakāpju izšķiršanas koordinātu tīkls ar kopēju sākumpunktu un standartizētu tīkla šūnu atrašanās vietu un izmēru.</skos:scopeNote>
    <skos:prefLabel xml:lang="mt">Sistemi ta' grilji ġeografiċi</skos:prefLabel>
    <skos:scopeNote xml:lang="mt">Grilja multi-risoluzzjoni armonizzata b'punt ta' oriġini komuni u pożizzjoni u daqs taċ-ċelluli tal-grilja standardizzati.</skos:scopeNote>
    <skos:prefLabel xml:lang="nl">Geografisch rastersysteem</skos:prefLabel>
    <skos:scopeNote xml:lang="nl">Geharmoniseerde multiresolutieraster met een gemeenschappelijk beginpunt en gestandaardiseerde plaats en grootte van de gridcellen.</skos:scopeNote>
    <skos:prefLabel xml:lang="pl">Systemy siatek geograficznych</skos:prefLabel>
    <skos:scopeNote xml:lang="pl">Zharmonizowana wielorozdzielcza siatka o wspólnym punkcie początkowym i znormalizowanym położeniu oraz wielkości pól siatki.</skos:scopeNote>
    <skos:prefLabel xml:lang="pt">Sistemas de quadrículas geográficas</skos:prefLabel>
    <skos:scopeNote xml:lang="pt">Quadrícula harmonizada multi-resolução com um ponto de origem comum e localização e dimensão normalizadas das células.</skos:scopeNote>
    <skos:prefLabel xml:lang="ro">Sisteme de caroiaj geografic</skos:prefLabel>
    <skos:scopeNote xml:lang="ro">Caroiaj multirezoluție armonizat, având un punct de origine comun, precum și localizare și mărime standardizate ale celulelor.</skos:scopeNote>
    <skos:prefLabel xml:lang="sk">Geografické systémy sietí</skos:prefLabel>
    <skos:scopeNote xml:lang="sk">Harmonizovaná sieť s viacúrovňovým rozlíšením so spoločným počiatočným bodom a štandardizovanou polohou a veľkosťou buniek siete.</skos:scopeNote>
    <skos:prefLabel xml:lang="sl">Geografska koordinatna mreža</skos:prefLabel>
    <skos:scopeNote xml:lang="sl">Usklajena večločljivostna mreža s skupno točko izvora in standardizirano lokacijo ter velikostjo mrežnih celic.</skos:scopeNote>
    <skos:prefLabel xml:lang="sv">Geografiska rutnätssystem</skos:prefLabel>
    <skos:scopeNote xml:lang="sv">Harmoniserade rutnät med flera upplösningar, gemensam utgångspunkt och standardiserad placering och storlek på rutorna.</skos:scopeNote>
    <skos:altLabel>gg</skos:altLabel>
    <skos:inScheme rdf:resource="http://inspire.ec.europa.eu/theme" />
  </skos:Concept>
  <skos:Concept xmlns:skos="http://www.w3.org/2004/02/skos/core#" rdf:about="http://inspire.ec.europa.eu/theme/cp">
    <skos:prefLabel xml:lang="en">Cadastral parcels</skos:prefLabel>
    <skos:scopeNote xml:lang="en">Areas defined by cadastral registers or equivalent.</skos:scopeNote>
    <skos:prefLabel xml:lang="bg">Кадастрални парцели</skos:prefLabel>
    <skos:scopeNote xml:lang="bg">Райони, посочени в кадастрални регистри или други равностойни документи.</skos:scopeNote>
    <skos:prefLabel xml:lang="cs">Katastrální parcely</skos:prefLabel>
    <skos:scopeNote xml:lang="cs">Území vymezená v katastru nemovitostí nebo v obdobném rejstříku.</skos:scopeNote>
    <skos:prefLabel xml:lang="hr">Katastarske čestice</skos:prefLabel>
    <skos:scopeNote xml:lang="hr">Područja koja određuju katastarski registri ili njihovi ekvivalenti.</skos:scopeNote>
    <skos:prefLabel xml:lang="da">Matrikulære parceller</skos:prefLabel>
    <skos:scopeNote xml:lang="da">Arealer, der er defineret i matrikelregistre eller lignende.</skos:scopeNote>
    <skos:prefLabel xml:lang="de">Flurstücke/Grundstücke (Katasterparzellen)</skos:prefLabel>
    <skos:scopeNote xml:lang="de">Gebiete, die anhand des Grundbuchs oder gleichwertiger Verzeichnisse bestimmt werden.</skos:scopeNote>
    <skos:prefLabel xml:lang="el">Γεωτεμάχια κτηματολογίου</skos:prefLabel>
    <skos:scopeNote xml:lang="el">Εκτάσεις που ορίζονται από κτηματολογικά μητρώα ή αντίστοιχες.</skos:scopeNote>
    <skos:prefLabel xml:lang="es">Parcelas catastrales</skos:prefLabel>
    <skos:scopeNote xml:lang="es">Áreas determinadas por registros catastrales o equivalentes.</skos:scopeNote>
    <skos:prefLabel xml:lang="et">Katastriüksused</skos:prefLabel>
    <skos:scopeNote xml:lang="et">Katastritunnuste või võrdväärsete tunnustega kindlaksmääratud alad.</skos:scopeNote>
    <skos:prefLabel xml:lang="fi">Kiinteistöt</skos:prefLabel>
    <skos:scopeNote xml:lang="fi">Alueet, jotka on määritelty kiinteistörekisterissä tai vastaavassa.</skos:scopeNote>
    <skos:prefLabel xml:lang="fr">Parcelles cadastrales</skos:prefLabel>
    <skos:scopeNote xml:lang="fr">Zones définies par les registres cadastraux ou équivalents.</skos:scopeNote>
    <skos:prefLabel xml:lang="hu">Kataszteri parcellák</skos:prefLabel>
    <skos:scopeNote xml:lang="hu">Kataszteri nyilvántartásokkal – vagy ezzel egyenértékű módon – meghatározott területek.</skos:scopeNote>
    <skos:prefLabel xml:lang="it">Parcelle catastali</skos:prefLabel>
    <skos:scopeNote xml:lang="it">Aree definite dai registri catastali o equivalenti.</skos:scopeNote>
    <skos:prefLabel xml:lang="lt">Kadastro sklypai</skos:prefLabel>
    <skos:scopeNote xml:lang="lt">Kadastrų registruose ar panašiai apibrėžti plotai.</skos:scopeNote>
    <skos:prefLabel xml:lang="lv">Kadastrāli zemes gabali</skos:prefLabel>
    <skos:scopeNote xml:lang="lv">Teritorijas, kas noteiktas kadastra reģistros vai līdzīgās sistēmās.</skos:scopeNote>
    <skos:prefLabel xml:lang="mt">Pakketti katastali</skos:prefLabel>
    <skos:scopeNote xml:lang="mt">Żoni ddefiniti b'reġistri katastali jew l-ekwivalenti.</skos:scopeNote>
    <skos:prefLabel xml:lang="nl">Kadastrale percelen</skos:prefLabel>
    <skos:scopeNote xml:lang="nl">Gebieden die worden bepaald door kadastrale registers of een equivalent daarvan.</skos:scopeNote>
    <skos:prefLabel xml:lang="pl">Działki katastralne</skos:prefLabel>
    <skos:scopeNote xml:lang="pl">Obszary określone na podstawie rejestrów katastralnych lub ich odpowiedników.</skos:scopeNote>
    <skos:prefLabel xml:lang="pt">Parcelas cadastrais</skos:prefLabel>
    <skos:scopeNote xml:lang="pt">Áreas definidas por registos cadastrais ou equivalentes.</skos:scopeNote>
    <skos:prefLabel xml:lang="ro">Parcele cadastrale</skos:prefLabel>
    <skos:scopeNote xml:lang="ro">Zone stabilite de registrele cadastrale sau echivalente.</skos:scopeNote>
    <skos:prefLabel xml:lang="sk">Katastrálne parcely</skos:prefLabel>
    <skos:scopeNote xml:lang="sk">Územia vymedzené katastrálnymi registrami alebo rovnocennými registrami.</skos:scopeNote>
    <skos:prefLabel xml:lang="sl">Katastrske parcele</skos:prefLabel>
    <skos:scopeNote xml:lang="sl">Področja, ki jih opredeljujejo zemljiški kataster ali enakovredni registri.</skos:scopeNote>
    <skos:prefLabel xml:lang="sv">Fastighetsområden</skos:prefLabel>
    <skos:scopeNote xml:lang="sv">Områden definierade av fastighetsregister eller motsvarande.</skos:scopeNote>
    <skos:altLabel>cp</skos:altLabel>
    <skos:inScheme rdf:resource="http://inspire.ec.europa.eu/theme" />
  </skos:Concept>
  <skos:Concept xmlns:skos="http://www.w3.org/2004/02/skos/core#" rdf:about="http://inspire.ec.europa.eu/theme/gn">
    <skos:prefLabel xml:lang="en">Geographical names</skos:prefLabel>
    <skos:scopeNote xml:lang="en">Names of areas, regions, localities, cities, suburbs, towns or settlements, or any geographical or topographical feature of public or historical interest.</skos:scopeNote>
    <skos:prefLabel xml:lang="bg">Географски наименования</skos:prefLabel>
    <skos:scopeNote xml:lang="bg">Наименования на области, региони, местности, големи градове, предградия, малки градове или населени места, или географска или топографска характеристика от обществен или исторически интерес.</skos:scopeNote>
    <skos:prefLabel xml:lang="cs">Zeměpisné názvy</skos:prefLabel>
    <skos:scopeNote xml:lang="cs">Jména oblastí, regionů, míst, velkoměst, předměstí, měst nebo sídel nebo jakýchkoli zeměpisných nebo topografických útvarů veřejného zájmu nebo historického významu.</skos:scopeNote>
    <skos:prefLabel xml:lang="hr">Geografska imena</skos:prefLabel>
    <skos:scopeNote xml:lang="hr">Imena područja, regija, mjesta, velikih gradova, predgrađa, gradova ili naselja, ili bilo koje geografskog ili topografskog obilježja od državnog ili povijesnog značenja.</skos:scopeNote>
    <skos:prefLabel xml:lang="da">Stednavne</skos:prefLabel>
    <skos:scopeNote xml:lang="da">Navne på områder, regioner, lokaliteter, byer, forstæder, bebyggelser og alle former for geografiske og topografiske objekter af offentlig eller historisk interesse.</skos:scopeNote>
    <skos:prefLabel xml:lang="de">Geografische Bezeichnungen</skos:prefLabel>
    <skos:scopeNote xml:lang="de">Namen von Gebieten, Regionen, Orten, Großstädten, Vororten, Städten oder Siedlungen sowie jedes geografische oder topografische Merkmal von öffentlichem oder historischem Interesse.</skos:scopeNote>
    <skos:prefLabel xml:lang="el">Τοπωνύμια</skos:prefLabel>
    <skos:scopeNote xml:lang="el">Τοπωνύμια εκτάσεων, περιοχών, τοποθεσιών, πόλεων, προαστίων, κωμοπόλεων ή οικισμών, ή οποιοδήποτε γεωγραφικό ή τοπογραφικό χαρακτηριστικό δημόσιου ή ιστορικού ενδιαφέροντος.</skos:scopeNote>
    <skos:prefLabel xml:lang="es">Nombres geográficos</skos:prefLabel>
    <skos:scopeNote xml:lang="es">Nombres de zonas, regiones, localidades, ciudades, periferias, poblaciones o asentamientos, o cualquier rasgo geográfico o topográfico de interés público o histórico.</skos:scopeNote>
    <skos:prefLabel xml:lang="et">Geograafilised nimed</skos:prefLabel>
    <skos:scopeNote xml:lang="et">Alade, piirkondade, kohtade, linnade, äärelinnade, alevite või asulate nimed või muud üldist või ajaloolist huvi pakkuvad mis tahes geograafilised või topograafilised tunnused.</skos:scopeNote>
    <skos:prefLabel xml:lang="fi">Paikannimet</skos:prefLabel>
    <skos:scopeNote xml:lang="fi">Maa-alueiden, alueiden, paikkakuntien, suurkaupunkien, esikaupunkien, kaupunkien tai taajamien nimet tai muut sellaisten maantieteellisten tai topografisten kohteiden nimet, joilla on yleistä tai historiallista merkitystä.</skos:scopeNote>
    <skos:prefLabel xml:lang="fr">Dénominations géographiques</skos:prefLabel>
    <skos:scopeNote xml:lang="fr">Noms de zones, de régions, de localités, de grandes villes, de banlieues, de villes moyennes ou d'implantations, ou tout autre élément géographique ou topographique d'intérêt public ou historique.</skos:scopeNote>
    <skos:prefLabel xml:lang="hu">Földrajzi nevek</skos:prefLabel>
    <skos:scopeNote xml:lang="hu">Területek, régiók, helységek, nagyvárosok, elővárosok, városok vagy települések, illetve bármely, a nyilvánosság érdeklődésére számot tartó vagy történeti jelentősségre szert tett földrajzi vagy topográfiai jellegzetesség.</skos:scopeNote>
    <skos:prefLabel xml:lang="it">Nomi geografici</skos:prefLabel>
    <skos:scopeNote xml:lang="it">Denominazione di aree, regioni, località, città, periferie, paesi o centri abitati, o qualsiasi elemento geografico o topografico di interesse pubblico o storico.</skos:scopeNote>
    <skos:prefLabel xml:lang="lt">Geografiniai pavadinimai</skos:prefLabel>
    <skos:scopeNote xml:lang="lt">Sričių, regionų, vietovių, miestų, priemiesčių, miestelių, gyvenviečių ar kitų viešąją ar istorinę reikšmę turinčių geografinių ar topografinių elementų pavadinimai.</skos:scopeNote>
    <skos:prefLabel xml:lang="lv">Toponīmi</skos:prefLabel>
    <skos:scopeNote xml:lang="lv">Rajonu, reģionu, apvidu, lielpilsētu, priekšpilsētu, pilsētu, apdzīvotu vietu vai jebkādu valsts mēroga vai vēsturiskas nozīmes ģeogrāfisku vai topogrāfisku objektu nosaukumi.</skos:scopeNote>
    <skos:prefLabel xml:lang="mt">Ismijiet ġeografiċi</skos:prefLabel>
    <skos:scopeNote xml:lang="mt">Ismijiet ta' żoni, reġjuni, lokalitajiet, bliet, subborgi, jew inħawi abitati oħra, jew kull karatteristika ġeografika jew topografika ta' interess pubbliku jew storiku.</skos:scopeNote>
    <skos:prefLabel xml:lang="nl">Geografische namen</skos:prefLabel>
    <skos:scopeNote xml:lang="nl">Namen van gebieden, regio's, plaatsen, steden, voorsteden, gemeenten, nederzettingen, of andere geografische of topografische kenmerken van openbaar of historisch belang.</skos:scopeNote>
    <skos:prefLabel xml:lang="pl">Nazwy geograficzne</skos:prefLabel>
    <skos:scopeNote xml:lang="pl">Nazwy obszarów, regionów, miejscowości, miast, przedmieść lub osiedli, albo każdy inny obiekt geograficzny lub topograficzny o znaczeniu publicznym lub historycznym.</skos:scopeNote>
    <skos:prefLabel xml:lang="pt">Toponímia</skos:prefLabel>
    <skos:scopeNote xml:lang="pt">Denominações das zonas, regiões, localidades, cidades, subúrbios, pequenas cidades ou povoações, ou de qualquer entidade geográfica ou topográfica de interesse público ou histórico.</skos:scopeNote>
    <skos:prefLabel xml:lang="ro">Denumiri geografice</skos:prefLabel>
    <skos:scopeNote xml:lang="ro">Nume de zone, regiuni, localități, orașe mari, suburbii, orașe mici sau așezări, sau orice alt element geografic ori topografic de interes public sau istoric.</skos:scopeNote>
    <skos:prefLabel xml:lang="sk">Zemepisné názvy</skos:prefLabel>
    <skos:scopeNote xml:lang="sk">Názvy oblastí, regiónov, lokalít, veľkomiest, predmestí, miest alebo osád alebo akéhokoľvek zemepisného či topografického prvku verejného alebo historického významu.</skos:scopeNote>
    <skos:prefLabel xml:lang="sl">Zemljepisna imena</skos:prefLabel>
    <skos:scopeNote xml:lang="sl">Imena območij, regij, krajev, velemest, predmestij, mest ali zaselkov ali kateri koli geografski ali topografski pojav javnega ali zgodovinskega pomena.</skos:scopeNote>
    <skos:prefLabel xml:lang="sv">Geografiska namn</skos:prefLabel>
    <skos:scopeNote xml:lang="sv">Namn på områden, regioner, platser, städer, förorter, tätorter och annan bebyggelse, samt andra geografiska och topografiska företeelser av allmänt eller historiskt intresse.</skos:scopeNote>
    <skos:altLabel>gn</skos:altLabel>
    <skos:inScheme rdf:resource="http://inspire.ec.europa.eu/theme" />
  </skos:Concept>
  <skos:Concept xmlns:skos="http://www.w3.org/2004/02/skos/core#" rdf:about="http://inspire.ec.europa.eu/theme/hy">
    <skos:prefLabel xml:lang="en">Hydrography</skos:prefLabel>
    <skos:scopeNote xml:lang="en">Hydrographic elements, including marine areas and all other water bodies and items related to them, including river basins and sub-basins. Where appropriate, according to the definitions set out in Directive 2000/60/EC of the European Parliament and of the Council of 23 October 2000 establishing a framework for Community action in the field of water policy (2) and in the form of networks.</skos:scopeNote>
    <skos:prefLabel xml:lang="bg">Хидрография</skos:prefLabel>
    <skos:scopeNote xml:lang="bg">Хидрографски елементи, включително морски райони и други водни маси и свързани с тях елементи, включително речни басейни и подбасейни. По целесъобразност съгласно определенията, посочени в Директива 2000/60/ЕО на Европейския парламент и на Съвета от 23 октомври 2000 г. за установяване на рамка за действията на Общността в областта на политиката за водите (2) и под формата на мрежи.</skos:scopeNote>
    <skos:prefLabel xml:lang="cs">Vodopis</skos:prefLabel>
    <skos:scopeNote xml:lang="cs">Přírodní prvky, včetně mořských oblastí a všech ostatních s nimi souvisejících vodních těles a prvků, včetně povodí a dílčích povodí. Případně v souladu s definicemi uvedenými ve směrnici Evropského parlamentu a Rady 2000/60/ES ze dne 23. října 2000, kterou se stanoví rámec pro činnost Společenství v oblasti vodní politiky (2), a v podobě sítí.</skos:scopeNote>
    <skos:prefLabel xml:lang="hr">Hidrografija</skos:prefLabel>
    <skos:scopeNote xml:lang="hr">Hidrografski elementi, uključujući morska područja i sva druga vodena tijela i s njima povezane jedinice, uključujući riječne bazene i pod-bazene. Prema potrebi, u skladu s odredbama koje su utvrđene u Direktivi 2000/60/EZ, Europskog parlamenta i Vijeća, od 23. listopada 2000. o uspostavljanju okvira za djelovanje Zajednice u području politike voda (2), i u obliku mreža.</skos:scopeNote>
    <skos:prefLabel xml:lang="da">Hydrograf</skos:prefLabel>
    <skos:scopeNote xml:lang="da">Hydrografiske elementer, herunder havområder og alle andre vandområder og dertil knyttede forekomster, herunder også vandløbsoplande og vandløbsdeloplande. I givet fald i henhold til definitionerne i Europa-Parlamentets og Rådets direktiv 2000/60/EF af 23. oktober 2000 om fastlæggelse af en ramme for Fællesskabets vandpolitiske foranstaltninger [2] og i form af net.</skos:scopeNote>
    <skos:prefLabel xml:lang="de">Gewässernetz</skos:prefLabel>
    <skos:scopeNote xml:lang="de">Elemente des Gewässernetzes, einschließlich Meeresgebieten und allen sonstigen Wasserkörpern und hiermit verbundenen Teilsystemen, darunter Einzugsgebiete und Teileinzugsgebiete. Gegebenenfalls gemäß den Definitionen der Richtlinie 2000/60/EG des Europäischen Parlaments und des Rates vom 23. Oktober 2000 zur Schaffung eines Ordnungsrahmens für Maßnahmen der Gemeinschaft im Bereich der Wasserpolitik [2] und in Form von Netzen.</skos:scopeNote>
    <skos:prefLabel xml:lang="el">Υδρογραφία</skos:prefLabel>
    <skos:scopeNote xml:lang="el">Υδρογραφικά στοιχεία, όπου περιλαμβάνονται οι θαλάσσιες περιοχές και όλα τα άλλα υδατικά συστήματα και σχετιζόμενα στοιχεία, μεταξύ των οποίων και οι λεκάνες και υπολεκάνες απορροής ποταμών. Κατά περίπτωση, σύμφωνα με τους ορισμούς της οδηγίας 2000/60/ΕΚ του Ευρωπαϊκού Κοινοβουλίου και του Συμβουλίου, της 23ης Οκτωβρίου 2000, για τη θέσπιση πλαισίου κοινοτικής δράσης στον τομέα της πολιτικής των υδάτων [2] και υπό μορφή δικτύων.</skos:scopeNote>
    <skos:prefLabel xml:lang="es">Hidrografía</skos:prefLabel>
    <skos:scopeNote xml:lang="es">Elementos hidrográficos, incluidas las zonas marinas y todas las otras masas de agua y elementos relacionados con ellas, así como las cuencas y subcuencas hidrográficas. Cuando proceda, según lo definido en la Directiva 2000/60/CE del Parlamento Europeo y del Consejo, de 23 de octubre de 2000, por la que se establece un marco comunitario de actuación en el ámbito de la política de aguas [2], y en forma de redes.</skos:scopeNote>
    <skos:prefLabel xml:lang="et">Hüdrograafia</skos:prefLabel>
    <skos:scopeNote xml:lang="et">Hüdrograafilised objektid, sealhulgas merealad ning kõik muud veekogud ja nendega seotud objektid, sealhulgas vesikonnad ja alamvesikonnad. Kui see on asjakohane, vastavalt Euroopa Parlamendi ja nõukogu 23. oktoobri 2000. aasta direktiivis 2000/60/EÜ, millega kehtestatakse ühenduse veepoliitika alane tegevusraamistik (2) määratletule ning võrkude kujul.</skos:scopeNote>
    <skos:prefLabel xml:lang="fi">Hydrografia</skos:prefLabel>
    <skos:scopeNote xml:lang="fi">Hydrografiset elementit, mukaan luettuina merialueet ja kaikki muut vesimuodostumat ja niihin liittyvät kohteet, mukaan lukien vesistöalueet ja vesistöalueen osat. Tarvittaessa yhteisön vesipolitiikan puitteista 23 päivänä lokakuuta 2000 annetussa Euroopan parlamentin ja neuvoston direktiivissä 2000/60/EY [2] olevien määritelmien mukaan ja verkostomuodossa.</skos:scopeNote>
    <skos:prefLabel xml:lang="fr">Hydrographie</skos:prefLabel>
    <skos:scopeNote xml:lang="fr">Éléments hydrographiques, y compris les zones maritimes ainsi que toutes les autres masses d'eau et les éléments qui y sont liés, y compris les bassins et sous-bassins hydrographiques. Conformes, le cas échéant, aux définitions établies par la directive 2000/60/CE du Parlement européen et du Conseil du 23 octobre 2000 établissant un cadre pour une politique communautaire dans le domaine de l'eau [2] et sous forme de réseaux.</skos:scopeNote>
    <skos:prefLabel xml:lang="hu">Vízrajz</skos:prefLabel>
    <skos:scopeNote xml:lang="hu">Vízrajzi elemek, beleértve a tengeri területeket, minden egyéb víztestet és azzal kapcsolatos elemet, többek között a vízgyűjtőket és részvízgyűjtőket. Adott esetben a vízpolitika terén a közösségi fellépés kereteinek meghatározásáról szóló, 2000. október 23-i 2000/60/EK európai parlamenti és tanácsi irányelv [2] fogalommeghatározásaival összhangban és hálózati formában.</skos:scopeNote>
    <skos:prefLabel xml:lang="it">Idrografia</skos:prefLabel>
    <skos:scopeNote xml:lang="it">Elementi idrografici, comprese le zone marine e tutti gli altri corpi ed elementi idrici ad esse correlati, tra cui i bacini e sub bacini idrografici. Eventualmente in conformità delle definizioni contenute nella direttiva 2000/60/CE del Parlamento europeo e del Consiglio, del 23 ottobre 2000, che istituisce un quadro per l'azione comunitaria in materia di acque [2], e sotto forma di reti.</skos:scopeNote>
    <skos:prefLabel xml:lang="lt">Hidrografija</skos:prefLabel>
    <skos:scopeNote xml:lang="lt">Hidrografiniai elementai, įskaitant jūros zonas ir visus kitus vandens telkinius bei su jais susijusius elementus, įskaitant upių baseinus ir pabaseinius. Kur tikslinga, pagal 2000 m. spalio 23 d. Europos Parlamento ir Tarybos direktyvą 2000/60/EB, nustatančią Bendrijos veiksmų vandens politikos srityje pagrindus [2], ir tinklų pavidalu.</skos:scopeNote>
    <skos:prefLabel xml:lang="lv">Hidrogrāfija</skos:prefLabel>
    <skos:scopeNote xml:lang="lv">Hidrogrāfijas elementi, tostarp jūras teritorijas un visas citas ūdenstilpnes un ar tiem saistītie elementi, tostarp upju baseini un apakšbaseini. Attiecīgā gadījumā atbilstīgi definīcijām, kas izklāstītas Eiropas Parlamenta un Padomes Direktīvā 2000/60/EK ( 2000. gada 23. oktobris), ar ko izveido sistēmu Kopienas rīcībai ūdens resursu politikas jomā [2], un tīklu veidā.</skos:scopeNote>
    <skos:prefLabel xml:lang="mt">Idrografija</skos:prefLabel>
    <skos:scopeNote xml:lang="mt">Elementi idrografiċi, inklużi żoni marittimi, u kull korp ieħor ta' l-ilma u oġġetti relatati magħhom, inklużi baċiri tax-xmajjar u sub-baċiri. Fejn xieraq, skond id-definizzjonijiet fid-Direttiva 2000/60/KE tal-Parlament Ewropew u tal-Kunsill tat- 23 ta' Ottubru 2000 li tistabbilixxi qafas għall-azzjoni Komunitarja fil-qasam tal-politika ta' l-ilma [2] u fil-forma ta' networks.</skos:scopeNote>
    <skos:prefLabel xml:lang="nl">Hydrografie</skos:prefLabel>
    <skos:scopeNote xml:lang="nl">Hydrografische elementen, waaronder mariene gebieden en alle andere waterlichamen en daarmee verband houdende elementen, met inbegrip van stroomgebieden en deelstroomgebieden, in voorkomend geval volgens de omschrijvingen vermeld in Richtlijn 2000/60/EG van het Europees Parlement en de Raad van 23 oktober 2000 tot vaststelling van een kader voor communautaire maatregelen betreffende het waterbeleid [2] en in de vorm van netwerken.</skos:scopeNote>
    <skos:prefLabel xml:lang="pl">Hydrografia</skos:prefLabel>
    <skos:scopeNote xml:lang="pl">Elementy hydrograficzne, w tym obszary morskie lub inne części wód oraz związane z nimi obiekty, łącznie z dorzeczami i zlewniami. W odpowiednich przypadkach zgodnie z definicjami zawartymi w dyrektywie 2000/60/WE Parlamentu Europejskiego i Rady z dnia 23 października 2000 r. ustanawiającej ramy wspólnotowego działania w dziedzinie polityki wodnej [2] oraz w formie sieci.</skos:scopeNote>
    <skos:prefLabel xml:lang="pt">Hidrografia</skos:prefLabel>
    <skos:scopeNote xml:lang="pt">Elementos hidrográficos, incluindo zonas marinhas e todas as outras massas de água e elementos com eles relacionados, incluindo bacias e sub-bacias hidrográficas. Quando adequado, de acordo com as definições da Directiva 2000/60/CE do Parlamento Europeu e do Conselho, de 23 de Outubro de 2000, que estabelece um quadro de acção comunitária no domínio da política da água [2], e sob a forma de redes.</skos:scopeNote>
    <skos:prefLabel xml:lang="ro">Hidrografie</skos:prefLabel>
    <skos:scopeNote xml:lang="ro">Elementele hidrografice, inclusiv zonele marine, precum și toate celelalte corpuri de apă și elementele legate de acestea, inclusiv bazinele și sub-bazinele hidrografice. După caz, în conformitate cu definițiile din Directiva 2000/60/CE a Parlamentului European și a Consiliului din 23 octombrie 2000 de stabilire a unui cadru de politică comunitară în domeniul apei (15) și sub formă de rețele.</skos:scopeNote>
    <skos:prefLabel xml:lang="sk">Hydrografia</skos:prefLabel>
    <skos:scopeNote xml:lang="sk">Hydrografické prvky vrátane morských oblastí a všetkých ostatných vodných útvarov a objektov vzťahujúcich sa k nim vrátane povodí riek a čiastkových povodí. Ak je to možné, v súlade s vymedzeniami pojmov ustanovenými v smernici Európskeho parlamentu a Rady 2000/60/ES z 23. októbra 2000, ktorou sa stanovuje rámec pôsobnosti pre opatrenia Spoločenstva v oblasti vodného hospodárstva [2], a v podobe sietí.</skos:scopeNote>
    <skos:prefLabel xml:lang="sl">Hidrografija</skos:prefLabel>
    <skos:scopeNote xml:lang="sl">Hidrografski elementi, ki vključujejo morska območja ter vsa druga vodna telesa in z njimi povezane dele, vključno s povodji in porečji. Po potrebi v skladu z opredelitvami v Direktivi 2000/60/ES Evropskega parlamenta in Sveta z dne 23. oktobra 2000 o določitvi okvira za ukrepe Skupnosti na področju vodne politike [2] in v obliki omrežij.</skos:scopeNote>
    <skos:prefLabel xml:lang="sv">Hydrografi</skos:prefLabel>
    <skos:scopeNote xml:lang="sv">Hydrografiska element, inbegripet havsområden och alla andra vattenförekomster och därtill hörande inslag, inbegripet avrinningsområden och delavrinningsområden. I förekommande fall i enlighet med definitionerna i Europaparlamentets och rådets direktiv 2000/60/EG av den 23 oktober 2000 om upprättande av en ram för gemenskapens åtgärder på vattenpolitikens område [2] och i form av nät.</skos:scopeNote>
    <skos:altLabel>hy</skos:altLabel>
    <skos:inScheme rdf:resource="http://inspire.ec.europa.eu/theme" />
  </skos:Concept>
  <skos:Concept xmlns:skos="http://www.w3.org/2004/02/skos/core#" rdf:about="http://inspire.ec.europa.eu/theme/ps">
    <skos:prefLabel xml:lang="en">Protected sites</skos:prefLabel>
    <skos:scopeNote xml:lang="en">Area designated or managed within a framework of international, Community and Member States' legislation to achieve specific conservation objectives.</skos:scopeNote>
    <skos:prefLabel xml:lang="bg">Защитени обекти</skos:prefLabel>
    <skos:scopeNote xml:lang="bg">Район, определен или управляван съгласно международно законодателство, законодателство на Общността или на държавите-членки за постигане на определени цели за опазване на такива обекти.</skos:scopeNote>
    <skos:prefLabel xml:lang="cs">Chráněná území</skos:prefLabel>
    <skos:scopeNote xml:lang="cs">Území určená nebo spravovaná v rámci mezinárodních právních předpisů a právních předpisů Společenství a členských států pro dosažení konkrétních cílů jejich ochrany.</skos:scopeNote>
    <skos:prefLabel xml:lang="hr">Zaštićene lokacije</skos:prefLabel>
    <skos:scopeNote xml:lang="hr">Područje koje je određeno ili kojim se upravlja u okviru međunarodnog prava, prava Zajednice i država članica, kako bi se postigli posebni ciljevi očuvanja.</skos:scopeNote>
    <skos:prefLabel xml:lang="da">Beskyttede lokaliteter</skos:prefLabel>
    <skos:scopeNote xml:lang="da">Områder, der er udpeget eller forvaltes inden for en ramme af international, fællesskabs- og medlemsstatslovgivning for at nå bestemte bevaringsmål.</skos:scopeNote>
    <skos:prefLabel xml:lang="de">Schutzgebiete</skos:prefLabel>
    <skos:scopeNote xml:lang="de">Gebiete, die im Rahmen des internationalen und des gemeinschaftlichen Rechts sowie des Rechts der Mitgliedstaaten ausgewiesen sind oder verwaltet werden, um spezifische Erhaltungsziele zu erreichen.</skos:scopeNote>
    <skos:prefLabel xml:lang="el">Προστατευόμενες τοποθεσίες</skos:prefLabel>
    <skos:scopeNote xml:lang="el">Εκτάσεις χαρακτηρισμένες ή υποκείμενες σε διαχείριση σε ένα πλαίσιο διεθνούς, κοινοτικού και εθνικού δικαίου για την επίτευξη συγκεκριμένων στόχων διατήρησης.</skos:scopeNote>
    <skos:prefLabel xml:lang="es">Lugares protegidos</skos:prefLabel>
    <skos:scopeNote xml:lang="es">Zonas designadas o gestionadas dentro de un marco legislativo internacional, comunitario o propio de los Estados miembros, para la consecución de unos objetivos de conservación específicos.</skos:scopeNote>
    <skos:prefLabel xml:lang="et">Kaitsealused kohad</skos:prefLabel>
    <skos:scopeNote xml:lang="et">Ala, mis on kindlaksmääratud või mida hallatakse rahvusvaheliste, ühenduse või liikmesriikide õigusaktide raames konkreetsete kaitse-eesmärkide saavutamiseks.</skos:scopeNote>
    <skos:prefLabel xml:lang="fi">Suojellut alueet</skos:prefLabel>
    <skos:scopeNote xml:lang="fi">Erityisten suojelutavoitteiden saavuttamiseksi kansainvälisen, yhteisön ja jäsenvaltioiden lainsäädännön puitteissa nimetty tai hoidettu alue.</skos:scopeNote>
    <skos:prefLabel xml:lang="fr">Sites protégés</skos:prefLabel>
    <skos:scopeNote xml:lang="fr">Zone désignée ou gérée dans un cadre législatif international, communautaire ou national en vue d'atteindre des objectifs spécifiques de conservation.</skos:scopeNote>
    <skos:prefLabel xml:lang="hu">Védett helyek</skos:prefLabel>
    <skos:scopeNote xml:lang="hu">Különleges természetvédelmi célok elérése érdekében – nemzetközi, közösségi és tagállami jogszabályok keretében – kijelölt vagy kezelt terület.</skos:scopeNote>
    <skos:prefLabel xml:lang="it">Siti protetti</skos:prefLabel>
    <skos:scopeNote xml:lang="it">Aree designate o gestite in un quadro legislativo internazionale, comunitario o degli Stati membri per conseguire obiettivi di conservazione specifici.</skos:scopeNote>
    <skos:prefLabel xml:lang="lt">Saugomos teritorijos</skos:prefLabel>
    <skos:scopeNote xml:lang="lt">Teritorija, nustatyta ar tvarkoma pagal tarptautinius, Bendrijos ir valstybių narių teisės aktus, siekiant konkrečių apsaugos tikslų.</skos:scopeNote>
    <skos:prefLabel xml:lang="lv">Aizsargājamas teritorijas</skos:prefLabel>
    <skos:scopeNote xml:lang="lv">Teritorijas, kas noteiktas vai pārvaldītas saistībā ar starptautiskiem, Kopienas un dalībvalstu tiesību aktiem, lai nodrošinātu īpašu dabas aizsardzības mērķu īstenošanu.</skos:scopeNote>
    <skos:prefLabel xml:lang="mt">Siti protetti</skos:prefLabel>
    <skos:scopeNote xml:lang="mt">Żona indikata jew amministrata f'qafas ta' leġiżlazzjoni internazzjonali, Komunitarja u ta' l-Istati Membri sabiex jintlaħqu objettivi speċifiċi ta' konservazzjoni.</skos:scopeNote>
    <skos:prefLabel xml:lang="nl">Beschermde gebieden</skos:prefLabel>
    <skos:scopeNote xml:lang="nl">Gebieden die worden aangeduid of beheerd in het kader van internationale en communautaire wetgeving of wetgeving van de lidstaten om specifieke doelstellingen op het vlak van milieubescherming te verwezenlijken.</skos:scopeNote>
    <skos:prefLabel xml:lang="pl">Obszary chronione</skos:prefLabel>
    <skos:scopeNote xml:lang="pl">Obszar wyznaczony lub zarządzany w ramach prawa międzynarodowego, wspólnotowego lub państw członkowskich, w celu osiągnięcia szczególnych celów ochrony.</skos:scopeNote>
    <skos:prefLabel xml:lang="pt">Sítios protegidos</skos:prefLabel>
    <skos:scopeNote xml:lang="pt">Zonas designadas ou geridas no âmbito de legislação internacional, comunitária ou dos Estados-Membros para a prossecução de objectivos específicos de conservação.</skos:scopeNote>
    <skos:prefLabel xml:lang="ro">Zone protejate</skos:prefLabel>
    <skos:scopeNote xml:lang="ro">Zone desemnate sau administrate într-un cadru legislativ internațional, comunitar sau intern, în vederea îndeplinirii unor obiective specifice de conservare.</skos:scopeNote>
    <skos:prefLabel xml:lang="sk">Chránené územia</skos:prefLabel>
    <skos:scopeNote xml:lang="sk">Oblasti vymedzené alebo spravované v rámci medzinárodných právnych predpisov, právnych predpisov Spoločenstva a právnych predpisov členských štátov na účely dosiahnutia osobitných ochranárskych cieľov.</skos:scopeNote>
    <skos:prefLabel xml:lang="sl">Zavarovana območja</skos:prefLabel>
    <skos:scopeNote xml:lang="sl">Področje, ki se določi ali upravlja v okviru mednarodnega prava in prava držav članic in Skupnosti z namenom, da se dosežejo posebni cilji ohranjanja.</skos:scopeNote>
    <skos:prefLabel xml:lang="sv">Skyddade områden</skos:prefLabel>
    <skos:scopeNote xml:lang="sv">Områden som är utsedda eller förvaltas inom ramen för internationell lagstiftning, gemenskapslagstiftning och medlemsstaternas lagstiftning för att uppnå specifika miljövårdsmål.</skos:scopeNote>
    <skos:altLabel>ps</skos:altLabel>
    <skos:inScheme rdf:resource="http://inspire.ec.europa.eu/theme" />
  </skos:Concept>
  <skos:Concept xmlns:skos="http://www.w3.org/2004/02/skos/core#" rdf:about="http://inspire.ec.europa.eu/theme/tn">
    <skos:prefLabel xml:lang="en">Transport networks</skos:prefLabel>
    <skos:scopeNote xml:lang="en">Road, rail, air and water transport networks and related infrastructure. Includes links between different networks. Also includes the trans-European transport network as defined in Decision No 1692/96/EC of the European Parliament and of the Council of 23 July 1996 on Community Guidelines for the development of the trans-European transport network (1) and future revisions of that Decision.</skos:scopeNote>
    <skos:prefLabel xml:lang="bg">Транспортни мрежи</skos:prefLabel>
    <skos:scopeNote xml:lang="bg">Автомобилни, железопътни, въздушни и водни транспортни мрежи и прилежаща инфраструктура. Включват връзки между различните мрежи. Включват също така и Трансевропейската транспортна мрежа, определена в Решение № 1692/96/ЕО на Европейския парламент и на Съвета от 23 юли 1996 г. относно общностните насоки за развитие на Трансевропейската транспортна мрежа (1) и бъдещо преразглеждане на това решение.</skos:scopeNote>
    <skos:prefLabel xml:lang="cs">Dopravní sítě</skos:prefLabel>
    <skos:scopeNote xml:lang="cs">Silniční, železniční, letecké a vodní dopravní sítě a související infrastruktura. Zahrnují spojnice mezi jednotlivými sítěmi. Zahrnují rovněž transevropskou dopravní síť, jak je vymezena v rozhodnutí Evropského parlamentu a Rady č. 1692/96/ES ze dne 23. července 1996 o hlavních směrech Společenství pro rozvoj transevropské dopravní sítě (1) a v budoucích změnách uvedeného rozhodnutí.</skos:scopeNote>
    <skos:prefLabel xml:lang="hr">Prometne mreže</skos:prefLabel>
    <skos:scopeNote xml:lang="hr">Mreže cestovnog, zračnog, željezničkog i vodnog prometa i pripadajuća infrastruktura. Uključuje veze između različitih mreža. Također uključuje transeuropsku prometnu mrežu kako je određena u Odluci br. 1692/96/EZ, Europskog parlamenta i Vijeća od 23. srpnja 1996. o smjernicama Zajednice za razvoj transeuropske prometne mreže (1) i u naknadnim revizijama te Odluke.</skos:scopeNote>
    <skos:prefLabel xml:lang="da">Transportnet</skos:prefLabel>
    <skos:scopeNote xml:lang="da">Transportnet for biler, tog, fly og skibe med tilhørende infrastruktur. Omfatter forbindelser mellem de forskellige net. Omfatter også det transeuropæiske transportnet som defineret i Europa-Parlamentets og Rådets beslutning nr. 1692/96/EF af 23. juli 1996 om Fællesskabets retningslinjer for udvikling af det transeuropæiske transportnet [1] og fremtidige ændringer af denne beslutning.</skos:scopeNote>
    <skos:prefLabel xml:lang="de">Verkehrsnetze</skos:prefLabel>
    <skos:scopeNote xml:lang="de">Verkehrsnetze und zugehörige Infrastruktureinrichtungen für Straßen-, Schienen- und Luftverkehr sowie Schifffahrt. Umfasst auch die Verbindungen zwischen den verschiedenen Netzen. Umfasst auch das transeuropäische Verkehrsnetz im Sinne der Entscheidung Nr. 1692/96/EG des Europäischen Parlaments und des Rates vom 23. Juli 1996 über gemeinschaftliche Leitlinien für den Aufbau eines transeuropäischen Verkehrsnetzes [1] und künftiger Überarbeitungen dieser Entscheidung.</skos:scopeNote>
    <skos:prefLabel xml:lang="el">Δίκτυα μεταφορών</skos:prefLabel>
    <skos:scopeNote xml:lang="el">Δίκτυα οδικών, σιδηροδρομικών, αεροπορικών και υδάτινων μεταφορών και οι αντίστοιχες υποδομές. Περιλαμβάνονται οι συνδέσεις μεταξύ των διαφόρων δικτύων. Περιλαμβάνεται επίσης το διευρωπαϊκό δίκτυο μεταφορών, όπως ορίζεται στην απόφαση αριθ. 1692/96/EΚ του Ευρωπαϊκού Κοινοβουλίου και του Συμβουλίου, της 23ης Ιουλίου 1996, περί των κοινοτικών προσανατολισμών για την ανάπτυξη του διευρωπαϊκού δικτύου μεταφορών [1] και στις μελλοντικές αναθεωρήσεις της εν λόγω απόφασης.</skos:scopeNote>
    <skos:prefLabel xml:lang="es">Redes de transporte</skos:prefLabel>
    <skos:scopeNote xml:lang="es">Redes de carreteras, ferrocarril, transporte aéreo y vías navegables, con sus correspondientes infraestructuras. Se incluirán las conexiones entre redes diferentes. Se incluirá también la red transeuropea de transporte, según la definición de la Decisión no 1692/96/CE del Parlamento Europeo y del Consejo, de 23 de julio de 1996, sobre las orientaciones comunitarias para el desarrollo de la red transeuropea de transporte [1], y de las futuras revisiones de dicha Decisión.</skos:scopeNote>
    <skos:prefLabel xml:lang="et">Transpordivõrgud</skos:prefLabel>
    <skos:scopeNote xml:lang="et">Maantee-, raudtee-, õhu- ja veetranspordivõrgud ja nendega seotud infrastruktuurid. Sisaldab eri võrkude vahelisi ühendusi. Hõlmab ka Euroopa Parlamendi ja nõukogu 23. juuli 1996. aasta otsuses 1692/96/EÜ üleeuroopalise transpordivõrgu arendamist käsitlevate ühenduse suuniste kohta, (1) määratletud üleeuroopalist transpordivõrku jaselle otsuse edaspidiseid muudatusi.</skos:scopeNote>
    <skos:prefLabel xml:lang="fi">Liikenneverkot</skos:prefLabel>
    <skos:scopeNote xml:lang="fi">Tie-, raide-, ilma- ja vesiliikenneverkot ja niihin liittyvä infrastruktuuri. Sisältää eri verkkojen väliset yhteydet. Sisältää myös Euroopan laajuisen liikenneverkon sellaisena kuin se on määritelty yhteisön suuntaviivoista Euroopan laajuisen liikenneverkon kehittämiseksi 23 päivänä heinäkuuta 1996 tehdyssä Euroopan parlamentin ja neuvoston päätöksessä N:o 1692/96/EY [1] ja tämän päätöksen tulevissa tarkistuksissa.</skos:scopeNote>
    <skos:prefLabel xml:lang="fr">Réseaux de transport</skos:prefLabel>
    <skos:scopeNote xml:lang="fr">Réseaux routier, ferroviaire, aérien et navigable ainsi que les infrastructures associées. Sont également incluses les correspondances entre les différents réseaux, ainsi que le réseau transeuropéen de transport tel que défini dans la décision no 1692/96/CE du Parlement européen et du Conseil du 23 juillet 1996 sur les orientations communautaires pour le développement du réseau transeuropéen de transport [1] et les révisions futures de cette décision.</skos:scopeNote>
    <skos:prefLabel xml:lang="hu">Közlekedési hálózatok</skos:prefLabel>
    <skos:scopeNote xml:lang="hu">Közúti, vasúti, légi és vízi közlekedési hálózatok és a kapcsolódó infrastruktúra. Ide tartoznak a különféle hálózatok közötti összeköttetések is. Magában foglalja továbbá a transzeurópai közlekedési hálózat fejlesztésére vonatkozó közösségi iránymutatásokról szóló, 1996. július 23-i 1692/96/EK európai parlamenti és tanácsi határozatban [1] meghatározott transzeurópai közlekedési hálózatot és e határozat jövőbeli felülvizsgálatait is.</skos:scopeNote>
    <skos:prefLabel xml:lang="it">Reti di trasporto</skos:prefLabel>
    <skos:scopeNote xml:lang="it">Reti di trasporto su strada, su rotaia, per via aerea e per vie navigabili e relative infrastrutture. Questa voce comprende i collegamenti tra le varie reti e anche la rete transeuropea di trasporto di cui alla decisione n. 1692/96/CE del Parlamento europeo e del Consiglio, del 23 luglio 1996, sugli orientamenti comunitari per lo sviluppo della rete transeuropee dei trasporti [1] e successive revisioni.</skos:scopeNote>
    <skos:prefLabel xml:lang="lt">Transporto tinklai</skos:prefLabel>
    <skos:scopeNote xml:lang="lt">Keliai, geležinkeliai, oro ir vandens transporto tinklai bei su jais susijusi infrastruktūra. Įtraukiamos sąsajos tarp skirtingų tinklų. Taip pat apima 1996 m. liepos 23 d. Europos Parlamente ir Tarybos sprendime Nr. 1692/96/EB, pateikiančiame Bendrijos gaires dėl transeuropinio transporto tinklo plėtros [1], ir jo vėlesniuose pakeitimuose apibrėžtą transeuropinį transporto tinklą.</skos:scopeNote>
    <skos:prefLabel xml:lang="lv">Transporta tīkli</skos:prefLabel>
    <skos:scopeNote xml:lang="lv">Autoceļi, dzelzceļa, gaisa un ūdens transporta tīkli un ar tiem saistītā infrastruktūra. Tie ietver arī dažādu tīklu savienojumus. Tie ietver arī Eiropas transporta tīklu, kā tas definēts Eiropas Parlamenta un Padomes Lēmumā Nr. 1692/96/EK ( 1996. gada 23. jūlijs) par Kopienas pamatnostādnēm Eiropas transporta tīkla attīstībai [1] un minētā lēmuma turpmākajos grozījumos.</skos:scopeNote>
    <skos:prefLabel xml:lang="mt">Networks tat-trasport</skos:prefLabel>
    <skos:scopeNote xml:lang="mt">Networks tat-trasport tat-triq, tal-ferrovija, ta' l-ajru u ta' l-ilma u infrastruttura relatata. Huma inklużi l-kollegamenti bejn networks differenti. Huma inklużi wkoll in-network trans-Ewropew tat-trasport kif definit fid-Deċiżjoni Nru 1692/96/KE tal-Parlament Ewropew u tal-Kunsill tat- 23 ta' Lulju 1996 dwar il-Linji Gwida tal-Komunità għall-iżvilupp ta' network trans-Ewropew tat-trasport [1] u r-reviżjonijiet futuri ta' dik id-Deċiżjoni.</skos:scopeNote>
    <skos:prefLabel xml:lang="nl">Vervoersnetwerken</skos:prefLabel>
    <skos:scopeNote xml:lang="nl">Netwerken voor vervoer over de weg, per spoor, in de lucht en over het water en de aanverwante infrastructuur met inbegrip van koppelingen tussen verschillende netwerken en het trans-Europees vervoersnetwerk, zoals gedefinieerd in Beschikking nr. 1692/96/EG van het Europees Parlement en de Raad van 23 juli 1996 betreffende communautaire richtsnoeren voor de ontwikkeling van een trans-Europees vervoersnet [1] en de latere herzieningen van deze beschikking.</skos:scopeNote>
    <skos:prefLabel xml:lang="pl">Sieci transportowe</skos:prefLabel>
    <skos:scopeNote xml:lang="pl">Sieci transportu drogowego, kolejowego, lotniczego i wodnego oraz związana z nimi infrastruktura. Obejmują połączenia pomiędzy różnymi sieciami. Zalicza się do nich także transeuropejską sieć transportową w rozumieniu decyzji nr 1692/96/WE Parlamentu Europejskiego i Rady z dnia 23 czerwca 1996 r. w sprawie wspólnotowych wytycznych dotyczących rozwoju transeuropejskiej sieci transportowej [1] wraz z jej przyszłymi zmianami.</skos:scopeNote>
    <skos:prefLabel xml:lang="pt">Redes de transporte</skos:prefLabel>
    <skos:scopeNote xml:lang="pt">Redes de transporte rodoviário, ferroviário, aéreo e por via navegável, e respectivas infra-estruturas. Inclui as ligações entre as diferentes redes. Inclui também a rede transeuropeia de transportes definida na Decisão n.o 1692/96/CE do Parlamento Europeu e do Conselho, de 23 de Julho de 1996, sobre as orientações comunitárias para o desenvolvimento da rede transeuropeia de transportes [1], e as futuras revisões dessa decisão.</skos:scopeNote>
    <skos:prefLabel xml:lang="ro">Rețele de transport</skos:prefLabel>
    <skos:scopeNote xml:lang="ro">Rețele de transport rutier, feroviar, aerian și pe apă și infrastructura asociată. Cuprinde, de asemenea, legături între diferite rețele. Mai cuprinde și rețeaua transeuropeană de transport, astfel cum este definită în Decizia nr. 1692/96/CE a Parlamentului European și a Consiliului din 23 iulie 1996 privind orientările comunitare pentru dezvoltarea rețelei transeuropene de transport (14) și modificările ulterioare.</skos:scopeNote>
    <skos:prefLabel xml:lang="sk">Dopravné siete</skos:prefLabel>
    <skos:scopeNote xml:lang="sk">Cestné, železničné, letecké a vodné dopravné siete a s nimi súvisiaca infraštruktúra. Patria sem prepojenia medzi jednotlivými sieťami. Zahŕňajú tiež transeurópsku dopravnú sieť vymedzenú v rozhodnutí Európskeho parlamentu a Rady č. 1692/96/ES z 23. júla 1996 o základných usmerneniach Spoločenstva pre rozvoj transeurópskej dopravnej siete [1] a budúcich revíziách uvedeného rozhodnutia.</skos:scopeNote>
    <skos:prefLabel xml:lang="sl">Prometna omrežja</skos:prefLabel>
    <skos:scopeNote xml:lang="sl">Cestna, železniška, zračna in vodna prometna omrežja ter z njimi povezana infrastruktura. Vključuje povezave med različnimi omrežji. Vključuje tudi vseevropsko prometno omrežje, kakor je določeno v Odločbi št. 1692/96/ES Evropskega parlamenta in Sveta z dne 23. julija 1996 o smernicah Skupnosti za razvoj vseevropskega prometnega omrežja [1], in prihodnje preglede te odločbe.</skos:scopeNote>
    <skos:prefLabel xml:lang="sv">Transportnät</skos:prefLabel>
    <skos:scopeNote xml:lang="sv">Väg-, järnvägs-, luft- och sjötransportnät och tillhörande infrastruktur. Innefattar länkar mellan olika nät. Innefattar också det transeuropeiska transportnät som definieras i Europaparlamentets och rådets beslut nr 1692/96/EG av den 23 juli 1996 om gemenskapens riktlinjer för utbyggnad av det transeuropeiska transportnätet [1] samt framtida ändringar av det beslutet.</skos:scopeNote>
    <skos:altLabel>tn</skos:altLabel>
    <skos:inScheme rdf:resource="http://inspire.ec.europa.eu/theme" />
  </skos:Concept>
  <skos:Concept xmlns:skos="http://www.w3.org/2004/02/skos/core#" rdf:about="http://inspire.ec.europa.eu/theme/el">
    <skos:prefLabel xml:lang="en">Elevation</skos:prefLabel>
    <skos:scopeNote xml:lang="en">Digital elevation models for land, ice and ocean surface. Includes terrestrial elevation, bathymetry and shoreline.</skos:scopeNote>
    <skos:prefLabel xml:lang="bg">Релеф</skos:prefLabel>
    <skos:scopeNote xml:lang="bg">Цифрови релефни модели за земната, ледената и океанската повърхност. Включва земен релеф, батиметрия и брегова линия.</skos:scopeNote>
    <skos:prefLabel xml:lang="cs">Nadmořská výška</skos:prefLabel>
    <skos:scopeNote xml:lang="cs">Digitální výškový model pevniny, povrchu ledovců a oceánů. Zahrnuje nadmořské výšky pevnin, vodní hloubky a pobřežní čáru.</skos:scopeNote>
    <skos:prefLabel xml:lang="hr">Visina</skos:prefLabel>
    <skos:scopeNote xml:lang="hr">Digitalni modeli visina za površinu kopna, leda i oceana. Uključuju nadmorske visine, dubine mora i obalne linije.</skos:scopeNote>
    <skos:prefLabel xml:lang="da">Højde</skos:prefLabel>
    <skos:scopeNote xml:lang="da">Digitale højdemodeller for land, is og havoverflade. Omfatter landhøjder, havdybder og kystlinje.</skos:scopeNote>
    <skos:prefLabel xml:lang="de">Höhe</skos:prefLabel>
    <skos:scopeNote xml:lang="de">Digitale Höhenmodelle für Land-, Eis- und Meeresflächen. Dazu gehören Geländemodell, Tiefenmessung und Küstenlinie.</skos:scopeNote>
    <skos:prefLabel xml:lang="el">Υψομετρία</skos:prefLabel>
    <skos:scopeNote xml:lang="el">Ψηφιακά υψομετρικά μοντέλα για χερσαίες εκτάσεις, εκτάσεις καλυπτόμενες από πάγους και ωκεανούς. Περιλαμβάνονται, εν προκειμένω, η χερσαία υψομετρία, η βαθυμετρία και οι ακτογραμμές.</skos:scopeNote>
    <skos:prefLabel xml:lang="es">Elevaciones</skos:prefLabel>
    <skos:scopeNote xml:lang="es">Modelos digitales de elevaciones para las superficies de tierra, hielo y mar. Se incluirán la altimetría, la batimetría y la línea de costa.</skos:scopeNote>
    <skos:prefLabel xml:lang="et">Kõrgused</skos:prefLabel>
    <skos:scopeNote xml:lang="et">Maa- ja jääpinna ning ookeani põhja digitaalsed reljeefimudelid. Hõlmab maapinna ja veekogude põhja reljeefi ning kaldajooni.</skos:scopeNote>
    <skos:prefLabel xml:lang="fi">Korkeus</skos:prefLabel>
    <skos:scopeNote xml:lang="fi">Digitaaliset maan-, jään- ja merenpintaa kuvaavat korkeusmallit. Sisältää maanpinnan korkeussuhteet, syvyystiedot ja rantaviivan.</skos:scopeNote>
    <skos:prefLabel xml:lang="fr">Altitude</skos:prefLabel>
    <skos:scopeNote xml:lang="fr">Modèles numériques pour l'altitude des surfaces terrestres, glaciaires et océaniques. Comprend l'altitude terrestre, la bathymétrie et la ligne de rivage.</skos:scopeNote>
    <skos:prefLabel xml:lang="hu">Domborzat</skos:prefLabel>
    <skos:scopeNote xml:lang="hu">Digitális domborzati modellek a szárazföldi, jéggel borított és óceáni felszínre. Ide tartozik a felszíni és víz alatti domborzat és a partvonal.</skos:scopeNote>
    <skos:prefLabel xml:lang="it">Elevazione</skos:prefLabel>
    <skos:scopeNote xml:lang="it">Modelli digitali di elevazione per superfici emerse, ghiacci e superfici oceaniche. La voce comprende l’altitudine terrestre, la batimetria e la linea di costa.</skos:scopeNote>
    <skos:prefLabel xml:lang="lt">Aukštis</skos:prefLabel>
    <skos:scopeNote xml:lang="lt">Sausumos, ledo ir vandenyno paviršių skaitmeniniai aukščio modeliai. Tai apima sausumos aukštį, batimetriją ir pakrantės liniją.</skos:scopeNote>
    <skos:prefLabel xml:lang="lv">Augstums</skos:prefLabel>
    <skos:scopeNote xml:lang="lv">Digitāli augstuma modeļi zemes, ledus un jūras virsmai. Tie ietver arī sauszemes reljefu, dziļumu un krasta līniju.</skos:scopeNote>
    <skos:prefLabel xml:lang="mt">Elevazzjoni</skos:prefLabel>
    <skos:scopeNote xml:lang="mt">Mudelli ta' elevazzjoni diġitali għall-art, is-silġ u l-wiċċ ta' l-oċean. Tinkludi l-elevazzjoni ta' l-art, il-batimetrija u l-linja tal-kosta.</skos:scopeNote>
    <skos:prefLabel xml:lang="nl">Hoogte</skos:prefLabel>
    <skos:scopeNote xml:lang="nl">Digitale hoogtemodellen voor land-, ijs- en oceaanoppervlakken, inclusief landhoogte, bathymetrie en kustlijn.</skos:scopeNote>
    <skos:prefLabel xml:lang="pl">Ukształtowanie terenu</skos:prefLabel>
    <skos:scopeNote xml:lang="pl">Cyfrowe modele wysokościowe powierzchni lądu, lodu i oceanu. Obejmuje również wysokość topograficzną terenu, batymetrię oraz linię brzegową.</skos:scopeNote>
    <skos:prefLabel xml:lang="pt">Altitude</skos:prefLabel>
    <skos:scopeNote xml:lang="pt">Modelos digitais de terreno aplicáveis às superfícies terrestre, gelada e oceânica. Inclui a elevação terrestre, a batimetria e a linha costeira.</skos:scopeNote>
    <skos:prefLabel xml:lang="ro">Elevație</skos:prefLabel>
    <skos:scopeNote xml:lang="ro">Modele digitale de elevații ale suprafețelor terestre, de gheață sau oceanice. Include altimetria, batimetria și linia de coastă.</skos:scopeNote>
    <skos:prefLabel xml:lang="sk">Výška</skos:prefLabel>
    <skos:scopeNote xml:lang="sk">Digitálne výškové modely zemského povrchu, ľadovcov a hladín oceánov. Patria sem pevninové vyvýšeniny, batymetria a pobrežná čiara.</skos:scopeNote>
    <skos:prefLabel xml:lang="sl">Digitalni model višin</skos:prefLabel>
    <skos:scopeNote xml:lang="sl">Digitalni model višin za kopensko, zaledenelo in oceansko površino. Vključuje nadmorske višine, batimetrijo in obalne mreže.</skos:scopeNote>
    <skos:prefLabel xml:lang="sv">Höjd</skos:prefLabel>
    <skos:scopeNote xml:lang="sv">Digitala höjdmodeller för mark-, is- och havsyta. Inbegriper höjdförhållanden på land, batymetri samt kustlinje.</skos:scopeNote>
    <skos:altLabel>el</skos:altLabel>
    <skos:inScheme rdf:resource="http://inspire.ec.europa.eu/theme" />
  </skos:Concept>
  <skos:Concept xmlns:skos="http://www.w3.org/2004/02/skos/core#" rdf:about="http://inspire.ec.europa.eu/theme/ge">
    <skos:prefLabel xml:lang="en">Geology</skos:prefLabel>
    <skos:scopeNote xml:lang="en">Geology characterised according to composition and structure. Includes bedrock, aquifers and geomorphology.</skos:scopeNote>
    <skos:prefLabel xml:lang="bg">Геология</skos:prefLabel>
    <skos:scopeNote xml:lang="bg">Геология, определена според състава и структурата. Включва земен слой, воден слой и геоморфология.</skos:scopeNote>
    <skos:prefLabel xml:lang="cs">Geologie</skos:prefLabel>
    <skos:scopeNote xml:lang="cs">Geologie charakterizovaná podle složení a struktury. Zahrnuje skalní podloží, zvodně a geomorfologii.</skos:scopeNote>
    <skos:prefLabel xml:lang="hr">Geologija</skos:prefLabel>
    <skos:scopeNote xml:lang="hr">Geologija je opisana u skladu sa sastavom i strukturom. Uključuje stjenovito tlo, podzemne vode i geomorfologiju.</skos:scopeNote>
    <skos:prefLabel xml:lang="da">Geologi</skos:prefLabel>
    <skos:scopeNote xml:lang="da">Geologi karakteriseret ved sammensætning og struktur. Omfatter grundfjeld, grundvandsmagasiner og geomorfologi.</skos:scopeNote>
    <skos:prefLabel xml:lang="de">Geologie</skos:prefLabel>
    <skos:scopeNote xml:lang="de">Geologische Beschreibung anhand von Zusammensetzung und Struktur. Dies umfasst auch Grundgestein, Grundwasserleiter und Geomorphologie.</skos:scopeNote>
    <skos:prefLabel xml:lang="el">Γεωλογία</skos:prefLabel>
    <skos:scopeNote xml:lang="el">Γεωλογικός χαρακτηρισμός με βάση τη σύσταση και τη δομή. Περιλαμβάνονται το μητρικό πέτρωμα, οι υδροφόροι ορίζοντες και η γεωμορφολογία.</skos:scopeNote>
    <skos:prefLabel xml:lang="es">Geología</skos:prefLabel>
    <skos:scopeNote xml:lang="es">Características geológicas según la composición y la estructura. Se incluirán la plataforma de roca firme, los acuíferos y la geomorfología.</skos:scopeNote>
    <skos:prefLabel xml:lang="et">Geoloogia</skos:prefLabel>
    <skos:scopeNote xml:lang="et">Maapinna geoloogiline iseloom vastavalt koostisele ja struktuurile. Hõlmab aluskivimeid, põhjaveekihte ja geomorfoloogiat.</skos:scopeNote>
    <skos:prefLabel xml:lang="fi">Geologia</skos:prefLabel>
    <skos:scopeNote xml:lang="fi">Geologia kuvattuna koostumuksen ja rakenteen mukaan. Sisältää kallioperän, akviferit ja pinnanmuodot.</skos:scopeNote>
    <skos:prefLabel xml:lang="fr">Géologie</skos:prefLabel>
    <skos:scopeNote xml:lang="fr">Géologie caractérisée en fonction de la composition et de la structure. Englobe le substratum rocheux, les aquifères et la géomorphologie.</skos:scopeNote>
    <skos:prefLabel xml:lang="hu">Földtan</skos:prefLabel>
    <skos:scopeNote xml:lang="hu">Az összetétel és szerkezet alapján jellemzett földtan. Ide tartozik az alapkőzet, a víztartó rétegek és a geomorfológia is.</skos:scopeNote>
    <skos:prefLabel xml:lang="it">Geologia</skos:prefLabel>
    <skos:scopeNote xml:lang="it">Classificazione geologica in base alla composizione e alla struttura. Questa voce comprende il basamento roccioso, gli acquiferi e la geomorfologia.</skos:scopeNote>
    <skos:prefLabel xml:lang="lt">Geologija</skos:prefLabel>
    <skos:scopeNote xml:lang="lt">Geologija apibūdinama pagal sudėtį ir struktūrą. Tai apima pamatinę uolieną, vandeninguosius sluoksnius ir geomorfologiją.</skos:scopeNote>
    <skos:prefLabel xml:lang="lv">Ģeoloģija</skos:prefLabel>
    <skos:scopeNote xml:lang="lv">Ģeoloģiskais stāvoklis, ko raksturo uzbūve un struktūra. Tostarp informācija par pamatiežiem, ūdens nesējslāņiem un ģeomorfoloģiju.</skos:scopeNote>
    <skos:prefLabel xml:lang="mt">Ġeologija</skos:prefLabel>
    <skos:scopeNote xml:lang="mt">Ġeoloġija kkaratterizzata skond il-kompożizzjoni u l-istruttura. Tinkludi s-sodda tal-blat, l-akwiferi u l-ġeomorfoloġija.</skos:scopeNote>
    <skos:prefLabel xml:lang="nl">Geologie</skos:prefLabel>
    <skos:scopeNote xml:lang="nl">Geologie, gekenmerkt volgens samenstelling en structuur, inclusief vast gesteente, waterhoudende grondlagen en geomorfologie.</skos:scopeNote>
    <skos:prefLabel xml:lang="pl">Geologia</skos:prefLabel>
    <skos:scopeNote xml:lang="pl">Geologia charakteryzowana na podstawie składu i struktury. Obejmuje podłoże skalne, warstwy wodonośne i geomorfologię.</skos:scopeNote>
    <skos:prefLabel xml:lang="pt">Geologia</skos:prefLabel>
    <skos:scopeNote xml:lang="pt">Geologia caracterizada de acordo com a composição e a estrutura. Inclui a base rochosa, os aquíferos e a geomorfologia.</skos:scopeNote>
    <skos:prefLabel xml:lang="ro">Geologie</skos:prefLabel>
    <skos:scopeNote xml:lang="ro">Geologie caracterizată în funcție de compoziție și structură. Include roca de bază, straturile acvifere și geomorfologia.</skos:scopeNote>
    <skos:prefLabel xml:lang="sk">Geológia</skos:prefLabel>
    <skos:scopeNote xml:lang="sk">Geológia charakterizovaná na základe zloženia a štruktúry. Zahŕňa skalné podložie, zvodnené vrstvy a geomorfológiu.</skos:scopeNote>
    <skos:prefLabel xml:lang="sl">Geologija</skos:prefLabel>
    <skos:scopeNote xml:lang="sl">Geologija je določena v skladu s sestavo in strukturo. Vključuje živo skalo, vodonosnike in geomorfologijo.</skos:scopeNote>
    <skos:prefLabel xml:lang="sv">Geologi</skos:prefLabel>
    <skos:scopeNote xml:lang="sv">Geologiska förhållanden indelade efter sammansättning och struktur. Innefattar berggrund, akviferer och geomorfologi.</skos:scopeNote>
    <skos:altLabel>ge</skos:altLabel>
    <skos:inScheme rdf:resource="http://inspire.ec.europa.eu/theme" />
  </skos:Concept>
  <skos:Concept xmlns:skos="http://www.w3.org/2004/02/skos/core#" rdf:about="http://inspire.ec.europa.eu/theme/lc">
    <skos:prefLabel xml:lang="en">Land cover</skos:prefLabel>
    <skos:scopeNote xml:lang="en">Physical and biological cover of the earth's surface including artificial surfaces, agricultural areas, forests, (semi-)natural areas, wetlands, water bodies.</skos:scopeNote>
    <skos:prefLabel xml:lang="bg">Земна покривка</skos:prefLabel>
    <skos:scopeNote xml:lang="bg">Физическа или биологична покривка на земната повърхност, включително изкуствени повърхности, селскостопански райони, гори, (полу-) естествени райони, влажни зони, водни маси.</skos:scopeNote>
    <skos:prefLabel xml:lang="cs">Krajinný pokryv</skos:prefLabel>
    <skos:scopeNote xml:lang="cs">Fyzický a biologický pokryv zemského povrchu, včetně uměle vytvořených ploch, zemědělských oblastí, lesů, přirozených a částečně přirozených oblastí, mokřadů, vodních těles.</skos:scopeNote>
    <skos:prefLabel xml:lang="hr">Prekrivenost tla</skos:prefLabel>
    <skos:scopeNote xml:lang="hr">Fizički ili biološki pokrov Zemljine površine, uključujući umjetne površine, poljoprivredna područja, šume, (polu-) prirodna područja, močvare, vodena tijela.</skos:scopeNote>
    <skos:prefLabel xml:lang="da">Arealdække</skos:prefLabel>
    <skos:scopeNote xml:lang="da">Jordens fysiske og biologiske overflade, herunder kunstige overflader, landbrugsarealer, skove, (halv-)naturlige områder, vådområder, vandområder.</skos:scopeNote>
    <skos:prefLabel xml:lang="de">Bodenbedeckung</skos:prefLabel>
    <skos:scopeNote xml:lang="de">Physische und biologische Bedeckung der Erdoberfläche, einschließlich künstlicher Flächen, landwirtschaftlicher Flächen, Wäldern, natürlicher (naturnaher) Gebiete, Feuchtgebieten und Wasserkörpern.</skos:scopeNote>
    <skos:prefLabel xml:lang="el">Κάλυψη γης</skos:prefLabel>
    <skos:scopeNote xml:lang="el">Φυσική και βιολογική κάλυψη της γήινης επιφάνειας, όπου συμπεριλαμβάνονται τεχνητές εκτάσεις, γεωργικές εκτάσεις, δάση, (ημι-)φυσικές εκτάσεις, υγρότοποι, υδατικά συστήματα.</skos:scopeNote>
    <skos:prefLabel xml:lang="es">Cubierta terrestre</skos:prefLabel>
    <skos:scopeNote xml:lang="es">Cubierta física y biológica de la superficie de la tierra, incluidas las superficies artificiales, las zonas agrarias, los bosques, las zonas naturales o seminaturales, los humedales, las láminas de agua.</skos:scopeNote>
    <skos:prefLabel xml:lang="et">Maakate</skos:prefLabel>
    <skos:scopeNote xml:lang="et">Maapinna elutust või elusainest kate, sealhulgas tehislikud pinnakatted, põllumajandusalad, metsad, (pool-)looduslikud alad, märgalad ning veekogud.</skos:scopeNote>
    <skos:prefLabel xml:lang="fi">Maanpeite</skos:prefLabel>
    <skos:scopeNote xml:lang="fi">Maapallon pinnan fysikaalinen ja biologinen peite, mukaan luettuina keinotekoiset peitteet, maatalousalueet, metsät, (osaksi) luonnontilassa olevat alueet, kosteikot ja vesistöt.</skos:scopeNote>
    <skos:prefLabel xml:lang="fr">Occupation des terres</skos:prefLabel>
    <skos:scopeNote xml:lang="fr">Couverture physique et biologique de la surface terrestre, y compris les surfaces artificielles, les zones agricoles, les forêts, les zones (semi-)naturelles, les zones humides et les masses d'eau.</skos:scopeNote>
    <skos:prefLabel xml:lang="hu">A felszín borítása</skos:prefLabel>
    <skos:scopeNote xml:lang="hu">A Föld felszínének fizikai és biológiai borítása, beleértve a mesterséges felszínt, a mezőgazdasági területeket, erdőket, a (félig) természetes területeket, a vizes élőhelyeket és a víztesteket.</skos:scopeNote>
    <skos:prefLabel xml:lang="it">Copertura del suolo</skos:prefLabel>
    <skos:scopeNote xml:lang="it">Copertura fisica e biologica della superficie terrestre comprese le superfici artificiali, le zone agricole, i boschi e le foreste, le aree (semi)naturali, le zone umide, i corpi idrici.</skos:scopeNote>
    <skos:prefLabel xml:lang="lt">Žemės danga</skos:prefLabel>
    <skos:scopeNote xml:lang="lt">Fizinė ir biologinė žemės paviršiaus danga, įskaitant dirbtinius paviršius, žemės ūkio plotus, miškus, (pusiau) natūralius plotus, šlapžemes, vandens telkinius.</skos:scopeNote>
    <skos:prefLabel xml:lang="lv">Zemes virsma</skos:prefLabel>
    <skos:scopeNote xml:lang="lv">Zemes virsmas fiziskais un bioloģiskais segums, tostarp mākslīgu virsmu, lauksaimniecības teritoriju, mežu, (daļēji) dabisku platību, mitrzemju, ūdenstilpņu fiziskais un bioloģiskais segums.</skos:scopeNote>
    <skos:prefLabel xml:lang="mt">Kopertura ta' l-art</skos:prefLabel>
    <skos:scopeNote xml:lang="mt">Kopertura fiżika u bijoloġika tal-wiċċ tad-dinja inklużi superfiċji artifiċjali, żoni agrikoli, foresti, żoni (semi-)naturali, artijiet mistagħdra, u korpi ta' ilma.</skos:scopeNote>
    <skos:prefLabel xml:lang="nl">Bodemgebruik</skos:prefLabel>
    <skos:scopeNote xml:lang="nl">Fysieke en biologische bedekking van het aardoppervlak, met inbegrip van kunstmatige oppervlakken, landbouwgebieden, bossen, halfnatuurlijke gebieden, moeraslanden en wateroppervlakken.</skos:scopeNote>
    <skos:prefLabel xml:lang="pl">Użytkowanie terenu</skos:prefLabel>
    <skos:scopeNote xml:lang="pl">Fizyczne i biologiczne użytkowanie powierzchni Ziemi, włączając w to powierzchnie sztuczne, obszary rolnicze, lasy, obszary (pół-)naturalne, tereny podmokłe, akweny.</skos:scopeNote>
    <skos:prefLabel xml:lang="pt">Ocupação do solo</skos:prefLabel>
    <skos:scopeNote xml:lang="pt">Cobertura física e biológica da superfície terrestre, incluindo superfícies artificiais, zonas agrícolas, florestas, zonas naturais ou semi-naturais, zonas húmidas, massas de água.</skos:scopeNote>
    <skos:prefLabel xml:lang="ro">Acoperire terestră</skos:prefLabel>
    <skos:scopeNote xml:lang="ro">Acoperirea fizică și biologică a suprafeței terestre, inclusiv suprafețele artificiale, zonele agricole, pădurile, zonele (semi)naturale, zonele umede și corpurile de apă.</skos:scopeNote>
    <skos:prefLabel xml:lang="sk">Krajinná pokrývka (land cover)</skos:prefLabel>
    <skos:scopeNote xml:lang="sk">Fyzikálna a biologická pokrývka zemského povrchu vrátane umelých povrchov, poľnohospodárskych oblastí, lesov, (polo)prírodných oblastí, mokradí, vodných útvarov.</skos:scopeNote>
    <skos:prefLabel xml:lang="sl">Pokrovnost tal</skos:prefLabel>
    <skos:scopeNote xml:lang="sl">Fizični in biološki pojavi na zemeljski površini, vključno z umetnimi površinami, kmetijskimi območji, gozdovi, (pol-)naravnimi območji, mokrišči, vodnimi telesi.</skos:scopeNote>
    <skos:prefLabel xml:lang="sv">Landtäcke</skos:prefLabel>
    <skos:scopeNote xml:lang="sv">Fysiskt och biologiskt landtäcke på jordytan, inbegripet artificiella ytor, jordbruksmark, skogar, (delvis) naturliga områden, våtmarker, vattenförekomster.</skos:scopeNote>
    <skos:altLabel>lc</skos:altLabel>
    <skos:inScheme rdf:resource="http://inspire.ec.europa.eu/theme" />
  </skos:Concept>
  <skos:Concept xmlns:skos="http://www.w3.org/2004/02/skos/core#" rdf:about="http://inspire.ec.europa.eu/theme/oi">
    <skos:prefLabel xml:lang="en">Orthoimagery</skos:prefLabel>
    <skos:scopeNote xml:lang="en">Geo-referenced image data of the Earth's surface, from either satellite or airborne sensors.</skos:scopeNote>
    <skos:prefLabel xml:lang="bg">Ортоизображение</skos:prefLabel>
    <skos:scopeNote xml:lang="bg">Данни от геоизображение на земната повърхност, направено от сателит или въздушни сензори.</skos:scopeNote>
    <skos:prefLabel xml:lang="cs">Ortofotosnímky</skos:prefLabel>
    <skos:scopeNote xml:lang="cs">Obrazová data pořízená satelitními nebo leteckými čidly vztažená k zemskému povrchu pomocí zeměpisné soustavy souřadnic.</skos:scopeNote>
    <skos:prefLabel xml:lang="hr">Ortofotografija</skos:prefLabel>
    <skos:scopeNote xml:lang="hr">Georeferencirani slikovni podaci Zemljine površine, ili sa satelita, ili iz zračnih senzora.</skos:scopeNote>
    <skos:prefLabel xml:lang="da">Ortofoto</skos:prefLabel>
    <skos:scopeNote xml:lang="da">Georefererede billeddata om Jordens overflade optaget fra enten satellit- eller flybaserede sensorer.</skos:scopeNote>
    <skos:prefLabel xml:lang="de">Orthofotografie</skos:prefLabel>
    <skos:scopeNote xml:lang="de">Georeferenzierte Bilddaten der Erdoberfläche von satelliten- oder luftfahrzeuggestützten Sensoren.</skos:scopeNote>
    <skos:prefLabel xml:lang="el">Ορθοφωτογραφία</skos:prefLabel>
    <skos:scopeNote xml:lang="el">Γεωαναφερόμενα δεδομένα από εικόνες της επιφάνειας της γης, από δορυφόρους ή αερομεταφερόμενους αισθητήρες.</skos:scopeNote>
    <skos:prefLabel xml:lang="es">Ortoimágenes</skos:prefLabel>
    <skos:scopeNote xml:lang="es">Imágenes georreferenciadas de la superficie de la tierra, obtenidas por satélite o por sensores aerotransportados.</skos:scopeNote>
    <skos:prefLabel xml:lang="et">Ortokujutised</skos:prefLabel>
    <skos:scopeNote xml:lang="et">Maapinna georefereeritud kujutised, mis on talletatud satelliitidel või lennuvahenditel asuvate sensorite abil.</skos:scopeNote>
    <skos:prefLabel xml:lang="fi">Ortoilmakuvat</skos:prefLabel>
    <skos:scopeNote xml:lang="fi">Joko satelliittien tai lentokäyttöisten sensorien toimittamia maantieteelliseen koordinaatistoon sidottuja kuvatietoja maapallon pinnasta.</skos:scopeNote>
    <skos:prefLabel xml:lang="fr">Ortho-imagerie</skos:prefLabel>
    <skos:scopeNote xml:lang="fr">Images géoréférencées de la surface terrestre, provenant de satellites ou de capteurs aéroportés.</skos:scopeNote>
    <skos:prefLabel xml:lang="hu">Ortofotók</skos:prefLabel>
    <skos:scopeNote xml:lang="hu">A Föld felszínének földrajzi hivatkozással ellátott, műhold vagy légi adatgyűjtők által készített képi adatai.</skos:scopeNote>
    <skos:prefLabel xml:lang="it">Orto immagini</skos:prefLabel>
    <skos:scopeNote xml:lang="it">Immagini georeferenziate della superficie terrestre prese da satellite o da telesensori.</skos:scopeNote>
    <skos:prefLabel xml:lang="lt">Ortofotografinis vaizdavimas</skos:prefLabel>
    <skos:scopeNote xml:lang="lt">Georeferencinis žemės paviršiaus atvaizdas, gaunamas iš palydove arba orlaivyje esančių jutiklių.</skos:scopeNote>
    <skos:prefLabel xml:lang="lv">Ortofotogrāfija</skos:prefLabel>
    <skos:scopeNote xml:lang="lv">Zemes virsmas attēli ar piekārtotu norādi par ģeogrāfisko novietojumu telpā, kas saņemti no satelīta vai gaisā esošiem sensoriem.</skos:scopeNote>
    <skos:prefLabel xml:lang="mt">Orthoimagery</skos:prefLabel>
    <skos:scopeNote xml:lang="mt">Data fil-forma ta' stampa ġeo-referenzjata tal-wiċċ tad-dinja, minn satellita jew minn sensuri fl-ajru.</skos:scopeNote>
    <skos:prefLabel xml:lang="nl">Orthobeeldvorming</skos:prefLabel>
    <skos:scopeNote xml:lang="nl">Geogerefereerde beeldgegevens van het aardoppervlak, afkomstig van sensoren op satellieten of vliegtuigen.</skos:scopeNote>
    <skos:prefLabel xml:lang="pl">Sporządzanie ortoobrazów</skos:prefLabel>
    <skos:scopeNote xml:lang="pl">Dane obrazowe powierzchni Ziemi posiadające odniesienie geograficzne, pochodzące z rejestracji z pokładu satelity lub samolotu.</skos:scopeNote>
    <skos:prefLabel xml:lang="pt">Ortoimagens</skos:prefLabel>
    <skos:scopeNote xml:lang="pt">Imagens georeferenciadas da superfície terrestre recolhidas por satélite ou sensores aéreos.</skos:scopeNote>
    <skos:prefLabel xml:lang="ro">Ortoimagini</skos:prefLabel>
    <skos:scopeNote xml:lang="ro">Imagini georeferențiate ale suprafeței terestre, înregistrate cu senzori plasați pe sateliți sau aeropurtați.</skos:scopeNote>
    <skos:prefLabel xml:lang="sk">Ortometria</skos:prefLabel>
    <skos:scopeNote xml:lang="sk">Georeferencované obrazové údaje o zemskom povrchu buď zo satelitu alebo z leteckých snímačov.</skos:scopeNote>
    <skos:prefLabel xml:lang="sl">Ortofoto</skos:prefLabel>
    <skos:scopeNote xml:lang="sl">Geolocirani slikovni podatki zemeljske površine iz satelita ali senzorjev v zraku.</skos:scopeNote>
    <skos:prefLabel xml:lang="sv">Ortofoto</skos:prefLabel>
    <skos:scopeNote xml:lang="sv">Georefererade bilddata över jordytan, antingen från satelliter eller från flygburna sensorer.</skos:scopeNote>
    <skos:altLabel>oi</skos:altLabel>
    <skos:inScheme rdf:resource="http://inspire.ec.europa.eu/theme" />
  </skos:Concept>
  <skos:Concept xmlns:skos="http://www.w3.org/2004/02/skos/core#" rdf:about="http://inspire.ec.europa.eu/theme/af">
    <skos:prefLabel xml:lang="en">Agricultural and aquaculture facilities</skos:prefLabel>
    <skos:scopeNote xml:lang="en">Farming equipment and production facilities (including irrigation systems, greenhouses and stables).</skos:scopeNote>
    <skos:prefLabel xml:lang="bg">Селскостопански и водностопански съоръжения</skos:prefLabel>
    <skos:scopeNote xml:lang="bg">Оборудване за селски стопанства и производствени мощности (включително поливни системи, парници и обори).</skos:scopeNote>
    <skos:prefLabel xml:lang="cs">Zemědělská a akvakulturní zařízení</skos:prefLabel>
    <skos:scopeNote xml:lang="cs">Vybavení a zařízení zemědělské výroby (včetně zavlažovacích systémů, skleníků a stájí).</skos:scopeNote>
    <skos:prefLabel xml:lang="hr">Objekti i strojevi za poljoprivredu i akvakulturu</skos:prefLabel>
    <skos:scopeNote xml:lang="hr">Oprema za poljodjelstvo i proizvodni objekti i strojevi (uključujući sustave navodnjavanja, staklenike i štale).</skos:scopeNote>
    <skos:prefLabel xml:lang="da">Landbrugs- og akvakulturanlæg</skos:prefLabel>
    <skos:scopeNote xml:lang="da">Landbrugsudstyr og -produktionsanlæg (herunder vandingssystemer, drivhuse og stalde).</skos:scopeNote>
    <skos:prefLabel xml:lang="de">Landwirtschaftliche Anlagen und Aquakulturanlagen</skos:prefLabel>
    <skos:scopeNote xml:lang="de">Landwirtschaftliche Anlagen und Produktionsstätten (einschließlich Bewässerungssystemen, Gewächshäusern und Ställen).</skos:scopeNote>
    <skos:prefLabel xml:lang="el">Γεωργικές εγκαταστάσεις και εγκαταστάσεις υδατοκαλλιέργειας</skos:prefLabel>
    <skos:scopeNote xml:lang="el">Γεωργικός εξοπλισμός και εγκαταστάσεις παραγωγής (συμπεριλαμβανομένων των συστημάτων άρδευσης, των θερμοκηπίων και των στάβλων).</skos:scopeNote>
    <skos:prefLabel xml:lang="es">Instalaciones agrícolas y de acuicultura</skos:prefLabel>
    <skos:scopeNote xml:lang="es">Equipamiento e instalaciones de producción agraria (incluidos sistemas de regadío, invernaderos y establos).</skos:scopeNote>
    <skos:prefLabel xml:lang="et">Põllumajandus- ja vesiviljelusrajatised</skos:prefLabel>
    <skos:scopeNote xml:lang="et">Põllumajandusseadmed ja tootmisrajatised (sealhulgas niisutussüsteemid, kasvuhooned ja laudad).</skos:scopeNote>
    <skos:prefLabel xml:lang="fi">Maatalous- ja vesiviljelylaitokset</skos:prefLabel>
    <skos:scopeNote xml:lang="fi">Maatalouden tuotantolaitteet ja -laitteistot (mukaan luettuina kastelujärjestelmät, kasvihuoneet ja eläinsuojat).</skos:scopeNote>
    <skos:prefLabel xml:lang="fr">Installations agricoles et aquacoles</skos:prefLabel>
    <skos:scopeNote xml:lang="fr">Équipement et installations de production agricoles (y compris les systèmes d'irrigation, les serres et les étables).</skos:scopeNote>
    <skos:prefLabel xml:lang="hu">Mezőgazdasági és akvakultúra-ágazati létesítmények</skos:prefLabel>
    <skos:scopeNote xml:lang="hu">Mezőgazdasági eszközök és termelőlétesítmények (beleértve az öntözőrendszereket, üvegházakat és istállókat).</skos:scopeNote>
    <skos:prefLabel xml:lang="it">Impianti agricoli e di acquacoltura</skos:prefLabel>
    <skos:scopeNote xml:lang="it">Apparecchiature e impianti di produzione agricola (compresi i sistemi di irrigazione, le serre e le stalle).</skos:scopeNote>
    <skos:prefLabel xml:lang="lt">Žemės ūkio ir akvakultūros infrastruktūra</skos:prefLabel>
    <skos:scopeNote xml:lang="lt">Žemės ūkio įrenginiai ir gamybos infrastruktūra (įskaitant drėkinimo sistemas, šiltnamius ir tvartus).</skos:scopeNote>
    <skos:prefLabel xml:lang="lv">Lauksaimniecības un akvakultūras iekārtas</skos:prefLabel>
    <skos:scopeNote xml:lang="lv">Lauksaimniecības ierīces un ražošanas iekārtas (tostarp apūdeņošanas sistēmas, siltumnīcas un staļļi).</skos:scopeNote>
    <skos:prefLabel xml:lang="mt">Faċilitajiet agrikoli u ta' l-akwakultura</skos:prefLabel>
    <skos:scopeNote xml:lang="mt">Tagħmir tal-biedja u faċilitajiet ta' produzzjoni (inklużi sistemi ta' irrigazzjoni, serer u stalel).</skos:scopeNote>
    <skos:prefLabel xml:lang="nl">Faciliteiten voor landbouw en aquacultuur</skos:prefLabel>
    <skos:scopeNote xml:lang="nl">Landbouwuitrusting en productiefaciliteiten (met inbegrip van irrigatiesystemen, broeikassen en stallen).</skos:scopeNote>
    <skos:prefLabel xml:lang="pl">Obiekty rolnicze oraz akwakultury</skos:prefLabel>
    <skos:scopeNote xml:lang="pl">Urządzenia rolnicze oraz urządzenia produkcyjne (łącznie z systemami nawadniania, szklarniami i stajniami).</skos:scopeNote>
    <skos:prefLabel xml:lang="pt">Instalações agrícolas e aquícolas</skos:prefLabel>
    <skos:scopeNote xml:lang="pt">Equipamento e instalações de explorações agrícolas e aquícolas (incluindo sistemas de irrigação, estufas e viveiros, e estábulos).</skos:scopeNote>
    <skos:prefLabel xml:lang="ro">Instalații agricole și pentru acvacultură</skos:prefLabel>
    <skos:scopeNote xml:lang="ro">Echipament și instalații de producție agricolă (inclusiv sisteme de irigație, sere și grajduri).</skos:scopeNote>
    <skos:prefLabel xml:lang="sk">Poľnohospodárske zariadenia a zariadenia akvakultúry</skos:prefLabel>
    <skos:scopeNote xml:lang="sk">Poľnohospodárske vybavenie a výrobné zariadenia (vrátane zavlažovacích systémov, skleníkov a stajní).</skos:scopeNote>
    <skos:prefLabel xml:lang="sl">Objekti in naprave za kmetijstvo in ribogojstvo</skos:prefLabel>
    <skos:scopeNote xml:lang="sl">Kmetijska oprema ter proizvodni objekti in naprave (vključno z namakalnimi sistemi, rastlinjaki in hlevi).</skos:scopeNote>
    <skos:prefLabel xml:lang="sv">Jordbruks- och vattenbruksanläggningar</skos:prefLabel>
    <skos:scopeNote xml:lang="sv">Jordbruksutrustning och produktionsanläggningar (inbegripet bevattningssystem, växthus och djurstallar).</skos:scopeNote>
    <skos:altLabel>af</skos:altLabel>
    <skos:inScheme rdf:resource="http://inspire.ec.europa.eu/theme" />
  </skos:Concept>
  <skos:Concept xmlns:skos="http://www.w3.org/2004/02/skos/core#" rdf:about="http://inspire.ec.europa.eu/theme/am">
    <skos:prefLabel xml:lang="en">Area management/restriction/regulation zones and reporting units</skos:prefLabel>
    <skos:scopeNote xml:lang="en">Areas managed, regulated or used for reporting at international, European, national, regional and local levels. Includes dumping sites, restricted areas around drinking water sources, nitrate-vulnerable zones, regulated fairways at sea or large inland waters, areas for the dumping of waste, noise restriction zones, prospecting and mining permit areas, river basin districts, relevant reporting units and coastal zone management areas.</skos:scopeNote>
    <skos:prefLabel xml:lang="bg">Управление на територията/ограничени/регулирани зони и отчетни единици</skos:prefLabel>
    <skos:scopeNote xml:lang="bg">Зони, управлявани, регулирани или използвани за докладване на международно, европейско, национално, регионално и местно равнище. Включва складови обекти, ограничени райони около източници на питейна вода, уязвими от замърсяване с нитрати зони, контролирани морски проходи или големи вътрешни водни пътища, райони за складиране на отпадъци, зони с наложени ограничения върху шума, проучвателни и минни райони, райони на речни басейни, съответни отчетни единици и зони за управление на брегови райони.</skos:scopeNote>
    <skos:prefLabel xml:lang="cs">Správní oblasti/chráněná pásma/regulovaná území a jednotky podávající hlášení</skos:prefLabel>
    <skos:scopeNote xml:lang="cs">Oblasti spravované, regulované nebo používané pro hlášení na mezinárodní, evropské, celostátní, regionální nebo místní úrovni. Zahrnuje skládky, pásma hygienické ochrany vodních zdrojů, oblasti zranitelné dusičnany, regulované plavební dráhy na moři nebo rozsáhlých vnitrozemských vodních plochách, oblasti pro ukládání odpadů, pásma s omezením hladiny hluku, povolená průzkumná a těžební území, oblasti povodí, příslušné jednotky pro podávání hlášení a pásma pobřežní správy.</skos:scopeNote>
    <skos:prefLabel xml:lang="hr">Područja upravljanja/zaštićena područja/uređena područja i jedinice za izvještavanje</skos:prefLabel>
    <skos:scopeNote xml:lang="hr">Područja kojima se upravlja, koja se uređuju ili koriste za izvještavanje na međunarodnoj, europskoj, državnoj ili regionalnoj razini. Uključuju odlagališta smeća, zaštićena područja oko izvora pitke vode, područja osjetljiva na nitrate, uređene plovne putovi na moru ili unutarnje vode, područja za odlaganje otpada, područja zaštićena od buke, područja s dozvolom za istraživanje ruda i rudarenje, područja riječnih bazena, odgovarajuće jedinice za izvještavanje i područja za upravljanje obalnim pojasom.</skos:scopeNote>
    <skos:prefLabel xml:lang="da">Forvaltede og regulerede områder samt områder med brugsbegrænsning og indberetningsenheder</skos:prefLabel>
    <skos:scopeNote xml:lang="da">Områder, der forvaltes, reguleres eller benyttes som indberetningsenheder på internationalt, europæisk, nationalt, regionalt og lokalt plan. Omfatter affaldsdepoter, områder med brugsbegrænsninger af hensyn til drikkevandsindvinding, nitratfølsomme områder, regulerede sejlruter til søs og på større indlandsvandområder, områder for dumpning af affald, områder med støjbegrænsning, områder, hvor der er tilladelse til efterforskning og minedrift, vandområdedistrikter, relevante indberetningsenheder samt områder for kystzoneforvaltning.</skos:scopeNote>
    <skos:prefLabel xml:lang="de">Bewirtschaftungsgebiete/Schutzgebiete/geregelte Gebiete und Berichterstattungseinheiten</skos:prefLabel>
    <skos:scopeNote xml:lang="de">Auf internationaler, europäischer, nationaler, regionaler und lokaler Ebene bewirtschaftete, geregelte oder zu Zwecken der Berichterstattung herangezogene Gebiete. Dazu zählen Deponien, Trinkwasserschutzgebiete, nitratempfindliche Gebiete, geregelte Fahrwasser auf See oder auf großen Binnengewässern, Gebiete für die Abfallverklappung, Lärmschutzgebiete, für Exploration und Bergbau ausgewiesene Gebiete, Flussgebietseinheiten, entsprechende Berichterstattungseinheiten und Gebiete des Küstenzonenmanagements.</skos:scopeNote>
    <skos:prefLabel xml:lang="el">Ζώνες διαχείρισης/περιορισμού/ρύθμισης εκτάσεων και μονάδες αναφοράς</skos:prefLabel>
    <skos:scopeNote xml:lang="el">Εκτάσεις υπό διαχείριση, υπό ρύθμιση ή χρησιμοποιούμενες για αναφορά σε διεθνές, ευρωπαϊκό, εθνικό, περιφερειακό και τοπικό επίπεδο. Περιλαμβάνονται χώροι απόρριψης, προστατευόμενες περιοχές γύρω από πηγές πόσιμου νερού, ζώνες ευάλωτες στη νιτρορρύπανση, κανονιστικά ρυθμιζόμενοι δίαυλοι θαλάσσιας ή εσωτερικής ναυσιπλοΐας, περιοχές για τη βύθιση αποβλήτων, ζώνες προστασίας από τον θόρυβο, περιοχές όπου επιτρέπεται η μεταλλευτική έρευνα και εξόρυξη, διοικητικές περιοχές ποτάμιων λεκανών, σχετικές μονάδες αναφοράς και περιοχές διαχείρισης παράκτιας ζώνης.</skos:scopeNote>
    <skos:prefLabel xml:lang="es">Zonas sujetas a ordenación, a restricciones o reglamentaciones y unidades de notificación</skos:prefLabel>
    <skos:scopeNote xml:lang="es">Zonas gestionadas, reglamentadas o utilizadas para la elaboración de informes para organismos internacionales, europeos, nacionales, regionales y locales. Se incluirán vertederos, zonas restringidas alrededor de lugares de extracción de agua potable, zonas sensibles a los nitratos, rutas marítimas o por grandes vías navegables reglamentadas, zonas de vertido, zonas de restricción de ruidos, zonas de prospección o extracción minera, demarcaciones hidrográficas, las correspondientes unidades de notificación y planes de ordenación de zonas costeras.</skos:scopeNote>
    <skos:prefLabel xml:lang="et">Üldplaneering/piirangu-/reguleeritud tsoonid ja aruandlusüksused</skos:prefLabel>
    <skos:scopeNote xml:lang="et">Alad, mille haldamisest, reguleerimisest või kasutamisest antakse aru rahvusvahelisel, Euroopa, riiklikul, piirkondlikul ja kohalikul tasandil. Hõlmab kaadamiskohti, joogiveeallikate ümber asuvaid piirangutsoone, nitraaditundlikke tsoone, reguleeritavaid laevateid merel või suurtel siseveekogudel, jäätmete kaadamise alasid, mürapiirangutsoone, geoloogiliste uuringute ja kaevanduste alasid, valgalasid, asjakohaseid aruandlusüksusi ning rannikukaitsealasid.</skos:scopeNote>
    <skos:prefLabel xml:lang="fi">Aluesuunnittelun, rajoitusten ja sääntelyn piiriin kuuluvat alueet ja raportointiyksiköt</skos:prefLabel>
    <skos:scopeNote xml:lang="fi">Alueet, joita hoidetaan, säännellään tai käytetään kansainvälisen, Euroopan, kansallisen, alueellisen tai paikallisen tason raportointiin. Sisältää kaatopaikat, juomavedenottopaikkoja ympäröivät suoja-alueet, nitraatin aiheuttamalle pilaantumiselle alttiit alueet, säännellyt laivaväylät merellä tai suurilla sisävesillä, jätteiden upottamiskiellon soveltamisalaan kuuluvat alueet, melurajoitusalueet, luonnonvarojen tai malmin etsintäalueet, ja kaivostoiminnan lupa-alueet, vesipiirit, asiaankuuluvat raportointiyksiköt ja rannikkoalueiden hallinta-alueet.</skos:scopeNote>
    <skos:prefLabel xml:lang="fr">Zones de gestion, de restriction ou de réglementation et unités de déclaration</skos:prefLabel>
    <skos:scopeNote xml:lang="fr">Zones gérées, réglementées ou utilisées pour les rapports aux niveaux international, européen, national, régional et local. Sont inclus les décharges, les zones restreintes aux alentours des sources d'eau potable, les zones vulnérables aux nitrates, les chenaux réglementés en mer ou les eaux intérieures importantes, les zones destinées à la décharge de déchets, les zones soumises à limitation du bruit, les zones faisant l'objet de permis d'exploration et d'extraction minière, les districts hydrographiques, les unités correspondantes utilisées pour les rapports et les zones de gestion du littoral.</skos:scopeNote>
    <skos:prefLabel xml:lang="hu">Területgazdálkodási/-korlátozási/-szabályozási övezetek és adatszolgáltató egységek</skos:prefLabel>
    <skos:scopeNote xml:lang="hu">A nemzetközi, európai, nemzeti, regionális és helyi szintű adatszolgáltatás céljából irányított, szabályozott vagy használt területek. Ide tartoznak a lerakóhelyek, az ivóvízforrásokat övező korlátozás alá tartozó területek, a nitrátérzékeny területek, a tengeri hajóutak vagy nagy kiterjedésű belvizek szabályozott hajózóútjai, a hulladéklerakásra kijelölt területek, a zajvédelmi zónák, az előkészítő és bányászatiengedély-köteles területek, a folyómedri kerületek, a megfelelő adatszolgáltató egységek és a tengerparti igazgatási térségek.</skos:scopeNote>
    <skos:prefLabel xml:lang="it">Zone sottoposte a gestione/limitazioni/regolamentazione e unità con obbligo di comunicare dati</skos:prefLabel>
    <skos:scopeNote xml:lang="it">Aree gestite, regolamentate o utilizzate per la comunicazione di dati a livello internazionale, europeo, nazionale, regionale e locale. Sono comprese le discariche, le zone vietate attorno alle sorgenti di acqua potabile, le zone sensibili ai nitrati, le vie navigabili regolamentate in mare o in acque interne di grandi dimensioni, le zone per lo smaltimento dei rifiuti, le zone di limitazione del rumore, le zone in cui sono autorizzate attività di prospezione ed estrazione, i distretti idrografici, le pertinenti unità con obbligo di comunicare dati e le aree in cui vigono piani di gestione delle zone costiere.</skos:scopeNote>
    <skos:prefLabel xml:lang="lt">Tvarkomos teritorijos, ribojamos ir reglamentuojamos zonos bei vienetai, už kuriuos atsiskaitoma</skos:prefLabel>
    <skos:scopeNote xml:lang="lt">Tvarkomos/ribojamos/reglamentuojamos zonos ir vienetai, už kuriuos atsiskaitoma tarptautiniu, Europos, nacionaliniu, regioniniu arba vietos lygmeniu tvarkomos ir reglamentuojamos zonos arba zonos, apie kurias rengiamos ataskaitos. Tai apima sąvartynus, ribotos veiklos zonas aplink geriamo vandens šaltinius, nitratų pažeidžiamas zonas, reglamentuojamus jūros arba didelių vidaus vandenų farvaterius, atliekų aikšteles, zonas, kuriose ribojamas triukšmas, vietas, kuriose reikalingas leidimas žvalgybai ar kasinėjimui, upių baseinų sritis, atitinkamas vietoves, apie kurias rengiamos ataskaitos, ir pakrančių zonos tvarkymo vietoves.</skos:scopeNote>
    <skos:prefLabel xml:lang="lv">Apgabala pārvaldības/ierobežojumu/reglamentētas zonas un ziņošanas vienības</skos:prefLabel>
    <skos:scopeNote xml:lang="lv">Apgabali, ko pārvalda, reglamentē vai lieto, lai sniegtu ziņojumus starptautiskā, Eiropas, valsts, reģiona un pašvaldības līmenī. Ietver izgāztuves, liegumus ap dzeramā ūdens avotiem, pret nitrātiem jutīgas zonas, reglamentētus kuģu ceļus jūrā vai lielos iekšzemes ūdeņos, atkritumu izgāšanas apgabalus, zonas ar trokšņu ierobežojumiem, zonas, kurās atļauta ģeoloģisko atradņu izpēte un izrakteņu ieguve, upju baseinu apgabalus, attiecīgas ziņošanas vienības un krasta zonas apsaimniekošanas apgabalus.</skos:scopeNote>
    <skos:prefLabel xml:lang="mt">Amministrazzjoni ta' żoni/restrizzjoni/żoni regolati u unitajiet ta' rapportar</skos:prefLabel>
    <skos:scopeNote xml:lang="mt">Żoni amministrati, regolati jew użati għar-rappurtar fuq il-livell internazzjonali, Ewropew, nazzjonali, reġjonali u lokali. Huma inklużi siti użati għar-radam, żoni ristretti madwar għejjun ta' l-ilma għax-xorb, żoni vulnerabbli għan-nitrati, kanali regolati fil-baħar jew f'ilmijiet interni kbar, żoni għar-radam ta' l-iskart, żoni għar-restrizzjoni ta' l-istorbju, żoni b'permess għat-tħaffir u għat-tiftix ta' minerali, distretti ta' baċiri tax-xmajjar, unitajiet ta' rapportar rilevanti u żoni ta' amministrazzjoni ta' l-inħawi tal-kosta.</skos:scopeNote>
    <skos:prefLabel xml:lang="nl">Gebiedsbeheer, gebieden waar beperkingen gelden, gereguleerde gebieden en rapportage-eenheden</skos:prefLabel>
    <skos:scopeNote xml:lang="nl">Gebieden die worden beheerd, gereguleerd of gebruikt voor rapportage op internationaal, Europees, nationaal, regionaal en lokaal niveau, met inbegrip van stortplaatsen, gebieden rond drinkwaterbronnen waar beperkingen gelden, nitraatgevoelige gebieden, gereguleerde vaarwegen op zee of op grote binnenwateren, gebieden voor het storten van afval, gebieden waar geluidsbeperkingen gelden, gebieden met toestemming voor exploratie en mijnbouw, stoomgebieden, relevante rapportage-eenheden en gebieden voor kustbeheer.</skos:scopeNote>
    <skos:prefLabel xml:lang="pl">Gospodarowanie obszarem/strefy ograniczone/regulacyjne oraz jednostki sprawozdawcze</skos:prefLabel>
    <skos:scopeNote xml:lang="pl">Obszary zarządzane, regulowane lub wykorzystywane do celów sprawozdawczych na poziomie międzynarodowym, europejskim, krajowym, regionalnym i lokalnym. Obejmują również wysypiska śmieci, obszary o ograniczonym dostępie wokół ujęć wody pitnej, strefy zagrożone przez azotany, uregulowane drogi wodne na morzach lub wodach śródlądowych o dużej powierzchni, obszary przeznaczone pod wysypiska śmieci, strefy ograniczeń hałasu, obszary wymagające zezwolenia na poszukiwania i wydobycie, obszary dorzeczy, odpowiednie jednostki sprawozdawcze i obszary zarządzania strefą brzegową.</skos:scopeNote>
    <skos:prefLabel xml:lang="pt">Zonas de gestão/restrição/regulamentação e unidades de referência</skos:prefLabel>
    <skos:scopeNote xml:lang="pt">Zonas geridas, regulamentadas ou utilizadas para a comunicação de dados a nível internacional, europeu, nacional, regional e local. Compreende aterros, zonas de acesso restrito em torno de nascentes de água potável, zonas sensíveis aos nitratos, vias navegáveis regulamentadas no mar ou em águas interiores de grandes dimensões, zonas de descarga de resíduos, zonas de ruído condicionado, zonas autorizadas para efeitos de prospecção e extracção mineira, bacias hidrográficas, unidades de referência pertinentes e zonas abrangidas pela gestão das zonas costeiras.</skos:scopeNote>
    <skos:prefLabel xml:lang="ro">Zone de administrare/restricție/reglementare și unități de raportare</skos:prefLabel>
    <skos:scopeNote xml:lang="ro">Zone administrate, reglementate sau folosite pentru raportarea la nivel internațional, european, național, regional și local. Sunt incluse gropile de gunoi, zonele restricționate din apropierea surselor de apă potabilă, zonele vulnerabile la nitrați, șenalele navigabile reglementate de pe mare sau din apele interne importante, zonele destinate descărcării deșeurilor, zonele în care au fost introduse limite de zgomot, zonele care fac obiectul unui permis de prospectare și de exploatare minieră, districtele hidrografice, unitățile de raportare corespunzătoare și zonele de administrare a litoralului.</skos:scopeNote>
    <skos:prefLabel xml:lang="sk">Spravované/obmedzené/regulované zóny a jednotky podávajúce správy</skos:prefLabel>
    <skos:scopeNote xml:lang="sk">Oblasti, ktoré sú spravované, regulované alebo využívané na podávanie správ na medzinárodnej, európskej, celoštátnej, regionálnej a miestnej úrovni. Patria sem skládky, ochranné pásma v okolí zdrojov pitnej vody, oblasti citlivé na dusík, regulované plavebné cesty na mori alebo na rozsiahlych vnútrozemských vodných plochách a tokoch, oblasti určené na skladovanie odpadu, oblasti s obmedzením hluku, oblasti, v ktorých je povolený prieskum a ťažba, oblasti povodí, príslušné jednotky na podávanie správ a oblasti správy pobrežných zón.</skos:scopeNote>
    <skos:prefLabel xml:lang="sl">Območja upravljanja/zaprta območja/regulirana območja in poročevalske enote</skos:prefLabel>
    <skos:scopeNote xml:lang="sl">Območja, ki se upravljajo, urejajo ali uporabljajo za poročanje na mednarodni, evropski, nacionalni, regionalni in lokalni ravni. Vključujejo odlagališča odpadkov, zaprta območja okrog virov pitne vode, cone, občutljive na nitrate, urejene plovne poti po morju ali velikih celinskih vodah, območja za odlaganje odpadkov, cone z omejitvijo hrupa, območja, kjer je potrebno dovoljenje za iskanje rud in rudarjenje, predele povodij, ustrezne poročevalske enote in območja upravljanja obalnih con.</skos:scopeNote>
    <skos:prefLabel xml:lang="sv">Områden med särskild förvaltning/begränsningar/reglering samt enheter för rapportering</skos:prefLabel>
    <skos:scopeNote xml:lang="sv">Områden som förvaltas, regleras eller används för rapportering på internationell, europeisk, nationell, regional och lokal nivå. Innefattar avfallsdeponier, skyddsområden runt dricksvattentäkter, områden som är känsliga för nitratbelastning, reglerade farleder till havs och i större inlandsvatten, områden för dumpning av avfall, områden med bullerrestriktioner, områden med tillstånd för prospektering och gruvbrytning, avrinningsdistrikt, relevanta enheter för rapportering och områden med kustförvaltning.</skos:scopeNote>
    <skos:altLabel>am</skos:altLabel>
    <skos:inScheme rdf:resource="http://inspire.ec.europa.eu/theme" />
  </skos:Concept>
  <skos:Concept xmlns:skos="http://www.w3.org/2004/02/skos/core#" rdf:about="http://inspire.ec.europa.eu/theme/ac">
    <skos:prefLabel xml:lang="en">Atmospheric conditions</skos:prefLabel>
    <skos:scopeNote xml:lang="en">Physical conditions in the atmosphere. Includes spatial data based on measurements, on models or on a combination thereof and includes measurement locations.</skos:scopeNote>
    <skos:prefLabel xml:lang="bg">Атмосферни условия</skos:prefLabel>
    <skos:scopeNote xml:lang="bg">Физически атмосферни условия. Включва пространствени данни, основаващи се на измервания, на модели или на комбинация от двете, както и местата, където са направени измерванията.</skos:scopeNote>
    <skos:prefLabel xml:lang="cs">Stav ovzduší</skos:prefLabel>
    <skos:scopeNote xml:lang="cs">Fyzikální stav ovzduší. Zahrnuje prostorová data založená na měřeních, modelech nebo jejich kombinaci, jakož i místa měření.</skos:scopeNote>
    <skos:prefLabel xml:lang="hr">Atmosferski uvjeti</skos:prefLabel>
    <skos:scopeNote xml:lang="hr">Fizikalni uvjeti u atmosferi. Uključujući prostorne podatke koji se temelje na mjerenjima, uzorcima ili na njihovom spoju i uključuju lokacije za mjerenje.</skos:scopeNote>
    <skos:prefLabel xml:lang="da">Atmosfæriske forhold</skos:prefLabel>
    <skos:scopeNote xml:lang="da">Fysiske forhold i atmosfæren. Omfatter geodata, der bygger på målinger, modeller eller begge dele; omfatter også målepunkternes placering.</skos:scopeNote>
    <skos:prefLabel xml:lang="de">Atmosphärische Bedingungen</skos:prefLabel>
    <skos:scopeNote xml:lang="de">Physikalische Bedingungen in der Atmosphäre. Dazu zählen Geodaten auf der Grundlage von Messungen, Modellen oder einer Kombination aus beiden sowie Angabe der Messstandorte.</skos:scopeNote>
    <skos:prefLabel xml:lang="el">Ατμοσφαιρικές συνθήκες</skos:prefLabel>
    <skos:scopeNote xml:lang="el">Φυσικές ιδιότητες της ατμόσφαιρας. Περιλαμβάνονται χωρικά δεδομένα βασιζόμενα σε μετρήσεις, σε μοντέλα ή σε συνδυασμό τους, καθώς και οι τοποθεσίες μετρήσεων.</skos:scopeNote>
    <skos:prefLabel xml:lang="es">Condiciones atmosféricas</skos:prefLabel>
    <skos:scopeNote xml:lang="es">Condiciones físicas de la atmósfera. Se incluirán datos espaciales basados en mediciones, modelos o en una combinación de ambos, así como los lugares de medición.</skos:scopeNote>
    <skos:prefLabel xml:lang="et">Atmosfääritingimused</skos:prefLabel>
    <skos:scopeNote xml:lang="et">Füüsikalised tingimused atmosfääris. Hõlmab mõõtmiste ja modelleerimise tulemusel või nende kahe meetodi kombineerimisel saadud ruumiandmeid ning mõõtmiskohti.</skos:scopeNote>
    <skos:prefLabel xml:lang="fi">Ilmakehän tila</skos:prefLabel>
    <skos:scopeNote xml:lang="fi">Ilmakehän fysikaaliset olosuhteet. Sisältää mittauksiin, malleihin tai näiden yhdistelmiin perustuvia paikkatietoja sekä tiedot mittauspaikoista.</skos:scopeNote>
    <skos:prefLabel xml:lang="fr">Conditions atmosphériques</skos:prefLabel>
    <skos:scopeNote xml:lang="fr">Conditions physiques dans l'atmosphère. Comprend les données géographiques fondées sur des mesures, sur des modèles ou sur une combinaison des deux, ainsi que les lieux de mesure.</skos:scopeNote>
    <skos:prefLabel xml:lang="hu">Légköri viszonyok</skos:prefLabel>
    <skos:scopeNote xml:lang="hu">A légkör fizikai jellemzői. Ide tartoznak a méréseken, modelleken vagy ezek kombinációján alapuló téradatok, továbbá a mérési helyek.</skos:scopeNote>
    <skos:prefLabel xml:lang="it">Condizioni atmosferiche</skos:prefLabel>
    <skos:scopeNote xml:lang="it">Condizioni fisiche dell’atmosfera. Questa voce comprende i dati territoriali basati su misurazioni, su modelli o su una combinazione dei due e comprende i punti di misurazione.</skos:scopeNote>
    <skos:prefLabel xml:lang="lt">Atmosferos sąlygos</skos:prefLabel>
    <skos:scopeNote xml:lang="lt">Fizinės atmosferos sąlygos. Tai apima matavimais, modeliais arba abiem būdais pagrįstus erdvinius duomenis, nurodant matavimo vietas.</skos:scopeNote>
    <skos:prefLabel xml:lang="lv">Atmosfēras apstākļi</skos:prefLabel>
    <skos:scopeNote xml:lang="lv">Fizikālie atmosfēras apstākļi. Tie ietver telpiskos datus, kuru pamatā ir mērījumi vai modeļi, vai to kombinācija, kā arī norādes par to veikšanas vietu.</skos:scopeNote>
    <skos:prefLabel xml:lang="mt">Kondizzjonijiet atmosferiċi</skos:prefLabel>
    <skos:scopeNote xml:lang="mt">Kondizzjonijiet fiżiċi fl-atmosfera. Hija inkluża data ġeografika bbażata fuq kejl, fuq mudelli jew fuq il-kombinazzjoni tagħhom kif ukoll is-siti tal-kejl.</skos:scopeNote>
    <skos:prefLabel xml:lang="nl">Atmosferische omstandigheden</skos:prefLabel>
    <skos:scopeNote xml:lang="nl">Fysische omstandigheden in de atmosfeer, met inbegrip van ruimtelijke gegevens die gebaseerd zijn op metingen, modellen of een combinatie daarvan, en met inbegrip van meetlocaties.</skos:scopeNote>
    <skos:prefLabel xml:lang="pl">Warunki atmosferyczne</skos:prefLabel>
    <skos:scopeNote xml:lang="pl">Warunki fizyczne w atmosferze. Obejmują dane przestrzenne oparte na pomiarach, modelach lub na kombinacji tych dwóch elementów, a także lokalizacje pomiarów.</skos:scopeNote>
    <skos:prefLabel xml:lang="pt">Condições atmosféricas</skos:prefLabel>
    <skos:scopeNote xml:lang="pt">Condições físicas da atmosfera. Inclui dados geográficos baseados em medições, em modelos ou numa combinação de ambos, bem como os sítios de medição.</skos:scopeNote>
    <skos:prefLabel xml:lang="ro">Condiții atmosferice</skos:prefLabel>
    <skos:scopeNote xml:lang="ro">Condițiile fizice din atmosferă. Sunt incluse datele spațiale bazate pe măsurători, pe modele sau pe o combinație între acestea, precum și locațiile de efectuare a măsurătorilor.</skos:scopeNote>
    <skos:prefLabel xml:lang="sk">Atmosférické podmienky</skos:prefLabel>
    <skos:scopeNote xml:lang="sk">Fyzikálne podmienky v atmosfére. Patria sem priestorové údaje založené na meraniach, modeloch alebo na kombinácii meraní a modelov vrátane miest meraní.</skos:scopeNote>
    <skos:prefLabel xml:lang="sl">Ozračje</skos:prefLabel>
    <skos:scopeNote xml:lang="sl">Fizikalne razmere v atmosferi. Vključujejo prostorske podatke, ki temeljijo na merjenjih, vzorcih ali na kombinaciji le-teh, in merilne lokacije.</skos:scopeNote>
    <skos:prefLabel xml:lang="sv">Atmosfäriska förhållanden</skos:prefLabel>
    <skos:scopeNote xml:lang="sv">Fysikaliska förhållanden i atmosfären. Inbegriper rumsliga data baserade på mätningar, modeller eller en kombination av dessa, samt mätpunkternas läge.</skos:scopeNote>
    <skos:altLabel>ac</skos:altLabel>
    <skos:inScheme rdf:resource="http://inspire.ec.europa.eu/theme" />
  </skos:Concept>
  <skos:Concept xmlns:skos="http://www.w3.org/2004/02/skos/core#" rdf:about="http://inspire.ec.europa.eu/theme/br">
    <skos:prefLabel xml:lang="en">Bio-geographical regions</skos:prefLabel>
    <skos:scopeNote xml:lang="en">Areas of relatively homogeneous ecological conditions with common characteristics.</skos:scopeNote>
    <skos:prefLabel xml:lang="bg">Биогеографски региони</skos:prefLabel>
    <skos:scopeNote xml:lang="bg">Райони с относително еднородни екологични условия с общи характеристики.</skos:scopeNote>
    <skos:prefLabel xml:lang="cs">Bioregiony</skos:prefLabel>
    <skos:scopeNote xml:lang="cs">Oblasti s poměrně stejnorodými ekologickými podmínkami a společnými vlastnostmi.</skos:scopeNote>
    <skos:prefLabel xml:lang="hr">Biogeografske regije</skos:prefLabel>
    <skos:scopeNote xml:lang="hr">Područja s relativno homogenim ekološkim uvjetima koja imaju zajedničke osobine.</skos:scopeNote>
    <skos:prefLabel xml:lang="da">Biogeografiske regioner</skos:prefLabel>
    <skos:scopeNote xml:lang="da">Områder, der har relativt ensartede økologiske forhold med fælles egenskaber.</skos:scopeNote>
    <skos:prefLabel xml:lang="de">Biogeografische Regionen</skos:prefLabel>
    <skos:scopeNote xml:lang="de">Gebiete mit relativ homogenen ökologischen Bedingungen und gemeinsamen Merkmalen.</skos:scopeNote>
    <skos:prefLabel xml:lang="el">Βιογεωγραφικές περιοχές</skos:prefLabel>
    <skos:scopeNote xml:lang="el">Περιοχές σχετικώς ομοιογενών οικολογικών συνθηκών με κοινά χαρακτηριστικά.</skos:scopeNote>
    <skos:prefLabel xml:lang="es">Regiones biogeográficas</skos:prefLabel>
    <skos:scopeNote xml:lang="es">Zonas dotadas de condiciones ecológicas relativamente homogéneas con unas características comunes.</skos:scopeNote>
    <skos:prefLabel xml:lang="et">Bio-geograafilised piirkonnad</skos:prefLabel>
    <skos:scopeNote xml:lang="et">Suhteliselt ühetaoliste ökoloogiliste tingimustega ja ühiste tunnustega piirkonnad.</skos:scopeNote>
    <skos:prefLabel xml:lang="fi">Biomaantieteelliset alueet</skos:prefLabel>
    <skos:scopeNote xml:lang="fi">Alueet, joilla on suhteellisen yhtenäiset ekologiset olosuhteet ja yhteisiä ominaispiirteitä.</skos:scopeNote>
    <skos:prefLabel xml:lang="fr">Régions biogéographiques</skos:prefLabel>
    <skos:scopeNote xml:lang="fr">Zones présentant des conditions écologiques relativement homogènes avec des caractéristiques communes.</skos:scopeNote>
    <skos:prefLabel xml:lang="hu">Biogeográfiai régiók</skos:prefLabel>
    <skos:scopeNote xml:lang="hu">Közös tulajdonságokkal bíró, viszonylag homogén ökológiai jellemzőkkel rendelkező térségek.</skos:scopeNote>
    <skos:prefLabel xml:lang="it">Regioni biogeografiche</skos:prefLabel>
    <skos:scopeNote xml:lang="it">Aree che presentano condizioni ecologiche relativamente omogenee con caratteristiche comuni.</skos:scopeNote>
    <skos:prefLabel xml:lang="lt">Biogeografiniai regionai</skos:prefLabel>
    <skos:scopeNote xml:lang="lt">Teritorijos, kurioms būdingos palyginti homogeniškos ekologinės sąlygos ir panašios charakteristikos.</skos:scopeNote>
    <skos:prefLabel xml:lang="lv">Bioģeogrāfiskie reģioni</skos:prefLabel>
    <skos:scopeNote xml:lang="lv">Apgabali ar relatīvi viendabīgiem ekoloģiskiem apstākļiem un noteiktām kopīgam iezīmēm.</skos:scopeNote>
    <skos:prefLabel xml:lang="mt">Reġjuni bijo-ġeografiċi</skos:prefLabel>
    <skos:scopeNote xml:lang="mt">Żoni ta' kondizzjonijiet ekoloġiċi relattivament omoġenji b'karatteristiċi komuni.</skos:scopeNote>
    <skos:prefLabel xml:lang="nl">Biogeografische gebieden</skos:prefLabel>
    <skos:scopeNote xml:lang="nl">Gebieden met betrekkelijk homogene ecologische omstandigheden die gemeenschappelijke kenmerken vertonen.</skos:scopeNote>
    <skos:prefLabel xml:lang="pl">Regiony biogeograficzne</skos:prefLabel>
    <skos:scopeNote xml:lang="pl">Obszary o stosunkowo jednorodnych warunkach ekologicznych i o wspólnych cechach.</skos:scopeNote>
    <skos:prefLabel xml:lang="pt">Regiões biogeográficas</skos:prefLabel>
    <skos:scopeNote xml:lang="pt">Zonas de condições ecológicas relativamente homogéneas com características comuns.</skos:scopeNote>
    <skos:prefLabel xml:lang="ro">Regiuni biogeografice</skos:prefLabel>
    <skos:scopeNote xml:lang="ro">Zone care prezintă condiții ecologice relativ omogene, având caracteristici comune.</skos:scopeNote>
    <skos:prefLabel xml:lang="sk">Biogeografické regióny</skos:prefLabel>
    <skos:scopeNote xml:lang="sk">Oblasti s pomerne rovnorodými ekologickými vlastnosťami so spoločnými vlastnosťami.</skos:scopeNote>
    <skos:prefLabel xml:lang="sl">Biogeografske regije</skos:prefLabel>
    <skos:scopeNote xml:lang="sl">Območja z relativno homogenimi ekološkimi razmerami s skupnimi značilnostmi.</skos:scopeNote>
    <skos:prefLabel xml:lang="sv">Biogeografiska regioner</skos:prefLabel>
    <skos:scopeNote xml:lang="sv">Områden som har relativt homogena ekologiska förhållanden med likartade egenskaper.</skos:scopeNote>
    <skos:altLabel>br</skos:altLabel>
    <skos:inScheme rdf:resource="http://inspire.ec.europa.eu/theme" />
  </skos:Concept>
  <skos:Concept xmlns:skos="http://www.w3.org/2004/02/skos/core#" rdf:about="http://inspire.ec.europa.eu/theme/bu">
    <skos:prefLabel xml:lang="en">Buildings</skos:prefLabel>
    <skos:scopeNote xml:lang="en">Geographical location of buildings.</skos:scopeNote>
    <skos:prefLabel xml:lang="bg">Сгради</skos:prefLabel>
    <skos:scopeNote xml:lang="bg">Географско разположение на сградите.</skos:scopeNote>
    <skos:prefLabel xml:lang="cs">Budovy</skos:prefLabel>
    <skos:scopeNote xml:lang="cs">Zeměpisná poloha budov.</skos:scopeNote>
    <skos:prefLabel xml:lang="hr">Zgrade</skos:prefLabel>
    <skos:scopeNote xml:lang="hr">Geografski položaj zgrada.</skos:scopeNote>
    <skos:prefLabel xml:lang="da">Bygninger</skos:prefLabel>
    <skos:scopeNote xml:lang="da">Geografisk stedfæstelse af bygninger.</skos:scopeNote>
    <skos:prefLabel xml:lang="de">Gebäude</skos:prefLabel>
    <skos:scopeNote xml:lang="de">Geografischer Standort von Gebäuden.</skos:scopeNote>
    <skos:prefLabel xml:lang="el">Κτίρια</skos:prefLabel>
    <skos:scopeNote xml:lang="el">Γεωγραφική θέση κτιρίων.</skos:scopeNote>
    <skos:prefLabel xml:lang="es">Edificios</skos:prefLabel>
    <skos:scopeNote xml:lang="es">Localización geográfica de los edificios.</skos:scopeNote>
    <skos:prefLabel xml:lang="et">Ehitised</skos:prefLabel>
    <skos:scopeNote xml:lang="et">Ehitiste geograafiline asukoht.</skos:scopeNote>
    <skos:prefLabel xml:lang="fi">Rakennukset</skos:prefLabel>
    <skos:scopeNote xml:lang="fi">Rakennusten maantieteellinen sijainti.</skos:scopeNote>
    <skos:prefLabel xml:lang="fr">Bâtiments</skos:prefLabel>
    <skos:scopeNote xml:lang="fr">Situation géographique des bâtiments.</skos:scopeNote>
    <skos:prefLabel xml:lang="hu">Épületek</skos:prefLabel>
    <skos:scopeNote xml:lang="hu">Az épületek földrajzi helye.</skos:scopeNote>
    <skos:prefLabel xml:lang="it">Edifici</skos:prefLabel>
    <skos:scopeNote xml:lang="it">Localizzazione geografica degli edifici.</skos:scopeNote>
    <skos:prefLabel xml:lang="lt">Pastatai</skos:prefLabel>
    <skos:scopeNote xml:lang="lt">Geografinė pastatų buvimo vieta.</skos:scopeNote>
    <skos:prefLabel xml:lang="lv">Ēkas</skos:prefLabel>
    <skos:scopeNote xml:lang="lv">Ēku ģeogrāfiskā atrašanās vieta.</skos:scopeNote>
    <skos:prefLabel xml:lang="mt">Bini</skos:prefLabel>
    <skos:scopeNote xml:lang="mt">Posizzjoni ġeografika ta' bini.</skos:scopeNote>
    <skos:prefLabel xml:lang="nl">Gebouwen</skos:prefLabel>
    <skos:scopeNote xml:lang="nl">Geografische locatie van gebouwen.</skos:scopeNote>
    <skos:prefLabel xml:lang="pl">Budynki</skos:prefLabel>
    <skos:scopeNote xml:lang="pl">Położenie geograficzne budynków.</skos:scopeNote>
    <skos:prefLabel xml:lang="pt">Edifícios</skos:prefLabel>
    <skos:scopeNote xml:lang="pt">Localização geográfica dos edifícios.</skos:scopeNote>
    <skos:prefLabel xml:lang="ro">Clădiri</skos:prefLabel>
    <skos:scopeNote xml:lang="ro">Localizarea geografică a clădirilor.</skos:scopeNote>
    <skos:prefLabel xml:lang="sk">Stavby</skos:prefLabel>
    <skos:scopeNote xml:lang="sk">Zemepisná poloha stavieb.</skos:scopeNote>
    <skos:prefLabel xml:lang="sl">Stavbe</skos:prefLabel>
    <skos:scopeNote xml:lang="sl">Prostorska lega stavb.</skos:scopeNote>
    <skos:prefLabel xml:lang="sv">Byggnader</skos:prefLabel>
    <skos:scopeNote xml:lang="sv">Geografiskt läge för byggnader.</skos:scopeNote>
    <skos:altLabel>bu</skos:altLabel>
    <skos:inScheme rdf:resource="http://inspire.ec.europa.eu/theme" />
  </skos:Concept>
  <skos:Concept xmlns:skos="http://www.w3.org/2004/02/skos/core#" rdf:about="http://inspire.ec.europa.eu/theme/er">
    <skos:prefLabel xml:lang="en">Energy resources</skos:prefLabel>
    <skos:scopeNote xml:lang="en">Energy resources including hydrocarbons, hydropower, bio-energy, solar, wind, etc., where relevant including depth/height information on the extent of the resource.</skos:scopeNote>
    <skos:prefLabel xml:lang="bg">Енергийни източници</skos:prefLabel>
    <skos:scopeNote xml:lang="bg">Енергийни източници, включително въглеводород, водна енергия, биоенергия, слънчева енергия, енергия от вятър и други; по целесъобразност се включва информация за дълбочина/височина на района на източника.</skos:scopeNote>
    <skos:prefLabel xml:lang="cs">Energetické zdroje</skos:prefLabel>
    <skos:scopeNote xml:lang="cs">Energetické zdroje, včetně uhlovodíků, vodní energie, bioenergie, sluneční a větrné energie atd., případně včetně informací o hloubce nebo výšce týkajících se rozsahu zdroje.</skos:scopeNote>
    <skos:prefLabel xml:lang="hr">Izvori energije</skos:prefLabel>
    <skos:scopeNote xml:lang="hr">Izvori energije, uključujući ugljikovodike, vodenu energiju, bioenergiju, solarnu energiju, vjetar itd., uključujući dubinske/visinske informacije o veličini izvora ako je potrebno.</skos:scopeNote>
    <skos:prefLabel xml:lang="da">Energiressourcer</skos:prefLabel>
    <skos:scopeNote xml:lang="da">Energiressourcer, herunder kulbrinter, vandkraft, bioenergi, sol, vind osv. samt, hvis det er relevant, dybde-/højdeoplysninger om ressourcens omfang.</skos:scopeNote>
    <skos:prefLabel xml:lang="de">Energiequellen</skos:prefLabel>
    <skos:scopeNote xml:lang="de">Energiequellen wie Kohlenwasserstoffe, Wasserkraft, Bioenergie, Sonnen- und Windenergie usw., gegebenenfalls mit Tiefen- bzw. Höhenangaben zur Ausdehnung der Energiequelle.</skos:scopeNote>
    <skos:prefLabel xml:lang="el">Ενεργειακοί πόροι</skos:prefLabel>
    <skos:scopeNote xml:lang="el">Ενεργειακοί πόροι, μεταξύ άλλων υδρογονάνθρακες, υδροηλεκτρική ενέργεια, βιοενέργεια, ηλιακή ενέργεια, αιολική ενέργεια, κ.λπ., συμπεριλαμβανομένων, κατά περίπτωση, πληροφοριών περί του βάθους και του ύψους όσον αφορά την έκταση του εκάστοτε πόρου.</skos:scopeNote>
    <skos:prefLabel xml:lang="es">Recursos energéticos</skos:prefLabel>
    <skos:scopeNote xml:lang="es">Recursos energéticos: hidrocarburos, energía hidroeléctrica, bioenergía, energía solar y eólica, etc., incluyendo, cuando proceda, la información de profundidad y altura del volumen de los recursos.</skos:scopeNote>
    <skos:prefLabel xml:lang="et">Energiaressursid</skos:prefLabel>
    <skos:scopeNote xml:lang="et">Energiaressursid, sealhulgas süsivesinikud, hüdroenergia, bioenergia, päikese-, tuule- jne energia, sealhulgas koos asjakohase sügavust/kõrgust puudutava teabega ressursi mahu kohta.</skos:scopeNote>
    <skos:prefLabel xml:lang="fi">Energiavarat</skos:prefLabel>
    <skos:scopeNote xml:lang="fi">Energiavarat, mukaan lukien hiilivedyt, vesivoima, bioenergia, aurinko, tuuli jne., mukaan luettuina tarvittaessa syvyys-/korkeustiedot kyseisen luonnonvaran laajuudesta.</skos:scopeNote>
    <skos:prefLabel xml:lang="fr">Sources d'énergie</skos:prefLabel>
    <skos:scopeNote xml:lang="fr">Sources d'énergie comprenant les hydrocarbures, l'énergie hydraulique, la bioénergie, l'énergie solaire, l'énergie éolienne, etc., le cas échéant accompagnées d'informations relatives à la profondeur/la hauteur de la source.</skos:scopeNote>
    <skos:prefLabel xml:lang="hu">Energiaforrások</skos:prefLabel>
    <skos:scopeNote xml:lang="hu">Energiaforrások, beleértve a szénhidrogéneket, vízenergiát, bioenergiát, nap- és szélenergiát stb., adott esetben beleértve az erőforrás mértékére vonatkozó mélységi/magassági információt.</skos:scopeNote>
    <skos:prefLabel xml:lang="it">Risorse energetiche</skos:prefLabel>
    <skos:scopeNote xml:lang="it">Risorse energetiche, compresi gli idrocarburi, l'energia idroelettrica, la bioenergia, l'energia solare, eolica, ecc., ove opportuno anche informazioni, in termini di altezza/profondità, sull'entità della risorsa.</skos:scopeNote>
    <skos:prefLabel xml:lang="lt">Energijos ištekliai</skos:prefLabel>
    <skos:scopeNote xml:lang="lt">Energijos ištekliai, įskaitant angliavandenilius, hidroenergiją, bioenergiją, saulės ir vėjo energiją ir t. t., tam tikrais atvejais įskaitant informaciją apie išteklių apimties gylį/aukštį.</skos:scopeNote>
    <skos:prefLabel xml:lang="lv">Enerģijas resursi</skos:prefLabel>
    <skos:scopeNote xml:lang="lv">Enerģijas resursi, tostarp ogļūdeņraži, ūdens enerģija, bioenerģija, saules enerģija, vēja enerģija, utt., attiecīgā gadījumā ietverot informāciju par dziļumu/augstumu attiecībā uz resursu apmēru.</skos:scopeNote>
    <skos:prefLabel xml:lang="mt">Riżorsi ta' enerġija</skos:prefLabel>
    <skos:scopeNote xml:lang="mt">Riżorsi ta' enerġija inklużi idrokarboni, enerġija idro-elettrika, bijo-enerġija, bix-xemx, bir-riħ, eċċ., fejn ikun rilevanti, inkluża informazzjoni dwar il-fond/l-għoli rigward id-daqs tar-riżors.</skos:scopeNote>
    <skos:prefLabel xml:lang="nl">Energiebronnen</skos:prefLabel>
    <skos:scopeNote xml:lang="nl">Energiebronnen met inbegrip van koolwaterstof, waterkracht, bio-energie, zon, wind enz., waar passend met inbegrip van diepte/hoogte-informatie over de omvang van de bron.</skos:scopeNote>
    <skos:prefLabel xml:lang="pl">Zasoby energetyczne</skos:prefLabel>
    <skos:scopeNote xml:lang="pl">Zasoby energii, w tym węglowodory, energia wodna, bioenergia, energia słoneczna, wiatrowa itd., w odpowiednich przypadkach łącznie z informacjami dotyczącymi głębokości/wysokości i rozmiarów danych zasobów.</skos:scopeNote>
    <skos:prefLabel xml:lang="pt">Recursos energéticos</skos:prefLabel>
    <skos:scopeNote xml:lang="pt">Recursos energéticos, incluindo os de hidrocarbonetos, hidroeléctricos, de bio-energias, de energia solar, eólica, etc., incluindo, quando pertinente, informação sobre as cotas de profundidade/altura do recurso.</skos:scopeNote>
    <skos:prefLabel xml:lang="ro">Resurse energetice</skos:prefLabel>
    <skos:scopeNote xml:lang="ro">Resurse energetice precum hidrocarburi, energia hidraulică, bioenergia, energia solară, energia eoliană etc., însoțite de informații privind adâncimea/înălțimea la care se află resursa, după caz.</skos:scopeNote>
    <skos:prefLabel xml:lang="sk">Zdroje energie</skos:prefLabel>
    <skos:scopeNote xml:lang="sk">Zdroje energie vrátane uhľovodíkov, vodnej energie, energie z biomasy, solárnej energie, veternej energie atď., ak je to možné vrátane informácie o šírke a dĺžke rozlohy zdroja.</skos:scopeNote>
    <skos:prefLabel xml:lang="sl">Energetski viri</skos:prefLabel>
    <skos:scopeNote xml:lang="sl">Energetski viri, vključno z ogljikovodiki, vodno energijo, bioenergijo, soncem, vetrom itd., kjer je to ustrezno vključno s podatki o globini/višini glede velikosti vira.</skos:scopeNote>
    <skos:prefLabel xml:lang="sv">Energiresurser</skos:prefLabel>
    <skos:scopeNote xml:lang="sv">Energiresurser, inbegripet kolväten, vattenkraft, bioenergi, sol, vind osv., i tillämpliga fall med djup-/höjdinformation om resursens omfattning.</skos:scopeNote>
    <skos:altLabel>er</skos:altLabel>
    <skos:inScheme rdf:resource="http://inspire.ec.europa.eu/theme" />
  </skos:Concept>
  <skos:Concept xmlns:skos="http://www.w3.org/2004/02/skos/core#" rdf:about="http://inspire.ec.europa.eu/theme/ef">
    <skos:prefLabel xml:lang="en">Environmental monitoring facilities</skos:prefLabel>
    <skos:scopeNote xml:lang="en">Location and operation of environmental monitoring facilities includes observation and measurement of emissions, of the state of environmental media and of other ecosystem parameters (biodiversity, ecological conditions of vegetation, etc.) by or on behalf of public authorities.</skos:scopeNote>
    <skos:prefLabel xml:lang="bg">Съоръжения за управление на околната среда</skos:prefLabel>
    <skos:scopeNote xml:lang="bg">Местонахождението и действието на съоръжения за мониторинг на околната среда включват наблюдение и измерване на емисиите, на състоянието на факторите на околната среда и на други параметри на екосистемата (биологично разнообразие, екологични условия на флората и други), извършвани от публичните власти или от тяхно име.</skos:scopeNote>
    <skos:prefLabel xml:lang="cs">Zařízení pro sledování životního prostředí</skos:prefLabel>
    <skos:scopeNote xml:lang="cs">Rozmístění a provoz zařízení pro sledování životního prostředí zahrnuje pozorování a měření emisí, stavu složek životního prostředí a dalších ukazatelů ekosystému (druhové rozmanitosti, ekologických podmínek rostlinstva atd.) orgány veřejné správy nebo jejich jménem.</skos:scopeNote>
    <skos:prefLabel xml:lang="hr">Sustavi za nadzor okoliša</skos:prefLabel>
    <skos:scopeNote xml:lang="hr">Lokacija i djelovanje sustava za nadzor okoliša koji uključuju promatranje i mjerenje emisija, stanje okoliša, kao i drugih parametara ekosustava (biološka raznolikost, ekološko stanje vegetacije itd.) putem ili u ime tijela javne vlasti.</skos:scopeNote>
    <skos:prefLabel xml:lang="da">Miljøovervågningsfaciliteter</skos:prefLabel>
    <skos:scopeNote xml:lang="da">Lokalisering og drift af miljøovervågningsfaciliteter omfatter observation og måling af emissioner, af miljøelementernes tilstand og af andre økosystemparametre (biodiversitet, plantevækstens økologiske betingelser, osv.) foretaget af eller på vegne af offentlige myndigheder.</skos:scopeNote>
    <skos:prefLabel xml:lang="de">Umweltüberwachung</skos:prefLabel>
    <skos:scopeNote xml:lang="de">Standort und Betrieb von Umweltüberwachungseinrichtungen einschließlich Beobachtung und Messung von Schadstoffen, des Zustands von Umweltmedien und anderen Parametern des Ökosystems (Artenvielfalt, ökologischer Zustand der Vegetation usw.) durch oder im Auftrag von öffentlichen Behörden.</skos:scopeNote>
    <skos:prefLabel xml:lang="el">Εγκαταστάσεις παρακολούθησης του περιβάλλοντος</skos:prefLabel>
    <skos:scopeNote xml:lang="el">Η τοποθεσία και η λειτουργία των εγκαταστάσεων παρακολούθησης του περιβάλλοντος περιλαμβάνει την παρατήρηση και τη μέτρηση των εκπομπών, της κατάστασης των στοιχείων του περιβάλλοντος και άλλων παραμέτρων του οικοσυστήματος (βιοποικιλότητα, οικολογική κατάσταση της βλάστησης, κ.λπ.) από τις δημόσιες αρχές ή για λογαριασμό τους.</skos:scopeNote>
    <skos:prefLabel xml:lang="es">Instalaciones de observación del medio ambiente</skos:prefLabel>
    <skos:scopeNote xml:lang="es">La ubicación y funcionamiento de instalaciones de observación del medio ambiente, encargadas de observar y medir emisiones, el estado del medio ambiente y otros parámetros del ecosistema (biodiversidad, condiciones ecológicas de la vegetación, etc.), por parte de las autoridades públicas o en nombre de ellas.</skos:scopeNote>
    <skos:prefLabel xml:lang="et">Keskkonnaseirerajatised</skos:prefLabel>
    <skos:scopeNote xml:lang="et">Keskkonnaseirerajatiste asukoht ja kasutamine hõlmab heidete, keskkonnaelementide seisundi ja muude ökosüsteemi parameetrite (bioloogilise mitmekesisuse, taimkatte ökoloogiliste tingimuste jne) vaatlust ja mõõtmist avaliku võimu kandjate poolt või nende nimel.</skos:scopeNote>
    <skos:prefLabel xml:lang="fi">Ympäristön tilan seurantalaitteet</skos:prefLabel>
    <skos:scopeNote xml:lang="fi">Ympäristön tilan seurantalaitteiden sijaintiin ja käyttöön kuuluu päästöjen, ilman, maaperän ja veden tilan ja muiden ekosysteemin muuttujien (luonnon monimuotoisuus, kasviston ekologiset olot jne.) seuranta ja mittaukset, joista vastaavat viranomaiset tai muut toimijat viranomaisten puolesta.</skos:scopeNote>
    <skos:prefLabel xml:lang="fr">Installations de suivi environnemental</skos:prefLabel>
    <skos:scopeNote xml:lang="fr">La situation et le fonctionnement des installations de suivi environnemental comprennent l'observation et la mesure des émissions, de l'état du milieu environnemental et d'autres paramètres de l'écosystème (biodiversité, conditions écologiques de la végétation, etc.) par les autorités publiques ou pour leur compte.</skos:scopeNote>
    <skos:prefLabel xml:lang="hu">Környezetvédelmi monitoringlétesítmények</skos:prefLabel>
    <skos:scopeNote xml:lang="hu">A környezetvédelmi monitoringlétesítmények elhelyezkedése és működése magában foglalja a kibocsátásnak, a környezeti elemek állapotának, valamint az ökoszisztéma egyéb paramétereinek (biodiverzitás, a növényzet ökológiai állapota stb.) a hatóságok általi vagy a nevükben történő megfigyelését és mérését.</skos:scopeNote>
    <skos:prefLabel xml:lang="it">Impianti di monitoraggio ambientale</skos:prefLabel>
    <skos:scopeNote xml:lang="it">L'ubicazione e il funzionamento degli impianti di monitoraggio ambientale comprendono l'osservazione e la misurazione delle emissioni, dello stato dei comparti ambientali e di altri parametri dell'ecosistema (biodiversità, condizioni ecologiche della vegetazione, ecc.) da parte o per conto delle autorità pubbliche.</skos:scopeNote>
    <skos:prefLabel xml:lang="lt">Aplinkos stebėsenos priemonės</skos:prefLabel>
    <skos:scopeNote xml:lang="lt">Aplinkos stebėsenos priemonių vieta ir veikla, įskaitant valdžios institucijų arba jų vardu atliekamą išmetamų teršalų, aplinkos terpių būklės ir kitų ekosistemos parametrų (biologinės įvairovės, ekologinių augalijos sąlygų ir t. t.) stebėjimą ir matavimą.</skos:scopeNote>
    <skos:prefLabel xml:lang="lv">Vides monitoringa iekārtas</skos:prefLabel>
    <skos:scopeNote xml:lang="lv">Vides monitoringa iekārtu atrašanās vietas un pārvaldība, kas ietver emisiju, apkārtējās vides stāvokļa un citu ekosistēmas parametru (bioloģiskās daudzveidības, veģetācijas ekoloģisko apstākļu, utt.) novērošanu un mērīšanu, ko veic publiskās iestādes vai publisko iestāžu vārdā.</skos:scopeNote>
    <skos:prefLabel xml:lang="mt">Faċilitajiet ta' monitoraġġ ambjentali</skos:prefLabel>
    <skos:scopeNote xml:lang="mt">Posizzjoni u operazzjoni ta' faċilitajiet ta' monitoraġġ ambjentali jinkludi l-osservazzjoni u l-kejl ta' emissjonijiet, ta' l-istat tal-medji ambjentali u ta' parametri oħra ta' l-ekosistema (biodiversità, kondizzjonijiet ekoloġiċi ta' veġetazzjoni, eċċ.) permezz jew f'isem l-awtoritajiet pubbliċi.</skos:scopeNote>
    <skos:prefLabel xml:lang="nl">Milieubewakingsvoorzieningen</skos:prefLabel>
    <skos:scopeNote xml:lang="nl">Locatie en werking van milieubewakingsvoorzieningen, met inbegrip van waarneming en meting van emissies, de staat van de milieucompartimenten en van andere ecosysteemparameters (biodiversiteit, ecologische omstandigheden van vegetatie, enz.) door of namens de overheidsinstanties.</skos:scopeNote>
    <skos:prefLabel xml:lang="pl">Urządzenia do monitorowania środowiska</skos:prefLabel>
    <skos:scopeNote xml:lang="pl">Lokalizacja i funkcjonowanie urządzeń do monitorowania środowiska obejmują obserwację i pomiary emisji, stanu zasobów środowiska i innych parametrów ekosystemu (różnorodności biologicznej, warunków ekologicznych wegetacji itd.) przez organy publiczne lub w ich imieniu.</skos:scopeNote>
    <skos:prefLabel xml:lang="pt">Instalações de monitorização do ambiente</skos:prefLabel>
    <skos:scopeNote xml:lang="pt">A localização e funcionamento de instalações de monitorização do ambiente inclui a observação e medição de emissões, do estado das diferentes componentes ambientais e de outros parâmetros dos ecossistemas (biodiversidade, condições ecológicas da vegetação, etc.) pelas autoridades públicas ou por conta destas.</skos:scopeNote>
    <skos:prefLabel xml:lang="ro">Instalații de supraveghere a mediului</skos:prefLabel>
    <skos:scopeNote xml:lang="ro">Amplasarea și exploatarea instalațiilor de supraveghere a mediului implică observarea și măsurarea emisiilor, a stării mediului înconjurător și a altor parametri ai ecosistemului (biodiversitate, condiții ecologice ale vegetației etc.) de către sau în numele autorităților publice.</skos:scopeNote>
    <skos:prefLabel xml:lang="sk">Zariadenia na monitorovanie životného prostredia</skos:prefLabel>
    <skos:scopeNote xml:lang="sk">Poloha a prevádzka zariadení na monitorovanie životného prostredia zahŕňa pozorovanie a meranie emisií, stavu zložiek životného prostredia a iných parametrov ekosystému (biodiverzity, ekologických podmienok vegetácie, atď.) vykonávané orgánmi verejnej moci alebo v ich mene.</skos:scopeNote>
    <skos:prefLabel xml:lang="sl">Naprave in objekti za monitoring okolja</skos:prefLabel>
    <skos:scopeNote xml:lang="sl">Nahajanje in delovanje naprav in objektov za spremljanje okolja vključuje opazovanje in merjenje emisij, stanja okolja in drugih parametrov ekosistema (biološka raznolikost, ekološki pogoji vegetacije itd.) s strani javnih organov ali v njihovem imenu.</skos:scopeNote>
    <skos:prefLabel xml:lang="sv">Anläggningar för miljöövervakning</skos:prefLabel>
    <skos:scopeNote xml:lang="sv">Placering och användning av anläggningar för miljöövervakning inbegriper iakttagelse och mätning av utsläpp, av situationen när det gäller miljömedier och av andra parametrar för ekosystemet (biologisk mångfald, ekologiska villkor för växtligheten etc.) som genomförs av offentliga myndigheter eller för deras räkning.</skos:scopeNote>
    <skos:altLabel>ef</skos:altLabel>
    <skos:inScheme rdf:resource="http://inspire.ec.europa.eu/theme" />
  </skos:Concept>
  <skos:Concept xmlns:skos="http://www.w3.org/2004/02/skos/core#" rdf:about="http://inspire.ec.europa.eu/theme/hb">
    <skos:prefLabel xml:lang="en">Habitats and biotopes</skos:prefLabel>
    <skos:scopeNote xml:lang="en">Geographical areas characterised by specific ecological conditions, processes, structure, and (life support) functions that physically support the organisms that live there. Includes terrestrial and aquatic areas distinguished by geographical, abiotic and biotic features, whether entirely natural or semi-natural.</skos:scopeNote>
    <skos:prefLabel xml:lang="bg">Местообитания и биотопи</skos:prefLabel>
    <skos:scopeNote xml:lang="bg">Географски райони, характеризиращи се със специфични екологични условия, процеси, структура и (животоподпомагащи) функции, подпомагащи физически организмите, които ги обитават. Включват земни или водни райони, отличаващи се с напълно естествени или полуестествени географски, абиотични и биотични характеристики.</skos:scopeNote>
    <skos:prefLabel xml:lang="cs">Stanoviště a biotopy</skos:prefLabel>
    <skos:scopeNote xml:lang="cs">Zeměpisné oblasti vyznačující se zvláštními ekologickými podmínkami, procesy, strukturami a (životně důležitými) funkcemi, které skýtají fyzickou podporu organismům, které v nich žijí. Zahrnují pozemské a vodní oblasti rozlišené podle zeměpisných, abiotických a biotických prvků, přirozené i částečně přirozené povahy.</skos:scopeNote>
    <skos:prefLabel xml:lang="hr">Staništa i biotopi</skos:prefLabel>
    <skos:scopeNote xml:lang="hr">Geografska područja za koja su svojstveni posebni ekološki uvjeti, procesi, strukture i funkcije (za održavanje života) koje fizički pomažu organizmima da žive na njima. Uključujući kopnena i vodena područja koja se razlikuju po geografskim, abiotičkim i biotičkim značajkama, bilo da su u potpunosti prirodna ili polu-prirodna.</skos:scopeNote>
    <skos:prefLabel xml:lang="da">Levesteder og biotoper</skos:prefLabel>
    <skos:scopeNote xml:lang="da">Geografiske områder, der er kendetegnet ved særlige økologiske forhold, processer, strukturer og (livsunderstøttende) funktioner, og som er det fysiske grundlag for de organismer, der lever der. Omfatter land- og vandområder, som er kendetegnet ved særlige geografiske, abiotiske eller biotiske forhold, uanset om de er helt eller delvis naturlige.</skos:scopeNote>
    <skos:prefLabel xml:lang="de">Lebensräume und Biotope</skos:prefLabel>
    <skos:scopeNote xml:lang="de">Geografische Gebiete mit spezifischen ökologischen Bedingungen, Prozessen, Strukturen und (lebensunterstützenden) Funktionen als physische Grundlage für dort lebende Organismen. Dies umfasst auch durch geografische, abiotische und biotische Merkmale gekennzeichnete natürliche oder naturnahe terrestrische und aquatische Gebiete.</skos:scopeNote>
    <skos:prefLabel xml:lang="el">Ενδιαιτήματα και βιότοποι</skos:prefLabel>
    <skos:scopeNote xml:lang="el">Γεωγραφικές περιοχές που χαρακτηρίζονται από ειδικές οικολογικές συνθήκες, διαδικασίες, δομή και λειτουργίες (υποστήριξης της ζωής) οι οποίες στηρίζουν φυσικά τους οργανισμούς που ενδιαιτούν. Περιλαμβάνονται χερσαίες και υδάτινες εκτάσεις, διακρινόμενες ανάλογα με τα γεωγραφικά, αβιοτικά και βιοτικά χαρακτηριστικά τους, ανεξαρτήτως εάν είναι πλήρως φυσικές ή ημιφυσικές.</skos:scopeNote>
    <skos:prefLabel xml:lang="es">Hábitats y biotopos</skos:prefLabel>
    <skos:scopeNote xml:lang="es">Zonas geográficas caracterizadas por unas condiciones ecológicas específicas, procesos, estructuras y funciones de apoyo vital que sean soporte físico de los organismos que viven en ellas. Se incluirán zonas terrestres y acuáticas diferenciadas por sus características geográficas, abióticas y bióticas, tanto si son enteramente naturales como seminaturales.</skos:scopeNote>
    <skos:prefLabel xml:lang="et">Elupaigad ja biotoobid</skos:prefLabel>
    <skos:scopeNote xml:lang="et">Geograafilised alad, mida iseloomustavad spetsiifilised ökoloogilised tingimused, protsessid, struktuurid ja (elu alalhoiu-) funktsioonid, mis füüsiliselt toetavad seal elavaid organisme. Hõlmab maa- ja veealasid, mida eristatakse geograafiliste, abiootiliste ja biootiliste tunnuste järgi ja mis on täielikult looduslikud või poollooduslikud.</skos:scopeNote>
    <skos:prefLabel xml:lang="fi">Elinympäristöt ja biotoopit</skos:prefLabel>
    <skos:scopeNote xml:lang="fi">Maantieteelliset alueet, joille ovat ominaisia erityiset ekologiset olosuhteet, prosessit, rakenne ja (elämää ylläpitävät) toiminnot, jotka tukevat fysikaalisesti alueella eläviä organismeja. Sisältää maa- ja vesialueet, joilla on omat maantieteelliset, abioottiset ja bioottiset ominaisuutensa ja jotka ovat joko luonnontilassa tai osittain luonnontilassa.</skos:scopeNote>
    <skos:prefLabel xml:lang="fr">Habitats et biotopes</skos:prefLabel>
    <skos:scopeNote xml:lang="fr">Zones géographiques ayant des caractéristiques écologiques particulières — conditions, processus, structures et fonctions (de maintien de la vie) — favorables aux organismes qui y vivent. Sont incluses les zones terrestres et aquatiques qui se distinguent par leurs caractéristiques géographiques, abiotiques ou biotiques, qu'elles soient naturelles ou semi-naturelles.</skos:scopeNote>
    <skos:prefLabel xml:lang="hu">Élőhelyek és biotópok</skos:prefLabel>
    <skos:scopeNote xml:lang="hu">Olyan földrajzi területek, amelyeket különleges ökológiai feltételek, folyamatok, struktúra és (az élet fenntartásához kapcsolódó) funkciók jellemeznek, amelyek az ott élő organizmusok számára kedvező fizikai feltételeket teremtenek. Ide tartoznak azok a szárazföldi és vízi térségek, amelyeket – akár teljesen természetesek, akár félig természetesek – földrajzi, abiotikus és biotikus jellemzőik alapján különböztetnek meg.</skos:scopeNote>
    <skos:prefLabel xml:lang="it">Habitat e biotopi</skos:prefLabel>
    <skos:scopeNote xml:lang="it">Aree geografiche caratterizzate da condizioni ecologiche specifiche, processi, strutture e funzioni (di supporto alla vita) che supportano materialmente gli organismi che le abitano. Sono comprese le zone terrestri e acquatiche, interamente naturali o seminaturali, distinte in base agli elementi geografici, abiotici e biotici.</skos:scopeNote>
    <skos:prefLabel xml:lang="lt">Buveinės ir biotopai</skos:prefLabel>
    <skos:scopeNote xml:lang="lt">Geografinės teritorijos, kurioms būdingos specifinės ekologinės sąlygos, procesai, struktūra ir (gyvybės palaikymo) funkcijos, sudarančios gyvenimui tinkamas fizines sąlygas ten gyvenantiems organizmams. Tai apima visiškai natūralias ir pusiau natūralias sausumos ir vandens teritorijas, kurios turi skirtingas geografines, abiotines ir biotines sąlygas.</skos:scopeNote>
    <skos:prefLabel xml:lang="lv">Dzīvotnes un biotopi</skos:prefLabel>
    <skos:scopeNote xml:lang="lv">Ģeogrāfiskie apgabali, kuros ir īpaši ekoloģiskie apstākļi, procesi, struktūra, un (dzīvības atbalsta) funkcijas, kas fiziski atbalsta organismus, kuri tajos dzīvo. Tie ietver pilnīgi un daļēji dabīgas sauszemes vai ūdens platības, ko raksturo ģeogrāfiski, abiotiski un biotiski faktori.</skos:scopeNote>
    <skos:prefLabel xml:lang="mt">L-abitati naturali u l-bijotopi</skos:prefLabel>
    <skos:scopeNote xml:lang="mt">Żoni ġeografiċi kkaratterizzati minn kondizzjonijiet ekoloġiċi, proċessi, struttura, u funzjonijiet (sostenn tal-ħajja) speċifiċi li jsostnu fiżikament l-organiżmi li jgħixu fihom. Huma inklużi żoni ta' l-art jew ta' l-ilma li jingħarfu permezz ta' karatteristiċi ġeografiċi, abijotiċi u bijotiċi, sew jekk għal kollox naturali kif ukoll jekk semi-naturali.</skos:scopeNote>
    <skos:prefLabel xml:lang="nl">Habitats en biotopen</skos:prefLabel>
    <skos:scopeNote xml:lang="nl">Geografische gebieden die worden gekenmerkt door specifieke ecologische omstandigheden, processen, structuur en (leven ondersteunende) functies die fysiek de daar levende organismen ondersteunen, met inbegrip van volledig natuurlijke of semi-natuurlijke land- en wateroppervlakken, onderscheiden naar geografische, abiotische en biotische kenmerken.</skos:scopeNote>
    <skos:prefLabel xml:lang="pl">Siedliska i obszary przyrodniczo jednorodne</skos:prefLabel>
    <skos:scopeNote xml:lang="pl">Obszary geograficzne odznaczające się szczególnymi warunkami przyrodniczymi, procesami, strukturą i (podtrzymującymi życie) funkcjami, które fizycznie umożliwiają egzystencję żyjącym na nich organizmom. Obejmują obszary lądowe i wodne wyróżniające się cechami geograficznymi, abiotycznymi i biotycznymi, czy to w całości naturalne czy też półnaturalne.</skos:scopeNote>
    <skos:prefLabel xml:lang="pt">Habitats e biótopos</skos:prefLabel>
    <skos:scopeNote xml:lang="pt">Zonas geográficas caracterizadas por condições ecológicas, processos, estrutura e funções (de apoio às necessidades básicas) específicos que constituem o suporte físico dos organismos que nelas vivem. Inclui zonas terrestres e aquáticas, naturais ou semi-naturais, diferenciadas pelas suas características geográficas, abióticas e bióticas.</skos:scopeNote>
    <skos:prefLabel xml:lang="ro">Habitate și biotopuri</skos:prefLabel>
    <skos:scopeNote xml:lang="ro">Zone geografice caracterizate prin condiții ecologice specifice, procese, structură și funcții (de menținere a vieții pe pământ) care sprijină fizic organismele care trăiesc acolo. Sunt incluse zonele terestre și acvatice care se disting prin caracteristicile lor geografice, abiotice și biotice, indiferent că acestea sunt naturale sau seminaturale.</skos:scopeNote>
    <skos:prefLabel xml:lang="sk">Habitaty a biotopy</skos:prefLabel>
    <skos:scopeNote xml:lang="sk">Geografické oblasti, pre ktoré sú charakteristické špecifické ekologické vlastnosti, procesy, štruktúra a (pre život dôležité) funkcie, ktoré fyzikálne podporujú organizmy žijúce na ich území. Patria sem suchozemské a vodné oblasti rozlíšené podľa geografických, abiotických a biotických prvkov, buď výhradne prírodné, alebo poloprírodné.</skos:scopeNote>
    <skos:prefLabel xml:lang="sl">Habitati in biotopi</skos:prefLabel>
    <skos:scopeNote xml:lang="sl">Geografska območja, za katera so značilne posebne ekološke razmere, procesi, struktura in funkcije, ki fizično omogočajo organizmom, da tam živijo. Vključujejo kopenska in vodna območja, ki se razlikujejo po geografskih, abiotskih in biotskih značilnostih, ne glede na to, ali so popolnoma naravna ali polnaravna.</skos:scopeNote>
    <skos:prefLabel xml:lang="sv">Naturtyper och biotoper</skos:prefLabel>
    <skos:scopeNote xml:lang="sv">Geografiska områden som kännetecknas av särskilda ekologiska förhållanden, processer, strukturer och (livsstödjande) funktioner och som är fysiska livsmiljöer för organismer som lever där. Inbegriper land- och vattenområden med särskilda geografiska, abiotiska och biotiska egenskaper, oavsett om de är naturliga eller delvis naturliga.</skos:scopeNote>
    <skos:altLabel>hb</skos:altLabel>
    <skos:inScheme rdf:resource="http://inspire.ec.europa.eu/theme" />
  </skos:Concept>
  <skos:Concept xmlns:skos="http://www.w3.org/2004/02/skos/core#" rdf:about="http://inspire.ec.europa.eu/theme/hh">
    <skos:prefLabel xml:lang="en">Human health and safety</skos:prefLabel>
    <skos:scopeNote xml:lang="en">Geographical distribution of dominance of pathologies (allergies, cancers, respiratory diseases, etc.), information indicating the effect on health (biomarkers, decline of fertility, epidemics) or well-being of humans (fatigue, stress, etc.) linked directly (air pollution, chemicals, depletion of the ozone layer, noise, etc.) or indirectly (food, genetically modified organisms, etc.) to the quality of the environment.</skos:scopeNote>
    <skos:prefLabel xml:lang="bg">Здраве и безопасност на човека</skos:prefLabel>
    <skos:scopeNote xml:lang="bg">Географско разпределение на преобладаващите патологии (алергии, рак, болести на дихателните пътища и др.), информация за въздействието върху човешкото здраве (биомаркери, намаляване на раждаемостта, епидемии) или за физическото състояние на човека (умора, стрес и други), пряко свързани (замърсяване на въздуха, химикали, изтъняване на озоновия слой, шум и др.) или непряко свързани (храна, генетично модифицирани организми и други) с качеството на околната среда.</skos:scopeNote>
    <skos:prefLabel xml:lang="cs">Lidské zdraví a bezpečnost</skos:prefLabel>
    <skos:scopeNote xml:lang="cs">Zeměpisné rozložení převládajícího výskytu patologických stavů (alergií, rakovin, nemocí dýchacího ústrojí atd.), informace o dopadu na zdraví (biomarkery, pokles plodnosti, epidemie) nebo životní podmínky (únava, stres atd.) související přímo (znečištění ovzduší, chemikálie, ztenčování ozonové vrstvy, hluk atd.) nebo nepřímo (potraviny, geneticky modifikované organismy atd.) s kvalitou životního prostředí.</skos:scopeNote>
    <skos:prefLabel xml:lang="hr">Ljudsko zdravlje i sigurnost</skos:prefLabel>
    <skos:scopeNote xml:lang="hr">Geografska raširenost prevladavajućih patoloških pojava (alergije, tumori, bolesti dišnih putova itd.), informacije koje pokazuju učinak na zdravlje (biomarkeri, smanjenje plodnosti, epidemije), ili dobrobit ljudi (umor, stres itd.), koji su direktno (onečišćenje zraka, kemikalije, prorijeđenost ozonskog omotača, buka itd.) ili indirektno povezani (hrana, genetski izmijenjeni organizmi itd.) s kakvoćom okoliša.</skos:scopeNote>
    <skos:prefLabel xml:lang="da">Sikkerhed</skos:prefLabel>
    <skos:scopeNote xml:lang="da">og sundhed Geografisk fordeling af dominansen af patologier (allergier, kræft, luftvejssygdomme, osv.), oplysninger om indvirkningen på menneskers sundhed (biologiske markører, nedsat frugtbarhed, epidemier) eller trivsel (træthed, stress, osv.), der er direkte (luftforurening, kemikalier, udtynding af ozonlaget, støj, osv.) eller indirekte (fødevarer, genmodificerede organismer, osv.) knyttet til miljøkvaliteten.</skos:scopeNote>
    <skos:prefLabel xml:lang="de">Gesundheit und Sicherheit</skos:prefLabel>
    <skos:scopeNote xml:lang="de">Geografische Verteilung verstärkt auftretender pathologischer Befunde (Allergien, Krebserkrankungen, Erkrankungen der Atemwege usw.), Informationen über Auswirkungen auf die Gesundheit (Biomarker, Rückgang der Fruchtbarkeit, Epidemien) oder auf das Wohlbefinden (Ermüdung, Stress usw.) der Menschen in unmittelbarem Zusammenhang mit der Umweltqualität (Luftverschmutzung, Chemikalien, Abbau der Ozonschicht, Lärm usw.) oder in mittelbarem Zusammenhang mit der Umweltqualität (Nahrung, genetisch veränderte Organismen usw.).</skos:scopeNote>
    <skos:prefLabel xml:lang="el">Ανθρώπινη υγεία και ασφάλεια</skos:prefLabel>
    <skos:scopeNote xml:lang="el">Γεωγραφική κατανομή της κυριαρχίας παθολογιών (αλλεργίες, καρκίνοι, αναπνευστικές ασθένειες, κ.λπ.), πληροφορίες που καταδεικνύουν τις επιπτώσεις στην υγεία (βιοδείκτες, πτώση της γονιμότητας, επιδημίες) ή την ευεξία των ανθρώπων (κούραση, υπερένταση, κ.λπ.) που συνδέονται άμεσα (ατμοσφαιρική ρύπανση, χημικές ουσίες, καταστροφή της στιβάδας του όζοντος, θόρυβος, κ.λπ.) ή έμμεσα (τρόφιμα, γενετικώς τροποποιημένοι οργανισμοί, κ.λπ.) με την ποιότητα του περιβάλλοντος.</skos:scopeNote>
    <skos:prefLabel xml:lang="es">Salud y seguridad humanas</skos:prefLabel>
    <skos:scopeNote xml:lang="es">Distribución geográfica de la dominancia de patologías (alergias, cáncer, enfermedades respiratorias, etc.), la información que indique el efecto sobre la salud (marcadores biológicos, declive de la fertilidad, epidemias) o el bienestar humanos (cansancio, estrés, etc.) directamente vinculada con la calidad del medio ambiente (contaminación del aire, productos químicos, enrarecimiento de la capa de ozono, ruido, etc.) o indirectamente vinculada con dicha calidad (alimentos, organismos modificados genéticamente, etc.).</skos:scopeNote>
    <skos:prefLabel xml:lang="et">Inimeste tervis ja ohutus</skos:prefLabel>
    <skos:scopeNote xml:lang="et">Haiguste (allergiad, vähk, hingamisteede haigused jne) domineerimise geograafiline jaotumine, keskkonna kvaliteediga otseselt (õhusaaste, kemikaalid, osoonikihi kahanemine, müra jne) või kaudselt (toit, geneetiliselt muundatud organismid jne) seotud mõjusid inimeste tervisele (biomarkerid, viljatushaiguste sagenemine, epideemiad) või heaolule (väsimus, stress jne) puudutav teave.</skos:scopeNote>
    <skos:prefLabel xml:lang="fi">Väestön terveys ja turvallisuus</skos:prefLabel>
    <skos:scopeNote xml:lang="fi">Ympäristön laatuun välittömästi (esimerkiksi ilman pilaantuminen, kemikaalit, otsonikerroksen oheneminen, melu) tai välillisesti (esimerkiksi elintarvikkeet, muuntogeeniset organismit) yhteydessä olevien sairauksien (esimerkiksi allergiat, syövät, hengityselinsairaudet) maantieteellinen esiintyminen, tiedot, jotka osoittavat vaikutuksen terveyteen (esimerkiksi biologiset merkkiaineet, hedelmällisyyden väheneminen, epidemiat) tai ihmisten hyvinvointiin (esimerkiksi väsymys, stressi).</skos:scopeNote>
    <skos:prefLabel xml:lang="fr">Santé et sécurité des personnes</skos:prefLabel>
    <skos:scopeNote xml:lang="fr">Répartition géographique des pathologies dominantes (allergies, cancers, maladies respiratoires, etc.) liées directement (pollution de l'air, produits chimiques, appauvrissement de la couche d'ozone, bruit, etc.) ou indirectement (alimentation, organismes génétiquement modifiés, etc.) à la qualité de l'environnement, et ensemble des informations relatif à l'effet de celle-ci sur la santé des hommes (marqueurs biologiques, déclin de la fertilité, épidémies) ou leur bien-être (fatigue, stress, etc.).</skos:scopeNote>
    <skos:prefLabel xml:lang="hu">Emberi egészség és biztonság</skos:prefLabel>
    <skos:scopeNote xml:lang="hu">A környezet minőségéhez közvetlenül (légszennyezés, vegyszerek, az ózonréteg elvékonyodása, zaj stb.) vagy közvetve (élelmiszer, genetikailag módosított szervezetek stb.) kapcsolódó patológiák (allergiás, daganatos és légúti megbetegedések stb.) dominanciájának földrajzi eloszlása, illetve ezen tényezőknek az emberi egészségre (biomarkerek, termékenységcsökkenés, járványok) vagy jólétre (fáradtság, stressz stb.) gyakorolt hatását jellemző információ.</skos:scopeNote>
    <skos:prefLabel xml:lang="it">Salute umana e sicurezza</skos:prefLabel>
    <skos:scopeNote xml:lang="it">Distribuzione geografica della prevalenza di patologie (allergie, tumori, malattie respiratorie, ecc.), le informazioni contenenti indicazioni sugli effetti relativi alla salute (indicatori biologici, riduzione della fertilità e epidemie) o al benessere degli esseri umani (affaticamento, stress, ecc.) in relazione alla qualità dell’ambiente, sia in via diretta (inquinamento atmosferico, sostanze chimiche, riduzione dello strato di ozono, rumore, ecc.) che indiretta (alimentazione, organismi geneticamente modificati, ecc.).</skos:scopeNote>
    <skos:prefLabel xml:lang="lt">Žmonių sveikata ir sauga</skos:prefLabel>
    <skos:scopeNote xml:lang="lt">Patologijų dominavimo geografinis pasiskirstymas (alergijos, vėžys, kvėpavimo takų ligos ir t. t.), informacija apie poveikį žmonių sveikatai (biomarkeriai, vaisingumo sumažėjimas, epidemijos) ar gerovei (nuovargis, stresas ir t. t.), tiesiogiai (oro tarša, cheminės medžiagos, ozono sluoksnio retėjimas, triukšmas ir t. t.) arba netiesiogiai (maistas, genetiškai modifikuoti organizmai ir t. t.) susijusi su aplinkos kokybe.</skos:scopeNote>
    <skos:prefLabel xml:lang="lv">Cilvēku veselība un drošība</skos:prefLabel>
    <skos:scopeNote xml:lang="lv">Dominējošo patoloģiju (alerģiju, vēža, elpošanas ceļu slimību, utt.) ģeogrāfiskā izplatība, informācija, kas norāda uz ietekmi uz veselību (biomarkeri, auglības mazināšana, epidēmijas) vai cilvēku labklājību (nogurumu, stresu, utt.), kas tieši (gaisa piesārņojums, ķīmiskās vielas, ozona slāņa noplicināšanās, trokšņi, utt.) vai netieši (pārtika, ģenētiski modificēti organismi, utt.) saistīta ar vides kvalitāti.</skos:scopeNote>
    <skos:prefLabel xml:lang="mt">Is-saħħa u s-siġurtà tal-bniedem</skos:prefLabel>
    <skos:scopeNote xml:lang="mt">Distribuzzjoni ġeografika tad-dominanza ta' patoloġiji (allerġiji, kankri, mard respiratorju, eċċ.), informazzjoni li tindika l-effett fuq is-saħħa (bijomarkaturi, tnaqqis fil-fertilità, epidemiji) jew il-benesseri tal-bnedmin (għejja, stress, eċċ.) b'konnessjoni diretta (tniġġis ta' l-arja, kimiki, tnaqqis tas-saff ta' l-ożonu, storbju, eċċ.) jew indiretta (ikel, organiżmi ġenetikament modifikati, eċċ.) mal-kwalità ta' l-ambjent.</skos:scopeNote>
    <skos:prefLabel xml:lang="nl">Menselijke gezondheid en veiligheid</skos:prefLabel>
    <skos:scopeNote xml:lang="nl">De geografische spreiding van ziekten (allergieën, kankers, ademhalingsziekten, enz.), informatie over de gevolgen voor de gezondheid (biomarkers, vruchtbaarheidsdaling, epidemieën) of het welzijn van de mens (vermoeidheid, stress, enz.) die direct (luchtvervuiling, chemicaliën, aantasting van de ozonlaag, lawaai, enz.) of indirect (voedsel, genetisch gemodificeerde organismen, enz.) samenhangen met de kwaliteit van het milieu.</skos:scopeNote>
    <skos:prefLabel xml:lang="pl">Zdrowie i bezpieczeństwo ludzi</skos:prefLabel>
    <skos:scopeNote xml:lang="pl">Rozmieszczenie geograficzne występowania patologii chorobowych (alergii, nowotworów, chorób układu oddechowego itd.), informacje dotyczące wpływu na zdrowie (biomarkery, spadek płodności, epidemie) lub dobre samopoczucie ludzi (zmęczenie, stres itd.) związane bezpośrednio (zanieczyszczenie powietrza, chemikalia, zubożenie warstwy ozonowej, hałas itd.) lub pośrednio (pożywienie, organizmy zmodyfikowane genetycznie itd.) z jakością środowiska.</skos:scopeNote>
    <skos:prefLabel xml:lang="pt">Saúde humana e segurança</skos:prefLabel>
    <skos:scopeNote xml:lang="pt">Distribuição geográfica da dominância de patologias (alergias, cancros, doenças respiratórias, etc.), informações que indiquem o efeito da qualidade do ambiente sobre a saúde (biomarcadores, declínio da fertilidade, epidemias) ou sobre o bem-estar dos seres humanos (fadiga, tensão, stress, etc.) de forma directa (poluição do ar, produtos químicos, empobrecimento da camada de ozono, ruído, etc.) ou indirecta (alimentação, organismos geneticamente modificados, etc.).</skos:scopeNote>
    <skos:prefLabel xml:lang="ro">Sănătate și siguranță umană</skos:prefLabel>
    <skos:scopeNote xml:lang="ro">Distribuția geografică a patologiilor dominante (alergii, tipuri de cancer, boli respiratorii etc.), precum și informațiile care indică efectul asupra sănătății (indicatorii biologici, scăderea fertilității, epidemiile) sau asupra bunăstării oamenilor (oboseala, stresul etc.), legat în mod direct (poluarea aerului, substanțele chimice, subțierea stratului de ozon, zgomotul etc.) sau indirect (mâncarea, organismele modificate genetic etc.) de calitatea mediului.</skos:scopeNote>
    <skos:prefLabel xml:lang="sk">Ľudské zdravie a bezpečnosť</skos:prefLabel>
    <skos:scopeNote xml:lang="sk">Geografická distribúcia najčastejších ochorení (alergie, nádorové ochorenia, ochorenia dýchacích ciest atď.), informácie o vplyve na zdravie (biologické ukazovatele, pokles plodnosti, epidémie) alebo telesný či duševný stav ľudí (únava, stres atď.), ktoré priamo (znečistenie ovzdušia, chemikálie, oslabenie ozónovej vrstvy, hluk atď.) alebo nepriamo (strava, geneticky upravené organizmy atď.) súvisia s kvalitou životného prostredia.</skos:scopeNote>
    <skos:prefLabel xml:lang="sl">Zdravje in varnost prebivalstva</skos:prefLabel>
    <skos:scopeNote xml:lang="sl">Geografska razporeditev pogostih patoloških pojavov (alergije, rakasta obolenja, obolenja dihalnih poti itd.), podatki o učinkih na zdravje (biološki označevalci, zmanjšana rodnost, epidemije) ali počutje ljudi (utrujenost, stres itd.), povezanih neposredno (onesnaženost zraka, kemikalije, tanjšanje ozonskega plašča, hrup itd.) ali posredno (hrana, genetsko spremenjeni organizmi itd.) s kakovostjo okolja.</skos:scopeNote>
    <skos:prefLabel xml:lang="sv">Människors hälsa och säkerhet</skos:prefLabel>
    <skos:scopeNote xml:lang="sv">Geografisk fördelning av dominansen av patologier (allergier, cancer, sjukdomar i andningsorganen osv.), all information om de effekter på människors hälsa (biomarkörer, minskad fertilitet, epidemier osv.) eller välbefinnande (trötthet, stress osv.) som har ett direkt (luftföroreningar, kemikalier, uttunning av ozonskiktet, buller osv.) eller ett indirekt (livsmedel, genetiskt modifierade organismer osv.) samband med miljöns kvalitet.</skos:scopeNote>
    <skos:altLabel>hh</skos:altLabel>
    <skos:inScheme rdf:resource="http://inspire.ec.europa.eu/theme" />
  </skos:Concept>
  <skos:Concept xmlns:skos="http://www.w3.org/2004/02/skos/core#" rdf:about="http://inspire.ec.europa.eu/theme/lu">
    <skos:prefLabel xml:lang="en">Land use</skos:prefLabel>
    <skos:scopeNote xml:lang="en">Territory characterised according to its current and future planned functional dimension or socio-economic purpose (e.g. residential, industrial, commercial, agricultural, forestry, recreational).</skos:scopeNote>
    <skos:prefLabel xml:lang="bg">Ползване на земята</skos:prefLabel>
    <skos:scopeNote xml:lang="bg">Територия, определена според настоящите и бъдещите ѝ планирани функционални параметри или социалноикономическо предназначение (например жилищна, промишлена, търговска, селскостопанска, горска, почивна).</skos:scopeNote>
    <skos:prefLabel xml:lang="cs">Využití území</skos:prefLabel>
    <skos:scopeNote xml:lang="cs">Území popsané podle své současné a plánované funkce nebo společensko-hospodářských účelů (např. obytné, průmyslové, obchodní, zemědělské, lesnické, rekreační).</skos:scopeNote>
    <skos:prefLabel xml:lang="hr">Korištenje zemljišta</skos:prefLabel>
    <skos:scopeNote xml:lang="hr">Područje opisano u skladu s njegovom sadašnjom i budućom planiranom funkcionalnom veličinom ili u skladu s njegovom društveno-gospodarskom namjenom (npr. stambenom, industrijskom, poslovnom, poljoprivrednom, za šumarstvo i sportsko-rekreacijskom).</skos:scopeNote>
    <skos:prefLabel xml:lang="da">Arealanvendelse</skos:prefLabel>
    <skos:scopeNote xml:lang="da">Området karakteriseret ved dets nuværende og fremtidige planlagte funktion eller samfundsøkonomiske formål (f.eks. beboelse, industri, handel, landbrug, skovbrug, rekreation).</skos:scopeNote>
    <skos:prefLabel xml:lang="de">Bodennutzung</skos:prefLabel>
    <skos:scopeNote xml:lang="de">Beschreibung von Gebieten anhand ihrer derzeitigen und geplanten künftigen Funktion oder ihres sozioökonomischen Zwecks (z. B. Wohn-, Industrie- oder Gewerbegebiete, land- oder forstwirtschaftliche Flächen, Freizeitgebiete).</skos:scopeNote>
    <skos:prefLabel xml:lang="el">Χρήσεις γης</skos:prefLabel>
    <skos:scopeNote xml:lang="el">Χαρακτηρισμός περιοχών ανάλογα με τη σημερινή και τη μελλοντική σχεδιαζόμενη λειτουργία τους ή τον κοινωνικοοικονομικό σκοπό τους (π.χ. αμιγώς οικιστική, βιομηχανική, εμπορική, γεωργική, δασική, αναψυχής).</skos:scopeNote>
    <skos:prefLabel xml:lang="es">Uso del suelo</skos:prefLabel>
    <skos:scopeNote xml:lang="es">Caracterización del territorio, de acuerdo con su dimensión funcional o su dedicación socioeconómica actual o futura planificadas (por ejemplo, residencial, industrial, comercial, agrario, forestal, recreativo).</skos:scopeNote>
    <skos:prefLabel xml:lang="et">Maakasutus</skos:prefLabel>
    <skos:scopeNote xml:lang="et">Maa-ala iseloomustus olemasolevate ja tulevaste kavandatud kasutusaspektide või sotsiaalmajandusliku sihtotstarbe järgi (nt elamu- tööstus-, äri-, põllumajandus-, metsa- või puhkemaa).</skos:scopeNote>
    <skos:prefLabel xml:lang="fi">Maankäyttö</skos:prefLabel>
    <skos:scopeNote xml:lang="fi">Alueen kuvaaminen sen nykyisen ja tulevan suunnitellun käyttötarkoituksen tai sosioekonomisen tarkoituksen (esimerkiksi asuin- tai teollisuusalue, liikekeskus, maa- tai metsätalousalue tai virkistysalue) mukaan.</skos:scopeNote>
    <skos:prefLabel xml:lang="fr">Usage des sols</skos:prefLabel>
    <skos:scopeNote xml:lang="fr">Territoire caractérisé selon sa dimension fonctionnelle prévue ou son objet socioéconomique actuel et futur (par exemple, résidentiel, industriel, commercial, agricole, forestier, récréatif).</skos:scopeNote>
    <skos:prefLabel xml:lang="hu">Földhasználat</skos:prefLabel>
    <skos:scopeNote xml:lang="hu">A jelenlegi és a jövőbeli tervezett funkcionális szempontok vagy a társadalmigazdasági rendeltetés (például lakó-, ipari, kereskedelmi, mezőgazdasági, erdő- vagy pihenőövezet) szerint jellemzett területek.</skos:scopeNote>
    <skos:prefLabel xml:lang="it">Utilizzo del territorio</skos:prefLabel>
    <skos:scopeNote xml:lang="it">Classificazione del territorio in base alla dimensione funzionale o alla destinazione socioeconomica presenti e programmate per il futuro (ad esempio ad uso residenziale, industriale, commerciale, agricolo, silvicolo, ricreativo).</skos:scopeNote>
    <skos:prefLabel xml:lang="lt">Žemės naudojimas</skos:prefLabel>
    <skos:scopeNote xml:lang="lt">Teritorija apibūdinama pagal jos esamą ir būsimą planuojamą funkcinę arba socialinę ir ekonominę paskirtį (pvz., gyvenamoji, pramoninė, komercinė, žemės ūkio, miškų, rekreacinė).</skos:scopeNote>
    <skos:prefLabel xml:lang="lv">Zemes izmantošana</skos:prefLabel>
    <skos:scopeNote xml:lang="lv">Teritorijas stāvoklis, ko raksturo tās pašreizējās un nākotnē plānotās funkcionālās izmantošanas dimensija vai sociāli ekonomiskais izmantošanas nolūks (piemēram, zeme dzīvojamiem namiem, rūpnieciskiem, komerciāliem, lauksaimniecības, mežniecības, atpūtas mērķiem).</skos:scopeNote>
    <skos:prefLabel xml:lang="mt">Użu ta' l-art</skos:prefLabel>
    <skos:scopeNote xml:lang="mt">Territorju kkaratterizzat skond id-dimensjoni funzjonali tiegħu ppjanata attwali u futura jew l-iskop soċjo-ekonomiku tiegħu (eż. residenzjali, industrijali, kummerċjali, agrikolu, forestali, rikreazzjonali).</skos:scopeNote>
    <skos:prefLabel xml:lang="nl">Landgebruik</skos:prefLabel>
    <skos:scopeNote xml:lang="nl">Het grondgebied, gekenmerkt volgens zijn huidige en geplande toekomstige functionele dimensie of sociaaleconomische bestemming (bv. wonen, industrieel, commercieel, landbouw, bosbouw, recreatie).</skos:scopeNote>
    <skos:prefLabel xml:lang="pl">Zagospodarowanie przestrzenne</skos:prefLabel>
    <skos:scopeNote xml:lang="pl">Terytorium charakteryzowane ze względu na jego obecny lub przyszły wymiar funkcjonalny lub przeznaczenie społeczno-gospodarcze (np. mieszkaniowe, przemysłowe, handlowe, rolnicze, leśne, wypoczynkowe).</skos:scopeNote>
    <skos:prefLabel xml:lang="pt">Uso do solo</skos:prefLabel>
    <skos:scopeNote xml:lang="pt">Caracterização do território de acordo com a dimensão funcional ou finalidade socioeconómica planeada, presente e futura (por exemplo, residencial, industrial, comercial, agrícola, silvícola, recreativa).</skos:scopeNote>
    <skos:prefLabel xml:lang="ro">Utilizarea terenului</skos:prefLabel>
    <skos:scopeNote xml:lang="ro">Teritoriu caracterizat în funcție de dimensiunea funcțională actuală sau viitoare planificată sau de scopul socio-economic (de exemplu rezidențial, industrial, comercial, agricol, forestier, de recreație).</skos:scopeNote>
    <skos:prefLabel xml:lang="sk">Využitie územia</skos:prefLabel>
    <skos:scopeNote xml:lang="sk">Územie charakterizované podľa jeho súčasného a budúceho plánovaného funkčného rozmeru alebo socio-ekonomického účelu (napr. obytný, priemyselný, obchodný, poľnohospodársky, lesnícky, rekreačný).</skos:scopeNote>
    <skos:prefLabel xml:lang="sl">Namenska raba tal</skos:prefLabel>
    <skos:scopeNote xml:lang="sl">Ozemlje, opredeljeno glede na svojo sedanjo in v prihodnje načrtovano funkcionalno razsežnost ali socialno-ekonomski namen (npr. stanovanjski, industrijski, trgovinski, kmetijski, gozdni, rekreacijski).</skos:scopeNote>
    <skos:prefLabel xml:lang="sv">Markanvändning</skos:prefLabel>
    <skos:scopeNote xml:lang="sv">Territorium indelat efter nuvarande och framtida planerade funktion eller socioekonomisk användning (t.ex. bostadsmark, industrimark, handel, jordbruk, skogsbruk, friluftsliv).</skos:scopeNote>
    <skos:altLabel>lu</skos:altLabel>
    <skos:inScheme rdf:resource="http://inspire.ec.europa.eu/theme" />
  </skos:Concept>
  <skos:Concept xmlns:skos="http://www.w3.org/2004/02/skos/core#" rdf:about="http://inspire.ec.europa.eu/theme/mr">
    <skos:prefLabel xml:lang="en">Mineral resources</skos:prefLabel>
    <skos:scopeNote xml:lang="en">Mineral resources including metal ores, industrial minerals, etc., where relevant including depth/height information on the extent of the resource.</skos:scopeNote>
    <skos:prefLabel xml:lang="bg">Минерални ресурси</skos:prefLabel>
    <skos:scopeNote xml:lang="bg">Минерални ресурси, включително метални руди, промишлени минерали и други; по целесъобразност се включва информация за дълбочина/височина на находището на ресурса.</skos:scopeNote>
    <skos:prefLabel xml:lang="cs">Nerostné suroviny</skos:prefLabel>
    <skos:scopeNote xml:lang="cs">Nerostné suroviny, včetně kovových rud, průmyslových surovin atd., případně včetně informací o hloubce nebo výšce týkajících se rozsahu zdroje.</skos:scopeNote>
    <skos:prefLabel xml:lang="hr">Izvori minerala</skos:prefLabel>
    <skos:scopeNote xml:lang="hr">Izvori minerala, uključujući kovinske rude, industrijske minerale itd., uključujući dubinske/visinske informacije o veličini izvora ako je potrebno.</skos:scopeNote>
    <skos:prefLabel xml:lang="da">Mineralressourcer</skos:prefLabel>
    <skos:scopeNote xml:lang="da">Mineralressourcer, herunder metalmalme, industrmineraler osv. samt, hvis det er relevant, dybde-/højdeoplysninger om ressourcens omfang.</skos:scopeNote>
    <skos:prefLabel xml:lang="de">Mineralische Bodenschätze</skos:prefLabel>
    <skos:scopeNote xml:lang="de">Mineralische Bodenschätze wie Metallerze, Industrieminerale usw., gegebenenfalls mit Tiefen- bzw. Höhenangaben zur Ausdehnung der Bodenschätze.</skos:scopeNote>
    <skos:prefLabel xml:lang="el">Ορυκτοί πόροι</skos:prefLabel>
    <skos:scopeNote xml:lang="el">Ορυκτοί πόροι, μεταξύ άλλων και μεταλλεύματα, βιομηχανικά μεταλλεύματα, κ.λπ., συμπεριλαμβανομένων, κατά περίπτωση, πληροφοριών περί του βάθους και του ύψους όσον αφορά την έκταση του εκάστοτε πόρου.</skos:scopeNote>
    <skos:prefLabel xml:lang="es">Recursos minerales</skos:prefLabel>
    <skos:scopeNote xml:lang="es">Recursos minerales: minerales metalíferos, minerales industriales, etc., incluyendo, cuando proceda, la información de profundidad y altura del volumen de los recursos.</skos:scopeNote>
    <skos:prefLabel xml:lang="et">Maavarad</skos:prefLabel>
    <skos:scopeNote xml:lang="et">Maavarad, sealhulgas metallimaagid, tööstuslikud mineraalid jne, sealhulgas koos asjakohase sügavust/kõrgust puudutava teabega ressursi mahu kohta.</skos:scopeNote>
    <skos:prefLabel xml:lang="fi">Mineraalivarat</skos:prefLabel>
    <skos:scopeNote xml:lang="fi">Mineraalivarat, mukaan lukien metallimalmit, teollisuusmineraalit jne., mukaan luettuina tarvittaessa syvyys-/korkeustiedot kyseisen luonnonvaran laajuudesta.</skos:scopeNote>
    <skos:prefLabel xml:lang="fr">Ressources minérales</skos:prefLabel>
    <skos:scopeNote xml:lang="fr">Ressources minérales comprenant les minerais métalliques, les minéraux industriels, etc., le cas échéant accompagnées d'informations relatives à la profondeur/la hauteur de la ressource.</skos:scopeNote>
    <skos:prefLabel xml:lang="hu">Ásványi nyersanyagok</skos:prefLabel>
    <skos:scopeNote xml:lang="hu">Ásványi nyersanyagok, beleértve a fémek érceit, ipari ásványokat stb., adott esetben beleértve a nyersanyag kiterjedésére vonatkozó mélységi/magassági információkat.</skos:scopeNote>
    <skos:prefLabel xml:lang="it">Risorse minerarie</skos:prefLabel>
    <skos:scopeNote xml:lang="it">Risorse minerarie, compresi i minerali metallici, i minerali industriali, ecc., ove opportuno anche informazioni, in termini di altezza/profondità, sull'entità della risorsa.</skos:scopeNote>
    <skos:prefLabel xml:lang="lt">Naudingosios iškasenos</skos:prefLabel>
    <skos:scopeNote xml:lang="lt">Naudingosios iškasenos, įskaitant metalų rūdas, pramonei naudojamas naudingąsias iškasenas ir t. t., tam tikrais atvejais įskaitant informaciją apie išteklių apimties gylį/aukštį.</skos:scopeNote>
    <skos:prefLabel xml:lang="lv">Derīgo izrakteņu resursi</skos:prefLabel>
    <skos:scopeNote xml:lang="lv">Derīgo izrakteņu resursi, tostarp metālu rūdas, rūpnieciski iegūstamie izrakteņi, utt., attiecīgā gadījumā ietverot informāciju par dziļumu/augstumu attiecībā uz resursu apmēru.</skos:scopeNote>
    <skos:prefLabel xml:lang="mt">Riżorsi minerali</skos:prefLabel>
    <skos:scopeNote xml:lang="mt">Riżorsi minerali inklużi minerali tal-metall, minerali industrijali, eċċ, fejn rilevanti inkluża informazzjoni dwar il-fond/l-għoli rigward id-daqs tar-riżors.</skos:scopeNote>
    <skos:prefLabel xml:lang="nl">Minerale bronnen</skos:prefLabel>
    <skos:scopeNote xml:lang="nl">Minerale bronnen met inbegrip van metaalertsen, industriële mineralen enz., waar passend met inbegrip van diepte/hoogte-informatie over de omvang van de bron.</skos:scopeNote>
    <skos:prefLabel xml:lang="pl">Zasoby mineralne</skos:prefLabel>
    <skos:scopeNote xml:lang="pl">Zasoby mineralne, w tym rudy metali, minerały przemysłowe itd., w odpowiednich przypadkach łącznie z informacjami dotyczącymi głębokości/wysokości i rozmiarów danych zasobów.</skos:scopeNote>
    <skos:prefLabel xml:lang="pt">Recursos minerais</skos:prefLabel>
    <skos:scopeNote xml:lang="pt">Recursos minerais, incluindo minérios metálicos, minerais industriais, etc., incluindo, quando pertinente, informação sobre as cotas de profundidade/altura do recurso.</skos:scopeNote>
    <skos:prefLabel xml:lang="ro">Resurse minerale</skos:prefLabel>
    <skos:scopeNote xml:lang="ro">Resurse minerale precum minereurile metalifere, minereurile industriale etc., însoțite de informații privind adâncimea/înălțimea la care se află resursa, după caz.</skos:scopeNote>
    <skos:prefLabel xml:lang="sk">Zdroje nerastných surovín</skos:prefLabel>
    <skos:scopeNote xml:lang="sk">Zdroje nerastných surovín vrátane kovových rúd, priemyselných nerastov atď., ak je to možné vrátane informácie o šírke a dĺžke rozlohy zdroja.</skos:scopeNote>
    <skos:prefLabel xml:lang="sl">Mineralni viri</skos:prefLabel>
    <skos:scopeNote xml:lang="sl">Mineralni viri, vključno s kovinskimi rudami, industrijskimi mineralnimi surovinami itd. kjer je ustrezno, vključno s podatki o globini/višini glede velikosti vira.</skos:scopeNote>
    <skos:prefLabel xml:lang="sv">Mineralfyndigheter</skos:prefLabel>
    <skos:scopeNote xml:lang="sv">Mineralfyndigheter, bland annat malm, industrimineraler osv., i tillämpliga fall med djup-/höjdinformation om resursens omfattning.</skos:scopeNote>
    <skos:altLabel>mr</skos:altLabel>
    <skos:inScheme rdf:resource="http://inspire.ec.europa.eu/theme" />
  </skos:Concept>
  <skos:Concept xmlns:skos="http://www.w3.org/2004/02/skos/core#" rdf:about="http://inspire.ec.europa.eu/theme/nz">
    <skos:prefLabel xml:lang="en">Natural risk zones</skos:prefLabel>
    <skos:scopeNote xml:lang="en">Vulnerable areas characterised according to natural hazards (all atmospheric, hydrologic, seismic, volcanic and wildfire phenomena that, because of their location, severity, and frequency, have the potential to seriously affect society), e.g. floods, landslides and subsidence, avalanches, forest fires, earthquakes, volcanic eruptions.</skos:scopeNote>
    <skos:prefLabel xml:lang="bg">Природни рискови зони</skos:prefLabel>
    <skos:scopeNote xml:lang="bg">Уязвими райони, определени в зависимост от вида природен риск (всички атмосферни, хидрологични, сеизмични, вулканични и огнени явления, които поради местонахождението, силата и честотата на проявление могат да засегнат сериозно обществото), например наводнения, свличане и пропадане на земни маси, лавини, горски пожари, земетресения, изригвания на вулкани.</skos:scopeNote>
    <skos:prefLabel xml:lang="cs">Oblasti ohrožené přírodními riziky</skos:prefLabel>
    <skos:scopeNote xml:lang="cs">Zranitelné oblasti označené podle přírodního nebezpečí (všechny povětrnostní, hydrologické, seismické a sopečné úkazy, jakož i ničivé požáry, které mohou mít vzhledem ke svému výskytu, závažnosti a četnosti vážný dopad na společnost), např. povodně, sesuvy a sesedání půdy, laviny, lesní požáry, zemětřesení, sopečné výbuchy.</skos:scopeNote>
    <skos:prefLabel xml:lang="hr">Područja s prirodnim opasnostima</skos:prefLabel>
    <skos:scopeNote xml:lang="hr">Osjetljiva područja koja su obilježena u skladu s prirodnim opasnostima (svim atmosferskim, hidrološkim, seizmološkim, vulkanskim pojavama i požarima, koji zbog svojeg položaja, težine i učestalosti imaju potencijal da ozbiljno utječu na društvo), npr. poplave, odroni zemlje i slijeganje tla, snježne lavine, šumski požari, potresi, vulkanske erupcije.</skos:scopeNote>
    <skos:prefLabel xml:lang="da">Områder med naturlige risici</skos:prefLabel>
    <skos:scopeNote xml:lang="da">Sårbare områder, karakteriseret efter naturlige risici (alle atmosfæriske, hydrologiske, seismiske og vulkanske fænomener samt brande, som på grund af stedet, hvor de forekommer, deres omfang og hyppighed kan få alvorlige følger for samfundet), f.eks. oversvømmelser, jordskred og sammensynkning, laviner, skovbrande, jordskælv og vulkanudbrud.</skos:scopeNote>
    <skos:prefLabel xml:lang="de">Gebiete mit naturbedingten Risiken</skos:prefLabel>
    <skos:scopeNote xml:lang="de">Gefährdete Gebiete, eingestuft nach naturbedingten Risiken (sämtliche atmosphärischen, hydrologischen, seismischen, vulkanischen Phänomene sowie Naturfeuer, die aufgrund ihres örtlichen Auftretens sowie ihrer Schwere und Häufigkeit signifikante Auswirkungen auf die Gesellschaft haben können), z. B. Überschwemmungen, Erdrutsche und Bodensenkungen, Lawinen, Waldbrände, Erdbeben oder Vulkanausbrüche.</skos:scopeNote>
    <skos:prefLabel xml:lang="el">Ζώνες φυσικών κινδύνων</skos:prefLabel>
    <skos:scopeNote xml:lang="el">Χαρακτηρισμός ευάλωτων περιοχών ανάλογα με τους φυσικούς κινδύνους (όλα τα ατμοσφαιρικά, υδρολογικά, σεισμικά, ηφαιστειακά φαινόμενα και τα φαινόμενα καταστροφικών πυρκαγιών που, λόγω της θέσης, της σφοδρότητας και της συχνότητάς τους, είναι δυνατό να έχουν σοβαρές επιπτώσεις στην κοινωνία), π.χ. πλημμύρες, κατολισθήσεις και καθιζήσεις, χιονοστιβάδες, δασικές πυρκαγιές, σεισμοί, εκρήξεις ηφαιστείων.</skos:scopeNote>
    <skos:prefLabel xml:lang="es">Zonas de riesgos naturales</skos:prefLabel>
    <skos:scopeNote xml:lang="es">Zonas vulnerables caracterizadas por la existencia de riesgos de carácter natural (cualquier fenómeno atmosférico, hidrológico, sísmico, volcánico o incendio natural que, debido a su localización, gravedad o frecuencia, pueda afectar negativamente a la población), p. ej., inundaciones, corrimientos de tierra y hundimientos, aludes, incendios forestales, terremotos, erupciones volcánicas.</skos:scopeNote>
    <skos:prefLabel xml:lang="et">Looduslikud ohutsoonid</skos:prefLabel>
    <skos:scopeNote xml:lang="et">Tundlikud alad, mida iseloomustavad looduslikud riskitegurid (kõik atmosfäärilised, hüdroloogilised, seismilised, vulkaanilised ja looduspõlengute nähtused, mis oma asukoha, intensiivsuse ja sageduse tõttu võivad ühiskonnale tõsist kahju tuua), nt üleujutused, maalihked ja pinnase vajumine, laviinid, metsatulekahjud, maavärinad, vulkaanipursked.</skos:scopeNote>
    <skos:prefLabel xml:lang="fi">Luonnonriskialueet</skos:prefLabel>
    <skos:scopeNote xml:lang="fi">Luonnonkatastrofien (kaikki ilmakehästä johtuvat, hydrologiset, seismiset, tuliperäiset ja maastopaloilmiöt, joilla sijaintinsa, vakavuutensa ja yleisyytensä vuoksi voi mahdollisesti olla vakavia vaikutuksia yhteiskuntaan), kuten tulvien, maanvyöryjen ja vajoamisen, lumivyöryjen, metsäpalojen, maanjäristysten ja tulivuortenpurkausten, mukaan luokitellut riskialueet.</skos:scopeNote>
    <skos:prefLabel xml:lang="fr">Zones à risque naturel</skos:prefLabel>
    <skos:scopeNote xml:lang="fr">Zones sensibles caractérisées en fonction des risques naturels (tous les phénomènes atmosphériques, hydrologiques, sismiques, volcaniques, ainsi que les feux de friche qui peuvent, en raison de leur situation, de leur gravité et de leur fréquence, nuire gravement à la société), tels qu'inondations, glissements et affaissements de terrain, avalanches, incendies de forêts, tremblements de terre et éruptions volcaniques.</skos:scopeNote>
    <skos:prefLabel xml:lang="hu">Természeti kockázati zónák</skos:prefLabel>
    <skos:scopeNote xml:lang="hu">Természeti veszélyek, így pl. árvizek, földcsuszamlások, felszínsüllyedések, lavinák, erdőtüzek, földrengések, vulkánkitörések (minden légköri, hidrológiai, szeizmikus, vulkanikus és futótűzjelenség, amely – helye, súlyossága és előfordulási gyakorisága alapján – magában hordozza a komoly társadalmi károk okozásának lehetőségét) alapján jellemzett veszélyeztetett területek.</skos:scopeNote>
    <skos:prefLabel xml:lang="it">Zone a rischio naturale</skos:prefLabel>
    <skos:scopeNote xml:lang="it">Zone sensibili caratterizzate in base ai rischi naturali (cioè tutti i fenomeni atmosferici, idrologici, sismici, vulcanici e gli incendi che, per l’ubicazione, la gravità e la frequenza, possono avere un grave impatto sulla società), ad esempio inondazioni, slavine e subsidenze, valanghe, incendi di boschi/foreste, terremoti, eruzioni vulcaniche.</skos:scopeNote>
    <skos:prefLabel xml:lang="lt">Gamtinių pavojų zonos</skos:prefLabel>
    <skos:scopeNote xml:lang="lt">Pažeidžiamos vietovės, suskirstytos pagal gamtinio pavojaus pobūdį (visi atmosferiniai, hidrologiniai, seisminiai, vulkaniniai ir savaiminių gaisrų reiškiniai, kurie dėl savo vietos, stiprumo ir dažnumo kelia didelę grėsmę visuomenei), pvz., potvyniai, nuošliaužos ir žemės nusėdimas, griūtys, miškų gaisrai, žemės drebėjimai, ugnikalnių išsiveržimai.</skos:scopeNote>
    <skos:prefLabel xml:lang="lv">Dabas apdraudējuma zonas</skos:prefLabel>
    <skos:scopeNote xml:lang="lv">Apgabali, kam raksturīgi dabas apdraudējumi (visas atmosfēriskās, hidroloģiskās, seismiskās, vulkāniskās parādības un dabiskie ugunsgrēki, kas sakarā ar atrašanās vietu, apjomu vai biežumu var nopietni skart sabiedrību), piemēram, plūdi, zemes nogruvumi un iegrimšana, lavīnas, mežu ugunsgrēki, zemestrīces un vulkānu izvirdumi.</skos:scopeNote>
    <skos:prefLabel xml:lang="mt">Żoni ta' riskju naturali</skos:prefLabel>
    <skos:scopeNote xml:lang="mt">Żoni vulnerabbli kkaratterizzati skond perikli naturali (kull fenomenu atmosferiku, idroloġiku, sismiku, vulkaniku u tan-nirien mifruxa li, minħabba fejn jinsabu, il-qawwa, u l-frekwenza tagħhom, għandhom il-potenzjal li jaffettwaw b'mod gravi s-soċjetà), eż. għargħar, żerżiq ta' l-art u ċediment ta' l-art, valangi, nirien fil-foresti, terremoti, eruzzjonijiet vulkaniċi.</skos:scopeNote>
    <skos:prefLabel xml:lang="nl">Gebieden met natuurrisico's</skos:prefLabel>
    <skos:scopeNote xml:lang="nl">Kwetsbare gebieden die worden gekenmerkt door natuurrisico's (alle atmosferische, hydrologische, seismische, vulkanische verschijnselen en ongecontroleerde branden die door hun locatie, hevigheid en frequentie, mogelijk ernstige maatschappelijke gevolgen kunnen hebben), zoals overstromingen, aardverschuivingen en -verzakkingen, lawines, bosbranden, aardbevingen en vulkaanuitbarstingen.</skos:scopeNote>
    <skos:prefLabel xml:lang="pl">Strefy zagrożenia naturalnego</skos:prefLabel>
    <skos:scopeNote xml:lang="pl">Obszary zagrożone charakteryzowane na podstawie zagrożeń naturalnych (wszystkie zjawiska atmosferyczne, hydrologiczne, sejsmiczne, wulkaniczne oraz pożary, które, ze względu na swoją lokalizację, dotkliwość i częstotliwość mogą wywierać poważny wpływ na społeczeństwo), np. powodzie, osunięcia ziemi i osiadanie gruntu, lawiny, pożary lasów, trzęsienia ziemi, wybuchy wulkanów.</skos:scopeNote>
    <skos:prefLabel xml:lang="pt">Zonas de risco natural</skos:prefLabel>
    <skos:scopeNote xml:lang="pt">Zonas sensíveis, caracterizadas de acordo com os riscos naturais (todos os fenómenos atmosféricos, hidrológicos, sísmicos, vulcânicos e os incêndios que, pela sua localização, gravidade e frequência, possam afectar gravemente a sociedade), como sejam inundações, deslizamentos de terras e subsidências, avalanches, incêndios florestais, sismos, erupções vulcânicas.</skos:scopeNote>
    <skos:prefLabel xml:lang="ro">Zone de risc natural</skos:prefLabel>
    <skos:scopeNote xml:lang="ro">Zone vulnerabile caracterizate în funcție de riscurile naturale (orice fenomen atmosferic, hidrologic, seismic, vulcanic, precum și incendiile, care, din cauza locației, a gravității și a frecvenței, pot afecta grav societatea), precum inundațiile, alunecările și surpările de teren, avalanșele, incendiile forestiere, cutremurele de pământ și erupțiile vulcanice.</skos:scopeNote>
    <skos:prefLabel xml:lang="sk">Zóny prírodného rizika</skos:prefLabel>
    <skos:scopeNote xml:lang="sk">Citlivé oblasti charakterizované podľa prírodných rizík (všetky atmosférické, hydrologické, seizmické, vulkanické javy a ničivé požiare, ktoré môžu mať s ohľadom na ich polohu, závažnosť a početnosť vážny vplyv na spoločnosť), napr. záplavy, zosuvy pôdy a pokles terénu, lavíny, lesné požiare, zemetrasenia, sopečné výbuchy.</skos:scopeNote>
    <skos:prefLabel xml:lang="sl">Območja nevarnosti naravnih nesreč</skos:prefLabel>
    <skos:scopeNote xml:lang="sl">Ranljiva območja, opredeljena glede na naravna tveganja (vsi atmosferski, hidrološki, seizmični, vulkanski pojavi in požari, ki zaradi svoje lokacije, resnosti in pogostosti lahko resno ogrozijo družbo), npr. poplave, zemeljski plazovi in pogrezanje tal, snežni plazovi, gozdni požari, potresi, vulkanski izbruhi.</skos:scopeNote>
    <skos:prefLabel xml:lang="sv">Naturliga riskområden</skos:prefLabel>
    <skos:scopeNote xml:lang="sv">Sårbara områden klassificerade efter naturliga risker (alla atmosfäriska, hydrologiska, seismiska och vulkaniska fenomen samt bränder som på grund av läge, omfattning och frekvens har potential att allvarligt påverka samhället), exempelvis översvämningar, jordskred och sättningar, laviner, skogsbränder, jordbävningar, vulkanutbrott.</skos:scopeNote>
    <skos:altLabel>nz</skos:altLabel>
    <skos:inScheme rdf:resource="http://inspire.ec.europa.eu/theme" />
  </skos:Concept>
  <skos:Concept xmlns:skos="http://www.w3.org/2004/02/skos/core#" rdf:about="http://inspire.ec.europa.eu/theme/of">
    <skos:prefLabel xml:lang="en">Oceanographic geographical features</skos:prefLabel>
    <skos:scopeNote xml:lang="en">Physical conditions of oceans (currents, salinity, wave heights, etc.).</skos:scopeNote>
    <skos:prefLabel xml:lang="bg">Океанографски географски характеристики</skos:prefLabel>
    <skos:scopeNote xml:lang="bg">Физическо състояние на океаните (течения, соленост, височина на вълните и други).</skos:scopeNote>
    <skos:prefLabel xml:lang="cs">Zeměpisné oceánografické prvky</skos:prefLabel>
    <skos:scopeNote xml:lang="cs">Fyzikální stav oceánů (proudy, slanost, výška vln atd.).</skos:scopeNote>
    <skos:prefLabel xml:lang="hr">Oceanografsko-geografske značajke</skos:prefLabel>
    <skos:scopeNote xml:lang="hr">Fizikalni uvjeti oceana (struje, slanost, visina valova itd.).</skos:scopeNote>
    <skos:prefLabel xml:lang="da">Oceanografiske/geografiske forhold</skos:prefLabel>
    <skos:scopeNote xml:lang="da">Fysiske forhold til havs (strømme, saltholdighed, bølgehøjde osv.)</skos:scopeNote>
    <skos:prefLabel xml:lang="de">Ozeanografisch-geografische Kennwerte</skos:prefLabel>
    <skos:scopeNote xml:lang="de">Physikalische Bedingungen der Ozeane (Strömungsverhältnisse, Salinität, Wellenhöhe usw.).</skos:scopeNote>
    <skos:prefLabel xml:lang="el">Ωκεανογραφικά γεωγραφικά χαρακτηριστικά</skos:prefLabel>
    <skos:scopeNote xml:lang="el">Φυσικές ιδιότητες των ωκεανών (ρεύματα, αλατότητα, ύψος κυμάτων, κ.λπ.).</skos:scopeNote>
    <skos:prefLabel xml:lang="es">Rasgos geográficos oceanográficos</skos:prefLabel>
    <skos:scopeNote xml:lang="es">Condiciones físicas de los océanos (corrientes, salinidad, altura del oleaje, etc.).</skos:scopeNote>
    <skos:prefLabel xml:lang="et">Okeanograafilis-geograafilised tunnusjooned</skos:prefLabel>
    <skos:scopeNote xml:lang="et">Füüsikalised tingimused ookeanides (hoovused, soolasisaldus, lainekõrgus jne).</skos:scopeNote>
    <skos:prefLabel xml:lang="fi">Merentutkimuksen maantieteelliset ominaispiirteet</skos:prefLabel>
    <skos:scopeNote xml:lang="fi">Merialueitten fysikaaliset olosuhteet (esimerkiksi virtaukset, suolapitoisuus ja aaltojen korkeus).</skos:scopeNote>
    <skos:prefLabel xml:lang="fr">Caractéristiques géographiques océanographiques</skos:prefLabel>
    <skos:scopeNote xml:lang="fr">Conditions physiques des océans (courants, salinité, hauteur des vagues, etc.).</skos:scopeNote>
    <skos:prefLabel xml:lang="hu">Oceanográfiai földrajzi jellemzők</skos:prefLabel>
    <skos:scopeNote xml:lang="hu">Az óceánok fizikai jellemzői (áramlatok, sótartalom, hullámmagasság stb.).</skos:scopeNote>
    <skos:prefLabel xml:lang="it">Elementi geografici oceanografici</skos:prefLabel>
    <skos:scopeNote xml:lang="it">Condizioni fisiche degli oceani (correnti, salinità, altezza delle onde, ecc.).</skos:scopeNote>
    <skos:prefLabel xml:lang="lt">Okeanografinės geografinės sąlygos</skos:prefLabel>
    <skos:scopeNote xml:lang="lt">Fizinės vandenynų charakteristikos (srovės, druskingumas, bangų aukštis ir t. t.).</skos:scopeNote>
    <skos:prefLabel xml:lang="lv">Okeanogrāfiski ģeogrāfiskie raksturlielumi</skos:prefLabel>
    <skos:scopeNote xml:lang="lv">Okeānu fizikālie apstākļi (straumes, sāļums, viļņu augstums, utt.).</skos:scopeNote>
    <skos:prefLabel xml:lang="mt">Karatteristiċi ġeografiċi oċeanografiċi</skos:prefLabel>
    <skos:scopeNote xml:lang="mt">Kondizzjonijiet fiżiċi ta' l-oċeani (kurrenti, imluħa, għoli tal-mewġ, eċċ.).</skos:scopeNote>
    <skos:prefLabel xml:lang="nl">Oceanografische geografische kenmerken</skos:prefLabel>
    <skos:scopeNote xml:lang="nl">Fysische kenmerken van oceanen (stroming, zoutgehalte, golfhoogte, enz.).</skos:scopeNote>
    <skos:prefLabel xml:lang="pl">Warunki oceanograficzno-geograficzne</skos:prefLabel>
    <skos:scopeNote xml:lang="pl">Warunki fizyczne oceanów (prądy, zasolenie, wysokość fal itd.).</skos:scopeNote>
    <skos:prefLabel xml:lang="pt">Características oceanográficas</skos:prefLabel>
    <skos:scopeNote xml:lang="pt">Condições físicas dos oceanos (correntes, salinidade, altura das ondas, etc.).</skos:scopeNote>
    <skos:prefLabel xml:lang="ro">Caracteristici geografice oceanografice</skos:prefLabel>
    <skos:scopeNote xml:lang="ro">Condiții fizice ale oceanelor (curenți, salinitate, înălțimea valurilor etc.).</skos:scopeNote>
    <skos:prefLabel xml:lang="sk">Oceánografické geografické prvky</skos:prefLabel>
    <skos:scopeNote xml:lang="sk">Fyzikálne vlastnosti oceánov (prúdy, slanosť, výška vĺn atď.).</skos:scopeNote>
    <skos:prefLabel xml:lang="sl">Oceanogeografske značilnosti</skos:prefLabel>
    <skos:scopeNote xml:lang="sl">Fizikalne razmere oceanov (tokovi, slanost, višina valov itd.).</skos:scopeNote>
    <skos:prefLabel xml:lang="sv">Geografiska oceanografiska förhållanden</skos:prefLabel>
    <skos:scopeNote xml:lang="sv">Fysikaliska förhållanden i oceanerna (strömmar, salthalt, våghöjd osv.).</skos:scopeNote>
    <skos:altLabel>of</skos:altLabel>
    <skos:inScheme rdf:resource="http://inspire.ec.europa.eu/theme" />
  </skos:Concept>
  <skos:Concept xmlns:skos="http://www.w3.org/2004/02/skos/core#" rdf:about="http://inspire.ec.europa.eu/theme/pd">
    <skos:prefLabel xml:lang="en">Population distribution — demography</skos:prefLabel>
    <skos:scopeNote xml:lang="en">Geographical distribution of people, including population characteristics and activity levels, aggregated by grid, region, administrative unit or other analytical unit.</skos:scopeNote>
    <skos:prefLabel xml:lang="bg">Разпределение на населението — демография</skos:prefLabel>
    <skos:scopeNote xml:lang="bg">Географско разпределение на населението, включително характеристики на населението и нива на дейност, представено обобщено по координати, регион, административна единица или друга аналитична единица.</skos:scopeNote>
    <skos:prefLabel xml:lang="cs">Rozložení obyvatelstva – demografie</skos:prefLabel>
    <skos:scopeNote xml:lang="cs">Zeměpisné rozložení osob, včetně charakteristik obyvatelstva a druhů činnosti, seskupených podle souřadnicové sítě, regionu, správní jednotky nebo jiné analytické jednotky.</skos:scopeNote>
    <skos:prefLabel xml:lang="hr">Raširenost stanovništva — demografija</skos:prefLabel>
    <skos:scopeNote xml:lang="hr">Geografska raširenost stanovništva, uključujući obilježja stanovništva i razine aktivnosti, razvrstana po mreži, regiji, administrativnoj jedinici ili drugoj analitičkoj jedinici.</skos:scopeNote>
    <skos:prefLabel xml:lang="da">Befolkningsfordeling — demografi</skos:prefLabel>
    <skos:scopeNote xml:lang="da">Den geografiske fordeling af befolkningen, herunder befolkningskarakteristika og aktivitetsniveauer, i kvadratnetceller, forvaltningsenheder eller andre analytiske enheder.</skos:scopeNote>
    <skos:prefLabel xml:lang="de">Verteilung der Bevölkerung — Demografie</skos:prefLabel>
    <skos:scopeNote xml:lang="de">Geografische Verteilung der Bevölkerung, einschließlich Bevölkerungsmerkmalen und Tätigkeitsebenen, zusammengefasst nach Gitter, Region, Verwaltungseinheit oder sonstigen analytischen Einheiten.</skos:scopeNote>
    <skos:prefLabel xml:lang="el">Κατανομή πληθυσμού — δημογραφία</skos:prefLabel>
    <skos:scopeNote xml:lang="el">Γεωγραφική κατανομή του πληθυσμού, συμπεριλαμβανομένων των χαρακτηριστικών του πληθυσμού και των επιπέδων δραστηριοτήτων, ανά κάνναβο, περιοχή, διοικητική ενότητα ή άλλη ενότητα ανάλυσης.</skos:scopeNote>
    <skos:prefLabel xml:lang="es">Distribución de la población — demografía</skos:prefLabel>
    <skos:scopeNote xml:lang="es">Distribución geográfica de la población referidas a una cuadrícula, región, unidad administrativa u otro tipo de unidad analítica, incluyendo las características de la población y sus niveles de actividad.</skos:scopeNote>
    <skos:prefLabel xml:lang="et">Elanikkonna jaotumine – demograafia</skos:prefLabel>
    <skos:scopeNote xml:lang="et">Elanike, sealhulgas rahvastiku näitajate ja tegevuste geograafiline jaotumine ruutvõrgu, piirkondade, haldusüksuste või muude analüütiliste üksuste alusel.</skos:scopeNote>
    <skos:prefLabel xml:lang="fi">Väestöjakauma – demografia</skos:prefLabel>
    <skos:scopeNote xml:lang="fi">Väestön maantieteellinen jakautuminen, mukaan lukien väestöä koskevat tunnusluvut ja taloudellisen toimeliaisuuden tasot, yhdisteltynä ruudukoittain, alueittain, hallintoyksiköittäin tai muiden analyyttisten yksiköitten mukaisesti jaoteltuna.</skos:scopeNote>
    <skos:prefLabel xml:lang="fr">Répartition de la population — démographie</skos:prefLabel>
    <skos:scopeNote xml:lang="fr">Répartition géographique des personnes, avec les caractéristiques de population et les niveaux d'activité, regroupées par grille, région, unité administrative ou autre unité analytique.</skos:scopeNote>
    <skos:prefLabel xml:lang="hu">A népesség eloszlása – demográfia</skos:prefLabel>
    <skos:scopeNote xml:lang="hu">A népesség földrajzi eloszlása – beleértve a népességi jellemzőket és a tevékenységi szinteket is – térképrács, régió, közigazgatási egység vagy más elemzési egység alapján összesítve.</skos:scopeNote>
    <skos:prefLabel xml:lang="it">Distribuzione della popolazione — demografia</skos:prefLabel>
    <skos:scopeNote xml:lang="it">Distribuzione geografica della popolazione, comprese le relative caratteristiche ed i livelli di attività, aggregata per griglia, regione, unità amministrativa o altra unità analitica.</skos:scopeNote>
    <skos:prefLabel xml:lang="lt">Gyventojų pasiskirstymas – demografija</skos:prefLabel>
    <skos:scopeNote xml:lang="lt">Geografinis žmonių pasiskirstymas, įskaitant gyventojų savybes ir aktyvumo lygius, pagal tinklelį, regioną, administracinį ar kitą analitinį vienetą.</skos:scopeNote>
    <skos:prefLabel xml:lang="lv">Iedzīvotāju sadalījums – demogrāfija</skos:prefLabel>
    <skos:scopeNote xml:lang="lv">Iedzīvotāju ģeogrāfiskais sadalījums, tostarp iedzīvotāju raksturojumi un darbības līmeņi, grupējot pēc koordinātu tīkla, reģiona, administratīvām vai citām analītiskām vienībām.</skos:scopeNote>
    <skos:prefLabel xml:lang="mt">Distribuzzjoni tal-popolazzjoni – demografija</skos:prefLabel>
    <skos:scopeNote xml:lang="mt">Distribuzzjoni ġeografika ta' nies, inkluż karatteristiċi ta' popolazzjoni u livelli ta' attivitajiet, miġbura flimkien skond il-grilja, ir-reġjun, l-unità amministrattiva jew unità analitika oħra.</skos:scopeNote>
    <skos:prefLabel xml:lang="nl">Spreiding van de bevolking — demografie</skos:prefLabel>
    <skos:scopeNote xml:lang="nl">Geografische spreiding van de bevolking, met inbegrip van bevolkingskenmerken en activiteitsniveaus, verzameld per raster, regio, administratieve eenheid of andere analytische eenheid.</skos:scopeNote>
    <skos:prefLabel xml:lang="pl">Rozmieszczenie ludności – demografia</skos:prefLabel>
    <skos:scopeNote xml:lang="pl">Geograficzne rozmieszczenie ludności, łącznie z poziomami aktywności i charakterystyką ludności, pogrupowanej według siatki geograficznej, regionu, jednostki administracyjnej lub innej jednostki analitycznej.</skos:scopeNote>
    <skos:prefLabel xml:lang="pt">Distribuição da população — demografia</skos:prefLabel>
    <skos:scopeNote xml:lang="pt">Distribuição geográfica da população, incluindo características demográficas e níveis de actividade, agregada por quadrícula, região, unidade administrativa ou outra unidade analítica.</skos:scopeNote>
    <skos:prefLabel xml:lang="ro">Repartizarea populației – demografie</skos:prefLabel>
    <skos:scopeNote xml:lang="ro">Repartizare geografică a populației, inclusiv caracteristicile populației și nivelurile de activitate, regrupate pe grilă, regiune, unitate administrativă sau altă unitate analitică.</skos:scopeNote>
    <skos:prefLabel xml:lang="sk">Rozmiestnenie obyvateľstva – demografia</skos:prefLabel>
    <skos:scopeNote xml:lang="sk">Geografické rozmiestnenie obyvateľstva vrátane charakteristík obyvateľstva a úrovní činností zoskupené podľa siete, regiónu, administratívnej jednotky alebo inej analytickej jednotky.</skos:scopeNote>
    <skos:prefLabel xml:lang="sl">Porazdelitev prebivalstva – demografski podatki</skos:prefLabel>
    <skos:scopeNote xml:lang="sl">Geografska porazdelitev ljudi, vključno z značilnostmi populacije in ravnmi aktivnosti, razvrščenih po koordinatah, regiji, upravni enoti ali drugi analitični enoti.</skos:scopeNote>
    <skos:prefLabel xml:lang="sv">Befolkningsfördelning – demografi</skos:prefLabel>
    <skos:scopeNote xml:lang="sv">Geografisk fördelning av människor, inbegripet befolkningskarakteristiska och sysselsättningsgrader, i rutnät, regioner, administrativa enheter eller andra analysenheter.</skos:scopeNote>
    <skos:altLabel>pd</skos:altLabel>
    <skos:inScheme rdf:resource="http://inspire.ec.europa.eu/theme" />
  </skos:Concept>
  <skos:Concept xmlns:skos="http://www.w3.org/2004/02/skos/core#" rdf:about="http://inspire.ec.europa.eu/theme/pf">
    <skos:prefLabel xml:lang="en">Production and industrial facilities</skos:prefLabel>
    <skos:scopeNote xml:lang="en">Industrial production sites, including installations covered by Council Directive 96/61/EC of 24 September 1996 concerning integrated pollution prevention and control (1) and water abstraction facilities, mining, storage sites.</skos:scopeNote>
    <skos:prefLabel xml:lang="bg">Производствени и промишлени съоръжения</skos:prefLabel>
    <skos:scopeNote xml:lang="bg">Промишлени обекти, включително инсталации, обхванати от Директива 96/61/ЕО на Съвета от 24 септември 1996 г. за комплексно предотвратяване и контрол на замърсяването (1), и съоръжения за водочерпене, минни съоръжения, складови обекти.</skos:scopeNote>
    <skos:prefLabel xml:lang="cs">Výrobní a průmyslová zařízení</skos:prefLabel>
    <skos:scopeNote xml:lang="cs">Místa s průmyslovou výrobou, včetně zařízení, na která se vztahuje směrnice Rady 96/61/ES ze dne 24. září 1996 o integrované prevenci a omezování znečištění (1), a zařízení na jímání vody, těžbu, skladiště a úložiště.</skos:scopeNote>
    <skos:prefLabel xml:lang="hr">Sustavi za proizvodnju i industriju</skos:prefLabel>
    <skos:scopeNote xml:lang="hr">Područja industrijske proizvodnje, uključujući i objekte koji su obuhvaćeni Direktivom Vijeća 96/61/EZ od 24. rujna 1996. o integriranom sprečavanju i kontroli onečišćenja (1), te postrojenja za izvlačenje vode, rudnici i skladišta.</skos:scopeNote>
    <skos:prefLabel xml:lang="da">Produktions- og industrifaciliteter</skos:prefLabel>
    <skos:scopeNote xml:lang="da">Industrielle produktionsanlæg, herunder de anlæg, der er omfattet af Rådets direktiv 96/61/EF af 24. september 1996 om forebyggelse og bekæmpelse af forurening [1], og vandudvindingsanlæg, miner, oplagspladser.</skos:scopeNote>
    <skos:prefLabel xml:lang="de">Produktions- und Industrieanlagen</skos:prefLabel>
    <skos:scopeNote xml:lang="de">Standorte für industrielle Produktion, einschließlich durch die Richtlinie 96/61/EG des Rates vom 24. September 1996 über die integrierte Vermeidung und Verminderung der Umweltverschmutzung [1] erfasste Anlagen und Einrichtungen zur Wasserentnahme sowie Bergbau- und Lagerstandorte.</skos:scopeNote>
    <skos:prefLabel xml:lang="el">Εγκαταστάσεις παραγωγής και βιομηχανικές εγκαταστάσεις</skos:prefLabel>
    <skos:scopeNote xml:lang="el">Τοποθεσίες βιομηχανικής παραγωγής, συμπεριλαμβανομένων των εγκαταστάσεων που καλύπτονται από την οδηγία 96/61/ΕΚ του Συμβουλίου, της 24ης Σεπτεμβρίου 1996, σχετικά με την ολοκληρωμένη πρόληψη και έλεγχο της ρύπανσης [1], και εγκαταστάσεις υδροληψίας, εξόρυξης, χώροι αποθήκευσης.</skos:scopeNote>
    <skos:prefLabel xml:lang="es">Instalaciones de producción e industriales</skos:prefLabel>
    <skos:scopeNote xml:lang="es">Centros de producción industrial, incluidas las instalaciones contempladas en la Directiva 96/61/CE del Consejo, de 24 de septiembre de 1996, sobre la prevención y el control integrado de la contaminación [1], e instalaciones de extracción de agua, instalaciones mineras, centros de almacenamiento.</skos:scopeNote>
    <skos:prefLabel xml:lang="et">Tootmis- ja tööstusrajatised</skos:prefLabel>
    <skos:scopeNote xml:lang="et">Tööstusliku tootmise asukohad, sealhulgas nõukogu 24. septembri 1996. aasta direktiiviga 96/61/EÜ saastuse kompleksse vältimise ja kontrolli kohta (1) hõlmatud rajatised ning veevõtukohad, kaevandused ja ladustamiskohad.</skos:scopeNote>
    <skos:prefLabel xml:lang="fi">Tuotanto- ja teollisuuslaitokset</skos:prefLabel>
    <skos:scopeNote xml:lang="fi">Teollisuusalueet, mukaan luettuina ympäristön pilaantumisen ehkäisemisen ja vähentämisen yhtenäistämiseksi 24 päivänä syyskuuta 1996 annetun neuvoston direktiivin 96/61/EY [1] soveltamisalaan kuuluvat laitokset sekä vedenottamot, kaivokset ja varastoalueet.</skos:scopeNote>
    <skos:prefLabel xml:lang="fr">Lieux de production et sites industriels</skos:prefLabel>
    <skos:scopeNote xml:lang="fr">Sites de production industrielle, y compris les installations couvertes par la directive 96/61/CE du Conseil du 24 septembre 1996 relative à la prévention et à la réduction intégrées de la pollution [1] et les installations de captage d'eau, d'extraction minière et de stockage.</skos:scopeNote>
    <skos:prefLabel xml:lang="hu">Termelő és ipari létesítmények</skos:prefLabel>
    <skos:scopeNote xml:lang="hu">Ipari termelőhelyek, beleértve a környezetszennyezés integrált megelőzéséről és csökkentéséről szóló, 1996. szeptember 24-i 96/61/EK tanácsi irányelv [1] által szabályozott berendezéseket, valamint a vízkivételt, a bányászati és a tárolólétesítményeket.</skos:scopeNote>
    <skos:prefLabel xml:lang="it">Produzione e impianti industriali</skos:prefLabel>
    <skos:scopeNote xml:lang="it">Siti di produzione industriale; compresi gli impianti di cui alla direttiva 96/61/CE del Consiglio, del 24 settembre 1996, sulla prevenzione e la riduzione integrate dell'inquinamento [1] e gli impianti di estrazione dell’acqua, le attività estrattive e i siti di stoccaggio.</skos:scopeNote>
    <skos:prefLabel xml:lang="lt">Gamybos ir pramonės įrenginiai</skos:prefLabel>
    <skos:scopeNote xml:lang="lt">Pramoninės gamybos įmonės, įskaitant įrenginius, kuriems taikoma 1996 m. rugsėjo 24 d. Tarybos direktyva 96/61/EB dėl taršos integruotos prevencijos ir kontrolės [1], ir vandens ėmimo įmones, kasybos, sandėliavimo vietas.</skos:scopeNote>
    <skos:prefLabel xml:lang="lv">Ražošanas un rūpniecības iekārtas</skos:prefLabel>
    <skos:scopeNote xml:lang="lv">Rūpniecības ražošanas novietnes, tostarp iekārtas, kas iekļautas Padomes Direktīvā 96/61/EK ( 1996. gada 24. septembris) par piesārņojuma integrētu novēršanu un kontroli [1], un iekārtas, ko izmanto ūdens ņemšanai, kalnrūpniecībā vai uzglabāšanai.</skos:scopeNote>
    <skos:prefLabel xml:lang="mt">Faċilitajiet ta' produzzjoni u industrijali</skos:prefLabel>
    <skos:scopeNote xml:lang="mt">Siti ta' produzzjoni industrijali, inklużi installazzjonijiet koperti mid-Direttiva tal-Kunsill 96/61/KE ta' l- 24 ta' Settembru 1996 dwar il-prevenzjoni u l-kontroll integrat tat-tniġġis [1] u faċilitajiet ta' astrazzjoni ta' l-ilma, tħaffir ta' minjieri, siti ta' ħażna.</skos:scopeNote>
    <skos:prefLabel xml:lang="nl">Faciliteiten voor productie en industrie</skos:prefLabel>
    <skos:scopeNote xml:lang="nl">Industriële productievestigingen, met inbegrip van installaties die onder Richtlijn 96/61/EG van de Raad van 24 september 1996 inzake geïntegreerde preventie en bestrijding van verontreiniging [1] vallen en waterontrekkingsfaciliteiten, mijnbouw, opslagplaatsen.</skos:scopeNote>
    <skos:prefLabel xml:lang="pl">Obiekty produkcyjne i przemysłowe</skos:prefLabel>
    <skos:scopeNote xml:lang="pl">Zakłady przemysłowe, w tym obiekty objęte dyrektywą 96/61/WE z dnia 24 września 1996 r. dotycząca zintegrowanego zapobiegania zanieczyszczeniom i ich kontroli [1] oraz urządzenia poboru wody, miejsca wydobycia i składowiska.</skos:scopeNote>
    <skos:prefLabel xml:lang="pt">Instalações industriais e de produção</skos:prefLabel>
    <skos:scopeNote xml:lang="pt">Locais de produção industrial, incluindo instalações abrangidas pela Directiva 96/61/CE do Conselho, de 24 de Setembro de 1996, relativa à prevenção e controlo integrados da poluição [1], e instalações de captação de água, minas, locais de armazenagem.</skos:scopeNote>
    <skos:prefLabel xml:lang="ro">Instalații de producție și industriale</skos:prefLabel>
    <skos:scopeNote xml:lang="ro">Parcuri de producție industrială, inclusiv instalațiile reglementate de Directiva 96/61/CE a Consiliului din 24 septembrie 1996 privind prevenirea și controlul integrat al poluării (16), precum și instalațiile de captare a apei, de extracție minieră și locurile de depozitare.</skos:scopeNote>
    <skos:prefLabel xml:lang="sk">Výrobné a priemyselné zariadenia</skos:prefLabel>
    <skos:scopeNote xml:lang="sk">Priemyselné výrobné podniky vrátane zariadení, na ktoré sa vzťahuje smernica Rady 96/61/ES z 24. septembra 1996 o integrovanej prevencii a kontrole znečisťovania životného prostredia [1], a zariadenia na čerpanie vody, bane, sklady.</skos:scopeNote>
    <skos:prefLabel xml:lang="sl">Proizvodni in industrijski objekti in naprave</skos:prefLabel>
    <skos:scopeNote xml:lang="sl">Območja za industrijsko proizvodnjo, vključno z obrati, ki jih zajema Direktiva Sveta 96/61/ES z dne 24. septembra 1996 o celovitem preprečevanju in nadzorovanju onesnaževanja [1] ter objekti in napravami za odvzem vode, rudniki, skladišči.</skos:scopeNote>
    <skos:prefLabel xml:lang="sv">Produktions- och industrianläggningar</skos:prefLabel>
    <skos:scopeNote xml:lang="sv">Industriella produktionsställen, inbegripet anläggningar som omfattas av rådets direktiv 96/61/EG av den 24 september 1996 om samordnande åtgärder för att förebygga och begränsa föroreningar [1] samt vattenverk, gruvor och upplagsplatser.</skos:scopeNote>
    <skos:altLabel>pf</skos:altLabel>
    <skos:inScheme rdf:resource="http://inspire.ec.europa.eu/theme" />
  </skos:Concept>
  <skos:Concept xmlns:skos="http://www.w3.org/2004/02/skos/core#" rdf:about="http://inspire.ec.europa.eu/theme/sr">
    <skos:prefLabel xml:lang="en">Sea regions</skos:prefLabel>
    <skos:scopeNote xml:lang="en">Physical conditions of seas and saline water bodies divided into regions and sub-regions with common characteristics.</skos:scopeNote>
    <skos:prefLabel xml:lang="bg">Морски региони</skos:prefLabel>
    <skos:scopeNote xml:lang="bg">Физическо състояние на моретата и солени водни маси, разделени на региони и подрегиони с общи характеристики.</skos:scopeNote>
    <skos:prefLabel xml:lang="cs">Mořské oblasti</skos:prefLabel>
    <skos:scopeNote xml:lang="cs">Fyzikální stav moří a slaných vod rozdělených do regionů a subregionů se společnými vlastnostmi.</skos:scopeNote>
    <skos:prefLabel xml:lang="hr">Morske regije</skos:prefLabel>
    <skos:scopeNote xml:lang="hr">Fizikalni uvjeti mora i slanih vodenih tijela koja su podijeljena u regije i podregije sa zajedničkim osobinama.</skos:scopeNote>
    <skos:prefLabel xml:lang="da">Havområder</skos:prefLabel>
    <skos:scopeNote xml:lang="da">Fysiske forhold i have og saltholdige søer, opdelt på områder og delområder med fælles egenskaber.</skos:scopeNote>
    <skos:prefLabel xml:lang="de">Meeresregionen</skos:prefLabel>
    <skos:scopeNote xml:lang="de">Physikalische Bedingungen von Meeren und salzhaltigen Gewässern, aufgeteilt nach Regionen und Teilregionen mit gemeinsamen Merkmalen.</skos:scopeNote>
    <skos:prefLabel xml:lang="el">Θαλάσσιες περιοχές</skos:prefLabel>
    <skos:scopeNote xml:lang="el">Φυσικές ιδιότητες των θαλασσών και των αλατούχων υδατικών συστημάτων, με υποδιαίρεση ανά περιοχές και υποπεριοχές με κοινά χαρακτηριστικά.</skos:scopeNote>
    <skos:prefLabel xml:lang="es">Regiones marinas</skos:prefLabel>
    <skos:scopeNote xml:lang="es">Condiciones físicas de los mares y masas de aguas salinas, por regiones y subregiones con características comunes.</skos:scopeNote>
    <skos:prefLabel xml:lang="et">Merepiirkonnad</skos:prefLabel>
    <skos:scopeNote xml:lang="et">Füüsikalised tingimused meredes ja soolase veega veekogudes, mis on ühiste tunnuste alusel jaotatud piirkondadeks ja alampiirkondadeks.</skos:scopeNote>
    <skos:prefLabel xml:lang="fi">Merialueet</skos:prefLabel>
    <skos:scopeNote xml:lang="fi">Yhteisten ominaispiirteitten mukaisesti alueisiin ja osa-alueisiin jaoteltujen merien ja suolaisten vesistöjen fyysiset olosuhteet.</skos:scopeNote>
    <skos:prefLabel xml:lang="fr">Régions maritimes</skos:prefLabel>
    <skos:scopeNote xml:lang="fr">Conditions physiques des mers et des masses d'eau salée divisées en régions et en sous-régions à caractéristiques communes.</skos:scopeNote>
    <skos:prefLabel xml:lang="hu">Tengeri régiók</skos:prefLabel>
    <skos:scopeNote xml:lang="hu">A tengerek és sósvizű víztestek fizikai jellemzői, közös tulajdonságaik alapján régiókra és alrégiókra osztva.</skos:scopeNote>
    <skos:prefLabel xml:lang="it">Regioni marine</skos:prefLabel>
    <skos:scopeNote xml:lang="it">Condizioni fisiche dei mari e dei corpi idrici salmastri suddivisi in regioni e sottoregioni con caratteristiche comuni.</skos:scopeNote>
    <skos:prefLabel xml:lang="lt">Jūrų regionai</skos:prefLabel>
    <skos:scopeNote xml:lang="lt">Jūrų ir sūrių vandens telkinių, pagal bendras charakteristikas suskirstytų į regionus ir paregionius, fizinės charakteristikos.</skos:scopeNote>
    <skos:prefLabel xml:lang="lv">Jūru reģioni</skos:prefLabel>
    <skos:scopeNote xml:lang="lv">Pēc noteiktām kopīgām iezīmēm izveidotos apgabalos un apakšapgabalos sadalītu jūru un sālsūdens ūdenstilpņu fiziskie stāvokļi.</skos:scopeNote>
    <skos:prefLabel xml:lang="mt">Reġjuni tal-baħar</skos:prefLabel>
    <skos:scopeNote xml:lang="mt">Kondizzjonijiet fiżiċi ta' l-ibħra u korpi ta' ilma mielaħ imqassma f'reġjuni u sub-reġjuni b'karatteristiċi komuni.</skos:scopeNote>
    <skos:prefLabel xml:lang="nl">Zeegebieden</skos:prefLabel>
    <skos:scopeNote xml:lang="nl">Fysische kenmerken van zeeën en zoutwateroppervlakken, ingedeeld in regio's en subregio's met gemeenschappelijke kenmerken.</skos:scopeNote>
    <skos:prefLabel xml:lang="pl">Regiony morskie</skos:prefLabel>
    <skos:scopeNote xml:lang="pl">Warunki fizyczne mórz i akwenów słonowodnych w podziale na regiony i subregiony o wspólnych cechach.</skos:scopeNote>
    <skos:prefLabel xml:lang="pt">Regiões marinhas</skos:prefLabel>
    <skos:scopeNote xml:lang="pt">Condições físicas dos mares e massas de água salinas divididas em regiões e sub-regiões com características comuns.</skos:scopeNote>
    <skos:prefLabel xml:lang="ro">Regiuni maritime</skos:prefLabel>
    <skos:scopeNote xml:lang="ro">Condiții fizice ale mărilor și corpurilor de apă sărată divizate în regiuni și subregiuni cu caracteristici comune.</skos:scopeNote>
    <skos:prefLabel xml:lang="sk">Morské regióny</skos:prefLabel>
    <skos:scopeNote xml:lang="sk">Fyzikálne vlastnosti morí a útvarov slanej vody rozdelených na regióny a podregióny so spoločnými vlastnosťami.</skos:scopeNote>
    <skos:prefLabel xml:lang="sl">Morske regije</skos:prefLabel>
    <skos:scopeNote xml:lang="sl">Fizikalne razmere morij in slanih vodnih teles, razdeljenih v regije in podregije s skupnimi značilnostmi.</skos:scopeNote>
    <skos:prefLabel xml:lang="sv">Havsområden</skos:prefLabel>
    <skos:scopeNote xml:lang="sv">Fysikaliska förhållanden i hav och saltsjöar indelade i områden och delområden med likartade egenskaper.</skos:scopeNote>
    <skos:altLabel>sr</skos:altLabel>
    <skos:inScheme rdf:resource="http://inspire.ec.europa.eu/theme" />
  </skos:Concept>
  <skos:Concept xmlns:skos="http://www.w3.org/2004/02/skos/core#" rdf:about="http://inspire.ec.europa.eu/theme/so">
    <skos:prefLabel xml:lang="en">Soil</skos:prefLabel>
    <skos:scopeNote xml:lang="en">Soils and subsoil characterised according to depth, texture, structure and content of particles and organic material, stoniness, erosion, where appropriate mean slope and anticipated water storage capacity.</skos:scopeNote>
    <skos:prefLabel xml:lang="bg">Почва</skos:prefLabel>
    <skos:scopeNote xml:lang="bg">Почви и подпочви, определени според дълбочина, строеж, структура, механичен състав и съдържание на органични материали, каменливост, ерозия и, по целесъобразност, среден наклон и предполагаема водопопиваемост.</skos:scopeNote>
    <skos:prefLabel xml:lang="cs">Půda</skos:prefLabel>
    <skos:scopeNote xml:lang="cs">Půda a její podloží popsané podle hloubky, zrnitosti, struktury a obsahu částic a organického materiálu, podílu skeletu, erozí, případně průměrného sklonu svahu a očekávané kapacity jímavosti vody.</skos:scopeNote>
    <skos:prefLabel xml:lang="hr">Tlo</skos:prefLabel>
    <skos:scopeNote xml:lang="hr">Tla i slojevi zemlje ispod površine, opisani prema debljini, teksturi, strukturi i sadržaju čestica i organske tvari, kamenitosti, eroziji, ako je primjereno prema postotku nagiba i prema predviđenom opsegu zaliha vode.</skos:scopeNote>
    <skos:prefLabel xml:lang="da">Jord</skos:prefLabel>
    <skos:scopeNote xml:lang="da">Jordbund og underjord karakteriseret efter dybde, tekstur, struktur og indhold af partikler og organisk materiale, stenindhold, erosion, i givet fald gennemsnitlig hældning og forventet vandlagringskapacitet.</skos:scopeNote>
    <skos:prefLabel xml:lang="de">Boden</skos:prefLabel>
    <skos:scopeNote xml:lang="de">Beschreibung von Boden und Unterboden anhand von Tiefe, Textur, Struktur und Gehalt an Teilchen sowie organischem Material, Steinigkeit, Erosion, gegebenenfalls durchschnittliches Gefälle und erwartete Wasserspeicherkapazität.</skos:scopeNote>
    <skos:prefLabel xml:lang="el">Έδαφος</skos:prefLabel>
    <skos:scopeNote xml:lang="el">Χαρακτηρισμός εδάφους και υπεδάφους ανάλογα με το βάθος, την υφή, τη δομή και την περιεκτικότητα σε σωματίδια και οργανικά υλικά, το πετρώδες, τη διάβρωση και, κατά περίπτωση, τη μέση κλίση και την προβλεπόμενη χωρητικότητα αποθήκευσης νερού.</skos:scopeNote>
    <skos:prefLabel xml:lang="es">Suelo</skos:prefLabel>
    <skos:scopeNote xml:lang="es">Suelo y subsuelo, caracterizados según su profundidad, textura, estructura y contenido de partículas y material orgánico, pedregosidad, erosión y, cuando proceda, pendiente media y capacidad estimada de almacenamiento de agua.</skos:scopeNote>
    <skos:prefLabel xml:lang="et">Pinnas</skos:prefLabel>
    <skos:scopeNote xml:lang="et">Pinnas ja aluspinnas, mida iseloomustatakse sügavuse, tekstuuri, struktuuri, osakeste ja orgaanilise materjali sisalduse, kivimisisalduse, erosiooni, vajadusel keskmise kalde ja eeldatava veemahutavuse järgi.</skos:scopeNote>
    <skos:prefLabel xml:lang="fi">Maaperä</skos:prefLabel>
    <skos:scopeNote xml:lang="fi">Maannoksen ja muuttumattoman pohjamaalajin kuvaaminen syvyyden, raekoostumuksen, rakenteen sekä hiukkasten ja orgaanisen aineksen sisällön, kivisyyden, eroosion ja tarvittaessa keskimääräisen kaltevuuden ja arvioidun veden varastointikapasiteetin mukaan.</skos:scopeNote>
    <skos:prefLabel xml:lang="fr">Sols</skos:prefLabel>
    <skos:scopeNote xml:lang="fr">Sols et sous-sol caractérisés selon leur profondeur, texture, structure et teneur en particules et en matières organiques, pierrosité, érosion, le cas échéant pente moyenne et capacité anticipée de stockage de l'eau.</skos:scopeNote>
    <skos:prefLabel xml:lang="hu">Talaj</skos:prefLabel>
    <skos:scopeNote xml:lang="hu">A mélység, állag, szerkezet, a részecskék és szerves anyagok jelenléte, a köves jelleg, az erózió, valamint adott esetben az átlagos lejtés és a becsült víztartó képesség alapján jellemzett talajok és altalaj.</skos:scopeNote>
    <skos:prefLabel xml:lang="it">Suolo</skos:prefLabel>
    <skos:scopeNote xml:lang="it">Caratterizzazione del suolo e del sottosuolo in base a profondità, tessitura (texture), struttura e contenuto delle particelle e della materia organica, pietrosità, erosione, eventualmente pendenza media e capacità prevista di ritenzione dell’acqua.</skos:scopeNote>
    <skos:prefLabel xml:lang="lt">Dirvožemis</skos:prefLabel>
    <skos:scopeNote xml:lang="lt">Dirvožemio ir podirvio charakteristikos: gylis, granuliometrinė sudėtis, dalelių ir organinių medžiagų struktūra ir sudėtis, akmeningumas, erozija ir tam tikrais atvejais vidutinis nuolydis bei numatomas vandens sulaikymo pajėgumas.</skos:scopeNote>
    <skos:prefLabel xml:lang="lv">Augsne</skos:prefLabel>
    <skos:scopeNote xml:lang="lv">Augsnes un tās apakškārtas stāvoklis, ko raksturo dziļums, faktūra, struktūra un daļiņu un organisko vielu saturs, akmeņainība, erozija un, attiecīgā gadījumā, vidējais slīpums un prognozējamā ūdens uzkrāšanas spēja.</skos:scopeNote>
    <skos:prefLabel xml:lang="mt">Ħamrija</skos:prefLabel>
    <skos:scopeNote xml:lang="mt">Tipi ta' ħamrija u sub-ħamrija kkaratterizzati skond il-fond, it-tessut, l-istruttura u l-kontenut ta' partiċelli u materjal organiku, il-kontenut ta' ġebel, it-tgħawwir, fejn xieraq il-medja tax-xaqlib ta' l-art u l-kapaċità antiċipata għall-ħażna ta' l-ilma.</skos:scopeNote>
    <skos:prefLabel xml:lang="nl">Bodem</skos:prefLabel>
    <skos:scopeNote xml:lang="nl">Bodem en ondergrond, gekenmerkt volgens diepte, textuur, structuur en inhoud van deeltjes en organisch materiaal, steenachtigheid, erosie en, waar passend, gemiddelde hellingsgraad en verwachte wateropslagcapaciteit.</skos:scopeNote>
    <skos:prefLabel xml:lang="pl">Gleba</skos:prefLabel>
    <skos:scopeNote xml:lang="pl">Gleby i podglebie charakteryzowane na podstawie głębokości, tekstury, struktury i zawartości cząstek oraz materiału organicznego, kamienistości, erozji, a w odpowiednich przypadkach na podstawie przeciętnego nachylenia oraz przewidywanej zdolności zatrzymywania wody.</skos:scopeNote>
    <skos:prefLabel xml:lang="pt">Solo</skos:prefLabel>
    <skos:scopeNote xml:lang="pt">Solo e subsolo caracterizado de acordo com a profundidade, textura, estrutura e conteúdo das partículas e material orgânico, carácter pedregoso, erosão, eventualmente declive médio e capacidade estimada de armazenamento de água.</skos:scopeNote>
    <skos:prefLabel xml:lang="ro">Soluri</skos:prefLabel>
    <skos:scopeNote xml:lang="ro">Soluri și subsoluri, caracterizate în funcție de adâncime, textură, structură și conținut al particulelor și materialului organic, schelet, eroziune, înclinație medie și capacitate anticipată de stocare a apei, după caz.</skos:scopeNote>
    <skos:prefLabel xml:lang="sk">Pôda</skos:prefLabel>
    <skos:scopeNote xml:lang="sk">Pôdy a podložia charakterizované podľa hĺbky, textúry, štruktúry a obsahu častíc a organického materiálu, kamenitosti, erózie, prípadne priemerným sklonom a predpokladanou schopnosťou zadržiavať vodu.</skos:scopeNote>
    <skos:prefLabel xml:lang="sl">Tla</skos:prefLabel>
    <skos:scopeNote xml:lang="sl">Tla in sloji prsti pod površjem, določeni po debelini, teksturi, zgradbi in vsebnosti delcev in organskih snovi, kamnitosti, eroziji, po potrebi povprečni nagib in predvidene zmogljivosti vodnih zalog.</skos:scopeNote>
    <skos:prefLabel xml:lang="sv">Mark</skos:prefLabel>
    <skos:scopeNote xml:lang="sv">Jordmåner och jordarter klassificerade efter djup, textur, struktur och innehåll av partiklar och organiskt material, stenighet, erosion, vid behov genomsnittlig lutning och beräknad vattenhållande förmåga.</skos:scopeNote>
    <skos:altLabel>so</skos:altLabel>
    <skos:inScheme rdf:resource="http://inspire.ec.europa.eu/theme" />
  </skos:Concept>
  <skos:Concept xmlns:skos="http://www.w3.org/2004/02/skos/core#" rdf:about="http://inspire.ec.europa.eu/theme/sd">
    <skos:prefLabel xml:lang="en">Species distribution</skos:prefLabel>
    <skos:scopeNote xml:lang="en">Geographical distribution of occurrence of animal and plant species aggregated by grid, region, administrative unit or other analytical unit.</skos:scopeNote>
    <skos:prefLabel xml:lang="bg">Разпределение на видовете</skos:prefLabel>
    <skos:scopeNote xml:lang="bg">Географско разпределение на животинските и растителните видове, представено обобщено по координати, регион, административна единица или друга аналитична единица.</skos:scopeNote>
    <skos:prefLabel xml:lang="cs">Rozložení druhů</skos:prefLabel>
    <skos:scopeNote xml:lang="cs">Zeměpisné rozložení výskytu živočišných a rostlinných druhů seskupených podle souřadnicové sítě, regionu, správní jednotky nebo jiné analytické jednotky.</skos:scopeNote>
    <skos:prefLabel xml:lang="hr">Raširenost vrsta</skos:prefLabel>
    <skos:scopeNote xml:lang="hr">Geografska raširenost životinjskih i biljnih vrsta, razvrstana po mreži, regiji, administrativnoj jedinici ili drugoj analitičkoj jedinici.</skos:scopeNote>
    <skos:prefLabel xml:lang="da">Artsfordeling</skos:prefLabel>
    <skos:scopeNote xml:lang="da">Den geografiske fordeling af forekomsten af dyre- og plantearter i kvadratnetceller, forvaltningsenheder eller andre analytiske enheder.</skos:scopeNote>
    <skos:prefLabel xml:lang="de">Verteilung der Arten</skos:prefLabel>
    <skos:scopeNote xml:lang="de">Geografische Verteilung des Auftretens von Tier- und Pflanzenarten, zusammengefasst in Gittern, Region, Verwaltungseinheit oder sonstigen analytischen Einheiten.</skos:scopeNote>
    <skos:prefLabel xml:lang="el">Κατανομή ειδών</skos:prefLabel>
    <skos:scopeNote xml:lang="el">Γεωγραφική κατανομή ειδών πανίδας και χλωρίδας, ανά κάνναβο, περιοχή, διοικητική ενότητα ή άλλη ενότητα ανάλυσης.</skos:scopeNote>
    <skos:prefLabel xml:lang="es">Distribución de las especies</skos:prefLabel>
    <skos:scopeNote xml:lang="es">Distribución geográfica de las especies animales y vegetales referidas a una cuadrícula, región, unidad administrativa u otro tipo de unidad analítica.</skos:scopeNote>
    <skos:prefLabel xml:lang="et">Liikide jaotumine</skos:prefLabel>
    <skos:scopeNote xml:lang="et">Taime- ja loomaliikide geograafiline levik ruutvõrgu, piirkondade, haldusüksuste või muude jaotusüksuste kaupa.</skos:scopeNote>
    <skos:prefLabel xml:lang="fi">Lajien levinneisyys</skos:prefLabel>
    <skos:scopeNote xml:lang="fi">Eläin- ja kasvilajien esiintymien maantieteellinen levinneisyys ruudukoittain, alueittain, hallintoyksiköittäin tai muiden analyyttisten yksiköitten mukaisesti jaoteltuna.</skos:scopeNote>
    <skos:prefLabel xml:lang="fr">Répartition des espèces</skos:prefLabel>
    <skos:scopeNote xml:lang="fr">Répartition géographique de l'occurrence des espèces animales et végétales regroupées par grille, région, unité administrative ou autre unité analytique.</skos:scopeNote>
    <skos:prefLabel xml:lang="hu">A fajok megoszlása</skos:prefLabel>
    <skos:scopeNote xml:lang="hu">Az állat- és növényfajok előfordulásának földrajzi eloszlása, térképrács, régió, közigazgatási egység vagy más elemzési egység alapján összesítve.</skos:scopeNote>
    <skos:prefLabel xml:lang="it">Distribuzione delle specie</skos:prefLabel>
    <skos:scopeNote xml:lang="it">Distribuzione geografica delle specie animali e vegetali aggregate per griglia, regione, unità amministrativa o altra unità analitica.</skos:scopeNote>
    <skos:prefLabel xml:lang="lt">Rūšių pasiskirstymas</skos:prefLabel>
    <skos:scopeNote xml:lang="lt">Geografinis gyvūnų ir augalų rūšių pasiskirstymas pagal tinklelį, regioną, administracinį ar kitą analitinį vienetą.</skos:scopeNote>
    <skos:prefLabel xml:lang="lv">Sugu izplatība</skos:prefLabel>
    <skos:scopeNote xml:lang="lv">Dzīvnieku un augu sugu ģeogrāfiskais sadalījums, grupējot pēc koordinātu tīkla, reģiona, administratīvām vai citām analītiskām vienībām.</skos:scopeNote>
    <skos:prefLabel xml:lang="mt">Distribuzzjoni ta' l-ispeċi</skos:prefLabel>
    <skos:scopeNote xml:lang="mt">Distribuzzjoni ġeografika ta' l-okkorrenza ta' speċi ta' annimali u ta' pjanti miġbura flimkien skond il-grilja, ir-reġjun, l-unità amministrattiva jew unità analitika oħra.</skos:scopeNote>
    <skos:prefLabel xml:lang="nl">Spreiding van soorten</skos:prefLabel>
    <skos:scopeNote xml:lang="nl">Geografische spreiding van dier- en plantensoorten per raster, regio, administratieve eenheid of andere analytische eenheid.</skos:scopeNote>
    <skos:prefLabel xml:lang="pl">Rozmieszczenie gatunków</skos:prefLabel>
    <skos:scopeNote xml:lang="pl">Geograficzne rozmieszczenie występowania gatunków zwierząt i roślin pogrupowanych według siatki geograficznej, regionu, jednostki administracyjnej lub innej jednostki analitycznej.</skos:scopeNote>
    <skos:prefLabel xml:lang="pt">Distribuição das espécies</skos:prefLabel>
    <skos:scopeNote xml:lang="pt">Distribuição geográfica da ocorrência de espécies animais e vegetais agregadas por quadrícula, região, unidade administrativa ou outra unidade analítica.</skos:scopeNote>
    <skos:prefLabel xml:lang="ro">Repartizarea speciilor</skos:prefLabel>
    <skos:scopeNote xml:lang="ro">Repartizarea geografică a speciilor de animale și plante, regrupate pe grilă, regiune, unitate administrativă sau altă unitate analitică.</skos:scopeNote>
    <skos:prefLabel xml:lang="sk">Výskyt druhov</skos:prefLabel>
    <skos:scopeNote xml:lang="sk">Geografické rozdelenie výskytu živočíšnych a rastlinných druhov zoskupený podľa siete, regiónu, administratívnej jednotky alebo inej analytickej jednotky.</skos:scopeNote>
    <skos:prefLabel xml:lang="sl">Porazdelitev vrst</skos:prefLabel>
    <skos:scopeNote xml:lang="sl">Geografska porazdelitev pojavljanja živalskih in rastlinskih vrst, razvrščenih po koordinatah, regiji, upravni enoti ali drugi analitični enoti.</skos:scopeNote>
    <skos:prefLabel xml:lang="sv">Arters utbredning</skos:prefLabel>
    <skos:scopeNote xml:lang="sv">Geografisk fördelning av djur- och växtarters förekomst i rutnät, regioner, administrativa enheter eller andra analytiska enheter.</skos:scopeNote>
    <skos:altLabel>sd</skos:altLabel>
    <skos:inScheme rdf:resource="http://inspire.ec.europa.eu/theme" />
  </skos:Concept>
  <skos:Concept xmlns:skos="http://www.w3.org/2004/02/skos/core#" rdf:about="http://inspire.ec.europa.eu/theme/su">
    <skos:prefLabel xml:lang="en">Statistical units</skos:prefLabel>
    <skos:scopeNote xml:lang="en">Units for dissemination or use of statistical information.</skos:scopeNote>
    <skos:prefLabel xml:lang="bg">Статистически единици</skos:prefLabel>
    <skos:scopeNote xml:lang="bg">Единици, разпространяващи или ползващи статистическа информация.</skos:scopeNote>
    <skos:prefLabel xml:lang="cs">Statistické jednotky</skos:prefLabel>
    <skos:scopeNote xml:lang="cs">Jednotky pro šíření nebo používání statistických informací.</skos:scopeNote>
    <skos:prefLabel xml:lang="hr">Statističke jedinice</skos:prefLabel>
    <skos:scopeNote xml:lang="hr">Jedinice za širenje ili korištenje statističkih informacija.</skos:scopeNote>
    <skos:prefLabel xml:lang="da">Statistiske enheder</skos:prefLabel>
    <skos:scopeNote xml:lang="da">Enheder for formidling eller anvendelse af statistiske oplysninger.</skos:scopeNote>
    <skos:prefLabel xml:lang="de">Statistische Einheiten</skos:prefLabel>
    <skos:scopeNote xml:lang="de">Einheiten für die Verbreitung oder Verwendung statistischer Daten.</skos:scopeNote>
    <skos:prefLabel xml:lang="el">Στατιστικές μονάδες</skos:prefLabel>
    <skos:scopeNote xml:lang="el">Μονάδες διάδοσης ή χρήσης στατιστικών πληροφοριών.</skos:scopeNote>
    <skos:prefLabel xml:lang="es">Unidades estadísticas</skos:prefLabel>
    <skos:scopeNote xml:lang="es">Unidades para la difusión o el uso de información estadística.</skos:scopeNote>
    <skos:prefLabel xml:lang="et">Statistilised üksused</skos:prefLabel>
    <skos:scopeNote xml:lang="et">Statistilise teabe levitamise või kasutamise üksused.</skos:scopeNote>
    <skos:prefLabel xml:lang="fi">Tilastoyksiköt</skos:prefLabel>
    <skos:scopeNote xml:lang="fi">Tilastotietojen levittämis- tai käyttöyksiköt.</skos:scopeNote>
    <skos:prefLabel xml:lang="fr">Unités statistiques</skos:prefLabel>
    <skos:scopeNote xml:lang="fr">Unités de diffusion ou d'utilisation d'autres informations statistiques.</skos:scopeNote>
    <skos:prefLabel xml:lang="hu">Statisztikai egységek</skos:prefLabel>
    <skos:scopeNote xml:lang="hu">Statisztikai információk terjesztésére vagy felhasználására szolgáló egységek.</skos:scopeNote>
    <skos:prefLabel xml:lang="it">Unità statistiche</skos:prefLabel>
    <skos:scopeNote xml:lang="it">Unità per la divulgazione o l'utilizzo di dati statistici.</skos:scopeNote>
    <skos:prefLabel xml:lang="lt">Statistiniai vienetai</skos:prefLabel>
    <skos:scopeNote xml:lang="lt">Vienetai, skirti statistinės informacijos platinimui ar panaudojimui.</skos:scopeNote>
    <skos:prefLabel xml:lang="lv">Statistikas vienības</skos:prefLabel>
    <skos:scopeNote xml:lang="lv">Vienības, kuras izmanto statistikas informācijas izplatīšanā vai izmantošanā.</skos:scopeNote>
    <skos:prefLabel xml:lang="mt">Unitajiet statistiċi</skos:prefLabel>
    <skos:scopeNote xml:lang="mt">Unitajiet biex issir disseminazzjoni jew użu ta' informazzjoni ta' l-istatistika.</skos:scopeNote>
    <skos:prefLabel xml:lang="nl">Statistische eenheden</skos:prefLabel>
    <skos:scopeNote xml:lang="nl">Eenheden voor verspreiding en gebruik van statistische informatie.</skos:scopeNote>
    <skos:prefLabel xml:lang="pl">Jednostki statystyczne</skos:prefLabel>
    <skos:scopeNote xml:lang="pl">Jednostki służące do rozpowszechniania lub wykorzystywania informacji statystycznych.</skos:scopeNote>
    <skos:prefLabel xml:lang="pt">Unidades estatísticas</skos:prefLabel>
    <skos:scopeNote xml:lang="pt">Unidades para fins de divulgação ou utilização da informação estatística.</skos:scopeNote>
    <skos:prefLabel xml:lang="ro">Unități statistice</skos:prefLabel>
    <skos:scopeNote xml:lang="ro">Unități de difuzare sau de utilizare a informațiilor statistice.</skos:scopeNote>
    <skos:prefLabel xml:lang="sk">Štatistické jednotky</skos:prefLabel>
    <skos:scopeNote xml:lang="sk">Jednotky pre šírenie alebo využívanie štatistických informácií.</skos:scopeNote>
    <skos:prefLabel xml:lang="sl">Statistični okoliši</skos:prefLabel>
    <skos:scopeNote xml:lang="sl">Enote za širjenje ali uporabo statističnih podatkov.</skos:scopeNote>
    <skos:prefLabel xml:lang="sv">Statistiska enheter</skos:prefLabel>
    <skos:scopeNote xml:lang="sv">Enheter för spridning och användning av statistisk information.</skos:scopeNote>
    <skos:altLabel>su</skos:altLabel>
    <skos:inScheme rdf:resource="http://inspire.ec.europa.eu/theme" />
  </skos:Concept>
  <skos:Concept xmlns:skos="http://www.w3.org/2004/02/skos/core#" rdf:about="http://inspire.ec.europa.eu/theme/us">
    <skos:prefLabel xml:lang="en">Utility and governmental services</skos:prefLabel>
    <skos:scopeNote xml:lang="en">Includes utility facilities such as sewage, waste management, energy supply and water supply, administrative and social governmental services such as public administrations, civil protection sites, schools and hospitals.</skos:scopeNote>
    <skos:prefLabel xml:lang="bg">Комунално-битови и обществени услуги</skos:prefLabel>
    <skos:scopeNote xml:lang="bg">Включват инфраструктура за комунално-битови услуги, например напоителни системи, управление на отпадъците, електроснабдяване и водоснабдяване, административни и социални обществени услуги, например публични администрации, обекти на гражданската защита, училища и болници.</skos:scopeNote>
    <skos:prefLabel xml:lang="cs">Veřejné služby a služby veřejné správy</skos:prefLabel>
    <skos:scopeNote xml:lang="cs">Zahrnují zařízení, jako například kanalizace, nakládání s odpady, zásobování energií a zásobování vodou, správní a sociální státní služby, jako například veřejnou správu, zařízení civilní ochrany, školy a nemocnice.</skos:scopeNote>
    <skos:prefLabel xml:lang="hr">Komunalne i državne usluge</skos:prefLabel>
    <skos:scopeNote xml:lang="hr">Uključuje komunalne sustave kao što su kanalizacija, zbrinjavanje otpada, opskrba energijom i opskrba vodom, upravne i socijalne državne usluge kao što su javna uprava, sjedišta civilne zaštite, škole i bolnice.</skos:scopeNote>
    <skos:prefLabel xml:lang="da">Offentlig forsyningsvirksomhed og offentlige tjenesteydelser</skos:prefLabel>
    <skos:scopeNote xml:lang="da">Omfatter forsyningsvirksomhed så som kloakering, affaldshåndtering, energiforsyning og vandforsyning, administrative og sociale offentlige tjenester som f.eks. offentlige administrationer, civilbeskyttelsesanlæg, skoler og hospitaler.</skos:scopeNote>
    <skos:prefLabel xml:lang="de">Versorgungswirtschaft und staatliche Dienste</skos:prefLabel>
    <skos:scopeNote xml:lang="de">Versorgungseinrichtungen wie Abwasser- und Abfallentsorgung, Energieversorgung und Wasserversorgung; staatliche Verwaltungs- und Sozialdienste wie öffentliche Verwaltung, Katastrophenschutz, Schulen und Krankenhäuser.</skos:scopeNote>
    <skos:prefLabel xml:lang="el">Επιχειρήσεις κοινής ωφελείας και κρατικές υπηρεσίες</skos:prefLabel>
    <skos:scopeNote xml:lang="el">Περιλαμβάνονται εγκαταστάσεις υπηρεσιών κοινής ωφελείας, όπως η αποχέτευση, η διαχείριση αποβλήτων, ο ενεργειακός εφοδιασμός και η υδροδότηση, οι διοικητικές και κοινωνικές κρατικές υπηρεσίες, όπως οι δημόσιες διοικήσεις, οι χώροι πολιτικής προστασίας, τα σχολεία και τα νοσοκομεία.</skos:scopeNote>
    <skos:prefLabel xml:lang="es">Servicios de utilidad pública y estatales</skos:prefLabel>
    <skos:scopeNote xml:lang="es">Incluye instalaciones de utilidad pública de alcantarillado, gestión de residuos, suministro de energía y suministro de agua, así como servicios estatales administrativos y sociales tales como administraciones públicas, sitios de protección civil, escuelas y hospitales.</skos:scopeNote>
    <skos:prefLabel xml:lang="et">Kommunaal- ja riiklikud teenused</skos:prefLabel>
    <skos:scopeNote xml:lang="et">Hõlmab tehnorajatisi nagu näiteks reovee ja jäätmete käitluse, energia- ja veevarustuse võrgud ja rajatised ning riiklikke haldus- ja sotsiaalteenuseid nagu riiklikud haldusorganid, kodanikukaitse alad, koolid ja haiglad.</skos:scopeNote>
    <skos:prefLabel xml:lang="fi">Yleishyödylliset ja muut julkiset palvelut</skos:prefLabel>
    <skos:scopeNote xml:lang="fi">Tämä käsittää yleishyödyllisten palvelujen laitokset, kuten viemäröinnin, jätehuollon, energiahuollon ja vesihuollon, sekä hallinnolliset ja sosiaaliset julkiset palvelut, kuten viranomaiset, väestönsuojat, koulut ja sairaalat.</skos:scopeNote>
    <skos:prefLabel xml:lang="fr">Services d'utilité publique et services publics</skos:prefLabel>
    <skos:scopeNote xml:lang="fr">Comprend les installations d'utilité publique, tels que les égouts ou les réseaux et installations liés à la gestion des déchets, à l'approvisionnement énergétique, à l'approvisionnement en eau, ainsi que les services administratifs et sociaux publics, tels que les administrations publiques, les sites de la protection civile, les écoles et les hôpitaux.</skos:scopeNote>
    <skos:prefLabel xml:lang="hu">Közüzemi és közszolgáltatások</skos:prefLabel>
    <skos:scopeNote xml:lang="hu">Magában foglalja az olyan közüzemi létesítményeket, mint például a szennyvíz- és hulladékgazdálkodás, az energiaellátás és a vízellátás, valamint az igazgatási és szociális közszolgáltatásokat, például a közigazgatási szerveket, a polgári védelmi létesítményeket, iskolákat és kórházakat.</skos:scopeNote>
    <skos:prefLabel xml:lang="it">Servizi di pubblica utilità e servizi amministrativi</skos:prefLabel>
    <skos:scopeNote xml:lang="it">Sono compresi sia impianti quali gli impianti fognari, di gestione dei rifiuti, di fornitura energetica, e di distribuzione idrica, sia servizi pubblici amministrativi e sociali quali le amministrazioni pubbliche, i siti della protezione civile, le scuole e gli ospedali.</skos:scopeNote>
    <skos:prefLabel xml:lang="lt">Komunalinės įmonės ir valstybės tarnybos</skos:prefLabel>
    <skos:scopeNote xml:lang="lt">Tai apima komunalinių įmonių infrastruktūrą, pavyzdžiui, kanalizaciją, atliekų tvarkymą, elektros energijos tiekimą ir vandens tiekimą, administracines ir socialines valstybės tarnybas, pavyzdžiui, viešojo administravimo įstaigas, civilinės saugos tarnybas, mokyklas ir ligonines.</skos:scopeNote>
    <skos:prefLabel xml:lang="lv">Komunālie un valsts dienesti</skos:prefLabel>
    <skos:scopeNote xml:lang="lv">Tas ietver tādu komunālo dienestu iekārtas kā kanalizācija, atkritumu apsaimniekošana, energoapgāde un ūdens apgāde, administratīvos un sociālos valsts dienestus, piemēram, valsts administrāciju, civilās aizsardzības novietnes, skolas un slimnīcas.</skos:scopeNote>
    <skos:prefLabel xml:lang="mt">Servizzi ta' utilità u tal-gvern</skos:prefLabel>
    <skos:scopeNote xml:lang="mt">Jinkludu faċilitajiet ta' utilità bħad-drenaġġ, l-immaniġġar ta' l-iskart, il-provvista ta' l-enerġija, il-provvista ta' l-ilma, is-servizzi amministrattivi u soċjali tal-gvern bħal amministrazzjonijiet pubbliċi, siti għall-protezzjoni ċivili, skejjel u sptarijiet.</skos:scopeNote>
    <skos:prefLabel xml:lang="nl">Nutsdiensten en overheidsdiensten</skos:prefLabel>
    <skos:scopeNote xml:lang="nl">Nutsvoorzieningen zoals riolering, afvalbeheer, energievoorziening, watervoorziening, bestuurlijke en maatschappelijke instanties van de overheid, zoals bestuurlijke overheden, civiele bescherming, scholen en ziekenhuizen.</skos:scopeNote>
    <skos:prefLabel xml:lang="pl">Usługi użyteczności publicznej i służby państwowe</skos:prefLabel>
    <skos:scopeNote xml:lang="pl">Obejmuje instalacje użyteczności publicznej takie jak: kanalizacja, zarządzanie odpadami, dostawa energii i dostawa wody, administracyjne i społeczne służby państwowe lub samorządowe, takie jak: administracja publiczna, obiekty ochrony cywilnej, szkoły i szpitale.</skos:scopeNote>
    <skos:prefLabel xml:lang="pt">Serviços de utilidade pública e do Estado</skos:prefLabel>
    <skos:scopeNote xml:lang="pt">Inclui instalações e serviços de utilidade pública, como redes de esgotos, gestão de resíduos, fornecimento de energia, abastecimento de água, serviços administrativos e sociais do Estado tais como administrações públicas, instalações da protecção civil, escolas e hospitais.</skos:scopeNote>
    <skos:prefLabel xml:lang="ro">Servicii de utilitate publică și servicii publice</skos:prefLabel>
    <skos:scopeNote xml:lang="ro">Includ instalațiile de utilitate publică, precum sistemele de canalizare, de gestionare a deșeurilor, de aprovizionare cu energie electrică și apă, și serviciile administrative și sociale publice, precum adăposturile de protecție civilă, școlile și spitalele.</skos:scopeNote>
    <skos:prefLabel xml:lang="sk">Verejné a štátne služby</skos:prefLabel>
    <skos:scopeNote xml:lang="sk">Patria sem verejné zariadenia, ako napríklad kanalizácia, nakladanie s odpadom, dodávka energie a dodávka vody, administratívne a sociálne štátne služby, ako napríklad verejná správa, miesta civilnej ochrany, školy a nemocnice.</skos:scopeNote>
    <skos:prefLabel xml:lang="sl">Komunalne in javne storitve</skos:prefLabel>
    <skos:scopeNote xml:lang="sl">Vključuje komunalne naprave kot so kanalizacija, ravnanje z odpadki, oskrba z energijo in preskrba z vodo, upravne in socialne vladne službe kot so javne uprave, sedeži civilne zaščite, šole in bolnišnice.</skos:scopeNote>
    <skos:prefLabel xml:lang="sv">Allmännyttiga och offentliga tjänster</skos:prefLabel>
    <skos:scopeNote xml:lang="sv">Inbegriper anläggningar för allmännyttiga tjänster, exempelvis för hantering av avloppsvatten, avfallshantering, energiförsörjning och vattenförsörjning, administrativa och sociala offentliga tjänster såsom offentliga förvaltningar, räddningstjänstens anläggningar, skolor och sjukhus.</skos:scopeNote>
    <skos:altLabel>us</skos:altLabel>
    <skos:inScheme rdf:resource="http://inspire.ec.europa.eu/theme" />
  </skos:Concept>
  <skos:Concept xmlns:skos="http://www.w3.org/2004/02/skos/core#" rdf:about="http://inspire.ec.europa.eu/theme/mf">
    <skos:prefLabel xml:lang="en">Meteorological geographical features</skos:prefLabel>
    <skos:scopeNote xml:lang="en">Weather conditions and their measurements; precipitation, temperature, evapotranspiration, wind speed and direction.</skos:scopeNote>
    <skos:prefLabel xml:lang="bg">Метеорологични географски характеристики</skos:prefLabel>
    <skos:scopeNote xml:lang="bg">Атмосферни условия и измерването им; валежи, температура, евапотранспирация, скорост и посока на вятъра.</skos:scopeNote>
    <skos:prefLabel xml:lang="cs">Zeměpisné meteorologické prvky</skos:prefLabel>
    <skos:scopeNote xml:lang="cs">Povětrnostní podmínky a jejich měření; srážky, teplota, výpar z půdy a rostlinného pokryvu, rychlost a směr větru.</skos:scopeNote>
    <skos:prefLabel xml:lang="hr">Meteorološko-geografske značajke</skos:prefLabel>
    <skos:scopeNote xml:lang="hr">Vremenski uvjeti i njihova mjerenja; padaline, temperature, ishlapljivanje, brzina i smjer vjetra.</skos:scopeNote>
    <skos:prefLabel xml:lang="da">Meteorologisk-geografiske forhold</skos:prefLabel>
    <skos:scopeNote xml:lang="da">Vejrforhold og målinger heraf; nedbør, temperatur, evapotranspiration, vindhastighed og -retning.</skos:scopeNote>
    <skos:prefLabel xml:lang="de">Meteorologisch-geografische Kennwerte</skos:prefLabel>
    <skos:scopeNote xml:lang="de">Witterungsbedingungen und deren Messung; Niederschlag, Temperatur, Gesamtverdunstung (Evapotranspiration), Windgeschwindigkeit und Windrichtung.</skos:scopeNote>
    <skos:prefLabel xml:lang="el">Μετεωρολογικά γεωγραφικά χαρακτηριστικά</skos:prefLabel>
    <skos:scopeNote xml:lang="el">Καιρικές συνθήκες και οι μετρήσεις τους· ατμοσφαιρικές κατακρημνίσεις, θερμοκρασία, εξατμισοδιαπνοή, ταχύτητα και διεύθυνση ανέμου.</skos:scopeNote>
    <skos:prefLabel xml:lang="es">Aspectos geográficos de carácter meteorológico</skos:prefLabel>
    <skos:scopeNote xml:lang="es">Condiciones meteorológicas y sus mediciones; precipitaciones, temperaturas, evapotranspiración, velocidad y dirección del viento.</skos:scopeNote>
    <skos:prefLabel xml:lang="et">Meteoroloogilis-geograafilised tunnusjooned</skos:prefLabel>
    <skos:scopeNote xml:lang="et">Ilmastikutingimused ja nende mõõtmine; sademed, temperatuur, aurumine, tuule kiirus ja suund.</skos:scopeNote>
    <skos:prefLabel xml:lang="fi">Ilmaston maantieteelliset ominaispiirteet</skos:prefLabel>
    <skos:scopeNote xml:lang="fi">Sääolot ja niihin liittyvät mittaukset; sademäärä, lämpötila, kokonaishaihdunta, tuulen nopeus ja suunta.</skos:scopeNote>
    <skos:prefLabel xml:lang="fr">Caractéristiques géographiques météorologiques</skos:prefLabel>
    <skos:scopeNote xml:lang="fr">Conditions météorologiques et leur mesure: précipitations, température, évapotranspiration, vitesse et direction du vent.</skos:scopeNote>
    <skos:prefLabel xml:lang="hu">Meteorológiai földrajzi jellemzők</skos:prefLabel>
    <skos:scopeNote xml:lang="hu">Időjárási viszonyok és mérésük; csapadék, hőmérséklet, a felszín és a növényzet párolgása, a szél sebessége és iránya.</skos:scopeNote>
    <skos:prefLabel xml:lang="it">Elementi geografici meteorologici</skos:prefLabel>
    <skos:scopeNote xml:lang="it">Condizioni meteorologiche e relative misurazioni; precipitazioni, temperatura, evapotraspirazione, velocità e direzione dei venti.</skos:scopeNote>
    <skos:prefLabel xml:lang="lt">Meteorologinės geografinės sąlygos</skos:prefLabel>
    <skos:scopeNote xml:lang="lt">Oro sąlygos ir jų matavimai; krituliai, temperatūra, evapotranspiracija, vėjo greitis ir kryptis.</skos:scopeNote>
    <skos:prefLabel xml:lang="lv">Meteoroloģiski ģeogrāfiskie raksturlielumi</skos:prefLabel>
    <skos:scopeNote xml:lang="lv">Laika apstākļi un to mērījumi; nokrišņi, temperatūra, iztvaikošana, vēja ātrums un virziens.</skos:scopeNote>
    <skos:prefLabel xml:lang="mt">Karatteristiċi ġeografiċi meteoroloġiċi</skos:prefLabel>
    <skos:scopeNote xml:lang="mt">Il-kondizzjonijiet tat-temp u l-kejl tagħhom; il-preċipitazzjoni, it-temperatura, l-evapotraspirazzjoni, il-veloċità u d-direzzjoni tar-riħ.</skos:scopeNote>
    <skos:prefLabel xml:lang="nl">Meteorologische geografische kenmerken</skos:prefLabel>
    <skos:scopeNote xml:lang="nl">Weersomstandigheden en de meting daarvan; neerslag, temperatuur, verdamping, windsnelheid en windrichting.</skos:scopeNote>
    <skos:prefLabel xml:lang="pl">Warunki meteorologiczno-geograficzne</skos:prefLabel>
    <skos:scopeNote xml:lang="pl">Warunki atmosferyczne i ich pomiary; opad atmosferyczny, temperatura, ewapotranspiracja, prędkość i kierunek wiatru.</skos:scopeNote>
    <skos:prefLabel xml:lang="pt">Características geometeorológicas</skos:prefLabel>
    <skos:scopeNote xml:lang="pt">Condições atmosféricas e sua medição; precipitação, temperatura, evapotranspiração, velocidade e direcção do vento.</skos:scopeNote>
    <skos:prefLabel xml:lang="ro">Caracteristici geografice meteorologice</skos:prefLabel>
    <skos:scopeNote xml:lang="ro">Condițiile meteorologice și măsurătorile acestora: precipitații, temperatură, evapotranspirație, viteza și direcția vântului.</skos:scopeNote>
    <skos:prefLabel xml:lang="sk">Meteorologické geografické prvky</skos:prefLabel>
    <skos:scopeNote xml:lang="sk">Poveternostné podmienky a ich merania; zrážky, teplota, evapotranspirácia, rýchlosť a smer vetra.</skos:scopeNote>
    <skos:prefLabel xml:lang="sl">Meteorološke značilnosti</skos:prefLabel>
    <skos:scopeNote xml:lang="sl">Vremenske razmere in njihova merjenja; padavine, temperatura, izhlapevanje, hitrost in smer vetra.</skos:scopeNote>
    <skos:prefLabel xml:lang="sv">Geografiska meteorologiska förhållanden</skos:prefLabel>
    <skos:scopeNote xml:lang="sv">Väderförhållanden och mätningar av dessa; nederbörd, temperatur, evapotranspiration, vindhastighet och vindriktning.</skos:scopeNote>
    <skos:altLabel>mf</skos:altLabel>
    <skos:inScheme rdf:resource="http://inspire.ec.europa.eu/theme" />
  </skos:Concept>
</rdf:RDF>

