<?xml version="1.0" encoding="UTF-8"?><?xml-stylesheet href="/VocabV2/skosrdf2html.xsl" type="text/xsl" media="screen"?><rdf:RDF xmlns:rdf="http://www.w3.org/1999/02/22-rdf-syntax-ns#" xmlns:skos="http://www.w3.org/2004/02/skos/core#" xmlns:dc="http://purl.org/dc/terms/" xmlns:dce="http://purl.org/dc/elements/1.1/" xmlns:rdfs="http://www.w3.org/2000/01/rdf-schema#" xmlns:grg="http://www.isotc211.org/schemas/grg/" xmlns:owl="http://www.w3.org/2002/07/owl#" xmlns:void="http://rdfs.org/ns/void#">
<skos:Collection rdf:about="http://vocab.nerc.ac.uk/collection/L02/current/">
<skos:prefLabel>SeaDataNet Geospatial Feature Types</skos:prefLabel>
<dc:title>SeaDataNet Geospatial Feature Types</dc:title>
<skos:altLabel>SeaDataNet Geospatial Feature Types</skos:altLabel>
<dc:alternative>SeaDataNet Geospatial Feature Types</dc:alternative>
<dc:description>SeaDataNet profile of ISO MD_GeometricObjectTypeCodeTerms code list.  Known in SEA-SEARCH as 'Library 2'  or cdi_measurement_codes.</dc:description>
<dc:date>2014-03-28 02:00:02.0</dc:date>
<owl:versionInfo>2</owl:versionInfo>
<grg:RE_RegisterManager>British Oceanographic Data Centre</grg:RE_RegisterManager>
<dc:publisher>Natural Environment Research Council</dc:publisher>
<dc:creator>SeaDataNet</dc:creator>
<grg:RE_RegisterOwner>SeaDataNet</grg:RE_RegisterOwner>
<rdfs:comment>Governance for vocabularies used in the EU SeaDataNet project implemented as consultation between BODC and the members of the SeaDataNet Technical Task Team</rdfs:comment>
<skos:member>
<skos:Concept rdf:about="http://vocab.nerc.ac.uk/collection/L02/current/003/">
<dc:identifier>SDN:L02::003</dc:identifier>
<dce:identifier>SDN:L02::003</dce:identifier>
<skos:notation>SDN:L02::003</skos:notation>
<skos:prefLabel xml:lang="en">curve</skos:prefLabel>
<skos:altLabel>LineString</skos:altLabel>
<skos:definition xml:lang="en">Bounded, 1-dimensional geometric primitive, representing the continuous image of a line</skos:definition>
<owl:versionInfo>2</owl:versionInfo>
<dc:date>2014-03-27 09:10:09.0</dc:date>
<skos:note xml:lang="en">accepted</skos:note>
<owl:deprecated>false</owl:deprecated>
<void:inDataset rdf:resource="http://vocab.nerc.ac.uk/.well-known/void"/>
</skos:Concept>
</skos:member>
<skos:member>
<skos:Concept rdf:about="http://vocab.nerc.ac.uk/collection/L02/current/004/">
<dc:identifier>SDN:L02::004</dc:identifier>
<dce:identifier>SDN:L02::004</dce:identifier>
<skos:notation>SDN:L02::004</skos:notation>
<skos:prefLabel xml:lang="en">point</skos:prefLabel>
<skos:altLabel>Point</skos:altLabel>
<skos:definition xml:lang="en">Zero-dimensional geometric primitive, representing a position but not having an extent</skos:definition>
<owl:versionInfo>2</owl:versionInfo>
<dc:date>2014-03-27 09:10:18.0</dc:date>
<skos:note xml:lang="en">accepted</skos:note>
<owl:deprecated>false</owl:deprecated>
<void:inDataset rdf:resource="http://vocab.nerc.ac.uk/.well-known/void"/>
</skos:Concept>
</skos:member>
<skos:member>
<skos:Concept rdf:about="http://vocab.nerc.ac.uk/collection/L02/current/006/">
<dc:identifier>SDN:L02::006</dc:identifier>
<dce:identifier>SDN:L02::006</dce:identifier>
<skos:notation>SDN:L02::006</skos:notation>
<skos:prefLabel xml:lang="en">surface</skos:prefLabel>
<skos:altLabel>Polygon</skos:altLabel>
<skos:definition xml:lang="en">Bounded, connected 2-dimensional geometric primitive, representing the continuous image of a region of a plane</skos:definition>
<owl:versionInfo>2</owl:versionInfo>
<dc:date>2014-03-27 09:10:25.0</dc:date>
<skos:note xml:lang="en">accepted</skos:note>
<owl:deprecated>false</owl:deprecated>
<void:inDataset rdf:resource="http://vocab.nerc.ac.uk/.well-known/void"/>
</skos:Concept>
</skos:member>
</skos:Collection>
</rdf:RDF>
