<rdf:RDF xmlns:rdf="http://www.w3.org/1999/02/22-rdf-syntax-ns#" xmlns:skos="http://www.w3.org/2004/02/skos/core#" xmlns:dc="http://purl.org/dc/terms/" xmlns:dce="http://purl.org/dc/elements/1.1/" xmlns:rdfs="http://www.w3.org/2000/01/rdf-schema#" xmlns:grg="https://schemas.isotc211.org/schemas/19135/-2/reg/1.0/registration.xsd" xmlns:owl="http://www.w3.org/2002/07/owl#" xmlns:void="http://rdfs.org/ns/void#" xmlns:pav="http://purl.org/pav/">
<skos:Collection rdf:about="http://vocab.nerc.ac.uk/collection/P35/current/">
<skos:prefLabel>EMODnet Chemistry aggregated parameter names</skos:prefLabel>
<dc:title>EMODnet Chemistry aggregated parameter names</dc:title>
<skos:altLabel>EMODNET chemistry aggregations</skos:altLabel>
<dc:alternative>EMODNET chemistry aggregations</dc:alternative>
<dc:description>Labels used for aggregated parameters in the EMODNET chemistry lot</dc:description>
<dc:date>2021-02-27 02:00:03.0</dc:date>
<owl:versionInfo>18</owl:versionInfo>
<grg:RE_RegisterManager>British Oceanographic Data Centre</grg:RE_RegisterManager>
<dc:publisher>Natural Environment Research Council</dc:publisher>
<dc:creator>EMODNet Chemistry Lot</dc:creator>
<grg:RE_RegisterOwner>EMODNet Chemistry Lot</grg:RE_RegisterOwner>
<rdfs:comment>A European project consortium aimed at the creation of data products using chemical data amassed through SeaDataNet. The governance is loosely defined as the scientific expertise within the consortium with no formal processes defined.</rdfs:comment>
<skos:member>
<skos:Concept rdf:about="http://vocab.nerc.ac.uk/collection/P35/current/EPC00180/">
<dc:identifier>SDN:P35::EPC00180</dc:identifier>
<dce:identifier>SDN:P35::EPC00180</dce:identifier>
<dc:date>2016-12-12 15:20:45.0</dc:date>
<skos:notation>SDN:P35::EPC00180</skos:notation>
<skos:prefLabel xml:lang="en">Ammonium in the sediment</skos:prefLabel>
<skos:altLabel>Ammonium in the sediment</skos:altLabel>
<skos:definition xml:lang="en">Concentration of ammonium in sediment pore water.</skos:definition>
<owl:versionInfo>5</owl:versionInfo>
<pav:hasCurrentVersion rdf:resource="http://vocab.nerc.ac.uk/collection/P35/current/EPC00180/5/"/>
<pav:version>5</pav:version>
<pav:authoredOn>2016-12-12 15:20:45.0</pav:authoredOn>
<skos:note xml:lang="en">accepted</skos:note>
<owl:deprecated>false</owl:deprecated>
<skos:narrower rdf:resource="http://vocab.nerc.ac.uk/collection/P01/current/AMONPWD1/"/>
<skos:related rdf:resource="http://vocab.nerc.ac.uk/collection/P06/current/KGUM/"/>
<skos:broader rdf:resource="http://vocab.nerc.ac.uk/collection/P36/current/FERTIL/"/>
<void:inDataset rdf:resource="http://vocab.nerc.ac.uk/.well-known/void"/>
</skos:Concept>
</skos:member>
<skos:member>
<skos:Concept rdf:about="http://vocab.nerc.ac.uk/collection/P35/current/EPC00182/">
<dc:identifier>SDN:P35::EPC00182</dc:identifier>
<dce:identifier>SDN:P35::EPC00182</dce:identifier>
<dc:date>2018-03-20 16:58:29.0</dc:date>
<skos:notation>SDN:P35::EPC00182</skos:notation>
<skos:prefLabel xml:lang="en">Anthracene in Mytilus</skos:prefLabel>
<skos:altLabel>Anthracene in Mytilus</skos:altLabel>
<skos:definition xml:lang="en">Concentration of anthracene per unit weight (dry or wet) of Mytilus spp. (regardless of Mytilus species and size class).</skos:definition>
<owl:versionInfo>6</owl:versionInfo>
<pav:hasCurrentVersion rdf:resource="http://vocab.nerc.ac.uk/collection/P35/current/EPC00182/6/"/>
<pav:version>6</pav:version>
<pav:authoredOn>2018-03-20 16:58:29.0</pav:authoredOn>
<skos:note xml:lang="en">deprecated</skos:note>
<owl:deprecated>true</owl:deprecated>
<skos:narrower rdf:resource="http://vocab.nerc.ac.uk/collection/P01/current/ACWW6569/"/>
<skos:narrower rdf:resource="http://vocab.nerc.ac.uk/collection/P01/current/ACMMCF14/"/>
<skos:narrower rdf:resource="http://vocab.nerc.ac.uk/collection/P01/current/MMUSANTH/"/>
<skos:narrower rdf:resource="http://vocab.nerc.ac.uk/collection/P01/current/ACDWCF14/"/>
<skos:related rdf:resource="http://vocab.nerc.ac.uk/collection/P06/current/UUKG/"/>
<skos:broader rdf:resource="http://vocab.nerc.ac.uk/collection/P36/current/HCARBS/"/>
<void:inDataset rdf:resource="http://vocab.nerc.ac.uk/.well-known/void"/>
</skos:Concept>
</skos:member>
<skos:member>
<skos:Concept rdf:about="http://vocab.nerc.ac.uk/collection/P35/current/EPC00187/">
<dc:identifier>SDN:P35::EPC00187</dc:identifier>
<dce:identifier>SDN:P35::EPC00187</dce:identifier>
<dc:date>2016-12-12 15:20:45.0</dc:date>
<skos:notation>SDN:P35::EPC00187</skos:notation>
<skos:prefLabel xml:lang="en">Anthracene in the sediment</skos:prefLabel>
<skos:altLabel>Anthracene in the sediment</skos:altLabel>
<skos:definition xml:lang="en">Concentration of anthracene per unit dry weight of sediment (regardless of sediment size class).</skos:definition>
<owl:versionInfo>5</owl:versionInfo>
<pav:hasCurrentVersion rdf:resource="http://vocab.nerc.ac.uk/collection/P35/current/EPC00187/5/"/>
<pav:version>5</pav:version>
<pav:authoredOn>2016-12-12 15:20:45.0</pav:authoredOn>
<skos:note xml:lang="en">accepted</skos:note>
<owl:deprecated>false</owl:deprecated>
<skos:narrower rdf:resource="http://vocab.nerc.ac.uk/collection/P01/current/HDCCZN01/"/>
<skos:narrower rdf:resource="http://vocab.nerc.ac.uk/collection/P01/current/ANTDWT01/"/>
<skos:related rdf:resource="http://vocab.nerc.ac.uk/collection/P06/current/UUKG/"/>
<skos:broader rdf:resource="http://vocab.nerc.ac.uk/collection/P36/current/HCARBS/"/>
<void:inDataset rdf:resource="http://vocab.nerc.ac.uk/.well-known/void"/>
</skos:Concept>
</skos:member>
<skos:member>
<skos:Concept rdf:about="http://vocab.nerc.ac.uk/collection/P35/current/EPC00109/">
<dc:identifier>SDN:P35::EPC00109</dc:identifier>
<dce:identifier>SDN:P35::EPC00109</dce:identifier>
<dc:date>2016-10-20 11:27:18.0</dc:date>
<skos:notation>SDN:P35::EPC00109</skos:notation>
<skos:prefLabel xml:lang="en">Arsenic per unit dry weight of sediment</skos:prefLabel>
<skos:altLabel>As sediment</skos:altLabel>
<skos:definition xml:lang="en">Concentration of the specified metal in unit weight of the unsieved or 2mm screened dried sediment.</skos:definition>
<owl:versionInfo>3</owl:versionInfo>
<pav:hasCurrentVersion rdf:resource="http://vocab.nerc.ac.uk/collection/P35/current/EPC00109/3/"/>
<pav:version>3</pav:version>
<pav:authoredOn>2016-10-20 11:27:18.0</pav:authoredOn>
<skos:note xml:lang="en">accepted</skos:note>
<owl:deprecated>false</owl:deprecated>
<skos:narrower rdf:resource="http://vocab.nerc.ac.uk/collection/P01/current/ASCNXTXT/"/>
<skos:narrower rdf:resource="http://vocab.nerc.ac.uk/collection/P01/current/ASCNICXT/"/>
<skos:narrower rdf:resource="http://vocab.nerc.ac.uk/collection/P01/current/ASSEDBD1/"/>
<skos:narrower rdf:resource="http://vocab.nerc.ac.uk/collection/P01/current/MASSP012/"/>
<skos:related rdf:resource="http://vocab.nerc.ac.uk/collection/P06/current/UMKG/"/>
<skos:broader rdf:resource="http://vocab.nerc.ac.uk/collection/P36/current/HVYMTL/"/>
<void:inDataset rdf:resource="http://vocab.nerc.ac.uk/.well-known/void"/>
</skos:Concept>
</skos:member>
<skos:member>
<skos:Concept rdf:about="http://vocab.nerc.ac.uk/collection/P35/current/EPC00120/">
<dc:identifier>SDN:P35::EPC00120</dc:identifier>
<dce:identifier>SDN:P35::EPC00120</dce:identifier>
<dc:date>2016-10-20 11:27:18.0</dc:date>
<skos:notation>SDN:P35::EPC00120</skos:notation>
<skos:prefLabel xml:lang="en">Arsenic per unit dry weight of sediment &lt;63um</skos:prefLabel>
<skos:altLabel>As sediment &lt;63um</skos:altLabel>
<skos:definition xml:lang="en">Concentration of the specified metal in unit weight of the sediment passed through a 63 micron sieve and dried.</skos:definition>
<owl:versionInfo>3</owl:versionInfo>
<pav:hasCurrentVersion rdf:resource="http://vocab.nerc.ac.uk/collection/P35/current/EPC00120/3/"/>
<pav:version>3</pav:version>
<pav:authoredOn>2016-10-20 11:27:18.0</pav:authoredOn>
<skos:note xml:lang="en">accepted</skos:note>
<owl:deprecated>false</owl:deprecated>
<skos:narrower rdf:resource="http://vocab.nerc.ac.uk/collection/P01/current/MTSDM007/"/>
<skos:narrower rdf:resource="http://vocab.nerc.ac.uk/collection/P01/current/RWSSED33/"/>
<skos:related rdf:resource="http://vocab.nerc.ac.uk/collection/P06/current/UMKG/"/>
<skos:broader rdf:resource="http://vocab.nerc.ac.uk/collection/P36/current/HVYMTL/"/>
<void:inDataset rdf:resource="http://vocab.nerc.ac.uk/.well-known/void"/>
</skos:Concept>
</skos:member>
<skos:member>
<skos:Concept rdf:about="http://vocab.nerc.ac.uk/collection/P35/current/EPC00140/">
<dc:identifier>SDN:P35::EPC00140</dc:identifier>
<dce:identifier>SDN:P35::EPC00140</dce:identifier>
<dc:date>2018-03-20 16:58:29.0</dc:date>
<skos:notation>SDN:P35::EPC00140</skos:notation>
<skos:prefLabel xml:lang="en">Benzo(a)pyrene in Mytilus</skos:prefLabel>
<skos:altLabel>Benzo(a)pyrene in Mytilus</skos:altLabel>
<skos:definition xml:lang="en">Concentration of Benzo(a)pyrene per unit weight (dry or wet) of Mytilus spp. (regardless of Mytilus species and size class).</skos:definition>
<owl:versionInfo>6</owl:versionInfo>
<pav:hasCurrentVersion rdf:resource="http://vocab.nerc.ac.uk/collection/P35/current/EPC00140/6/"/>
<pav:version>6</pav:version>
<pav:authoredOn>2018-03-20 16:58:29.0</pav:authoredOn>
<skos:note xml:lang="en">deprecated</skos:note>
<owl:deprecated>true</owl:deprecated>
<skos:narrower rdf:resource="http://vocab.nerc.ac.uk/collection/P01/current/IFRPAH19/"/>
<skos:narrower rdf:resource="http://vocab.nerc.ac.uk/collection/P01/current/BPDWCF14/"/>
<skos:narrower rdf:resource="http://vocab.nerc.ac.uk/collection/P01/current/BPMMCF14/"/>
<skos:narrower rdf:resource="http://vocab.nerc.ac.uk/collection/P01/current/BPYW6569/"/>
<skos:related rdf:resource="http://vocab.nerc.ac.uk/collection/P06/current/UUKG/"/>
<skos:broader rdf:resource="http://vocab.nerc.ac.uk/collection/P36/current/HCARBS/"/>
<void:inDataset rdf:resource="http://vocab.nerc.ac.uk/.well-known/void"/>
</skos:Concept>
</skos:member>
<skos:member>
<skos:Concept rdf:about="http://vocab.nerc.ac.uk/collection/P35/current/EPC00171/">
<dc:identifier>SDN:P35::EPC00171</dc:identifier>
<dce:identifier>SDN:P35::EPC00171</dce:identifier>
<dc:date>2016-12-12 15:20:45.0</dc:date>
<skos:notation>SDN:P35::EPC00171</skos:notation>
<skos:prefLabel xml:lang="en">Benzo(a)pyrene in the sediment</skos:prefLabel>
<skos:altLabel>Benzo(a)pyrene in the sediment</skos:altLabel>
<skos:definition xml:lang="en">Concentration of benzo(a)pyrene per unit dry weight of sediment (regardless of sediment size class, analytical and normalization method).</skos:definition>
<owl:versionInfo>5</owl:versionInfo>
<pav:hasCurrentVersion rdf:resource="http://vocab.nerc.ac.uk/collection/P35/current/EPC00171/5/"/>
<pav:version>5</pav:version>
<pav:authoredOn>2016-12-12 15:20:45.0</pav:authoredOn>
<skos:note xml:lang="en">accepted</skos:note>
<owl:deprecated>false</owl:deprecated>
<skos:narrower rdf:resource="http://vocab.nerc.ac.uk/collection/P01/current/HDCCZAPY/"/>
<skos:narrower rdf:resource="http://vocab.nerc.ac.uk/collection/P01/current/BAPSEDBD/"/>
<skos:related rdf:resource="http://vocab.nerc.ac.uk/collection/P06/current/UUKG/"/>
<skos:broader rdf:resource="http://vocab.nerc.ac.uk/collection/P36/current/HCARBS/"/>
<void:inDataset rdf:resource="http://vocab.nerc.ac.uk/.well-known/void"/>
</skos:Concept>
</skos:member>
<skos:member>
<skos:Concept rdf:about="http://vocab.nerc.ac.uk/collection/P35/current/EPC00188/">
<dc:identifier>SDN:P35::EPC00188</dc:identifier>
<dce:identifier>SDN:P35::EPC00188</dce:identifier>
<dc:date>2018-03-20 16:58:29.0</dc:date>
<skos:notation>SDN:P35::EPC00188</skos:notation>
<skos:prefLabel xml:lang="en">Cadmium in Mytilus</skos:prefLabel>
<skos:altLabel>Cadmium in Mytilus</skos:altLabel>
<skos:definition xml:lang="en">Concentration of cadmium per unit weight (dry or wet) of Mytilus spp. (regardless of Mytilus species and size class).</skos:definition>
<owl:versionInfo>6</owl:versionInfo>
<pav:hasCurrentVersion rdf:resource="http://vocab.nerc.ac.uk/collection/P35/current/EPC00188/6/"/>
<pav:version>6</pav:version>
<pav:authoredOn>2018-03-20 16:58:29.0</pav:authoredOn>
<skos:note xml:lang="en">deprecated</skos:note>
<owl:deprecated>true</owl:deprecated>
<skos:narrower rdf:resource="http://vocab.nerc.ac.uk/collection/P01/current/XMETAL12/"/>
<skos:narrower rdf:resource="http://vocab.nerc.ac.uk/collection/P01/current/CDWW6569/"/>
<skos:narrower rdf:resource="http://vocab.nerc.ac.uk/collection/P01/current/MBTOCDM5/"/>
<skos:narrower rdf:resource="http://vocab.nerc.ac.uk/collection/P01/current/XMETAL11/"/>
<skos:narrower rdf:resource="http://vocab.nerc.ac.uk/collection/P01/current/MBTOCDM4/"/>
<skos:narrower rdf:resource="http://vocab.nerc.ac.uk/collection/P01/current/XMETAL10/"/>
<skos:narrower rdf:resource="http://vocab.nerc.ac.uk/collection/P01/current/MBTOCDM2/"/>
<skos:narrower rdf:resource="http://vocab.nerc.ac.uk/collection/P01/current/XMETAL09/"/>
<skos:narrower rdf:resource="http://vocab.nerc.ac.uk/collection/P01/current/MBTOCDM3/"/>
<skos:narrower rdf:resource="http://vocab.nerc.ac.uk/collection/P01/current/CDDWCF14/"/>
<skos:narrower rdf:resource="http://vocab.nerc.ac.uk/collection/P01/current/XMETAL01/"/>
<skos:narrower rdf:resource="http://vocab.nerc.ac.uk/collection/P01/current/XMETAL13/"/>
<skos:narrower rdf:resource="http://vocab.nerc.ac.uk/collection/P01/current/MMUSCDXX/"/>
<skos:narrower rdf:resource="http://vocab.nerc.ac.uk/collection/P01/current/MBTOCDM1/"/>
<skos:narrower rdf:resource="http://vocab.nerc.ac.uk/collection/P01/current/XMETAL08/"/>
<skos:related rdf:resource="http://vocab.nerc.ac.uk/collection/P06/current/UUKG/"/>
<skos:broader rdf:resource="http://vocab.nerc.ac.uk/collection/P36/current/HVYMTL/"/>
<void:inDataset rdf:resource="http://vocab.nerc.ac.uk/.well-known/void"/>
</skos:Concept>
</skos:member>
<skos:member>
<skos:Concept rdf:about="http://vocab.nerc.ac.uk/collection/P35/current/EPC00167/">
<dc:identifier>SDN:P35::EPC00167</dc:identifier>
<dce:identifier>SDN:P35::EPC00167</dce:identifier>
<dc:date>2018-03-20 16:58:29.0</dc:date>
<skos:notation>SDN:P35::EPC00167</skos:notation>
<skos:prefLabel xml:lang="en">Cadmium in the sediment</skos:prefLabel>
<skos:altLabel>Cadmium in the sediment</skos:altLabel>
<skos:definition xml:lang="en">Concentration of cadmium in sediment and sediment pore waters (regardless of sediment size class and analytical method).</skos:definition>
<owl:versionInfo>6</owl:versionInfo>
<pav:hasCurrentVersion rdf:resource="http://vocab.nerc.ac.uk/collection/P35/current/EPC00167/6/"/>
<pav:version>6</pav:version>
<pav:authoredOn>2018-03-20 16:58:29.0</pav:authoredOn>
<skos:note xml:lang="en">deprecated</skos:note>
<owl:deprecated>true</owl:deprecated>
<skos:narrower rdf:resource="http://vocab.nerc.ac.uk/collection/P01/current/MTSDM001/"/>
<skos:narrower rdf:resource="http://vocab.nerc.ac.uk/collection/P01/current/CDCNAAWF/"/>
<skos:narrower rdf:resource="http://vocab.nerc.ac.uk/collection/P01/current/CDCNICXT/"/>
<skos:narrower rdf:resource="http://vocab.nerc.ac.uk/collection/P01/current/CONCDS02/"/>
<skos:narrower rdf:resource="http://vocab.nerc.ac.uk/collection/P01/current/MCDSP012/"/>
<skos:narrower rdf:resource="http://vocab.nerc.ac.uk/collection/P01/current/CONCDS01/"/>
<skos:narrower rdf:resource="http://vocab.nerc.ac.uk/collection/P01/current/MTSDM005/"/>
<skos:related rdf:resource="http://vocab.nerc.ac.uk/collection/P06/current/UMKG/"/>
<skos:broader rdf:resource="http://vocab.nerc.ac.uk/collection/P36/current/HVYMTL/"/>
<void:inDataset rdf:resource="http://vocab.nerc.ac.uk/.well-known/void"/>
</skos:Concept>
</skos:member>
<skos:member>
<skos:Concept rdf:about="http://vocab.nerc.ac.uk/collection/P35/current/EPC00110/">
<dc:identifier>SDN:P35::EPC00110</dc:identifier>
<dce:identifier>SDN:P35::EPC00110</dce:identifier>
<dc:date>2016-10-20 11:27:18.0</dc:date>
<skos:notation>SDN:P35::EPC00110</skos:notation>
<skos:prefLabel xml:lang="en">Cadmium per unit dry weight of sediment</skos:prefLabel>
<skos:altLabel>Cd sediment</skos:altLabel>
<skos:definition xml:lang="en">Concentration of the specified metal in unit weight of the unsieved or 2mm screened dried sediment.</skos:definition>
<owl:versionInfo>3</owl:versionInfo>
<pav:hasCurrentVersion rdf:resource="http://vocab.nerc.ac.uk/collection/P35/current/EPC00110/3/"/>
<pav:version>3</pav:version>
<pav:authoredOn>2016-10-20 11:27:18.0</pav:authoredOn>
<skos:note xml:lang="en">accepted</skos:note>
<owl:deprecated>false</owl:deprecated>
<skos:narrower rdf:resource="http://vocab.nerc.ac.uk/collection/P01/current/CDCNICXT/"/>
<skos:narrower rdf:resource="http://vocab.nerc.ac.uk/collection/P01/current/CONCDS01/"/>
<skos:narrower rdf:resource="http://vocab.nerc.ac.uk/collection/P01/current/MCDSP012/"/>
<skos:related rdf:resource="http://vocab.nerc.ac.uk/collection/P06/current/UMKG/"/>
<skos:broader rdf:resource="http://vocab.nerc.ac.uk/collection/P36/current/HVYMTL/"/>
<void:inDataset rdf:resource="http://vocab.nerc.ac.uk/.well-known/void"/>
</skos:Concept>
</skos:member>
<skos:member>
<skos:Concept rdf:about="http://vocab.nerc.ac.uk/collection/P35/current/EPC00121/">
<dc:identifier>SDN:P35::EPC00121</dc:identifier>
<dce:identifier>SDN:P35::EPC00121</dce:identifier>
<dc:date>2016-10-20 11:27:18.0</dc:date>
<skos:notation>SDN:P35::EPC00121</skos:notation>
<skos:prefLabel xml:lang="en">Cadmium per unit dry weight of sediment &lt;63um</skos:prefLabel>
<skos:altLabel>Cd sediment &lt;63um</skos:altLabel>
<skos:definition xml:lang="en">Concentration of the specified metal in unit weight of the sediment passed through a 63 micron sieve and dried.</skos:definition>
<owl:versionInfo>3</owl:versionInfo>
<pav:hasCurrentVersion rdf:resource="http://vocab.nerc.ac.uk/collection/P35/current/EPC00121/3/"/>
<pav:version>3</pav:version>
<pav:authoredOn>2016-10-20 11:27:18.0</pav:authoredOn>
<skos:note xml:lang="en">accepted</skos:note>
<owl:deprecated>false</owl:deprecated>
<skos:narrower rdf:resource="http://vocab.nerc.ac.uk/collection/P01/current/CONCDS02/"/>
<skos:narrower rdf:resource="http://vocab.nerc.ac.uk/collection/P01/current/CDCNAAWF/"/>
<skos:narrower rdf:resource="http://vocab.nerc.ac.uk/collection/P01/current/MTSDM001/"/>
<skos:related rdf:resource="http://vocab.nerc.ac.uk/collection/P06/current/UMKG/"/>
<skos:broader rdf:resource="http://vocab.nerc.ac.uk/collection/P36/current/HVYMTL/"/>
<void:inDataset rdf:resource="http://vocab.nerc.ac.uk/.well-known/void"/>
</skos:Concept>
</skos:member>
<skos:member>
<skos:Concept rdf:about="http://vocab.nerc.ac.uk/collection/P35/current/EPC00177/">
<dc:identifier>SDN:P35::EPC00177</dc:identifier>
<dce:identifier>SDN:P35::EPC00177</dce:identifier>
<dc:date>2016-12-12 15:20:45.0</dc:date>
<skos:notation>SDN:P35::EPC00177</skos:notation>
<skos:prefLabel xml:lang="en">Caesium-137 in the sediment</skos:prefLabel>
<skos:altLabel>Caesium-137 in the sediment</skos:altLabel>
<skos:definition xml:lang="en">Activity of caesium-137 per unit dry weight of sediment.</skos:definition>
<owl:versionInfo>5</owl:versionInfo>
<pav:hasCurrentVersion rdf:resource="http://vocab.nerc.ac.uk/collection/P35/current/EPC00177/5/"/>
<pav:version>5</pav:version>
<pav:authoredOn>2016-12-12 15:20:45.0</pav:authoredOn>
<skos:note xml:lang="en">accepted</skos:note>
<owl:deprecated>false</owl:deprecated>
<skos:narrower rdf:resource="http://vocab.nerc.ac.uk/collection/P01/current/C37CGSXT/"/>
<skos:related rdf:resource="http://vocab.nerc.ac.uk/collection/P06/current/UBQK/"/>
<skos:broader rdf:resource="http://vocab.nerc.ac.uk/collection/P36/current/RADNUC/"/>
<void:inDataset rdf:resource="http://vocab.nerc.ac.uk/.well-known/void"/>
</skos:Concept>
</skos:member>
<skos:member>
<skos:Concept rdf:about="http://vocab.nerc.ac.uk/collection/P35/current/EPC00113/">
<dc:identifier>SDN:P35::EPC00113</dc:identifier>
<dce:identifier>SDN:P35::EPC00113</dce:identifier>
<dc:date>2016-10-20 11:27:18.0</dc:date>
<skos:notation>SDN:P35::EPC00113</skos:notation>
<skos:prefLabel xml:lang="en">Chromium per unit dry weight of sediment</skos:prefLabel>
<skos:altLabel>Cr sediment</skos:altLabel>
<skos:definition xml:lang="en">Concentration of the specified metal in unit weight of the unsieved or 2mm screened dried sediment.</skos:definition>
<owl:versionInfo>3</owl:versionInfo>
<pav:hasCurrentVersion rdf:resource="http://vocab.nerc.ac.uk/collection/P35/current/EPC00113/3/"/>
<pav:version>3</pav:version>
<pav:authoredOn>2016-10-20 11:27:18.0</pav:authoredOn>
<skos:note xml:lang="en">accepted</skos:note>
<owl:deprecated>false</owl:deprecated>
<skos:narrower rdf:resource="http://vocab.nerc.ac.uk/collection/P01/current/CRCNICXT/"/>
<skos:narrower rdf:resource="http://vocab.nerc.ac.uk/collection/P01/current/MCRSP012/"/>
<skos:narrower rdf:resource="http://vocab.nerc.ac.uk/collection/P01/current/CRSEDBD1/"/>
<skos:narrower rdf:resource="http://vocab.nerc.ac.uk/collection/P01/current/CRCNXTXT/"/>
<skos:narrower rdf:resource="http://vocab.nerc.ac.uk/collection/P01/current/CRCNPEXT/"/>
<skos:related rdf:resource="http://vocab.nerc.ac.uk/collection/P06/current/UMKG/"/>
<skos:broader rdf:resource="http://vocab.nerc.ac.uk/collection/P36/current/HVYMTL/"/>
<void:inDataset rdf:resource="http://vocab.nerc.ac.uk/.well-known/void"/>
</skos:Concept>
</skos:member>
<skos:member>
<skos:Concept rdf:about="http://vocab.nerc.ac.uk/collection/P35/current/EPC00122/">
<dc:identifier>SDN:P35::EPC00122</dc:identifier>
<dce:identifier>SDN:P35::EPC00122</dce:identifier>
<dc:date>2016-10-20 11:27:18.0</dc:date>
<skos:notation>SDN:P35::EPC00122</skos:notation>
<skos:prefLabel xml:lang="en">Chromium per unit dry weight of sediment &lt;63um</skos:prefLabel>
<skos:altLabel>Cr sediment &lt;63um</skos:altLabel>
<skos:definition xml:lang="en">Concentration of the specified metal in unit weight of the sediment passed through a 63 micron sieve and dried.</skos:definition>
<owl:versionInfo>3</owl:versionInfo>
<pav:hasCurrentVersion rdf:resource="http://vocab.nerc.ac.uk/collection/P35/current/EPC00122/3/"/>
<pav:version>3</pav:version>
<pav:authoredOn>2016-10-20 11:27:18.0</pav:authoredOn>
<skos:note xml:lang="en">accepted</skos:note>
<owl:deprecated>false</owl:deprecated>
<skos:narrower rdf:resource="http://vocab.nerc.ac.uk/collection/P01/current/CRCNAAWF/"/>
<skos:narrower rdf:resource="http://vocab.nerc.ac.uk/collection/P01/current/MTSDM002/"/>
<skos:narrower rdf:resource="http://vocab.nerc.ac.uk/collection/P01/current/RWSSED29/"/>
<skos:related rdf:resource="http://vocab.nerc.ac.uk/collection/P06/current/UMKG/"/>
<skos:broader rdf:resource="http://vocab.nerc.ac.uk/collection/P36/current/HVYMTL/"/>
<void:inDataset rdf:resource="http://vocab.nerc.ac.uk/.well-known/void"/>
</skos:Concept>
</skos:member>
<skos:member>
<skos:Concept rdf:about="http://vocab.nerc.ac.uk/collection/P35/current/EPC00111/">
<dc:identifier>SDN:P35::EPC00111</dc:identifier>
<dce:identifier>SDN:P35::EPC00111</dce:identifier>
<dc:date>2016-10-20 11:27:18.0</dc:date>
<skos:notation>SDN:P35::EPC00111</skos:notation>
<skos:prefLabel xml:lang="en">Cobalt per unit dry weight of sediment</skos:prefLabel>
<skos:altLabel>Co sediment</skos:altLabel>
<skos:definition xml:lang="en">Concentration of the specified metal in unit weight of the unsieved or 2mm screened dried sediment.</skos:definition>
<owl:versionInfo>3</owl:versionInfo>
<pav:hasCurrentVersion rdf:resource="http://vocab.nerc.ac.uk/collection/P35/current/EPC00111/3/"/>
<pav:version>3</pav:version>
<pav:authoredOn>2016-10-20 11:27:18.0</pav:authoredOn>
<skos:note xml:lang="en">accepted</skos:note>
<owl:deprecated>false</owl:deprecated>
<skos:narrower rdf:resource="http://vocab.nerc.ac.uk/collection/P01/current/MCOSP012/"/>
<skos:narrower rdf:resource="http://vocab.nerc.ac.uk/collection/P01/current/COSEDBD1/"/>
<skos:narrower rdf:resource="http://vocab.nerc.ac.uk/collection/P01/current/COCNPEXT/"/>
<skos:narrower rdf:resource="http://vocab.nerc.ac.uk/collection/P01/current/COCNICXT/"/>
<skos:related rdf:resource="http://vocab.nerc.ac.uk/collection/P06/current/UMKG/"/>
<skos:broader rdf:resource="http://vocab.nerc.ac.uk/collection/P36/current/HVYMTL/"/>
<void:inDataset rdf:resource="http://vocab.nerc.ac.uk/.well-known/void"/>
</skos:Concept>
</skos:member>
<skos:member>
<skos:Concept rdf:about="http://vocab.nerc.ac.uk/collection/P35/current/EPC00123/">
<dc:identifier>SDN:P35::EPC00123</dc:identifier>
<dce:identifier>SDN:P35::EPC00123</dce:identifier>
<dc:date>2016-10-20 11:27:18.0</dc:date>
<skos:notation>SDN:P35::EPC00123</skos:notation>
<skos:prefLabel xml:lang="en">Cobalt per unit dry weight of sediment &lt;63um</skos:prefLabel>
<skos:altLabel>Co sediment &lt;63um</skos:altLabel>
<skos:definition xml:lang="en">Concentration of the specified metal in unit weight of the sediment passed through a 63 micron sieve and dried.</skos:definition>
<owl:versionInfo>3</owl:versionInfo>
<pav:hasCurrentVersion rdf:resource="http://vocab.nerc.ac.uk/collection/P35/current/EPC00123/3/"/>
<pav:version>3</pav:version>
<pav:authoredOn>2016-10-20 11:27:18.0</pav:authoredOn>
<skos:note xml:lang="en">accepted</skos:note>
<owl:deprecated>false</owl:deprecated>
<skos:narrower rdf:resource="http://vocab.nerc.ac.uk/collection/P01/current/COCNAAWF/"/>
<skos:narrower rdf:resource="http://vocab.nerc.ac.uk/collection/P01/current/RWSSED36/"/>
<skos:related rdf:resource="http://vocab.nerc.ac.uk/collection/P06/current/UMKG/"/>
<skos:broader rdf:resource="http://vocab.nerc.ac.uk/collection/P36/current/HVYMTL/"/>
<void:inDataset rdf:resource="http://vocab.nerc.ac.uk/.well-known/void"/>
</skos:Concept>
</skos:member>
<skos:member>
<skos:Concept rdf:about="http://vocab.nerc.ac.uk/collection/P35/current/EPC00143/">
<dc:identifier>SDN:P35::EPC00143</dc:identifier>
<dce:identifier>SDN:P35::EPC00143</dce:identifier>
<dc:date>2018-03-20 16:58:29.0</dc:date>
<skos:notation>SDN:P35::EPC00143</skos:notation>
<skos:prefLabel xml:lang="en">Copper in Mytilus</skos:prefLabel>
<skos:altLabel>Copper in Mytilus</skos:altLabel>
<skos:definition xml:lang="en">Concentration of copper per unit weight (dry or wet) of Mytilus spp. (regardless of Mytilus species and size class).</skos:definition>
<owl:versionInfo>6</owl:versionInfo>
<pav:hasCurrentVersion rdf:resource="http://vocab.nerc.ac.uk/collection/P35/current/EPC00143/6/"/>
<pav:version>6</pav:version>
<pav:authoredOn>2018-03-20 16:58:29.0</pav:authoredOn>
<skos:note xml:lang="en">deprecated</skos:note>
<owl:deprecated>true</owl:deprecated>
<skos:narrower rdf:resource="http://vocab.nerc.ac.uk/collection/P01/current/IFRMET21/"/>
<skos:narrower rdf:resource="http://vocab.nerc.ac.uk/collection/P01/current/CF002DME/"/>
<skos:narrower rdf:resource="http://vocab.nerc.ac.uk/collection/P01/current/CUWW6569/"/>
<skos:related rdf:resource="http://vocab.nerc.ac.uk/collection/P06/current/UUKG/"/>
<skos:broader rdf:resource="http://vocab.nerc.ac.uk/collection/P36/current/HVYMTL/"/>
<void:inDataset rdf:resource="http://vocab.nerc.ac.uk/.well-known/void"/>
</skos:Concept>
</skos:member>
<skos:member>
<skos:Concept rdf:about="http://vocab.nerc.ac.uk/collection/P35/current/EPC00144/">
<dc:identifier>SDN:P35::EPC00144</dc:identifier>
<dce:identifier>SDN:P35::EPC00144</dce:identifier>
<dc:date>2018-03-20 16:58:29.0</dc:date>
<skos:notation>SDN:P35::EPC00144</skos:notation>
<skos:prefLabel xml:lang="en">Copper in the sediment</skos:prefLabel>
<skos:altLabel>Copper in the sediment</skos:altLabel>
<skos:definition xml:lang="en">Concentration of copper in sediment and sediment pore waters (regardless of sediment size class and analytical method).</skos:definition>
<owl:versionInfo>6</owl:versionInfo>
<pav:hasCurrentVersion rdf:resource="http://vocab.nerc.ac.uk/collection/P35/current/EPC00144/6/"/>
<pav:version>6</pav:version>
<pav:authoredOn>2018-03-20 16:58:29.0</pav:authoredOn>
<skos:note xml:lang="en">deprecated</skos:note>
<owl:deprecated>true</owl:deprecated>
<skos:narrower rdf:resource="http://vocab.nerc.ac.uk/collection/P01/current/MCUSP012/"/>
<skos:narrower rdf:resource="http://vocab.nerc.ac.uk/collection/P01/current/CUSEDBD1/"/>
<skos:narrower rdf:resource="http://vocab.nerc.ac.uk/collection/P01/current/RWSSED30/"/>
<skos:narrower rdf:resource="http://vocab.nerc.ac.uk/collection/P01/current/CUCNAAWF/"/>
<skos:narrower rdf:resource="http://vocab.nerc.ac.uk/collection/P01/current/CUCNSTXT/"/>
<skos:narrower rdf:resource="http://vocab.nerc.ac.uk/collection/P01/current/CUCNXTXT/"/>
<skos:narrower rdf:resource="http://vocab.nerc.ac.uk/collection/P01/current/CUCNICXT/"/>
<skos:narrower rdf:resource="http://vocab.nerc.ac.uk/collection/P01/current/MTSDM003/"/>
<skos:narrower rdf:resource="http://vocab.nerc.ac.uk/collection/P01/current/CUCNPEXT/"/>
<skos:related rdf:resource="http://vocab.nerc.ac.uk/collection/P06/current/UMKG/"/>
<skos:broader rdf:resource="http://vocab.nerc.ac.uk/collection/P36/current/HVYMTL/"/>
<void:inDataset rdf:resource="http://vocab.nerc.ac.uk/.well-known/void"/>
</skos:Concept>
</skos:member>
<skos:member>
<skos:Concept rdf:about="http://vocab.nerc.ac.uk/collection/P35/current/EPC00112/">
<dc:identifier>SDN:P35::EPC00112</dc:identifier>
<dce:identifier>SDN:P35::EPC00112</dce:identifier>
<dc:date>2016-10-20 11:27:18.0</dc:date>
<skos:notation>SDN:P35::EPC00112</skos:notation>
<skos:prefLabel xml:lang="en">Copper per unit dry weight of sediment</skos:prefLabel>
<skos:altLabel>Cu sediment</skos:altLabel>
<skos:definition xml:lang="en">Concentration of the specified metal in unit weight of the unsieved or 2mm screened dried sediment.</skos:definition>
<owl:versionInfo>3</owl:versionInfo>
<pav:hasCurrentVersion rdf:resource="http://vocab.nerc.ac.uk/collection/P35/current/EPC00112/3/"/>
<pav:version>3</pav:version>
<pav:authoredOn>2016-10-20 11:27:18.0</pav:authoredOn>
<skos:note xml:lang="en">accepted</skos:note>
<owl:deprecated>false</owl:deprecated>
<skos:narrower rdf:resource="http://vocab.nerc.ac.uk/collection/P01/current/MCUSP012/"/>
<skos:narrower rdf:resource="http://vocab.nerc.ac.uk/collection/P01/current/CUSEDBD1/"/>
<skos:narrower rdf:resource="http://vocab.nerc.ac.uk/collection/P01/current/CUCNXTXT/"/>
<skos:narrower rdf:resource="http://vocab.nerc.ac.uk/collection/P01/current/CUCNSTXT/"/>
<skos:narrower rdf:resource="http://vocab.nerc.ac.uk/collection/P01/current/CUCNPEXT/"/>
<skos:narrower rdf:resource="http://vocab.nerc.ac.uk/collection/P01/current/CUCNICXT/"/>
<skos:related rdf:resource="http://vocab.nerc.ac.uk/collection/P06/current/UMKG/"/>
<skos:broader rdf:resource="http://vocab.nerc.ac.uk/collection/P36/current/HVYMTL/"/>
<void:inDataset rdf:resource="http://vocab.nerc.ac.uk/.well-known/void"/>
</skos:Concept>
</skos:member>
<skos:member>
<skos:Concept rdf:about="http://vocab.nerc.ac.uk/collection/P35/current/EPC00124/">
<dc:identifier>SDN:P35::EPC00124</dc:identifier>
<dce:identifier>SDN:P35::EPC00124</dce:identifier>
<dc:date>2016-10-20 11:27:18.0</dc:date>
<skos:notation>SDN:P35::EPC00124</skos:notation>
<skos:prefLabel xml:lang="en">Copper per unit dry weight of sediment &lt;63um</skos:prefLabel>
<skos:altLabel>Cu sediment &lt;63um</skos:altLabel>
<skos:definition xml:lang="en">Concentration of the specified metal in unit weight of the sediment passed through a 63 micron sieve and dried.</skos:definition>
<owl:versionInfo>3</owl:versionInfo>
<pav:hasCurrentVersion rdf:resource="http://vocab.nerc.ac.uk/collection/P35/current/EPC00124/3/"/>
<pav:version>3</pav:version>
<pav:authoredOn>2016-10-20 11:27:18.0</pav:authoredOn>
<skos:note xml:lang="en">accepted</skos:note>
<owl:deprecated>false</owl:deprecated>
<skos:narrower rdf:resource="http://vocab.nerc.ac.uk/collection/P01/current/MTSDM003/"/>
<skos:narrower rdf:resource="http://vocab.nerc.ac.uk/collection/P01/current/CUCNAAWF/"/>
<skos:narrower rdf:resource="http://vocab.nerc.ac.uk/collection/P01/current/RWSSED30/"/>
<skos:related rdf:resource="http://vocab.nerc.ac.uk/collection/P06/current/UMKG/"/>
<skos:broader rdf:resource="http://vocab.nerc.ac.uk/collection/P36/current/HVYMTL/"/>
<void:inDataset rdf:resource="http://vocab.nerc.ac.uk/.well-known/void"/>
</skos:Concept>
</skos:member>
<skos:member>
<skos:Concept rdf:about="http://vocab.nerc.ac.uk/collection/P35/current/EPC00161/">
<dc:identifier>SDN:P35::EPC00161</dc:identifier>
<dce:identifier>SDN:P35::EPC00161</dce:identifier>
<dc:date>2018-03-20 16:58:29.0</dc:date>
<skos:notation>SDN:P35::EPC00161</skos:notation>
<skos:prefLabel xml:lang="en">Fluoranthene in Mytilus</skos:prefLabel>
<skos:altLabel>Fluoranthene in Mytilus</skos:altLabel>
<skos:definition xml:lang="en">Concentration of fluoranthene per unit weight (dry or wet) of Mytilus spp. (regardless of Mytilus species and size class).</skos:definition>
<owl:versionInfo>6</owl:versionInfo>
<pav:hasCurrentVersion rdf:resource="http://vocab.nerc.ac.uk/collection/P35/current/EPC00161/6/"/>
<pav:version>6</pav:version>
<pav:authoredOn>2018-03-20 16:58:29.0</pav:authoredOn>
<skos:note xml:lang="en">deprecated</skos:note>
<owl:deprecated>true</owl:deprecated>
<skos:narrower rdf:resource="http://vocab.nerc.ac.uk/collection/P01/current/FLDW6569/"/>
<skos:narrower rdf:resource="http://vocab.nerc.ac.uk/collection/P01/current/FAMMCF14/"/>
<skos:narrower rdf:resource="http://vocab.nerc.ac.uk/collection/P01/current/FADWCF14/"/>
<skos:narrower rdf:resource="http://vocab.nerc.ac.uk/collection/P01/current/FLWW6569/"/>
<skos:related rdf:resource="http://vocab.nerc.ac.uk/collection/P06/current/UUKG/"/>
<skos:broader rdf:resource="http://vocab.nerc.ac.uk/collection/P36/current/HCARBS/"/>
<void:inDataset rdf:resource="http://vocab.nerc.ac.uk/.well-known/void"/>
</skos:Concept>
</skos:member>
<skos:member>
<skos:Concept rdf:about="http://vocab.nerc.ac.uk/collection/P35/current/EPC00162/">
<dc:identifier>SDN:P35::EPC00162</dc:identifier>
<dce:identifier>SDN:P35::EPC00162</dce:identifier>
<dc:date>2016-12-12 15:20:45.0</dc:date>
<skos:notation>SDN:P35::EPC00162</skos:notation>
<skos:prefLabel xml:lang="en">Fluoranthene in the sediment</skos:prefLabel>
<skos:altLabel>Fluoranthene in the sediment</skos:altLabel>
<skos:definition xml:lang="en">Concentration of fluoranthene per unit dry weight of sediment (regardless of sediment size class).</skos:definition>
<owl:versionInfo>5</owl:versionInfo>
<pav:hasCurrentVersion rdf:resource="http://vocab.nerc.ac.uk/collection/P35/current/EPC00162/5/"/>
<pav:version>5</pav:version>
<pav:authoredOn>2016-12-12 15:20:45.0</pav:authoredOn>
<skos:note xml:lang="en">accepted</skos:note>
<owl:deprecated>false</owl:deprecated>
<skos:narrower rdf:resource="http://vocab.nerc.ac.uk/collection/P01/current/FLUSED01/"/>
<skos:narrower rdf:resource="http://vocab.nerc.ac.uk/collection/P01/current/FLXXSD01/"/>
<skos:related rdf:resource="http://vocab.nerc.ac.uk/collection/P06/current/UUKG/"/>
<skos:broader rdf:resource="http://vocab.nerc.ac.uk/collection/P36/current/HCARBS/"/>
<void:inDataset rdf:resource="http://vocab.nerc.ac.uk/.well-known/void"/>
</skos:Concept>
</skos:member>
<skos:member>
<skos:Concept rdf:about="http://vocab.nerc.ac.uk/collection/P35/current/EPC00207/">
<dc:identifier>SDN:P35::EPC00207</dc:identifier>
<dce:identifier>SDN:P35::EPC00207</dce:identifier>
<dc:date>2018-03-20 16:58:29.0</dc:date>
<skos:notation>SDN:P35::EPC00207</skos:notation>
<skos:prefLabel xml:lang="en">Hexachlorobenzene {HCB} in Mytilus</skos:prefLabel>
<skos:altLabel>Hexachlorobenzene {HCB} in Mytilus</skos:altLabel>
<skos:definition xml:lang="en">Concentration of hexachlorobenzene per unit weight (dry or wet) of Mytilus spp. (regardless of Mytilus species and size class).</skos:definition>
<owl:versionInfo>6</owl:versionInfo>
<pav:hasCurrentVersion rdf:resource="http://vocab.nerc.ac.uk/collection/P35/current/EPC00207/6/"/>
<pav:version>6</pav:version>
<pav:authoredOn>2018-03-20 16:58:29.0</pav:authoredOn>
<skos:note xml:lang="en">deprecated</skos:note>
<owl:deprecated>true</owl:deprecated>
<skos:narrower rdf:resource="http://vocab.nerc.ac.uk/collection/P01/current/HCBWCF14/"/>
<skos:narrower rdf:resource="http://vocab.nerc.ac.uk/collection/P01/current/HDCBME05/"/>
<skos:narrower rdf:resource="http://vocab.nerc.ac.uk/collection/P01/current/HDCBME04/"/>
<skos:narrower rdf:resource="http://vocab.nerc.ac.uk/collection/P01/current/HDCBME03/"/>
<skos:narrower rdf:resource="http://vocab.nerc.ac.uk/collection/P01/current/HCBW6569/"/>
<skos:narrower rdf:resource="http://vocab.nerc.ac.uk/collection/P01/current/HDCBME01/"/>
<skos:narrower rdf:resource="http://vocab.nerc.ac.uk/collection/P01/current/HDCBME02/"/>
<skos:narrower rdf:resource="http://vocab.nerc.ac.uk/collection/P01/current/MMUSHCBX/"/>
<skos:narrower rdf:resource="http://vocab.nerc.ac.uk/collection/P01/current/CBIOM020/"/>
<skos:related rdf:resource="http://vocab.nerc.ac.uk/collection/P06/current/UUKG/"/>
<skos:broader rdf:resource="http://vocab.nerc.ac.uk/collection/P36/current/PESTBI/"/>
<void:inDataset rdf:resource="http://vocab.nerc.ac.uk/.well-known/void"/>
</skos:Concept>
</skos:member>
<skos:member>
<skos:Concept rdf:about="http://vocab.nerc.ac.uk/collection/P35/current/EPC00208/">
<dc:identifier>SDN:P35::EPC00208</dc:identifier>
<dce:identifier>SDN:P35::EPC00208</dce:identifier>
<dc:date>2016-12-12 15:20:45.0</dc:date>
<skos:notation>SDN:P35::EPC00208</skos:notation>
<skos:prefLabel xml:lang="en">Hexachlorobenzene {HCB} in the sediment</skos:prefLabel>
<skos:altLabel>Hexachlorobenzene {HCB} in the sediment</skos:altLabel>
<skos:definition xml:lang="en">Concentration of hexachlorobenzene per unit dry weight of sediment (regardless of sediment size class).</skos:definition>
<owl:versionInfo>5</owl:versionInfo>
<pav:hasCurrentVersion rdf:resource="http://vocab.nerc.ac.uk/collection/P35/current/EPC00208/5/"/>
<pav:version>5</pav:version>
<pav:authoredOn>2016-12-12 15:20:45.0</pav:authoredOn>
<skos:note xml:lang="en">accepted</skos:note>
<owl:deprecated>false</owl:deprecated>
<skos:narrower rdf:resource="http://vocab.nerc.ac.uk/collection/P01/current/HXCLBSED/"/>
<skos:related rdf:resource="http://vocab.nerc.ac.uk/collection/P06/current/UUKG/"/>
<skos:broader rdf:resource="http://vocab.nerc.ac.uk/collection/P36/current/PESTBI/"/>
<void:inDataset rdf:resource="http://vocab.nerc.ac.uk/.well-known/void"/>
</skos:Concept>
</skos:member>
<skos:member>
<skos:Concept rdf:about="http://vocab.nerc.ac.uk/collection/P35/current/WATERTEMP/">
<dc:identifier>SDN:P35::WATERTEMP</dc:identifier>
<dce:identifier>SDN:P35::WATERTEMP</dce:identifier>
<dc:date>2016-10-20 11:27:18.0</dc:date>
<skos:notation>SDN:P35::WATERTEMP</skos:notation>
<skos:prefLabel xml:lang="en">ITS-90 water temperature</skos:prefLabel>
<skos:altLabel>ITS-90 temperature</skos:altLabel>
<skos:definition xml:lang="en">All measures of the temperature of any water body by any method. Includes P01 codes that are either explicitly labelled ITS-90 or have no explicit temperature scale label. Additional filters such as collection date will be required to be certain IPTS-68 data are excluded from the aggregation.</skos:definition>
<owl:versionInfo>4</owl:versionInfo>
<pav:hasCurrentVersion rdf:resource="http://vocab.nerc.ac.uk/collection/P35/current/WATERTEMP/4/"/>
<pav:version>4</pav:version>
<pav:authoredOn>2016-10-20 11:27:18.0</pav:authoredOn>
<skos:note xml:lang="en">accepted</skos:note>
<owl:deprecated>false</owl:deprecated>
<skos:narrower rdf:resource="http://vocab.nerc.ac.uk/collection/P01/current/TEMPTC12/"/>
<skos:narrower rdf:resource="http://vocab.nerc.ac.uk/collection/P01/current/TEMPZZXX/"/>
<skos:narrower rdf:resource="http://vocab.nerc.ac.uk/collection/P01/current/TMCLCCI1/"/>
<skos:narrower rdf:resource="http://vocab.nerc.ac.uk/collection/P01/current/TMCLCCL1/"/>
<skos:narrower rdf:resource="http://vocab.nerc.ac.uk/collection/P01/current/PSSTBK01/"/>
<skos:narrower rdf:resource="http://vocab.nerc.ac.uk/collection/P01/current/PSSTTS01/"/>
<skos:narrower rdf:resource="http://vocab.nerc.ac.uk/collection/P01/current/PSSTZZ01/"/>
<skos:narrower rdf:resource="http://vocab.nerc.ac.uk/collection/P01/current/PTMATS01/"/>
<skos:narrower rdf:resource="http://vocab.nerc.ac.uk/collection/P01/current/PTMATS02/"/>
<skos:narrower rdf:resource="http://vocab.nerc.ac.uk/collection/P01/current/PTMATS03/"/>
<skos:narrower rdf:resource="http://vocab.nerc.ac.uk/collection/P01/current/PTMATS04/"/>
<skos:narrower rdf:resource="http://vocab.nerc.ac.uk/collection/P01/current/PTMATS05/"/>
<skos:narrower rdf:resource="http://vocab.nerc.ac.uk/collection/P01/current/PTMATS06/"/>
<skos:narrower rdf:resource="http://vocab.nerc.ac.uk/collection/P01/current/PTMATS07/"/>
<skos:narrower rdf:resource="http://vocab.nerc.ac.uk/collection/P01/current/PTMATS08/"/>
<skos:narrower rdf:resource="http://vocab.nerc.ac.uk/collection/P01/current/PTMATS09/"/>
<skos:narrower rdf:resource="http://vocab.nerc.ac.uk/collection/P01/current/PTMATS10/"/>
<skos:narrower rdf:resource="http://vocab.nerc.ac.uk/collection/P01/current/PTMATS11/"/>
<skos:narrower rdf:resource="http://vocab.nerc.ac.uk/collection/P01/current/PTMATS12/"/>
<skos:narrower rdf:resource="http://vocab.nerc.ac.uk/collection/P01/current/PTMATS13/"/>
<skos:narrower rdf:resource="http://vocab.nerc.ac.uk/collection/P01/current/PTMATS14/"/>
<skos:narrower rdf:resource="http://vocab.nerc.ac.uk/collection/P01/current/PTMATS15/"/>
<skos:narrower rdf:resource="http://vocab.nerc.ac.uk/collection/P01/current/PTMAZZ01/"/>
<skos:narrower rdf:resource="http://vocab.nerc.ac.uk/collection/P01/current/TEMPAPRT/"/>
<skos:narrower rdf:resource="http://vocab.nerc.ac.uk/collection/P01/current/TEMPBT01/"/>
<skos:narrower rdf:resource="http://vocab.nerc.ac.uk/collection/P01/current/TEMPCC01/"/>
<skos:narrower rdf:resource="http://vocab.nerc.ac.uk/collection/P01/current/TEMPCC02/"/>
<skos:narrower rdf:resource="http://vocab.nerc.ac.uk/collection/P01/current/TEMPCU01/"/>
<skos:narrower rdf:resource="http://vocab.nerc.ac.uk/collection/P01/current/TEMPCU02/"/>
<skos:narrower rdf:resource="http://vocab.nerc.ac.uk/collection/P01/current/TEMPDTNX/"/>
<skos:narrower rdf:resource="http://vocab.nerc.ac.uk/collection/P01/current/TEMPET01/"/>
<skos:narrower rdf:resource="http://vocab.nerc.ac.uk/collection/P01/current/TEMPHG01/"/>
<skos:narrower rdf:resource="http://vocab.nerc.ac.uk/collection/P01/current/TEMPHGNX/"/>
<skos:narrower rdf:resource="http://vocab.nerc.ac.uk/collection/P01/current/TEMPHU01/"/>
<skos:narrower rdf:resource="http://vocab.nerc.ac.uk/collection/P01/current/TEMPMC01/"/>
<skos:narrower rdf:resource="http://vocab.nerc.ac.uk/collection/P01/current/TEMPMT01/"/>
<skos:narrower rdf:resource="http://vocab.nerc.ac.uk/collection/P01/current/TEMPMV01/"/>
<skos:narrower rdf:resource="http://vocab.nerc.ac.uk/collection/P01/current/TEMPP901/"/>
<skos:narrower rdf:resource="http://vocab.nerc.ac.uk/collection/P01/current/TEMPPH01/"/>
<skos:narrower rdf:resource="http://vocab.nerc.ac.uk/collection/P01/current/TEMPPP01/"/>
<skos:narrower rdf:resource="http://vocab.nerc.ac.uk/collection/P01/current/TEMPPP02/"/>
<skos:narrower rdf:resource="http://vocab.nerc.ac.uk/collection/P01/current/TEMPPR01/"/>
<skos:narrower rdf:resource="http://vocab.nerc.ac.uk/collection/P01/current/TEMPPR02/"/>
<skos:narrower rdf:resource="http://vocab.nerc.ac.uk/collection/P01/current/TEMPPR03/"/>
<skos:narrower rdf:resource="http://vocab.nerc.ac.uk/collection/P01/current/TEMPR901/"/>
<skos:narrower rdf:resource="http://vocab.nerc.ac.uk/collection/P01/current/TEMPRTNX/"/>
<skos:narrower rdf:resource="http://vocab.nerc.ac.uk/collection/P01/current/TEMPS901/"/>
<skos:narrower rdf:resource="http://vocab.nerc.ac.uk/collection/P01/current/TEMPS902/"/>
<skos:narrower rdf:resource="http://vocab.nerc.ac.uk/collection/P01/current/TEMPSB35/"/>
<skos:narrower rdf:resource="http://vocab.nerc.ac.uk/collection/P01/current/TEMPSG01/"/>
<skos:narrower rdf:resource="http://vocab.nerc.ac.uk/collection/P01/current/TEMPST01/"/>
<skos:narrower rdf:resource="http://vocab.nerc.ac.uk/collection/P01/current/TEMPST02/"/>
<skos:narrower rdf:resource="http://vocab.nerc.ac.uk/collection/P01/current/TEMPSU01/"/>
<skos:narrower rdf:resource="http://vocab.nerc.ac.uk/collection/P01/current/TEMPSZ01/"/>
<skos:narrower rdf:resource="http://vocab.nerc.ac.uk/collection/P01/current/TEMPTB01/"/>
<skos:narrower rdf:resource="http://vocab.nerc.ac.uk/collection/P01/current/TEMPTC01/"/>
<skos:narrower rdf:resource="http://vocab.nerc.ac.uk/collection/P01/current/TEMPTC02/"/>
<skos:narrower rdf:resource="http://vocab.nerc.ac.uk/collection/P01/current/TEMPTC03/"/>
<skos:narrower rdf:resource="http://vocab.nerc.ac.uk/collection/P01/current/TEMPTC04/"/>
<skos:narrower rdf:resource="http://vocab.nerc.ac.uk/collection/P01/current/TEMPTC05/"/>
<skos:narrower rdf:resource="http://vocab.nerc.ac.uk/collection/P01/current/TEMPTC06/"/>
<skos:narrower rdf:resource="http://vocab.nerc.ac.uk/collection/P01/current/TEMPTC07/"/>
<skos:narrower rdf:resource="http://vocab.nerc.ac.uk/collection/P01/current/TEMPTC08/"/>
<skos:narrower rdf:resource="http://vocab.nerc.ac.uk/collection/P01/current/TEMPTC09/"/>
<skos:narrower rdf:resource="http://vocab.nerc.ac.uk/collection/P01/current/TEMPTC10/"/>
<skos:narrower rdf:resource="http://vocab.nerc.ac.uk/collection/P01/current/TEMPTC11/"/>
<skos:related rdf:resource="http://vocab.nerc.ac.uk/collection/P06/current/UPAA/"/>
<void:inDataset rdf:resource="http://vocab.nerc.ac.uk/.well-known/void"/>
</skos:Concept>
</skos:member>
<skos:member>
<skos:Concept rdf:about="http://vocab.nerc.ac.uk/collection/P35/current/EPC00178/">
<dc:identifier>SDN:P35::EPC00178</dc:identifier>
<dce:identifier>SDN:P35::EPC00178</dce:identifier>
<dc:date>2016-12-12 15:20:45.0</dc:date>
<skos:notation>SDN:P35::EPC00178</skos:notation>
<skos:prefLabel xml:lang="en">Inorganic carbon in the sediment</skos:prefLabel>
<skos:altLabel>Inorganic carbon in the sediment</skos:altLabel>
<skos:definition xml:lang="en">Concentration of total inorganic carbon in sediment pore water.</skos:definition>
<owl:versionInfo>5</owl:versionInfo>
<pav:hasCurrentVersion rdf:resource="http://vocab.nerc.ac.uk/collection/P35/current/EPC00178/5/"/>
<pav:version>5</pav:version>
<pav:authoredOn>2016-12-12 15:20:45.0</pav:authoredOn>
<skos:note xml:lang="en">accepted</skos:note>
<owl:deprecated>false</owl:deprecated>
<skos:narrower rdf:resource="http://vocab.nerc.ac.uk/collection/P01/current/TCO2CAPW/"/>
<skos:narrower rdf:resource="http://vocab.nerc.ac.uk/collection/P01/current/TCO2PWCL/"/>
<skos:related rdf:resource="http://vocab.nerc.ac.uk/collection/P06/current/UGKG/"/>
<skos:broader rdf:resource="http://vocab.nerc.ac.uk/collection/P36/current/ACIDIT/"/>
<void:inDataset rdf:resource="http://vocab.nerc.ac.uk/.well-known/void"/>
</skos:Concept>
</skos:member>
<skos:member>
<skos:Concept rdf:about="http://vocab.nerc.ac.uk/collection/P35/current/EPC00152/">
<dc:identifier>SDN:P35::EPC00152</dc:identifier>
<dce:identifier>SDN:P35::EPC00152</dce:identifier>
<dc:date>2016-12-12 15:20:45.0</dc:date>
<skos:notation>SDN:P35::EPC00152</skos:notation>
<skos:prefLabel xml:lang="en">Inorganic nitrogen in the sediment</skos:prefLabel>
<skos:altLabel>Inorganic nitrogen in the sediment</skos:altLabel>
<skos:definition xml:lang="en">Concentration of inorganic nitrogen per unit dry weight of sediment (regardless of sediment size class).</skos:definition>
<owl:versionInfo>7</owl:versionInfo>
<pav:hasCurrentVersion rdf:resource="http://vocab.nerc.ac.uk/collection/P35/current/EPC00152/7/"/>
<pav:version>7</pav:version>
<pav:authoredOn>2016-12-12 15:20:45.0</pav:authoredOn>
<skos:note xml:lang="en">accepted</skos:note>
<owl:deprecated>false</owl:deprecated>
<skos:narrower rdf:resource="http://vocab.nerc.ac.uk/collection/P01/current/INCNCIWF/"/>
<skos:related rdf:resource="http://vocab.nerc.ac.uk/collection/P06/current/KGUM/"/>
<skos:broader rdf:resource="http://vocab.nerc.ac.uk/collection/P36/current/FERTIL/"/>
<void:inDataset rdf:resource="http://vocab.nerc.ac.uk/.well-known/void"/>
</skos:Concept>
</skos:member>
<skos:member>
<skos:Concept rdf:about="http://vocab.nerc.ac.uk/collection/P35/current/EPC00114/">
<dc:identifier>SDN:P35::EPC00114</dc:identifier>
<dce:identifier>SDN:P35::EPC00114</dce:identifier>
<dc:date>2016-10-20 11:27:18.0</dc:date>
<skos:notation>SDN:P35::EPC00114</skos:notation>
<skos:prefLabel xml:lang="en">Iron (total chemical species) per unit dry weight of sediment</skos:prefLabel>
<skos:altLabel>Total Fe sediment</skos:altLabel>
<skos:definition xml:lang="en">Concentration of the specified metal in unit weight of the unsieved or 2mm screened dried sediment.</skos:definition>
<owl:versionInfo>3</owl:versionInfo>
<pav:hasCurrentVersion rdf:resource="http://vocab.nerc.ac.uk/collection/P35/current/EPC00114/3/"/>
<pav:version>3</pav:version>
<pav:authoredOn>2016-10-20 11:27:18.0</pav:authoredOn>
<skos:note xml:lang="en">accepted</skos:note>
<owl:deprecated>false</owl:deprecated>
<skos:narrower rdf:resource="http://vocab.nerc.ac.uk/collection/P01/current/MFESP012/"/>
<skos:narrower rdf:resource="http://vocab.nerc.ac.uk/collection/P01/current/FESEDBD1/"/>
<skos:narrower rdf:resource="http://vocab.nerc.ac.uk/collection/P01/current/FECNXMXT/"/>
<skos:narrower rdf:resource="http://vocab.nerc.ac.uk/collection/P01/current/FECNXIXT/"/>
<skos:narrower rdf:resource="http://vocab.nerc.ac.uk/collection/P01/current/FECNSTXT/"/>
<skos:narrower rdf:resource="http://vocab.nerc.ac.uk/collection/P01/current/FECNPEXT/"/>
<skos:narrower rdf:resource="http://vocab.nerc.ac.uk/collection/P01/current/FECNPEXX/"/>
<skos:related rdf:resource="http://vocab.nerc.ac.uk/collection/P06/current/UMKG/"/>
<skos:broader rdf:resource="http://vocab.nerc.ac.uk/collection/P36/current/HVYMTL/"/>
<void:inDataset rdf:resource="http://vocab.nerc.ac.uk/.well-known/void"/>
</skos:Concept>
</skos:member>
<skos:member>
<skos:Concept rdf:about="http://vocab.nerc.ac.uk/collection/P35/current/EPC00125/">
<dc:identifier>SDN:P35::EPC00125</dc:identifier>
<dce:identifier>SDN:P35::EPC00125</dce:identifier>
<dc:date>2016-10-20 11:27:18.0</dc:date>
<skos:notation>SDN:P35::EPC00125</skos:notation>
<skos:prefLabel xml:lang="en">Iron (total chemical species) per unit dry weight of sediment &lt;63um</skos:prefLabel>
<skos:altLabel>Total Fe sediment &lt;63um</skos:altLabel>
<skos:definition xml:lang="en">Concentration of the specified metal in unit weight of the sediment passed through a 63 micron sieve and dried.</skos:definition>
<owl:versionInfo>3</owl:versionInfo>
<pav:hasCurrentVersion rdf:resource="http://vocab.nerc.ac.uk/collection/P35/current/EPC00125/3/"/>
<pav:version>3</pav:version>
<pav:authoredOn>2016-10-20 11:27:18.0</pav:authoredOn>
<skos:note xml:lang="en">accepted</skos:note>
<owl:deprecated>false</owl:deprecated>
<skos:narrower rdf:resource="http://vocab.nerc.ac.uk/collection/P01/current/FECNAAWF/"/>
<skos:narrower rdf:resource="http://vocab.nerc.ac.uk/collection/P01/current/RWSSED38/"/>
<skos:related rdf:resource="http://vocab.nerc.ac.uk/collection/P06/current/UMKG/"/>
<skos:broader rdf:resource="http://vocab.nerc.ac.uk/collection/P36/current/HVYMTL/"/>
<void:inDataset rdf:resource="http://vocab.nerc.ac.uk/.well-known/void"/>
</skos:Concept>
</skos:member>
<skos:member>
<skos:Concept rdf:about="http://vocab.nerc.ac.uk/collection/P35/current/EPC00155/">
<dc:identifier>SDN:P35::EPC00155</dc:identifier>
<dce:identifier>SDN:P35::EPC00155</dce:identifier>
<dc:date>2018-03-20 16:58:29.0</dc:date>
<skos:notation>SDN:P35::EPC00155</skos:notation>
<skos:prefLabel xml:lang="en">Lead in Mytilus</skos:prefLabel>
<skos:altLabel>Lead in Mytilus</skos:altLabel>
<skos:definition xml:lang="en">Concentration of lead per unit weight (dry or wet) of Mytilus spp. (reardless of Mytilus species and size class).</skos:definition>
<owl:versionInfo>6</owl:versionInfo>
<pav:hasCurrentVersion rdf:resource="http://vocab.nerc.ac.uk/collection/P35/current/EPC00155/6/"/>
<pav:version>6</pav:version>
<pav:authoredOn>2018-03-20 16:58:29.0</pav:authoredOn>
<skos:note xml:lang="en">deprecated</skos:note>
<owl:deprecated>true</owl:deprecated>
<skos:narrower rdf:resource="http://vocab.nerc.ac.uk/collection/P01/current/MBTOFEM2/"/>
<skos:narrower rdf:resource="http://vocab.nerc.ac.uk/collection/P01/current/MMUSPBXX/"/>
<skos:narrower rdf:resource="http://vocab.nerc.ac.uk/collection/P01/current/MBTOFEM3/"/>
<skos:narrower rdf:resource="http://vocab.nerc.ac.uk/collection/P01/current/XMETAL28/"/>
<skos:narrower rdf:resource="http://vocab.nerc.ac.uk/collection/P01/current/MBTOFEM4/"/>
<skos:narrower rdf:resource="http://vocab.nerc.ac.uk/collection/P01/current/XMETAL29/"/>
<skos:narrower rdf:resource="http://vocab.nerc.ac.uk/collection/P01/current/MBTOFEM5/"/>
<skos:narrower rdf:resource="http://vocab.nerc.ac.uk/collection/P01/current/XMETAL30/"/>
<skos:narrower rdf:resource="http://vocab.nerc.ac.uk/collection/P01/current/PBWW6569/"/>
<skos:narrower rdf:resource="http://vocab.nerc.ac.uk/collection/P01/current/XMETAL27/"/>
<skos:narrower rdf:resource="http://vocab.nerc.ac.uk/collection/P01/current/MBTOFEM1/"/>
<skos:narrower rdf:resource="http://vocab.nerc.ac.uk/collection/P01/current/XMETAL26/"/>
<skos:narrower rdf:resource="http://vocab.nerc.ac.uk/collection/P01/current/PBDWCF14/"/>
<skos:narrower rdf:resource="http://vocab.nerc.ac.uk/collection/P01/current/XMETAL24/"/>
<skos:narrower rdf:resource="http://vocab.nerc.ac.uk/collection/P01/current/XMETAL31/"/>
<skos:related rdf:resource="http://vocab.nerc.ac.uk/collection/P06/current/UUKG/"/>
<skos:broader rdf:resource="http://vocab.nerc.ac.uk/collection/P36/current/HVYMTL/"/>
<void:inDataset rdf:resource="http://vocab.nerc.ac.uk/.well-known/void"/>
</skos:Concept>
</skos:member>
<skos:member>
<skos:Concept rdf:about="http://vocab.nerc.ac.uk/collection/P35/current/EPC00197/">
<dc:identifier>SDN:P35::EPC00197</dc:identifier>
<dce:identifier>SDN:P35::EPC00197</dce:identifier>
<dc:date>2018-03-20 16:58:29.0</dc:date>
<skos:notation>SDN:P35::EPC00197</skos:notation>
<skos:prefLabel xml:lang="en">Lead in the sediment</skos:prefLabel>
<skos:altLabel>Lead in the sediment</skos:altLabel>
<skos:definition xml:lang="en">Concentration of lead in sediment and sediment pore waters (regardless of sediment size class and analytical method).</skos:definition>
<owl:versionInfo>6</owl:versionInfo>
<pav:hasCurrentVersion rdf:resource="http://vocab.nerc.ac.uk/collection/P35/current/EPC00197/6/"/>
<pav:version>6</pav:version>
<pav:authoredOn>2018-03-20 16:58:29.0</pav:authoredOn>
<skos:note xml:lang="en">deprecated</skos:note>
<owl:deprecated>true</owl:deprecated>
<skos:narrower rdf:resource="http://vocab.nerc.ac.uk/collection/P01/current/MPBSP012/"/>
<skos:narrower rdf:resource="http://vocab.nerc.ac.uk/collection/P01/current/CONPBS01/"/>
<skos:narrower rdf:resource="http://vocab.nerc.ac.uk/collection/P01/current/CONPBS02/"/>
<skos:narrower rdf:resource="http://vocab.nerc.ac.uk/collection/P01/current/MTSDM004/"/>
<skos:narrower rdf:resource="http://vocab.nerc.ac.uk/collection/P01/current/PBCNAAWF/"/>
<skos:narrower rdf:resource="http://vocab.nerc.ac.uk/collection/P01/current/PBCNPEXT/"/>
<skos:narrower rdf:resource="http://vocab.nerc.ac.uk/collection/P01/current/PBCNXTXT/"/>
<skos:narrower rdf:resource="http://vocab.nerc.ac.uk/collection/P01/current/PBCNICXT/"/>
<skos:related rdf:resource="http://vocab.nerc.ac.uk/collection/P06/current/UMKG/"/>
<skos:broader rdf:resource="http://vocab.nerc.ac.uk/collection/P36/current/HVYMTL/"/>
<void:inDataset rdf:resource="http://vocab.nerc.ac.uk/.well-known/void"/>
</skos:Concept>
</skos:member>
<skos:member>
<skos:Concept rdf:about="http://vocab.nerc.ac.uk/collection/P35/current/EPC00115/">
<dc:identifier>SDN:P35::EPC00115</dc:identifier>
<dce:identifier>SDN:P35::EPC00115</dce:identifier>
<dc:date>2016-10-20 11:27:18.0</dc:date>
<skos:notation>SDN:P35::EPC00115</skos:notation>
<skos:prefLabel xml:lang="en">Lead per unit dry weight of sediment</skos:prefLabel>
<skos:altLabel>Pb sediment</skos:altLabel>
<skos:definition xml:lang="en">Concentration of the specified metal in unit weight of the unsieved or 2mm screened dried sediment.</skos:definition>
<owl:versionInfo>3</owl:versionInfo>
<pav:hasCurrentVersion rdf:resource="http://vocab.nerc.ac.uk/collection/P35/current/EPC00115/3/"/>
<pav:version>3</pav:version>
<pav:authoredOn>2016-10-20 11:27:18.0</pav:authoredOn>
<skos:note xml:lang="en">accepted</skos:note>
<owl:deprecated>false</owl:deprecated>
<skos:narrower rdf:resource="http://vocab.nerc.ac.uk/collection/P01/current/CONPBS01/"/>
<skos:narrower rdf:resource="http://vocab.nerc.ac.uk/collection/P01/current/MPBSP012/"/>
<skos:narrower rdf:resource="http://vocab.nerc.ac.uk/collection/P01/current/PBCNPEXT/"/>
<skos:narrower rdf:resource="http://vocab.nerc.ac.uk/collection/P01/current/PBCNICXT/"/>
<skos:narrower rdf:resource="http://vocab.nerc.ac.uk/collection/P01/current/PBCNXTXT/"/>
<skos:related rdf:resource="http://vocab.nerc.ac.uk/collection/P06/current/UMKG/"/>
<skos:broader rdf:resource="http://vocab.nerc.ac.uk/collection/P36/current/HVYMTL/"/>
<void:inDataset rdf:resource="http://vocab.nerc.ac.uk/.well-known/void"/>
</skos:Concept>
</skos:member>
<skos:member>
<skos:Concept rdf:about="http://vocab.nerc.ac.uk/collection/P35/current/EPC00126/">
<dc:identifier>SDN:P35::EPC00126</dc:identifier>
<dce:identifier>SDN:P35::EPC00126</dce:identifier>
<dc:date>2016-10-20 11:27:18.0</dc:date>
<skos:notation>SDN:P35::EPC00126</skos:notation>
<skos:prefLabel xml:lang="en">Lead per unit dry weight of sediment &lt;63um</skos:prefLabel>
<skos:altLabel>Pb sediment &lt;63um</skos:altLabel>
<skos:definition xml:lang="en">Concentration of the specified metal in unit weight of the sediment passed through a 63 micron sieve and dried.</skos:definition>
<owl:versionInfo>3</owl:versionInfo>
<pav:hasCurrentVersion rdf:resource="http://vocab.nerc.ac.uk/collection/P35/current/EPC00126/3/"/>
<pav:version>3</pav:version>
<pav:authoredOn>2016-10-20 11:27:18.0</pav:authoredOn>
<skos:note xml:lang="en">accepted</skos:note>
<owl:deprecated>false</owl:deprecated>
<skos:narrower rdf:resource="http://vocab.nerc.ac.uk/collection/P01/current/CONPBS02/"/>
<skos:narrower rdf:resource="http://vocab.nerc.ac.uk/collection/P01/current/MTSDM004/"/>
<skos:narrower rdf:resource="http://vocab.nerc.ac.uk/collection/P01/current/PBCNAAWF/"/>
<skos:related rdf:resource="http://vocab.nerc.ac.uk/collection/P06/current/UMKG/"/>
<skos:broader rdf:resource="http://vocab.nerc.ac.uk/collection/P36/current/HVYMTL/"/>
<void:inDataset rdf:resource="http://vocab.nerc.ac.uk/.well-known/void"/>
</skos:Concept>
</skos:member>
<skos:member>
<skos:Concept rdf:about="http://vocab.nerc.ac.uk/collection/P35/current/EPC00116/">
<dc:identifier>SDN:P35::EPC00116</dc:identifier>
<dce:identifier>SDN:P35::EPC00116</dce:identifier>
<dc:date>2016-10-20 11:27:18.0</dc:date>
<skos:notation>SDN:P35::EPC00116</skos:notation>
<skos:prefLabel xml:lang="en">Manganese (total chemical species) per unit dry weight of sediment</skos:prefLabel>
<skos:altLabel>Total Mn sediment</skos:altLabel>
<skos:definition xml:lang="en">Concentration of the specified metal in unit weight of the unsieved or 2mm screened dried sediment.</skos:definition>
<owl:versionInfo>3</owl:versionInfo>
<pav:hasCurrentVersion rdf:resource="http://vocab.nerc.ac.uk/collection/P35/current/EPC00116/3/"/>
<pav:version>3</pav:version>
<pav:authoredOn>2016-10-20 11:27:18.0</pav:authoredOn>
<skos:note xml:lang="en">accepted</skos:note>
<owl:deprecated>false</owl:deprecated>
<skos:narrower rdf:resource="http://vocab.nerc.ac.uk/collection/P01/current/MNSEDBD1/"/>
<skos:narrower rdf:resource="http://vocab.nerc.ac.uk/collection/P01/current/MNCNXMXT/"/>
<skos:narrower rdf:resource="http://vocab.nerc.ac.uk/collection/P01/current/MNCNXTXT/"/>
<skos:narrower rdf:resource="http://vocab.nerc.ac.uk/collection/P01/current/MNCNSTXT/"/>
<skos:narrower rdf:resource="http://vocab.nerc.ac.uk/collection/P01/current/MMNSP012/"/>
<skos:narrower rdf:resource="http://vocab.nerc.ac.uk/collection/P01/current/MNCNPEXT/"/>
<skos:narrower rdf:resource="http://vocab.nerc.ac.uk/collection/P01/current/MNCNPEXX/"/>
<skos:related rdf:resource="http://vocab.nerc.ac.uk/collection/P06/current/UMKG/"/>
<skos:broader rdf:resource="http://vocab.nerc.ac.uk/collection/P36/current/HVYMTL/"/>
<void:inDataset rdf:resource="http://vocab.nerc.ac.uk/.well-known/void"/>
</skos:Concept>
</skos:member>
<skos:member>
<skos:Concept rdf:about="http://vocab.nerc.ac.uk/collection/P35/current/EPC00127/">
<dc:identifier>SDN:P35::EPC00127</dc:identifier>
<dce:identifier>SDN:P35::EPC00127</dce:identifier>
<dc:date>2016-10-20 11:27:18.0</dc:date>
<skos:notation>SDN:P35::EPC00127</skos:notation>
<skos:prefLabel xml:lang="en">Manganese (total chemical species) per unit dry weight of sediment &lt;63um</skos:prefLabel>
<skos:altLabel>Total Mn sediment &lt;63um</skos:altLabel>
<skos:definition xml:lang="en">Concentration of the specified metal in unit weight of the sediment passed through a 63 micron sieve and dried.</skos:definition>
<owl:versionInfo>3</owl:versionInfo>
<pav:hasCurrentVersion rdf:resource="http://vocab.nerc.ac.uk/collection/P35/current/EPC00127/3/"/>
<pav:version>3</pav:version>
<pav:authoredOn>2016-10-20 11:27:18.0</pav:authoredOn>
<skos:note xml:lang="en">accepted</skos:note>
<owl:deprecated>false</owl:deprecated>
<skos:narrower rdf:resource="http://vocab.nerc.ac.uk/collection/P01/current/MNCNAAWF/"/>
<skos:narrower rdf:resource="http://vocab.nerc.ac.uk/collection/P01/current/RWSSED37/"/>
<skos:related rdf:resource="http://vocab.nerc.ac.uk/collection/P06/current/UMKG/"/>
<skos:broader rdf:resource="http://vocab.nerc.ac.uk/collection/P36/current/HVYMTL/"/>
<void:inDataset rdf:resource="http://vocab.nerc.ac.uk/.well-known/void"/>
</skos:Concept>
</skos:member>
<skos:member>
<skos:Concept rdf:about="http://vocab.nerc.ac.uk/collection/P35/current/EPC00158/">
<dc:identifier>SDN:P35::EPC00158</dc:identifier>
<dce:identifier>SDN:P35::EPC00158</dce:identifier>
<dc:date>2016-12-12 15:20:45.0</dc:date>
<skos:notation>SDN:P35::EPC00158</skos:notation>
<skos:prefLabel xml:lang="en">Mercury (total chemical species) in the sediment</skos:prefLabel>
<skos:altLabel>Mercury (total chemical species) in the sediment</skos:altLabel>
<skos:definition xml:lang="en">Unavailable.</skos:definition>
<owl:versionInfo>6</owl:versionInfo>
<pav:hasCurrentVersion rdf:resource="http://vocab.nerc.ac.uk/collection/P35/current/EPC00158/6/"/>
<pav:version>6</pav:version>
<pav:authoredOn>2016-12-12 15:20:45.0</pav:authoredOn>
<skos:note xml:lang="en">deprecated</skos:note>
<owl:deprecated>true</owl:deprecated>
<void:inDataset rdf:resource="http://vocab.nerc.ac.uk/.well-known/void"/>
</skos:Concept>
</skos:member>
<skos:member>
<skos:Concept rdf:about="http://vocab.nerc.ac.uk/collection/P35/current/EPC00128/">
<dc:identifier>SDN:P35::EPC00128</dc:identifier>
<dce:identifier>SDN:P35::EPC00128</dce:identifier>
<dc:date>2016-10-20 11:27:18.0</dc:date>
<skos:notation>SDN:P35::EPC00128</skos:notation>
<skos:prefLabel xml:lang="en">Mercury (total chemical species) per unit dry weight of sediment &lt;63um</skos:prefLabel>
<skos:altLabel>Total Hg sediment &lt;63um</skos:altLabel>
<skos:definition xml:lang="en">Concentration of the specified metal in unit weight of the sediment passed through a 63 micron sieve and dried.</skos:definition>
<owl:versionInfo>3</owl:versionInfo>
<pav:hasCurrentVersion rdf:resource="http://vocab.nerc.ac.uk/collection/P35/current/EPC00128/3/"/>
<pav:version>3</pav:version>
<pav:authoredOn>2016-10-20 11:27:18.0</pav:authoredOn>
<skos:note xml:lang="en">accepted</skos:note>
<owl:deprecated>false</owl:deprecated>
<skos:narrower rdf:resource="http://vocab.nerc.ac.uk/collection/P01/current/CONHGS02/"/>
<skos:narrower rdf:resource="http://vocab.nerc.ac.uk/collection/P01/current/HGCNAAWF/"/>
<skos:narrower rdf:resource="http://vocab.nerc.ac.uk/collection/P01/current/MTSDM005/"/>
<skos:related rdf:resource="http://vocab.nerc.ac.uk/collection/P06/current/UMKG/"/>
<skos:broader rdf:resource="http://vocab.nerc.ac.uk/collection/P36/current/HVYMTL/"/>
<void:inDataset rdf:resource="http://vocab.nerc.ac.uk/.well-known/void"/>
</skos:Concept>
</skos:member>
<skos:member>
<skos:Concept rdf:about="http://vocab.nerc.ac.uk/collection/P35/current/EPC00189/">
<dc:identifier>SDN:P35::EPC00189</dc:identifier>
<dce:identifier>SDN:P35::EPC00189</dce:identifier>
<dc:date>2018-03-20 16:58:29.0</dc:date>
<skos:notation>SDN:P35::EPC00189</skos:notation>
<skos:prefLabel xml:lang="en">Mercury in Mytilus</skos:prefLabel>
<skos:altLabel>Mercury in Mytilus</skos:altLabel>
<skos:definition xml:lang="en">Concentration of mercury per unit weight (dry or wet) of Mytilus spp. (regardless of Mytilus species and size class).</skos:definition>
<owl:versionInfo>6</owl:versionInfo>
<pav:hasCurrentVersion rdf:resource="http://vocab.nerc.ac.uk/collection/P35/current/EPC00189/6/"/>
<pav:version>6</pav:version>
<pav:authoredOn>2018-03-20 16:58:29.0</pav:authoredOn>
<skos:note xml:lang="en">deprecated</skos:note>
<owl:deprecated>true</owl:deprecated>
<skos:narrower rdf:resource="http://vocab.nerc.ac.uk/collection/P01/current/MBTOHGM1/"/>
<skos:narrower rdf:resource="http://vocab.nerc.ac.uk/collection/P01/current/D2930561/"/>
<skos:narrower rdf:resource="http://vocab.nerc.ac.uk/collection/P01/current/XMETAL32/"/>
<skos:narrower rdf:resource="http://vocab.nerc.ac.uk/collection/P01/current/MBTOHGM2/"/>
<skos:narrower rdf:resource="http://vocab.nerc.ac.uk/collection/P01/current/MBTOHGM3/"/>
<skos:narrower rdf:resource="http://vocab.nerc.ac.uk/collection/P01/current/D2930515/"/>
<skos:narrower rdf:resource="http://vocab.nerc.ac.uk/collection/P01/current/W2930193/"/>
<skos:narrower rdf:resource="http://vocab.nerc.ac.uk/collection/P01/current/MBTOHGM5/"/>
<skos:narrower rdf:resource="http://vocab.nerc.ac.uk/collection/P01/current/MBTOHGM4/"/>
<skos:narrower rdf:resource="http://vocab.nerc.ac.uk/collection/P01/current/XMETAL33/"/>
<skos:related rdf:resource="http://vocab.nerc.ac.uk/collection/P06/current/UUKG/"/>
<skos:broader rdf:resource="http://vocab.nerc.ac.uk/collection/P36/current/HVYMTL/"/>
<void:inDataset rdf:resource="http://vocab.nerc.ac.uk/.well-known/void"/>
</skos:Concept>
</skos:member>
<skos:member>
<skos:Concept rdf:about="http://vocab.nerc.ac.uk/collection/P35/current/EPC00117/">
<dc:identifier>SDN:P35::EPC00117</dc:identifier>
<dce:identifier>SDN:P35::EPC00117</dce:identifier>
<dc:date>2018-03-28 15:20:47.0</dc:date>
<skos:notation>SDN:P35::EPC00117</skos:notation>
<skos:prefLabel xml:lang="en">Mercury per unit dry weight of sediment</skos:prefLabel>
<skos:altLabel>Hg sediment</skos:altLabel>
<skos:definition xml:lang="en">Concentration of the specified metal in unit weight of the unsieved or 2mm screened dried sediment.</skos:definition>
<owl:versionInfo>5</owl:versionInfo>
<pav:hasCurrentVersion rdf:resource="http://vocab.nerc.ac.uk/collection/P35/current/EPC00117/5/"/>
<pav:version>5</pav:version>
<pav:authoredOn>2018-03-28 15:20:47.0</pav:authoredOn>
<skos:note xml:lang="en">accepted</skos:note>
<owl:deprecated>false</owl:deprecated>
<skos:narrower rdf:resource="http://vocab.nerc.ac.uk/collection/P01/current/MHGSP012/"/>
<skos:narrower rdf:resource="http://vocab.nerc.ac.uk/collection/P01/current/HGCNCFXT/"/>
<skos:narrower rdf:resource="http://vocab.nerc.ac.uk/collection/P01/current/CONHGS01/"/>
<skos:related rdf:resource="http://vocab.nerc.ac.uk/collection/P06/current/UMKG/"/>
<skos:broader rdf:resource="http://vocab.nerc.ac.uk/collection/P36/current/HVYMTL/"/>
<void:inDataset rdf:resource="http://vocab.nerc.ac.uk/.well-known/void"/>
</skos:Concept>
</skos:member>
<skos:member>
<skos:Concept rdf:about="http://vocab.nerc.ac.uk/collection/P35/current/EPC00202/">
<dc:identifier>SDN:P35::EPC00202</dc:identifier>
<dce:identifier>SDN:P35::EPC00202</dce:identifier>
<dc:date>2018-03-20 16:58:29.0</dc:date>
<skos:notation>SDN:P35::EPC00202</skos:notation>
<skos:prefLabel xml:lang="en">Naphthalene in Mytilus</skos:prefLabel>
<skos:altLabel>Naphthalene in Mytilus</skos:altLabel>
<skos:definition xml:lang="en">Concentration of naphtalene per unit weight (dry or wet) of Mytilus spp. (regardless of Mytilus species and size class).</skos:definition>
<owl:versionInfo>6</owl:versionInfo>
<pav:hasCurrentVersion rdf:resource="http://vocab.nerc.ac.uk/collection/P35/current/EPC00202/6/"/>
<pav:version>6</pav:version>
<pav:authoredOn>2018-03-20 16:58:29.0</pav:authoredOn>
<skos:note xml:lang="en">deprecated</skos:note>
<owl:deprecated>true</owl:deprecated>
<skos:narrower rdf:resource="http://vocab.nerc.ac.uk/collection/P01/current/IFRPAH53/"/>
<skos:narrower rdf:resource="http://vocab.nerc.ac.uk/collection/P01/current/IFRPAH52/"/>
<skos:narrower rdf:resource="http://vocab.nerc.ac.uk/collection/P01/current/W2930279/"/>
<skos:narrower rdf:resource="http://vocab.nerc.ac.uk/collection/P01/current/CF101WME/"/>
<skos:related rdf:resource="http://vocab.nerc.ac.uk/collection/P06/current/UUKG/"/>
<skos:broader rdf:resource="http://vocab.nerc.ac.uk/collection/P36/current/HCARBS/"/>
<void:inDataset rdf:resource="http://vocab.nerc.ac.uk/.well-known/void"/>
</skos:Concept>
</skos:member>
<skos:member>
<skos:Concept rdf:about="http://vocab.nerc.ac.uk/collection/P35/current/EPC00214/">
<dc:identifier>SDN:P35::EPC00214</dc:identifier>
<dce:identifier>SDN:P35::EPC00214</dce:identifier>
<dc:date>2016-12-12 15:20:45.0</dc:date>
<skos:notation>SDN:P35::EPC00214</skos:notation>
<skos:prefLabel xml:lang="en">Naphthalene in the sediment</skos:prefLabel>
<skos:altLabel>Naphthalene in the sediment</skos:altLabel>
<skos:definition xml:lang="en">Concentration of napthalene per unit dry weight of sediment (regardless of sediment size class).</skos:definition>
<owl:versionInfo>5</owl:versionInfo>
<pav:hasCurrentVersion rdf:resource="http://vocab.nerc.ac.uk/collection/P35/current/EPC00214/5/"/>
<pav:version>5</pav:version>
<pav:authoredOn>2016-12-12 15:20:45.0</pav:authoredOn>
<skos:note xml:lang="en">accepted</skos:note>
<owl:deprecated>false</owl:deprecated>
<skos:narrower rdf:resource="http://vocab.nerc.ac.uk/collection/P01/current/NAPSEDXD/"/>
<skos:narrower rdf:resource="http://vocab.nerc.ac.uk/collection/P01/current/NAPSEDBD/"/>
<skos:related rdf:resource="http://vocab.nerc.ac.uk/collection/P06/current/UUKG/"/>
<skos:broader rdf:resource="http://vocab.nerc.ac.uk/collection/P36/current/HCARBS/"/>
<void:inDataset rdf:resource="http://vocab.nerc.ac.uk/.well-known/void"/>
</skos:Concept>
</skos:member>
<skos:member>
<skos:Concept rdf:about="http://vocab.nerc.ac.uk/collection/P35/current/EPC00118/">
<dc:identifier>SDN:P35::EPC00118</dc:identifier>
<dce:identifier>SDN:P35::EPC00118</dce:identifier>
<dc:date>2016-10-20 11:27:18.0</dc:date>
<skos:notation>SDN:P35::EPC00118</skos:notation>
<skos:prefLabel xml:lang="en">Nickel per unit dry weight of sediment</skos:prefLabel>
<skos:altLabel>Ni sediment</skos:altLabel>
<skos:definition xml:lang="en">Concentration of the specified metal in unit weight of the unsieved or 2mm screened dried sediment.</skos:definition>
<owl:versionInfo>3</owl:versionInfo>
<pav:hasCurrentVersion rdf:resource="http://vocab.nerc.ac.uk/collection/P35/current/EPC00118/3/"/>
<pav:version>3</pav:version>
<pav:authoredOn>2016-10-20 11:27:18.0</pav:authoredOn>
<skos:note xml:lang="en">accepted</skos:note>
<owl:deprecated>false</owl:deprecated>
<skos:narrower rdf:resource="http://vocab.nerc.ac.uk/collection/P01/current/NISEDBD1/"/>
<skos:narrower rdf:resource="http://vocab.nerc.ac.uk/collection/P01/current/NICNXTXT/"/>
<skos:narrower rdf:resource="http://vocab.nerc.ac.uk/collection/P01/current/NICNPEXT/"/>
<skos:narrower rdf:resource="http://vocab.nerc.ac.uk/collection/P01/current/NICNICXT/"/>
<skos:narrower rdf:resource="http://vocab.nerc.ac.uk/collection/P01/current/MNISP012/"/>
<skos:related rdf:resource="http://vocab.nerc.ac.uk/collection/P06/current/UMKG/"/>
<skos:broader rdf:resource="http://vocab.nerc.ac.uk/collection/P36/current/HVYMTL/"/>
<void:inDataset rdf:resource="http://vocab.nerc.ac.uk/.well-known/void"/>
</skos:Concept>
</skos:member>
<skos:member>
<skos:Concept rdf:about="http://vocab.nerc.ac.uk/collection/P35/current/EPC00129/">
<dc:identifier>SDN:P35::EPC00129</dc:identifier>
<dce:identifier>SDN:P35::EPC00129</dce:identifier>
<dc:date>2016-10-20 11:27:18.0</dc:date>
<skos:notation>SDN:P35::EPC00129</skos:notation>
<skos:prefLabel xml:lang="en">Nickel per unit dry weight of sediment &lt;63um</skos:prefLabel>
<skos:altLabel>Ni sediment &lt;63um</skos:altLabel>
<skos:definition xml:lang="en">Concentration of the specified metal in unit weight of the sediment passed through a 63 micron sieve and dried.</skos:definition>
<owl:versionInfo>3</owl:versionInfo>
<pav:hasCurrentVersion rdf:resource="http://vocab.nerc.ac.uk/collection/P35/current/EPC00129/3/"/>
<pav:version>3</pav:version>
<pav:authoredOn>2016-10-20 11:27:18.0</pav:authoredOn>
<skos:note xml:lang="en">accepted</skos:note>
<owl:deprecated>false</owl:deprecated>
<skos:narrower rdf:resource="http://vocab.nerc.ac.uk/collection/P01/current/MTSDM006/"/>
<skos:narrower rdf:resource="http://vocab.nerc.ac.uk/collection/P01/current/NICNAAWF/"/>
<skos:narrower rdf:resource="http://vocab.nerc.ac.uk/collection/P01/current/RWSSED31/"/>
<skos:related rdf:resource="http://vocab.nerc.ac.uk/collection/P06/current/UMKG/"/>
<skos:broader rdf:resource="http://vocab.nerc.ac.uk/collection/P36/current/HVYMTL/"/>
<void:inDataset rdf:resource="http://vocab.nerc.ac.uk/.well-known/void"/>
</skos:Concept>
</skos:member>
<skos:member>
<skos:Concept rdf:about="http://vocab.nerc.ac.uk/collection/P35/current/EPC00199/">
<dc:identifier>SDN:P35::EPC00199</dc:identifier>
<dce:identifier>SDN:P35::EPC00199</dce:identifier>
<dc:date>2016-12-12 15:20:45.0</dc:date>
<skos:notation>SDN:P35::EPC00199</skos:notation>
<skos:prefLabel xml:lang="en">Nitrate in the sediment</skos:prefLabel>
<skos:altLabel>Nitrate in the sediment</skos:altLabel>
<skos:definition xml:lang="en">Concentration of nitrate per unit volume of the sediment pore water.</skos:definition>
<owl:versionInfo>5</owl:versionInfo>
<pav:hasCurrentVersion rdf:resource="http://vocab.nerc.ac.uk/collection/P35/current/EPC00199/5/"/>
<pav:version>5</pav:version>
<pav:authoredOn>2016-12-12 15:20:45.0</pav:authoredOn>
<skos:note xml:lang="en">accepted</skos:note>
<owl:deprecated>false</owl:deprecated>
<skos:narrower rdf:resource="http://vocab.nerc.ac.uk/collection/P01/current/NTRAAADC/"/>
<skos:narrower rdf:resource="http://vocab.nerc.ac.uk/collection/P01/current/NTRIPWD2/"/>
<skos:related rdf:resource="http://vocab.nerc.ac.uk/collection/P06/current/KGUM/"/>
<skos:broader rdf:resource="http://vocab.nerc.ac.uk/collection/P36/current/FERTIL/"/>
<void:inDataset rdf:resource="http://vocab.nerc.ac.uk/.well-known/void"/>
</skos:Concept>
</skos:member>
<skos:member>
<skos:Concept rdf:about="http://vocab.nerc.ac.uk/collection/P35/current/EPC00139/">
<dc:identifier>SDN:P35::EPC00139</dc:identifier>
<dce:identifier>SDN:P35::EPC00139</dce:identifier>
<dc:date>2016-12-12 15:20:45.0</dc:date>
<skos:notation>SDN:P35::EPC00139</skos:notation>
<skos:prefLabel xml:lang="en">Nitrate plus nitrite in the sediment</skos:prefLabel>
<skos:altLabel>Nitrate plus nitrite in the sediment</skos:altLabel>
<skos:definition xml:lang="en">Concentration of nitrate plus nitrite per unit volume of sediment pore waters.</skos:definition>
<owl:versionInfo>6</owl:versionInfo>
<pav:hasCurrentVersion rdf:resource="http://vocab.nerc.ac.uk/collection/P35/current/EPC00139/6/"/>
<pav:version>6</pav:version>
<pav:authoredOn>2016-12-12 15:20:45.0</pav:authoredOn>
<skos:note xml:lang="en">accepted</skos:note>
<owl:deprecated>false</owl:deprecated>
<skos:narrower rdf:resource="http://vocab.nerc.ac.uk/collection/P01/current/NTRZPWD3/"/>
<skos:related rdf:resource="http://vocab.nerc.ac.uk/collection/P06/current/KGUM/"/>
<skos:broader rdf:resource="http://vocab.nerc.ac.uk/collection/P36/current/FERTIL/"/>
<void:inDataset rdf:resource="http://vocab.nerc.ac.uk/.well-known/void"/>
</skos:Concept>
</skos:member>
<skos:member>
<skos:Concept rdf:about="http://vocab.nerc.ac.uk/collection/P35/current/EPC00170/">
<dc:identifier>SDN:P35::EPC00170</dc:identifier>
<dce:identifier>SDN:P35::EPC00170</dce:identifier>
<dc:date>2016-12-12 15:20:45.0</dc:date>
<skos:notation>SDN:P35::EPC00170</skos:notation>
<skos:prefLabel xml:lang="en">Nitrogen in the sediment</skos:prefLabel>
<skos:altLabel>Nitrogen in the sediment</skos:altLabel>
<skos:definition xml:lang="en">Concentration of nitrogen per unit dry weight of sediment (regardless of sediment size class).</skos:definition>
<owl:versionInfo>5</owl:versionInfo>
<pav:hasCurrentVersion rdf:resource="http://vocab.nerc.ac.uk/collection/P35/current/EPC00170/5/"/>
<pav:version>5</pav:version>
<pav:authoredOn>2016-12-12 15:20:45.0</pav:authoredOn>
<skos:note xml:lang="en">accepted</skos:note>
<owl:deprecated>false</owl:deprecated>
<skos:narrower rdf:resource="http://vocab.nerc.ac.uk/collection/P01/current/NSEDXD01/"/>
<skos:related rdf:resource="http://vocab.nerc.ac.uk/collection/P06/current/UGKG/"/>
<skos:broader rdf:resource="http://vocab.nerc.ac.uk/collection/P36/current/FERTIL/"/>
<void:inDataset rdf:resource="http://vocab.nerc.ac.uk/.well-known/void"/>
</skos:Concept>
</skos:member>
<skos:member>
<skos:Concept rdf:about="http://vocab.nerc.ac.uk/collection/P35/current/EPC00173/">
<dc:identifier>SDN:P35::EPC00173</dc:identifier>
<dce:identifier>SDN:P35::EPC00173</dce:identifier>
<dc:date>2016-12-12 15:20:45.0</dc:date>
<skos:notation>SDN:P35::EPC00173</skos:notation>
<skos:prefLabel xml:lang="en">Organic carbon in the sediment</skos:prefLabel>
<skos:altLabel>Organic carbon in the sediment</skos:altLabel>
<skos:definition xml:lang="en">Concentration of organic carbon per unit dry weight of sediment (regardless of sediment size class).</skos:definition>
<owl:versionInfo>5</owl:versionInfo>
<pav:hasCurrentVersion rdf:resource="http://vocab.nerc.ac.uk/collection/P35/current/EPC00173/5/"/>
<pav:version>5</pav:version>
<pav:authoredOn>2016-12-12 15:20:45.0</pav:authoredOn>
<skos:note xml:lang="en">accepted</skos:note>
<owl:deprecated>false</owl:deprecated>
<skos:narrower rdf:resource="http://vocab.nerc.ac.uk/collection/P01/current/CORGSE02/"/>
<skos:narrower rdf:resource="http://vocab.nerc.ac.uk/collection/P01/current/OCCNXXXX/"/>
<skos:narrower rdf:resource="http://vocab.nerc.ac.uk/collection/P01/current/CORGSE01/"/>
<skos:narrower rdf:resource="http://vocab.nerc.ac.uk/collection/P01/current/HCMR0021/"/>
<skos:narrower rdf:resource="http://vocab.nerc.ac.uk/collection/P01/current/OCCNCAXT/"/>
<skos:narrower rdf:resource="http://vocab.nerc.ac.uk/collection/P01/current/OCCNCIWF/"/>
<skos:related rdf:resource="http://vocab.nerc.ac.uk/collection/P06/current/UGKG/"/>
<skos:broader rdf:resource="http://vocab.nerc.ac.uk/collection/P36/current/ORGMAT/"/>
<void:inDataset rdf:resource="http://vocab.nerc.ac.uk/.well-known/void"/>
</skos:Concept>
</skos:member>
<skos:member>
<skos:Concept rdf:about="http://vocab.nerc.ac.uk/collection/P35/current/EPC00200/">
<dc:identifier>SDN:P35::EPC00200</dc:identifier>
<dce:identifier>SDN:P35::EPC00200</dce:identifier>
<dc:date>2016-12-12 15:20:45.0</dc:date>
<skos:notation>SDN:P35::EPC00200</skos:notation>
<skos:prefLabel xml:lang="en">Organic nitrogen in the sediment</skos:prefLabel>
<skos:altLabel>Organic nitrogen in the sediment</skos:altLabel>
<skos:definition xml:lang="en">Concentration of organic nitrogen per unit dry weight of sediment (regardless of sediment size class).</skos:definition>
<owl:versionInfo>5</owl:versionInfo>
<pav:hasCurrentVersion rdf:resource="http://vocab.nerc.ac.uk/collection/P35/current/EPC00200/5/"/>
<pav:version>5</pav:version>
<pav:authoredOn>2016-12-12 15:20:45.0</pav:authoredOn>
<skos:note xml:lang="en">accepted</skos:note>
<owl:deprecated>false</owl:deprecated>
<skos:narrower rdf:resource="http://vocab.nerc.ac.uk/collection/P01/current/TNCNCNXT/"/>
<skos:narrower rdf:resource="http://vocab.nerc.ac.uk/collection/P01/current/ONCNCIWF/"/>
<skos:narrower rdf:resource="http://vocab.nerc.ac.uk/collection/P01/current/TNCNCNWF/"/>
<skos:related rdf:resource="http://vocab.nerc.ac.uk/collection/P06/current/UGKG/"/>
<skos:broader rdf:resource="http://vocab.nerc.ac.uk/collection/P36/current/FERTIL/"/>
<void:inDataset rdf:resource="http://vocab.nerc.ac.uk/.well-known/void"/>
</skos:Concept>
</skos:member>
<skos:member>
<skos:Concept rdf:about="http://vocab.nerc.ac.uk/collection/P35/current/EPC00219/">
<dc:identifier>SDN:P35::EPC00219</dc:identifier>
<dce:identifier>SDN:P35::EPC00219</dce:identifier>
<dc:date>2018-03-20 16:58:29.0</dc:date>
<skos:notation>SDN:P35::EPC00219</skos:notation>
<skos:prefLabel xml:lang="en">PCB101 in Mytilus</skos:prefLabel>
<skos:altLabel>PCB101 in Mytilus</skos:altLabel>
<skos:definition xml:lang="en">Concentration of PCB101 per unit weight (dry or wet) of Mytilus spp. (regardless of Mytilus species and size class).</skos:definition>
<owl:versionInfo>6</owl:versionInfo>
<pav:hasCurrentVersion rdf:resource="http://vocab.nerc.ac.uk/collection/P35/current/EPC00219/6/"/>
<pav:version>6</pav:version>
<pav:authoredOn>2018-03-20 16:58:29.0</pav:authoredOn>
<skos:note xml:lang="en">deprecated</skos:note>
<owl:deprecated>true</owl:deprecated>
<skos:narrower rdf:resource="http://vocab.nerc.ac.uk/collection/P01/current/P1016569/"/>
<skos:narrower rdf:resource="http://vocab.nerc.ac.uk/collection/P01/current/IFRPCB24/"/>
<skos:narrower rdf:resource="http://vocab.nerc.ac.uk/collection/P01/current/IFRPCB23/"/>
<skos:related rdf:resource="http://vocab.nerc.ac.uk/collection/P06/current/UUKG/"/>
<skos:broader rdf:resource="http://vocab.nerc.ac.uk/collection/P36/current/PCBSXX/"/>
<void:inDataset rdf:resource="http://vocab.nerc.ac.uk/.well-known/void"/>
</skos:Concept>
</skos:member>
<skos:member>
<skos:Concept rdf:about="http://vocab.nerc.ac.uk/collection/P35/current/EPC00164/">
<dc:identifier>SDN:P35::EPC00164</dc:identifier>
<dce:identifier>SDN:P35::EPC00164</dce:identifier>
<dc:date>2016-12-12 15:20:45.0</dc:date>
<skos:notation>SDN:P35::EPC00164</skos:notation>
<skos:prefLabel xml:lang="en">PCB101 in the sediment</skos:prefLabel>
<skos:altLabel>PCB101 in the sediment</skos:altLabel>
<skos:definition xml:lang="en">Concentration of PCB101 per unit dry weight of sediment (regardless of sediment size class).</skos:definition>
<owl:versionInfo>5</owl:versionInfo>
<pav:hasCurrentVersion rdf:resource="http://vocab.nerc.ac.uk/collection/P35/current/EPC00164/5/"/>
<pav:version>5</pav:version>
<pav:authoredOn>2016-12-12 15:20:45.0</pav:authoredOn>
<skos:note xml:lang="en">accepted</skos:note>
<owl:deprecated>false</owl:deprecated>
<skos:narrower rdf:resource="http://vocab.nerc.ac.uk/collection/P01/current/PCBSD022/"/>
<skos:narrower rdf:resource="http://vocab.nerc.ac.uk/collection/P01/current/PCBSD161/"/>
<skos:narrower rdf:resource="http://vocab.nerc.ac.uk/collection/P01/current/PCBSD066/"/>
<skos:narrower rdf:resource="http://vocab.nerc.ac.uk/collection/P01/current/CB101SBD/"/>
<skos:related rdf:resource="http://vocab.nerc.ac.uk/collection/P06/current/UUKG/"/>
<skos:broader rdf:resource="http://vocab.nerc.ac.uk/collection/P36/current/PCBSXX/"/>
<void:inDataset rdf:resource="http://vocab.nerc.ac.uk/.well-known/void"/>
</skos:Concept>
</skos:member>
<skos:member>
<skos:Concept rdf:about="http://vocab.nerc.ac.uk/collection/P35/current/EPC00149/">
<dc:identifier>SDN:P35::EPC00149</dc:identifier>
<dce:identifier>SDN:P35::EPC00149</dce:identifier>
<dc:date>2018-03-20 16:58:29.0</dc:date>
<skos:notation>SDN:P35::EPC00149</skos:notation>
<skos:prefLabel xml:lang="en">PCB105 in Mytilus</skos:prefLabel>
<skos:altLabel>PCB105 in Mytilus</skos:altLabel>
<skos:definition xml:lang="en">Concentration of PCB105 per unit weight (dry or wet) of Mytilus spp. (regardless of Mytilus species and size class).</skos:definition>
<owl:versionInfo>7</owl:versionInfo>
<pav:hasCurrentVersion rdf:resource="http://vocab.nerc.ac.uk/collection/P35/current/EPC00149/7/"/>
<pav:version>7</pav:version>
<pav:authoredOn>2018-03-20 16:58:29.0</pav:authoredOn>
<skos:note xml:lang="en">deprecated</skos:note>
<owl:deprecated>true</owl:deprecated>
<skos:narrower rdf:resource="http://vocab.nerc.ac.uk/collection/P01/current/IFRPCB41/"/>
<skos:narrower rdf:resource="http://vocab.nerc.ac.uk/collection/P01/current/IFRPCB42/"/>
<skos:related rdf:resource="http://vocab.nerc.ac.uk/collection/P06/current/UUKG/"/>
<skos:broader rdf:resource="http://vocab.nerc.ac.uk/collection/P36/current/PCBSXX/"/>
<void:inDataset rdf:resource="http://vocab.nerc.ac.uk/.well-known/void"/>
</skos:Concept>
</skos:member>
<skos:member>
<skos:Concept rdf:about="http://vocab.nerc.ac.uk/collection/P35/current/EPC00166/">
<dc:identifier>SDN:P35::EPC00166</dc:identifier>
<dce:identifier>SDN:P35::EPC00166</dce:identifier>
<dc:date>2018-03-20 16:58:29.0</dc:date>
<skos:notation>SDN:P35::EPC00166</skos:notation>
<skos:prefLabel xml:lang="en">PCB105 in the sediment</skos:prefLabel>
<skos:altLabel>PCB105 in the sediment</skos:altLabel>
<skos:definition xml:lang="en">Concentration of PCB105 per unit dry weight of sediment (reardless of sediment size class).</skos:definition>
<owl:versionInfo>7</owl:versionInfo>
<pav:hasCurrentVersion rdf:resource="http://vocab.nerc.ac.uk/collection/P35/current/EPC00166/7/"/>
<pav:version>7</pav:version>
<pav:authoredOn>2018-03-20 16:58:29.0</pav:authoredOn>
<skos:note xml:lang="en">deprecated</skos:note>
<owl:deprecated>true</owl:deprecated>
<skos:narrower rdf:resource="http://vocab.nerc.ac.uk/collection/P01/current/PCBSD030/"/>
<skos:narrower rdf:resource="http://vocab.nerc.ac.uk/collection/P01/current/CB105SBD/"/>
<skos:narrower rdf:resource="http://vocab.nerc.ac.uk/collection/P01/current/PCBSD136/"/>
<skos:narrower rdf:resource="http://vocab.nerc.ac.uk/collection/P01/current/CB105SAD/"/>
<skos:related rdf:resource="http://vocab.nerc.ac.uk/collection/P06/current/UUKG/"/>
<skos:broader rdf:resource="http://vocab.nerc.ac.uk/collection/P36/current/PCBSXX/"/>
<void:inDataset rdf:resource="http://vocab.nerc.ac.uk/.well-known/void"/>
</skos:Concept>
</skos:member>
<skos:member>
<skos:Concept rdf:about="http://vocab.nerc.ac.uk/collection/P35/current/EPC00204/">
<dc:identifier>SDN:P35::EPC00204</dc:identifier>
<dce:identifier>SDN:P35::EPC00204</dce:identifier>
<dc:date>2018-03-20 16:58:29.0</dc:date>
<skos:notation>SDN:P35::EPC00204</skos:notation>
<skos:prefLabel xml:lang="en">PCB118 in Mytilus</skos:prefLabel>
<skos:altLabel>PCB118 in Mytilus</skos:altLabel>
<skos:definition xml:lang="en">Concentration of PCB118 per unit weight (dry or wet) of Mytilus spp. (regardless of Mytilus species and size class).</skos:definition>
<owl:versionInfo>7</owl:versionInfo>
<pav:hasCurrentVersion rdf:resource="http://vocab.nerc.ac.uk/collection/P35/current/EPC00204/7/"/>
<pav:version>7</pav:version>
<pav:authoredOn>2018-03-20 16:58:29.0</pav:authoredOn>
<skos:note xml:lang="en">deprecated</skos:note>
<owl:deprecated>true</owl:deprecated>
<skos:narrower rdf:resource="http://vocab.nerc.ac.uk/collection/P01/current/IFRPCB48/"/>
<skos:narrower rdf:resource="http://vocab.nerc.ac.uk/collection/P01/current/CF039WME/"/>
<skos:narrower rdf:resource="http://vocab.nerc.ac.uk/collection/P01/current/P1186569/"/>
<skos:narrower rdf:resource="http://vocab.nerc.ac.uk/collection/P01/current/IFRPCB47/"/>
<skos:related rdf:resource="http://vocab.nerc.ac.uk/collection/P06/current/UUKG/"/>
<skos:broader rdf:resource="http://vocab.nerc.ac.uk/collection/P36/current/PCBSXX/"/>
<void:inDataset rdf:resource="http://vocab.nerc.ac.uk/.well-known/void"/>
</skos:Concept>
</skos:member>
<skos:member>
<skos:Concept rdf:about="http://vocab.nerc.ac.uk/collection/P35/current/EPC00174/">
<dc:identifier>SDN:P35::EPC00174</dc:identifier>
<dce:identifier>SDN:P35::EPC00174</dce:identifier>
<dc:date>2016-12-12 15:20:45.0</dc:date>
<skos:notation>SDN:P35::EPC00174</skos:notation>
<skos:prefLabel xml:lang="en">PCB118 in the sediment</skos:prefLabel>
<skos:altLabel>PCB118 in the sediment</skos:altLabel>
<skos:definition xml:lang="en">Concentration of PCB118 per unit dry weight of sediment (regardless of sediment size class).</skos:definition>
<owl:versionInfo>6</owl:versionInfo>
<pav:hasCurrentVersion rdf:resource="http://vocab.nerc.ac.uk/collection/P35/current/EPC00174/6/"/>
<pav:version>6</pav:version>
<pav:authoredOn>2016-12-12 15:20:45.0</pav:authoredOn>
<skos:note xml:lang="en">accepted</skos:note>
<owl:deprecated>false</owl:deprecated>
<skos:narrower rdf:resource="http://vocab.nerc.ac.uk/collection/P01/current/PCBSD070/"/>
<skos:narrower rdf:resource="http://vocab.nerc.ac.uk/collection/P01/current/PCBSD132/"/>
<skos:narrower rdf:resource="http://vocab.nerc.ac.uk/collection/P01/current/CB118SAD/"/>
<skos:narrower rdf:resource="http://vocab.nerc.ac.uk/collection/P01/current/CB118SBD/"/>
<skos:narrower rdf:resource="http://vocab.nerc.ac.uk/collection/P01/current/PCBSD026/"/>
<skos:narrower rdf:resource="http://vocab.nerc.ac.uk/collection/P01/current/PCBSD165/"/>
<skos:related rdf:resource="http://vocab.nerc.ac.uk/collection/P06/current/UUKG/"/>
<skos:broader rdf:resource="http://vocab.nerc.ac.uk/collection/P36/current/PCBSXX/"/>
<void:inDataset rdf:resource="http://vocab.nerc.ac.uk/.well-known/void"/>
</skos:Concept>
</skos:member>
<skos:member>
<skos:Concept rdf:about="http://vocab.nerc.ac.uk/collection/P35/current/EPC00191/">
<dc:identifier>SDN:P35::EPC00191</dc:identifier>
<dce:identifier>SDN:P35::EPC00191</dce:identifier>
<dc:date>2018-03-20 16:58:29.0</dc:date>
<skos:notation>SDN:P35::EPC00191</skos:notation>
<skos:prefLabel xml:lang="en">PCB138 in Mytilus</skos:prefLabel>
<skos:altLabel>PCB138 in Mytilus</skos:altLabel>
<skos:definition xml:lang="en">Concentration of PCB138 per unit weight (dry or wet) of Mytilus spp. (reagardless of Mytilus species and size class).</skos:definition>
<owl:versionInfo>6</owl:versionInfo>
<pav:hasCurrentVersion rdf:resource="http://vocab.nerc.ac.uk/collection/P35/current/EPC00191/6/"/>
<pav:version>6</pav:version>
<pav:authoredOn>2018-03-20 16:58:29.0</pav:authoredOn>
<skos:note xml:lang="en">deprecated</skos:note>
<owl:deprecated>true</owl:deprecated>
<skos:narrower rdf:resource="http://vocab.nerc.ac.uk/collection/P01/current/IFRPCB11/"/>
<skos:narrower rdf:resource="http://vocab.nerc.ac.uk/collection/P01/current/P1386569/"/>
<skos:narrower rdf:resource="http://vocab.nerc.ac.uk/collection/P01/current/IFRPCB12/"/>
<skos:related rdf:resource="http://vocab.nerc.ac.uk/collection/P06/current/UUKG/"/>
<skos:broader rdf:resource="http://vocab.nerc.ac.uk/collection/P36/current/PCBSXX/"/>
<void:inDataset rdf:resource="http://vocab.nerc.ac.uk/.well-known/void"/>
</skos:Concept>
</skos:member>
<skos:member>
<skos:Concept rdf:about="http://vocab.nerc.ac.uk/collection/P35/current/EPC00216/">
<dc:identifier>SDN:P35::EPC00216</dc:identifier>
<dce:identifier>SDN:P35::EPC00216</dce:identifier>
<dc:date>2016-12-12 15:20:45.0</dc:date>
<skos:notation>SDN:P35::EPC00216</skos:notation>
<skos:prefLabel xml:lang="en">PCB138 in the sediment</skos:prefLabel>
<skos:altLabel>PCB138 in the sediment</skos:altLabel>
<skos:definition xml:lang="en">Concentration of PCB138 per unit dry weight of sediment (regardless of sediment size class).</skos:definition>
<owl:versionInfo>5</owl:versionInfo>
<pav:hasCurrentVersion rdf:resource="http://vocab.nerc.ac.uk/collection/P35/current/EPC00216/5/"/>
<pav:version>5</pav:version>
<pav:authoredOn>2016-12-12 15:20:45.0</pav:authoredOn>
<skos:note xml:lang="en">accepted</skos:note>
<owl:deprecated>false</owl:deprecated>
<skos:narrower rdf:resource="http://vocab.nerc.ac.uk/collection/P01/current/PCBSD008/"/>
<skos:narrower rdf:resource="http://vocab.nerc.ac.uk/collection/P01/current/PCBSD052/"/>
<skos:narrower rdf:resource="http://vocab.nerc.ac.uk/collection/P01/current/PCBSD147/"/>
<skos:narrower rdf:resource="http://vocab.nerc.ac.uk/collection/P01/current/CB138SBD/"/>
<skos:related rdf:resource="http://vocab.nerc.ac.uk/collection/P06/current/UUKG/"/>
<skos:broader rdf:resource="http://vocab.nerc.ac.uk/collection/P36/current/PCBSXX/"/>
<void:inDataset rdf:resource="http://vocab.nerc.ac.uk/.well-known/void"/>
</skos:Concept>
</skos:member>
<skos:member>
<skos:Concept rdf:about="http://vocab.nerc.ac.uk/collection/P35/current/EPC00192/">
<dc:identifier>SDN:P35::EPC00192</dc:identifier>
<dce:identifier>SDN:P35::EPC00192</dce:identifier>
<dc:date>2018-03-20 16:58:29.0</dc:date>
<skos:notation>SDN:P35::EPC00192</skos:notation>
<skos:prefLabel xml:lang="en">PCB153 in Mytilus</skos:prefLabel>
<skos:altLabel>PCB153 in Mytilus</skos:altLabel>
<skos:definition xml:lang="en">Concentration of PCB153 per unit weight (dry or wet) of Mytilus spp. (regardless of Mytilus species and size class).</skos:definition>
<owl:versionInfo>6</owl:versionInfo>
<pav:hasCurrentVersion rdf:resource="http://vocab.nerc.ac.uk/collection/P35/current/EPC00192/6/"/>
<pav:version>6</pav:version>
<pav:authoredOn>2018-03-20 16:58:29.0</pav:authoredOn>
<skos:note xml:lang="en">deprecated</skos:note>
<owl:deprecated>true</owl:deprecated>
<skos:narrower rdf:resource="http://vocab.nerc.ac.uk/collection/P01/current/CF029WME/"/>
<skos:narrower rdf:resource="http://vocab.nerc.ac.uk/collection/P01/current/IFRPCB18/"/>
<skos:narrower rdf:resource="http://vocab.nerc.ac.uk/collection/P01/current/IFRPCB17/"/>
<skos:narrower rdf:resource="http://vocab.nerc.ac.uk/collection/P01/current/P1536569/"/>
<skos:related rdf:resource="http://vocab.nerc.ac.uk/collection/P06/current/UUKG/"/>
<skos:broader rdf:resource="http://vocab.nerc.ac.uk/collection/P36/current/PCBSXX/"/>
<void:inDataset rdf:resource="http://vocab.nerc.ac.uk/.well-known/void"/>
</skos:Concept>
</skos:member>
<skos:member>
<skos:Concept rdf:about="http://vocab.nerc.ac.uk/collection/P35/current/EPC00218/">
<dc:identifier>SDN:P35::EPC00218</dc:identifier>
<dce:identifier>SDN:P35::EPC00218</dce:identifier>
<dc:date>2016-12-12 15:20:45.0</dc:date>
<skos:notation>SDN:P35::EPC00218</skos:notation>
<skos:prefLabel xml:lang="en">PCB153 in the sediment</skos:prefLabel>
<skos:altLabel>PCB153 in the sediment</skos:altLabel>
<skos:definition xml:lang="en">Concentration of PCB153 per unit dry weight of sediment (regardless of sediment size class).</skos:definition>
<owl:versionInfo>5</owl:versionInfo>
<pav:hasCurrentVersion rdf:resource="http://vocab.nerc.ac.uk/collection/P35/current/EPC00218/5/"/>
<pav:version>5</pav:version>
<pav:authoredOn>2016-12-12 15:20:45.0</pav:authoredOn>
<skos:note xml:lang="en">accepted</skos:note>
<owl:deprecated>false</owl:deprecated>
<skos:narrower rdf:resource="http://vocab.nerc.ac.uk/collection/P01/current/PCBSD063/"/>
<skos:narrower rdf:resource="http://vocab.nerc.ac.uk/collection/P01/current/PCBSD158/"/>
<skos:narrower rdf:resource="http://vocab.nerc.ac.uk/collection/P01/current/PCBSD019/"/>
<skos:narrower rdf:resource="http://vocab.nerc.ac.uk/collection/P01/current/CB153SBD/"/>
<skos:related rdf:resource="http://vocab.nerc.ac.uk/collection/P06/current/UUKG/"/>
<skos:broader rdf:resource="http://vocab.nerc.ac.uk/collection/P36/current/PCBSXX/"/>
<void:inDataset rdf:resource="http://vocab.nerc.ac.uk/.well-known/void"/>
</skos:Concept>
</skos:member>
<skos:member>
<skos:Concept rdf:about="http://vocab.nerc.ac.uk/collection/P35/current/EPC00184/">
<dc:identifier>SDN:P35::EPC00184</dc:identifier>
<dce:identifier>SDN:P35::EPC00184</dce:identifier>
<dc:date>2018-03-20 16:58:29.0</dc:date>
<skos:notation>SDN:P35::EPC00184</skos:notation>
<skos:prefLabel xml:lang="en">PCB180 in Mytilus</skos:prefLabel>
<skos:altLabel>PCB180 in Mytilus</skos:altLabel>
<skos:definition xml:lang="en">Concentration of PCB180 per unit weight (dry or wet) of Mytilus spp. (reardless of Mytilus species and size class).</skos:definition>
<owl:versionInfo>6</owl:versionInfo>
<pav:hasCurrentVersion rdf:resource="http://vocab.nerc.ac.uk/collection/P35/current/EPC00184/6/"/>
<pav:version>6</pav:version>
<pav:authoredOn>2018-03-20 16:58:29.0</pav:authoredOn>
<skos:note xml:lang="en">deprecated</skos:note>
<owl:deprecated>true</owl:deprecated>
<skos:narrower rdf:resource="http://vocab.nerc.ac.uk/collection/P01/current/P1806569/"/>
<skos:narrower rdf:resource="http://vocab.nerc.ac.uk/collection/P01/current/IFRPCB06/"/>
<skos:narrower rdf:resource="http://vocab.nerc.ac.uk/collection/P01/current/IFRPCB05/"/>
<skos:related rdf:resource="http://vocab.nerc.ac.uk/collection/P06/current/UUKG/"/>
<skos:broader rdf:resource="http://vocab.nerc.ac.uk/collection/P36/current/PCBSXX/"/>
<void:inDataset rdf:resource="http://vocab.nerc.ac.uk/.well-known/void"/>
</skos:Concept>
</skos:member>
<skos:member>
<skos:Concept rdf:about="http://vocab.nerc.ac.uk/collection/P35/current/EPC00217/">
<dc:identifier>SDN:P35::EPC00217</dc:identifier>
<dce:identifier>SDN:P35::EPC00217</dce:identifier>
<dc:date>2016-12-12 15:20:45.0</dc:date>
<skos:notation>SDN:P35::EPC00217</skos:notation>
<skos:prefLabel xml:lang="en">PCB180 in the sediment</skos:prefLabel>
<skos:altLabel>PCB180 in the sediment</skos:altLabel>
<skos:definition xml:lang="en">Concentration of PCB180 per unit dry weight of sediment (regardless of sediment size class).</skos:definition>
<owl:versionInfo>5</owl:versionInfo>
<pav:hasCurrentVersion rdf:resource="http://vocab.nerc.ac.uk/collection/P35/current/EPC00217/5/"/>
<pav:version>5</pav:version>
<pav:authoredOn>2016-12-12 15:20:45.0</pav:authoredOn>
<skos:note xml:lang="en">accepted</skos:note>
<owl:deprecated>false</owl:deprecated>
<skos:narrower rdf:resource="http://vocab.nerc.ac.uk/collection/P01/current/PCBSD148/"/>
<skos:narrower rdf:resource="http://vocab.nerc.ac.uk/collection/P01/current/PCBSD009/"/>
<skos:narrower rdf:resource="http://vocab.nerc.ac.uk/collection/P01/current/CB180SBD/"/>
<skos:narrower rdf:resource="http://vocab.nerc.ac.uk/collection/P01/current/PCBSD053/"/>
<skos:related rdf:resource="http://vocab.nerc.ac.uk/collection/P06/current/UUKG/"/>
<skos:broader rdf:resource="http://vocab.nerc.ac.uk/collection/P36/current/PCBSXX/"/>
<void:inDataset rdf:resource="http://vocab.nerc.ac.uk/.well-known/void"/>
</skos:Concept>
</skos:member>
<skos:member>
<skos:Concept rdf:about="http://vocab.nerc.ac.uk/collection/P35/current/EPC00205/">
<dc:identifier>SDN:P35::EPC00205</dc:identifier>
<dce:identifier>SDN:P35::EPC00205</dce:identifier>
<dc:date>2018-03-20 16:58:29.0</dc:date>
<skos:notation>SDN:P35::EPC00205</skos:notation>
<skos:prefLabel xml:lang="en">PCB28 in Mytilus</skos:prefLabel>
<skos:altLabel>PCB28 in Mytilus</skos:altLabel>
<skos:definition xml:lang="en">Concentration of PCB28 per unit weight (dry or wet) of Mytilus spp. (regardless of Mytilus species and size class).</skos:definition>
<owl:versionInfo>7</owl:versionInfo>
<pav:hasCurrentVersion rdf:resource="http://vocab.nerc.ac.uk/collection/P35/current/EPC00205/7/"/>
<pav:version>7</pav:version>
<pav:authoredOn>2018-03-20 16:58:29.0</pav:authoredOn>
<skos:note xml:lang="en">deprecated</skos:note>
<owl:deprecated>true</owl:deprecated>
<skos:narrower rdf:resource="http://vocab.nerc.ac.uk/collection/P01/current/IFRPCB54/"/>
<skos:narrower rdf:resource="http://vocab.nerc.ac.uk/collection/P01/current/P0286569/"/>
<skos:narrower rdf:resource="http://vocab.nerc.ac.uk/collection/P01/current/IFRPCB53/"/>
<skos:related rdf:resource="http://vocab.nerc.ac.uk/collection/P06/current/UUKG/"/>
<skos:broader rdf:resource="http://vocab.nerc.ac.uk/collection/P36/current/PCBSXX/"/>
<void:inDataset rdf:resource="http://vocab.nerc.ac.uk/.well-known/void"/>
</skos:Concept>
</skos:member>
<skos:member>
<skos:Concept rdf:about="http://vocab.nerc.ac.uk/collection/P35/current/EPC00206/">
<dc:identifier>SDN:P35::EPC00206</dc:identifier>
<dce:identifier>SDN:P35::EPC00206</dce:identifier>
<dc:date>2016-12-12 15:20:45.0</dc:date>
<skos:notation>SDN:P35::EPC00206</skos:notation>
<skos:prefLabel xml:lang="en">PCB28 in the sediment</skos:prefLabel>
<skos:altLabel>PCB28 in the sediment</skos:altLabel>
<skos:definition xml:lang="en">Concentration of PCB28 per unit dry weight of sediment (regardless of sediment size class).</skos:definition>
<owl:versionInfo>6</owl:versionInfo>
<pav:hasCurrentVersion rdf:resource="http://vocab.nerc.ac.uk/collection/P35/current/EPC00206/6/"/>
<pav:version>6</pav:version>
<pav:authoredOn>2016-12-12 15:20:45.0</pav:authoredOn>
<skos:note xml:lang="en">accepted</skos:note>
<owl:deprecated>false</owl:deprecated>
<skos:narrower rdf:resource="http://vocab.nerc.ac.uk/collection/P01/current/PCBSD171/"/>
<skos:narrower rdf:resource="http://vocab.nerc.ac.uk/collection/P01/current/PCBSD076/"/>
<skos:narrower rdf:resource="http://vocab.nerc.ac.uk/collection/P01/current/PCBSD138/"/>
<skos:narrower rdf:resource="http://vocab.nerc.ac.uk/collection/P01/current/CB28SDAD/"/>
<skos:narrower rdf:resource="http://vocab.nerc.ac.uk/collection/P01/current/PCBSD032/"/>
<skos:narrower rdf:resource="http://vocab.nerc.ac.uk/collection/P01/current/CB28SDBD/"/>
<skos:related rdf:resource="http://vocab.nerc.ac.uk/collection/P06/current/UUKG/"/>
<skos:broader rdf:resource="http://vocab.nerc.ac.uk/collection/P36/current/PCBSXX/"/>
<void:inDataset rdf:resource="http://vocab.nerc.ac.uk/.well-known/void"/>
</skos:Concept>
</skos:member>
<skos:member>
<skos:Concept rdf:about="http://vocab.nerc.ac.uk/collection/P35/current/EPC00165/">
<dc:identifier>SDN:P35::EPC00165</dc:identifier>
<dce:identifier>SDN:P35::EPC00165</dce:identifier>
<dc:date>2018-03-20 16:58:29.0</dc:date>
<skos:notation>SDN:P35::EPC00165</skos:notation>
<skos:prefLabel xml:lang="en">PCB52 in Mytilus</skos:prefLabel>
<skos:altLabel>PCB52 in Mytilus</skos:altLabel>
<skos:definition xml:lang="en">Concentration of PCB52 per unit weight (dry or wet) of Mytilus spp. (regardless of Mytilus species and size class).</skos:definition>
<owl:versionInfo>6</owl:versionInfo>
<pav:hasCurrentVersion rdf:resource="http://vocab.nerc.ac.uk/collection/P35/current/EPC00165/6/"/>
<pav:version>6</pav:version>
<pav:authoredOn>2018-03-20 16:58:29.0</pav:authoredOn>
<skos:note xml:lang="en">deprecated</skos:note>
<owl:deprecated>true</owl:deprecated>
<skos:narrower rdf:resource="http://vocab.nerc.ac.uk/collection/P01/current/P0526569/"/>
<skos:narrower rdf:resource="http://vocab.nerc.ac.uk/collection/P01/current/IFRPCB30/"/>
<skos:narrower rdf:resource="http://vocab.nerc.ac.uk/collection/P01/current/IFRPCB29/"/>
<skos:related rdf:resource="http://vocab.nerc.ac.uk/collection/P06/current/UUKG/"/>
<skos:broader rdf:resource="http://vocab.nerc.ac.uk/collection/P36/current/PCBSXX/"/>
<void:inDataset rdf:resource="http://vocab.nerc.ac.uk/.well-known/void"/>
</skos:Concept>
</skos:member>
<skos:member>
<skos:Concept rdf:about="http://vocab.nerc.ac.uk/collection/P35/current/EPC00193/">
<dc:identifier>SDN:P35::EPC00193</dc:identifier>
<dce:identifier>SDN:P35::EPC00193</dce:identifier>
<dc:date>2016-12-12 15:20:45.0</dc:date>
<skos:notation>SDN:P35::EPC00193</skos:notation>
<skos:prefLabel xml:lang="en">PCB52 in the sediment</skos:prefLabel>
<skos:altLabel>PCB52 in the sediment</skos:altLabel>
<skos:definition xml:lang="en">Concentration of PCB52 per unit dry weight of sediment (regardless of sediment size class).</skos:definition>
<owl:versionInfo>5</owl:versionInfo>
<pav:hasCurrentVersion rdf:resource="http://vocab.nerc.ac.uk/collection/P35/current/EPC00193/5/"/>
<pav:version>5</pav:version>
<pav:authoredOn>2016-12-12 15:20:45.0</pav:authoredOn>
<skos:note xml:lang="en">accepted</skos:note>
<owl:deprecated>false</owl:deprecated>
<skos:narrower rdf:resource="http://vocab.nerc.ac.uk/collection/P01/current/PCBSD023/"/>
<skos:narrower rdf:resource="http://vocab.nerc.ac.uk/collection/P01/current/CB52SDBD/"/>
<skos:narrower rdf:resource="http://vocab.nerc.ac.uk/collection/P01/current/PCBSD067/"/>
<skos:narrower rdf:resource="http://vocab.nerc.ac.uk/collection/P01/current/PCBSD162/"/>
<skos:related rdf:resource="http://vocab.nerc.ac.uk/collection/P06/current/UUKG/"/>
<skos:broader rdf:resource="http://vocab.nerc.ac.uk/collection/P36/current/PCBSXX/"/>
<void:inDataset rdf:resource="http://vocab.nerc.ac.uk/.well-known/void"/>
</skos:Concept>
</skos:member>
<skos:member>
<skos:Concept rdf:about="http://vocab.nerc.ac.uk/collection/P35/current/EPC00203/">
<dc:identifier>SDN:P35::EPC00203</dc:identifier>
<dce:identifier>SDN:P35::EPC00203</dce:identifier>
<dc:date>2018-03-20 16:58:29.0</dc:date>
<skos:notation>SDN:P35::EPC00203</skos:notation>
<skos:prefLabel xml:lang="en">Phenanthrene in Mytilus</skos:prefLabel>
<skos:altLabel>Phenanthrene in Mytilus</skos:altLabel>
<skos:definition xml:lang="en">Concentration of phenantrene per unit weight (dry or wet) of Mytilus spp. (regardless of Mytilus species and size class).</skos:definition>
<owl:versionInfo>6</owl:versionInfo>
<pav:hasCurrentVersion rdf:resource="http://vocab.nerc.ac.uk/collection/P35/current/EPC00203/6/"/>
<pav:version>6</pav:version>
<pav:authoredOn>2018-03-20 16:58:29.0</pav:authoredOn>
<skos:note xml:lang="en">deprecated</skos:note>
<owl:deprecated>true</owl:deprecated>
<skos:narrower rdf:resource="http://vocab.nerc.ac.uk/collection/P01/current/PHMMCF14/"/>
<skos:narrower rdf:resource="http://vocab.nerc.ac.uk/collection/P01/current/IFRPAH57/"/>
<skos:narrower rdf:resource="http://vocab.nerc.ac.uk/collection/P01/current/PHWW6569/"/>
<skos:narrower rdf:resource="http://vocab.nerc.ac.uk/collection/P01/current/PHDWCF14/"/>
<skos:related rdf:resource="http://vocab.nerc.ac.uk/collection/P06/current/UUKG/"/>
<skos:broader rdf:resource="http://vocab.nerc.ac.uk/collection/P36/current/HCARBS/"/>
<void:inDataset rdf:resource="http://vocab.nerc.ac.uk/.well-known/void"/>
</skos:Concept>
</skos:member>
<skos:member>
<skos:Concept rdf:about="http://vocab.nerc.ac.uk/collection/P35/current/EPC00142/">
<dc:identifier>SDN:P35::EPC00142</dc:identifier>
<dce:identifier>SDN:P35::EPC00142</dce:identifier>
<dc:date>2016-12-12 15:20:45.0</dc:date>
<skos:notation>SDN:P35::EPC00142</skos:notation>
<skos:prefLabel xml:lang="en">Phenanthrene in the sediment</skos:prefLabel>
<skos:altLabel>Phenanthrene in the sediment</skos:altLabel>
<skos:definition xml:lang="en">Concentration of phenanthrene per unit dry weight of sediment (regardless of sediment size class).</skos:definition>
<owl:versionInfo>5</owl:versionInfo>
<pav:hasCurrentVersion rdf:resource="http://vocab.nerc.ac.uk/collection/P35/current/EPC00142/5/"/>
<pav:version>5</pav:version>
<pav:authoredOn>2016-12-12 15:20:45.0</pav:authoredOn>
<skos:note xml:lang="en">accepted</skos:note>
<owl:deprecated>false</owl:deprecated>
<skos:narrower rdf:resource="http://vocab.nerc.ac.uk/collection/P01/current/HDCCZHAN/"/>
<skos:narrower rdf:resource="http://vocab.nerc.ac.uk/collection/P01/current/PASEDBD1/"/>
<skos:related rdf:resource="http://vocab.nerc.ac.uk/collection/P06/current/UUKG/"/>
<skos:broader rdf:resource="http://vocab.nerc.ac.uk/collection/P36/current/HCARBS/"/>
<void:inDataset rdf:resource="http://vocab.nerc.ac.uk/.well-known/void"/>
</skos:Concept>
</skos:member>
<skos:member>
<skos:Concept rdf:about="http://vocab.nerc.ac.uk/collection/P35/current/EPC00181/">
<dc:identifier>SDN:P35::EPC00181</dc:identifier>
<dce:identifier>SDN:P35::EPC00181</dce:identifier>
<dc:date>2016-12-12 15:20:45.0</dc:date>
<skos:notation>SDN:P35::EPC00181</skos:notation>
<skos:prefLabel xml:lang="en">Phosphate in the sediment</skos:prefLabel>
<skos:altLabel>Phosphate in the sediment</skos:altLabel>
<skos:definition xml:lang="en">Concentration of phosphate in sediment pore water.</skos:definition>
<owl:versionInfo>5</owl:versionInfo>
<pav:hasCurrentVersion rdf:resource="http://vocab.nerc.ac.uk/collection/P35/current/EPC00181/5/"/>
<pav:version>5</pav:version>
<pav:authoredOn>2016-12-12 15:20:45.0</pav:authoredOn>
<skos:note xml:lang="en">accepted</skos:note>
<owl:deprecated>false</owl:deprecated>
<skos:narrower rdf:resource="http://vocab.nerc.ac.uk/collection/P01/current/PHOSPWD1/"/>
<skos:related rdf:resource="http://vocab.nerc.ac.uk/collection/P06/current/KGUM/"/>
<skos:broader rdf:resource="http://vocab.nerc.ac.uk/collection/P36/current/FERTIL/"/>
<void:inDataset rdf:resource="http://vocab.nerc.ac.uk/.well-known/void"/>
</skos:Concept>
</skos:member>
<skos:member>
<skos:Concept rdf:about="http://vocab.nerc.ac.uk/collection/P35/current/EPC00211/">
<dc:identifier>SDN:P35::EPC00211</dc:identifier>
<dce:identifier>SDN:P35::EPC00211</dce:identifier>
<dc:date>2016-12-12 15:20:45.0</dc:date>
<skos:notation>SDN:P35::EPC00211</skos:notation>
<skos:prefLabel xml:lang="en">Silicate in the sediment</skos:prefLabel>
<skos:altLabel>Silicate in the sediment</skos:altLabel>
<skos:definition xml:lang="en">Concentration of dissolved silicate per unit volume of sediment pore waters.</skos:definition>
<owl:versionInfo>5</owl:versionInfo>
<pav:hasCurrentVersion rdf:resource="http://vocab.nerc.ac.uk/collection/P35/current/EPC00211/5/"/>
<pav:version>5</pav:version>
<pav:authoredOn>2016-12-12 15:20:45.0</pav:authoredOn>
<skos:note xml:lang="en">accepted</skos:note>
<owl:deprecated>false</owl:deprecated>
<skos:narrower rdf:resource="http://vocab.nerc.ac.uk/collection/P01/current/SICNPWD3/"/>
<skos:related rdf:resource="http://vocab.nerc.ac.uk/collection/P06/current/KGUM/"/>
<skos:broader rdf:resource="http://vocab.nerc.ac.uk/collection/P36/current/FERTIL/"/>
<void:inDataset rdf:resource="http://vocab.nerc.ac.uk/.well-known/void"/>
</skos:Concept>
</skos:member>
<skos:member>
<skos:Concept rdf:about="http://vocab.nerc.ac.uk/collection/P35/current/EPC00084/">
<dc:identifier>SDN:P35::EPC00084</dc:identifier>
<dce:identifier>SDN:P35::EPC00084</dce:identifier>
<dc:date>2016-10-20 11:27:18.0</dc:date>
<skos:notation>SDN:P35::EPC00084</skos:notation>
<skos:prefLabel xml:lang="en">Suspended particulate material aluminium content</skos:prefLabel>
<skos:altLabel>SPM Al</skos:altLabel>
<skos:definition xml:lang="en">Concentration of the metal in particles extracted by filtration (any type of filter) from a sample of a river, estuary, sea or ocean water or trapped in situ expressed per unit dry weight of the particles by any method.</skos:definition>
<owl:versionInfo>3</owl:versionInfo>
<pav:hasCurrentVersion rdf:resource="http://vocab.nerc.ac.uk/collection/P35/current/EPC00084/3/"/>
<pav:version>3</pav:version>
<pav:authoredOn>2016-10-20 11:27:18.0</pav:authoredOn>
<skos:note xml:lang="en">accepted</skos:note>
<owl:deprecated>false</owl:deprecated>
<skos:narrower rdf:resource="http://vocab.nerc.ac.uk/collection/P01/current/ALCNICP2/"/>
<skos:narrower rdf:resource="http://vocab.nerc.ac.uk/collection/P01/current/ALCNPEXX/"/>
<skos:narrower rdf:resource="http://vocab.nerc.ac.uk/collection/P01/current/ALCNAAP2/"/>
<skos:narrower rdf:resource="http://vocab.nerc.ac.uk/collection/P01/current/ALCNAAPC/"/>
<skos:narrower rdf:resource="http://vocab.nerc.ac.uk/collection/P01/current/MALPP012/"/>
<skos:related rdf:resource="http://vocab.nerc.ac.uk/collection/P06/current/UMKG/"/>
<skos:broader rdf:resource="http://vocab.nerc.ac.uk/collection/P36/current/HVYMTL/"/>
<void:inDataset rdf:resource="http://vocab.nerc.ac.uk/.well-known/void"/>
</skos:Concept>
</skos:member>
<skos:member>
<skos:Concept rdf:about="http://vocab.nerc.ac.uk/collection/P35/current/EPC00085/">
<dc:identifier>SDN:P35::EPC00085</dc:identifier>
<dce:identifier>SDN:P35::EPC00085</dce:identifier>
<dc:date>2016-10-20 11:27:18.0</dc:date>
<skos:notation>SDN:P35::EPC00085</skos:notation>
<skos:prefLabel xml:lang="en">Suspended particulate material arsenic content</skos:prefLabel>
<skos:altLabel>SPM As</skos:altLabel>
<skos:definition xml:lang="en">Concentration of the metal in particles extracted by filtration (any type of filter) from a sample of a river, estuary, sea or ocean water or trapped in situ expressed per unit dry weight of the particles by any method.</skos:definition>
<owl:versionInfo>3</owl:versionInfo>
<pav:hasCurrentVersion rdf:resource="http://vocab.nerc.ac.uk/collection/P35/current/EPC00085/3/"/>
<pav:version>3</pav:version>
<pav:authoredOn>2016-10-20 11:27:18.0</pav:authoredOn>
<skos:note xml:lang="en">accepted</skos:note>
<owl:deprecated>false</owl:deprecated>
<skos:narrower rdf:resource="http://vocab.nerc.ac.uk/collection/P01/current/MSPMM024/"/>
<skos:narrower rdf:resource="http://vocab.nerc.ac.uk/collection/P01/current/MSPMM003/"/>
<skos:related rdf:resource="http://vocab.nerc.ac.uk/collection/P06/current/UMKG/"/>
<skos:broader rdf:resource="http://vocab.nerc.ac.uk/collection/P36/current/HVYMTL/"/>
<void:inDataset rdf:resource="http://vocab.nerc.ac.uk/.well-known/void"/>
</skos:Concept>
</skos:member>
<skos:member>
<skos:Concept rdf:about="http://vocab.nerc.ac.uk/collection/P35/current/EPC00086/">
<dc:identifier>SDN:P35::EPC00086</dc:identifier>
<dce:identifier>SDN:P35::EPC00086</dce:identifier>
<dc:date>2016-10-20 11:27:18.0</dc:date>
<skos:notation>SDN:P35::EPC00086</skos:notation>
<skos:prefLabel xml:lang="en">Suspended particulate material barium content</skos:prefLabel>
<skos:altLabel>SPM Ba</skos:altLabel>
<skos:definition xml:lang="en">Concentration of the metal in particles extracted by filtration (any type of filter) from a sample of a river, estuary, sea or ocean water or trapped in situ expressed per unit dry weight of the particles by any method.</skos:definition>
<owl:versionInfo>3</owl:versionInfo>
<pav:hasCurrentVersion rdf:resource="http://vocab.nerc.ac.uk/collection/P35/current/EPC00086/3/"/>
<pav:version>3</pav:version>
<pav:authoredOn>2016-10-20 11:27:18.0</pav:authoredOn>
<skos:note xml:lang="en">accepted</skos:note>
<owl:deprecated>false</owl:deprecated>
<skos:narrower rdf:resource="http://vocab.nerc.ac.uk/collection/P01/current/MBAPP012/"/>
<skos:narrower rdf:resource="http://vocab.nerc.ac.uk/collection/P01/current/BACNPEXX/"/>
<skos:narrower rdf:resource="http://vocab.nerc.ac.uk/collection/P01/current/BACNICXX/"/>
<skos:narrower rdf:resource="http://vocab.nerc.ac.uk/collection/P01/current/BACNAAP2/"/>
<skos:narrower rdf:resource="http://vocab.nerc.ac.uk/collection/P01/current/BACNICP2/"/>
<skos:related rdf:resource="http://vocab.nerc.ac.uk/collection/P06/current/UMKG/"/>
<skos:broader rdf:resource="http://vocab.nerc.ac.uk/collection/P36/current/HVYMTL/"/>
<void:inDataset rdf:resource="http://vocab.nerc.ac.uk/.well-known/void"/>
</skos:Concept>
</skos:member>
<skos:member>
<skos:Concept rdf:about="http://vocab.nerc.ac.uk/collection/P35/current/EPC00087/">
<dc:identifier>SDN:P35::EPC00087</dc:identifier>
<dce:identifier>SDN:P35::EPC00087</dce:identifier>
<dc:date>2016-10-20 11:27:18.0</dc:date>
<skos:notation>SDN:P35::EPC00087</skos:notation>
<skos:prefLabel xml:lang="en">Suspended particulate material cadmium content</skos:prefLabel>
<skos:altLabel>SPM Cd</skos:altLabel>
<skos:definition xml:lang="en">Concentration of the metal in particles extracted by filtration (any type of filter) from a sample of a river, estuary, sea or ocean water or trapped in situ expressed per unit dry weight of the particles by any method.</skos:definition>
<owl:versionInfo>3</owl:versionInfo>
<pav:hasCurrentVersion rdf:resource="http://vocab.nerc.ac.uk/collection/P35/current/EPC00087/3/"/>
<pav:version>3</pav:version>
<pav:authoredOn>2016-10-20 11:27:18.0</pav:authoredOn>
<skos:note xml:lang="en">accepted</skos:note>
<owl:deprecated>false</owl:deprecated>
<skos:narrower rdf:resource="http://vocab.nerc.ac.uk/collection/P01/current/CDCNAAPC/"/>
<skos:narrower rdf:resource="http://vocab.nerc.ac.uk/collection/P01/current/MSPMM017/"/>
<skos:narrower rdf:resource="http://vocab.nerc.ac.uk/collection/P01/current/CDCNAAP2/"/>
<skos:narrower rdf:resource="http://vocab.nerc.ac.uk/collection/P01/current/CDCNICP2/"/>
<skos:narrower rdf:resource="http://vocab.nerc.ac.uk/collection/P01/current/MSPMM005/"/>
<skos:related rdf:resource="http://vocab.nerc.ac.uk/collection/P06/current/UMKG/"/>
<skos:broader rdf:resource="http://vocab.nerc.ac.uk/collection/P36/current/HVYMTL/"/>
<void:inDataset rdf:resource="http://vocab.nerc.ac.uk/.well-known/void"/>
</skos:Concept>
</skos:member>
<skos:member>
<skos:Concept rdf:about="http://vocab.nerc.ac.uk/collection/P35/current/EPC00088/">
<dc:identifier>SDN:P35::EPC00088</dc:identifier>
<dce:identifier>SDN:P35::EPC00088</dce:identifier>
<dc:date>2016-10-20 11:27:18.0</dc:date>
<skos:notation>SDN:P35::EPC00088</skos:notation>
<skos:prefLabel xml:lang="en">Suspended particulate material chromium content</skos:prefLabel>
<skos:altLabel>SPM Cr</skos:altLabel>
<skos:definition xml:lang="en">Concentration of the metal in particles extracted by filtration (any type of filter) from a sample of a river, estuary, sea or ocean water or trapped in situ expressed per unit dry weight of the particles by any method.</skos:definition>
<owl:versionInfo>3</owl:versionInfo>
<pav:hasCurrentVersion rdf:resource="http://vocab.nerc.ac.uk/collection/P35/current/EPC00088/3/"/>
<pav:version>3</pav:version>
<pav:authoredOn>2016-10-20 11:27:18.0</pav:authoredOn>
<skos:note xml:lang="en">accepted</skos:note>
<owl:deprecated>false</owl:deprecated>
<skos:narrower rdf:resource="http://vocab.nerc.ac.uk/collection/P01/current/MSPMM018/"/>
<skos:narrower rdf:resource="http://vocab.nerc.ac.uk/collection/P01/current/CRCNAAP2/"/>
<skos:narrower rdf:resource="http://vocab.nerc.ac.uk/collection/P01/current/CRCNAAPC/"/>
<skos:narrower rdf:resource="http://vocab.nerc.ac.uk/collection/P01/current/MSPMM006/"/>
<skos:related rdf:resource="http://vocab.nerc.ac.uk/collection/P06/current/UMKG/"/>
<skos:broader rdf:resource="http://vocab.nerc.ac.uk/collection/P36/current/HVYMTL/"/>
<void:inDataset rdf:resource="http://vocab.nerc.ac.uk/.well-known/void"/>
</skos:Concept>
</skos:member>
<skos:member>
<skos:Concept rdf:about="http://vocab.nerc.ac.uk/collection/P35/current/EPC00089/">
<dc:identifier>SDN:P35::EPC00089</dc:identifier>
<dce:identifier>SDN:P35::EPC00089</dce:identifier>
<dc:date>2016-10-20 11:27:18.0</dc:date>
<skos:notation>SDN:P35::EPC00089</skos:notation>
<skos:prefLabel xml:lang="en">Suspended particulate material cobalt content</skos:prefLabel>
<skos:altLabel>SPM Co</skos:altLabel>
<skos:definition xml:lang="en">Concentration of the metal in particles extracted by filtration (any type of filter) from a sample of a river, estuary, sea or ocean water or trapped in situ expressed per unit dry weight of the particles by any method.</skos:definition>
<owl:versionInfo>3</owl:versionInfo>
<pav:hasCurrentVersion rdf:resource="http://vocab.nerc.ac.uk/collection/P35/current/EPC00089/3/"/>
<pav:version>3</pav:version>
<pav:authoredOn>2016-10-20 11:27:18.0</pav:authoredOn>
<skos:note xml:lang="en">accepted</skos:note>
<owl:deprecated>false</owl:deprecated>
<skos:narrower rdf:resource="http://vocab.nerc.ac.uk/collection/P01/current/COCNAAPC/"/>
<skos:narrower rdf:resource="http://vocab.nerc.ac.uk/collection/P01/current/COCNICP2/"/>
<skos:narrower rdf:resource="http://vocab.nerc.ac.uk/collection/P01/current/COCNXXP2/"/>
<skos:narrower rdf:resource="http://vocab.nerc.ac.uk/collection/P01/current/COCNAAP2/"/>
<skos:related rdf:resource="http://vocab.nerc.ac.uk/collection/P06/current/UMKG/"/>
<skos:broader rdf:resource="http://vocab.nerc.ac.uk/collection/P36/current/HVYMTL/"/>
<void:inDataset rdf:resource="http://vocab.nerc.ac.uk/.well-known/void"/>
</skos:Concept>
</skos:member>
<skos:member>
<skos:Concept rdf:about="http://vocab.nerc.ac.uk/collection/P35/current/EPC00090/">
<dc:identifier>SDN:P35::EPC00090</dc:identifier>
<dce:identifier>SDN:P35::EPC00090</dce:identifier>
<dc:date>2016-10-20 11:27:18.0</dc:date>
<skos:notation>SDN:P35::EPC00090</skos:notation>
<skos:prefLabel xml:lang="en">Suspended particulate material copper content</skos:prefLabel>
<skos:altLabel>SPM Cu</skos:altLabel>
<skos:definition xml:lang="en">Concentration of the metal in particles extracted by filtration (any type of filter) from a sample of a river, estuary, sea or ocean water or trapped in situ expressed per unit dry weight of the particles by any method.</skos:definition>
<owl:versionInfo>3</owl:versionInfo>
<pav:hasCurrentVersion rdf:resource="http://vocab.nerc.ac.uk/collection/P35/current/EPC00090/3/"/>
<pav:version>3</pav:version>
<pav:authoredOn>2016-10-20 11:27:18.0</pav:authoredOn>
<skos:note xml:lang="en">accepted</skos:note>
<owl:deprecated>false</owl:deprecated>
<skos:narrower rdf:resource="http://vocab.nerc.ac.uk/collection/P01/current/MSPMM019/"/>
<skos:narrower rdf:resource="http://vocab.nerc.ac.uk/collection/P01/current/CUCNICP2/"/>
<skos:narrower rdf:resource="http://vocab.nerc.ac.uk/collection/P01/current/CUCNAAPC/"/>
<skos:narrower rdf:resource="http://vocab.nerc.ac.uk/collection/P01/current/CUCNAAP2/"/>
<skos:narrower rdf:resource="http://vocab.nerc.ac.uk/collection/P01/current/MSPMM007/"/>
<skos:related rdf:resource="http://vocab.nerc.ac.uk/collection/P06/current/UMKG/"/>
<skos:broader rdf:resource="http://vocab.nerc.ac.uk/collection/P36/current/HVYMTL/"/>
<void:inDataset rdf:resource="http://vocab.nerc.ac.uk/.well-known/void"/>
</skos:Concept>
</skos:member>
<skos:member>
<skos:Concept rdf:about="http://vocab.nerc.ac.uk/collection/P35/current/EPC00091/">
<dc:identifier>SDN:P35::EPC00091</dc:identifier>
<dce:identifier>SDN:P35::EPC00091</dce:identifier>
<dc:date>2016-10-20 11:27:18.0</dc:date>
<skos:notation>SDN:P35::EPC00091</skos:notation>
<skos:prefLabel xml:lang="en">Suspended particulate material iron (total chemical species) content</skos:prefLabel>
<skos:altLabel>SPM total Fe</skos:altLabel>
<skos:definition xml:lang="en">Concentration of the metal in particles extracted by filtration (any type of filter) from a sample of a river, estuary, sea or ocean water or trapped in situ expressed per unit dry weight of the particles by any method. Total means the element in all possible states of valency and chemical combination.</skos:definition>
<owl:versionInfo>4</owl:versionInfo>
<pav:hasCurrentVersion rdf:resource="http://vocab.nerc.ac.uk/collection/P35/current/EPC00091/4/"/>
<pav:version>4</pav:version>
<pav:authoredOn>2016-10-20 11:27:18.0</pav:authoredOn>
<skos:note xml:lang="en">accepted</skos:note>
<owl:deprecated>false</owl:deprecated>
<skos:narrower rdf:resource="http://vocab.nerc.ac.uk/collection/P01/current/FECNAAP2/"/>
<skos:narrower rdf:resource="http://vocab.nerc.ac.uk/collection/P01/current/MFEPP012/"/>
<skos:narrower rdf:resource="http://vocab.nerc.ac.uk/collection/P01/current/FECNICP2/"/>
<skos:narrower rdf:resource="http://vocab.nerc.ac.uk/collection/P01/current/FECNPEXX/"/>
<skos:narrower rdf:resource="http://vocab.nerc.ac.uk/collection/P01/current/FECNXXP2/"/>
<skos:narrower rdf:resource="http://vocab.nerc.ac.uk/collection/P01/current/FECNAAPC/"/>
<skos:related rdf:resource="http://vocab.nerc.ac.uk/collection/P06/current/UMKG/"/>
<skos:broader rdf:resource="http://vocab.nerc.ac.uk/collection/P36/current/HVYMTL/"/>
<void:inDataset rdf:resource="http://vocab.nerc.ac.uk/.well-known/void"/>
</skos:Concept>
</skos:member>
<skos:member>
<skos:Concept rdf:about="http://vocab.nerc.ac.uk/collection/P35/current/EPC00092/">
<dc:identifier>SDN:P35::EPC00092</dc:identifier>
<dce:identifier>SDN:P35::EPC00092</dce:identifier>
<dc:date>2016-10-20 11:27:18.0</dc:date>
<skos:notation>SDN:P35::EPC00092</skos:notation>
<skos:prefLabel xml:lang="en">Suspended particulate material lead content</skos:prefLabel>
<skos:altLabel>SPM Pb</skos:altLabel>
<skos:definition xml:lang="en">Concentration of the metal in particles extracted by filtration (any type of filter) from a sample of a river, estuary, sea or ocean water or trapped in situ expressed per unit dry weight of the particles by any method.</skos:definition>
<owl:versionInfo>3</owl:versionInfo>
<pav:hasCurrentVersion rdf:resource="http://vocab.nerc.ac.uk/collection/P35/current/EPC00092/3/"/>
<pav:version>3</pav:version>
<pav:authoredOn>2016-10-20 11:27:18.0</pav:authoredOn>
<skos:note xml:lang="en">accepted</skos:note>
<owl:deprecated>false</owl:deprecated>
<skos:narrower rdf:resource="http://vocab.nerc.ac.uk/collection/P01/current/PBCNICXX/"/>
<skos:narrower rdf:resource="http://vocab.nerc.ac.uk/collection/P01/current/MSPMM020/"/>
<skos:narrower rdf:resource="http://vocab.nerc.ac.uk/collection/P01/current/PBCNXXP2/"/>
<skos:narrower rdf:resource="http://vocab.nerc.ac.uk/collection/P01/current/PBCNICP2/"/>
<skos:narrower rdf:resource="http://vocab.nerc.ac.uk/collection/P01/current/PBCNAAPC/"/>
<skos:narrower rdf:resource="http://vocab.nerc.ac.uk/collection/P01/current/PBCNAAP2/"/>
<skos:narrower rdf:resource="http://vocab.nerc.ac.uk/collection/P01/current/MSPMM008/"/>
<skos:related rdf:resource="http://vocab.nerc.ac.uk/collection/P06/current/UMKG/"/>
<skos:broader rdf:resource="http://vocab.nerc.ac.uk/collection/P36/current/HVYMTL/"/>
<void:inDataset rdf:resource="http://vocab.nerc.ac.uk/.well-known/void"/>
</skos:Concept>
</skos:member>
<skos:member>
<skos:Concept rdf:about="http://vocab.nerc.ac.uk/collection/P35/current/EPC00093/">
<dc:identifier>SDN:P35::EPC00093</dc:identifier>
<dce:identifier>SDN:P35::EPC00093</dce:identifier>
<dc:date>2016-10-20 11:27:18.0</dc:date>
<skos:notation>SDN:P35::EPC00093</skos:notation>
<skos:prefLabel xml:lang="en">Suspended particulate material lithium content</skos:prefLabel>
<skos:altLabel>SPM Li</skos:altLabel>
<skos:definition xml:lang="en">Concentration of the metal in particles extracted by filtration (any type of filter) from a sample of a river, estuary, sea or ocean water or trapped in situ expressed per unit dry weight of the particles by any method.</skos:definition>
<owl:versionInfo>3</owl:versionInfo>
<pav:hasCurrentVersion rdf:resource="http://vocab.nerc.ac.uk/collection/P35/current/EPC00093/3/"/>
<pav:version>3</pav:version>
<pav:authoredOn>2016-10-20 11:27:18.0</pav:authoredOn>
<skos:note xml:lang="en">accepted</skos:note>
<owl:deprecated>false</owl:deprecated>
<skos:narrower rdf:resource="http://vocab.nerc.ac.uk/collection/P01/current/LICNAAP2/"/>
<skos:narrower rdf:resource="http://vocab.nerc.ac.uk/collection/P01/current/LICNAAPC/"/>
<skos:related rdf:resource="http://vocab.nerc.ac.uk/collection/P06/current/UMKG/"/>
<skos:broader rdf:resource="http://vocab.nerc.ac.uk/collection/P36/current/HVYMTL/"/>
<void:inDataset rdf:resource="http://vocab.nerc.ac.uk/.well-known/void"/>
</skos:Concept>
</skos:member>
<skos:member>
<skos:Concept rdf:about="http://vocab.nerc.ac.uk/collection/P35/current/EPC00094/">
<dc:identifier>SDN:P35::EPC00094</dc:identifier>
<dce:identifier>SDN:P35::EPC00094</dce:identifier>
<dc:date>2016-10-20 11:27:18.0</dc:date>
<skos:notation>SDN:P35::EPC00094</skos:notation>
<skos:prefLabel xml:lang="en">Suspended particulate material manganese (total chemical species) content</skos:prefLabel>
<skos:altLabel>SPM total Mn</skos:altLabel>
<skos:definition xml:lang="en">Concentration of the metal in particles extracted by filtration (any type of filter) from a sample of a river, estuary, sea or ocean water or trapped in situ expressed per unit dry weight of the particles by any method. Total means the element in all possible states of valency and chemical combination.</skos:definition>
<owl:versionInfo>3</owl:versionInfo>
<pav:hasCurrentVersion rdf:resource="http://vocab.nerc.ac.uk/collection/P35/current/EPC00094/3/"/>
<pav:version>3</pav:version>
<pav:authoredOn>2016-10-20 11:27:18.0</pav:authoredOn>
<skos:note xml:lang="en">accepted</skos:note>
<owl:deprecated>false</owl:deprecated>
<skos:narrower rdf:resource="http://vocab.nerc.ac.uk/collection/P01/current/MNCNAAPC/"/>
<skos:narrower rdf:resource="http://vocab.nerc.ac.uk/collection/P01/current/MNCNAAP2/"/>
<skos:narrower rdf:resource="http://vocab.nerc.ac.uk/collection/P01/current/MNCNPEXX/"/>
<skos:narrower rdf:resource="http://vocab.nerc.ac.uk/collection/P01/current/MMNPP012/"/>
<skos:related rdf:resource="http://vocab.nerc.ac.uk/collection/P06/current/UMKG/"/>
<skos:broader rdf:resource="http://vocab.nerc.ac.uk/collection/P36/current/HVYMTL/"/>
<void:inDataset rdf:resource="http://vocab.nerc.ac.uk/.well-known/void"/>
</skos:Concept>
</skos:member>
<skos:member>
<skos:Concept rdf:about="http://vocab.nerc.ac.uk/collection/P35/current/EPC00095/">
<dc:identifier>SDN:P35::EPC00095</dc:identifier>
<dce:identifier>SDN:P35::EPC00095</dce:identifier>
<dc:date>2016-10-20 11:27:18.0</dc:date>
<skos:notation>SDN:P35::EPC00095</skos:notation>
<skos:prefLabel xml:lang="en">Suspended particulate material mercury (total chemical species) content</skos:prefLabel>
<skos:altLabel>SPM total Hg</skos:altLabel>
<skos:definition xml:lang="en">Concentration of the metal in particles extracted by filtration (any type of filter) from a sample of a river, estuary, sea or ocean water or trapped in situ expressed per unit dry weight of the particles by any method. Total means the element in all possible states of valency and chemical combination.</skos:definition>
<owl:versionInfo>3</owl:versionInfo>
<pav:hasCurrentVersion rdf:resource="http://vocab.nerc.ac.uk/collection/P35/current/EPC00095/3/"/>
<pav:version>3</pav:version>
<pav:authoredOn>2016-10-20 11:27:18.0</pav:authoredOn>
<skos:note xml:lang="en">accepted</skos:note>
<owl:deprecated>false</owl:deprecated>
<skos:narrower rdf:resource="http://vocab.nerc.ac.uk/collection/P01/current/CHEMM005/"/>
<skos:narrower rdf:resource="http://vocab.nerc.ac.uk/collection/P01/current/MSPMM021/"/>
<skos:narrower rdf:resource="http://vocab.nerc.ac.uk/collection/P01/current/MSPMM001/"/>
<skos:related rdf:resource="http://vocab.nerc.ac.uk/collection/P06/current/UMKG/"/>
<skos:broader rdf:resource="http://vocab.nerc.ac.uk/collection/P36/current/HVYMTL/"/>
<void:inDataset rdf:resource="http://vocab.nerc.ac.uk/.well-known/void"/>
</skos:Concept>
</skos:member>
<skos:member>
<skos:Concept rdf:about="http://vocab.nerc.ac.uk/collection/P35/current/EPC00096/">
<dc:identifier>SDN:P35::EPC00096</dc:identifier>
<dce:identifier>SDN:P35::EPC00096</dce:identifier>
<dc:date>2016-10-20 11:27:18.0</dc:date>
<skos:notation>SDN:P35::EPC00096</skos:notation>
<skos:prefLabel xml:lang="en">Suspended particulate material molybdenum content</skos:prefLabel>
<skos:altLabel>SPM Mo</skos:altLabel>
<skos:definition xml:lang="en">Concentration of the metal in particles extracted by filtration (any type of filter) from a sample of a river, estuary, sea or ocean water or trapped in situ expressed per unit dry weight of the particles by any method.</skos:definition>
<owl:versionInfo>3</owl:versionInfo>
<pav:hasCurrentVersion rdf:resource="http://vocab.nerc.ac.uk/collection/P35/current/EPC00096/3/"/>
<pav:version>3</pav:version>
<pav:authoredOn>2016-10-20 11:27:18.0</pav:authoredOn>
<skos:note xml:lang="en">accepted</skos:note>
<owl:deprecated>false</owl:deprecated>
<skos:narrower rdf:resource="http://vocab.nerc.ac.uk/collection/P01/current/MOCNXXP2/"/>
<skos:related rdf:resource="http://vocab.nerc.ac.uk/collection/P06/current/UMKG/"/>
<skos:broader rdf:resource="http://vocab.nerc.ac.uk/collection/P36/current/HVYMTL/"/>
<void:inDataset rdf:resource="http://vocab.nerc.ac.uk/.well-known/void"/>
</skos:Concept>
</skos:member>
<skos:member>
<skos:Concept rdf:about="http://vocab.nerc.ac.uk/collection/P35/current/EPC00097/">
<dc:identifier>SDN:P35::EPC00097</dc:identifier>
<dce:identifier>SDN:P35::EPC00097</dce:identifier>
<dc:date>2016-10-20 11:27:18.0</dc:date>
<skos:notation>SDN:P35::EPC00097</skos:notation>
<skos:prefLabel xml:lang="en">Suspended particulate material nickel content</skos:prefLabel>
<skos:altLabel>SPM Ni</skos:altLabel>
<skos:definition xml:lang="en">Concentration of the metal in particles extracted by filtration (any type of filter) from a sample of a river, estuary, sea or ocean water or trapped in situ expressed per unit dry weight of the particles by any method.</skos:definition>
<owl:versionInfo>3</owl:versionInfo>
<pav:hasCurrentVersion rdf:resource="http://vocab.nerc.ac.uk/collection/P35/current/EPC00097/3/"/>
<pav:version>3</pav:version>
<pav:authoredOn>2016-10-20 11:27:18.0</pav:authoredOn>
<skos:note xml:lang="en">accepted</skos:note>
<owl:deprecated>false</owl:deprecated>
<skos:narrower rdf:resource="http://vocab.nerc.ac.uk/collection/P01/current/NICNXXP2/"/>
<skos:narrower rdf:resource="http://vocab.nerc.ac.uk/collection/P01/current/NICNICP2/"/>
<skos:narrower rdf:resource="http://vocab.nerc.ac.uk/collection/P01/current/NICNAAP2/"/>
<skos:narrower rdf:resource="http://vocab.nerc.ac.uk/collection/P01/current/MSPMM022/"/>
<skos:narrower rdf:resource="http://vocab.nerc.ac.uk/collection/P01/current/MSPMM009/"/>
<skos:narrower rdf:resource="http://vocab.nerc.ac.uk/collection/P01/current/NICNAAPC/"/>
<skos:related rdf:resource="http://vocab.nerc.ac.uk/collection/P06/current/UMKG/"/>
<skos:broader rdf:resource="http://vocab.nerc.ac.uk/collection/P36/current/HVYMTL/"/>
<void:inDataset rdf:resource="http://vocab.nerc.ac.uk/.well-known/void"/>
</skos:Concept>
</skos:member>
<skos:member>
<skos:Concept rdf:about="http://vocab.nerc.ac.uk/collection/P35/current/EPC00098/">
<dc:identifier>SDN:P35::EPC00098</dc:identifier>
<dce:identifier>SDN:P35::EPC00098</dce:identifier>
<dc:date>2016-10-20 11:27:18.0</dc:date>
<skos:notation>SDN:P35::EPC00098</skos:notation>
<skos:prefLabel xml:lang="en">Suspended particulate material rubidium content</skos:prefLabel>
<skos:altLabel>SPM Rb</skos:altLabel>
<skos:definition xml:lang="en">Concentration of the metal in particles extracted by filtration (any type of filter) from a sample of a river, estuary, sea or ocean water or trapped in situ expressed per unit dry weight of the particles by any method.</skos:definition>
<owl:versionInfo>3</owl:versionInfo>
<pav:hasCurrentVersion rdf:resource="http://vocab.nerc.ac.uk/collection/P35/current/EPC00098/3/"/>
<pav:version>3</pav:version>
<pav:authoredOn>2016-10-20 11:27:18.0</pav:authoredOn>
<skos:note xml:lang="en">accepted</skos:note>
<owl:deprecated>false</owl:deprecated>
<skos:narrower rdf:resource="http://vocab.nerc.ac.uk/collection/P01/current/RBCNICXX/"/>
<skos:related rdf:resource="http://vocab.nerc.ac.uk/collection/P06/current/UMKG/"/>
<skos:broader rdf:resource="http://vocab.nerc.ac.uk/collection/P36/current/HVYMTL/"/>
<void:inDataset rdf:resource="http://vocab.nerc.ac.uk/.well-known/void"/>
</skos:Concept>
</skos:member>
<skos:member>
<skos:Concept rdf:about="http://vocab.nerc.ac.uk/collection/P35/current/EPC00099/">
<dc:identifier>SDN:P35::EPC00099</dc:identifier>
<dce:identifier>SDN:P35::EPC00099</dce:identifier>
<dc:date>2016-10-20 11:27:18.0</dc:date>
<skos:notation>SDN:P35::EPC00099</skos:notation>
<skos:prefLabel xml:lang="en">Suspended particulate material silver content</skos:prefLabel>
<skos:altLabel>SPM Ag</skos:altLabel>
<skos:definition xml:lang="en">Concentration of the metal in particles extracted by filtration (any type of filter) from a sample of a river, estuary, sea or ocean water or trapped in situ expressed per unit dry weight of the particles by any method.</skos:definition>
<owl:versionInfo>3</owl:versionInfo>
<pav:hasCurrentVersion rdf:resource="http://vocab.nerc.ac.uk/collection/P35/current/EPC00099/3/"/>
<pav:version>3</pav:version>
<pav:authoredOn>2016-10-20 11:27:18.0</pav:authoredOn>
<skos:note xml:lang="en">accepted</skos:note>
<owl:deprecated>false</owl:deprecated>
<skos:narrower rdf:resource="http://vocab.nerc.ac.uk/collection/P01/current/AGCNICP2/"/>
<skos:narrower rdf:resource="http://vocab.nerc.ac.uk/collection/P01/current/AGCNAAP2/"/>
<skos:related rdf:resource="http://vocab.nerc.ac.uk/collection/P06/current/UMKG/"/>
<skos:broader rdf:resource="http://vocab.nerc.ac.uk/collection/P36/current/HVYMTL/"/>
<void:inDataset rdf:resource="http://vocab.nerc.ac.uk/.well-known/void"/>
</skos:Concept>
</skos:member>
<skos:member>
<skos:Concept rdf:about="http://vocab.nerc.ac.uk/collection/P35/current/EPC00100/">
<dc:identifier>SDN:P35::EPC00100</dc:identifier>
<dce:identifier>SDN:P35::EPC00100</dce:identifier>
<dc:date>2016-10-20 11:27:18.0</dc:date>
<skos:notation>SDN:P35::EPC00100</skos:notation>
<skos:prefLabel xml:lang="en">Suspended particulate material strontium content</skos:prefLabel>
<skos:altLabel>SPM Sr</skos:altLabel>
<skos:definition xml:lang="en">Concentration of the metal in particles extracted by filtration (any type of filter) from a sample of a river, estuary, sea or ocean water or trapped in situ expressed per unit dry weight of the particles by any method.</skos:definition>
<owl:versionInfo>3</owl:versionInfo>
<pav:hasCurrentVersion rdf:resource="http://vocab.nerc.ac.uk/collection/P35/current/EPC00100/3/"/>
<pav:version>3</pav:version>
<pav:authoredOn>2016-10-20 11:27:18.0</pav:authoredOn>
<skos:note xml:lang="en">accepted</skos:note>
<owl:deprecated>false</owl:deprecated>
<skos:narrower rdf:resource="http://vocab.nerc.ac.uk/collection/P01/current/SRCNAAP2/"/>
<skos:narrower rdf:resource="http://vocab.nerc.ac.uk/collection/P01/current/SRCNICP2/"/>
<skos:narrower rdf:resource="http://vocab.nerc.ac.uk/collection/P01/current/SRCNICXX/"/>
<skos:related rdf:resource="http://vocab.nerc.ac.uk/collection/P06/current/UMKG/"/>
<skos:broader rdf:resource="http://vocab.nerc.ac.uk/collection/P36/current/HVYMTL/"/>
<void:inDataset rdf:resource="http://vocab.nerc.ac.uk/.well-known/void"/>
</skos:Concept>
</skos:member>
<skos:member>
<skos:Concept rdf:about="http://vocab.nerc.ac.uk/collection/P35/current/EPC00101/">
<dc:identifier>SDN:P35::EPC00101</dc:identifier>
<dce:identifier>SDN:P35::EPC00101</dce:identifier>
<dc:date>2016-10-20 11:27:18.0</dc:date>
<skos:notation>SDN:P35::EPC00101</skos:notation>
<skos:prefLabel xml:lang="en">Suspended particulate material titanium content</skos:prefLabel>
<skos:altLabel>SPM Ti</skos:altLabel>
<skos:definition xml:lang="en">Concentration of the metal in particles extracted by filtration (any type of filter) from a sample of a river, estuary, sea or ocean water or trapped in situ expressed per unit dry weight of the particles by any method.</skos:definition>
<owl:versionInfo>3</owl:versionInfo>
<pav:hasCurrentVersion rdf:resource="http://vocab.nerc.ac.uk/collection/P35/current/EPC00101/3/"/>
<pav:version>3</pav:version>
<pav:authoredOn>2016-10-20 11:27:18.0</pav:authoredOn>
<skos:note xml:lang="en">accepted</skos:note>
<owl:deprecated>false</owl:deprecated>
<skos:narrower rdf:resource="http://vocab.nerc.ac.uk/collection/P01/current/MTIPP012/"/>
<skos:narrower rdf:resource="http://vocab.nerc.ac.uk/collection/P01/current/TICNPEXX/"/>
<skos:related rdf:resource="http://vocab.nerc.ac.uk/collection/P06/current/UMKG/"/>
<skos:broader rdf:resource="http://vocab.nerc.ac.uk/collection/P36/current/HVYMTL/"/>
<void:inDataset rdf:resource="http://vocab.nerc.ac.uk/.well-known/void"/>
</skos:Concept>
</skos:member>
<skos:member>
<skos:Concept rdf:about="http://vocab.nerc.ac.uk/collection/P35/current/EPC00102/">
<dc:identifier>SDN:P35::EPC00102</dc:identifier>
<dce:identifier>SDN:P35::EPC00102</dce:identifier>
<dc:date>2016-10-20 11:27:18.0</dc:date>
<skos:notation>SDN:P35::EPC00102</skos:notation>
<skos:prefLabel xml:lang="en">Suspended particulate material uranium content</skos:prefLabel>
<skos:altLabel>SPM U</skos:altLabel>
<skos:definition xml:lang="en">Concentration of the metal in particles extracted by filtration (any type of filter) from a sample of a river, estuary, sea or ocean water or trapped in situ expressed per unit dry weight of the particles by any method.</skos:definition>
<owl:versionInfo>3</owl:versionInfo>
<pav:hasCurrentVersion rdf:resource="http://vocab.nerc.ac.uk/collection/P35/current/EPC00102/3/"/>
<pav:version>3</pav:version>
<pav:authoredOn>2016-10-20 11:27:18.0</pav:authoredOn>
<skos:note xml:lang="en">accepted</skos:note>
<owl:deprecated>false</owl:deprecated>
<skos:narrower rdf:resource="http://vocab.nerc.ac.uk/collection/P01/current/UXCNICXX/"/>
<skos:related rdf:resource="http://vocab.nerc.ac.uk/collection/P06/current/UMKG/"/>
<skos:broader rdf:resource="http://vocab.nerc.ac.uk/collection/P36/current/HVYMTL/"/>
<void:inDataset rdf:resource="http://vocab.nerc.ac.uk/.well-known/void"/>
</skos:Concept>
</skos:member>
<skos:member>
<skos:Concept rdf:about="http://vocab.nerc.ac.uk/collection/P35/current/EPC00103/">
<dc:identifier>SDN:P35::EPC00103</dc:identifier>
<dce:identifier>SDN:P35::EPC00103</dce:identifier>
<dc:date>2016-10-20 11:27:18.0</dc:date>
<skos:notation>SDN:P35::EPC00103</skos:notation>
<skos:prefLabel xml:lang="en">Suspended particulate material vanadium content</skos:prefLabel>
<skos:altLabel>SPM V</skos:altLabel>
<skos:definition xml:lang="en">Concentration of the metal in particles extracted by filtration (any type of filter) from a sample of a river, estuary, sea or ocean water or trapped in situ expressed per unit dry weight of the particles by any method.</skos:definition>
<owl:versionInfo>3</owl:versionInfo>
<pav:hasCurrentVersion rdf:resource="http://vocab.nerc.ac.uk/collection/P35/current/EPC00103/3/"/>
<pav:version>3</pav:version>
<pav:authoredOn>2016-10-20 11:27:18.0</pav:authoredOn>
<skos:note xml:lang="en">accepted</skos:note>
<owl:deprecated>false</owl:deprecated>
<skos:narrower rdf:resource="http://vocab.nerc.ac.uk/collection/P01/current/VXCNXXP2/"/>
<skos:related rdf:resource="http://vocab.nerc.ac.uk/collection/P06/current/UMKG/"/>
<skos:broader rdf:resource="http://vocab.nerc.ac.uk/collection/P36/current/HVYMTL/"/>
<void:inDataset rdf:resource="http://vocab.nerc.ac.uk/.well-known/void"/>
</skos:Concept>
</skos:member>
<skos:member>
<skos:Concept rdf:about="http://vocab.nerc.ac.uk/collection/P35/current/EPC00104/">
<dc:identifier>SDN:P35::EPC00104</dc:identifier>
<dce:identifier>SDN:P35::EPC00104</dce:identifier>
<dc:date>2016-10-20 11:27:18.0</dc:date>
<skos:notation>SDN:P35::EPC00104</skos:notation>
<skos:prefLabel xml:lang="en">Suspended particulate material zinc content</skos:prefLabel>
<skos:altLabel>SPM Zn</skos:altLabel>
<skos:definition xml:lang="en">Concentration of the metal in particles extracted by filtration (any type of filter) from a sample of a river, estuary, sea or ocean water or trapped in situ expressed per unit dry weight of the particles by any method.</skos:definition>
<owl:versionInfo>3</owl:versionInfo>
<pav:hasCurrentVersion rdf:resource="http://vocab.nerc.ac.uk/collection/P35/current/EPC00104/3/"/>
<pav:version>3</pav:version>
<pav:authoredOn>2016-10-20 11:27:18.0</pav:authoredOn>
<skos:note xml:lang="en">accepted</skos:note>
<owl:deprecated>false</owl:deprecated>
<skos:narrower rdf:resource="http://vocab.nerc.ac.uk/collection/P01/current/MSPMM010/"/>
<skos:narrower rdf:resource="http://vocab.nerc.ac.uk/collection/P01/current/MSPMM023/"/>
<skos:narrower rdf:resource="http://vocab.nerc.ac.uk/collection/P01/current/ZNCNAAP2/"/>
<skos:narrower rdf:resource="http://vocab.nerc.ac.uk/collection/P01/current/ZNCNAAPC/"/>
<skos:narrower rdf:resource="http://vocab.nerc.ac.uk/collection/P01/current/ZNCNICP2/"/>
<skos:narrower rdf:resource="http://vocab.nerc.ac.uk/collection/P01/current/ZNCNXXP2/"/>
<skos:related rdf:resource="http://vocab.nerc.ac.uk/collection/P06/current/UMKG/"/>
<skos:broader rdf:resource="http://vocab.nerc.ac.uk/collection/P36/current/HVYMTL/"/>
<void:inDataset rdf:resource="http://vocab.nerc.ac.uk/.well-known/void"/>
</skos:Concept>
</skos:member>
<skos:member>
<skos:Concept rdf:about="http://vocab.nerc.ac.uk/collection/P35/current/EPC00209/">
<dc:identifier>SDN:P35::EPC00209</dc:identifier>
<dce:identifier>SDN:P35::EPC00209</dce:identifier>
<dc:date>2016-12-12 15:20:45.0</dc:date>
<skos:notation>SDN:P35::EPC00209</skos:notation>
<skos:prefLabel xml:lang="en">Total alkalinity in the sediment</skos:prefLabel>
<skos:altLabel>Total alkalinity in the sediment</skos:altLabel>
<skos:definition xml:lang="en">Total alkalinity in sediment pore water.</skos:definition>
<owl:versionInfo>5</owl:versionInfo>
<pav:hasCurrentVersion rdf:resource="http://vocab.nerc.ac.uk/collection/P35/current/EPC00209/5/"/>
<pav:version>5</pav:version>
<pav:authoredOn>2016-12-12 15:20:45.0</pav:authoredOn>
<skos:note xml:lang="en">accepted</skos:note>
<owl:deprecated>false</owl:deprecated>
<skos:narrower rdf:resource="http://vocab.nerc.ac.uk/collection/P01/current/SEDPWALK/"/>
<skos:narrower rdf:resource="http://vocab.nerc.ac.uk/collection/P01/current/NEWCXX10/"/>
<skos:related rdf:resource="http://vocab.nerc.ac.uk/collection/P06/current/UUKG/"/>
<skos:broader rdf:resource="http://vocab.nerc.ac.uk/collection/P36/current/ACIDIT/"/>
<void:inDataset rdf:resource="http://vocab.nerc.ac.uk/.well-known/void"/>
</skos:Concept>
</skos:member>
<skos:member>
<skos:Concept rdf:about="http://vocab.nerc.ac.uk/collection/P35/current/EPC00169/">
<dc:identifier>SDN:P35::EPC00169</dc:identifier>
<dce:identifier>SDN:P35::EPC00169</dce:identifier>
<dc:date>2018-03-20 16:58:29.0</dc:date>
<skos:notation>SDN:P35::EPC00169</skos:notation>
<skos:prefLabel xml:lang="en">Tributyltin (TBT) in Mytilus</skos:prefLabel>
<skos:altLabel>Tributyltin (TBT) in Mytilus</skos:altLabel>
<skos:definition xml:lang="en">Concentration of tributyltin per unit weight (dry or wet) of Mytilus spp. (regardless of Mytilus size class).</skos:definition>
<owl:versionInfo>8</owl:versionInfo>
<pav:hasCurrentVersion rdf:resource="http://vocab.nerc.ac.uk/collection/P35/current/EPC00169/8/"/>
<pav:version>8</pav:version>
<pav:authoredOn>2018-03-20 16:58:29.0</pav:authoredOn>
<skos:note xml:lang="en">deprecated</skos:note>
<owl:deprecated>true</owl:deprecated>
<skos:narrower rdf:resource="http://vocab.nerc.ac.uk/collection/P01/current/ICES0616/"/>
<skos:narrower rdf:resource="http://vocab.nerc.ac.uk/collection/P01/current/TBMMCF14/"/>
<skos:narrower rdf:resource="http://vocab.nerc.ac.uk/collection/P01/current/MMUSTTBT/"/>
<skos:narrower rdf:resource="http://vocab.nerc.ac.uk/collection/P01/current/TBDWCF14/"/>
<skos:narrower rdf:resource="http://vocab.nerc.ac.uk/collection/P01/current/ICES0594/"/>
<skos:related rdf:resource="http://vocab.nerc.ac.uk/collection/P06/current/UUKG/"/>
<skos:broader rdf:resource="http://vocab.nerc.ac.uk/collection/P36/current/ANTIFL/"/>
<void:inDataset rdf:resource="http://vocab.nerc.ac.uk/.well-known/void"/>
</skos:Concept>
</skos:member>
<skos:member>
<skos:Concept rdf:about="http://vocab.nerc.ac.uk/collection/P35/current/EPC00210/">
<dc:identifier>SDN:P35::EPC00210</dc:identifier>
<dce:identifier>SDN:P35::EPC00210</dce:identifier>
<dc:date>2018-03-20 15:59:49.0</dc:date>
<skos:notation>SDN:P35::EPC00210</skos:notation>
<skos:prefLabel xml:lang="en">Tributyltin (TBT) in the sediment</skos:prefLabel>
<skos:altLabel>Tributyltin (TBT) in the sediment</skos:altLabel>
<skos:definition xml:lang="en">Concentration of tributyltin per unit dry weight of sediment (regardless of sediment size class).</skos:definition>
<owl:versionInfo>7</owl:versionInfo>
<pav:hasCurrentVersion rdf:resource="http://vocab.nerc.ac.uk/collection/P35/current/EPC00210/7/"/>
<pav:version>7</pav:version>
<pav:authoredOn>2018-03-20 15:59:49.0</pav:authoredOn>
<skos:note xml:lang="en">accepted</skos:note>
<owl:deprecated>false</owl:deprecated>
<skos:narrower rdf:resource="http://vocab.nerc.ac.uk/collection/P01/current/TBTSNSD1/"/>
<skos:narrower rdf:resource="http://vocab.nerc.ac.uk/collection/P01/current/AFLGMZZZ/"/>
<skos:related rdf:resource="http://vocab.nerc.ac.uk/collection/P06/current/UUKG/"/>
<skos:broader rdf:resource="http://vocab.nerc.ac.uk/collection/P36/current/ANTIFL/"/>
<void:inDataset rdf:resource="http://vocab.nerc.ac.uk/.well-known/void"/>
</skos:Concept>
</skos:member>
<skos:member>
<skos:Concept rdf:about="http://vocab.nerc.ac.uk/collection/P35/current/EPC00137/">
<dc:identifier>SDN:P35::EPC00137</dc:identifier>
<dce:identifier>SDN:P35::EPC00137</dce:identifier>
<dc:date>2018-03-20 16:58:29.0</dc:date>
<skos:notation>SDN:P35::EPC00137</skos:notation>
<skos:prefLabel xml:lang="en">Triphenyltin (TPT) in Mytilus</skos:prefLabel>
<skos:altLabel>Triphenyltin (TPT) in Mytilus</skos:altLabel>
<skos:definition xml:lang="en">Concentration of triphenyltin cation per unit weight (dry or wet) of Mytilus spp. (regardless of Mytilus species and size class).</skos:definition>
<owl:versionInfo>6</owl:versionInfo>
<pav:hasCurrentVersion rdf:resource="http://vocab.nerc.ac.uk/collection/P35/current/EPC00137/6/"/>
<pav:version>6</pav:version>
<pav:authoredOn>2018-03-20 16:58:29.0</pav:authoredOn>
<skos:note xml:lang="en">deprecated</skos:note>
<owl:deprecated>true</owl:deprecated>
<skos:narrower rdf:resource="http://vocab.nerc.ac.uk/collection/P01/current/CBIOM026/"/>
<skos:narrower rdf:resource="http://vocab.nerc.ac.uk/collection/P01/current/ICES0595/"/>
<skos:narrower rdf:resource="http://vocab.nerc.ac.uk/collection/P01/current/TPMMCF14/"/>
<skos:related rdf:resource="http://vocab.nerc.ac.uk/collection/P06/current/UUKG/"/>
<skos:broader rdf:resource="http://vocab.nerc.ac.uk/collection/P36/current/ANTIFL/"/>
<void:inDataset rdf:resource="http://vocab.nerc.ac.uk/.well-known/void"/>
</skos:Concept>
</skos:member>
<skos:member>
<skos:Concept rdf:about="http://vocab.nerc.ac.uk/collection/P35/current/EPC00151/">
<dc:identifier>SDN:P35::EPC00151</dc:identifier>
<dce:identifier>SDN:P35::EPC00151</dce:identifier>
<dc:date>2016-12-12 15:20:45.0</dc:date>
<skos:notation>SDN:P35::EPC00151</skos:notation>
<skos:prefLabel xml:lang="en">Triphenyltin (TPT) in the sediment</skos:prefLabel>
<skos:altLabel>Triphenyltin (TPT) in the sediment</skos:altLabel>
<skos:definition xml:lang="en">Concentration of triphenyltin cation per unit dry weight of sediment (regardless of sediment size class, analytical and normalization method).</skos:definition>
<owl:versionInfo>5</owl:versionInfo>
<pav:hasCurrentVersion rdf:resource="http://vocab.nerc.ac.uk/collection/P35/current/EPC00151/5/"/>
<pav:version>5</pav:version>
<pav:authoredOn>2016-12-12 15:20:45.0</pav:authoredOn>
<skos:note xml:lang="en">accepted</skos:note>
<owl:deprecated>false</owl:deprecated>
<skos:narrower rdf:resource="http://vocab.nerc.ac.uk/collection/P01/current/SDCTM005/"/>
<skos:narrower rdf:resource="http://vocab.nerc.ac.uk/collection/P01/current/AFLGMXXX/"/>
<skos:related rdf:resource="http://vocab.nerc.ac.uk/collection/P06/current/UUKG/"/>
<skos:broader rdf:resource="http://vocab.nerc.ac.uk/collection/P36/current/ANTIFL/"/>
<void:inDataset rdf:resource="http://vocab.nerc.ac.uk/.well-known/void"/>
</skos:Concept>
</skos:member>
<skos:member>
<skos:Concept rdf:about="http://vocab.nerc.ac.uk/collection/P35/current/EPC00195/">
<dc:identifier>SDN:P35::EPC00195</dc:identifier>
<dce:identifier>SDN:P35::EPC00195</dce:identifier>
<dc:date>2016-12-12 15:20:45.0</dc:date>
<skos:notation>SDN:P35::EPC00195</skos:notation>
<skos:prefLabel xml:lang="en">Water body Hexachlorobenzene {HCB}</skos:prefLabel>
<skos:altLabel>Water body Hexachlorobenzene {HCB}</skos:altLabel>
<skos:definition xml:lang="en">Concentration of hexachlorobenzene (dissolved, reactive particulate or suspended particulate material) per unit volume of a river, estuary, sea or ocean by any method in filtered or unfiltered water.</skos:definition>
<owl:versionInfo>5</owl:versionInfo>
<pav:hasCurrentVersion rdf:resource="http://vocab.nerc.ac.uk/collection/P35/current/EPC00195/5/"/>
<pav:version>5</pav:version>
<pav:authoredOn>2016-12-12 15:20:45.0</pav:authoredOn>
<skos:note xml:lang="en">accepted</skos:note>
<owl:deprecated>false</owl:deprecated>
<skos:narrower rdf:resource="http://vocab.nerc.ac.uk/collection/P01/current/HCBAFW01/"/>
<skos:narrower rdf:resource="http://vocab.nerc.ac.uk/collection/P01/current/WTCTM016/"/>
<skos:narrower rdf:resource="http://vocab.nerc.ac.uk/collection/P01/current/HCBUFW02/"/>
<skos:related rdf:resource="http://vocab.nerc.ac.uk/collection/P06/current/UGPL/"/>
<skos:broader rdf:resource="http://vocab.nerc.ac.uk/collection/P36/current/PESTBI/"/>
<void:inDataset rdf:resource="http://vocab.nerc.ac.uk/.well-known/void"/>
</skos:Concept>
</skos:member>
<skos:member>
<skos:Concept rdf:about="http://vocab.nerc.ac.uk/collection/P35/current/EPC00148/">
<dc:identifier>SDN:P35::EPC00148</dc:identifier>
<dce:identifier>SDN:P35::EPC00148</dce:identifier>
<dc:date>2016-12-12 15:20:45.0</dc:date>
<skos:notation>SDN:P35::EPC00148</skos:notation>
<skos:prefLabel xml:lang="en">Water body PCB101</skos:prefLabel>
<skos:altLabel>Water body PCB101</skos:altLabel>
<skos:definition xml:lang="en">Concentration of PCB101 (dissolved, reactive particulate or suspended particulate material) in river, estuary, sea or ocean by any method in filtered or unfiltered water.</skos:definition>
<owl:versionInfo>5</owl:versionInfo>
<pav:hasCurrentVersion rdf:resource="http://vocab.nerc.ac.uk/collection/P35/current/EPC00148/5/"/>
<pav:version>5</pav:version>
<pav:authoredOn>2016-12-12 15:20:45.0</pav:authoredOn>
<skos:note xml:lang="en">accepted</skos:note>
<owl:deprecated>false</owl:deprecated>
<skos:narrower rdf:resource="http://vocab.nerc.ac.uk/collection/P01/current/SCES0022/"/>
<skos:related rdf:resource="http://vocab.nerc.ac.uk/collection/P06/current/UGPL/"/>
<skos:broader rdf:resource="http://vocab.nerc.ac.uk/collection/P36/current/PCBSXX/"/>
<void:inDataset rdf:resource="http://vocab.nerc.ac.uk/.well-known/void"/>
</skos:Concept>
</skos:member>
<skos:member>
<skos:Concept rdf:about="http://vocab.nerc.ac.uk/collection/P35/current/EPC00175/">
<dc:identifier>SDN:P35::EPC00175</dc:identifier>
<dce:identifier>SDN:P35::EPC00175</dce:identifier>
<dc:date>2016-12-12 15:20:45.0</dc:date>
<skos:notation>SDN:P35::EPC00175</skos:notation>
<skos:prefLabel xml:lang="en">Water body PCB105</skos:prefLabel>
<skos:altLabel>Water body PCB105</skos:altLabel>
<skos:definition xml:lang="en">Concentration of PCB105 (dissolved, reactive particulate or suspended particulate material) per unit volume of a river, estuary, sea or ocean by any method in filtered or unfiltered water.</skos:definition>
<owl:versionInfo>5</owl:versionInfo>
<pav:hasCurrentVersion rdf:resource="http://vocab.nerc.ac.uk/collection/P35/current/EPC00175/5/"/>
<pav:version>5</pav:version>
<pav:authoredOn>2016-12-12 15:20:45.0</pav:authoredOn>
<skos:note xml:lang="en">accepted</skos:note>
<owl:deprecated>false</owl:deprecated>
<skos:related rdf:resource="http://vocab.nerc.ac.uk/collection/P06/current/UGPL/"/>
<skos:broader rdf:resource="http://vocab.nerc.ac.uk/collection/P36/current/PCBSXX/"/>
<void:inDataset rdf:resource="http://vocab.nerc.ac.uk/.well-known/void"/>
</skos:Concept>
</skos:member>
<skos:member>
<skos:Concept rdf:about="http://vocab.nerc.ac.uk/collection/P35/current/EPC00220/">
<dc:identifier>SDN:P35::EPC00220</dc:identifier>
<dce:identifier>SDN:P35::EPC00220</dce:identifier>
<dc:date>2016-12-12 15:20:45.0</dc:date>
<skos:notation>SDN:P35::EPC00220</skos:notation>
<skos:prefLabel xml:lang="en">Water body PCB118</skos:prefLabel>
<skos:altLabel>Water body PCB118</skos:altLabel>
<skos:definition xml:lang="en">Concentration of PCB118 (dissolved, reactive particulate or suspended particulate material) in a river, estaury, sea or ocean.</skos:definition>
<owl:versionInfo>5</owl:versionInfo>
<pav:hasCurrentVersion rdf:resource="http://vocab.nerc.ac.uk/collection/P35/current/EPC00220/5/"/>
<pav:version>5</pav:version>
<pav:authoredOn>2016-12-12 15:20:45.0</pav:authoredOn>
<skos:note xml:lang="en">accepted</skos:note>
<owl:deprecated>false</owl:deprecated>
<skos:narrower rdf:resource="http://vocab.nerc.ac.uk/collection/P01/current/AI18GCD1/"/>
<skos:narrower rdf:resource="http://vocab.nerc.ac.uk/collection/P01/current/SCES0027/"/>
<skos:related rdf:resource="http://vocab.nerc.ac.uk/collection/P06/current/UGPL/"/>
<skos:broader rdf:resource="http://vocab.nerc.ac.uk/collection/P36/current/PCBSXX/"/>
<void:inDataset rdf:resource="http://vocab.nerc.ac.uk/.well-known/void"/>
</skos:Concept>
</skos:member>
<skos:member>
<skos:Concept rdf:about="http://vocab.nerc.ac.uk/collection/P35/current/EPC00146/">
<dc:identifier>SDN:P35::EPC00146</dc:identifier>
<dce:identifier>SDN:P35::EPC00146</dce:identifier>
<dc:date>2016-12-12 15:20:45.0</dc:date>
<skos:notation>SDN:P35::EPC00146</skos:notation>
<skos:prefLabel xml:lang="en">Water body PCB138</skos:prefLabel>
<skos:altLabel>Water body PCB138</skos:altLabel>
<skos:definition xml:lang="en">Concentration of PCB138 (dissolved, reactive particulate or suspended particulate material) in river, estuary, sea or ocean by any method in filtered or unfiltered water.</skos:definition>
<owl:versionInfo>5</owl:versionInfo>
<pav:hasCurrentVersion rdf:resource="http://vocab.nerc.ac.uk/collection/P35/current/EPC00146/5/"/>
<pav:version>5</pav:version>
<pav:authoredOn>2016-12-12 15:20:45.0</pav:authoredOn>
<skos:note xml:lang="en">accepted</skos:note>
<owl:deprecated>false</owl:deprecated>
<skos:narrower rdf:resource="http://vocab.nerc.ac.uk/collection/P01/current/SCES0032/"/>
<skos:related rdf:resource="http://vocab.nerc.ac.uk/collection/P06/current/UGPL/"/>
<skos:broader rdf:resource="http://vocab.nerc.ac.uk/collection/P36/current/PCBSXX/"/>
<void:inDataset rdf:resource="http://vocab.nerc.ac.uk/.well-known/void"/>
</skos:Concept>
</skos:member>
<skos:member>
<skos:Concept rdf:about="http://vocab.nerc.ac.uk/collection/P35/current/EPC00163/">
<dc:identifier>SDN:P35::EPC00163</dc:identifier>
<dce:identifier>SDN:P35::EPC00163</dce:identifier>
<dc:date>2016-12-12 15:20:45.0</dc:date>
<skos:notation>SDN:P35::EPC00163</skos:notation>
<skos:prefLabel xml:lang="en">Water body PCB153</skos:prefLabel>
<skos:altLabel>Water body PCB153</skos:altLabel>
<skos:definition xml:lang="en">Concentration of PCB153 (dissolved, reactive particulate or suspended particulate material) in river, estuary, sea or ocean.</skos:definition>
<owl:versionInfo>5</owl:versionInfo>
<pav:hasCurrentVersion rdf:resource="http://vocab.nerc.ac.uk/collection/P35/current/EPC00163/5/"/>
<pav:version>5</pav:version>
<pav:authoredOn>2016-12-12 15:20:45.0</pav:authoredOn>
<skos:note xml:lang="en">accepted</skos:note>
<owl:deprecated>false</owl:deprecated>
<skos:narrower rdf:resource="http://vocab.nerc.ac.uk/collection/P01/current/SCES0036/"/>
<skos:related rdf:resource="http://vocab.nerc.ac.uk/collection/P06/current/UGPL/"/>
<skos:broader rdf:resource="http://vocab.nerc.ac.uk/collection/P36/current/PCBSXX/"/>
<void:inDataset rdf:resource="http://vocab.nerc.ac.uk/.well-known/void"/>
</skos:Concept>
</skos:member>
<skos:member>
<skos:Concept rdf:about="http://vocab.nerc.ac.uk/collection/P35/current/EPC00147/">
<dc:identifier>SDN:P35::EPC00147</dc:identifier>
<dce:identifier>SDN:P35::EPC00147</dce:identifier>
<dc:date>2016-12-12 15:20:45.0</dc:date>
<skos:notation>SDN:P35::EPC00147</skos:notation>
<skos:prefLabel xml:lang="en">Water body PCB180</skos:prefLabel>
<skos:altLabel>Water body PCB180</skos:altLabel>
<skos:definition xml:lang="en">Concentration of PCB180 (dissolved, reactive particulate or suspended particulate material) in river, estuary, sea or ocean by any method in filtered or unfiltered water.</skos:definition>
<owl:versionInfo>5</owl:versionInfo>
<pav:hasCurrentVersion rdf:resource="http://vocab.nerc.ac.uk/collection/P35/current/EPC00147/5/"/>
<pav:version>5</pav:version>
<pav:authoredOn>2016-12-12 15:20:45.0</pav:authoredOn>
<skos:note xml:lang="en">accepted</skos:note>
<owl:deprecated>false</owl:deprecated>
<skos:narrower rdf:resource="http://vocab.nerc.ac.uk/collection/P01/current/SCES0045/"/>
<skos:related rdf:resource="http://vocab.nerc.ac.uk/collection/P06/current/UGPL/"/>
<skos:broader rdf:resource="http://vocab.nerc.ac.uk/collection/P36/current/PCBSXX/"/>
<void:inDataset rdf:resource="http://vocab.nerc.ac.uk/.well-known/void"/>
</skos:Concept>
</skos:member>
<skos:member>
<skos:Concept rdf:about="http://vocab.nerc.ac.uk/collection/P35/current/EPC00221/">
<dc:identifier>SDN:P35::EPC00221</dc:identifier>
<dce:identifier>SDN:P35::EPC00221</dce:identifier>
<dc:date>2016-12-12 15:20:45.0</dc:date>
<skos:notation>SDN:P35::EPC00221</skos:notation>
<skos:prefLabel xml:lang="en">Water body PCB28</skos:prefLabel>
<skos:altLabel>Water body PCB28</skos:altLabel>
<skos:definition xml:lang="en">Concentration of PCB28 (dissolved, reactive particulate or suspended particulate material) in a river, estaury, sea or ocean.</skos:definition>
<owl:versionInfo>5</owl:versionInfo>
<pav:hasCurrentVersion rdf:resource="http://vocab.nerc.ac.uk/collection/P35/current/EPC00221/5/"/>
<pav:version>5</pav:version>
<pav:authoredOn>2016-12-12 15:20:45.0</pav:authoredOn>
<skos:note xml:lang="en">accepted</skos:note>
<owl:deprecated>false</owl:deprecated>
<skos:narrower rdf:resource="http://vocab.nerc.ac.uk/collection/P01/current/SCES0006/"/>
<skos:related rdf:resource="http://vocab.nerc.ac.uk/collection/P06/current/UGPL/"/>
<skos:broader rdf:resource="http://vocab.nerc.ac.uk/collection/P36/current/PCBSXX/"/>
<void:inDataset rdf:resource="http://vocab.nerc.ac.uk/.well-known/void"/>
</skos:Concept>
</skos:member>
<skos:member>
<skos:Concept rdf:about="http://vocab.nerc.ac.uk/collection/P35/current/EPC00194/">
<dc:identifier>SDN:P35::EPC00194</dc:identifier>
<dce:identifier>SDN:P35::EPC00194</dce:identifier>
<dc:date>2016-12-12 15:20:45.0</dc:date>
<skos:notation>SDN:P35::EPC00194</skos:notation>
<skos:prefLabel xml:lang="en">Water body PCB52</skos:prefLabel>
<skos:altLabel>Water body PCB52</skos:altLabel>
<skos:definition xml:lang="en">Concentration of PCB52 (dissolved, reactive particulate or suspended particulate material) in river, estuary, sea or ocean.</skos:definition>
<owl:versionInfo>5</owl:versionInfo>
<pav:hasCurrentVersion rdf:resource="http://vocab.nerc.ac.uk/collection/P35/current/EPC00194/5/"/>
<pav:version>5</pav:version>
<pav:authoredOn>2016-12-12 15:20:45.0</pav:authoredOn>
<skos:note xml:lang="en">accepted</skos:note>
<owl:deprecated>false</owl:deprecated>
<skos:narrower rdf:resource="http://vocab.nerc.ac.uk/collection/P01/current/SCES0011/"/>
<skos:related rdf:resource="http://vocab.nerc.ac.uk/collection/P06/current/UGPL/"/>
<skos:broader rdf:resource="http://vocab.nerc.ac.uk/collection/P36/current/PCBSXX/"/>
<void:inDataset rdf:resource="http://vocab.nerc.ac.uk/.well-known/void"/>
</skos:Concept>
</skos:member>
<skos:member>
<skos:Concept rdf:about="http://vocab.nerc.ac.uk/collection/P35/current/EPC00009/">
<dc:identifier>SDN:P35::EPC00009</dc:identifier>
<dce:identifier>SDN:P35::EPC00009</dce:identifier>
<dc:date>2016-10-20 11:27:18.0</dc:date>
<skos:notation>SDN:P35::EPC00009</skos:notation>
<skos:prefLabel xml:lang="en">Water body ammonium</skos:prefLabel>
<skos:altLabel>NH4</skos:altLabel>
<skos:definition xml:lang="en">Concentration of ammonium per unit volume of a river, estuary, sea or ocean by any method in filtered or unfiltered water.</skos:definition>
<owl:versionInfo>3</owl:versionInfo>
<pav:hasCurrentVersion rdf:resource="http://vocab.nerc.ac.uk/collection/P35/current/EPC00009/3/"/>
<pav:version>3</pav:version>
<pav:authoredOn>2016-10-20 11:27:18.0</pav:authoredOn>
<skos:note xml:lang="en">accepted</skos:note>
<owl:deprecated>false</owl:deprecated>
<skos:narrower rdf:resource="http://vocab.nerc.ac.uk/collection/P01/current/AMONAAD4/"/>
<skos:narrower rdf:resource="http://vocab.nerc.ac.uk/collection/P01/current/AMONZZXX/"/>
<skos:narrower rdf:resource="http://vocab.nerc.ac.uk/collection/P01/current/AMONMAD3/"/>
<skos:narrower rdf:resource="http://vocab.nerc.ac.uk/collection/P01/current/AMONKGD1/"/>
<skos:narrower rdf:resource="http://vocab.nerc.ac.uk/collection/P01/current/AMONHOTX/"/>
<skos:narrower rdf:resource="http://vocab.nerc.ac.uk/collection/P01/current/MDMAP004/"/>
<skos:narrower rdf:resource="http://vocab.nerc.ac.uk/collection/P01/current/AMONMPD1/"/>
<skos:narrower rdf:resource="http://vocab.nerc.ac.uk/collection/P01/current/AMONFSG1/"/>
<skos:narrower rdf:resource="http://vocab.nerc.ac.uk/collection/P01/current/AMONAADZ/"/>
<skos:narrower rdf:resource="http://vocab.nerc.ac.uk/collection/P01/current/AMONMP12/"/>
<skos:narrower rdf:resource="http://vocab.nerc.ac.uk/collection/P01/current/AMONAAD5/"/>
<skos:narrower rdf:resource="http://vocab.nerc.ac.uk/collection/P01/current/AMONAAZX/"/>
<skos:narrower rdf:resource="http://vocab.nerc.ac.uk/collection/P01/current/AMONAAD2/"/>
<skos:narrower rdf:resource="http://vocab.nerc.ac.uk/collection/P01/current/AMONAATX/"/>
<skos:narrower rdf:resource="http://vocab.nerc.ac.uk/collection/P01/current/AMONMATX/"/>
<skos:narrower rdf:resource="http://vocab.nerc.ac.uk/collection/P01/current/AMONAAD3/"/>
<skos:narrower rdf:resource="http://vocab.nerc.ac.uk/collection/P01/current/AMONNATX/"/>
<skos:narrower rdf:resource="http://vocab.nerc.ac.uk/collection/P01/current/AMONFID2/"/>
<skos:narrower rdf:resource="http://vocab.nerc.ac.uk/collection/P01/current/AMONAAD1/"/>
<skos:related rdf:resource="http://vocab.nerc.ac.uk/collection/P06/current/UPOX/"/>
<skos:broader rdf:resource="http://vocab.nerc.ac.uk/collection/P36/current/FERTIL/"/>
<void:inDataset rdf:resource="http://vocab.nerc.ac.uk/.well-known/void"/>
</skos:Concept>
</skos:member>
<skos:member>
<skos:Concept rdf:about="http://vocab.nerc.ac.uk/collection/P35/current/EPC00154/">
<dc:identifier>SDN:P35::EPC00154</dc:identifier>
<dce:identifier>SDN:P35::EPC00154</dce:identifier>
<dc:date>2016-12-12 15:20:45.0</dc:date>
<skos:notation>SDN:P35::EPC00154</skos:notation>
<skos:prefLabel xml:lang="en">Water body anthracene</skos:prefLabel>
<skos:altLabel>Water body anthracene</skos:altLabel>
<skos:definition xml:lang="en">Concentration of anthracene (dissolved, reactive particulate or suspended particulate material) in river, estuary, sea or ocean by any method in filtered or unfiltered water.</skos:definition>
<owl:versionInfo>5</owl:versionInfo>
<pav:hasCurrentVersion rdf:resource="http://vocab.nerc.ac.uk/collection/P35/current/EPC00154/5/"/>
<pav:version>5</pav:version>
<pav:authoredOn>2016-12-12 15:20:45.0</pav:authoredOn>
<skos:note xml:lang="en">accepted</skos:note>
<owl:deprecated>false</owl:deprecated>
<skos:narrower rdf:resource="http://vocab.nerc.ac.uk/collection/P01/current/ANUFWC02/"/>
<skos:narrower rdf:resource="http://vocab.nerc.ac.uk/collection/P01/current/ANAFWC01/"/>
<skos:narrower rdf:resource="http://vocab.nerc.ac.uk/collection/P01/current/CPAHWC05/"/>
<skos:narrower rdf:resource="http://vocab.nerc.ac.uk/collection/P01/current/WTCTM010/"/>
<skos:related rdf:resource="http://vocab.nerc.ac.uk/collection/P06/current/UGPL/"/>
<skos:broader rdf:resource="http://vocab.nerc.ac.uk/collection/P36/current/HCARBS/"/>
<void:inDataset rdf:resource="http://vocab.nerc.ac.uk/.well-known/void"/>
</skos:Concept>
</skos:member>
<skos:member>
<skos:Concept rdf:about="http://vocab.nerc.ac.uk/collection/P35/current/EPC00141/">
<dc:identifier>SDN:P35::EPC00141</dc:identifier>
<dce:identifier>SDN:P35::EPC00141</dce:identifier>
<dc:date>2016-12-12 15:20:45.0</dc:date>
<skos:notation>SDN:P35::EPC00141</skos:notation>
<skos:prefLabel xml:lang="en">Water body benzo(a)pyrene</skos:prefLabel>
<skos:altLabel>Water body benzo(a)pyrene</skos:altLabel>
<skos:definition xml:lang="en">Concentration of Benzo(a)pyrene (dissolved, reactive particulate or suspended particulate material) a river, estuary, sea or ocean by any method in filtered or unfiltered water.</skos:definition>
<owl:versionInfo>5</owl:versionInfo>
<pav:hasCurrentVersion rdf:resource="http://vocab.nerc.ac.uk/collection/P35/current/EPC00141/5/"/>
<pav:version>5</pav:version>
<pav:authoredOn>2016-12-12 15:20:45.0</pav:authoredOn>
<skos:note xml:lang="en">accepted</skos:note>
<owl:deprecated>false</owl:deprecated>
<skos:narrower rdf:resource="http://vocab.nerc.ac.uk/collection/P01/current/CPAHWC07/"/>
<skos:related rdf:resource="http://vocab.nerc.ac.uk/collection/P06/current/UGPL/"/>
<skos:broader rdf:resource="http://vocab.nerc.ac.uk/collection/P36/current/HCARBS/"/>
<void:inDataset rdf:resource="http://vocab.nerc.ac.uk/.well-known/void"/>
</skos:Concept>
</skos:member>
<skos:member>
<skos:Concept rdf:about="http://vocab.nerc.ac.uk/collection/P35/current/EPC00196/">
<dc:identifier>SDN:P35::EPC00196</dc:identifier>
<dce:identifier>SDN:P35::EPC00196</dce:identifier>
<dc:date>2016-12-12 15:20:45.0</dc:date>
<skos:notation>SDN:P35::EPC00196</skos:notation>
<skos:prefLabel xml:lang="en">Water body caesium-137</skos:prefLabel>
<skos:altLabel>Water body caesium-137</skos:altLabel>
<skos:definition xml:lang="en">Activity of caesium-137 (dissolved, reactive particulate or suspended particulate material) per unit volume of a river, estuary, sea or ocean by any method in filtered or unfiltered water.</skos:definition>
<owl:versionInfo>5</owl:versionInfo>
<pav:hasCurrentVersion rdf:resource="http://vocab.nerc.ac.uk/collection/P35/current/EPC00196/5/"/>
<pav:version>5</pav:version>
<pav:authoredOn>2016-12-12 15:20:45.0</pav:authoredOn>
<skos:note xml:lang="en">accepted</skos:note>
<owl:deprecated>false</owl:deprecated>
<skos:narrower rdf:resource="http://vocab.nerc.ac.uk/collection/P01/current/CS37GSTX/"/>
<skos:related rdf:resource="http://vocab.nerc.ac.uk/collection/P06/current/UBQL/"/>
<skos:broader rdf:resource="http://vocab.nerc.ac.uk/collection/P36/current/RADNUC/"/>
<void:inDataset rdf:resource="http://vocab.nerc.ac.uk/.well-known/void"/>
</skos:Concept>
</skos:member>
<skos:member>
<skos:Concept rdf:about="http://vocab.nerc.ac.uk/collection/P35/current/EPC00133/">
<dc:identifier>SDN:P35::EPC00133</dc:identifier>
<dce:identifier>SDN:P35::EPC00133</dce:identifier>
<dc:date>2016-10-20 11:27:18.0</dc:date>
<skos:notation>SDN:P35::EPC00133</skos:notation>
<skos:prefLabel xml:lang="en">Water body carbon dioxide partial pressure</skos:prefLabel>
<skos:altLabel>pCO2</skos:altLabel>
<skos:definition xml:lang="en">The partial pressure of carbon dioxide gas in an atmosphere that is in equilibrium with a sample from any body of fresh or salt water.</skos:definition>
<owl:versionInfo>3</owl:versionInfo>
<pav:hasCurrentVersion rdf:resource="http://vocab.nerc.ac.uk/collection/P35/current/EPC00133/3/"/>
<pav:version>3</pav:version>
<pav:authoredOn>2016-10-20 11:27:18.0</pav:authoredOn>
<skos:note xml:lang="en">accepted</skos:note>
<owl:deprecated>false</owl:deprecated>
<skos:narrower rdf:resource="http://vocab.nerc.ac.uk/collection/P01/current/PCO2XXXX/"/>
<skos:narrower rdf:resource="http://vocab.nerc.ac.uk/collection/P01/current/PCO2TK02/"/>
<skos:narrower rdf:resource="http://vocab.nerc.ac.uk/collection/P01/current/PCO2TU01/"/>
<skos:narrower rdf:resource="http://vocab.nerc.ac.uk/collection/P01/current/PCO2TK01/"/>
<skos:narrower rdf:resource="http://vocab.nerc.ac.uk/collection/P01/current/PCO2SS01/"/>
<skos:narrower rdf:resource="http://vocab.nerc.ac.uk/collection/P01/current/PCO2EG01/"/>
<skos:narrower rdf:resource="http://vocab.nerc.ac.uk/collection/P01/current/PCO2GC01/"/>
<skos:narrower rdf:resource="http://vocab.nerc.ac.uk/collection/P01/current/PCO2IERR/"/>
<skos:narrower rdf:resource="http://vocab.nerc.ac.uk/collection/P01/current/PCO2IG02/"/>
<skos:related rdf:resource="http://vocab.nerc.ac.uk/collection/P06/current/UATM/"/>
<skos:broader rdf:resource="http://vocab.nerc.ac.uk/collection/P36/current/DISGAS/"/>
<skos:broader rdf:resource="http://vocab.nerc.ac.uk/collection/P36/current/ACIDIT/"/>
<void:inDataset rdf:resource="http://vocab.nerc.ac.uk/.well-known/void"/>
</skos:Concept>
</skos:member>
<skos:member>
<skos:Concept rdf:about="http://vocab.nerc.ac.uk/collection/P35/current/EPC00105/">
<dc:identifier>SDN:P35::EPC00105</dc:identifier>
<dce:identifier>SDN:P35::EPC00105</dce:identifier>
<dc:date>2021-02-26 17:53:42.0</dc:date>
<skos:notation>SDN:P35::EPC00105</skos:notation>
<skos:prefLabel xml:lang="en">Water body chlorophyll-a</skos:prefLabel>
<skos:altLabel>Water body chlorophyll-a</skos:altLabel>
<skos:definition xml:lang="en">Concentration of the pigment chlorophyll-a contained in the particulate material of a specified volume of any body of salt or fresh water.</skos:definition>
<owl:versionInfo>6</owl:versionInfo>
<pav:hasCurrentVersion rdf:resource="http://vocab.nerc.ac.uk/collection/P35/current/EPC00105/6/"/>
<pav:version>6</pav:version>
<pav:authoredOn>2021-02-26 17:53:42.0</pav:authoredOn>
<skos:note xml:lang="en">accepted</skos:note>
<owl:deprecated>false</owl:deprecated>
<skos:narrower rdf:resource="http://vocab.nerc.ac.uk/collection/P01/current/CPHLSSP6/"/>
<skos:narrower rdf:resource="http://vocab.nerc.ac.uk/collection/P01/current/CPHLSSPC/"/>
<skos:narrower rdf:resource="http://vocab.nerc.ac.uk/collection/P01/current/CPHLSXP1/"/>
<skos:narrower rdf:resource="http://vocab.nerc.ac.uk/collection/P01/current/CPHLUA01/"/>
<skos:narrower rdf:resource="http://vocab.nerc.ac.uk/collection/P01/current/CPHLUB01/"/>
<skos:narrower rdf:resource="http://vocab.nerc.ac.uk/collection/P01/current/CPHLULAQ/"/>
<skos:narrower rdf:resource="http://vocab.nerc.ac.uk/collection/P01/current/CPHLULTF/"/>
<skos:narrower rdf:resource="http://vocab.nerc.ac.uk/collection/P01/current/CPHLUMAQ/"/>
<skos:narrower rdf:resource="http://vocab.nerc.ac.uk/collection/P01/current/CPHLUMTF/"/>
<skos:narrower rdf:resource="http://vocab.nerc.ac.uk/collection/P01/current/CPHLUT01/"/>
<skos:narrower rdf:resource="http://vocab.nerc.ac.uk/collection/P01/current/CPHLUW01/"/>
<skos:narrower rdf:resource="http://vocab.nerc.ac.uk/collection/P01/current/CPHLYMP1/"/>
<skos:narrower rdf:resource="http://vocab.nerc.ac.uk/collection/P01/current/CPHLZZXX/"/>
<skos:narrower rdf:resource="http://vocab.nerc.ac.uk/collection/P01/current/CHLADMFA/"/>
<skos:narrower rdf:resource="http://vocab.nerc.ac.uk/collection/P01/current/CHLAMSAT/"/>
<skos:narrower rdf:resource="http://vocab.nerc.ac.uk/collection/P01/current/CHLMEAL1/"/>
<skos:narrower rdf:resource="http://vocab.nerc.ac.uk/collection/P01/current/CHLMEOC5/"/>
<skos:narrower rdf:resource="http://vocab.nerc.ac.uk/collection/P01/current/CHLMOOC5/"/>
<skos:narrower rdf:resource="http://vocab.nerc.ac.uk/collection/P01/current/CPHLFEP1/"/>
<skos:narrower rdf:resource="http://vocab.nerc.ac.uk/collection/P01/current/CPHLFLP1/"/>
<skos:narrower rdf:resource="http://vocab.nerc.ac.uk/collection/P01/current/CPHLFLP2/"/>
<skos:narrower rdf:resource="http://vocab.nerc.ac.uk/collection/P01/current/CPHLFLP3/"/>
<skos:narrower rdf:resource="http://vocab.nerc.ac.uk/collection/P01/current/CPHLFLP4/"/>
<skos:narrower rdf:resource="http://vocab.nerc.ac.uk/collection/P01/current/CPHLFLP5/"/>
<skos:narrower rdf:resource="http://vocab.nerc.ac.uk/collection/P01/current/CPHLFLP6/"/>
<skos:narrower rdf:resource="http://vocab.nerc.ac.uk/collection/P01/current/CPHLFLPC/"/>
<skos:narrower rdf:resource="http://vocab.nerc.ac.uk/collection/P01/current/CPHLFLPZ/"/>
<skos:narrower rdf:resource="http://vocab.nerc.ac.uk/collection/P01/current/CPHLFMP1/"/>
<skos:narrower rdf:resource="http://vocab.nerc.ac.uk/collection/P01/current/CPHLHPP1/"/>
<skos:narrower rdf:resource="http://vocab.nerc.ac.uk/collection/P01/current/CPHLHPP2/"/>
<skos:narrower rdf:resource="http://vocab.nerc.ac.uk/collection/P01/current/CPHLHPP4/"/>
<skos:narrower rdf:resource="http://vocab.nerc.ac.uk/collection/P01/current/CPHLHPP5/"/>
<skos:narrower rdf:resource="http://vocab.nerc.ac.uk/collection/P01/current/CPHLHPPZ/"/>
<skos:narrower rdf:resource="http://vocab.nerc.ac.uk/collection/P01/current/CPHLMHP1/"/>
<skos:narrower rdf:resource="http://vocab.nerc.ac.uk/collection/P01/current/CPHLPL01/"/>
<skos:narrower rdf:resource="http://vocab.nerc.ac.uk/collection/P01/current/CPHLPM01/"/>
<skos:narrower rdf:resource="http://vocab.nerc.ac.uk/collection/P01/current/CPHLPM02/"/>
<skos:narrower rdf:resource="http://vocab.nerc.ac.uk/collection/P01/current/CPHLPR01/"/>
<skos:narrower rdf:resource="http://vocab.nerc.ac.uk/collection/P01/current/CPHLPS01/"/>
<skos:narrower rdf:resource="http://vocab.nerc.ac.uk/collection/P01/current/CPHLSEP1/"/>
<skos:narrower rdf:resource="http://vocab.nerc.ac.uk/collection/P01/current/CPHLSPP1/"/>
<skos:narrower rdf:resource="http://vocab.nerc.ac.uk/collection/P01/current/CPHLSPP3/"/>
<skos:narrower rdf:resource="http://vocab.nerc.ac.uk/collection/P01/current/CPHLSPPC/"/>
<skos:narrower rdf:resource="http://vocab.nerc.ac.uk/collection/P01/current/CPHLSPPZ/"/>
<skos:narrower rdf:resource="http://vocab.nerc.ac.uk/collection/P01/current/CPHLSSP1/"/>
<skos:narrower rdf:resource="http://vocab.nerc.ac.uk/collection/P01/current/CPHLSSP2/"/>
<skos:related rdf:resource="http://vocab.nerc.ac.uk/collection/P06/current/UMMC/"/>
<skos:broader rdf:resource="http://vocab.nerc.ac.uk/collection/P36/current/CHPHYL/"/>
<void:inDataset rdf:resource="http://vocab.nerc.ac.uk/.well-known/void"/>
</skos:Concept>
</skos:member>
<skos:member>
<skos:Concept rdf:about="http://vocab.nerc.ac.uk/collection/P35/current/EPC00106/">
<dc:identifier>SDN:P35::EPC00106</dc:identifier>
<dce:identifier>SDN:P35::EPC00106</dce:identifier>
<dc:date>2021-02-26 17:53:42.0</dc:date>
<skos:notation>SDN:P35::EPC00106</skos:notation>
<skos:prefLabel xml:lang="en">Water body chlorophyll-b</skos:prefLabel>
<skos:altLabel>Water body chlorophyll-b</skos:altLabel>
<skos:definition xml:lang="en">Concentration of the pigment chlorophyll-b contained in the particulate material of a specified volume of any body of salt or fresh water.</skos:definition>
<owl:versionInfo>6</owl:versionInfo>
<pav:hasCurrentVersion rdf:resource="http://vocab.nerc.ac.uk/collection/P35/current/EPC00106/6/"/>
<pav:version>6</pav:version>
<pav:authoredOn>2021-02-26 17:53:42.0</pav:authoredOn>
<skos:note xml:lang="en">accepted</skos:note>
<owl:deprecated>false</owl:deprecated>
<skos:narrower rdf:resource="http://vocab.nerc.ac.uk/collection/P01/current/CHLBHPP5/"/>
<skos:narrower rdf:resource="http://vocab.nerc.ac.uk/collection/P01/current/CHLBHPP1/"/>
<skos:narrower rdf:resource="http://vocab.nerc.ac.uk/collection/P01/current/CHLBMHP1/"/>
<skos:narrower rdf:resource="http://vocab.nerc.ac.uk/collection/P01/current/CHLBSSP1/"/>
<skos:narrower rdf:resource="http://vocab.nerc.ac.uk/collection/P01/current/CHLBXXPX/"/>
<skos:related rdf:resource="http://vocab.nerc.ac.uk/collection/P06/current/UMMC/"/>
<skos:broader rdf:resource="http://vocab.nerc.ac.uk/collection/P36/current/CHPHYL/"/>
<void:inDataset rdf:resource="http://vocab.nerc.ac.uk/.well-known/void"/>
</skos:Concept>
</skos:member>
<skos:member>
<skos:Concept rdf:about="http://vocab.nerc.ac.uk/collection/P35/current/EPC00107/">
<dc:identifier>SDN:P35::EPC00107</dc:identifier>
<dce:identifier>SDN:P35::EPC00107</dce:identifier>
<dc:date>2021-02-26 17:53:42.0</dc:date>
<skos:notation>SDN:P35::EPC00107</skos:notation>
<skos:prefLabel xml:lang="en">Water body chlorophyll-c</skos:prefLabel>
<skos:altLabel>Water body chlorophyll-c</skos:altLabel>
<skos:definition xml:lang="en">Concentration of the pigment chlorophyll-c contained in the particulate material of a specified volume of any body of salt or fresh water.</skos:definition>
<owl:versionInfo>6</owl:versionInfo>
<pav:hasCurrentVersion rdf:resource="http://vocab.nerc.ac.uk/collection/P35/current/EPC00107/6/"/>
<pav:version>6</pav:version>
<pav:authoredOn>2021-02-26 17:53:42.0</pav:authoredOn>
<skos:note xml:lang="en">accepted</skos:note>
<owl:deprecated>false</owl:deprecated>
<skos:narrower rdf:resource="http://vocab.nerc.ac.uk/collection/P01/current/CHLCHPP1/"/>
<skos:narrower rdf:resource="http://vocab.nerc.ac.uk/collection/P01/current/CHLCHPP5/"/>
<skos:narrower rdf:resource="http://vocab.nerc.ac.uk/collection/P01/current/CHLCSSP1/"/>
<skos:narrower rdf:resource="http://vocab.nerc.ac.uk/collection/P01/current/CHLCXXPX/"/>
<skos:related rdf:resource="http://vocab.nerc.ac.uk/collection/P06/current/UMMC/"/>
<skos:broader rdf:resource="http://vocab.nerc.ac.uk/collection/P36/current/CHPHYL/"/>
<void:inDataset rdf:resource="http://vocab.nerc.ac.uk/.well-known/void"/>
</skos:Concept>
</skos:member>
<skos:member>
<skos:Concept rdf:about="http://vocab.nerc.ac.uk/collection/P35/current/EPC00156/">
<dc:identifier>SDN:P35::EPC00156</dc:identifier>
<dce:identifier>SDN:P35::EPC00156</dce:identifier>
<dc:date>2016-12-12 15:20:45.0</dc:date>
<skos:notation>SDN:P35::EPC00156</skos:notation>
<skos:prefLabel xml:lang="en">Water body dissolved Mercury</skos:prefLabel>
<skos:altLabel>Water body dissolved Mercury</skos:altLabel>
<skos:definition xml:lang="en">Concentration of the metal per unit volume of a river, estuary, sea or ocean by any method in filtered water (any filter type). Total means the element in all possible states of valency and chemical combination.</skos:definition>
<owl:versionInfo>6</owl:versionInfo>
<pav:hasCurrentVersion rdf:resource="http://vocab.nerc.ac.uk/collection/P35/current/EPC00156/6/"/>
<pav:version>6</pav:version>
<pav:authoredOn>2016-12-12 15:20:45.0</pav:authoredOn>
<skos:note xml:lang="en">deprecated</skos:note>
<owl:deprecated>true</owl:deprecated>
<void:inDataset rdf:resource="http://vocab.nerc.ac.uk/.well-known/void"/>
</skos:Concept>
</skos:member>
<skos:member>
<skos:Concept rdf:about="http://vocab.nerc.ac.uk/collection/P35/current/EPC00011/">
<dc:identifier>SDN:P35::EPC00011</dc:identifier>
<dce:identifier>SDN:P35::EPC00011</dce:identifier>
<dc:date>2016-10-20 11:27:18.0</dc:date>
<skos:notation>SDN:P35::EPC00011</skos:notation>
<skos:prefLabel xml:lang="en">Water body dissolved aluminium</skos:prefLabel>
<skos:altLabel>Dissolved Al</skos:altLabel>
<skos:definition xml:lang="en">Concentration of the metal per unit volume of a river, estuary, sea or ocean by any method in filtered water (any filter type).</skos:definition>
<owl:versionInfo>3</owl:versionInfo>
<pav:hasCurrentVersion rdf:resource="http://vocab.nerc.ac.uk/collection/P35/current/EPC00011/3/"/>
<pav:version>3</pav:version>
<pav:authoredOn>2016-10-20 11:27:18.0</pav:authoredOn>
<skos:note xml:lang="en">accepted</skos:note>
<owl:deprecated>false</owl:deprecated>
<skos:narrower rdf:resource="http://vocab.nerc.ac.uk/collection/P01/current/ALXXLGD4/"/>
<skos:narrower rdf:resource="http://vocab.nerc.ac.uk/collection/P01/current/ALXXFIP5/"/>
<skos:narrower rdf:resource="http://vocab.nerc.ac.uk/collection/P01/current/ALXXLGD2/"/>
<skos:narrower rdf:resource="http://vocab.nerc.ac.uk/collection/P01/current/DALFICHL/"/>
<skos:narrower rdf:resource="http://vocab.nerc.ac.uk/collection/P01/current/ALXXLGD3/"/>
<skos:related rdf:resource="http://vocab.nerc.ac.uk/collection/P06/current/UPNM/"/>
<skos:broader rdf:resource="http://vocab.nerc.ac.uk/collection/P36/current/HVYMTL/"/>
<void:inDataset rdf:resource="http://vocab.nerc.ac.uk/.well-known/void"/>
</skos:Concept>
</skos:member>
<skos:member>
<skos:Concept rdf:about="http://vocab.nerc.ac.uk/collection/P35/current/EPC00012/">
<dc:identifier>SDN:P35::EPC00012</dc:identifier>
<dce:identifier>SDN:P35::EPC00012</dce:identifier>
<dc:date>2016-10-20 11:27:18.0</dc:date>
<skos:notation>SDN:P35::EPC00012</skos:notation>
<skos:prefLabel xml:lang="en">Water body dissolved antimony</skos:prefLabel>
<skos:altLabel>Dissolved Sb</skos:altLabel>
<skos:definition xml:lang="en">Concentration of the metal per unit volume of a river, estuary, sea or ocean by any method in filtered water (any filter type).</skos:definition>
<owl:versionInfo>3</owl:versionInfo>
<pav:hasCurrentVersion rdf:resource="http://vocab.nerc.ac.uk/collection/P35/current/EPC00012/3/"/>
<pav:version>3</pav:version>
<pav:authoredOn>2016-10-20 11:27:18.0</pav:authoredOn>
<skos:note xml:lang="en">accepted</skos:note>
<owl:deprecated>false</owl:deprecated>
<skos:narrower rdf:resource="http://vocab.nerc.ac.uk/collection/P01/current/RWS00143/"/>
<skos:related rdf:resource="http://vocab.nerc.ac.uk/collection/P06/current/UPNM/"/>
<skos:broader rdf:resource="http://vocab.nerc.ac.uk/collection/P36/current/HVYMTL/"/>
<void:inDataset rdf:resource="http://vocab.nerc.ac.uk/.well-known/void"/>
</skos:Concept>
</skos:member>
<skos:member>
<skos:Concept rdf:about="http://vocab.nerc.ac.uk/collection/P35/current/EPC00013/">
<dc:identifier>SDN:P35::EPC00013</dc:identifier>
<dce:identifier>SDN:P35::EPC00013</dce:identifier>
<dc:date>2016-10-20 11:27:18.0</dc:date>
<skos:notation>SDN:P35::EPC00013</skos:notation>
<skos:prefLabel xml:lang="en">Water body dissolved arsenic</skos:prefLabel>
<skos:altLabel>Dissolved As</skos:altLabel>
<skos:definition xml:lang="en">Concentration of the metal per unit volume of a river, estuary, sea or ocean by any method in filtered water (any filter type).</skos:definition>
<owl:versionInfo>3</owl:versionInfo>
<pav:hasCurrentVersion rdf:resource="http://vocab.nerc.ac.uk/collection/P35/current/EPC00013/3/"/>
<pav:version>3</pav:version>
<pav:authoredOn>2016-10-20 11:27:18.0</pav:authoredOn>
<skos:note xml:lang="en">accepted</skos:note>
<owl:deprecated>false</owl:deprecated>
<skos:narrower rdf:resource="http://vocab.nerc.ac.uk/collection/P01/current/AS35ASV1/"/>
<skos:narrower rdf:resource="http://vocab.nerc.ac.uk/collection/P01/current/RWS00141/"/>
<skos:narrower rdf:resource="http://vocab.nerc.ac.uk/collection/P01/current/ASXXAAD2/"/>
<skos:narrower rdf:resource="http://vocab.nerc.ac.uk/collection/P01/current/MDWD0010/"/>
<skos:related rdf:resource="http://vocab.nerc.ac.uk/collection/P06/current/UPNM/"/>
<skos:broader rdf:resource="http://vocab.nerc.ac.uk/collection/P36/current/HVYMTL/"/>
<void:inDataset rdf:resource="http://vocab.nerc.ac.uk/.well-known/void"/>
</skos:Concept>
</skos:member>
<skos:member>
<skos:Concept rdf:about="http://vocab.nerc.ac.uk/collection/P35/current/EPC00014/">
<dc:identifier>SDN:P35::EPC00014</dc:identifier>
<dce:identifier>SDN:P35::EPC00014</dce:identifier>
<dc:date>2016-10-20 11:27:18.0</dc:date>
<skos:notation>SDN:P35::EPC00014</skos:notation>
<skos:prefLabel xml:lang="en">Water body dissolved barium</skos:prefLabel>
<skos:altLabel>Dissolved Ba</skos:altLabel>
<skos:definition xml:lang="en">Concentration of the metal per unit volume of a river, estuary, sea or ocean by any method in filtered water (any filter type).</skos:definition>
<owl:versionInfo>3</owl:versionInfo>
<pav:hasCurrentVersion rdf:resource="http://vocab.nerc.ac.uk/collection/P35/current/EPC00014/3/"/>
<pav:version>3</pav:version>
<pav:authoredOn>2016-10-20 11:27:18.0</pav:authoredOn>
<skos:note xml:lang="en">accepted</skos:note>
<owl:deprecated>false</owl:deprecated>
<skos:narrower rdf:resource="http://vocab.nerc.ac.uk/collection/P01/current/RWS00147/"/>
<skos:narrower rdf:resource="http://vocab.nerc.ac.uk/collection/P01/current/BAICPMS1/"/>
<skos:related rdf:resource="http://vocab.nerc.ac.uk/collection/P06/current/UPNM/"/>
<skos:broader rdf:resource="http://vocab.nerc.ac.uk/collection/P36/current/HVYMTL/"/>
<void:inDataset rdf:resource="http://vocab.nerc.ac.uk/.well-known/void"/>
</skos:Concept>
</skos:member>
<skos:member>
<skos:Concept rdf:about="http://vocab.nerc.ac.uk/collection/P35/current/EPC00015/">
<dc:identifier>SDN:P35::EPC00015</dc:identifier>
<dce:identifier>SDN:P35::EPC00015</dce:identifier>
<dc:date>2016-10-20 11:27:18.0</dc:date>
<skos:notation>SDN:P35::EPC00015</skos:notation>
<skos:prefLabel xml:lang="en">Water body dissolved beryllium</skos:prefLabel>
<skos:altLabel>Dissolved Be</skos:altLabel>
<skos:definition xml:lang="en">Concentration of the metal per unit volume of a river, estuary, sea or ocean by any method in filtered water (any filter type).</skos:definition>
<owl:versionInfo>3</owl:versionInfo>
<pav:hasCurrentVersion rdf:resource="http://vocab.nerc.ac.uk/collection/P35/current/EPC00015/3/"/>
<pav:version>3</pav:version>
<pav:authoredOn>2016-10-20 11:27:18.0</pav:authoredOn>
<skos:note xml:lang="en">accepted</skos:note>
<owl:deprecated>false</owl:deprecated>
<skos:narrower rdf:resource="http://vocab.nerc.ac.uk/collection/P01/current/RWS00148/"/>
<skos:related rdf:resource="http://vocab.nerc.ac.uk/collection/P06/current/UPNM/"/>
<skos:broader rdf:resource="http://vocab.nerc.ac.uk/collection/P36/current/HVYMTL/"/>
<void:inDataset rdf:resource="http://vocab.nerc.ac.uk/.well-known/void"/>
</skos:Concept>
</skos:member>
<skos:member>
<skos:Concept rdf:about="http://vocab.nerc.ac.uk/collection/P35/current/EPC00016/">
<dc:identifier>SDN:P35::EPC00016</dc:identifier>
<dce:identifier>SDN:P35::EPC00016</dce:identifier>
<dc:date>2016-10-20 11:27:18.0</dc:date>
<skos:notation>SDN:P35::EPC00016</skos:notation>
<skos:prefLabel xml:lang="en">Water body dissolved boron</skos:prefLabel>
<skos:altLabel>Dissolved B</skos:altLabel>
<skos:definition xml:lang="en">Concentration of the metal per unit volume of a river, estuary, sea or ocean by any method in filtered water (any filter type).</skos:definition>
<owl:versionInfo>3</owl:versionInfo>
<pav:hasCurrentVersion rdf:resource="http://vocab.nerc.ac.uk/collection/P35/current/EPC00016/3/"/>
<pav:version>3</pav:version>
<pav:authoredOn>2016-10-20 11:27:18.0</pav:authoredOn>
<skos:note xml:lang="en">accepted</skos:note>
<owl:deprecated>false</owl:deprecated>
<skos:narrower rdf:resource="http://vocab.nerc.ac.uk/collection/P01/current/MDWD0054/"/>
<skos:narrower rdf:resource="http://vocab.nerc.ac.uk/collection/P01/current/RWS00144/"/>
<skos:related rdf:resource="http://vocab.nerc.ac.uk/collection/P06/current/UPNM/"/>
<skos:broader rdf:resource="http://vocab.nerc.ac.uk/collection/P36/current/HVYMTL/"/>
<void:inDataset rdf:resource="http://vocab.nerc.ac.uk/.well-known/void"/>
</skos:Concept>
</skos:member>
<skos:member>
<skos:Concept rdf:about="http://vocab.nerc.ac.uk/collection/P35/current/EPC00017/">
<dc:identifier>SDN:P35::EPC00017</dc:identifier>
<dce:identifier>SDN:P35::EPC00017</dce:identifier>
<dc:date>2016-10-20 11:27:18.0</dc:date>
<skos:notation>SDN:P35::EPC00017</skos:notation>
<skos:prefLabel xml:lang="en">Water body dissolved cadmium</skos:prefLabel>
<skos:altLabel>Dissolved Cd</skos:altLabel>
<skos:definition xml:lang="en">Concentration of the metal per unit volume of a river, estuary, sea or ocean by any method in filtered water (any filter type).</skos:definition>
<owl:versionInfo>3</owl:versionInfo>
<pav:hasCurrentVersion rdf:resource="http://vocab.nerc.ac.uk/collection/P35/current/EPC00017/3/"/>
<pav:version>3</pav:version>
<pav:authoredOn>2016-10-20 11:27:18.0</pav:authoredOn>
<skos:note xml:lang="en">accepted</skos:note>
<owl:deprecated>false</owl:deprecated>
<skos:narrower rdf:resource="http://vocab.nerc.ac.uk/collection/P01/current/CDXXAADZ/"/>
<skos:narrower rdf:resource="http://vocab.nerc.ac.uk/collection/P01/current/CDXXCVDX/"/>
<skos:narrower rdf:resource="http://vocab.nerc.ac.uk/collection/P01/current/ODSDM009/"/>
<skos:narrower rdf:resource="http://vocab.nerc.ac.uk/collection/P01/current/MTWD0009/"/>
<skos:narrower rdf:resource="http://vocab.nerc.ac.uk/collection/P01/current/CDAFWC01/"/>
<skos:narrower rdf:resource="http://vocab.nerc.ac.uk/collection/P01/current/CDXXFXD2/"/>
<skos:narrower rdf:resource="http://vocab.nerc.ac.uk/collection/P01/current/CDXXICD2/"/>
<skos:narrower rdf:resource="http://vocab.nerc.ac.uk/collection/P01/current/CDCDICP1/"/>
<skos:narrower rdf:resource="http://vocab.nerc.ac.uk/collection/P01/current/CDVOLDMS/"/>
<skos:related rdf:resource="http://vocab.nerc.ac.uk/collection/P06/current/UPNM/"/>
<skos:broader rdf:resource="http://vocab.nerc.ac.uk/collection/P36/current/HVYMTL/"/>
<void:inDataset rdf:resource="http://vocab.nerc.ac.uk/.well-known/void"/>
</skos:Concept>
</skos:member>
<skos:member>
<skos:Concept rdf:about="http://vocab.nerc.ac.uk/collection/P35/current/EPC00018/">
<dc:identifier>SDN:P35::EPC00018</dc:identifier>
<dce:identifier>SDN:P35::EPC00018</dce:identifier>
<dc:date>2016-10-20 11:27:18.0</dc:date>
<skos:notation>SDN:P35::EPC00018</skos:notation>
<skos:prefLabel xml:lang="en">Water body dissolved chromium</skos:prefLabel>
<skos:altLabel>Dissolved Cr</skos:altLabel>
<skos:definition xml:lang="en">Concentration of the metal per unit volume of a river, estuary, sea or ocean by any method in filtered water (any filter type).</skos:definition>
<owl:versionInfo>3</owl:versionInfo>
<pav:hasCurrentVersion rdf:resource="http://vocab.nerc.ac.uk/collection/P35/current/EPC00018/3/"/>
<pav:version>3</pav:version>
<pav:authoredOn>2016-10-20 11:27:18.0</pav:authoredOn>
<skos:note xml:lang="en">accepted</skos:note>
<owl:deprecated>false</owl:deprecated>
<skos:narrower rdf:resource="http://vocab.nerc.ac.uk/collection/P01/current/MTWD0055/"/>
<skos:narrower rdf:resource="http://vocab.nerc.ac.uk/collection/P01/current/CRAFWC01/"/>
<skos:related rdf:resource="http://vocab.nerc.ac.uk/collection/P06/current/UPNM/"/>
<skos:broader rdf:resource="http://vocab.nerc.ac.uk/collection/P36/current/HVYMTL/"/>
<void:inDataset rdf:resource="http://vocab.nerc.ac.uk/.well-known/void"/>
</skos:Concept>
</skos:member>
<skos:member>
<skos:Concept rdf:about="http://vocab.nerc.ac.uk/collection/P35/current/EPC00019/">
<dc:identifier>SDN:P35::EPC00019</dc:identifier>
<dce:identifier>SDN:P35::EPC00019</dce:identifier>
<dc:date>2016-10-20 11:27:18.0</dc:date>
<skos:notation>SDN:P35::EPC00019</skos:notation>
<skos:prefLabel xml:lang="en">Water body dissolved cobalt</skos:prefLabel>
<skos:altLabel>Dissolved Co</skos:altLabel>
<skos:definition xml:lang="en">Concentration of the metal per unit volume of a river, estuary, sea or ocean by any method in filtered water (any filter type).</skos:definition>
<owl:versionInfo>3</owl:versionInfo>
<pav:hasCurrentVersion rdf:resource="http://vocab.nerc.ac.uk/collection/P35/current/EPC00019/3/"/>
<pav:version>3</pav:version>
<pav:authoredOn>2016-10-20 11:27:18.0</pav:authoredOn>
<skos:note xml:lang="en">accepted</skos:note>
<owl:deprecated>false</owl:deprecated>
<skos:narrower rdf:resource="http://vocab.nerc.ac.uk/collection/P01/current/COXXFXD2/"/>
<skos:narrower rdf:resource="http://vocab.nerc.ac.uk/collection/P01/current/COLCSV04/"/>
<skos:narrower rdf:resource="http://vocab.nerc.ac.uk/collection/P01/current/CDCOICP1/"/>
<skos:narrower rdf:resource="http://vocab.nerc.ac.uk/collection/P01/current/COFICLD5/"/>
<skos:narrower rdf:resource="http://vocab.nerc.ac.uk/collection/P01/current/CDCOICP5/"/>
<skos:narrower rdf:resource="http://vocab.nerc.ac.uk/collection/P01/current/RWS00156/"/>
<skos:narrower rdf:resource="http://vocab.nerc.ac.uk/collection/P01/current/CO02CSVX/"/>
<skos:narrower rdf:resource="http://vocab.nerc.ac.uk/collection/P01/current/COL02CSV/"/>
<skos:narrower rdf:resource="http://vocab.nerc.ac.uk/collection/P01/current/COCSV04X/"/>
<skos:narrower rdf:resource="http://vocab.nerc.ac.uk/collection/P01/current/COFICLD2/"/>
<skos:related rdf:resource="http://vocab.nerc.ac.uk/collection/P06/current/UPNM/"/>
<skos:broader rdf:resource="http://vocab.nerc.ac.uk/collection/P36/current/HVYMTL/"/>
<void:inDataset rdf:resource="http://vocab.nerc.ac.uk/.well-known/void"/>
</skos:Concept>
</skos:member>
<skos:member>
<skos:Concept rdf:about="http://vocab.nerc.ac.uk/collection/P35/current/EPC00020/">
<dc:identifier>SDN:P35::EPC00020</dc:identifier>
<dce:identifier>SDN:P35::EPC00020</dce:identifier>
<dc:date>2016-10-20 11:27:18.0</dc:date>
<skos:notation>SDN:P35::EPC00020</skos:notation>
<skos:prefLabel xml:lang="en">Water body dissolved copper</skos:prefLabel>
<skos:altLabel>Dissolved Cu</skos:altLabel>
<skos:definition xml:lang="en">Concentration of the metal per unit volume of a river, estuary, sea or ocean by any method in filtered water (any filter type).</skos:definition>
<owl:versionInfo>3</owl:versionInfo>
<pav:hasCurrentVersion rdf:resource="http://vocab.nerc.ac.uk/collection/P35/current/EPC00020/3/"/>
<pav:version>3</pav:version>
<pav:authoredOn>2016-10-20 11:27:18.0</pav:authoredOn>
<skos:note xml:lang="en">accepted</skos:note>
<owl:deprecated>false</owl:deprecated>
<skos:narrower rdf:resource="http://vocab.nerc.ac.uk/collection/P01/current/CUXXASV1/"/>
<skos:narrower rdf:resource="http://vocab.nerc.ac.uk/collection/P01/current/MTWD0044/"/>
<skos:narrower rdf:resource="http://vocab.nerc.ac.uk/collection/P01/current/CUAFWC01/"/>
<skos:narrower rdf:resource="http://vocab.nerc.ac.uk/collection/P01/current/ODSDM008/"/>
<skos:narrower rdf:resource="http://vocab.nerc.ac.uk/collection/P01/current/CUVOLDMS/"/>
<skos:narrower rdf:resource="http://vocab.nerc.ac.uk/collection/P01/current/CUXXICD2/"/>
<skos:narrower rdf:resource="http://vocab.nerc.ac.uk/collection/P01/current/CDCUICP1/"/>
<skos:narrower rdf:resource="http://vocab.nerc.ac.uk/collection/P01/current/CUXXCVDX/"/>
<skos:narrower rdf:resource="http://vocab.nerc.ac.uk/collection/P01/current/CUXXAADZ/"/>
<skos:narrower rdf:resource="http://vocab.nerc.ac.uk/collection/P01/current/CUXXFXD2/"/>
<skos:related rdf:resource="http://vocab.nerc.ac.uk/collection/P06/current/UPNM/"/>
<skos:broader rdf:resource="http://vocab.nerc.ac.uk/collection/P36/current/HVYMTL/"/>
<void:inDataset rdf:resource="http://vocab.nerc.ac.uk/.well-known/void"/>
</skos:Concept>
</skos:member>
<skos:member>
<skos:Concept rdf:about="http://vocab.nerc.ac.uk/collection/P35/current/EPC00132/">
<dc:identifier>SDN:P35::EPC00132</dc:identifier>
<dce:identifier>SDN:P35::EPC00132</dce:identifier>
<dc:date>2016-10-20 11:27:18.0</dc:date>
<skos:notation>SDN:P35::EPC00132</skos:notation>
<skos:prefLabel xml:lang="en">Water body dissolved inorganic carbon</skos:prefLabel>
<skos:altLabel>TCO2</skos:altLabel>
<skos:definition xml:lang="en">Concentration of carbonate plus bicarbonate in a sample from any body of fresh or salt water.</skos:definition>
<owl:versionInfo>4</owl:versionInfo>
<pav:hasCurrentVersion rdf:resource="http://vocab.nerc.ac.uk/collection/P35/current/EPC00132/4/"/>
<pav:version>4</pav:version>
<pav:authoredOn>2016-10-20 11:27:18.0</pav:authoredOn>
<skos:note xml:lang="en">accepted</skos:note>
<owl:deprecated>false</owl:deprecated>
<skos:narrower rdf:resource="http://vocab.nerc.ac.uk/collection/P01/current/TCO2CBD5/"/>
<skos:narrower rdf:resource="http://vocab.nerc.ac.uk/collection/P01/current/TCO2CBTX/"/>
<skos:narrower rdf:resource="http://vocab.nerc.ac.uk/collection/P01/current/TCO2CBD2/"/>
<skos:narrower rdf:resource="http://vocab.nerc.ac.uk/collection/P01/current/TCO2CAD2/"/>
<skos:narrower rdf:resource="http://vocab.nerc.ac.uk/collection/P01/current/NZTW0009/"/>
<skos:narrower rdf:resource="http://vocab.nerc.ac.uk/collection/P01/current/TCO2MATX/"/>
<skos:narrower rdf:resource="http://vocab.nerc.ac.uk/collection/P01/current/TCO2MSXX/"/>
<skos:narrower rdf:resource="http://vocab.nerc.ac.uk/collection/P01/current/TCO2POTX/"/>
<skos:narrower rdf:resource="http://vocab.nerc.ac.uk/collection/P01/current/TCO2CPD5/"/>
<skos:narrower rdf:resource="http://vocab.nerc.ac.uk/collection/P01/current/TCO2KG01/"/>
<skos:narrower rdf:resource="http://vocab.nerc.ac.uk/collection/P01/current/TCO2ZZXX/"/>
<skos:related rdf:resource="http://vocab.nerc.ac.uk/collection/P06/current/UPOX/"/>
<skos:broader rdf:resource="http://vocab.nerc.ac.uk/collection/P36/current/ACIDIT/"/>
<void:inDataset rdf:resource="http://vocab.nerc.ac.uk/.well-known/void"/>
</skos:Concept>
</skos:member>
<skos:member>
<skos:Concept rdf:about="http://vocab.nerc.ac.uk/collection/P35/current/EPC00198/">
<dc:identifier>SDN:P35::EPC00198</dc:identifier>
<dce:identifier>SDN:P35::EPC00198</dce:identifier>
<dc:date>2016-12-12 15:20:45.0</dc:date>
<skos:notation>SDN:P35::EPC00198</skos:notation>
<skos:prefLabel xml:lang="en">Water body dissolved inorganic nitrogen (DIN)</skos:prefLabel>
<skos:altLabel>Water body dissolved inorganic nitrogen (DIN)</skos:altLabel>
<skos:definition xml:lang="en">Concentration of dissolved inorganic nitrogen per unit volume of a river, estuary, sea or ocean by any method in filtered or unfiltered water.</skos:definition>
<owl:versionInfo>5</owl:versionInfo>
<pav:hasCurrentVersion rdf:resource="http://vocab.nerc.ac.uk/collection/P35/current/EPC00198/5/"/>
<pav:version>5</pav:version>
<pav:authoredOn>2016-12-12 15:20:45.0</pav:authoredOn>
<skos:note xml:lang="en">accepted</skos:note>
<owl:deprecated>false</owl:deprecated>
<skos:narrower rdf:resource="http://vocab.nerc.ac.uk/collection/P01/current/DINXZZZZ/"/>
<skos:narrower rdf:resource="http://vocab.nerc.ac.uk/collection/P01/current/ODSDM017/"/>
<skos:related rdf:resource="http://vocab.nerc.ac.uk/collection/P06/current/UPOX/"/>
<skos:broader rdf:resource="http://vocab.nerc.ac.uk/collection/P36/current/FERTIL/"/>
<void:inDataset rdf:resource="http://vocab.nerc.ac.uk/.well-known/void"/>
</skos:Concept>
</skos:member>
<skos:member>
<skos:Concept rdf:about="http://vocab.nerc.ac.uk/collection/P35/current/EPC00021/">
<dc:identifier>SDN:P35::EPC00021</dc:identifier>
<dce:identifier>SDN:P35::EPC00021</dce:identifier>
<dc:date>2016-10-20 11:27:18.0</dc:date>
<skos:notation>SDN:P35::EPC00021</skos:notation>
<skos:prefLabel xml:lang="en">Water body dissolved iron (total chemical species)</skos:prefLabel>
<skos:altLabel>Dissolved total Fe</skos:altLabel>
<skos:definition xml:lang="en">Concentration of the metal per unit volume of a river, estuary, sea or ocean by any method in filtered water (any filter type). Total means the element in all possible states of valency and chemical combination.</skos:definition>
<owl:versionInfo>3</owl:versionInfo>
<pav:hasCurrentVersion rdf:resource="http://vocab.nerc.ac.uk/collection/P35/current/EPC00021/3/"/>
<pav:version>3</pav:version>
<pav:authoredOn>2016-10-20 11:27:18.0</pav:authoredOn>
<skos:note xml:lang="en">accepted</skos:note>
<owl:deprecated>false</owl:deprecated>
<skos:narrower rdf:resource="http://vocab.nerc.ac.uk/collection/P01/current/FEXXFXD2/"/>
<skos:narrower rdf:resource="http://vocab.nerc.ac.uk/collection/P01/current/DFEFICHL/"/>
<skos:narrower rdf:resource="http://vocab.nerc.ac.uk/collection/P01/current/MTWD0021/"/>
<skos:narrower rdf:resource="http://vocab.nerc.ac.uk/collection/P01/current/RWS00151/"/>
<skos:narrower rdf:resource="http://vocab.nerc.ac.uk/collection/P01/current/FEFICLDA/"/>
<skos:narrower rdf:resource="http://vocab.nerc.ac.uk/collection/P01/current/FEXXICD2/"/>
<skos:narrower rdf:resource="http://vocab.nerc.ac.uk/collection/P01/current/FETOTAAD/"/>
<skos:narrower rdf:resource="http://vocab.nerc.ac.uk/collection/P01/current/CDFEICP1/"/>
<skos:related rdf:resource="http://vocab.nerc.ac.uk/collection/P06/current/UPNM/"/>
<skos:broader rdf:resource="http://vocab.nerc.ac.uk/collection/P36/current/HVYMTL/"/>
<void:inDataset rdf:resource="http://vocab.nerc.ac.uk/.well-known/void"/>
</skos:Concept>
</skos:member>
<skos:member>
<skos:Concept rdf:about="http://vocab.nerc.ac.uk/collection/P35/current/EPC00022/">
<dc:identifier>SDN:P35::EPC00022</dc:identifier>
<dce:identifier>SDN:P35::EPC00022</dce:identifier>
<dc:date>2016-10-20 11:27:18.0</dc:date>
<skos:notation>SDN:P35::EPC00022</skos:notation>
<skos:prefLabel xml:lang="en">Water body dissolved lead</skos:prefLabel>
<skos:altLabel>Dissolved Pb</skos:altLabel>
<skos:definition xml:lang="en">Concentration of the metal per unit volume of a river, estuary, sea or ocean by any method in filtered water (any filter type).</skos:definition>
<owl:versionInfo>3</owl:versionInfo>
<pav:hasCurrentVersion rdf:resource="http://vocab.nerc.ac.uk/collection/P35/current/EPC00022/3/"/>
<pav:version>3</pav:version>
<pav:authoredOn>2016-10-20 11:27:18.0</pav:authoredOn>
<skos:note xml:lang="en">accepted</skos:note>
<owl:deprecated>false</owl:deprecated>
<skos:narrower rdf:resource="http://vocab.nerc.ac.uk/collection/P01/current/PBAFWC01/"/>
<skos:narrower rdf:resource="http://vocab.nerc.ac.uk/collection/P01/current/ODSDM011/"/>
<skos:narrower rdf:resource="http://vocab.nerc.ac.uk/collection/P01/current/CDPBICP1/"/>
<skos:narrower rdf:resource="http://vocab.nerc.ac.uk/collection/P01/current/PBVOLDMS/"/>
<skos:narrower rdf:resource="http://vocab.nerc.ac.uk/collection/P01/current/PBXXICD2/"/>
<skos:narrower rdf:resource="http://vocab.nerc.ac.uk/collection/P01/current/PBXXFXD2/"/>
<skos:narrower rdf:resource="http://vocab.nerc.ac.uk/collection/P01/current/PBXXAADZ/"/>
<skos:narrower rdf:resource="http://vocab.nerc.ac.uk/collection/P01/current/MTWD0046/"/>
<skos:related rdf:resource="http://vocab.nerc.ac.uk/collection/P06/current/UPNM/"/>
<skos:broader rdf:resource="http://vocab.nerc.ac.uk/collection/P36/current/HVYMTL/"/>
<void:inDataset rdf:resource="http://vocab.nerc.ac.uk/.well-known/void"/>
</skos:Concept>
</skos:member>
<skos:member>
<skos:Concept rdf:about="http://vocab.nerc.ac.uk/collection/P35/current/EPC00023/">
<dc:identifier>SDN:P35::EPC00023</dc:identifier>
<dce:identifier>SDN:P35::EPC00023</dce:identifier>
<dc:date>2016-10-20 11:27:18.0</dc:date>
<skos:notation>SDN:P35::EPC00023</skos:notation>
<skos:prefLabel xml:lang="en">Water body dissolved lithium</skos:prefLabel>
<skos:altLabel>Dissolved Li</skos:altLabel>
<skos:definition xml:lang="en">Concentration of the metal per unit volume of a river, estuary, sea or ocean by any method in filtered water (any filter type).</skos:definition>
<owl:versionInfo>3</owl:versionInfo>
<pav:hasCurrentVersion rdf:resource="http://vocab.nerc.ac.uk/collection/P35/current/EPC00023/3/"/>
<pav:version>3</pav:version>
<pav:authoredOn>2016-10-20 11:27:18.0</pav:authoredOn>
<skos:note xml:lang="en">accepted</skos:note>
<owl:deprecated>false</owl:deprecated>
<skos:narrower rdf:resource="http://vocab.nerc.ac.uk/collection/P01/current/RWS00149/"/>
<skos:related rdf:resource="http://vocab.nerc.ac.uk/collection/P06/current/UPNM/"/>
<skos:broader rdf:resource="http://vocab.nerc.ac.uk/collection/P36/current/HVYMTL/"/>
<void:inDataset rdf:resource="http://vocab.nerc.ac.uk/.well-known/void"/>
</skos:Concept>
</skos:member>
<skos:member>
<skos:Concept rdf:about="http://vocab.nerc.ac.uk/collection/P35/current/EPC00024/">
<dc:identifier>SDN:P35::EPC00024</dc:identifier>
<dce:identifier>SDN:P35::EPC00024</dce:identifier>
<dc:date>2016-10-20 11:27:18.0</dc:date>
<skos:notation>SDN:P35::EPC00024</skos:notation>
<skos:prefLabel xml:lang="en">Water body dissolved manganese (total chemical species)</skos:prefLabel>
<skos:altLabel>Dissolved total Mn</skos:altLabel>
<skos:definition xml:lang="en">Concentration of the metal per unit volume of a river, estuary, sea or ocean by any method in filtered water (any filter type). Total means the element in all possible states of valency and chemical combination.</skos:definition>
<owl:versionInfo>3</owl:versionInfo>
<pav:hasCurrentVersion rdf:resource="http://vocab.nerc.ac.uk/collection/P35/current/EPC00024/3/"/>
<pav:version>3</pav:version>
<pav:authoredOn>2016-10-20 11:27:18.0</pav:authoredOn>
<skos:note xml:lang="en">accepted</skos:note>
<owl:deprecated>false</owl:deprecated>
<skos:narrower rdf:resource="http://vocab.nerc.ac.uk/collection/P01/current/MNXXICD2/"/>
<skos:narrower rdf:resource="http://vocab.nerc.ac.uk/collection/P01/current/MNXXFXD2/"/>
<skos:narrower rdf:resource="http://vocab.nerc.ac.uk/collection/P01/current/MNFICD01/"/>
<skos:narrower rdf:resource="http://vocab.nerc.ac.uk/collection/P01/current/MNVOLDMS/"/>
<skos:narrower rdf:resource="http://vocab.nerc.ac.uk/collection/P01/current/MNXXAAD2/"/>
<skos:narrower rdf:resource="http://vocab.nerc.ac.uk/collection/P01/current/RWS00150/"/>
<skos:narrower rdf:resource="http://vocab.nerc.ac.uk/collection/P01/current/MNXXAADZ/"/>
<skos:related rdf:resource="http://vocab.nerc.ac.uk/collection/P06/current/UPNM/"/>
<skos:broader rdf:resource="http://vocab.nerc.ac.uk/collection/P36/current/HVYMTL/"/>
<void:inDataset rdf:resource="http://vocab.nerc.ac.uk/.well-known/void"/>
</skos:Concept>
</skos:member>
<skos:member>
<skos:Concept rdf:about="http://vocab.nerc.ac.uk/collection/P35/current/EPC00025/">
<dc:identifier>SDN:P35::EPC00025</dc:identifier>
<dce:identifier>SDN:P35::EPC00025</dce:identifier>
<dc:date>2016-10-20 11:27:18.0</dc:date>
<skos:notation>SDN:P35::EPC00025</skos:notation>
<skos:prefLabel xml:lang="en">Water body dissolved mercury</skos:prefLabel>
<skos:altLabel>Dissolved Hg</skos:altLabel>
<skos:definition xml:lang="en">Concentration of the metal per unit volume of a river, estuary, sea or ocean by any method in filtered water (any filter type). Total means the element in all possible states of valency and chemical combination.</skos:definition>
<owl:versionInfo>4</owl:versionInfo>
<pav:hasCurrentVersion rdf:resource="http://vocab.nerc.ac.uk/collection/P35/current/EPC00025/4/"/>
<pav:version>4</pav:version>
<pav:authoredOn>2016-10-20 11:27:18.0</pav:authoredOn>
<skos:note xml:lang="en">accepted</skos:note>
<owl:deprecated>false</owl:deprecated>
<skos:narrower rdf:resource="http://vocab.nerc.ac.uk/collection/P01/current/MTWD0008/"/>
<skos:narrower rdf:resource="http://vocab.nerc.ac.uk/collection/P01/current/HGAFWC01/"/>
<skos:narrower rdf:resource="http://vocab.nerc.ac.uk/collection/P01/current/HGRXAAD1/"/>
<skos:narrower rdf:resource="http://vocab.nerc.ac.uk/collection/P01/current/WTCTM017/"/>
<skos:narrower rdf:resource="http://vocab.nerc.ac.uk/collection/P01/current/HGTXAAD1/"/>
<skos:narrower rdf:resource="http://vocab.nerc.ac.uk/collection/P01/current/HGXXCFD2/"/>
<skos:related rdf:resource="http://vocab.nerc.ac.uk/collection/P06/current/UPNM/"/>
<skos:broader rdf:resource="http://vocab.nerc.ac.uk/collection/P36/current/HVYMTL/"/>
<void:inDataset rdf:resource="http://vocab.nerc.ac.uk/.well-known/void"/>
</skos:Concept>
</skos:member>
<skos:member>
<skos:Concept rdf:about="http://vocab.nerc.ac.uk/collection/P35/current/EPC00026/">
<dc:identifier>SDN:P35::EPC00026</dc:identifier>
<dce:identifier>SDN:P35::EPC00026</dce:identifier>
<dc:date>2016-10-20 11:27:18.0</dc:date>
<skos:notation>SDN:P35::EPC00026</skos:notation>
<skos:prefLabel xml:lang="en">Water body dissolved molybdenum</skos:prefLabel>
<skos:altLabel>Dissolved Mo</skos:altLabel>
<skos:definition xml:lang="en">Concentration of the metal per unit volume of a river, estuary, sea or ocean by any method in filtered water (any filter type).</skos:definition>
<owl:versionInfo>3</owl:versionInfo>
<pav:hasCurrentVersion rdf:resource="http://vocab.nerc.ac.uk/collection/P35/current/EPC00026/3/"/>
<pav:version>3</pav:version>
<pav:authoredOn>2016-10-20 11:27:18.0</pav:authoredOn>
<skos:note xml:lang="en">accepted</skos:note>
<owl:deprecated>false</owl:deprecated>
<skos:narrower rdf:resource="http://vocab.nerc.ac.uk/collection/P01/current/MTWD00MO/"/>
<skos:narrower rdf:resource="http://vocab.nerc.ac.uk/collection/P01/current/RWS00157/"/>
<skos:narrower rdf:resource="http://vocab.nerc.ac.uk/collection/P01/current/MBICPMS1/"/>
<skos:related rdf:resource="http://vocab.nerc.ac.uk/collection/P06/current/UPNM/"/>
<skos:broader rdf:resource="http://vocab.nerc.ac.uk/collection/P36/current/HVYMTL/"/>
<void:inDataset rdf:resource="http://vocab.nerc.ac.uk/.well-known/void"/>
</skos:Concept>
</skos:member>
<skos:member>
<skos:Concept rdf:about="http://vocab.nerc.ac.uk/collection/P35/current/EPC00027/">
<dc:identifier>SDN:P35::EPC00027</dc:identifier>
<dce:identifier>SDN:P35::EPC00027</dce:identifier>
<dc:date>2016-10-20 11:27:18.0</dc:date>
<skos:notation>SDN:P35::EPC00027</skos:notation>
<skos:prefLabel xml:lang="en">Water body dissolved nickel</skos:prefLabel>
<skos:altLabel>Dissolved Ni</skos:altLabel>
<skos:definition xml:lang="en">Concentration of the metal per unit volume of a river, estuary, sea or ocean by any method in filtered water (any filter type).</skos:definition>
<owl:versionInfo>3</owl:versionInfo>
<pav:hasCurrentVersion rdf:resource="http://vocab.nerc.ac.uk/collection/P35/current/EPC00027/3/"/>
<pav:version>3</pav:version>
<pav:authoredOn>2016-10-20 11:27:18.0</pav:authoredOn>
<skos:note xml:lang="en">accepted</skos:note>
<owl:deprecated>false</owl:deprecated>
<skos:narrower rdf:resource="http://vocab.nerc.ac.uk/collection/P01/current/MTWD0051/"/>
<skos:narrower rdf:resource="http://vocab.nerc.ac.uk/collection/P01/current/NIXXICD2/"/>
<skos:narrower rdf:resource="http://vocab.nerc.ac.uk/collection/P01/current/ODSDM012/"/>
<skos:narrower rdf:resource="http://vocab.nerc.ac.uk/collection/P01/current/CDNIICP5/"/>
<skos:narrower rdf:resource="http://vocab.nerc.ac.uk/collection/P01/current/NIXXFXD2/"/>
<skos:narrower rdf:resource="http://vocab.nerc.ac.uk/collection/P01/current/CDNIICP1/"/>
<skos:narrower rdf:resource="http://vocab.nerc.ac.uk/collection/P01/current/NIXXZZZZ/"/>
<skos:related rdf:resource="http://vocab.nerc.ac.uk/collection/P06/current/UPNM/"/>
<skos:broader rdf:resource="http://vocab.nerc.ac.uk/collection/P36/current/HVYMTL/"/>
<void:inDataset rdf:resource="http://vocab.nerc.ac.uk/.well-known/void"/>
</skos:Concept>
</skos:member>
<skos:member>
<skos:Concept rdf:about="http://vocab.nerc.ac.uk/collection/P35/current/EPC00160/">
<dc:identifier>SDN:P35::EPC00160</dc:identifier>
<dce:identifier>SDN:P35::EPC00160</dce:identifier>
<dc:date>2016-12-12 15:20:45.0</dc:date>
<skos:notation>SDN:P35::EPC00160</skos:notation>
<skos:prefLabel xml:lang="en">Water body dissolved nitrogen</skos:prefLabel>
<skos:altLabel>Water body dissolved nitrogen</skos:altLabel>
<skos:definition xml:lang="en">Concentration of total dissolved nitrogen per unit volume of a river, estuary, sea or ocean by any method in filtered or unfiltered water.</skos:definition>
<owl:versionInfo>5</owl:versionInfo>
<pav:hasCurrentVersion rdf:resource="http://vocab.nerc.ac.uk/collection/P35/current/EPC00160/5/"/>
<pav:version>5</pav:version>
<pav:authoredOn>2016-12-12 15:20:45.0</pav:authoredOn>
<skos:note xml:lang="en">accepted</skos:note>
<owl:deprecated>false</owl:deprecated>
<skos:narrower rdf:resource="http://vocab.nerc.ac.uk/collection/P01/current/NTOTWCDZ/"/>
<skos:narrower rdf:resource="http://vocab.nerc.ac.uk/collection/P01/current/NTOTZZD2/"/>
<skos:narrower rdf:resource="http://vocab.nerc.ac.uk/collection/P01/current/NTOTWCD1/"/>
<skos:related rdf:resource="http://vocab.nerc.ac.uk/collection/P06/current/UPOX/"/>
<skos:broader rdf:resource="http://vocab.nerc.ac.uk/collection/P36/current/FERTIL/"/>
<void:inDataset rdf:resource="http://vocab.nerc.ac.uk/.well-known/void"/>
</skos:Concept>
</skos:member>
<skos:member>
<skos:Concept rdf:about="http://vocab.nerc.ac.uk/collection/P35/current/EPC00190/">
<dc:identifier>SDN:P35::EPC00190</dc:identifier>
<dce:identifier>SDN:P35::EPC00190</dce:identifier>
<dc:date>2016-12-12 15:20:45.0</dc:date>
<skos:notation>SDN:P35::EPC00190</skos:notation>
<skos:prefLabel xml:lang="en">Water body dissolved organic carbon {DOC}</skos:prefLabel>
<skos:altLabel>Water body dissolved organic carbon {DOC}</skos:altLabel>
<skos:definition xml:lang="en">Concentration of dissolved organic carbon per unit volume of a river, estuary, sea or ocean by any method in filtered or unfiltered water.</skos:definition>
<owl:versionInfo>5</owl:versionInfo>
<pav:hasCurrentVersion rdf:resource="http://vocab.nerc.ac.uk/collection/P35/current/EPC00190/5/"/>
<pav:version>5</pav:version>
<pav:authoredOn>2016-12-12 15:20:45.0</pav:authoredOn>
<skos:note xml:lang="en">accepted</skos:note>
<owl:deprecated>false</owl:deprecated>
<skos:narrower rdf:resource="http://vocab.nerc.ac.uk/collection/P01/current/CORGZZTL/"/>
<skos:narrower rdf:resource="http://vocab.nerc.ac.uk/collection/P01/current/CORGWCDZ/"/>
<skos:narrower rdf:resource="http://vocab.nerc.ac.uk/collection/P01/current/CORGZZZX/"/>
<skos:related rdf:resource="http://vocab.nerc.ac.uk/collection/P06/current/UPOX/"/>
<skos:broader rdf:resource="http://vocab.nerc.ac.uk/collection/P36/current/ORGMAT/"/>
<void:inDataset rdf:resource="http://vocab.nerc.ac.uk/.well-known/void"/>
</skos:Concept>
</skos:member>
<skos:member>
<skos:Concept rdf:about="http://vocab.nerc.ac.uk/collection/P35/current/EPC00002/">
<dc:identifier>SDN:P35::EPC00002</dc:identifier>
<dce:identifier>SDN:P35::EPC00002</dce:identifier>
<dc:date>2016-10-20 11:27:18.0</dc:date>
<skos:notation>SDN:P35::EPC00002</skos:notation>
<skos:prefLabel xml:lang="en">Water body dissolved oxygen concentration</skos:prefLabel>
<skos:altLabel>Oxygen</skos:altLabel>
<skos:definition xml:lang="en">Dissolved oxygen per unit volume of a river, estuary, sea or ocean by any method.</skos:definition>
<owl:versionInfo>3</owl:versionInfo>
<pav:hasCurrentVersion rdf:resource="http://vocab.nerc.ac.uk/collection/P35/current/EPC00002/3/"/>
<pav:version>3</pav:version>
<pav:authoredOn>2016-10-20 11:27:18.0</pav:authoredOn>
<skos:note xml:lang="en">accepted</skos:note>
<owl:deprecated>false</owl:deprecated>
<skos:narrower rdf:resource="http://vocab.nerc.ac.uk/collection/P01/current/DOXYCZ01/"/>
<skos:narrower rdf:resource="http://vocab.nerc.ac.uk/collection/P01/current/DOXYOP01/"/>
<skos:narrower rdf:resource="http://vocab.nerc.ac.uk/collection/P01/current/DOXYPE01/"/>
<skos:narrower rdf:resource="http://vocab.nerc.ac.uk/collection/P01/current/DOXYPR02/"/>
<skos:narrower rdf:resource="http://vocab.nerc.ac.uk/collection/P01/current/DOXYSC01/"/>
<skos:narrower rdf:resource="http://vocab.nerc.ac.uk/collection/P01/current/DOXYSU01/"/>
<skos:narrower rdf:resource="http://vocab.nerc.ac.uk/collection/P01/current/DOXYSU02/"/>
<skos:narrower rdf:resource="http://vocab.nerc.ac.uk/collection/P01/current/DOXYUZ01/"/>
<skos:narrower rdf:resource="http://vocab.nerc.ac.uk/collection/P01/current/DOXYWITX/"/>
<skos:narrower rdf:resource="http://vocab.nerc.ac.uk/collection/P01/current/DOXYZZ01/"/>
<skos:narrower rdf:resource="http://vocab.nerc.ac.uk/collection/P01/current/DOXYZZXX/"/>
<skos:narrower rdf:resource="http://vocab.nerc.ac.uk/collection/P01/current/DOXMZZXX/"/>
<skos:narrower rdf:resource="http://vocab.nerc.ac.uk/collection/P01/current/DOKGWITX/"/>
<skos:narrower rdf:resource="http://vocab.nerc.ac.uk/collection/P01/current/DOXYSE01/"/>
<skos:narrower rdf:resource="http://vocab.nerc.ac.uk/collection/P01/current/DOXYAAOP/"/>
<skos:narrower rdf:resource="http://vocab.nerc.ac.uk/collection/P01/current/DOXYPR01/"/>
<skos:narrower rdf:resource="http://vocab.nerc.ac.uk/collection/P01/current/DOXYSE02/"/>
<skos:narrower rdf:resource="http://vocab.nerc.ac.uk/collection/P01/current/DOXYUZ02/"/>
<skos:related rdf:resource="http://vocab.nerc.ac.uk/collection/P06/current/UPOX/"/>
<skos:broader rdf:resource="http://vocab.nerc.ac.uk/collection/P36/current/DISGAS/"/>
<void:inDataset rdf:resource="http://vocab.nerc.ac.uk/.well-known/void"/>
</skos:Concept>
</skos:member>
<skos:member>
<skos:Concept rdf:about="http://vocab.nerc.ac.uk/collection/P35/current/EPC00003/">
<dc:identifier>SDN:P35::EPC00003</dc:identifier>
<dce:identifier>SDN:P35::EPC00003</dce:identifier>
<dc:date>2016-10-20 11:27:18.0</dc:date>
<skos:notation>SDN:P35::EPC00003</skos:notation>
<skos:prefLabel xml:lang="en">Water body dissolved oxygen saturation</skos:prefLabel>
<skos:altLabel>Oxygen Saturation</skos:altLabel>
<skos:definition xml:lang="en">The measured oxygen concentration expressed as a percentage of its theoretical value in a river, estaury, sea or ocean.</skos:definition>
<owl:versionInfo>3</owl:versionInfo>
<pav:hasCurrentVersion rdf:resource="http://vocab.nerc.ac.uk/collection/P35/current/EPC00003/3/"/>
<pav:version>3</pav:version>
<pav:authoredOn>2016-10-20 11:27:18.0</pav:authoredOn>
<skos:note xml:lang="en">accepted</skos:note>
<owl:deprecated>false</owl:deprecated>
<skos:narrower rdf:resource="http://vocab.nerc.ac.uk/collection/P01/current/OXYSBB02/"/>
<skos:narrower rdf:resource="http://vocab.nerc.ac.uk/collection/P01/current/OXYSBE01/"/>
<skos:narrower rdf:resource="http://vocab.nerc.ac.uk/collection/P01/current/OXYSOP01/"/>
<skos:narrower rdf:resource="http://vocab.nerc.ac.uk/collection/P01/current/OXYSSC01/"/>
<skos:narrower rdf:resource="http://vocab.nerc.ac.uk/collection/P01/current/OXYSSE01/"/>
<skos:narrower rdf:resource="http://vocab.nerc.ac.uk/collection/P01/current/OXYSWB01/"/>
<skos:narrower rdf:resource="http://vocab.nerc.ac.uk/collection/P01/current/OXYSWW01/"/>
<skos:narrower rdf:resource="http://vocab.nerc.ac.uk/collection/P01/current/OXYSZZ01/"/>
<skos:narrower rdf:resource="http://vocab.nerc.ac.uk/collection/P01/current/OXYSZZ02/"/>
<skos:narrower rdf:resource="http://vocab.nerc.ac.uk/collection/P01/current/OXYSZW01/"/>
<skos:narrower rdf:resource="http://vocab.nerc.ac.uk/collection/P01/current/OXYSWE01/"/>
<skos:narrower rdf:resource="http://vocab.nerc.ac.uk/collection/P01/current/OXYSBB01/"/>
<skos:narrower rdf:resource="http://vocab.nerc.ac.uk/collection/P01/current/OXYSBW01/"/>
<skos:narrower rdf:resource="http://vocab.nerc.ac.uk/collection/P01/current/OXYSSU01/"/>
<skos:related rdf:resource="http://vocab.nerc.ac.uk/collection/P06/current/UPCT/"/>
<skos:broader rdf:resource="http://vocab.nerc.ac.uk/collection/P36/current/DISGAS/"/>
<void:inDataset rdf:resource="http://vocab.nerc.ac.uk/.well-known/void"/>
</skos:Concept>
</skos:member>
<skos:member>
<skos:Concept rdf:about="http://vocab.nerc.ac.uk/collection/P35/current/EPC00186/">
<dc:identifier>SDN:P35::EPC00186</dc:identifier>
<dce:identifier>SDN:P35::EPC00186</dce:identifier>
<dc:date>2016-12-12 15:20:45.0</dc:date>
<skos:notation>SDN:P35::EPC00186</skos:notation>
<skos:prefLabel xml:lang="en">Water body dissolved phosphorus</skos:prefLabel>
<skos:altLabel>Water body dissolved phosphorus</skos:altLabel>
<skos:definition xml:lang="en">Concentration of total dissolved phosphorus per unit volume of a river, estuary, sea or ocean by any method in filtered or unfiltered water.</skos:definition>
<owl:versionInfo>5</owl:versionInfo>
<pav:hasCurrentVersion rdf:resource="http://vocab.nerc.ac.uk/collection/P35/current/EPC00186/5/"/>
<pav:version>5</pav:version>
<pav:authoredOn>2016-12-12 15:20:45.0</pav:authoredOn>
<skos:note xml:lang="en">accepted</skos:note>
<owl:deprecated>false</owl:deprecated>
<skos:narrower rdf:resource="http://vocab.nerc.ac.uk/collection/P01/current/TPHSWCD1/"/>
<skos:narrower rdf:resource="http://vocab.nerc.ac.uk/collection/P01/current/TPHSDSZZ/"/>
<skos:narrower rdf:resource="http://vocab.nerc.ac.uk/collection/P01/current/TPHSWCDZ/"/>
<skos:related rdf:resource="http://vocab.nerc.ac.uk/collection/P06/current/UPOX/"/>
<skos:broader rdf:resource="http://vocab.nerc.ac.uk/collection/P36/current/FERTIL/"/>
<void:inDataset rdf:resource="http://vocab.nerc.ac.uk/.well-known/void"/>
</skos:Concept>
</skos:member>
<skos:member>
<skos:Concept rdf:about="http://vocab.nerc.ac.uk/collection/P35/current/EPC00028/">
<dc:identifier>SDN:P35::EPC00028</dc:identifier>
<dce:identifier>SDN:P35::EPC00028</dce:identifier>
<dc:date>2016-10-20 11:27:18.0</dc:date>
<skos:notation>SDN:P35::EPC00028</skos:notation>
<skos:prefLabel xml:lang="en">Water body dissolved rubidium</skos:prefLabel>
<skos:altLabel>Dissolved Rb</skos:altLabel>
<skos:definition xml:lang="en">Concentration of the metal per unit volume of a river, estuary, sea or ocean by any method in filtered water (any filter type).</skos:definition>
<owl:versionInfo>3</owl:versionInfo>
<pav:hasCurrentVersion rdf:resource="http://vocab.nerc.ac.uk/collection/P35/current/EPC00028/3/"/>
<pav:version>3</pav:version>
<pav:authoredOn>2016-10-20 11:27:18.0</pav:authoredOn>
<skos:note xml:lang="en">accepted</skos:note>
<owl:deprecated>false</owl:deprecated>
<skos:narrower rdf:resource="http://vocab.nerc.ac.uk/collection/P01/current/RWS00152/"/>
<skos:related rdf:resource="http://vocab.nerc.ac.uk/collection/P06/current/UPNM/"/>
<skos:broader rdf:resource="http://vocab.nerc.ac.uk/collection/P36/current/HVYMTL/"/>
<void:inDataset rdf:resource="http://vocab.nerc.ac.uk/.well-known/void"/>
</skos:Concept>
</skos:member>
<skos:member>
<skos:Concept rdf:about="http://vocab.nerc.ac.uk/collection/P35/current/EPC00029/">
<dc:identifier>SDN:P35::EPC00029</dc:identifier>
<dce:identifier>SDN:P35::EPC00029</dce:identifier>
<dc:date>2016-10-20 11:27:18.0</dc:date>
<skos:notation>SDN:P35::EPC00029</skos:notation>
<skos:prefLabel xml:lang="en">Water body dissolved selenium</skos:prefLabel>
<skos:altLabel>Dissolved Se</skos:altLabel>
<skos:definition xml:lang="en">Concentration of the metal per unit volume of a river, estuary, sea or ocean by any method in filtered water (any filter type).</skos:definition>
<owl:versionInfo>3</owl:versionInfo>
<pav:hasCurrentVersion rdf:resource="http://vocab.nerc.ac.uk/collection/P35/current/EPC00029/3/"/>
<pav:version>3</pav:version>
<pav:authoredOn>2016-10-20 11:27:18.0</pav:authoredOn>
<skos:note xml:lang="en">accepted</skos:note>
<owl:deprecated>false</owl:deprecated>
<skos:narrower rdf:resource="http://vocab.nerc.ac.uk/collection/P01/current/RWS00142/"/>
<skos:related rdf:resource="http://vocab.nerc.ac.uk/collection/P06/current/UPNM/"/>
<skos:broader rdf:resource="http://vocab.nerc.ac.uk/collection/P36/current/HVYMTL/"/>
<void:inDataset rdf:resource="http://vocab.nerc.ac.uk/.well-known/void"/>
</skos:Concept>
</skos:member>
<skos:member>
<skos:Concept rdf:about="http://vocab.nerc.ac.uk/collection/P35/current/EPC00030/">
<dc:identifier>SDN:P35::EPC00030</dc:identifier>
<dce:identifier>SDN:P35::EPC00030</dce:identifier>
<dc:date>2016-10-20 11:27:18.0</dc:date>
<skos:notation>SDN:P35::EPC00030</skos:notation>
<skos:prefLabel xml:lang="en">Water body dissolved silver</skos:prefLabel>
<skos:altLabel>Dissolved Ag</skos:altLabel>
<skos:definition xml:lang="en">Concentration of the metal per unit volume of a river, estuary, sea or ocean by any method in filtered water (any filter type).</skos:definition>
<owl:versionInfo>3</owl:versionInfo>
<pav:hasCurrentVersion rdf:resource="http://vocab.nerc.ac.uk/collection/P35/current/EPC00030/3/"/>
<pav:version>3</pav:version>
<pav:authoredOn>2016-10-20 11:27:18.0</pav:authoredOn>
<skos:note xml:lang="en">accepted</skos:note>
<owl:deprecated>false</owl:deprecated>
<skos:narrower rdf:resource="http://vocab.nerc.ac.uk/collection/P01/current/AGVOLDMS/"/>
<skos:narrower rdf:resource="http://vocab.nerc.ac.uk/collection/P01/current/RWS00154/"/>
<skos:narrower rdf:resource="http://vocab.nerc.ac.uk/collection/P01/current/MTWD00AG/"/>
<skos:related rdf:resource="http://vocab.nerc.ac.uk/collection/P06/current/UPNM/"/>
<skos:broader rdf:resource="http://vocab.nerc.ac.uk/collection/P36/current/HVYMTL/"/>
<void:inDataset rdf:resource="http://vocab.nerc.ac.uk/.well-known/void"/>
</skos:Concept>
</skos:member>
<skos:member>
<skos:Concept rdf:about="http://vocab.nerc.ac.uk/collection/P35/current/EPC00031/">
<dc:identifier>SDN:P35::EPC00031</dc:identifier>
<dce:identifier>SDN:P35::EPC00031</dce:identifier>
<dc:date>2016-10-20 11:27:18.0</dc:date>
<skos:notation>SDN:P35::EPC00031</skos:notation>
<skos:prefLabel xml:lang="en">Water body dissolved strontium</skos:prefLabel>
<skos:altLabel>Dissolved Sr</skos:altLabel>
<skos:definition xml:lang="en">Concentration of the metal per unit volume of a river, estuary, sea or ocean by any method in filtered water (any filter type).</skos:definition>
<owl:versionInfo>3</owl:versionInfo>
<pav:hasCurrentVersion rdf:resource="http://vocab.nerc.ac.uk/collection/P35/current/EPC00031/3/"/>
<pav:version>3</pav:version>
<pav:authoredOn>2016-10-20 11:27:18.0</pav:authoredOn>
<skos:note xml:lang="en">accepted</skos:note>
<owl:deprecated>false</owl:deprecated>
<skos:narrower rdf:resource="http://vocab.nerc.ac.uk/collection/P01/current/RWS00161/"/>
<skos:related rdf:resource="http://vocab.nerc.ac.uk/collection/P06/current/UPNM/"/>
<skos:broader rdf:resource="http://vocab.nerc.ac.uk/collection/P36/current/HVYMTL/"/>
<void:inDataset rdf:resource="http://vocab.nerc.ac.uk/.well-known/void"/>
</skos:Concept>
</skos:member>
<skos:member>
<skos:Concept rdf:about="http://vocab.nerc.ac.uk/collection/P35/current/EPC00032/">
<dc:identifier>SDN:P35::EPC00032</dc:identifier>
<dce:identifier>SDN:P35::EPC00032</dce:identifier>
<dc:date>2016-10-20 11:27:18.0</dc:date>
<skos:notation>SDN:P35::EPC00032</skos:notation>
<skos:prefLabel xml:lang="en">Water body dissolved tellurium</skos:prefLabel>
<skos:altLabel>Dissolved Te</skos:altLabel>
<skos:definition xml:lang="en">Concentration of the metal per unit volume of a river, estuary, sea or ocean by any method in filtered water (any filter type).</skos:definition>
<owl:versionInfo>3</owl:versionInfo>
<pav:hasCurrentVersion rdf:resource="http://vocab.nerc.ac.uk/collection/P35/current/EPC00032/3/"/>
<pav:version>3</pav:version>
<pav:authoredOn>2016-10-20 11:27:18.0</pav:authoredOn>
<skos:note xml:lang="en">accepted</skos:note>
<owl:deprecated>false</owl:deprecated>
<skos:narrower rdf:resource="http://vocab.nerc.ac.uk/collection/P01/current/RWS00145/"/>
<skos:related rdf:resource="http://vocab.nerc.ac.uk/collection/P06/current/UPNM/"/>
<skos:broader rdf:resource="http://vocab.nerc.ac.uk/collection/P36/current/HVYMTL/"/>
<void:inDataset rdf:resource="http://vocab.nerc.ac.uk/.well-known/void"/>
</skos:Concept>
</skos:member>
<skos:member>
<skos:Concept rdf:about="http://vocab.nerc.ac.uk/collection/P35/current/EPC00033/">
<dc:identifier>SDN:P35::EPC00033</dc:identifier>
<dce:identifier>SDN:P35::EPC00033</dce:identifier>
<dc:date>2016-10-20 11:27:18.0</dc:date>
<skos:notation>SDN:P35::EPC00033</skos:notation>
<skos:prefLabel xml:lang="en">Water body dissolved thallium</skos:prefLabel>
<skos:altLabel>Dissolved Tl</skos:altLabel>
<skos:definition xml:lang="en">Concentration of the metal per unit volume of a river, estuary, sea or ocean by any method in filtered water (any filter type).</skos:definition>
<owl:versionInfo>3</owl:versionInfo>
<pav:hasCurrentVersion rdf:resource="http://vocab.nerc.ac.uk/collection/P35/current/EPC00033/3/"/>
<pav:version>3</pav:version>
<pav:authoredOn>2016-10-20 11:27:18.0</pav:authoredOn>
<skos:note xml:lang="en">accepted</skos:note>
<owl:deprecated>false</owl:deprecated>
<skos:narrower rdf:resource="http://vocab.nerc.ac.uk/collection/P01/current/RWS00160/"/>
<skos:related rdf:resource="http://vocab.nerc.ac.uk/collection/P06/current/UPNM/"/>
<skos:broader rdf:resource="http://vocab.nerc.ac.uk/collection/P36/current/HVYMTL/"/>
<void:inDataset rdf:resource="http://vocab.nerc.ac.uk/.well-known/void"/>
</skos:Concept>
</skos:member>
<skos:member>
<skos:Concept rdf:about="http://vocab.nerc.ac.uk/collection/P35/current/EPC00034/">
<dc:identifier>SDN:P35::EPC00034</dc:identifier>
<dce:identifier>SDN:P35::EPC00034</dce:identifier>
<dc:date>2016-10-20 11:27:18.0</dc:date>
<skos:notation>SDN:P35::EPC00034</skos:notation>
<skos:prefLabel xml:lang="en">Water body dissolved tin</skos:prefLabel>
<skos:altLabel>Dissolved Sn</skos:altLabel>
<skos:definition xml:lang="en">Concentration of the metal per unit volume of a river, estuary, sea or ocean by any method in filtered water (any filter type).</skos:definition>
<owl:versionInfo>3</owl:versionInfo>
<pav:hasCurrentVersion rdf:resource="http://vocab.nerc.ac.uk/collection/P35/current/EPC00034/3/"/>
<pav:version>3</pav:version>
<pav:authoredOn>2016-10-20 11:27:18.0</pav:authoredOn>
<skos:note xml:lang="en">accepted</skos:note>
<owl:deprecated>false</owl:deprecated>
<skos:narrower rdf:resource="http://vocab.nerc.ac.uk/collection/P01/current/RWS00158/"/>
<skos:related rdf:resource="http://vocab.nerc.ac.uk/collection/P06/current/UPNM/"/>
<skos:broader rdf:resource="http://vocab.nerc.ac.uk/collection/P36/current/HVYMTL/"/>
<void:inDataset rdf:resource="http://vocab.nerc.ac.uk/.well-known/void"/>
</skos:Concept>
</skos:member>
<skos:member>
<skos:Concept rdf:about="http://vocab.nerc.ac.uk/collection/P35/current/EPC00035/">
<dc:identifier>SDN:P35::EPC00035</dc:identifier>
<dce:identifier>SDN:P35::EPC00035</dce:identifier>
<dc:date>2016-10-20 11:27:18.0</dc:date>
<skos:notation>SDN:P35::EPC00035</skos:notation>
<skos:prefLabel xml:lang="en">Water body dissolved titanium</skos:prefLabel>
<skos:altLabel>Dissolved Ti</skos:altLabel>
<skos:definition xml:lang="en">Concentration of the metal per unit volume of a river, estuary, sea or ocean by any method in filtered water (any filter type).</skos:definition>
<owl:versionInfo>3</owl:versionInfo>
<pav:hasCurrentVersion rdf:resource="http://vocab.nerc.ac.uk/collection/P35/current/EPC00035/3/"/>
<pav:version>3</pav:version>
<pav:authoredOn>2016-10-20 11:27:18.0</pav:authoredOn>
<skos:note xml:lang="en">accepted</skos:note>
<owl:deprecated>false</owl:deprecated>
<skos:narrower rdf:resource="http://vocab.nerc.ac.uk/collection/P01/current/RWS00155/"/>
<skos:related rdf:resource="http://vocab.nerc.ac.uk/collection/P06/current/UPNM/"/>
<skos:broader rdf:resource="http://vocab.nerc.ac.uk/collection/P36/current/HVYMTL/"/>
<void:inDataset rdf:resource="http://vocab.nerc.ac.uk/.well-known/void"/>
</skos:Concept>
</skos:member>
<skos:member>
<skos:Concept rdf:about="http://vocab.nerc.ac.uk/collection/P35/current/EPC00036/">
<dc:identifier>SDN:P35::EPC00036</dc:identifier>
<dce:identifier>SDN:P35::EPC00036</dce:identifier>
<dc:date>2016-10-20 11:27:18.0</dc:date>
<skos:notation>SDN:P35::EPC00036</skos:notation>
<skos:prefLabel xml:lang="en">Water body dissolved uranium</skos:prefLabel>
<skos:altLabel>Dissolved U</skos:altLabel>
<skos:definition xml:lang="en">Concentration of the metal per unit volume of a river, estuary, sea or ocean by any method in filtered water (any filter type).</skos:definition>
<owl:versionInfo>3</owl:versionInfo>
<pav:hasCurrentVersion rdf:resource="http://vocab.nerc.ac.uk/collection/P35/current/EPC00036/3/"/>
<pav:version>3</pav:version>
<pav:authoredOn>2016-10-20 11:27:18.0</pav:authoredOn>
<skos:note xml:lang="en">accepted</skos:note>
<owl:deprecated>false</owl:deprecated>
<skos:narrower rdf:resource="http://vocab.nerc.ac.uk/collection/P01/current/RWS00153/"/>
<skos:narrower rdf:resource="http://vocab.nerc.ac.uk/collection/P01/current/URICPMS1/"/>
<skos:related rdf:resource="http://vocab.nerc.ac.uk/collection/P06/current/UPNM/"/>
<skos:broader rdf:resource="http://vocab.nerc.ac.uk/collection/P36/current/HVYMTL/"/>
<void:inDataset rdf:resource="http://vocab.nerc.ac.uk/.well-known/void"/>
</skos:Concept>
</skos:member>
<skos:member>
<skos:Concept rdf:about="http://vocab.nerc.ac.uk/collection/P35/current/EPC00037/">
<dc:identifier>SDN:P35::EPC00037</dc:identifier>
<dce:identifier>SDN:P35::EPC00037</dce:identifier>
<dc:date>2016-10-20 11:27:18.0</dc:date>
<skos:notation>SDN:P35::EPC00037</skos:notation>
<skos:prefLabel xml:lang="en">Water body dissolved vanadium</skos:prefLabel>
<skos:altLabel>Dissolved V</skos:altLabel>
<skos:definition xml:lang="en">Concentration of the metal per unit volume of a river, estuary, sea or ocean by any method in filtered water (any filter type).</skos:definition>
<owl:versionInfo>3</owl:versionInfo>
<pav:hasCurrentVersion rdf:resource="http://vocab.nerc.ac.uk/collection/P35/current/EPC00037/3/"/>
<pav:version>3</pav:version>
<pav:authoredOn>2016-10-20 11:27:18.0</pav:authoredOn>
<skos:note xml:lang="en">accepted</skos:note>
<owl:deprecated>false</owl:deprecated>
<skos:narrower rdf:resource="http://vocab.nerc.ac.uk/collection/P01/current/RWS00159/"/>
<skos:narrower rdf:resource="http://vocab.nerc.ac.uk/collection/P01/current/MTWD0001/"/>
<skos:related rdf:resource="http://vocab.nerc.ac.uk/collection/P06/current/UPNM/"/>
<skos:broader rdf:resource="http://vocab.nerc.ac.uk/collection/P36/current/HVYMTL/"/>
<void:inDataset rdf:resource="http://vocab.nerc.ac.uk/.well-known/void"/>
</skos:Concept>
</skos:member>
<skos:member>
<skos:Concept rdf:about="http://vocab.nerc.ac.uk/collection/P35/current/EPC00038/">
<dc:identifier>SDN:P35::EPC00038</dc:identifier>
<dce:identifier>SDN:P35::EPC00038</dce:identifier>
<dc:date>2016-10-20 11:27:18.0</dc:date>
<skos:notation>SDN:P35::EPC00038</skos:notation>
<skos:prefLabel xml:lang="en">Water body dissolved zinc</skos:prefLabel>
<skos:altLabel>Dissolved Zn</skos:altLabel>
<skos:definition xml:lang="en">Concentration of the metal per unit volume of a river, estuary, sea or ocean by any method in filtered water (any filter type).</skos:definition>
<owl:versionInfo>3</owl:versionInfo>
<pav:hasCurrentVersion rdf:resource="http://vocab.nerc.ac.uk/collection/P35/current/EPC00038/3/"/>
<pav:version>3</pav:version>
<pav:authoredOn>2016-10-20 11:27:18.0</pav:authoredOn>
<skos:note xml:lang="en">accepted</skos:note>
<owl:deprecated>false</owl:deprecated>
<skos:narrower rdf:resource="http://vocab.nerc.ac.uk/collection/P01/current/MTWD0057/"/>
<skos:narrower rdf:resource="http://vocab.nerc.ac.uk/collection/P01/current/ZNXXFXD2/"/>
<skos:narrower rdf:resource="http://vocab.nerc.ac.uk/collection/P01/current/ZNVGFAAS/"/>
<skos:narrower rdf:resource="http://vocab.nerc.ac.uk/collection/P01/current/ZNCOICP5/"/>
<skos:narrower rdf:resource="http://vocab.nerc.ac.uk/collection/P01/current/ZN04ICP6/"/>
<skos:narrower rdf:resource="http://vocab.nerc.ac.uk/collection/P01/current/ZN02FIF1/"/>
<skos:narrower rdf:resource="http://vocab.nerc.ac.uk/collection/P01/current/RWS00146/"/>
<skos:narrower rdf:resource="http://vocab.nerc.ac.uk/collection/P01/current/ODSDM010/"/>
<skos:narrower rdf:resource="http://vocab.nerc.ac.uk/collection/P01/current/CDZNICP1/"/>
<skos:narrower rdf:resource="http://vocab.nerc.ac.uk/collection/P01/current/ZNXXAADZ/"/>
<skos:narrower rdf:resource="http://vocab.nerc.ac.uk/collection/P01/current/ZNXXCVDX/"/>
<skos:related rdf:resource="http://vocab.nerc.ac.uk/collection/P06/current/UPNM/"/>
<skos:broader rdf:resource="http://vocab.nerc.ac.uk/collection/P36/current/HVYMTL/"/>
<void:inDataset rdf:resource="http://vocab.nerc.ac.uk/.well-known/void"/>
</skos:Concept>
</skos:member>
<skos:member>
<skos:Concept rdf:about="http://vocab.nerc.ac.uk/collection/P35/current/EPC00039/">
<dc:identifier>SDN:P35::EPC00039</dc:identifier>
<dce:identifier>SDN:P35::EPC00039</dce:identifier>
<dc:date>2016-10-20 11:27:18.0</dc:date>
<skos:notation>SDN:P35::EPC00039</skos:notation>
<skos:prefLabel xml:lang="en">Water body dissolved+particulate aluminium</skos:prefLabel>
<skos:altLabel>Dissolved+particulate Al</skos:altLabel>
<skos:definition xml:lang="en">Concentration of the metal per unit volume of a river, estuary, sea or ocean by any method in unfiltered water.</skos:definition>
<owl:versionInfo>3</owl:versionInfo>
<pav:hasCurrentVersion rdf:resource="http://vocab.nerc.ac.uk/collection/P35/current/EPC00039/3/"/>
<pav:version>3</pav:version>
<pav:authoredOn>2016-10-20 11:27:18.0</pav:authoredOn>
<skos:note xml:lang="en">accepted</skos:note>
<owl:deprecated>false</owl:deprecated>
<skos:narrower rdf:resource="http://vocab.nerc.ac.uk/collection/P01/current/ALVOLLGF/"/>
<skos:narrower rdf:resource="http://vocab.nerc.ac.uk/collection/P01/current/DGTLALXX/"/>
<skos:narrower rdf:resource="http://vocab.nerc.ac.uk/collection/P01/current/ALXXLGTX/"/>
<skos:related rdf:resource="http://vocab.nerc.ac.uk/collection/P06/current/UPNM/"/>
<skos:broader rdf:resource="http://vocab.nerc.ac.uk/collection/P36/current/HVYMTL/"/>
<void:inDataset rdf:resource="http://vocab.nerc.ac.uk/.well-known/void"/>
</skos:Concept>
</skos:member>
<skos:member>
<skos:Concept rdf:about="http://vocab.nerc.ac.uk/collection/P35/current/EPC00040/">
<dc:identifier>SDN:P35::EPC00040</dc:identifier>
<dce:identifier>SDN:P35::EPC00040</dce:identifier>
<dc:date>2016-10-20 11:27:18.0</dc:date>
<skos:notation>SDN:P35::EPC00040</skos:notation>
<skos:prefLabel xml:lang="en">Water body dissolved+particulate antimony</skos:prefLabel>
<skos:altLabel>Dissolved+particulate Sb</skos:altLabel>
<skos:definition xml:lang="en">Concentration of the metal per unit volume of a river, estuary, sea or ocean by any method in unfiltered water.</skos:definition>
<owl:versionInfo>3</owl:versionInfo>
<pav:hasCurrentVersion rdf:resource="http://vocab.nerc.ac.uk/collection/P35/current/EPC00040/3/"/>
<pav:version>3</pav:version>
<pav:authoredOn>2016-10-20 11:27:18.0</pav:authoredOn>
<skos:note xml:lang="en">accepted</skos:note>
<owl:deprecated>false</owl:deprecated>
<skos:narrower rdf:resource="http://vocab.nerc.ac.uk/collection/P01/current/RWS00031/"/>
<skos:related rdf:resource="http://vocab.nerc.ac.uk/collection/P06/current/UPNM/"/>
<skos:broader rdf:resource="http://vocab.nerc.ac.uk/collection/P36/current/HVYMTL/"/>
<void:inDataset rdf:resource="http://vocab.nerc.ac.uk/.well-known/void"/>
</skos:Concept>
</skos:member>
<skos:member>
<skos:Concept rdf:about="http://vocab.nerc.ac.uk/collection/P35/current/EPC00041/">
<dc:identifier>SDN:P35::EPC00041</dc:identifier>
<dce:identifier>SDN:P35::EPC00041</dce:identifier>
<dc:date>2016-10-20 11:27:18.0</dc:date>
<skos:notation>SDN:P35::EPC00041</skos:notation>
<skos:prefLabel xml:lang="en">Water body dissolved+particulate arsenic</skos:prefLabel>
<skos:altLabel>Dissolved+particulate As</skos:altLabel>
<skos:definition xml:lang="en">Concentration of the metal per unit volume of a river, estuary, sea or ocean by any method in unfiltered water.</skos:definition>
<owl:versionInfo>3</owl:versionInfo>
<pav:hasCurrentVersion rdf:resource="http://vocab.nerc.ac.uk/collection/P35/current/EPC00041/3/"/>
<pav:version>3</pav:version>
<pav:authoredOn>2016-10-20 11:27:18.0</pav:authoredOn>
<skos:note xml:lang="en">accepted</skos:note>
<owl:deprecated>false</owl:deprecated>
<skos:narrower rdf:resource="http://vocab.nerc.ac.uk/collection/P01/current/RWS00025/"/>
<skos:related rdf:resource="http://vocab.nerc.ac.uk/collection/P06/current/UPNM/"/>
<skos:broader rdf:resource="http://vocab.nerc.ac.uk/collection/P36/current/HVYMTL/"/>
<void:inDataset rdf:resource="http://vocab.nerc.ac.uk/.well-known/void"/>
</skos:Concept>
</skos:member>
<skos:member>
<skos:Concept rdf:about="http://vocab.nerc.ac.uk/collection/P35/current/EPC00042/">
<dc:identifier>SDN:P35::EPC00042</dc:identifier>
<dce:identifier>SDN:P35::EPC00042</dce:identifier>
<dc:date>2016-10-20 11:27:18.0</dc:date>
<skos:notation>SDN:P35::EPC00042</skos:notation>
<skos:prefLabel xml:lang="en">Water body dissolved+particulate barium</skos:prefLabel>
<skos:altLabel>Dissolved+particulate Ba</skos:altLabel>
<skos:definition xml:lang="en">Concentration of the metal per unit volume of a river, estuary, sea or ocean by any method in unfiltered water.</skos:definition>
<owl:versionInfo>3</owl:versionInfo>
<pav:hasCurrentVersion rdf:resource="http://vocab.nerc.ac.uk/collection/P35/current/EPC00042/3/"/>
<pav:version>3</pav:version>
<pav:authoredOn>2016-10-20 11:27:18.0</pav:authoredOn>
<skos:note xml:lang="en">accepted</skos:note>
<owl:deprecated>false</owl:deprecated>
<skos:narrower rdf:resource="http://vocab.nerc.ac.uk/collection/P01/current/RWS00029/"/>
<skos:narrower rdf:resource="http://vocab.nerc.ac.uk/collection/P01/current/BAXXXXMS/"/>
<skos:narrower rdf:resource="http://vocab.nerc.ac.uk/collection/P01/current/BAXXICP3/"/>
<skos:related rdf:resource="http://vocab.nerc.ac.uk/collection/P06/current/UPNM/"/>
<skos:broader rdf:resource="http://vocab.nerc.ac.uk/collection/P36/current/HVYMTL/"/>
<void:inDataset rdf:resource="http://vocab.nerc.ac.uk/.well-known/void"/>
</skos:Concept>
</skos:member>
<skos:member>
<skos:Concept rdf:about="http://vocab.nerc.ac.uk/collection/P35/current/EPC00043/">
<dc:identifier>SDN:P35::EPC00043</dc:identifier>
<dce:identifier>SDN:P35::EPC00043</dce:identifier>
<dc:date>2016-10-20 11:27:18.0</dc:date>
<skos:notation>SDN:P35::EPC00043</skos:notation>
<skos:prefLabel xml:lang="en">Water body dissolved+particulate beryllium</skos:prefLabel>
<skos:altLabel>Dissolved+particulate Be</skos:altLabel>
<skos:definition xml:lang="en">Concentration of the metal per unit volume of a river, estuary, sea or ocean by any method in unfiltered water.</skos:definition>
<owl:versionInfo>3</owl:versionInfo>
<pav:hasCurrentVersion rdf:resource="http://vocab.nerc.ac.uk/collection/P35/current/EPC00043/3/"/>
<pav:version>3</pav:version>
<pav:authoredOn>2016-10-20 11:27:18.0</pav:authoredOn>
<skos:note xml:lang="en">accepted</skos:note>
<owl:deprecated>false</owl:deprecated>
<skos:narrower rdf:resource="http://vocab.nerc.ac.uk/collection/P01/current/RWS00030/"/>
<skos:related rdf:resource="http://vocab.nerc.ac.uk/collection/P06/current/UPNM/"/>
<skos:broader rdf:resource="http://vocab.nerc.ac.uk/collection/P36/current/HVYMTL/"/>
<void:inDataset rdf:resource="http://vocab.nerc.ac.uk/.well-known/void"/>
</skos:Concept>
</skos:member>
<skos:member>
<skos:Concept rdf:about="http://vocab.nerc.ac.uk/collection/P35/current/EPC00044/">
<dc:identifier>SDN:P35::EPC00044</dc:identifier>
<dce:identifier>SDN:P35::EPC00044</dce:identifier>
<dc:date>2016-10-20 11:27:18.0</dc:date>
<skos:notation>SDN:P35::EPC00044</skos:notation>
<skos:prefLabel xml:lang="en">Water body dissolved+particulate boron</skos:prefLabel>
<skos:altLabel>Dissolved+particulate B</skos:altLabel>
<skos:definition xml:lang="en">Concentration of the metal per unit volume of a river, estuary, sea or ocean by any method in unfiltered water.</skos:definition>
<owl:versionInfo>3</owl:versionInfo>
<pav:hasCurrentVersion rdf:resource="http://vocab.nerc.ac.uk/collection/P35/current/EPC00044/3/"/>
<pav:version>3</pav:version>
<pav:authoredOn>2016-10-20 11:27:18.0</pav:authoredOn>
<skos:note xml:lang="en">accepted</skos:note>
<owl:deprecated>false</owl:deprecated>
<skos:narrower rdf:resource="http://vocab.nerc.ac.uk/collection/P01/current/RWS00034/"/>
<skos:related rdf:resource="http://vocab.nerc.ac.uk/collection/P06/current/UPNM/"/>
<skos:broader rdf:resource="http://vocab.nerc.ac.uk/collection/P36/current/HVYMTL/"/>
<void:inDataset rdf:resource="http://vocab.nerc.ac.uk/.well-known/void"/>
</skos:Concept>
</skos:member>
<skos:member>
<skos:Concept rdf:about="http://vocab.nerc.ac.uk/collection/P35/current/EPC00045/">
<dc:identifier>SDN:P35::EPC00045</dc:identifier>
<dce:identifier>SDN:P35::EPC00045</dce:identifier>
<dc:date>2016-10-20 11:27:18.0</dc:date>
<skos:notation>SDN:P35::EPC00045</skos:notation>
<skos:prefLabel xml:lang="en">Water body dissolved+particulate cadmium</skos:prefLabel>
<skos:altLabel>Dissolved+particulate Cd</skos:altLabel>
<skos:definition xml:lang="en">Concentration of the metal per unit volume of a river, estuary, sea or ocean by any method in unfiltered water.</skos:definition>
<owl:versionInfo>3</owl:versionInfo>
<pav:hasCurrentVersion rdf:resource="http://vocab.nerc.ac.uk/collection/P35/current/EPC00045/3/"/>
<pav:version>3</pav:version>
<pav:authoredOn>2016-10-20 11:27:18.0</pav:authoredOn>
<skos:note xml:lang="en">accepted</skos:note>
<owl:deprecated>false</owl:deprecated>
<skos:narrower rdf:resource="http://vocab.nerc.ac.uk/collection/P01/current/DGTLCDXX/"/>
<skos:narrower rdf:resource="http://vocab.nerc.ac.uk/collection/P01/current/CDUFICXX/"/>
<skos:narrower rdf:resource="http://vocab.nerc.ac.uk/collection/P01/current/CDUFWC02/"/>
<skos:related rdf:resource="http://vocab.nerc.ac.uk/collection/P06/current/UPNM/"/>
<skos:broader rdf:resource="http://vocab.nerc.ac.uk/collection/P36/current/HVYMTL/"/>
<void:inDataset rdf:resource="http://vocab.nerc.ac.uk/.well-known/void"/>
</skos:Concept>
</skos:member>
<skos:member>
<skos:Concept rdf:about="http://vocab.nerc.ac.uk/collection/P35/current/EPC00046/">
<dc:identifier>SDN:P35::EPC00046</dc:identifier>
<dce:identifier>SDN:P35::EPC00046</dce:identifier>
<dc:date>2016-10-20 11:27:18.0</dc:date>
<skos:notation>SDN:P35::EPC00046</skos:notation>
<skos:prefLabel xml:lang="en">Water body dissolved+particulate chromium</skos:prefLabel>
<skos:altLabel>Dissolved+particulate Cr</skos:altLabel>
<skos:definition xml:lang="en">Concentration of the metal per unit volume of a river, estuary, sea or ocean by any method in unfiltered water.</skos:definition>
<owl:versionInfo>3</owl:versionInfo>
<pav:hasCurrentVersion rdf:resource="http://vocab.nerc.ac.uk/collection/P35/current/EPC00046/3/"/>
<pav:version>3</pav:version>
<pav:authoredOn>2016-10-20 11:27:18.0</pav:authoredOn>
<skos:note xml:lang="en">accepted</skos:note>
<owl:deprecated>false</owl:deprecated>
<skos:narrower rdf:resource="http://vocab.nerc.ac.uk/collection/P01/current/CRUFWC02/"/>
<skos:narrower rdf:resource="http://vocab.nerc.ac.uk/collection/P01/current/CRXXCVDX/"/>
<skos:related rdf:resource="http://vocab.nerc.ac.uk/collection/P06/current/UPNM/"/>
<skos:broader rdf:resource="http://vocab.nerc.ac.uk/collection/P36/current/HVYMTL/"/>
<void:inDataset rdf:resource="http://vocab.nerc.ac.uk/.well-known/void"/>
</skos:Concept>
</skos:member>
<skos:member>
<skos:Concept rdf:about="http://vocab.nerc.ac.uk/collection/P35/current/EPC00047/">
<dc:identifier>SDN:P35::EPC00047</dc:identifier>
<dce:identifier>SDN:P35::EPC00047</dce:identifier>
<dc:date>2016-10-20 11:27:18.0</dc:date>
<skos:notation>SDN:P35::EPC00047</skos:notation>
<skos:prefLabel xml:lang="en">Water body dissolved+particulate cobalt</skos:prefLabel>
<skos:altLabel>Dissolved+particulate Co</skos:altLabel>
<skos:definition xml:lang="en">Concentration of the metal per unit volume of a river, estuary, sea or ocean by any method in unfiltered water.</skos:definition>
<owl:versionInfo>3</owl:versionInfo>
<pav:hasCurrentVersion rdf:resource="http://vocab.nerc.ac.uk/collection/P35/current/EPC00047/3/"/>
<pav:version>3</pav:version>
<pav:authoredOn>2016-10-20 11:27:18.0</pav:authoredOn>
<skos:note xml:lang="en">accepted</skos:note>
<owl:deprecated>false</owl:deprecated>
<skos:narrower rdf:resource="http://vocab.nerc.ac.uk/collection/P01/current/COXXCVDX/"/>
<skos:narrower rdf:resource="http://vocab.nerc.ac.uk/collection/P01/current/RWS00039/"/>
<skos:narrower rdf:resource="http://vocab.nerc.ac.uk/collection/P01/current/DGTLCOXX/"/>
<skos:related rdf:resource="http://vocab.nerc.ac.uk/collection/P06/current/UPNM/"/>
<skos:broader rdf:resource="http://vocab.nerc.ac.uk/collection/P36/current/HVYMTL/"/>
<void:inDataset rdf:resource="http://vocab.nerc.ac.uk/.well-known/void"/>
</skos:Concept>
</skos:member>
<skos:member>
<skos:Concept rdf:about="http://vocab.nerc.ac.uk/collection/P35/current/EPC00048/">
<dc:identifier>SDN:P35::EPC00048</dc:identifier>
<dce:identifier>SDN:P35::EPC00048</dce:identifier>
<dc:date>2016-10-20 11:27:18.0</dc:date>
<skos:notation>SDN:P35::EPC00048</skos:notation>
<skos:prefLabel xml:lang="en">Water body dissolved+particulate copper</skos:prefLabel>
<skos:altLabel>Dissolved+particulate Cu</skos:altLabel>
<skos:definition xml:lang="en">Concentration of the metal per unit volume of a river, estuary, sea or ocean by any method in unfiltered water.</skos:definition>
<owl:versionInfo>3</owl:versionInfo>
<pav:hasCurrentVersion rdf:resource="http://vocab.nerc.ac.uk/collection/P35/current/EPC00048/3/"/>
<pav:version>3</pav:version>
<pav:authoredOn>2016-10-20 11:27:18.0</pav:authoredOn>
<skos:note xml:lang="en">accepted</skos:note>
<owl:deprecated>false</owl:deprecated>
<skos:narrower rdf:resource="http://vocab.nerc.ac.uk/collection/P01/current/CUTDICP5/"/>
<skos:narrower rdf:resource="http://vocab.nerc.ac.uk/collection/P01/current/DGTLCUXX/"/>
<skos:narrower rdf:resource="http://vocab.nerc.ac.uk/collection/P01/current/CUXXZZZZ/"/>
<skos:related rdf:resource="http://vocab.nerc.ac.uk/collection/P06/current/UPNM/"/>
<skos:broader rdf:resource="http://vocab.nerc.ac.uk/collection/P36/current/HVYMTL/"/>
<void:inDataset rdf:resource="http://vocab.nerc.ac.uk/.well-known/void"/>
</skos:Concept>
</skos:member>
<skos:member>
<skos:Concept rdf:about="http://vocab.nerc.ac.uk/collection/P35/current/EPC00049/">
<dc:identifier>SDN:P35::EPC00049</dc:identifier>
<dce:identifier>SDN:P35::EPC00049</dce:identifier>
<dc:date>2016-10-20 11:27:18.0</dc:date>
<skos:notation>SDN:P35::EPC00049</skos:notation>
<skos:prefLabel xml:lang="en">Water body dissolved+particulate iron (total chemical species)</skos:prefLabel>
<skos:altLabel>Dissolved+particulate total Fe</skos:altLabel>
<skos:definition xml:lang="en">Concentration of the metal per unit volume of a river, estuary, sea or ocean by any method in unfiltered water. Total means the element in all possible states of valency and chemical combination.</skos:definition>
<owl:versionInfo>3</owl:versionInfo>
<pav:hasCurrentVersion rdf:resource="http://vocab.nerc.ac.uk/collection/P35/current/EPC00049/3/"/>
<pav:version>3</pav:version>
<pav:authoredOn>2016-10-20 11:27:18.0</pav:authoredOn>
<skos:note xml:lang="en">accepted</skos:note>
<owl:deprecated>false</owl:deprecated>
<skos:narrower rdf:resource="http://vocab.nerc.ac.uk/collection/P01/current/DGTLFEXX/"/>
<skos:narrower rdf:resource="http://vocab.nerc.ac.uk/collection/P01/current/FEXXCLDX/"/>
<skos:narrower rdf:resource="http://vocab.nerc.ac.uk/collection/P01/current/RWS00033/"/>
<skos:narrower rdf:resource="http://vocab.nerc.ac.uk/collection/P01/current/FEXXCVDX/"/>
<skos:related rdf:resource="http://vocab.nerc.ac.uk/collection/P06/current/UPNM/"/>
<skos:broader rdf:resource="http://vocab.nerc.ac.uk/collection/P36/current/HVYMTL/"/>
<void:inDataset rdf:resource="http://vocab.nerc.ac.uk/.well-known/void"/>
</skos:Concept>
</skos:member>
<skos:member>
<skos:Concept rdf:about="http://vocab.nerc.ac.uk/collection/P35/current/EPC00050/">
<dc:identifier>SDN:P35::EPC00050</dc:identifier>
<dce:identifier>SDN:P35::EPC00050</dce:identifier>
<dc:date>2016-10-20 11:27:18.0</dc:date>
<skos:notation>SDN:P35::EPC00050</skos:notation>
<skos:prefLabel xml:lang="en">Water body dissolved+particulate lead</skos:prefLabel>
<skos:altLabel>Dissolved+particulate Pb</skos:altLabel>
<skos:definition xml:lang="en">Concentration of the metal per unit volume of a river, estuary, sea or ocean by any method in unfiltered water.</skos:definition>
<owl:versionInfo>3</owl:versionInfo>
<pav:hasCurrentVersion rdf:resource="http://vocab.nerc.ac.uk/collection/P35/current/EPC00050/3/"/>
<pav:version>3</pav:version>
<pav:authoredOn>2016-10-20 11:27:18.0</pav:authoredOn>
<skos:note xml:lang="en">accepted</skos:note>
<owl:deprecated>false</owl:deprecated>
<skos:narrower rdf:resource="http://vocab.nerc.ac.uk/collection/P01/current/PBUFICXX/"/>
<skos:narrower rdf:resource="http://vocab.nerc.ac.uk/collection/P01/current/PBUFWC02/"/>
<skos:narrower rdf:resource="http://vocab.nerc.ac.uk/collection/P01/current/DGTLPBXX/"/>
<skos:related rdf:resource="http://vocab.nerc.ac.uk/collection/P06/current/UPNM/"/>
<skos:broader rdf:resource="http://vocab.nerc.ac.uk/collection/P36/current/HVYMTL/"/>
<void:inDataset rdf:resource="http://vocab.nerc.ac.uk/.well-known/void"/>
</skos:Concept>
</skos:member>
<skos:member>
<skos:Concept rdf:about="http://vocab.nerc.ac.uk/collection/P35/current/EPC00051/">
<dc:identifier>SDN:P35::EPC00051</dc:identifier>
<dce:identifier>SDN:P35::EPC00051</dce:identifier>
<dc:date>2016-10-20 11:27:18.0</dc:date>
<skos:notation>SDN:P35::EPC00051</skos:notation>
<skos:prefLabel xml:lang="en">Water body dissolved+particulate lithium</skos:prefLabel>
<skos:altLabel>Dissolved+particulate Li</skos:altLabel>
<skos:definition xml:lang="en">Concentration of the metal per unit volume of a river, estuary, sea or ocean by any method in unfiltered water.</skos:definition>
<owl:versionInfo>3</owl:versionInfo>
<pav:hasCurrentVersion rdf:resource="http://vocab.nerc.ac.uk/collection/P35/current/EPC00051/3/"/>
<pav:version>3</pav:version>
<pav:authoredOn>2016-10-20 11:27:18.0</pav:authoredOn>
<skos:note xml:lang="en">accepted</skos:note>
<owl:deprecated>false</owl:deprecated>
<skos:narrower rdf:resource="http://vocab.nerc.ac.uk/collection/P01/current/RWS00045/"/>
<skos:related rdf:resource="http://vocab.nerc.ac.uk/collection/P06/current/UPNM/"/>
<skos:broader rdf:resource="http://vocab.nerc.ac.uk/collection/P36/current/HVYMTL/"/>
<void:inDataset rdf:resource="http://vocab.nerc.ac.uk/.well-known/void"/>
</skos:Concept>
</skos:member>
<skos:member>
<skos:Concept rdf:about="http://vocab.nerc.ac.uk/collection/P35/current/EPC00052/">
<dc:identifier>SDN:P35::EPC00052</dc:identifier>
<dce:identifier>SDN:P35::EPC00052</dce:identifier>
<dc:date>2016-10-20 11:27:18.0</dc:date>
<skos:notation>SDN:P35::EPC00052</skos:notation>
<skos:prefLabel xml:lang="en">Water body dissolved+particulate manganese (total chemical species)</skos:prefLabel>
<skos:altLabel>Dissolved+particulate total Mn</skos:altLabel>
<skos:definition xml:lang="en">Concentration of the metal per unit volume of a river, estuary, sea or ocean by any method in unfiltered water. Total means the element in all possible states of valency and chemical combination. Total means the element in all possible states of valency and chemical combination.</skos:definition>
<owl:versionInfo>3</owl:versionInfo>
<pav:hasCurrentVersion rdf:resource="http://vocab.nerc.ac.uk/collection/P35/current/EPC00052/3/"/>
<pav:version>3</pav:version>
<pav:authoredOn>2016-10-20 11:27:18.0</pav:authoredOn>
<skos:note xml:lang="en">accepted</skos:note>
<owl:deprecated>false</owl:deprecated>
<skos:narrower rdf:resource="http://vocab.nerc.ac.uk/collection/P01/current/DGTLMNXX/"/>
<skos:narrower rdf:resource="http://vocab.nerc.ac.uk/collection/P01/current/RWS00032/"/>
<skos:related rdf:resource="http://vocab.nerc.ac.uk/collection/P06/current/UPNM/"/>
<skos:broader rdf:resource="http://vocab.nerc.ac.uk/collection/P36/current/HVYMTL/"/>
<void:inDataset rdf:resource="http://vocab.nerc.ac.uk/.well-known/void"/>
</skos:Concept>
</skos:member>
<skos:member>
<skos:Concept rdf:about="http://vocab.nerc.ac.uk/collection/P35/current/EPC00053/">
<dc:identifier>SDN:P35::EPC00053</dc:identifier>
<dce:identifier>SDN:P35::EPC00053</dce:identifier>
<dc:date>2016-10-20 11:27:18.0</dc:date>
<skos:notation>SDN:P35::EPC00053</skos:notation>
<skos:prefLabel xml:lang="en">Water body dissolved+particulate mercury (total chemical species)</skos:prefLabel>
<skos:altLabel>Dissolved+particulate total Hg</skos:altLabel>
<skos:definition xml:lang="en">Concentration of the metal per unit volume of a river, estuary, sea or ocean by any method in unfiltered water. Total means the element in all possible states of valency and chemical combination.</skos:definition>
<owl:versionInfo>3</owl:versionInfo>
<pav:hasCurrentVersion rdf:resource="http://vocab.nerc.ac.uk/collection/P35/current/EPC00053/3/"/>
<pav:version>3</pav:version>
<pav:authoredOn>2016-10-20 11:27:18.0</pav:authoredOn>
<skos:note xml:lang="en">accepted</skos:note>
<owl:deprecated>false</owl:deprecated>
<skos:narrower rdf:resource="http://vocab.nerc.ac.uk/collection/P01/current/HGTXAATX/"/>
<skos:narrower rdf:resource="http://vocab.nerc.ac.uk/collection/P01/current/HGUFCFXX/"/>
<skos:narrower rdf:resource="http://vocab.nerc.ac.uk/collection/P01/current/HGUFWC02/"/>
<skos:related rdf:resource="http://vocab.nerc.ac.uk/collection/P06/current/UPNM/"/>
<skos:broader rdf:resource="http://vocab.nerc.ac.uk/collection/P36/current/HVYMTL/"/>
<void:inDataset rdf:resource="http://vocab.nerc.ac.uk/.well-known/void"/>
</skos:Concept>
</skos:member>
<skos:member>
<skos:Concept rdf:about="http://vocab.nerc.ac.uk/collection/P35/current/EPC00054/">
<dc:identifier>SDN:P35::EPC00054</dc:identifier>
<dce:identifier>SDN:P35::EPC00054</dce:identifier>
<dc:date>2016-10-20 11:27:18.0</dc:date>
<skos:notation>SDN:P35::EPC00054</skos:notation>
<skos:prefLabel xml:lang="en">Water body dissolved+particulate molybdenum</skos:prefLabel>
<skos:altLabel>Dissolved+particulate Mo</skos:altLabel>
<skos:definition xml:lang="en">Concentration of the metal per unit volume of a river, estuary, sea or ocean by any method in unfiltered water.</skos:definition>
<owl:versionInfo>3</owl:versionInfo>
<pav:hasCurrentVersion rdf:resource="http://vocab.nerc.ac.uk/collection/P35/current/EPC00054/3/"/>
<pav:version>3</pav:version>
<pav:authoredOn>2016-10-20 11:27:18.0</pav:authoredOn>
<skos:note xml:lang="en">accepted</skos:note>
<owl:deprecated>false</owl:deprecated>
<skos:narrower rdf:resource="http://vocab.nerc.ac.uk/collection/P01/current/RWS00040/"/>
<skos:related rdf:resource="http://vocab.nerc.ac.uk/collection/P06/current/UPNM/"/>
<skos:broader rdf:resource="http://vocab.nerc.ac.uk/collection/P36/current/HVYMTL/"/>
<void:inDataset rdf:resource="http://vocab.nerc.ac.uk/.well-known/void"/>
</skos:Concept>
</skos:member>
<skos:member>
<skos:Concept rdf:about="http://vocab.nerc.ac.uk/collection/P35/current/EPC00055/">
<dc:identifier>SDN:P35::EPC00055</dc:identifier>
<dce:identifier>SDN:P35::EPC00055</dce:identifier>
<dc:date>2016-10-20 11:27:18.0</dc:date>
<skos:notation>SDN:P35::EPC00055</skos:notation>
<skos:prefLabel xml:lang="en">Water body dissolved+particulate nickel</skos:prefLabel>
<skos:altLabel>Dissolved+particulate Ni</skos:altLabel>
<skos:definition xml:lang="en">Concentration of the metal per unit volume of a river, estuary, sea or ocean by any method in unfiltered water.</skos:definition>
<owl:versionInfo>3</owl:versionInfo>
<pav:hasCurrentVersion rdf:resource="http://vocab.nerc.ac.uk/collection/P35/current/EPC00055/3/"/>
<pav:version>3</pav:version>
<pav:authoredOn>2016-10-20 11:27:18.0</pav:authoredOn>
<skos:note xml:lang="en">accepted</skos:note>
<owl:deprecated>false</owl:deprecated>
<skos:narrower rdf:resource="http://vocab.nerc.ac.uk/collection/P01/current/DGTLNIXX/"/>
<skos:narrower rdf:resource="http://vocab.nerc.ac.uk/collection/P01/current/NIXXCVDX/"/>
<skos:narrower rdf:resource="http://vocab.nerc.ac.uk/collection/P01/current/RWS00027/"/>
<skos:related rdf:resource="http://vocab.nerc.ac.uk/collection/P06/current/UPNM/"/>
<skos:broader rdf:resource="http://vocab.nerc.ac.uk/collection/P36/current/HVYMTL/"/>
<void:inDataset rdf:resource="http://vocab.nerc.ac.uk/.well-known/void"/>
</skos:Concept>
</skos:member>
<skos:member>
<skos:Concept rdf:about="http://vocab.nerc.ac.uk/collection/P35/current/EPC00056/">
<dc:identifier>SDN:P35::EPC00056</dc:identifier>
<dce:identifier>SDN:P35::EPC00056</dce:identifier>
<dc:date>2016-10-20 11:27:18.0</dc:date>
<skos:notation>SDN:P35::EPC00056</skos:notation>
<skos:prefLabel xml:lang="en">Water body dissolved+particulate rubidium</skos:prefLabel>
<skos:altLabel>Dissolved+particulate Rb</skos:altLabel>
<skos:definition xml:lang="en">Concentration of the metal per unit volume of a river, estuary, sea or ocean by any method in unfiltered water.</skos:definition>
<owl:versionInfo>3</owl:versionInfo>
<pav:hasCurrentVersion rdf:resource="http://vocab.nerc.ac.uk/collection/P35/current/EPC00056/3/"/>
<pav:version>3</pav:version>
<pav:authoredOn>2016-10-20 11:27:18.0</pav:authoredOn>
<skos:note xml:lang="en">accepted</skos:note>
<owl:deprecated>false</owl:deprecated>
<skos:narrower rdf:resource="http://vocab.nerc.ac.uk/collection/P01/current/RWS00046/"/>
<skos:related rdf:resource="http://vocab.nerc.ac.uk/collection/P06/current/UPNM/"/>
<skos:broader rdf:resource="http://vocab.nerc.ac.uk/collection/P36/current/HVYMTL/"/>
<void:inDataset rdf:resource="http://vocab.nerc.ac.uk/.well-known/void"/>
</skos:Concept>
</skos:member>
<skos:member>
<skos:Concept rdf:about="http://vocab.nerc.ac.uk/collection/P35/current/EPC00057/">
<dc:identifier>SDN:P35::EPC00057</dc:identifier>
<dce:identifier>SDN:P35::EPC00057</dce:identifier>
<dc:date>2016-10-20 11:27:18.0</dc:date>
<skos:notation>SDN:P35::EPC00057</skos:notation>
<skos:prefLabel xml:lang="en">Water body dissolved+particulate selenium</skos:prefLabel>
<skos:altLabel>Dissolved+particulate Se</skos:altLabel>
<skos:definition xml:lang="en">Concentration of the metal per unit volume of a river, estuary, sea or ocean by any method in unfiltered water.</skos:definition>
<owl:versionInfo>3</owl:versionInfo>
<pav:hasCurrentVersion rdf:resource="http://vocab.nerc.ac.uk/collection/P35/current/EPC00057/3/"/>
<pav:version>3</pav:version>
<pav:authoredOn>2016-10-20 11:27:18.0</pav:authoredOn>
<skos:note xml:lang="en">accepted</skos:note>
<owl:deprecated>false</owl:deprecated>
<skos:narrower rdf:resource="http://vocab.nerc.ac.uk/collection/P01/current/RWS00026/"/>
<skos:related rdf:resource="http://vocab.nerc.ac.uk/collection/P06/current/UPNM/"/>
<skos:broader rdf:resource="http://vocab.nerc.ac.uk/collection/P36/current/HVYMTL/"/>
<void:inDataset rdf:resource="http://vocab.nerc.ac.uk/.well-known/void"/>
</skos:Concept>
</skos:member>
<skos:member>
<skos:Concept rdf:about="http://vocab.nerc.ac.uk/collection/P35/current/EPC00058/">
<dc:identifier>SDN:P35::EPC00058</dc:identifier>
<dce:identifier>SDN:P35::EPC00058</dce:identifier>
<dc:date>2016-10-20 11:27:18.0</dc:date>
<skos:notation>SDN:P35::EPC00058</skos:notation>
<skos:prefLabel xml:lang="en">Water body dissolved+particulate silver</skos:prefLabel>
<skos:altLabel>Dissolved+particulate Ag</skos:altLabel>
<skos:definition xml:lang="en">Concentration of the metal per unit volume of a river, estuary, sea or ocean by any method in unfiltered water.</skos:definition>
<owl:versionInfo>3</owl:versionInfo>
<pav:hasCurrentVersion rdf:resource="http://vocab.nerc.ac.uk/collection/P35/current/EPC00058/3/"/>
<pav:version>3</pav:version>
<pav:authoredOn>2016-10-20 11:27:18.0</pav:authoredOn>
<skos:note xml:lang="en">accepted</skos:note>
<owl:deprecated>false</owl:deprecated>
<skos:narrower rdf:resource="http://vocab.nerc.ac.uk/collection/P01/current/RWS00037/"/>
<skos:related rdf:resource="http://vocab.nerc.ac.uk/collection/P06/current/UPNM/"/>
<skos:broader rdf:resource="http://vocab.nerc.ac.uk/collection/P36/current/HVYMTL/"/>
<void:inDataset rdf:resource="http://vocab.nerc.ac.uk/.well-known/void"/>
</skos:Concept>
</skos:member>
<skos:member>
<skos:Concept rdf:about="http://vocab.nerc.ac.uk/collection/P35/current/EPC00059/">
<dc:identifier>SDN:P35::EPC00059</dc:identifier>
<dce:identifier>SDN:P35::EPC00059</dce:identifier>
<dc:date>2016-10-20 11:27:18.0</dc:date>
<skos:notation>SDN:P35::EPC00059</skos:notation>
<skos:prefLabel xml:lang="en">Water body dissolved+particulate strontium</skos:prefLabel>
<skos:altLabel>Dissolved+particulate Sr</skos:altLabel>
<skos:definition xml:lang="en">Concentration of the metal per unit volume of a river, estuary, sea or ocean by any method in unfiltered water.</skos:definition>
<owl:versionInfo>3</owl:versionInfo>
<pav:hasCurrentVersion rdf:resource="http://vocab.nerc.ac.uk/collection/P35/current/EPC00059/3/"/>
<pav:version>3</pav:version>
<pav:authoredOn>2016-10-20 11:27:18.0</pav:authoredOn>
<skos:note xml:lang="en">accepted</skos:note>
<owl:deprecated>false</owl:deprecated>
<skos:narrower rdf:resource="http://vocab.nerc.ac.uk/collection/P01/current/RWS00044/"/>
<skos:related rdf:resource="http://vocab.nerc.ac.uk/collection/P06/current/UPNM/"/>
<skos:broader rdf:resource="http://vocab.nerc.ac.uk/collection/P36/current/HVYMTL/"/>
<void:inDataset rdf:resource="http://vocab.nerc.ac.uk/.well-known/void"/>
</skos:Concept>
</skos:member>
<skos:member>
<skos:Concept rdf:about="http://vocab.nerc.ac.uk/collection/P35/current/EPC00060/">
<dc:identifier>SDN:P35::EPC00060</dc:identifier>
<dce:identifier>SDN:P35::EPC00060</dce:identifier>
<dc:date>2016-10-20 11:27:18.0</dc:date>
<skos:notation>SDN:P35::EPC00060</skos:notation>
<skos:prefLabel xml:lang="en">Water body dissolved+particulate tellurium</skos:prefLabel>
<skos:altLabel>Dissolved+particulate Te</skos:altLabel>
<skos:definition xml:lang="en">Concentration of the metal per unit volume of a river, estuary, sea or ocean by any method in unfiltered water.</skos:definition>
<owl:versionInfo>3</owl:versionInfo>
<pav:hasCurrentVersion rdf:resource="http://vocab.nerc.ac.uk/collection/P35/current/EPC00060/3/"/>
<pav:version>3</pav:version>
<pav:authoredOn>2016-10-20 11:27:18.0</pav:authoredOn>
<skos:note xml:lang="en">accepted</skos:note>
<owl:deprecated>false</owl:deprecated>
<skos:narrower rdf:resource="http://vocab.nerc.ac.uk/collection/P01/current/RWS00036/"/>
<skos:related rdf:resource="http://vocab.nerc.ac.uk/collection/P06/current/UPNM/"/>
<skos:broader rdf:resource="http://vocab.nerc.ac.uk/collection/P36/current/HVYMTL/"/>
<void:inDataset rdf:resource="http://vocab.nerc.ac.uk/.well-known/void"/>
</skos:Concept>
</skos:member>
<skos:member>
<skos:Concept rdf:about="http://vocab.nerc.ac.uk/collection/P35/current/EPC00061/">
<dc:identifier>SDN:P35::EPC00061</dc:identifier>
<dce:identifier>SDN:P35::EPC00061</dce:identifier>
<dc:date>2016-10-20 11:27:18.0</dc:date>
<skos:notation>SDN:P35::EPC00061</skos:notation>
<skos:prefLabel xml:lang="en">Water body dissolved+particulate thallium</skos:prefLabel>
<skos:altLabel>Dissolved+particulate Tl</skos:altLabel>
<skos:definition xml:lang="en">Concentration of the metal per unit volume of a river, estuary, sea or ocean by any method in unfiltered water.</skos:definition>
<owl:versionInfo>3</owl:versionInfo>
<pav:hasCurrentVersion rdf:resource="http://vocab.nerc.ac.uk/collection/P35/current/EPC00061/3/"/>
<pav:version>3</pav:version>
<pav:authoredOn>2016-10-20 11:27:18.0</pav:authoredOn>
<skos:note xml:lang="en">accepted</skos:note>
<owl:deprecated>false</owl:deprecated>
<skos:narrower rdf:resource="http://vocab.nerc.ac.uk/collection/P01/current/RWS00043/"/>
<skos:related rdf:resource="http://vocab.nerc.ac.uk/collection/P06/current/UPNM/"/>
<skos:broader rdf:resource="http://vocab.nerc.ac.uk/collection/P36/current/HVYMTL/"/>
<void:inDataset rdf:resource="http://vocab.nerc.ac.uk/.well-known/void"/>
</skos:Concept>
</skos:member>
<skos:member>
<skos:Concept rdf:about="http://vocab.nerc.ac.uk/collection/P35/current/EPC00062/">
<dc:identifier>SDN:P35::EPC00062</dc:identifier>
<dce:identifier>SDN:P35::EPC00062</dce:identifier>
<dc:date>2016-10-20 11:27:18.0</dc:date>
<skos:notation>SDN:P35::EPC00062</skos:notation>
<skos:prefLabel xml:lang="en">Water body dissolved+particulate tin</skos:prefLabel>
<skos:altLabel>Dissolved+particulate Sn</skos:altLabel>
<skos:definition xml:lang="en">Concentration of the metal per unit volume of a river, estuary, sea or ocean by any method in unfiltered water.</skos:definition>
<owl:versionInfo>3</owl:versionInfo>
<pav:hasCurrentVersion rdf:resource="http://vocab.nerc.ac.uk/collection/P35/current/EPC00062/3/"/>
<pav:version>3</pav:version>
<pav:authoredOn>2016-10-20 11:27:18.0</pav:authoredOn>
<skos:note xml:lang="en">accepted</skos:note>
<owl:deprecated>false</owl:deprecated>
<skos:narrower rdf:resource="http://vocab.nerc.ac.uk/collection/P01/current/RWS00041/"/>
<skos:related rdf:resource="http://vocab.nerc.ac.uk/collection/P06/current/UPNM/"/>
<skos:broader rdf:resource="http://vocab.nerc.ac.uk/collection/P36/current/HVYMTL/"/>
<void:inDataset rdf:resource="http://vocab.nerc.ac.uk/.well-known/void"/>
</skos:Concept>
</skos:member>
<skos:member>
<skos:Concept rdf:about="http://vocab.nerc.ac.uk/collection/P35/current/EPC00063/">
<dc:identifier>SDN:P35::EPC00063</dc:identifier>
<dce:identifier>SDN:P35::EPC00063</dce:identifier>
<dc:date>2016-10-20 11:27:18.0</dc:date>
<skos:notation>SDN:P35::EPC00063</skos:notation>
<skos:prefLabel xml:lang="en">Water body dissolved+particulate titanium</skos:prefLabel>
<skos:altLabel>Dissolved+particulate Ti</skos:altLabel>
<skos:definition xml:lang="en">Concentration of the metal per unit volume of a river, estuary, sea or ocean by any method in unfiltered water.</skos:definition>
<owl:versionInfo>3</owl:versionInfo>
<pav:hasCurrentVersion rdf:resource="http://vocab.nerc.ac.uk/collection/P35/current/EPC00063/3/"/>
<pav:version>3</pav:version>
<pav:authoredOn>2016-10-20 11:27:18.0</pav:authoredOn>
<skos:note xml:lang="en">accepted</skos:note>
<owl:deprecated>false</owl:deprecated>
<skos:narrower rdf:resource="http://vocab.nerc.ac.uk/collection/P01/current/RWS00038/"/>
<skos:related rdf:resource="http://vocab.nerc.ac.uk/collection/P06/current/UPNM/"/>
<skos:broader rdf:resource="http://vocab.nerc.ac.uk/collection/P36/current/HVYMTL/"/>
<void:inDataset rdf:resource="http://vocab.nerc.ac.uk/.well-known/void"/>
</skos:Concept>
</skos:member>
<skos:member>
<skos:Concept rdf:about="http://vocab.nerc.ac.uk/collection/P35/current/EPC00064/">
<dc:identifier>SDN:P35::EPC00064</dc:identifier>
<dce:identifier>SDN:P35::EPC00064</dce:identifier>
<dc:date>2016-10-20 11:27:18.0</dc:date>
<skos:notation>SDN:P35::EPC00064</skos:notation>
<skos:prefLabel xml:lang="en">Water body dissolved+particulate uranium</skos:prefLabel>
<skos:altLabel>Dissolved+particulate U</skos:altLabel>
<skos:definition xml:lang="en">Concentration of the metal per unit volume of a river, estuary, sea or ocean by any method in unfiltered water.</skos:definition>
<owl:versionInfo>3</owl:versionInfo>
<pav:hasCurrentVersion rdf:resource="http://vocab.nerc.ac.uk/collection/P35/current/EPC00064/3/"/>
<pav:version>3</pav:version>
<pav:authoredOn>2016-10-20 11:27:18.0</pav:authoredOn>
<skos:note xml:lang="en">accepted</skos:note>
<owl:deprecated>false</owl:deprecated>
<skos:narrower rdf:resource="http://vocab.nerc.ac.uk/collection/P01/current/RWS00035/"/>
<skos:related rdf:resource="http://vocab.nerc.ac.uk/collection/P06/current/UPNM/"/>
<skos:broader rdf:resource="http://vocab.nerc.ac.uk/collection/P36/current/HVYMTL/"/>
<void:inDataset rdf:resource="http://vocab.nerc.ac.uk/.well-known/void"/>
</skos:Concept>
</skos:member>
<skos:member>
<skos:Concept rdf:about="http://vocab.nerc.ac.uk/collection/P35/current/EPC00065/">
<dc:identifier>SDN:P35::EPC00065</dc:identifier>
<dce:identifier>SDN:P35::EPC00065</dce:identifier>
<dc:date>2016-10-20 11:27:18.0</dc:date>
<skos:notation>SDN:P35::EPC00065</skos:notation>
<skos:prefLabel xml:lang="en">Water body dissolved+particulate vanadium</skos:prefLabel>
<skos:altLabel>Dissolved+particulate V</skos:altLabel>
<skos:definition xml:lang="en">Concentration of the metal per unit volume of a river, estuary, sea or ocean by any method in unfiltered water.</skos:definition>
<owl:versionInfo>3</owl:versionInfo>
<pav:hasCurrentVersion rdf:resource="http://vocab.nerc.ac.uk/collection/P35/current/EPC00065/3/"/>
<pav:version>3</pav:version>
<pav:authoredOn>2016-10-20 11:27:18.0</pav:authoredOn>
<skos:note xml:lang="en">accepted</skos:note>
<owl:deprecated>false</owl:deprecated>
<skos:narrower rdf:resource="http://vocab.nerc.ac.uk/collection/P01/current/RWS00042/"/>
<skos:related rdf:resource="http://vocab.nerc.ac.uk/collection/P06/current/UPNM/"/>
<skos:broader rdf:resource="http://vocab.nerc.ac.uk/collection/P36/current/HVYMTL/"/>
<void:inDataset rdf:resource="http://vocab.nerc.ac.uk/.well-known/void"/>
</skos:Concept>
</skos:member>
<skos:member>
<skos:Concept rdf:about="http://vocab.nerc.ac.uk/collection/P35/current/EPC00066/">
<dc:identifier>SDN:P35::EPC00066</dc:identifier>
<dce:identifier>SDN:P35::EPC00066</dce:identifier>
<dc:date>2016-10-20 11:27:18.0</dc:date>
<skos:notation>SDN:P35::EPC00066</skos:notation>
<skos:prefLabel xml:lang="en">Water body dissolved+particulate zinc</skos:prefLabel>
<skos:altLabel>Dissolved+particulate Zn</skos:altLabel>
<skos:definition xml:lang="en">Concentration of the metal per unit volume of a river, estuary, sea or ocean by any method in unfiltered water.</skos:definition>
<owl:versionInfo>3</owl:versionInfo>
<pav:hasCurrentVersion rdf:resource="http://vocab.nerc.ac.uk/collection/P35/current/EPC00066/3/"/>
<pav:version>3</pav:version>
<pav:authoredOn>2016-10-20 11:27:18.0</pav:authoredOn>
<skos:note xml:lang="en">accepted</skos:note>
<owl:deprecated>false</owl:deprecated>
<skos:narrower rdf:resource="http://vocab.nerc.ac.uk/collection/P01/current/RWS00028/"/>
<skos:narrower rdf:resource="http://vocab.nerc.ac.uk/collection/P01/current/ZNINCVDX/"/>
<skos:related rdf:resource="http://vocab.nerc.ac.uk/collection/P06/current/UPNM/"/>
<skos:broader rdf:resource="http://vocab.nerc.ac.uk/collection/P36/current/HVYMTL/"/>
<void:inDataset rdf:resource="http://vocab.nerc.ac.uk/.well-known/void"/>
</skos:Concept>
</skos:member>
<skos:member>
<skos:Concept rdf:about="http://vocab.nerc.ac.uk/collection/P35/current/EPC00213/">
<dc:identifier>SDN:P35::EPC00213</dc:identifier>
<dce:identifier>SDN:P35::EPC00213</dce:identifier>
<dc:date>2016-12-12 15:20:45.0</dc:date>
<skos:notation>SDN:P35::EPC00213</skos:notation>
<skos:prefLabel xml:lang="en">Water body fluoranthene</skos:prefLabel>
<skos:altLabel>Water body fluoranthene</skos:altLabel>
<skos:definition xml:lang="en">Concentration of fluoranthene (dissolved, reactive particulate or suspended particulate material) per unit volume of a river, estuary, sea or ocean by any method in filtered or unfiltered water.</skos:definition>
<owl:versionInfo>5</owl:versionInfo>
<pav:hasCurrentVersion rdf:resource="http://vocab.nerc.ac.uk/collection/P35/current/EPC00213/5/"/>
<pav:version>5</pav:version>
<pav:authoredOn>2016-12-12 15:20:45.0</pav:authoredOn>
<skos:note xml:lang="en">accepted</skos:note>
<owl:deprecated>false</owl:deprecated>
<skos:narrower rdf:resource="http://vocab.nerc.ac.uk/collection/P01/current/FLUFWC02/"/>
<skos:narrower rdf:resource="http://vocab.nerc.ac.uk/collection/P01/current/WTCTM015/"/>
<skos:narrower rdf:resource="http://vocab.nerc.ac.uk/collection/P01/current/AFLAGCD1/"/>
<skos:narrower rdf:resource="http://vocab.nerc.ac.uk/collection/P01/current/FLAFWC01/"/>
<skos:narrower rdf:resource="http://vocab.nerc.ac.uk/collection/P01/current/CPAHWC01/"/>
<skos:related rdf:resource="http://vocab.nerc.ac.uk/collection/P06/current/UGPL/"/>
<skos:broader rdf:resource="http://vocab.nerc.ac.uk/collection/P36/current/HCARBS/"/>
<void:inDataset rdf:resource="http://vocab.nerc.ac.uk/.well-known/void"/>
</skos:Concept>
</skos:member>
<skos:member>
<skos:Concept rdf:about="http://vocab.nerc.ac.uk/collection/P35/current/EPC00183/">
<dc:identifier>SDN:P35::EPC00183</dc:identifier>
<dce:identifier>SDN:P35::EPC00183</dce:identifier>
<dc:date>2016-12-12 15:20:45.0</dc:date>
<skos:notation>SDN:P35::EPC00183</skos:notation>
<skos:prefLabel xml:lang="en">Water body naphthalene</skos:prefLabel>
<skos:altLabel>Water body naphthalene</skos:altLabel>
<skos:definition xml:lang="en">Concentration of naphtalene (dissolved, reactive particulate or suspended particulate material) per unit volume of a river, estuary, sea or ocean by any method in filtered or unfiltered water.</skos:definition>
<owl:versionInfo>5</owl:versionInfo>
<pav:hasCurrentVersion rdf:resource="http://vocab.nerc.ac.uk/collection/P35/current/EPC00183/5/"/>
<pav:version>5</pav:version>
<pav:authoredOn>2016-12-12 15:20:45.0</pav:authoredOn>
<skos:note xml:lang="en">accepted</skos:note>
<owl:deprecated>false</owl:deprecated>
<skos:narrower rdf:resource="http://vocab.nerc.ac.uk/collection/P01/current/RWS00110/"/>
<skos:narrower rdf:resource="http://vocab.nerc.ac.uk/collection/P01/current/CPAHWC15/"/>
<skos:related rdf:resource="http://vocab.nerc.ac.uk/collection/P06/current/UGPL/"/>
<skos:broader rdf:resource="http://vocab.nerc.ac.uk/collection/P36/current/HCARBS/"/>
<void:inDataset rdf:resource="http://vocab.nerc.ac.uk/.well-known/void"/>
</skos:Concept>
</skos:member>
<skos:member>
<skos:Concept rdf:about="http://vocab.nerc.ac.uk/collection/P35/current/EPC00004/">
<dc:identifier>SDN:P35::EPC00004</dc:identifier>
<dce:identifier>SDN:P35::EPC00004</dce:identifier>
<dc:date>2016-10-20 11:27:18.0</dc:date>
<skos:notation>SDN:P35::EPC00004</skos:notation>
<skos:prefLabel xml:lang="en">Water body nitrate</skos:prefLabel>
<skos:altLabel>NO3</skos:altLabel>
<skos:definition xml:lang="en">Concentration of nitrate per unit volume of a river, estuary, sea or ocean by any method in filtered or unfiltered water.</skos:definition>
<owl:versionInfo>3</owl:versionInfo>
<pav:hasCurrentVersion rdf:resource="http://vocab.nerc.ac.uk/collection/P35/current/EPC00004/3/"/>
<pav:version>3</pav:version>
<pav:authoredOn>2016-10-20 11:27:18.0</pav:authoredOn>
<skos:note xml:lang="en">accepted</skos:note>
<owl:deprecated>false</owl:deprecated>
<skos:narrower rdf:resource="http://vocab.nerc.ac.uk/collection/P01/current/ODSDM2UM/"/>
<skos:narrower rdf:resource="http://vocab.nerc.ac.uk/collection/P01/current/ODSDM1UM/"/>
<skos:narrower rdf:resource="http://vocab.nerc.ac.uk/collection/P01/current/NTRTFSG1/"/>
<skos:narrower rdf:resource="http://vocab.nerc.ac.uk/collection/P01/current/ODSDM014/"/>
<skos:narrower rdf:resource="http://vocab.nerc.ac.uk/collection/P01/current/NO3FLTIC/"/>
<skos:narrower rdf:resource="http://vocab.nerc.ac.uk/collection/P01/current/NTRAYYDZ/"/>
<skos:narrower rdf:resource="http://vocab.nerc.ac.uk/collection/P01/current/CHEMM012/"/>
<skos:narrower rdf:resource="http://vocab.nerc.ac.uk/collection/P01/current/NTRAZZXX/"/>
<skos:narrower rdf:resource="http://vocab.nerc.ac.uk/collection/P01/current/NTRAAAD4/"/>
<skos:narrower rdf:resource="http://vocab.nerc.ac.uk/collection/P01/current/NTRAAAD1/"/>
<skos:narrower rdf:resource="http://vocab.nerc.ac.uk/collection/P01/current/NTRZMS01/"/>
<skos:narrower rdf:resource="http://vocab.nerc.ac.uk/collection/P01/current/NTRA04LW/"/>
<skos:narrower rdf:resource="http://vocab.nerc.ac.uk/collection/P01/current/MDMAP005/"/>
<skos:narrower rdf:resource="http://vocab.nerc.ac.uk/collection/P01/current/NO3UFLIC/"/>
<skos:narrower rdf:resource="http://vocab.nerc.ac.uk/collection/P01/current/NTRAAA04/"/>
<skos:narrower rdf:resource="http://vocab.nerc.ac.uk/collection/P01/current/NTRAXXDZ/"/>
<skos:narrower rdf:resource="http://vocab.nerc.ac.uk/collection/P01/current/NTRAMADZ/"/>
<skos:narrower rdf:resource="http://vocab.nerc.ac.uk/collection/P01/current/NTRZMC01/"/>
<skos:related rdf:resource="http://vocab.nerc.ac.uk/collection/P06/current/UPOX/"/>
<skos:broader rdf:resource="http://vocab.nerc.ac.uk/collection/P36/current/FERTIL/"/>
<void:inDataset rdf:resource="http://vocab.nerc.ac.uk/.well-known/void"/>
</skos:Concept>
</skos:member>
<skos:member>
<skos:Concept rdf:about="http://vocab.nerc.ac.uk/collection/P35/current/EPC00005/">
<dc:identifier>SDN:P35::EPC00005</dc:identifier>
<dce:identifier>SDN:P35::EPC00005</dce:identifier>
<dc:date>2016-10-20 11:27:18.0</dc:date>
<skos:notation>SDN:P35::EPC00005</skos:notation>
<skos:prefLabel xml:lang="en">Water body nitrate plus nitrite</skos:prefLabel>
<skos:altLabel>NO3+NO2</skos:altLabel>
<skos:definition xml:lang="en">Concentration of nitrate plus nitrite per unit volume of a river, estuary, sea or ocean by any method in filtered or unfiltered water.</skos:definition>
<owl:versionInfo>4</owl:versionInfo>
<pav:hasCurrentVersion rdf:resource="http://vocab.nerc.ac.uk/collection/P35/current/EPC00005/4/"/>
<pav:version>4</pav:version>
<pav:authoredOn>2016-10-20 11:27:18.0</pav:authoredOn>
<skos:note xml:lang="en">accepted</skos:note>
<owl:deprecated>false</owl:deprecated>
<skos:narrower rdf:resource="http://vocab.nerc.ac.uk/collection/P01/current/NTRZAAD5/"/>
<skos:narrower rdf:resource="http://vocab.nerc.ac.uk/collection/P01/current/NTRZAAD2/"/>
<skos:narrower rdf:resource="http://vocab.nerc.ac.uk/collection/P01/current/NTRZAAD3/"/>
<skos:narrower rdf:resource="http://vocab.nerc.ac.uk/collection/P01/current/NTRZMAD3/"/>
<skos:narrower rdf:resource="http://vocab.nerc.ac.uk/collection/P01/current/NTRZAAD1/"/>
<skos:narrower rdf:resource="http://vocab.nerc.ac.uk/collection/P01/current/NTRAFSG1/"/>
<skos:narrower rdf:resource="http://vocab.nerc.ac.uk/collection/P01/current/NTRZXXDZ/"/>
<skos:narrower rdf:resource="http://vocab.nerc.ac.uk/collection/P01/current/NTRZAADZ/"/>
<skos:narrower rdf:resource="http://vocab.nerc.ac.uk/collection/P01/current/NTRZMADZ/"/>
<skos:narrower rdf:resource="http://vocab.nerc.ac.uk/collection/P01/current/NTRZYYDZ/"/>
<skos:narrower rdf:resource="http://vocab.nerc.ac.uk/collection/P01/current/NTRZAATX/"/>
<skos:narrower rdf:resource="http://vocab.nerc.ac.uk/collection/P01/current/NTRZNS01/"/>
<skos:narrower rdf:resource="http://vocab.nerc.ac.uk/collection/P01/current/NTRZMATX/"/>
<skos:narrower rdf:resource="http://vocab.nerc.ac.uk/collection/P01/current/NTRZZZXX/"/>
<skos:narrower rdf:resource="http://vocab.nerc.ac.uk/collection/P01/current/NTRZAAZX/"/>
<skos:narrower rdf:resource="http://vocab.nerc.ac.uk/collection/P01/current/NTRZMAZX/"/>
<skos:narrower rdf:resource="http://vocab.nerc.ac.uk/collection/P01/current/MDMAP006/"/>
<skos:narrower rdf:resource="http://vocab.nerc.ac.uk/collection/P01/current/NTRAMS01/"/>
<skos:narrower rdf:resource="http://vocab.nerc.ac.uk/collection/P01/current/NTRZLWTX/"/>
<skos:narrower rdf:resource="http://vocab.nerc.ac.uk/collection/P01/current/NTRZAA01/"/>
<skos:narrower rdf:resource="http://vocab.nerc.ac.uk/collection/P01/current/NTRZNNTX/"/>
<skos:related rdf:resource="http://vocab.nerc.ac.uk/collection/P06/current/UPOX/"/>
<skos:broader rdf:resource="http://vocab.nerc.ac.uk/collection/P36/current/FERTIL/"/>
<void:inDataset rdf:resource="http://vocab.nerc.ac.uk/.well-known/void"/>
</skos:Concept>
</skos:member>
<skos:member>
<skos:Concept rdf:about="http://vocab.nerc.ac.uk/collection/P35/current/EPC00006/">
<dc:identifier>SDN:P35::EPC00006</dc:identifier>
<dce:identifier>SDN:P35::EPC00006</dce:identifier>
<dc:date>2016-10-20 11:27:18.0</dc:date>
<skos:notation>SDN:P35::EPC00006</skos:notation>
<skos:prefLabel xml:lang="en">Water body nitrite</skos:prefLabel>
<skos:altLabel>NO2</skos:altLabel>
<skos:definition xml:lang="en">Concentration of nitrite per unit volume of a river, estuary, sea or ocean by any method in filtered or unfiltered water.</skos:definition>
<owl:versionInfo>3</owl:versionInfo>
<pav:hasCurrentVersion rdf:resource="http://vocab.nerc.ac.uk/collection/P35/current/EPC00006/3/"/>
<pav:version>3</pav:version>
<pav:authoredOn>2016-10-20 11:27:18.0</pav:authoredOn>
<skos:note xml:lang="en">accepted</skos:note>
<owl:deprecated>false</owl:deprecated>
<skos:narrower rdf:resource="http://vocab.nerc.ac.uk/collection/P01/current/NTRIAAD5/"/>
<skos:narrower rdf:resource="http://vocab.nerc.ac.uk/collection/P01/current/NTRIAAD2/"/>
<skos:narrower rdf:resource="http://vocab.nerc.ac.uk/collection/P01/current/NTRIMA12/"/>
<skos:narrower rdf:resource="http://vocab.nerc.ac.uk/collection/P01/current/NTRIAAD1/"/>
<skos:narrower rdf:resource="http://vocab.nerc.ac.uk/collection/P01/current/NTRFSG01/"/>
<skos:narrower rdf:resource="http://vocab.nerc.ac.uk/collection/P01/current/NTRIAADZ/"/>
<skos:narrower rdf:resource="http://vocab.nerc.ac.uk/collection/P01/current/NTRIMADZ/"/>
<skos:narrower rdf:resource="http://vocab.nerc.ac.uk/collection/P01/current/NTRIYYDZ/"/>
<skos:narrower rdf:resource="http://vocab.nerc.ac.uk/collection/P01/current/NTRIAATX/"/>
<skos:narrower rdf:resource="http://vocab.nerc.ac.uk/collection/P01/current/NTRIMATX/"/>
<skos:narrower rdf:resource="http://vocab.nerc.ac.uk/collection/P01/current/NTRIZZXX/"/>
<skos:narrower rdf:resource="http://vocab.nerc.ac.uk/collection/P01/current/NTRI04LW/"/>
<skos:narrower rdf:resource="http://vocab.nerc.ac.uk/collection/P01/current/MDMAP007/"/>
<skos:narrower rdf:resource="http://vocab.nerc.ac.uk/collection/P01/current/NTRIKGD1/"/>
<skos:narrower rdf:resource="http://vocab.nerc.ac.uk/collection/P01/current/NTRILWTX/"/>
<skos:narrower rdf:resource="http://vocab.nerc.ac.uk/collection/P01/current/NTRIAAD4/"/>
<skos:narrower rdf:resource="http://vocab.nerc.ac.uk/collection/P01/current/NTRIAAD3/"/>
<skos:narrower rdf:resource="http://vocab.nerc.ac.uk/collection/P01/current/NTRIXXDZ/"/>
<skos:narrower rdf:resource="http://vocab.nerc.ac.uk/collection/P01/current/NO2FLTIC/"/>
<skos:narrower rdf:resource="http://vocab.nerc.ac.uk/collection/P01/current/NO2UFLIC/"/>
<skos:narrower rdf:resource="http://vocab.nerc.ac.uk/collection/P01/current/NTRIAAZX/"/>
<skos:related rdf:resource="http://vocab.nerc.ac.uk/collection/P06/current/UPOX/"/>
<skos:broader rdf:resource="http://vocab.nerc.ac.uk/collection/P36/current/FERTIL/"/>
<void:inDataset rdf:resource="http://vocab.nerc.ac.uk/.well-known/void"/>
</skos:Concept>
</skos:member>
<skos:member>
<skos:Concept rdf:about="http://vocab.nerc.ac.uk/collection/P35/current/EPC00159/">
<dc:identifier>SDN:P35::EPC00159</dc:identifier>
<dce:identifier>SDN:P35::EPC00159</dce:identifier>
<dc:date>2016-12-12 15:20:45.0</dc:date>
<skos:notation>SDN:P35::EPC00159</skos:notation>
<skos:prefLabel xml:lang="en">Water body organic nitrogen</skos:prefLabel>
<skos:altLabel>Water body organic nitrogen</skos:altLabel>
<skos:definition xml:lang="en">Concentration of organic nitrogen per unit volume of a river, estuary, sea or ocean by any method in filtered or unfiltered water.</skos:definition>
<owl:versionInfo>5</owl:versionInfo>
<pav:hasCurrentVersion rdf:resource="http://vocab.nerc.ac.uk/collection/P35/current/EPC00159/5/"/>
<pav:version>5</pav:version>
<pav:authoredOn>2016-12-12 15:20:45.0</pav:authoredOn>
<skos:note xml:lang="en">accepted</skos:note>
<owl:deprecated>false</owl:deprecated>
<skos:narrower rdf:resource="http://vocab.nerc.ac.uk/collection/P01/current/MDMAP009/"/>
<skos:narrower rdf:resource="http://vocab.nerc.ac.uk/collection/P01/current/MDMAP008/"/>
<skos:related rdf:resource="http://vocab.nerc.ac.uk/collection/P06/current/UPOX/"/>
<skos:broader rdf:resource="http://vocab.nerc.ac.uk/collection/P36/current/FERTIL/"/>
<void:inDataset rdf:resource="http://vocab.nerc.ac.uk/.well-known/void"/>
</skos:Concept>
</skos:member>
<skos:member>
<skos:Concept rdf:about="http://vocab.nerc.ac.uk/collection/P35/current/EPC00153/">
<dc:identifier>SDN:P35::EPC00153</dc:identifier>
<dce:identifier>SDN:P35::EPC00153</dce:identifier>
<dc:date>2016-12-12 15:20:45.0</dc:date>
<skos:notation>SDN:P35::EPC00153</skos:notation>
<skos:prefLabel xml:lang="en">Water body organic phosphorus</skos:prefLabel>
<skos:altLabel>Water body organic phosphorus</skos:altLabel>
<skos:definition xml:lang="en">Concentration of organic phosphorus per unit volume of river, estuary, sea or ocean by any method in filtered or unfiltered water.</skos:definition>
<owl:versionInfo>5</owl:versionInfo>
<pav:hasCurrentVersion rdf:resource="http://vocab.nerc.ac.uk/collection/P35/current/EPC00153/5/"/>
<pav:version>5</pav:version>
<pav:authoredOn>2016-12-12 15:20:45.0</pav:authoredOn>
<skos:note xml:lang="en">accepted</skos:note>
<owl:deprecated>false</owl:deprecated>
<skos:narrower rdf:resource="http://vocab.nerc.ac.uk/collection/P01/current/OPHSVLPT/"/>
<skos:narrower rdf:resource="http://vocab.nerc.ac.uk/collection/P01/current/ORGPDSZZ/"/>
<skos:related rdf:resource="http://vocab.nerc.ac.uk/collection/P06/current/UPOX/"/>
<skos:broader rdf:resource="http://vocab.nerc.ac.uk/collection/P36/current/FERTIL/"/>
<void:inDataset rdf:resource="http://vocab.nerc.ac.uk/.well-known/void"/>
</skos:Concept>
</skos:member>
<skos:member>
<skos:Concept rdf:about="http://vocab.nerc.ac.uk/collection/P35/current/EPC00226/">
<dc:identifier>SDN:P35::EPC00226</dc:identifier>
<dce:identifier>SDN:P35::EPC00226</dce:identifier>
<dc:date>2016-12-12 15:20:45.0</dc:date>
<skos:notation>SDN:P35::EPC00226</skos:notation>
<skos:prefLabel xml:lang="en">Water body p,p'-DDD</skos:prefLabel>
<skos:altLabel>Water body p,p'-DDD</skos:altLabel>
<skos:definition xml:lang="en">Concentration of p,p'-DDD per unit volume of a river, estuary, sea or ocean by any method in filtered or unfiltered water.</skos:definition>
<owl:versionInfo>2</owl:versionInfo>
<pav:hasCurrentVersion rdf:resource="http://vocab.nerc.ac.uk/collection/P35/current/EPC00226/2/"/>
<pav:version>2</pav:version>
<pav:authoredOn>2016-12-12 15:20:45.0</pav:authoredOn>
<skos:note xml:lang="en">accepted</skos:note>
<owl:deprecated>false</owl:deprecated>
<skos:narrower rdf:resource="http://vocab.nerc.ac.uk/collection/P01/current/RWS00049/"/>
<skos:narrower rdf:resource="http://vocab.nerc.ac.uk/collection/P01/current/TDEPPAF1/"/>
<skos:related rdf:resource="http://vocab.nerc.ac.uk/collection/P06/current/UGPL/"/>
<skos:broader rdf:resource="http://vocab.nerc.ac.uk/collection/P36/current/PESTBI/"/>
<void:inDataset rdf:resource="http://vocab.nerc.ac.uk/.well-known/void"/>
</skos:Concept>
</skos:member>
<skos:member>
<skos:Concept rdf:about="http://vocab.nerc.ac.uk/collection/P35/current/EPC00227/">
<dc:identifier>SDN:P35::EPC00227</dc:identifier>
<dce:identifier>SDN:P35::EPC00227</dce:identifier>
<dc:date>2016-12-12 15:20:45.0</dc:date>
<skos:notation>SDN:P35::EPC00227</skos:notation>
<skos:prefLabel xml:lang="en">Water body p,p'-DDE</skos:prefLabel>
<skos:altLabel>Water body p,p'-DDE</skos:altLabel>
<skos:definition xml:lang="en">Concentration of p,p'-DDE per unit volume of a river, estuary, sea or ocean by any method in filtered or unfiltered water.</skos:definition>
<owl:versionInfo>2</owl:versionInfo>
<pav:hasCurrentVersion rdf:resource="http://vocab.nerc.ac.uk/collection/P35/current/EPC00227/2/"/>
<pav:version>2</pav:version>
<pav:authoredOn>2016-12-12 15:20:45.0</pav:authoredOn>
<skos:note xml:lang="en">accepted</skos:note>
<owl:deprecated>false</owl:deprecated>
<skos:narrower rdf:resource="http://vocab.nerc.ac.uk/collection/P01/current/DDEPPAF1/"/>
<skos:narrower rdf:resource="http://vocab.nerc.ac.uk/collection/P01/current/RWS00050/"/>
<skos:related rdf:resource="http://vocab.nerc.ac.uk/collection/P06/current/UGPL/"/>
<skos:broader rdf:resource="http://vocab.nerc.ac.uk/collection/P36/current/PESTBI/"/>
<void:inDataset rdf:resource="http://vocab.nerc.ac.uk/.well-known/void"/>
</skos:Concept>
</skos:member>
<skos:member>
<skos:Concept rdf:about="http://vocab.nerc.ac.uk/collection/P35/current/EPC00225/">
<dc:identifier>SDN:P35::EPC00225</dc:identifier>
<dce:identifier>SDN:P35::EPC00225</dce:identifier>
<dc:date>2016-12-12 15:20:45.0</dc:date>
<skos:notation>SDN:P35::EPC00225</skos:notation>
<skos:prefLabel xml:lang="en">Water body p,p'-DDT</skos:prefLabel>
<skos:altLabel>Water body p,p'-DDT</skos:altLabel>
<skos:definition xml:lang="en">Concentration of p,p'-DDT per unit volume of a river, estuary, sea or ocean by any method in filtered or unfiltered water.</skos:definition>
<owl:versionInfo>2</owl:versionInfo>
<pav:hasCurrentVersion rdf:resource="http://vocab.nerc.ac.uk/collection/P35/current/EPC00225/2/"/>
<pav:version>2</pav:version>
<pav:authoredOn>2016-12-12 15:20:45.0</pav:authoredOn>
<skos:note xml:lang="en">accepted</skos:note>
<owl:deprecated>false</owl:deprecated>
<skos:narrower rdf:resource="http://vocab.nerc.ac.uk/collection/P01/current/DDTDISUF/"/>
<skos:narrower rdf:resource="http://vocab.nerc.ac.uk/collection/P01/current/PDDTUF02/"/>
<skos:narrower rdf:resource="http://vocab.nerc.ac.uk/collection/P01/current/WTCTM014/"/>
<skos:related rdf:resource="http://vocab.nerc.ac.uk/collection/P06/current/UGPL/"/>
<skos:broader rdf:resource="http://vocab.nerc.ac.uk/collection/P36/current/PESTBI/"/>
<void:inDataset rdf:resource="http://vocab.nerc.ac.uk/.well-known/void"/>
</skos:Concept>
</skos:member>
<skos:member>
<skos:Concept rdf:about="http://vocab.nerc.ac.uk/collection/P35/current/EPC00185/">
<dc:identifier>SDN:P35::EPC00185</dc:identifier>
<dce:identifier>SDN:P35::EPC00185</dce:identifier>
<dc:date>2016-12-12 15:20:45.0</dc:date>
<skos:notation>SDN:P35::EPC00185</skos:notation>
<skos:prefLabel xml:lang="en">Water body p,p'-DDT+DDD+DDE</skos:prefLabel>
<skos:altLabel>Water body p,p'-DDT+DDD+DDE</skos:altLabel>
<skos:definition xml:lang="en">Concentration of p,p'-DDT+DDD+DDE per unit volume of a river, estuary, sea or ocean by any method in filtered or unfiltered water.</skos:definition>
<owl:versionInfo>6</owl:versionInfo>
<pav:hasCurrentVersion rdf:resource="http://vocab.nerc.ac.uk/collection/P35/current/EPC00185/6/"/>
<pav:version>6</pav:version>
<pav:authoredOn>2016-12-12 15:20:45.0</pav:authoredOn>
<skos:note xml:lang="en">accepted</skos:note>
<owl:deprecated>false</owl:deprecated>
<skos:narrower rdf:resource="http://vocab.nerc.ac.uk/collection/P01/current/SCES0056/"/>
<skos:related rdf:resource="http://vocab.nerc.ac.uk/collection/P06/current/UGPL/"/>
<skos:broader rdf:resource="http://vocab.nerc.ac.uk/collection/P36/current/PESTBI/"/>
<void:inDataset rdf:resource="http://vocab.nerc.ac.uk/.well-known/void"/>
</skos:Concept>
</skos:member>
<skos:member>
<skos:Concept rdf:about="http://vocab.nerc.ac.uk/collection/P35/current/EPC00168/">
<dc:identifier>SDN:P35::EPC00168</dc:identifier>
<dce:identifier>SDN:P35::EPC00168</dce:identifier>
<dc:date>2016-12-12 15:20:45.0</dc:date>
<skos:notation>SDN:P35::EPC00168</skos:notation>
<skos:prefLabel xml:lang="en">Water body pH</skos:prefLabel>
<skos:altLabel>Water body pH</skos:altLabel>
<skos:definition xml:lang="en">Water body pH.</skos:definition>
<owl:versionInfo>5</owl:versionInfo>
<pav:hasCurrentVersion rdf:resource="http://vocab.nerc.ac.uk/collection/P35/current/EPC00168/5/"/>
<pav:version>5</pav:version>
<pav:authoredOn>2016-12-12 15:20:45.0</pav:authoredOn>
<skos:note xml:lang="en">accepted</skos:note>
<owl:deprecated>false</owl:deprecated>
<skos:narrower rdf:resource="http://vocab.nerc.ac.uk/collection/P01/current/ACIDZZXX/"/>
<skos:narrower rdf:resource="http://vocab.nerc.ac.uk/collection/P01/current/PHXXPR01/"/>
<skos:narrower rdf:resource="http://vocab.nerc.ac.uk/collection/P01/current/PHXXZZYY/"/>
<skos:narrower rdf:resource="http://vocab.nerc.ac.uk/collection/P01/current/PHMASSXX/"/>
<skos:narrower rdf:resource="http://vocab.nerc.ac.uk/collection/P01/current/PHXXZZXX/"/>
<skos:related rdf:resource="http://vocab.nerc.ac.uk/collection/P06/current/UUPH/"/>
<skos:broader rdf:resource="http://vocab.nerc.ac.uk/collection/P36/current/ACIDIT/"/>
<void:inDataset rdf:resource="http://vocab.nerc.ac.uk/.well-known/void"/>
</skos:Concept>
</skos:member>
<skos:member>
<skos:Concept rdf:about="http://vocab.nerc.ac.uk/collection/P35/current/EPC00067/">
<dc:identifier>SDN:P35::EPC00067</dc:identifier>
<dce:identifier>SDN:P35::EPC00067</dce:identifier>
<dc:date>2016-10-20 11:27:18.0</dc:date>
<skos:notation>SDN:P35::EPC00067</skos:notation>
<skos:prefLabel xml:lang="en">Water body particulate aluminium</skos:prefLabel>
<skos:altLabel>Particulate Al</skos:altLabel>
<skos:definition xml:lang="en">Concentration of the metal in particles extracted by filtration (any type of filter) in the water of a river, estuary, sea or ocean by any method and expressed per unit of water volume.</skos:definition>
<owl:versionInfo>3</owl:versionInfo>
<pav:hasCurrentVersion rdf:resource="http://vocab.nerc.ac.uk/collection/P35/current/EPC00067/3/"/>
<pav:version>3</pav:version>
<pav:authoredOn>2016-10-20 11:27:18.0</pav:authoredOn>
<skos:note xml:lang="en">accepted</skos:note>
<owl:deprecated>false</owl:deprecated>
<skos:narrower rdf:resource="http://vocab.nerc.ac.uk/collection/P01/current/ALPICP01/"/>
<skos:narrower rdf:resource="http://vocab.nerc.ac.uk/collection/P01/current/ALPSIN01/"/>
<skos:narrower rdf:resource="http://vocab.nerc.ac.uk/collection/P01/current/ALPSUS01/"/>
<skos:narrower rdf:resource="http://vocab.nerc.ac.uk/collection/P01/current/ALPTLMS1/"/>
<skos:narrower rdf:resource="http://vocab.nerc.ac.uk/collection/P01/current/ALXXAAP2/"/>
<skos:narrower rdf:resource="http://vocab.nerc.ac.uk/collection/P01/current/ALXXXFP2/"/>
<skos:narrower rdf:resource="http://vocab.nerc.ac.uk/collection/P01/current/ALXXICP2/"/>
<skos:related rdf:resource="http://vocab.nerc.ac.uk/collection/P06/current/UPNM/"/>
<skos:broader rdf:resource="http://vocab.nerc.ac.uk/collection/P36/current/HVYMTL/"/>
<void:inDataset rdf:resource="http://vocab.nerc.ac.uk/.well-known/void"/>
</skos:Concept>
</skos:member>
<skos:member>
<skos:Concept rdf:about="http://vocab.nerc.ac.uk/collection/P35/current/EPC00068/">
<dc:identifier>SDN:P35::EPC00068</dc:identifier>
<dce:identifier>SDN:P35::EPC00068</dce:identifier>
<dc:date>2016-10-20 11:27:18.0</dc:date>
<skos:notation>SDN:P35::EPC00068</skos:notation>
<skos:prefLabel xml:lang="en">Water body particulate barium</skos:prefLabel>
<skos:altLabel>Particulate Ba</skos:altLabel>
<skos:definition xml:lang="en">Concentration of the metal in particles extracted by filtration (any type of filter) in the water of a river, estuary, sea or ocean by any method and expressed per unit of water volume.</skos:definition>
<owl:versionInfo>3</owl:versionInfo>
<pav:hasCurrentVersion rdf:resource="http://vocab.nerc.ac.uk/collection/P35/current/EPC00068/3/"/>
<pav:version>3</pav:version>
<pav:authoredOn>2016-10-20 11:27:18.0</pav:authoredOn>
<skos:note xml:lang="en">accepted</skos:note>
<owl:deprecated>false</owl:deprecated>
<skos:narrower rdf:resource="http://vocab.nerc.ac.uk/collection/P01/current/BAXXXFP2/"/>
<skos:narrower rdf:resource="http://vocab.nerc.ac.uk/collection/P01/current/BAXXICP2/"/>
<skos:narrower rdf:resource="http://vocab.nerc.ac.uk/collection/P01/current/BAXXAAP2/"/>
<skos:narrower rdf:resource="http://vocab.nerc.ac.uk/collection/P01/current/BAXSPTMS/"/>
<skos:narrower rdf:resource="http://vocab.nerc.ac.uk/collection/P01/current/BAPSUS01/"/>
<skos:narrower rdf:resource="http://vocab.nerc.ac.uk/collection/P01/current/BAPICP01/"/>
<skos:narrower rdf:resource="http://vocab.nerc.ac.uk/collection/P01/current/BAPSIN01/"/>
<skos:related rdf:resource="http://vocab.nerc.ac.uk/collection/P06/current/UPNM/"/>
<skos:broader rdf:resource="http://vocab.nerc.ac.uk/collection/P36/current/HVYMTL/"/>
<void:inDataset rdf:resource="http://vocab.nerc.ac.uk/.well-known/void"/>
</skos:Concept>
</skos:member>
<skos:member>
<skos:Concept rdf:about="http://vocab.nerc.ac.uk/collection/P35/current/EPC00069/">
<dc:identifier>SDN:P35::EPC00069</dc:identifier>
<dce:identifier>SDN:P35::EPC00069</dce:identifier>
<dc:date>2016-10-20 11:27:18.0</dc:date>
<skos:notation>SDN:P35::EPC00069</skos:notation>
<skos:prefLabel xml:lang="en">Water body particulate cadmium</skos:prefLabel>
<skos:altLabel>Particulate Cd</skos:altLabel>
<skos:definition xml:lang="en">Concentration of the metal in particles extracted by filtration (any type of filter) in the water of a river, estuary, sea or ocean by any method and expressed per unit of water volume.</skos:definition>
<owl:versionInfo>3</owl:versionInfo>
<pav:hasCurrentVersion rdf:resource="http://vocab.nerc.ac.uk/collection/P35/current/EPC00069/3/"/>
<pav:version>3</pav:version>
<pav:authoredOn>2016-10-20 11:27:18.0</pav:authoredOn>
<skos:note xml:lang="en">accepted</skos:note>
<owl:deprecated>false</owl:deprecated>
<skos:narrower rdf:resource="http://vocab.nerc.ac.uk/collection/P01/current/CDXXAAP2/"/>
<skos:narrower rdf:resource="http://vocab.nerc.ac.uk/collection/P01/current/CDPSUS01/"/>
<skos:narrower rdf:resource="http://vocab.nerc.ac.uk/collection/P01/current/CDPSIN01/"/>
<skos:narrower rdf:resource="http://vocab.nerc.ac.uk/collection/P01/current/CDPICP01/"/>
<skos:narrower rdf:resource="http://vocab.nerc.ac.uk/collection/P01/current/CDXXICP2/"/>
<skos:related rdf:resource="http://vocab.nerc.ac.uk/collection/P06/current/UPNM/"/>
<skos:broader rdf:resource="http://vocab.nerc.ac.uk/collection/P36/current/HVYMTL/"/>
<void:inDataset rdf:resource="http://vocab.nerc.ac.uk/.well-known/void"/>
</skos:Concept>
</skos:member>
<skos:member>
<skos:Concept rdf:about="http://vocab.nerc.ac.uk/collection/P35/current/EPC00070/">
<dc:identifier>SDN:P35::EPC00070</dc:identifier>
<dce:identifier>SDN:P35::EPC00070</dce:identifier>
<dc:date>2016-10-20 11:27:18.0</dc:date>
<skos:notation>SDN:P35::EPC00070</skos:notation>
<skos:prefLabel xml:lang="en">Water body particulate chromium</skos:prefLabel>
<skos:altLabel>Particulate Cr</skos:altLabel>
<skos:definition xml:lang="en">Concentration of the metal in particles extracted by filtration (any type of filter) in the water of a river, estuary, sea or ocean by any method and expressed per unit of water volume.</skos:definition>
<owl:versionInfo>3</owl:versionInfo>
<pav:hasCurrentVersion rdf:resource="http://vocab.nerc.ac.uk/collection/P35/current/EPC00070/3/"/>
<pav:version>3</pav:version>
<pav:authoredOn>2016-10-20 11:27:18.0</pav:authoredOn>
<skos:note xml:lang="en">accepted</skos:note>
<owl:deprecated>false</owl:deprecated>
<skos:narrower rdf:resource="http://vocab.nerc.ac.uk/collection/P01/current/CRXXAAP2/"/>
<skos:related rdf:resource="http://vocab.nerc.ac.uk/collection/P06/current/UPNM/"/>
<skos:broader rdf:resource="http://vocab.nerc.ac.uk/collection/P36/current/HVYMTL/"/>
<void:inDataset rdf:resource="http://vocab.nerc.ac.uk/.well-known/void"/>
</skos:Concept>
</skos:member>
<skos:member>
<skos:Concept rdf:about="http://vocab.nerc.ac.uk/collection/P35/current/EPC00071/">
<dc:identifier>SDN:P35::EPC00071</dc:identifier>
<dce:identifier>SDN:P35::EPC00071</dce:identifier>
<dc:date>2016-10-20 11:27:18.0</dc:date>
<skos:notation>SDN:P35::EPC00071</skos:notation>
<skos:prefLabel xml:lang="en">Water body particulate cobalt</skos:prefLabel>
<skos:altLabel>Particulate Co</skos:altLabel>
<skos:definition xml:lang="en">Concentration of the metal in particles extracted by filtration (any type of filter) in the water of a river, estuary, sea or ocean by any method and expressed per unit of water volume.</skos:definition>
<owl:versionInfo>3</owl:versionInfo>
<pav:hasCurrentVersion rdf:resource="http://vocab.nerc.ac.uk/collection/P35/current/EPC00071/3/"/>
<pav:version>3</pav:version>
<pav:authoredOn>2016-10-20 11:27:18.0</pav:authoredOn>
<skos:note xml:lang="en">accepted</skos:note>
<owl:deprecated>false</owl:deprecated>
<skos:narrower rdf:resource="http://vocab.nerc.ac.uk/collection/P01/current/COXXAAP2/"/>
<skos:narrower rdf:resource="http://vocab.nerc.ac.uk/collection/P01/current/COPSIN01/"/>
<skos:narrower rdf:resource="http://vocab.nerc.ac.uk/collection/P01/current/COPICP01/"/>
<skos:narrower rdf:resource="http://vocab.nerc.ac.uk/collection/P01/current/COXXICP2/"/>
<skos:narrower rdf:resource="http://vocab.nerc.ac.uk/collection/P01/current/COPSUS01/"/>
<skos:related rdf:resource="http://vocab.nerc.ac.uk/collection/P06/current/UPNM/"/>
<skos:broader rdf:resource="http://vocab.nerc.ac.uk/collection/P36/current/HVYMTL/"/>
<void:inDataset rdf:resource="http://vocab.nerc.ac.uk/.well-known/void"/>
</skos:Concept>
</skos:member>
<skos:member>
<skos:Concept rdf:about="http://vocab.nerc.ac.uk/collection/P35/current/EPC00072/">
<dc:identifier>SDN:P35::EPC00072</dc:identifier>
<dce:identifier>SDN:P35::EPC00072</dce:identifier>
<dc:date>2016-10-20 11:27:18.0</dc:date>
<skos:notation>SDN:P35::EPC00072</skos:notation>
<skos:prefLabel xml:lang="en">Water body particulate copper</skos:prefLabel>
<skos:altLabel>Particulate Cu</skos:altLabel>
<skos:definition xml:lang="en">Concentration of the metal in particles extracted by filtration (any type of filter) in the water of a river, estuary, sea or ocean by any method and expressed per unit of water volume.</skos:definition>
<owl:versionInfo>3</owl:versionInfo>
<pav:hasCurrentVersion rdf:resource="http://vocab.nerc.ac.uk/collection/P35/current/EPC00072/3/"/>
<pav:version>3</pav:version>
<pav:authoredOn>2016-10-20 11:27:18.0</pav:authoredOn>
<skos:note xml:lang="en">accepted</skos:note>
<owl:deprecated>false</owl:deprecated>
<skos:narrower rdf:resource="http://vocab.nerc.ac.uk/collection/P01/current/CUPICP01/"/>
<skos:narrower rdf:resource="http://vocab.nerc.ac.uk/collection/P01/current/CUXXICP2/"/>
<skos:narrower rdf:resource="http://vocab.nerc.ac.uk/collection/P01/current/CUPSIN01/"/>
<skos:narrower rdf:resource="http://vocab.nerc.ac.uk/collection/P01/current/CUXXAAP2/"/>
<skos:narrower rdf:resource="http://vocab.nerc.ac.uk/collection/P01/current/CUPSUS01/"/>
<skos:related rdf:resource="http://vocab.nerc.ac.uk/collection/P06/current/UPNM/"/>
<skos:broader rdf:resource="http://vocab.nerc.ac.uk/collection/P36/current/HVYMTL/"/>
<void:inDataset rdf:resource="http://vocab.nerc.ac.uk/.well-known/void"/>
</skos:Concept>
</skos:member>
<skos:member>
<skos:Concept rdf:about="http://vocab.nerc.ac.uk/collection/P35/current/EPC00073/">
<dc:identifier>SDN:P35::EPC00073</dc:identifier>
<dce:identifier>SDN:P35::EPC00073</dce:identifier>
<dc:date>2016-10-20 11:27:18.0</dc:date>
<skos:notation>SDN:P35::EPC00073</skos:notation>
<skos:prefLabel xml:lang="en">Water body particulate iron (total chemical species)</skos:prefLabel>
<skos:altLabel>Particulate total Fe</skos:altLabel>
<skos:definition xml:lang="en">Concentration of the metal in particles extracted by filtration (any type of filter) in the water of a river, estuary, sea or ocean by any method and expressed per unit of water volume. Total means the element in all possible states of valency and chemical combination.</skos:definition>
<owl:versionInfo>3</owl:versionInfo>
<pav:hasCurrentVersion rdf:resource="http://vocab.nerc.ac.uk/collection/P35/current/EPC00073/3/"/>
<pav:version>3</pav:version>
<pav:authoredOn>2016-10-20 11:27:18.0</pav:authoredOn>
<skos:note xml:lang="en">accepted</skos:note>
<owl:deprecated>false</owl:deprecated>
<skos:narrower rdf:resource="http://vocab.nerc.ac.uk/collection/P01/current/FEXXICP2/"/>
<skos:narrower rdf:resource="http://vocab.nerc.ac.uk/collection/P01/current/FEPSIN01/"/>
<skos:narrower rdf:resource="http://vocab.nerc.ac.uk/collection/P01/current/FEXXAAP2/"/>
<skos:narrower rdf:resource="http://vocab.nerc.ac.uk/collection/P01/current/FEXXXFP2/"/>
<skos:narrower rdf:resource="http://vocab.nerc.ac.uk/collection/P01/current/FEPTLMS1/"/>
<skos:narrower rdf:resource="http://vocab.nerc.ac.uk/collection/P01/current/FEPSUS01/"/>
<skos:narrower rdf:resource="http://vocab.nerc.ac.uk/collection/P01/current/FEPICP01/"/>
<skos:related rdf:resource="http://vocab.nerc.ac.uk/collection/P06/current/UPNM/"/>
<skos:broader rdf:resource="http://vocab.nerc.ac.uk/collection/P36/current/HVYMTL/"/>
<void:inDataset rdf:resource="http://vocab.nerc.ac.uk/.well-known/void"/>
</skos:Concept>
</skos:member>
<skos:member>
<skos:Concept rdf:about="http://vocab.nerc.ac.uk/collection/P35/current/EPC00074/">
<dc:identifier>SDN:P35::EPC00074</dc:identifier>
<dce:identifier>SDN:P35::EPC00074</dce:identifier>
<dc:date>2016-10-20 11:27:18.0</dc:date>
<skos:notation>SDN:P35::EPC00074</skos:notation>
<skos:prefLabel xml:lang="en">Water body particulate lead</skos:prefLabel>
<skos:altLabel>Particulate Pb</skos:altLabel>
<skos:definition xml:lang="en">Concentration of the metal in particles extracted by filtration (any type of filter) in the water of a river, estuary, sea or ocean by any method and expressed per unit of water volume.</skos:definition>
<owl:versionInfo>3</owl:versionInfo>
<pav:hasCurrentVersion rdf:resource="http://vocab.nerc.ac.uk/collection/P35/current/EPC00074/3/"/>
<pav:version>3</pav:version>
<pav:authoredOn>2016-10-20 11:27:18.0</pav:authoredOn>
<skos:note xml:lang="en">accepted</skos:note>
<owl:deprecated>false</owl:deprecated>
<skos:narrower rdf:resource="http://vocab.nerc.ac.uk/collection/P01/current/PBPSIN01/"/>
<skos:narrower rdf:resource="http://vocab.nerc.ac.uk/collection/P01/current/PBPICP01/"/>
<skos:narrower rdf:resource="http://vocab.nerc.ac.uk/collection/P01/current/PBXXICP2/"/>
<skos:narrower rdf:resource="http://vocab.nerc.ac.uk/collection/P01/current/PBPSUS01/"/>
<skos:narrower rdf:resource="http://vocab.nerc.ac.uk/collection/P01/current/PBXXAAP2/"/>
<skos:related rdf:resource="http://vocab.nerc.ac.uk/collection/P06/current/UPNM/"/>
<skos:broader rdf:resource="http://vocab.nerc.ac.uk/collection/P36/current/HVYMTL/"/>
<void:inDataset rdf:resource="http://vocab.nerc.ac.uk/.well-known/void"/>
</skos:Concept>
</skos:member>
<skos:member>
<skos:Concept rdf:about="http://vocab.nerc.ac.uk/collection/P35/current/EPC00075/">
<dc:identifier>SDN:P35::EPC00075</dc:identifier>
<dce:identifier>SDN:P35::EPC00075</dce:identifier>
<dc:date>2016-10-20 11:27:18.0</dc:date>
<skos:notation>SDN:P35::EPC00075</skos:notation>
<skos:prefLabel xml:lang="en">Water body particulate manganese (total chemical species)</skos:prefLabel>
<skos:altLabel>Particulate total Mn</skos:altLabel>
<skos:definition xml:lang="en">Concentration of the metal in particles extracted by filtration (any type of filter) in the water of a river, estuary, sea or ocean by any method and expressed per unit of water volume. Total means the element in all possible states of valency and chemical combination.</skos:definition>
<owl:versionInfo>3</owl:versionInfo>
<pav:hasCurrentVersion rdf:resource="http://vocab.nerc.ac.uk/collection/P35/current/EPC00075/3/"/>
<pav:version>3</pav:version>
<pav:authoredOn>2016-10-20 11:27:18.0</pav:authoredOn>
<skos:note xml:lang="en">accepted</skos:note>
<owl:deprecated>false</owl:deprecated>
<skos:narrower rdf:resource="http://vocab.nerc.ac.uk/collection/P01/current/MNPICP01/"/>
<skos:narrower rdf:resource="http://vocab.nerc.ac.uk/collection/P01/current/MNXXAAP2/"/>
<skos:narrower rdf:resource="http://vocab.nerc.ac.uk/collection/P01/current/MNXXICP2/"/>
<skos:narrower rdf:resource="http://vocab.nerc.ac.uk/collection/P01/current/MNPSIN01/"/>
<skos:narrower rdf:resource="http://vocab.nerc.ac.uk/collection/P01/current/MNXXXFP2/"/>
<skos:narrower rdf:resource="http://vocab.nerc.ac.uk/collection/P01/current/MNPSUS01/"/>
<skos:related rdf:resource="http://vocab.nerc.ac.uk/collection/P06/current/UPNM/"/>
<skos:broader rdf:resource="http://vocab.nerc.ac.uk/collection/P36/current/HVYMTL/"/>
<void:inDataset rdf:resource="http://vocab.nerc.ac.uk/.well-known/void"/>
</skos:Concept>
</skos:member>
<skos:member>
<skos:Concept rdf:about="http://vocab.nerc.ac.uk/collection/P35/current/EPC00076/">
<dc:identifier>SDN:P35::EPC00076</dc:identifier>
<dce:identifier>SDN:P35::EPC00076</dce:identifier>
<dc:date>2016-10-20 11:27:18.0</dc:date>
<skos:notation>SDN:P35::EPC00076</skos:notation>
<skos:prefLabel xml:lang="en">Water body particulate molybdenum</skos:prefLabel>
<skos:altLabel>Particulate Mo</skos:altLabel>
<skos:definition xml:lang="en">Concentration of the metal in particles extracted by filtration (any type of filter) in the water of a river, estuary, sea or ocean by any method and expressed per unit of water volume.</skos:definition>
<owl:versionInfo>3</owl:versionInfo>
<pav:hasCurrentVersion rdf:resource="http://vocab.nerc.ac.uk/collection/P35/current/EPC00076/3/"/>
<pav:version>3</pav:version>
<pav:authoredOn>2016-10-20 11:27:18.0</pav:authoredOn>
<skos:note xml:lang="en">accepted</skos:note>
<owl:deprecated>false</owl:deprecated>
<skos:narrower rdf:resource="http://vocab.nerc.ac.uk/collection/P01/current/MOXXXXP2/"/>
<skos:narrower rdf:resource="http://vocab.nerc.ac.uk/collection/P01/current/MOPICP01/"/>
<skos:related rdf:resource="http://vocab.nerc.ac.uk/collection/P06/current/UPNM/"/>
<skos:broader rdf:resource="http://vocab.nerc.ac.uk/collection/P36/current/HVYMTL/"/>
<void:inDataset rdf:resource="http://vocab.nerc.ac.uk/.well-known/void"/>
</skos:Concept>
</skos:member>
<skos:member>
<skos:Concept rdf:about="http://vocab.nerc.ac.uk/collection/P35/current/EPC00077/">
<dc:identifier>SDN:P35::EPC00077</dc:identifier>
<dce:identifier>SDN:P35::EPC00077</dce:identifier>
<dc:date>2016-10-20 11:27:18.0</dc:date>
<skos:notation>SDN:P35::EPC00077</skos:notation>
<skos:prefLabel xml:lang="en">Water body particulate nickel</skos:prefLabel>
<skos:altLabel>Particulate Ni</skos:altLabel>
<skos:definition xml:lang="en">Concentration of the metal in particles extracted by filtration (any type of filter) in the water of a river, estuary, sea or ocean by any method and expressed per unit of water volume.</skos:definition>
<owl:versionInfo>3</owl:versionInfo>
<pav:hasCurrentVersion rdf:resource="http://vocab.nerc.ac.uk/collection/P35/current/EPC00077/3/"/>
<pav:version>3</pav:version>
<pav:authoredOn>2016-10-20 11:27:18.0</pav:authoredOn>
<skos:note xml:lang="en">accepted</skos:note>
<owl:deprecated>false</owl:deprecated>
<skos:narrower rdf:resource="http://vocab.nerc.ac.uk/collection/P01/current/NIPSIN01/"/>
<skos:narrower rdf:resource="http://vocab.nerc.ac.uk/collection/P01/current/NIXXAAP2/"/>
<skos:narrower rdf:resource="http://vocab.nerc.ac.uk/collection/P01/current/NIXXICP2/"/>
<skos:narrower rdf:resource="http://vocab.nerc.ac.uk/collection/P01/current/NIPSUS01/"/>
<skos:narrower rdf:resource="http://vocab.nerc.ac.uk/collection/P01/current/NIPICP01/"/>
<skos:related rdf:resource="http://vocab.nerc.ac.uk/collection/P06/current/UPNM/"/>
<skos:broader rdf:resource="http://vocab.nerc.ac.uk/collection/P36/current/HVYMTL/"/>
<void:inDataset rdf:resource="http://vocab.nerc.ac.uk/.well-known/void"/>
</skos:Concept>
</skos:member>
<skos:member>
<skos:Concept rdf:about="http://vocab.nerc.ac.uk/collection/P35/current/EPC00212/">
<dc:identifier>SDN:P35::EPC00212</dc:identifier>
<dce:identifier>SDN:P35::EPC00212</dce:identifier>
<dc:date>2016-12-12 15:20:45.0</dc:date>
<skos:notation>SDN:P35::EPC00212</skos:notation>
<skos:prefLabel xml:lang="en">Water body particulate nitrogen</skos:prefLabel>
<skos:altLabel>Water body particulate nitrogen</skos:altLabel>
<skos:definition xml:lang="en">Concentration of nitrogen in suspended particulate matter (regardless of filter porosity) per unit volume of a river, estuary, sea or ocean by any method in filtered water.</skos:definition>
<owl:versionInfo>5</owl:versionInfo>
<pav:hasCurrentVersion rdf:resource="http://vocab.nerc.ac.uk/collection/P35/current/EPC00212/5/"/>
<pav:version>5</pav:version>
<pav:authoredOn>2016-12-12 15:20:45.0</pav:authoredOn>
<skos:note xml:lang="en">accepted</skos:note>
<owl:deprecated>false</owl:deprecated>
<skos:narrower rdf:resource="http://vocab.nerc.ac.uk/collection/P01/current/NTOTCAP1/"/>
<skos:narrower rdf:resource="http://vocab.nerc.ac.uk/collection/P01/current/NTOTZZZZ/"/>
<skos:narrower rdf:resource="http://vocab.nerc.ac.uk/collection/P01/current/ODSDM018/"/>
<skos:narrower rdf:resource="http://vocab.nerc.ac.uk/collection/P01/current/NTOTCN10/"/>
<skos:narrower rdf:resource="http://vocab.nerc.ac.uk/collection/P01/current/TNCNCNP1/"/>
<skos:narrower rdf:resource="http://vocab.nerc.ac.uk/collection/P01/current/MDMAP013/"/>
<skos:related rdf:resource="http://vocab.nerc.ac.uk/collection/P06/current/UPOX/"/>
<skos:broader rdf:resource="http://vocab.nerc.ac.uk/collection/P36/current/FERTIL/"/>
<void:inDataset rdf:resource="http://vocab.nerc.ac.uk/.well-known/void"/>
</skos:Concept>
</skos:member>
<skos:member>
<skos:Concept rdf:about="http://vocab.nerc.ac.uk/collection/P35/current/EPC00157/">
<dc:identifier>SDN:P35::EPC00157</dc:identifier>
<dce:identifier>SDN:P35::EPC00157</dce:identifier>
<dc:date>2016-12-12 15:20:45.0</dc:date>
<skos:notation>SDN:P35::EPC00157</skos:notation>
<skos:prefLabel xml:lang="en">Water body particulate organic carbon {POC}</skos:prefLabel>
<skos:altLabel>Water body particulate organic carbon {POC}</skos:altLabel>
<skos:definition xml:lang="en">Concentration of organic carbon in suspended particulate matter (regardless of filter porosity) in river, estuary, sea or ocean.</skos:definition>
<owl:versionInfo>5</owl:versionInfo>
<pav:hasCurrentVersion rdf:resource="http://vocab.nerc.ac.uk/collection/P35/current/EPC00157/5/"/>
<pav:version>5</pav:version>
<pav:authoredOn>2016-12-12 15:20:45.0</pav:authoredOn>
<skos:note xml:lang="en">accepted</skos:note>
<owl:deprecated>false</owl:deprecated>
<skos:narrower rdf:resource="http://vocab.nerc.ac.uk/collection/P01/current/OCCNGCPZ/"/>
<skos:narrower rdf:resource="http://vocab.nerc.ac.uk/collection/P01/current/OCCNCAP1/"/>
<skos:narrower rdf:resource="http://vocab.nerc.ac.uk/collection/P01/current/CORGCA53/"/>
<skos:narrower rdf:resource="http://vocab.nerc.ac.uk/collection/P01/current/CHEMM017/"/>
<skos:narrower rdf:resource="http://vocab.nerc.ac.uk/collection/P01/current/MDMAP010/"/>
<skos:narrower rdf:resource="http://vocab.nerc.ac.uk/collection/P01/current/CORGCAP1/"/>
<skos:related rdf:resource="http://vocab.nerc.ac.uk/collection/P06/current/UPOX/"/>
<skos:broader rdf:resource="http://vocab.nerc.ac.uk/collection/P36/current/ORGMAT/"/>
<void:inDataset rdf:resource="http://vocab.nerc.ac.uk/.well-known/void"/>
</skos:Concept>
</skos:member>
<skos:member>
<skos:Concept rdf:about="http://vocab.nerc.ac.uk/collection/P35/current/EPC00201/">
<dc:identifier>SDN:P35::EPC00201</dc:identifier>
<dce:identifier>SDN:P35::EPC00201</dce:identifier>
<dc:date>2016-12-12 15:20:45.0</dc:date>
<skos:notation>SDN:P35::EPC00201</skos:notation>
<skos:prefLabel xml:lang="en">Water body particulate phosphorus</skos:prefLabel>
<skos:altLabel>Water body particulate phosphorus</skos:altLabel>
<skos:definition xml:lang="en">Concentration of phosphorus in suspended particulate matter (regardless of filter porosity) per unit volume of a river, estuary, sea or ocean by any method in filtered water.</skos:definition>
<owl:versionInfo>5</owl:versionInfo>
<pav:hasCurrentVersion rdf:resource="http://vocab.nerc.ac.uk/collection/P35/current/EPC00201/5/"/>
<pav:version>5</pav:version>
<pav:authoredOn>2016-12-12 15:20:45.0</pav:authoredOn>
<skos:note xml:lang="en">accepted</skos:note>
<owl:deprecated>false</owl:deprecated>
<skos:narrower rdf:resource="http://vocab.nerc.ac.uk/collection/P01/current/TPHSVLPT/"/>
<skos:narrower rdf:resource="http://vocab.nerc.ac.uk/collection/P01/current/TPHSWCPZ/"/>
<skos:related rdf:resource="http://vocab.nerc.ac.uk/collection/P06/current/UPOX/"/>
<skos:broader rdf:resource="http://vocab.nerc.ac.uk/collection/P36/current/FERTIL/"/>
<void:inDataset rdf:resource="http://vocab.nerc.ac.uk/.well-known/void"/>
</skos:Concept>
</skos:member>
<skos:member>
<skos:Concept rdf:about="http://vocab.nerc.ac.uk/collection/P35/current/EPC00078/">
<dc:identifier>SDN:P35::EPC00078</dc:identifier>
<dce:identifier>SDN:P35::EPC00078</dce:identifier>
<dc:date>2016-10-20 11:27:18.0</dc:date>
<skos:notation>SDN:P35::EPC00078</skos:notation>
<skos:prefLabel xml:lang="en">Water body particulate silver</skos:prefLabel>
<skos:altLabel>Particulate Ag</skos:altLabel>
<skos:definition xml:lang="en">Concentration of the metal in particles extracted by filtration (any type of filter) in the water of a river, estuary, sea or ocean by any method and expressed per unit of water volume.</skos:definition>
<owl:versionInfo>3</owl:versionInfo>
<pav:hasCurrentVersion rdf:resource="http://vocab.nerc.ac.uk/collection/P35/current/EPC00078/3/"/>
<pav:version>3</pav:version>
<pav:authoredOn>2016-10-20 11:27:18.0</pav:authoredOn>
<skos:note xml:lang="en">accepted</skos:note>
<owl:deprecated>false</owl:deprecated>
<skos:narrower rdf:resource="http://vocab.nerc.ac.uk/collection/P01/current/AGXXICP2/"/>
<skos:narrower rdf:resource="http://vocab.nerc.ac.uk/collection/P01/current/AGXXAAP2/"/>
<skos:narrower rdf:resource="http://vocab.nerc.ac.uk/collection/P01/current/AGPSIN01/"/>
<skos:narrower rdf:resource="http://vocab.nerc.ac.uk/collection/P01/current/AGPICP01/"/>
<skos:narrower rdf:resource="http://vocab.nerc.ac.uk/collection/P01/current/AGPSUS01/"/>
<skos:related rdf:resource="http://vocab.nerc.ac.uk/collection/P06/current/UPNM/"/>
<skos:broader rdf:resource="http://vocab.nerc.ac.uk/collection/P36/current/HVYMTL/"/>
<void:inDataset rdf:resource="http://vocab.nerc.ac.uk/.well-known/void"/>
</skos:Concept>
</skos:member>
<skos:member>
<skos:Concept rdf:about="http://vocab.nerc.ac.uk/collection/P35/current/EPC00079/">
<dc:identifier>SDN:P35::EPC00079</dc:identifier>
<dce:identifier>SDN:P35::EPC00079</dce:identifier>
<dc:date>2016-10-20 11:27:18.0</dc:date>
<skos:notation>SDN:P35::EPC00079</skos:notation>
<skos:prefLabel xml:lang="en">Water body particulate strontium</skos:prefLabel>
<skos:altLabel>Particulate Sr</skos:altLabel>
<skos:definition xml:lang="en">Concentration of the metal in particles extracted by filtration (any type of filter) in the water of a river, estuary, sea or ocean by any method and expressed per unit of water volume.</skos:definition>
<owl:versionInfo>3</owl:versionInfo>
<pav:hasCurrentVersion rdf:resource="http://vocab.nerc.ac.uk/collection/P35/current/EPC00079/3/"/>
<pav:version>3</pav:version>
<pav:authoredOn>2016-10-20 11:27:18.0</pav:authoredOn>
<skos:note xml:lang="en">accepted</skos:note>
<owl:deprecated>false</owl:deprecated>
<skos:narrower rdf:resource="http://vocab.nerc.ac.uk/collection/P01/current/SRXXAAP2/"/>
<skos:narrower rdf:resource="http://vocab.nerc.ac.uk/collection/P01/current/SRXXICP2/"/>
<skos:related rdf:resource="http://vocab.nerc.ac.uk/collection/P06/current/UPNM/"/>
<skos:broader rdf:resource="http://vocab.nerc.ac.uk/collection/P36/current/HVYMTL/"/>
<void:inDataset rdf:resource="http://vocab.nerc.ac.uk/.well-known/void"/>
</skos:Concept>
</skos:member>
<skos:member>
<skos:Concept rdf:about="http://vocab.nerc.ac.uk/collection/P35/current/EPC00080/">
<dc:identifier>SDN:P35::EPC00080</dc:identifier>
<dce:identifier>SDN:P35::EPC00080</dce:identifier>
<dc:date>2016-10-20 11:27:18.0</dc:date>
<skos:notation>SDN:P35::EPC00080</skos:notation>
<skos:prefLabel xml:lang="en">Water body particulate titanium</skos:prefLabel>
<skos:altLabel>Particulate Ti</skos:altLabel>
<skos:definition xml:lang="en">Concentration of the metal in particles extracted by filtration (any type of filter) in the water of a river, estuary, sea or ocean by any method and expressed per unit of water volume.</skos:definition>
<owl:versionInfo>3</owl:versionInfo>
<pav:hasCurrentVersion rdf:resource="http://vocab.nerc.ac.uk/collection/P35/current/EPC00080/3/"/>
<pav:version>3</pav:version>
<pav:authoredOn>2016-10-20 11:27:18.0</pav:authoredOn>
<skos:note xml:lang="en">accepted</skos:note>
<owl:deprecated>false</owl:deprecated>
<skos:narrower rdf:resource="http://vocab.nerc.ac.uk/collection/P01/current/TIXXXFP2/"/>
<skos:narrower rdf:resource="http://vocab.nerc.ac.uk/collection/P01/current/TIPSUS01/"/>
<skos:narrower rdf:resource="http://vocab.nerc.ac.uk/collection/P01/current/TIPSIN01/"/>
<skos:narrower rdf:resource="http://vocab.nerc.ac.uk/collection/P01/current/TIPICP01/"/>
<skos:related rdf:resource="http://vocab.nerc.ac.uk/collection/P06/current/UPNM/"/>
<skos:broader rdf:resource="http://vocab.nerc.ac.uk/collection/P36/current/HVYMTL/"/>
<void:inDataset rdf:resource="http://vocab.nerc.ac.uk/.well-known/void"/>
</skos:Concept>
</skos:member>
<skos:member>
<skos:Concept rdf:about="http://vocab.nerc.ac.uk/collection/P35/current/EPC00081/">
<dc:identifier>SDN:P35::EPC00081</dc:identifier>
<dce:identifier>SDN:P35::EPC00081</dce:identifier>
<dc:date>2016-10-20 11:27:18.0</dc:date>
<skos:notation>SDN:P35::EPC00081</skos:notation>
<skos:prefLabel xml:lang="en">Water body particulate uranium</skos:prefLabel>
<skos:altLabel>Particulate U</skos:altLabel>
<skos:definition xml:lang="en">Concentration of the metal in particles extracted by filtration (any type of filter) in the water of a river, estuary, sea or ocean by any method and expressed per unit of water volume.</skos:definition>
<owl:versionInfo>3</owl:versionInfo>
<pav:hasCurrentVersion rdf:resource="http://vocab.nerc.ac.uk/collection/P35/current/EPC00081/3/"/>
<pav:version>3</pav:version>
<pav:authoredOn>2016-10-20 11:27:18.0</pav:authoredOn>
<skos:note xml:lang="en">accepted</skos:note>
<owl:deprecated>false</owl:deprecated>
<skos:narrower rdf:resource="http://vocab.nerc.ac.uk/collection/P01/current/URPICP01/"/>
<skos:related rdf:resource="http://vocab.nerc.ac.uk/collection/P06/current/UPNM/"/>
<skos:broader rdf:resource="http://vocab.nerc.ac.uk/collection/P36/current/HVYMTL/"/>
<void:inDataset rdf:resource="http://vocab.nerc.ac.uk/.well-known/void"/>
</skos:Concept>
</skos:member>
<skos:member>
<skos:Concept rdf:about="http://vocab.nerc.ac.uk/collection/P35/current/EPC00082/">
<dc:identifier>SDN:P35::EPC00082</dc:identifier>
<dce:identifier>SDN:P35::EPC00082</dce:identifier>
<dc:date>2016-10-20 11:27:18.0</dc:date>
<skos:notation>SDN:P35::EPC00082</skos:notation>
<skos:prefLabel xml:lang="en">Water body particulate vanadium</skos:prefLabel>
<skos:altLabel>Particulate V</skos:altLabel>
<skos:definition xml:lang="en">Concentration of the metal in particles extracted by filtration (any type of filter) in the water of a river, estuary, sea or ocean by any method and expressed per unit of water volume.</skos:definition>
<owl:versionInfo>3</owl:versionInfo>
<pav:hasCurrentVersion rdf:resource="http://vocab.nerc.ac.uk/collection/P35/current/EPC00082/3/"/>
<pav:version>3</pav:version>
<pav:authoredOn>2016-10-20 11:27:18.0</pav:authoredOn>
<skos:note xml:lang="en">accepted</skos:note>
<owl:deprecated>false</owl:deprecated>
<skos:narrower rdf:resource="http://vocab.nerc.ac.uk/collection/P01/current/VAPICP01/"/>
<skos:narrower rdf:resource="http://vocab.nerc.ac.uk/collection/P01/current/VAPSIN01/"/>
<skos:narrower rdf:resource="http://vocab.nerc.ac.uk/collection/P01/current/VAPSUS01/"/>
<skos:related rdf:resource="http://vocab.nerc.ac.uk/collection/P06/current/UPNM/"/>
<skos:broader rdf:resource="http://vocab.nerc.ac.uk/collection/P36/current/HVYMTL/"/>
<void:inDataset rdf:resource="http://vocab.nerc.ac.uk/.well-known/void"/>
</skos:Concept>
</skos:member>
<skos:member>
<skos:Concept rdf:about="http://vocab.nerc.ac.uk/collection/P35/current/EPC00083/">
<dc:identifier>SDN:P35::EPC00083</dc:identifier>
<dce:identifier>SDN:P35::EPC00083</dce:identifier>
<dc:date>2016-10-20 11:27:18.0</dc:date>
<skos:notation>SDN:P35::EPC00083</skos:notation>
<skos:prefLabel xml:lang="en">Water body particulate zinc</skos:prefLabel>
<skos:altLabel>Particulate Zn</skos:altLabel>
<skos:definition xml:lang="en">Concentration of the metal in particles extracted by filtration (any type of filter) in the water of a river, estuary, sea or ocean by any method and expressed per unit of water volume.</skos:definition>
<owl:versionInfo>3</owl:versionInfo>
<pav:hasCurrentVersion rdf:resource="http://vocab.nerc.ac.uk/collection/P35/current/EPC00083/3/"/>
<pav:version>3</pav:version>
<pav:authoredOn>2016-10-20 11:27:18.0</pav:authoredOn>
<skos:note xml:lang="en">accepted</skos:note>
<owl:deprecated>false</owl:deprecated>
<skos:narrower rdf:resource="http://vocab.nerc.ac.uk/collection/P01/current/ZNXXAAP2/"/>
<skos:narrower rdf:resource="http://vocab.nerc.ac.uk/collection/P01/current/ZNPSUS01/"/>
<skos:narrower rdf:resource="http://vocab.nerc.ac.uk/collection/P01/current/ZNPICP01/"/>
<skos:narrower rdf:resource="http://vocab.nerc.ac.uk/collection/P01/current/ZNPSIN01/"/>
<skos:narrower rdf:resource="http://vocab.nerc.ac.uk/collection/P01/current/ZNXXICP2/"/>
<skos:related rdf:resource="http://vocab.nerc.ac.uk/collection/P06/current/UPNM/"/>
<skos:broader rdf:resource="http://vocab.nerc.ac.uk/collection/P36/current/HVYMTL/"/>
<void:inDataset rdf:resource="http://vocab.nerc.ac.uk/.well-known/void"/>
</skos:Concept>
</skos:member>
<skos:member>
<skos:Concept rdf:about="http://vocab.nerc.ac.uk/collection/P35/current/EPC00108/">
<dc:identifier>SDN:P35::EPC00108</dc:identifier>
<dce:identifier>SDN:P35::EPC00108</dce:identifier>
<dc:date>2020-04-15 12:53:01.0</dc:date>
<skos:notation>SDN:P35::EPC00108</skos:notation>
<skos:prefLabel xml:lang="en">Water body phaeopigments</skos:prefLabel>
<skos:altLabel>Water body phaeopigments</skos:altLabel>
<skos:definition xml:lang="en">The total amount of all chlorophyll degradation products contained in the particulate material of a specified volume of any body of salt or fresh water.</skos:definition>
<owl:versionInfo>5</owl:versionInfo>
<pav:hasCurrentVersion rdf:resource="http://vocab.nerc.ac.uk/collection/P35/current/EPC00108/5/"/>
<pav:version>5</pav:version>
<pav:authoredOn>2020-04-15 12:53:01.0</pav:authoredOn>
<skos:note xml:lang="en">accepted</skos:note>
<owl:deprecated>false</owl:deprecated>
<skos:narrower rdf:resource="http://vocab.nerc.ac.uk/collection/P01/current/PHAEFLP3/"/>
<skos:narrower rdf:resource="http://vocab.nerc.ac.uk/collection/P01/current/PHAEFLP1/"/>
<skos:narrower rdf:resource="http://vocab.nerc.ac.uk/collection/P01/current/PHAEFLP4/"/>
<skos:narrower rdf:resource="http://vocab.nerc.ac.uk/collection/P01/current/PHAEZZXX/"/>
<skos:narrower rdf:resource="http://vocab.nerc.ac.uk/collection/P01/current/PHAESPPZ/"/>
<skos:narrower rdf:resource="http://vocab.nerc.ac.uk/collection/P01/current/PHAESPP3/"/>
<skos:narrower rdf:resource="http://vocab.nerc.ac.uk/collection/P01/current/PHAEFLP5/"/>
<skos:narrower rdf:resource="http://vocab.nerc.ac.uk/collection/P01/current/PHAEFLPZ/"/>
<skos:narrower rdf:resource="http://vocab.nerc.ac.uk/collection/P01/current/PHAEFMP1/"/>
<skos:narrower rdf:resource="http://vocab.nerc.ac.uk/collection/P01/current/PHAESPP1/"/>
<skos:related rdf:resource="http://vocab.nerc.ac.uk/collection/P06/current/UMMC/"/>
<skos:broader rdf:resource="http://vocab.nerc.ac.uk/collection/P36/current/CHPHYL/"/>
<void:inDataset rdf:resource="http://vocab.nerc.ac.uk/.well-known/void"/>
</skos:Concept>
</skos:member>
<skos:member>
<skos:Concept rdf:about="http://vocab.nerc.ac.uk/collection/P35/current/EPC00172/">
<dc:identifier>SDN:P35::EPC00172</dc:identifier>
<dce:identifier>SDN:P35::EPC00172</dce:identifier>
<dc:date>2016-12-12 15:20:45.0</dc:date>
<skos:notation>SDN:P35::EPC00172</skos:notation>
<skos:prefLabel xml:lang="en">Water body phenanthrene</skos:prefLabel>
<skos:altLabel>Water body phenanthrene</skos:altLabel>
<skos:definition xml:lang="en">Concentration of phenantrene (dissolved, reactive particulate or suspended particulate material) in river, estuary, sea or ocean.</skos:definition>
<owl:versionInfo>5</owl:versionInfo>
<pav:hasCurrentVersion rdf:resource="http://vocab.nerc.ac.uk/collection/P35/current/EPC00172/5/"/>
<pav:version>5</pav:version>
<pav:authoredOn>2016-12-12 15:20:45.0</pav:authoredOn>
<skos:note xml:lang="en">accepted</skos:note>
<owl:deprecated>false</owl:deprecated>
<skos:narrower rdf:resource="http://vocab.nerc.ac.uk/collection/P01/current/CPAHWC16/"/>
<skos:related rdf:resource="http://vocab.nerc.ac.uk/collection/P06/current/UGPL/"/>
<skos:broader rdf:resource="http://vocab.nerc.ac.uk/collection/P36/current/HCARBS/"/>
<void:inDataset rdf:resource="http://vocab.nerc.ac.uk/.well-known/void"/>
</skos:Concept>
</skos:member>
<skos:member>
<skos:Concept rdf:about="http://vocab.nerc.ac.uk/collection/P35/current/EPC00007/">
<dc:identifier>SDN:P35::EPC00007</dc:identifier>
<dce:identifier>SDN:P35::EPC00007</dce:identifier>
<dc:date>2016-10-20 11:27:18.0</dc:date>
<skos:notation>SDN:P35::EPC00007</skos:notation>
<skos:prefLabel xml:lang="en">Water body phosphate</skos:prefLabel>
<skos:altLabel>PO4</skos:altLabel>
<skos:definition xml:lang="en">Concentration of phosphate per unit volume of a river, estuary, sea or ocean by any method in filtered or unfiltered water.</skos:definition>
<owl:versionInfo>3</owl:versionInfo>
<pav:hasCurrentVersion rdf:resource="http://vocab.nerc.ac.uk/collection/P35/current/EPC00007/3/"/>
<pav:version>3</pav:version>
<pav:authoredOn>2016-10-20 11:27:18.0</pav:authoredOn>
<skos:note xml:lang="en">accepted</skos:note>
<owl:deprecated>false</owl:deprecated>
<skos:narrower rdf:resource="http://vocab.nerc.ac.uk/collection/P01/current/PHOSMATX/"/>
<skos:narrower rdf:resource="http://vocab.nerc.ac.uk/collection/P01/current/PHOSYYDZ/"/>
<skos:narrower rdf:resource="http://vocab.nerc.ac.uk/collection/P01/current/PHOSAAD2/"/>
<skos:narrower rdf:resource="http://vocab.nerc.ac.uk/collection/P01/current/PHOSMAZX/"/>
<skos:narrower rdf:resource="http://vocab.nerc.ac.uk/collection/P01/current/PHOSMA12/"/>
<skos:narrower rdf:resource="http://vocab.nerc.ac.uk/collection/P01/current/PHOSAAZX/"/>
<skos:narrower rdf:resource="http://vocab.nerc.ac.uk/collection/P01/current/PHKGAATX/"/>
<skos:narrower rdf:resource="http://vocab.nerc.ac.uk/collection/P01/current/PHOSMS01/"/>
<skos:narrower rdf:resource="http://vocab.nerc.ac.uk/collection/P01/current/MDMAP906/"/>
<skos:narrower rdf:resource="http://vocab.nerc.ac.uk/collection/P01/current/PHOS04LW/"/>
<skos:narrower rdf:resource="http://vocab.nerc.ac.uk/collection/P01/current/PHOSAAD1/"/>
<skos:narrower rdf:resource="http://vocab.nerc.ac.uk/collection/P01/current/PHOSAATX/"/>
<skos:narrower rdf:resource="http://vocab.nerc.ac.uk/collection/P01/current/PHOSZZXX/"/>
<skos:narrower rdf:resource="http://vocab.nerc.ac.uk/collection/P01/current/PHOSAAD5/"/>
<skos:narrower rdf:resource="http://vocab.nerc.ac.uk/collection/P01/current/PHOSMAD2/"/>
<skos:narrower rdf:resource="http://vocab.nerc.ac.uk/collection/P01/current/PHOSAA01/"/>
<skos:narrower rdf:resource="http://vocab.nerc.ac.uk/collection/P01/current/PHOSAAD3/"/>
<skos:narrower rdf:resource="http://vocab.nerc.ac.uk/collection/P01/current/PHOSMAD3/"/>
<skos:narrower rdf:resource="http://vocab.nerc.ac.uk/collection/P01/current/PHOSMAD1/"/>
<skos:narrower rdf:resource="http://vocab.nerc.ac.uk/collection/P01/current/PHOSXXDZ/"/>
<skos:narrower rdf:resource="http://vocab.nerc.ac.uk/collection/P01/current/PHOSMADZ/"/>
<skos:narrower rdf:resource="http://vocab.nerc.ac.uk/collection/P01/current/PHOSAADZ/"/>
<skos:related rdf:resource="http://vocab.nerc.ac.uk/collection/P06/current/UPOX/"/>
<skos:broader rdf:resource="http://vocab.nerc.ac.uk/collection/P36/current/FERTIL/"/>
<void:inDataset rdf:resource="http://vocab.nerc.ac.uk/.well-known/void"/>
</skos:Concept>
</skos:member>
<skos:member>
<skos:Concept rdf:about="http://vocab.nerc.ac.uk/collection/P35/current/EPC00001/">
<dc:identifier>SDN:P35::EPC00001</dc:identifier>
<dce:identifier>SDN:P35::EPC00001</dce:identifier>
<dc:date>2016-10-20 11:27:18.0</dc:date>
<skos:notation>SDN:P35::EPC00001</skos:notation>
<skos:prefLabel xml:lang="en">Water body salinity</skos:prefLabel>
<skos:altLabel>Salinity</skos:altLabel>
<skos:definition xml:lang="en">Salinity of a river, estuary, sea or ocean by any method and on any measurement scale.</skos:definition>
<owl:versionInfo>3</owl:versionInfo>
<pav:hasCurrentVersion rdf:resource="http://vocab.nerc.ac.uk/collection/P35/current/EPC00001/3/"/>
<pav:version>3</pav:version>
<pav:authoredOn>2016-10-20 11:27:18.0</pav:authoredOn>
<skos:note xml:lang="en">accepted</skos:note>
<owl:deprecated>false</owl:deprecated>
<skos:narrower rdf:resource="http://vocab.nerc.ac.uk/collection/P01/current/PSALST02/"/>
<skos:narrower rdf:resource="http://vocab.nerc.ac.uk/collection/P01/current/PSALCU02/"/>
<skos:narrower rdf:resource="http://vocab.nerc.ac.uk/collection/P01/current/PSALCC02/"/>
<skos:narrower rdf:resource="http://vocab.nerc.ac.uk/collection/P01/current/PSALPR02/"/>
<skos:narrower rdf:resource="http://vocab.nerc.ac.uk/collection/P01/current/PSALTC02/"/>
<skos:narrower rdf:resource="http://vocab.nerc.ac.uk/collection/P01/current/PSALSG02/"/>
<skos:narrower rdf:resource="http://vocab.nerc.ac.uk/collection/P01/current/PSALTC06/"/>
<skos:narrower rdf:resource="http://vocab.nerc.ac.uk/collection/P01/current/PSALTC03/"/>
<skos:narrower rdf:resource="http://vocab.nerc.ac.uk/collection/P01/current/PSALST01/"/>
<skos:narrower rdf:resource="http://vocab.nerc.ac.uk/collection/P01/current/PSALCU01/"/>
<skos:narrower rdf:resource="http://vocab.nerc.ac.uk/collection/P01/current/PSALCC01/"/>
<skos:narrower rdf:resource="http://vocab.nerc.ac.uk/collection/P01/current/PSALBRBR/"/>
<skos:narrower rdf:resource="http://vocab.nerc.ac.uk/collection/P01/current/PSALBSTX/"/>
<skos:narrower rdf:resource="http://vocab.nerc.ac.uk/collection/P01/current/PSALZZXX/"/>
<skos:narrower rdf:resource="http://vocab.nerc.ac.uk/collection/P01/current/PSALPR01/"/>
<skos:narrower rdf:resource="http://vocab.nerc.ac.uk/collection/P01/current/PSALTC01/"/>
<skos:narrower rdf:resource="http://vocab.nerc.ac.uk/collection/P01/current/PSCLCCI1/"/>
<skos:narrower rdf:resource="http://vocab.nerc.ac.uk/collection/P01/current/PSALMV01/"/>
<skos:narrower rdf:resource="http://vocab.nerc.ac.uk/collection/P01/current/PSALMC01/"/>
<skos:narrower rdf:resource="http://vocab.nerc.ac.uk/collection/P01/current/PSALSZ01/"/>
<skos:narrower rdf:resource="http://vocab.nerc.ac.uk/collection/P01/current/PSALSU01/"/>
<skos:narrower rdf:resource="http://vocab.nerc.ac.uk/collection/P01/current/PSALSG01/"/>
<skos:narrower rdf:resource="http://vocab.nerc.ac.uk/collection/P01/current/PSSDCU02/"/>
<skos:narrower rdf:resource="http://vocab.nerc.ac.uk/collection/P01/current/PSSDCU01/"/>
<skos:narrower rdf:resource="http://vocab.nerc.ac.uk/collection/P01/current/PSALSD01/"/>
<skos:narrower rdf:resource="http://vocab.nerc.ac.uk/collection/P01/current/PSSDBSTX/"/>
<skos:narrower rdf:resource="http://vocab.nerc.ac.uk/collection/P01/current/SSALSL01/"/>
<skos:narrower rdf:resource="http://vocab.nerc.ac.uk/collection/P01/current/SSALBSTX/"/>
<skos:narrower rdf:resource="http://vocab.nerc.ac.uk/collection/P01/current/SSALSG01/"/>
<skos:narrower rdf:resource="http://vocab.nerc.ac.uk/collection/P01/current/SSALAGT1/"/>
<skos:narrower rdf:resource="http://vocab.nerc.ac.uk/collection/P01/current/ASLTZZ01/"/>
<skos:narrower rdf:resource="http://vocab.nerc.ac.uk/collection/P01/current/PSALTC05/"/>
<skos:narrower rdf:resource="http://vocab.nerc.ac.uk/collection/P01/current/PSALTC04/"/>
<skos:narrower rdf:resource="http://vocab.nerc.ac.uk/collection/P01/current/PSLTZZ01/"/>
<skos:narrower rdf:resource="http://vocab.nerc.ac.uk/collection/P01/current/PSCLCCL1/"/>
<skos:narrower rdf:resource="http://vocab.nerc.ac.uk/collection/P01/current/ODSDM021/"/>
<skos:narrower rdf:resource="http://vocab.nerc.ac.uk/collection/P01/current/SSALST01/"/>
<skos:narrower rdf:resource="http://vocab.nerc.ac.uk/collection/P01/current/SSALPR01/"/>
<skos:related rdf:resource="http://vocab.nerc.ac.uk/collection/P06/current/UPPT/"/>
<void:inDataset rdf:resource="http://vocab.nerc.ac.uk/.well-known/void"/>
</skos:Concept>
</skos:member>
<skos:member>
<skos:Concept rdf:about="http://vocab.nerc.ac.uk/collection/P35/current/EPC00008/">
<dc:identifier>SDN:P35::EPC00008</dc:identifier>
<dce:identifier>SDN:P35::EPC00008</dce:identifier>
<dc:date>2016-10-20 11:27:18.0</dc:date>
<skos:notation>SDN:P35::EPC00008</skos:notation>
<skos:prefLabel xml:lang="en">Water body silicate</skos:prefLabel>
<skos:altLabel>SiO4</skos:altLabel>
<skos:definition xml:lang="en">Concentration of silicate per unit volume of a river, estuary, sea or ocean by any method in filtered or unfiltered water.</skos:definition>
<owl:versionInfo>3</owl:versionInfo>
<pav:hasCurrentVersion rdf:resource="http://vocab.nerc.ac.uk/collection/P35/current/EPC00008/3/"/>
<pav:version>3</pav:version>
<pav:authoredOn>2016-10-20 11:27:18.0</pav:authoredOn>
<skos:note xml:lang="en">accepted</skos:note>
<owl:deprecated>false</owl:deprecated>
<skos:narrower rdf:resource="http://vocab.nerc.ac.uk/collection/P01/current/SLCAMAZX/"/>
<skos:narrower rdf:resource="http://vocab.nerc.ac.uk/collection/P01/current/SLCAAAD1/"/>
<skos:narrower rdf:resource="http://vocab.nerc.ac.uk/collection/P01/current/SLCAMATX/"/>
<skos:narrower rdf:resource="http://vocab.nerc.ac.uk/collection/P01/current/SLCAAADZ/"/>
<skos:narrower rdf:resource="http://vocab.nerc.ac.uk/collection/P01/current/SLCAAAD3/"/>
<skos:narrower rdf:resource="http://vocab.nerc.ac.uk/collection/P01/current/SLCAAAD2/"/>
<skos:narrower rdf:resource="http://vocab.nerc.ac.uk/collection/P01/current/SLCAMS01/"/>
<skos:narrower rdf:resource="http://vocab.nerc.ac.uk/collection/P01/current/SLCAKGD1/"/>
<skos:narrower rdf:resource="http://vocab.nerc.ac.uk/collection/P01/current/MDMAP012/"/>
<skos:narrower rdf:resource="http://vocab.nerc.ac.uk/collection/P01/current/SLCAAAZX/"/>
<skos:narrower rdf:resource="http://vocab.nerc.ac.uk/collection/P01/current/SLCAZZXX/"/>
<skos:narrower rdf:resource="http://vocab.nerc.ac.uk/collection/P01/current/SLCANS01/"/>
<skos:narrower rdf:resource="http://vocab.nerc.ac.uk/collection/P01/current/SLCAAATX/"/>
<skos:narrower rdf:resource="http://vocab.nerc.ac.uk/collection/P01/current/SLCAMAD3/"/>
<skos:narrower rdf:resource="http://vocab.nerc.ac.uk/collection/P01/current/SLCAAA01/"/>
<skos:narrower rdf:resource="http://vocab.nerc.ac.uk/collection/P01/current/SLCAMA12/"/>
<skos:narrower rdf:resource="http://vocab.nerc.ac.uk/collection/P01/current/SLCAAAD5/"/>
<skos:related rdf:resource="http://vocab.nerc.ac.uk/collection/P06/current/UPOX/"/>
<skos:broader rdf:resource="http://vocab.nerc.ac.uk/collection/P36/current/SLCATE/"/>
<void:inDataset rdf:resource="http://vocab.nerc.ac.uk/.well-known/void"/>
</skos:Concept>
</skos:member>
<skos:member>
<skos:Concept rdf:about="http://vocab.nerc.ac.uk/collection/P35/current/EPC00131/">
<dc:identifier>SDN:P35::EPC00131</dc:identifier>
<dce:identifier>SDN:P35::EPC00131</dce:identifier>
<dc:date>2016-10-20 11:27:18.0</dc:date>
<skos:notation>SDN:P35::EPC00131</skos:notation>
<skos:prefLabel xml:lang="en">Water body total alkalinity</skos:prefLabel>
<skos:altLabel>Talk</skos:altLabel>
<skos:definition xml:lang="en">Concentration of alkali in the form of carbonate, bicarbonate and hydroxide in a sample from any body of fresh or salt water.</skos:definition>
<owl:versionInfo>3</owl:versionInfo>
<pav:hasCurrentVersion rdf:resource="http://vocab.nerc.ac.uk/collection/P35/current/EPC00131/3/"/>
<pav:version>3</pav:version>
<pav:authoredOn>2016-10-20 11:27:18.0</pav:authoredOn>
<skos:note xml:lang="en">accepted</skos:note>
<owl:deprecated>false</owl:deprecated>
<skos:narrower rdf:resource="http://vocab.nerc.ac.uk/collection/P01/current/ALKYSPTX/"/>
<skos:narrower rdf:resource="http://vocab.nerc.ac.uk/collection/P01/current/ALKYPOTX/"/>
<skos:narrower rdf:resource="http://vocab.nerc.ac.uk/collection/P01/current/MDMAP014/"/>
<skos:narrower rdf:resource="http://vocab.nerc.ac.uk/collection/P01/current/ALKYZZYY/"/>
<skos:narrower rdf:resource="http://vocab.nerc.ac.uk/collection/P01/current/ALKYZZXX/"/>
<skos:related rdf:resource="http://vocab.nerc.ac.uk/collection/P06/current/MEQL/"/>
<skos:broader rdf:resource="http://vocab.nerc.ac.uk/collection/P36/current/ACIDIT/"/>
<void:inDataset rdf:resource="http://vocab.nerc.ac.uk/.well-known/void"/>
</skos:Concept>
</skos:member>
<skos:member>
<skos:Concept rdf:about="http://vocab.nerc.ac.uk/collection/P35/current/EPC00134/">
<dc:identifier>SDN:P35::EPC00134</dc:identifier>
<dce:identifier>SDN:P35::EPC00134</dce:identifier>
<dc:date>2016-10-20 11:27:18.0</dc:date>
<skos:notation>SDN:P35::EPC00134</skos:notation>
<skos:prefLabel xml:lang="en">Water body total nitrogen</skos:prefLabel>
<skos:altLabel>TotN</skos:altLabel>
<skos:definition xml:lang="en">Concentration of organic plus inorganic nitrogen in the dissolved phase plus the particulate phase in a given volume of a sample from any body of salt or fresh water.</skos:definition>
<owl:versionInfo>3</owl:versionInfo>
<pav:hasCurrentVersion rdf:resource="http://vocab.nerc.ac.uk/collection/P35/current/EPC00134/3/"/>
<pav:version>3</pav:version>
<pav:authoredOn>2016-10-20 11:27:18.0</pav:authoredOn>
<skos:note xml:lang="en">accepted</skos:note>
<owl:deprecated>false</owl:deprecated>
<skos:narrower rdf:resource="http://vocab.nerc.ac.uk/collection/P01/current/NTOTZZXX/"/>
<skos:narrower rdf:resource="http://vocab.nerc.ac.uk/collection/P01/current/NTOTWCTX/"/>
<skos:related rdf:resource="http://vocab.nerc.ac.uk/collection/P06/current/UPOX/"/>
<skos:broader rdf:resource="http://vocab.nerc.ac.uk/collection/P36/current/FERTIL/"/>
<void:inDataset rdf:resource="http://vocab.nerc.ac.uk/.well-known/void"/>
</skos:Concept>
</skos:member>
<skos:member>
<skos:Concept rdf:about="http://vocab.nerc.ac.uk/collection/P35/current/EPC00135/">
<dc:identifier>SDN:P35::EPC00135</dc:identifier>
<dce:identifier>SDN:P35::EPC00135</dce:identifier>
<dc:date>2016-10-20 11:27:18.0</dc:date>
<skos:notation>SDN:P35::EPC00135</skos:notation>
<skos:prefLabel xml:lang="en">Water body total phosphorus</skos:prefLabel>
<skos:altLabel>TotP</skos:altLabel>
<skos:definition xml:lang="en">Concentration of organic plus inorganic phosphorus in the dissolved phase plus the particulate phase in a given volume of a sample from any body of salt or fresh water.</skos:definition>
<owl:versionInfo>3</owl:versionInfo>
<pav:hasCurrentVersion rdf:resource="http://vocab.nerc.ac.uk/collection/P35/current/EPC00135/3/"/>
<pav:version>3</pav:version>
<pav:authoredOn>2016-10-20 11:27:18.0</pav:authoredOn>
<skos:note xml:lang="en">accepted</skos:note>
<owl:deprecated>false</owl:deprecated>
<skos:narrower rdf:resource="http://vocab.nerc.ac.uk/collection/P01/current/TPHSZZXX/"/>
<skos:narrower rdf:resource="http://vocab.nerc.ac.uk/collection/P01/current/TPHSPP01/"/>
<skos:related rdf:resource="http://vocab.nerc.ac.uk/collection/P06/current/UPOX/"/>
<skos:broader rdf:resource="http://vocab.nerc.ac.uk/collection/P36/current/FERTIL/"/>
<void:inDataset rdf:resource="http://vocab.nerc.ac.uk/.well-known/void"/>
</skos:Concept>
</skos:member>
<skos:member>
<skos:Concept rdf:about="http://vocab.nerc.ac.uk/collection/P35/current/EPC00179/">
<dc:identifier>SDN:P35::EPC00179</dc:identifier>
<dce:identifier>SDN:P35::EPC00179</dce:identifier>
<dc:date>2018-03-20 16:01:06.0</dc:date>
<skos:notation>SDN:P35::EPC00179</skos:notation>
<skos:prefLabel xml:lang="en">Water body tributyltin (TBT)</skos:prefLabel>
<skos:altLabel>Water body tributyltin (TBT)</skos:altLabel>
<skos:definition xml:lang="en">Concentration of tributyltin in the water (dissolved, reactive particulate or suspended particulate material) regardless of analytical method per unit volume of a river, estuary, sea or ocean by any method in filtered or unfiltered water.</skos:definition>
<owl:versionInfo>7</owl:versionInfo>
<pav:hasCurrentVersion rdf:resource="http://vocab.nerc.ac.uk/collection/P35/current/EPC00179/7/"/>
<pav:version>7</pav:version>
<pav:authoredOn>2018-03-20 16:01:06.0</pav:authoredOn>
<skos:note xml:lang="en">accepted</skos:note>
<owl:deprecated>false</owl:deprecated>
<skos:narrower rdf:resource="http://vocab.nerc.ac.uk/collection/P01/current/POLLM010/"/>
<skos:narrower rdf:resource="http://vocab.nerc.ac.uk/collection/P01/current/ADISSTBT/"/>
<skos:related rdf:resource="http://vocab.nerc.ac.uk/collection/P06/current/UGPL/"/>
<skos:broader rdf:resource="http://vocab.nerc.ac.uk/collection/P36/current/ANTIFL/"/>
<void:inDataset rdf:resource="http://vocab.nerc.ac.uk/.well-known/void"/>
</skos:Concept>
</skos:member>
<skos:member>
<skos:Concept rdf:about="http://vocab.nerc.ac.uk/collection/P35/current/EPC00138/">
<dc:identifier>SDN:P35::EPC00138</dc:identifier>
<dce:identifier>SDN:P35::EPC00138</dce:identifier>
<dc:date>2016-12-12 15:20:45.0</dc:date>
<skos:notation>SDN:P35::EPC00138</skos:notation>
<skos:prefLabel xml:lang="en">Water body triphenyltin (TPT)</skos:prefLabel>
<skos:altLabel>Water body triphenyltin (TPT)</skos:altLabel>
<skos:definition xml:lang="en">Concentration of triphenyltin cation in the water (dissolved, reactive particulate or suspended particulate material) regardless of analytical or normalization method.</skos:definition>
<owl:versionInfo>5</owl:versionInfo>
<pav:hasCurrentVersion rdf:resource="http://vocab.nerc.ac.uk/collection/P35/current/EPC00138/5/"/>
<pav:version>5</pav:version>
<pav:authoredOn>2016-12-12 15:20:45.0</pav:authoredOn>
<skos:note xml:lang="en">accepted</skos:note>
<owl:deprecated>false</owl:deprecated>
<skos:narrower rdf:resource="http://vocab.nerc.ac.uk/collection/P01/current/ADISSTPT/"/>
<skos:related rdf:resource="http://vocab.nerc.ac.uk/collection/P06/current/UGPL/"/>
<skos:broader rdf:resource="http://vocab.nerc.ac.uk/collection/P36/current/ANTIFL/"/>
<void:inDataset rdf:resource="http://vocab.nerc.ac.uk/.well-known/void"/>
</skos:Concept>
</skos:member>
<skos:member>
<skos:Concept rdf:about="http://vocab.nerc.ac.uk/collection/P35/current/EPC00010/">
<dc:identifier>SDN:P35::EPC00010</dc:identifier>
<dce:identifier>SDN:P35::EPC00010</dce:identifier>
<dc:date>2016-10-20 11:27:18.0</dc:date>
<skos:notation>SDN:P35::EPC00010</skos:notation>
<skos:prefLabel xml:lang="en">Water body urea</skos:prefLabel>
<skos:altLabel>Urea</skos:altLabel>
<skos:definition xml:lang="en">Concentration of urea per unit volume of a river, estuary, sea or ocean by any method in filtered or unfiltered water.</skos:definition>
<owl:versionInfo>3</owl:versionInfo>
<pav:hasCurrentVersion rdf:resource="http://vocab.nerc.ac.uk/collection/P35/current/EPC00010/3/"/>
<pav:version>3</pav:version>
<pav:authoredOn>2016-10-20 11:27:18.0</pav:authoredOn>
<skos:note xml:lang="en">accepted</skos:note>
<owl:deprecated>false</owl:deprecated>
<skos:narrower rdf:resource="http://vocab.nerc.ac.uk/collection/P01/current/UREAZZZZ/"/>
<skos:narrower rdf:resource="http://vocab.nerc.ac.uk/collection/P01/current/UREAAATX/"/>
<skos:narrower rdf:resource="http://vocab.nerc.ac.uk/collection/P01/current/UREAAAD3/"/>
<skos:narrower rdf:resource="http://vocab.nerc.ac.uk/collection/P01/current/UREAAADZ/"/>
<skos:narrower rdf:resource="http://vocab.nerc.ac.uk/collection/P01/current/UREAAAD2/"/>
<skos:narrower rdf:resource="http://vocab.nerc.ac.uk/collection/P01/current/UREAAAZX/"/>
<skos:narrower rdf:resource="http://vocab.nerc.ac.uk/collection/P01/current/UREAAAD1/"/>
<skos:related rdf:resource="http://vocab.nerc.ac.uk/collection/P06/current/UPOX/"/>
<skos:broader rdf:resource="http://vocab.nerc.ac.uk/collection/P36/current/FERTIL/"/>
<void:inDataset rdf:resource="http://vocab.nerc.ac.uk/.well-known/void"/>
</skos:Concept>
</skos:member>
<skos:member>
<skos:Concept rdf:about="http://vocab.nerc.ac.uk/collection/P35/current/EPC00215/">
<dc:identifier>SDN:P35::EPC00215</dc:identifier>
<dce:identifier>SDN:P35::EPC00215</dce:identifier>
<dc:date>2018-03-20 16:58:29.0</dc:date>
<skos:notation>SDN:P35::EPC00215</skos:notation>
<skos:prefLabel xml:lang="en">Zinc in Mytilus</skos:prefLabel>
<skos:altLabel>Zinc in Mytilus</skos:altLabel>
<skos:definition xml:lang="en">Concentration of zinc per unit weight (dry or wet) of Mytilus spp. (regardless of Mytilus species and size class).</skos:definition>
<owl:versionInfo>6</owl:versionInfo>
<pav:hasCurrentVersion rdf:resource="http://vocab.nerc.ac.uk/collection/P35/current/EPC00215/6/"/>
<pav:version>6</pav:version>
<pav:authoredOn>2018-03-20 16:58:29.0</pav:authoredOn>
<skos:note xml:lang="en">deprecated</skos:note>
<owl:deprecated>true</owl:deprecated>
<skos:narrower rdf:resource="http://vocab.nerc.ac.uk/collection/P01/current/ZNWW6569/"/>
<skos:narrower rdf:resource="http://vocab.nerc.ac.uk/collection/P01/current/MYTGAL02/"/>
<skos:narrower rdf:resource="http://vocab.nerc.ac.uk/collection/P01/current/ZNDWCF14/"/>
<skos:related rdf:resource="http://vocab.nerc.ac.uk/collection/P06/current/UUKG/"/>
<skos:broader rdf:resource="http://vocab.nerc.ac.uk/collection/P36/current/HVYMTL/"/>
<void:inDataset rdf:resource="http://vocab.nerc.ac.uk/.well-known/void"/>
</skos:Concept>
</skos:member>
<skos:member>
<skos:Concept rdf:about="http://vocab.nerc.ac.uk/collection/P35/current/EPC00145/">
<dc:identifier>SDN:P35::EPC00145</dc:identifier>
<dce:identifier>SDN:P35::EPC00145</dce:identifier>
<dc:date>2018-03-20 16:58:29.0</dc:date>
<skos:notation>SDN:P35::EPC00145</skos:notation>
<skos:prefLabel xml:lang="en">Zinc in the sediment</skos:prefLabel>
<skos:altLabel>Zinc in the sediment</skos:altLabel>
<skos:definition xml:lang="en">Concentration of zinc in sediment and sediment pore waters (regardless of sediment size class and analytical method).</skos:definition>
<owl:versionInfo>6</owl:versionInfo>
<pav:hasCurrentVersion rdf:resource="http://vocab.nerc.ac.uk/collection/P35/current/EPC00145/6/"/>
<pav:version>6</pav:version>
<pav:authoredOn>2018-03-20 16:58:29.0</pav:authoredOn>
<skos:note xml:lang="en">deprecated</skos:note>
<owl:deprecated>true</owl:deprecated>
<skos:narrower rdf:resource="http://vocab.nerc.ac.uk/collection/P01/current/MZNSP012/"/>
<skos:narrower rdf:resource="http://vocab.nerc.ac.uk/collection/P01/current/ZNSEDBD1/"/>
<skos:narrower rdf:resource="http://vocab.nerc.ac.uk/collection/P01/current/RWSSED32/"/>
<skos:narrower rdf:resource="http://vocab.nerc.ac.uk/collection/P01/current/MTSDM008/"/>
<skos:narrower rdf:resource="http://vocab.nerc.ac.uk/collection/P01/current/ZNCNAAWF/"/>
<skos:narrower rdf:resource="http://vocab.nerc.ac.uk/collection/P01/current/ZNCNPEXT/"/>
<skos:narrower rdf:resource="http://vocab.nerc.ac.uk/collection/P01/current/ZNCNXTXT/"/>
<skos:narrower rdf:resource="http://vocab.nerc.ac.uk/collection/P01/current/ZNCNICXT/"/>
<skos:related rdf:resource="http://vocab.nerc.ac.uk/collection/P06/current/UMKG/"/>
<skos:broader rdf:resource="http://vocab.nerc.ac.uk/collection/P36/current/HVYMTL/"/>
<void:inDataset rdf:resource="http://vocab.nerc.ac.uk/.well-known/void"/>
</skos:Concept>
</skos:member>
<skos:member>
<skos:Concept rdf:about="http://vocab.nerc.ac.uk/collection/P35/current/EPC00119/">
<dc:identifier>SDN:P35::EPC00119</dc:identifier>
<dce:identifier>SDN:P35::EPC00119</dce:identifier>
<dc:date>2016-10-20 11:27:18.0</dc:date>
<skos:notation>SDN:P35::EPC00119</skos:notation>
<skos:prefLabel xml:lang="en">Zinc per unit dry weight of sediment</skos:prefLabel>
<skos:altLabel>Zn sediment</skos:altLabel>
<skos:definition xml:lang="en">Concentration of the specified metal in unit weight of the unsieved or 2mm screened dried sediment.</skos:definition>
<owl:versionInfo>3</owl:versionInfo>
<pav:hasCurrentVersion rdf:resource="http://vocab.nerc.ac.uk/collection/P35/current/EPC00119/3/"/>
<pav:version>3</pav:version>
<pav:authoredOn>2016-10-20 11:27:18.0</pav:authoredOn>
<skos:note xml:lang="en">accepted</skos:note>
<owl:deprecated>false</owl:deprecated>
<skos:narrower rdf:resource="http://vocab.nerc.ac.uk/collection/P01/current/MZNSP012/"/>
<skos:narrower rdf:resource="http://vocab.nerc.ac.uk/collection/P01/current/ZNCNICXT/"/>
<skos:narrower rdf:resource="http://vocab.nerc.ac.uk/collection/P01/current/ZNCNPEXT/"/>
<skos:narrower rdf:resource="http://vocab.nerc.ac.uk/collection/P01/current/ZNCNXTXT/"/>
<skos:narrower rdf:resource="http://vocab.nerc.ac.uk/collection/P01/current/ZNSEDBD1/"/>
<skos:related rdf:resource="http://vocab.nerc.ac.uk/collection/P06/current/UMKG/"/>
<skos:broader rdf:resource="http://vocab.nerc.ac.uk/collection/P36/current/HVYMTL/"/>
<void:inDataset rdf:resource="http://vocab.nerc.ac.uk/.well-known/void"/>
</skos:Concept>
</skos:member>
<skos:member>
<skos:Concept rdf:about="http://vocab.nerc.ac.uk/collection/P35/current/EPC00130/">
<dc:identifier>SDN:P35::EPC00130</dc:identifier>
<dce:identifier>SDN:P35::EPC00130</dce:identifier>
<dc:date>2016-10-20 11:27:18.0</dc:date>
<skos:notation>SDN:P35::EPC00130</skos:notation>
<skos:prefLabel xml:lang="en">Zinc per unit dry weight of sediment &lt;63um</skos:prefLabel>
<skos:altLabel>Zn sediment &lt;63um</skos:altLabel>
<skos:definition xml:lang="en">Concentration of the specified metal in unit weight of the sediment passed through a 63 micron sieve and dried.</skos:definition>
<owl:versionInfo>3</owl:versionInfo>
<pav:hasCurrentVersion rdf:resource="http://vocab.nerc.ac.uk/collection/P35/current/EPC00130/3/"/>
<pav:version>3</pav:version>
<pav:authoredOn>2016-10-20 11:27:18.0</pav:authoredOn>
<skos:note xml:lang="en">accepted</skos:note>
<owl:deprecated>false</owl:deprecated>
<skos:narrower rdf:resource="http://vocab.nerc.ac.uk/collection/P01/current/ZNCNAAWF/"/>
<skos:narrower rdf:resource="http://vocab.nerc.ac.uk/collection/P01/current/RWSSED32/"/>
<skos:narrower rdf:resource="http://vocab.nerc.ac.uk/collection/P01/current/MTSDM008/"/>
<skos:related rdf:resource="http://vocab.nerc.ac.uk/collection/P06/current/UMKG/"/>
<skos:broader rdf:resource="http://vocab.nerc.ac.uk/collection/P36/current/HVYMTL/"/>
<void:inDataset rdf:resource="http://vocab.nerc.ac.uk/.well-known/void"/>
</skos:Concept>
</skos:member>
<skos:member>
<skos:Concept rdf:about="http://vocab.nerc.ac.uk/collection/P35/current/EPC00229/">
<dc:identifier>SDN:P35::EPC00229</dc:identifier>
<dce:identifier>SDN:P35::EPC00229</dce:identifier>
<dc:date>2018-03-20 16:58:29.0</dc:date>
<skos:notation>SDN:P35::EPC00229</skos:notation>
<skos:prefLabel xml:lang="en">p,p'-DDD in Mytilus</skos:prefLabel>
<skos:altLabel>p,p'-DDD in Mytilus</skos:altLabel>
<skos:definition xml:lang="en">Concentration of p,p'-DDD per unit weight (dry or wet) of Mytilus spp. (regardless of Mytilus species and size class).</skos:definition>
<owl:versionInfo>3</owl:versionInfo>
<pav:hasCurrentVersion rdf:resource="http://vocab.nerc.ac.uk/collection/P35/current/EPC00229/3/"/>
<pav:version>3</pav:version>
<pav:authoredOn>2018-03-20 16:58:29.0</pav:authoredOn>
<skos:note xml:lang="en">deprecated</skos:note>
<owl:deprecated>true</owl:deprecated>
<skos:narrower rdf:resource="http://vocab.nerc.ac.uk/collection/P01/current/PDDW6569/"/>
<skos:narrower rdf:resource="http://vocab.nerc.ac.uk/collection/P01/current/PDADCF14/"/>
<skos:narrower rdf:resource="http://vocab.nerc.ac.uk/collection/P01/current/IFRPST04/"/>
<skos:related rdf:resource="http://vocab.nerc.ac.uk/collection/P06/current/UUKG/"/>
<skos:broader rdf:resource="http://vocab.nerc.ac.uk/collection/P36/current/PESTBI/"/>
<void:inDataset rdf:resource="http://vocab.nerc.ac.uk/.well-known/void"/>
</skos:Concept>
</skos:member>
<skos:member>
<skos:Concept rdf:about="http://vocab.nerc.ac.uk/collection/P35/current/EPC00223/">
<dc:identifier>SDN:P35::EPC00223</dc:identifier>
<dce:identifier>SDN:P35::EPC00223</dce:identifier>
<dc:date>2016-12-12 15:20:45.0</dc:date>
<skos:notation>SDN:P35::EPC00223</skos:notation>
<skos:prefLabel xml:lang="en">p,p'-DDD in the sediment</skos:prefLabel>
<skos:altLabel>p,p'-DDD in the sediment</skos:altLabel>
<skos:definition xml:lang="en">Concentration of p,p'-DDD per unit dry weight of sediment (regardless of sediment size class).</skos:definition>
<owl:versionInfo>2</owl:versionInfo>
<pav:hasCurrentVersion rdf:resource="http://vocab.nerc.ac.uk/collection/P35/current/EPC00223/2/"/>
<pav:version>2</pav:version>
<pav:authoredOn>2016-12-12 15:20:45.0</pav:authoredOn>
<skos:note xml:lang="en">accepted</skos:note>
<owl:deprecated>false</owl:deprecated>
<skos:narrower rdf:resource="http://vocab.nerc.ac.uk/collection/P01/current/PDDDDTSD/"/>
<skos:related rdf:resource="http://vocab.nerc.ac.uk/collection/P06/current/UUKG/"/>
<skos:broader rdf:resource="http://vocab.nerc.ac.uk/collection/P36/current/PESTBI/"/>
<void:inDataset rdf:resource="http://vocab.nerc.ac.uk/.well-known/void"/>
</skos:Concept>
</skos:member>
<skos:member>
<skos:Concept rdf:about="http://vocab.nerc.ac.uk/collection/P35/current/EPC00230/">
<dc:identifier>SDN:P35::EPC00230</dc:identifier>
<dce:identifier>SDN:P35::EPC00230</dce:identifier>
<dc:date>2018-03-20 16:58:29.0</dc:date>
<skos:notation>SDN:P35::EPC00230</skos:notation>
<skos:prefLabel xml:lang="en">p,p'-DDE in Mytilus</skos:prefLabel>
<skos:altLabel>p,p'-DDE in Mytilus</skos:altLabel>
<skos:definition xml:lang="en">Concentration of p,p'-DDE per unit weight (dry or wet) of Mytilus spp. (regardless of Mytilus species and size class).</skos:definition>
<owl:versionInfo>3</owl:versionInfo>
<pav:hasCurrentVersion rdf:resource="http://vocab.nerc.ac.uk/collection/P35/current/EPC00230/3/"/>
<pav:version>3</pav:version>
<pav:authoredOn>2018-03-20 16:58:29.0</pav:authoredOn>
<skos:note xml:lang="en">deprecated</skos:note>
<owl:deprecated>true</owl:deprecated>
<skos:narrower rdf:resource="http://vocab.nerc.ac.uk/collection/P01/current/PDDDCF14/"/>
<skos:narrower rdf:resource="http://vocab.nerc.ac.uk/collection/P01/current/PDDWCF14/"/>
<skos:narrower rdf:resource="http://vocab.nerc.ac.uk/collection/P01/current/PDEW6569/"/>
<skos:narrower rdf:resource="http://vocab.nerc.ac.uk/collection/P01/current/MUM13134/"/>
<skos:narrower rdf:resource="http://vocab.nerc.ac.uk/collection/P01/current/IFRPST07/"/>
<skos:related rdf:resource="http://vocab.nerc.ac.uk/collection/P06/current/UUKG/"/>
<skos:broader rdf:resource="http://vocab.nerc.ac.uk/collection/P36/current/PESTBI/"/>
<void:inDataset rdf:resource="http://vocab.nerc.ac.uk/.well-known/void"/>
</skos:Concept>
</skos:member>
<skos:member>
<skos:Concept rdf:about="http://vocab.nerc.ac.uk/collection/P35/current/EPC00224/">
<dc:identifier>SDN:P35::EPC00224</dc:identifier>
<dce:identifier>SDN:P35::EPC00224</dce:identifier>
<dc:date>2016-12-12 15:20:45.0</dc:date>
<skos:notation>SDN:P35::EPC00224</skos:notation>
<skos:prefLabel xml:lang="en">p,p'-DDE in the sediment</skos:prefLabel>
<skos:altLabel>p,p'-DDE in the sediment</skos:altLabel>
<skos:definition xml:lang="en">Concentration of p,p'-DDE per unit dry weight of sediment (regardless of sediment size class).</skos:definition>
<owl:versionInfo>2</owl:versionInfo>
<pav:hasCurrentVersion rdf:resource="http://vocab.nerc.ac.uk/collection/P35/current/EPC00224/2/"/>
<pav:version>2</pav:version>
<pav:authoredOn>2016-12-12 15:20:45.0</pav:authoredOn>
<skos:note xml:lang="en">accepted</skos:note>
<owl:deprecated>false</owl:deprecated>
<skos:narrower rdf:resource="http://vocab.nerc.ac.uk/collection/P01/current/PDDEDTSD/"/>
<skos:related rdf:resource="http://vocab.nerc.ac.uk/collection/P06/current/UUKG/"/>
<skos:broader rdf:resource="http://vocab.nerc.ac.uk/collection/P36/current/PESTBI/"/>
<void:inDataset rdf:resource="http://vocab.nerc.ac.uk/.well-known/void"/>
</skos:Concept>
</skos:member>
<skos:member>
<skos:Concept rdf:about="http://vocab.nerc.ac.uk/collection/P35/current/EPC00228/">
<dc:identifier>SDN:P35::EPC00228</dc:identifier>
<dce:identifier>SDN:P35::EPC00228</dce:identifier>
<dc:date>2018-03-20 16:58:29.0</dc:date>
<skos:notation>SDN:P35::EPC00228</skos:notation>
<skos:prefLabel xml:lang="en">p,p'-DDT in Mytilus</skos:prefLabel>
<skos:altLabel>p,p'-DDT in Mytilus</skos:altLabel>
<skos:definition xml:lang="en">Concentration of p,p'-DDT per unit weight (dry or wet) of Mytilus spp. (regardless of Mytilus species and size class).</skos:definition>
<owl:versionInfo>3</owl:versionInfo>
<pav:hasCurrentVersion rdf:resource="http://vocab.nerc.ac.uk/collection/P35/current/EPC00228/3/"/>
<pav:version>3</pav:version>
<pav:authoredOn>2018-03-20 16:58:29.0</pav:authoredOn>
<skos:note xml:lang="en">deprecated</skos:note>
<owl:deprecated>true</owl:deprecated>
<skos:narrower rdf:resource="http://vocab.nerc.ac.uk/collection/P01/current/PDTW6569/"/>
<skos:narrower rdf:resource="http://vocab.nerc.ac.uk/collection/P01/current/MUM13142/"/>
<skos:narrower rdf:resource="http://vocab.nerc.ac.uk/collection/P01/current/PDTDCF14/"/>
<skos:narrower rdf:resource="http://vocab.nerc.ac.uk/collection/P01/current/MMUSDDTP/"/>
<skos:narrower rdf:resource="http://vocab.nerc.ac.uk/collection/P01/current/PDTWCF14/"/>
<skos:related rdf:resource="http://vocab.nerc.ac.uk/collection/P06/current/UUKG/"/>
<skos:broader rdf:resource="http://vocab.nerc.ac.uk/collection/P36/current/PESTBI/"/>
<void:inDataset rdf:resource="http://vocab.nerc.ac.uk/.well-known/void"/>
</skos:Concept>
</skos:member>
<skos:member>
<skos:Concept rdf:about="http://vocab.nerc.ac.uk/collection/P35/current/EPC00222/">
<dc:identifier>SDN:P35::EPC00222</dc:identifier>
<dce:identifier>SDN:P35::EPC00222</dce:identifier>
<dc:date>2016-12-12 15:20:45.0</dc:date>
<skos:notation>SDN:P35::EPC00222</skos:notation>
<skos:prefLabel xml:lang="en">p,p'-DDT in the sediment</skos:prefLabel>
<skos:altLabel>p,p'-DDT in the sediment</skos:altLabel>
<skos:definition xml:lang="en">Concentration of p,p'-DDT per unit dry weight of sediment (regardless of sediment size class).</skos:definition>
<owl:versionInfo>2</owl:versionInfo>
<pav:hasCurrentVersion rdf:resource="http://vocab.nerc.ac.uk/collection/P35/current/EPC00222/2/"/>
<pav:version>2</pav:version>
<pav:authoredOn>2016-12-12 15:20:45.0</pav:authoredOn>
<skos:note xml:lang="en">accepted</skos:note>
<owl:deprecated>false</owl:deprecated>
<skos:narrower rdf:resource="http://vocab.nerc.ac.uk/collection/P01/current/PDDTDTSD/"/>
<skos:related rdf:resource="http://vocab.nerc.ac.uk/collection/P06/current/UUKG/"/>
<skos:broader rdf:resource="http://vocab.nerc.ac.uk/collection/P36/current/PESTBI/"/>
<void:inDataset rdf:resource="http://vocab.nerc.ac.uk/.well-known/void"/>
</skos:Concept>
</skos:member>
<skos:member>
<skos:Concept rdf:about="http://vocab.nerc.ac.uk/collection/P35/current/EPC00176/">
<dc:identifier>SDN:P35::EPC00176</dc:identifier>
<dce:identifier>SDN:P35::EPC00176</dce:identifier>
<dc:date>2018-03-20 16:58:29.0</dc:date>
<skos:notation>SDN:P35::EPC00176</skos:notation>
<skos:prefLabel xml:lang="en">p,p'-DDT+DDD+DDE in Mytilus</skos:prefLabel>
<skos:altLabel>p,p'-DDT+DDD+DDE in Mytilus</skos:altLabel>
<skos:definition xml:lang="en">Concentration of p,p'-DDT+DDD+DDE per unit weight (dry or wet) of Mytilus spp. (regardless of Mytilus species and size class).</skos:definition>
<owl:versionInfo>7</owl:versionInfo>
<pav:hasCurrentVersion rdf:resource="http://vocab.nerc.ac.uk/collection/P35/current/EPC00176/7/"/>
<pav:version>7</pav:version>
<pav:authoredOn>2018-03-20 16:58:29.0</pav:authoredOn>
<skos:note xml:lang="en">deprecated</skos:note>
<owl:deprecated>true</owl:deprecated>
<skos:related rdf:resource="http://vocab.nerc.ac.uk/collection/P06/current/UUKG/"/>
<skos:broader rdf:resource="http://vocab.nerc.ac.uk/collection/P36/current/PESTBI/"/>
<void:inDataset rdf:resource="http://vocab.nerc.ac.uk/.well-known/void"/>
</skos:Concept>
</skos:member>
<skos:member>
<skos:Concept rdf:about="http://vocab.nerc.ac.uk/collection/P35/current/EPC00150/">
<dc:identifier>SDN:P35::EPC00150</dc:identifier>
<dce:identifier>SDN:P35::EPC00150</dce:identifier>
<dc:date>2016-12-12 15:20:45.0</dc:date>
<skos:notation>SDN:P35::EPC00150</skos:notation>
<skos:prefLabel xml:lang="en">p,p'-DDT+DDD+DDE in the sediment</skos:prefLabel>
<skos:altLabel>p,p'-DDT+DDD+DDE in the sediment</skos:altLabel>
<skos:definition xml:lang="en">Concentration of p,p'-DDT+DDD+DDE per unit dry weight of sediment (regardless of sediment size class).</skos:definition>
<owl:versionInfo>6</owl:versionInfo>
<pav:hasCurrentVersion rdf:resource="http://vocab.nerc.ac.uk/collection/P35/current/EPC00150/6/"/>
<pav:version>6</pav:version>
<pav:authoredOn>2016-12-12 15:20:45.0</pav:authoredOn>
<skos:note xml:lang="en">accepted</skos:note>
<owl:deprecated>false</owl:deprecated>
<skos:narrower rdf:resource="http://vocab.nerc.ac.uk/collection/P01/current/SED00009/"/>
<skos:related rdf:resource="http://vocab.nerc.ac.uk/collection/P06/current/UUKG/"/>
<skos:broader rdf:resource="http://vocab.nerc.ac.uk/collection/P36/current/PESTBI/"/>
<void:inDataset rdf:resource="http://vocab.nerc.ac.uk/.well-known/void"/>
</skos:Concept>
</skos:member>
<skos:member>
<skos:Concept rdf:about="http://vocab.nerc.ac.uk/collection/P35/current/EPC00136/">
<dc:identifier>SDN:P35::EPC00136</dc:identifier>
<dce:identifier>SDN:P35::EPC00136</dce:identifier>
<dc:date>2016-12-12 15:20:45.0</dc:date>
<skos:notation>SDN:P35::EPC00136</skos:notation>
<skos:prefLabel xml:lang="en">pH in the sediment</skos:prefLabel>
<skos:altLabel>pH in the sediment</skos:altLabel>
<skos:definition xml:lang="en">pH in sediment and sediment pore waters.</skos:definition>
<owl:versionInfo>5</owl:versionInfo>
<pav:hasCurrentVersion rdf:resource="http://vocab.nerc.ac.uk/collection/P35/current/EPC00136/5/"/>
<pav:version>5</pav:version>
<pav:authoredOn>2016-12-12 15:20:45.0</pav:authoredOn>
<skos:note xml:lang="en">accepted</skos:note>
<owl:deprecated>false</owl:deprecated>
<skos:narrower rdf:resource="http://vocab.nerc.ac.uk/collection/P01/current/PHNBSSPW/"/>
<skos:narrower rdf:resource="http://vocab.nerc.ac.uk/collection/P01/current/NEWCXX07/"/>
<skos:related rdf:resource="http://vocab.nerc.ac.uk/collection/P06/current/UUPH/"/>
<skos:broader rdf:resource="http://vocab.nerc.ac.uk/collection/P36/current/ACIDIT/"/>
<void:inDataset rdf:resource="http://vocab.nerc.ac.uk/.well-known/void"/>
</skos:Concept>
</skos:member>
</skos:Collection>
</rdf:RDF>
