<?xml version="1.0" encoding="UTF-8"?>
<rdf:RDF xmlns:rdf="http://www.w3.org/1999/02/22-rdf-syntax-ns#"
         xmlns:at="http://publications.europa.eu/ontology/authority/"
         xmlns:rdfs="http://www.w3.org/2000/01/rdf-schema#"
         xmlns:owl="http://www.w3.org/2002/07/owl#"
         xmlns:skos="http://www.w3.org/2004/02/skos/core#"
         xmlns:atold="http://publications.europa.eu/resource/authority/"
         xmlns:dc="http://purl.org/dc/elements/1.1/"
         xml:base="http://publications.europa.eu/resource/authority/licence">
   <skos:ConceptScheme rdf:about="http://publications.europa.eu/resource/authority/licence"
                       at:table.id="licence"
                       at:table.version.number="20230927-0">
      <at:prefLabel xml:lang="en">Licence</at:prefLabel>
      <rdfs:label xml:lang="en">Licence</rdfs:label>
      <owl:versionInfo>20230927-0</owl:versionInfo>
      <skos:prefLabel xml:lang="en">Licence</skos:prefLabel>
   </skos:ConceptScheme>
   <skos:Concept rdf:about="http://publications.europa.eu/resource/authority/licence/0BSD"
                 at:deprecated="false">
      <skos:prefLabel xml:lang="en">Zero-Clause BSD / Free Public License 1.0.0 (0BSD)</skos:prefLabel>
      <at:authority-code>0BSD</at:authority-code>
      <at:op-code>0BSD</at:op-code>
      <at:start.use>2006-07-01</at:start.use>
      <atold:op-code>0BSD</atold:op-code>
      <dc:identifier>0BSD</dc:identifier>
      <skos:altLabel xml:lang="bg">0BSD</skos:altLabel>
      <skos:altLabel xml:lang="cs">0BSD</skos:altLabel>
      <skos:altLabel xml:lang="da">0BSD</skos:altLabel>
      <skos:altLabel xml:lang="de">0BSD</skos:altLabel>
      <skos:altLabel xml:lang="el">0BSD</skos:altLabel>
      <skos:altLabel xml:lang="en">0BSD</skos:altLabel>
      <skos:altLabel xml:lang="es">0BSD</skos:altLabel>
      <skos:altLabel xml:lang="et">0BSD</skos:altLabel>
      <skos:altLabel xml:lang="fi">0BSD</skos:altLabel>
      <skos:altLabel xml:lang="fr">0BSD</skos:altLabel>
      <skos:altLabel xml:lang="ga">0BSD</skos:altLabel>
      <skos:altLabel xml:lang="hr">0BSD</skos:altLabel>
      <skos:altLabel xml:lang="hu">0BSD</skos:altLabel>
      <skos:altLabel xml:lang="it">0BSD</skos:altLabel>
      <skos:altLabel xml:lang="lt">0BSD</skos:altLabel>
      <skos:altLabel xml:lang="lv">0BSD</skos:altLabel>
      <skos:altLabel xml:lang="mt">0BSD</skos:altLabel>
      <skos:altLabel xml:lang="nl">0BSD</skos:altLabel>
      <skos:altLabel xml:lang="pl">0BSD</skos:altLabel>
      <skos:altLabel xml:lang="pt">0BSD</skos:altLabel>
      <skos:altLabel xml:lang="ro">0BSD</skos:altLabel>
      <skos:altLabel xml:lang="sk">0BSD</skos:altLabel>
      <skos:altLabel xml:lang="sl">0BSD</skos:altLabel>
      <skos:altLabel xml:lang="sv">0BSD</skos:altLabel>
      <skos:changeNote xml:lang="en">The source of the start-use date: https://spdx.org/licenses/0BSD.html</skos:changeNote>
      <skos:definition xml:lang="en">The BSD 0-clause licence, 0BSD, goes further than the 2-clause licence by dropping the requirements to include the copyright notice, licence text or disclaimer in either source or binary forms. Doing so forms a public-domain-equivalent licence. It is approved by the Open Source Initiative.</skos:definition>
      <skos:exactMatch rdf:resource="https://opensource.org/licenses/0BSD"/>
      <skos:inScheme rdf:resource="http://publications.europa.eu/resource/authority/licence"/>
      <skos:topConceptOf rdf:resource="http://publications.europa.eu/resource/authority/licence"/>
   </skos:Concept>
   <skos:Concept rdf:about="http://publications.europa.eu/resource/authority/licence/AGPL_3_0"
                 at:deprecated="false">
      <skos:prefLabel xml:lang="en">GNU Affero General Public License version 3</skos:prefLabel>
      <at:authority-code>AGPL_3_0</at:authority-code>
      <at:op-code>AGPL_3_0</at:op-code>
      <at:start.use>2007-11-19</at:start.use>
      <atold:op-code>AGPL_3_0</atold:op-code>
      <dc:identifier>AGPL_3_0</dc:identifier>
      <skos:altLabel xml:lang="bg">AGPL-3.0</skos:altLabel>
      <skos:altLabel xml:lang="cs">AGPL-3.0</skos:altLabel>
      <skos:altLabel xml:lang="da">AGPL-3.0</skos:altLabel>
      <skos:altLabel xml:lang="de">AGPL-3.0</skos:altLabel>
      <skos:altLabel xml:lang="el">AGPL-3.0</skos:altLabel>
      <skos:altLabel xml:lang="en">AGPL-3.0</skos:altLabel>
      <skos:altLabel xml:lang="es">AGPL-3.0</skos:altLabel>
      <skos:altLabel xml:lang="et">AGPL-3.0</skos:altLabel>
      <skos:altLabel xml:lang="fi">AGPL-3.0</skos:altLabel>
      <skos:altLabel xml:lang="fr">AGPL-3.0</skos:altLabel>
      <skos:altLabel xml:lang="ga">AGPL-3.0</skos:altLabel>
      <skos:altLabel xml:lang="hr">AGPL-3.0</skos:altLabel>
      <skos:altLabel xml:lang="hu">AGPL-3.0</skos:altLabel>
      <skos:altLabel xml:lang="it">AGPL-3.0</skos:altLabel>
      <skos:altLabel xml:lang="lt">AGPL-3.0</skos:altLabel>
      <skos:altLabel xml:lang="lv">AGPL-3.0</skos:altLabel>
      <skos:altLabel xml:lang="mt">AGPL-3.0</skos:altLabel>
      <skos:altLabel xml:lang="nl">AGPL-3.0</skos:altLabel>
      <skos:altLabel xml:lang="pl">AGPL-3.0</skos:altLabel>
      <skos:altLabel xml:lang="pt">AGPL-3.0</skos:altLabel>
      <skos:altLabel xml:lang="ro">AGPL-3.0</skos:altLabel>
      <skos:altLabel xml:lang="sk">AGPL-3.0</skos:altLabel>
      <skos:altLabel xml:lang="sl">AGPL-3.0</skos:altLabel>
      <skos:altLabel xml:lang="sv">AGPL-3.0</skos:altLabel>
      <skos:changeNote xml:lang="en">The source of the start-use date: https://en.wikipedia.org/wiki/Affero_General_Public_License</skos:changeNote>
      <skos:definition xml:lang="en">AGPL-3.0 is a modified GPL-3.0 extended to network or Web services distribution (SaaS). Strong copyleft: copies and derivatives may be distributed under the same AGPL only. Need to document derivatives’ changes and dates. Incompatible with other licences except linking with code covered by the original GPL-3.0.</skos:definition>
      <skos:exactMatch rdf:resource="https://opensource.org/licenses/AGPL-3.0"/>
      <skos:inScheme rdf:resource="http://publications.europa.eu/resource/authority/licence"/>
      <skos:topConceptOf rdf:resource="http://publications.europa.eu/resource/authority/licence"/>
   </skos:Concept>
   <skos:Concept rdf:about="http://publications.europa.eu/resource/authority/licence/APACHE_1_1"
                 at:deprecated="true">
      <skos:prefLabel xml:lang="en">Apache Software License, version 1.1 (Apache-1.1)</skos:prefLabel>
      <skos:prefLabel xml:lang="et">Apache tarkvara litsents, versioon 1.1 (Apache-1.1)</skos:prefLabel>
      <at:authority-code>APACHE_1_1</at:authority-code>
      <at:op-code>APACHE_1_1</at:op-code>
      <at:start.use>2000-01-01</at:start.use>
      <atold:op-code>APACHE_1_1</atold:op-code>
      <dc:identifier>APACHE_1_1</dc:identifier>
      <skos:altLabel xml:lang="bg">Apache 1.1</skos:altLabel>
      <skos:altLabel xml:lang="cs">Apache 1.1</skos:altLabel>
      <skos:altLabel xml:lang="da">Apache 1.1</skos:altLabel>
      <skos:altLabel xml:lang="de">Apache 1.1</skos:altLabel>
      <skos:altLabel xml:lang="el">Apache 1.1</skos:altLabel>
      <skos:altLabel xml:lang="en">Apache 1.1</skos:altLabel>
      <skos:altLabel xml:lang="es">Apache 1.1</skos:altLabel>
      <skos:altLabel xml:lang="et">Apache 1.1</skos:altLabel>
      <skos:altLabel xml:lang="fi">Apache 1.1</skos:altLabel>
      <skos:altLabel xml:lang="fr">Apache 1.1</skos:altLabel>
      <skos:altLabel xml:lang="ga">Apache 1.1</skos:altLabel>
      <skos:altLabel xml:lang="hr">Apache 1.1</skos:altLabel>
      <skos:altLabel xml:lang="hu">Apache 1.1</skos:altLabel>
      <skos:altLabel xml:lang="it">Apache 1.1</skos:altLabel>
      <skos:altLabel xml:lang="lt">Apache 1.1</skos:altLabel>
      <skos:altLabel xml:lang="lv">Apache 1.1</skos:altLabel>
      <skos:altLabel xml:lang="mt">Apache 1.1</skos:altLabel>
      <skos:altLabel xml:lang="nl">Apache 1.1</skos:altLabel>
      <skos:altLabel xml:lang="pl">Apache 1.1</skos:altLabel>
      <skos:altLabel xml:lang="pt">Apache 1.1</skos:altLabel>
      <skos:altLabel xml:lang="ro">Apache 1.1</skos:altLabel>
      <skos:altLabel xml:lang="sk">Apache 1.1</skos:altLabel>
      <skos:altLabel xml:lang="sl">Apache 1.1</skos:altLabel>
      <skos:altLabel xml:lang="sv">Apache 1.1</skos:altLabel>
      <skos:changeNote xml:lang="en">The source of the start-use date: https://opensource.org/licenses/Apache-1.1</skos:changeNote>
      <skos:definition xml:lang="en">Apache-1.1 is a permissive free software licence approved by the Open Source Initiative. It is superseded by Apache-2.0.</skos:definition>
      <skos:exactMatch rdf:resource="https://opensource.org/licenses/Apache-1.1"/>
      <skos:inScheme rdf:resource="http://publications.europa.eu/resource/authority/licence"/>
      <skos:topConceptOf rdf:resource="http://publications.europa.eu/resource/authority/licence"/>
      <at:end.use>2004-01-01</at:end.use>
   </skos:Concept>
   <skos:Concept rdf:about="http://publications.europa.eu/resource/authority/licence/APACHE_2_0"
                 at:deprecated="false">
      <skos:prefLabel xml:lang="en">Apache License, Version 2.0</skos:prefLabel>
      <skos:prefLabel xml:lang="et">Apache litsents, versioon 2.0</skos:prefLabel>
      <at:authority-code>APACHE_2_0</at:authority-code>
      <at:op-code>APACHE_2_0</at:op-code>
      <at:start.use>2004-01-02</at:start.use>
      <atold:op-code>APACHE_2_0</atold:op-code>
      <dc:identifier>APACHE_2_0</dc:identifier>
      <skos:altLabel xml:lang="bg">Apache 2.0</skos:altLabel>
      <skos:altLabel xml:lang="cs">Apache 2.0</skos:altLabel>
      <skos:altLabel xml:lang="da">Apache 2.0</skos:altLabel>
      <skos:altLabel xml:lang="de">Apache 2.0</skos:altLabel>
      <skos:altLabel xml:lang="el">Apache 2.0</skos:altLabel>
      <skos:altLabel xml:lang="en">Apache 2.0</skos:altLabel>
      <skos:altLabel xml:lang="es">Apache 2.0</skos:altLabel>
      <skos:altLabel xml:lang="et">Apache 2.0</skos:altLabel>
      <skos:altLabel xml:lang="fi">Apache 2.0</skos:altLabel>
      <skos:altLabel xml:lang="fr">Apache 2.0</skos:altLabel>
      <skos:altLabel xml:lang="ga">Apache 2.0</skos:altLabel>
      <skos:altLabel xml:lang="hr">Apache 2.0</skos:altLabel>
      <skos:altLabel xml:lang="hu">Apache 2.0</skos:altLabel>
      <skos:altLabel xml:lang="it">Apache 2.0</skos:altLabel>
      <skos:altLabel xml:lang="lt">Apache 2.0</skos:altLabel>
      <skos:altLabel xml:lang="lv">Apache 2.0</skos:altLabel>
      <skos:altLabel xml:lang="mt">Apache 2.0</skos:altLabel>
      <skos:altLabel xml:lang="nl">Apache 2.0</skos:altLabel>
      <skos:altLabel xml:lang="pl">Apache 2.0</skos:altLabel>
      <skos:altLabel xml:lang="pt">Apache 2.0</skos:altLabel>
      <skos:altLabel xml:lang="ro">Apache 2.0</skos:altLabel>
      <skos:altLabel xml:lang="sk">Apache 2.0</skos:altLabel>
      <skos:altLabel xml:lang="sl">Apache 2.0</skos:altLabel>
      <skos:altLabel xml:lang="sv">Apache 2.0</skos:altLabel>
      <skos:changeNote xml:lang="en">The source of the start-use date: https://opensource.org/licenses/Apache-2.0</skos:changeNote>
      <skos:definition xml:lang="en">Apache-2.0 is a permissive free software licence approved by the Open Source Initiative. It gives complete freedom to use the given works, as long as the required notices are included. Compared with the MIT, recipients receive a patent licence from the contributors of the code.</skos:definition>
      <skos:exactMatch rdf:resource="https://opensource.org/licenses/Apache-2.0"/>
      <skos:inScheme rdf:resource="http://publications.europa.eu/resource/authority/licence"/>
      <skos:topConceptOf rdf:resource="http://publications.europa.eu/resource/authority/licence"/>
   </skos:Concept>
   <skos:Concept rdf:about="http://publications.europa.eu/resource/authority/licence/APL_1_0"
                 at:deprecated="false">
      <skos:prefLabel xml:lang="en">Adaptive Public License 1.0</skos:prefLabel>
      <at:authority-code>APL_1_0</at:authority-code>
      <at:op-code>APL_1_0</at:op-code>
      <at:start.use>2003-07-01</at:start.use>
      <atold:op-code>APL_1_0</atold:op-code>
      <dc:identifier>APL_1_0</dc:identifier>
      <skos:altLabel xml:lang="bg">APL-1.0</skos:altLabel>
      <skos:altLabel xml:lang="cs">APL-1.0</skos:altLabel>
      <skos:altLabel xml:lang="da">APL-1.0</skos:altLabel>
      <skos:altLabel xml:lang="de">APL-1.0</skos:altLabel>
      <skos:altLabel xml:lang="el">APL-1.0</skos:altLabel>
      <skos:altLabel xml:lang="en">APL-1.0</skos:altLabel>
      <skos:altLabel xml:lang="es">APL-1.0</skos:altLabel>
      <skos:altLabel xml:lang="et">APL-1.0</skos:altLabel>
      <skos:altLabel xml:lang="fi">APL-1.0</skos:altLabel>
      <skos:altLabel xml:lang="fr">APL-1.0</skos:altLabel>
      <skos:altLabel xml:lang="ga">APL-1.0</skos:altLabel>
      <skos:altLabel xml:lang="hr">APL-1.0</skos:altLabel>
      <skos:altLabel xml:lang="hu">APL-1.0</skos:altLabel>
      <skos:altLabel xml:lang="it">APL-1.0</skos:altLabel>
      <skos:altLabel xml:lang="lt">APL-1.0</skos:altLabel>
      <skos:altLabel xml:lang="lv">APL-1.0</skos:altLabel>
      <skos:altLabel xml:lang="mt">APL-1.0</skos:altLabel>
      <skos:altLabel xml:lang="nl">APL-1.0</skos:altLabel>
      <skos:altLabel xml:lang="pl">APL-1.0</skos:altLabel>
      <skos:altLabel xml:lang="pt">APL-1.0</skos:altLabel>
      <skos:altLabel xml:lang="ro">APL-1.0</skos:altLabel>
      <skos:altLabel xml:lang="sk">APL-1.0</skos:altLabel>
      <skos:altLabel xml:lang="sl">APL-1.0</skos:altLabel>
      <skos:altLabel xml:lang="sv">APL-1.0</skos:altLabel>
      <skos:changeNote xml:lang="en">The source of the start-use date: http://www.worldlii.org/int/other/PubRL/2009/1.html</skos:changeNote>
      <skos:definition xml:lang="en">APL-1.0 is a copyleft-style, free software licence approved by the Open Source Initiative. It allows combining the covered code with other components not governed by the APL licence provided the APL requirements are fulfilled for the covered portion of the larger work.</skos:definition>
      <skos:exactMatch rdf:resource="https://opensource.org/licenses/APL-1.0"/>
      <skos:inScheme rdf:resource="http://publications.europa.eu/resource/authority/licence"/>
      <skos:topConceptOf rdf:resource="http://publications.europa.eu/resource/authority/licence"/>
   </skos:Concept>
   <skos:Concept rdf:about="http://publications.europa.eu/resource/authority/licence/APSL_2_0"
                 at:deprecated="false">
      <skos:prefLabel xml:lang="en">Apple Public Source License 2.0</skos:prefLabel>
      <at:authority-code>APSL_2_0</at:authority-code>
      <at:op-code>APSL_2_0</at:op-code>
      <at:start.use>2003-08-06</at:start.use>
      <atold:op-code>APSL_2_0</atold:op-code>
      <dc:identifier>APSL_2_0</dc:identifier>
      <skos:altLabel xml:lang="bg">APSL-2.0</skos:altLabel>
      <skos:altLabel xml:lang="cs">APSL-2.0</skos:altLabel>
      <skos:altLabel xml:lang="da">APSL-2.0</skos:altLabel>
      <skos:altLabel xml:lang="de">APSL-2.0</skos:altLabel>
      <skos:altLabel xml:lang="el">APSL-2.0</skos:altLabel>
      <skos:altLabel xml:lang="en">APSL-2.0</skos:altLabel>
      <skos:altLabel xml:lang="es">APSL-2.0</skos:altLabel>
      <skos:altLabel xml:lang="et">APSL-2.0</skos:altLabel>
      <skos:altLabel xml:lang="fi">APSL-2.0</skos:altLabel>
      <skos:altLabel xml:lang="fr">APSL-2.0</skos:altLabel>
      <skos:altLabel xml:lang="ga">APSL-2.0</skos:altLabel>
      <skos:altLabel xml:lang="hr">APSL-2.0</skos:altLabel>
      <skos:altLabel xml:lang="hu">APSL-2.0</skos:altLabel>
      <skos:altLabel xml:lang="it">APSL-2.0</skos:altLabel>
      <skos:altLabel xml:lang="lt">APSL-2.0</skos:altLabel>
      <skos:altLabel xml:lang="lv">APSL-2.0</skos:altLabel>
      <skos:altLabel xml:lang="mt">APSL-2.0</skos:altLabel>
      <skos:altLabel xml:lang="nl">APSL-2.0</skos:altLabel>
      <skos:altLabel xml:lang="pl">APSL-2.0</skos:altLabel>
      <skos:altLabel xml:lang="pt">APSL-2.0</skos:altLabel>
      <skos:altLabel xml:lang="ro">APSL-2.0</skos:altLabel>
      <skos:altLabel xml:lang="sk">APSL-2.0</skos:altLabel>
      <skos:altLabel xml:lang="sl">APSL-2.0</skos:altLabel>
      <skos:altLabel xml:lang="sv">APSL-2.0</skos:altLabel>
      <skos:changeNote xml:lang="en">The source of the start-use date: https://en.wikipedia.org/wiki/Apple_Public_Source_License</skos:changeNote>
      <skos:definition xml:lang="en">APSL-2.0 is a copyleft-style, free software licence approved by the Open Source Initiative. Under this licence, it is possible to create a larger work by combining covered code with other code not governed by the terms of this licence and distribute the larger work as a single product. In each such instance, it must be ensured that requirements of this licence are fulfilled for the covered code or any portion thereof.</skos:definition>
      <skos:exactMatch rdf:resource="https://opensource.org/licenses/APSL-2.0"/>
      <skos:inScheme rdf:resource="http://publications.europa.eu/resource/authority/licence"/>
      <skos:topConceptOf rdf:resource="http://publications.europa.eu/resource/authority/licence"/>
   </skos:Concept>
   <skos:Concept rdf:about="http://publications.europa.eu/resource/authority/licence/ARTISTIC_1_0"
                 at:deprecated="true">
      <skos:prefLabel xml:lang="en">Artistic License 1.0 (Artistic-1.0)</skos:prefLabel>
      <at:authority-code>ARTISTIC_1_0</at:authority-code>
      <at:op-code>ARTISTIC_1_0</at:op-code>
      <at:start.use>1997-08-15</at:start.use>
      <atold:op-code>ARTISTIC_1_0</atold:op-code>
      <dc:identifier>ARTISTIC_1_0</dc:identifier>
      <skos:altLabel xml:lang="bg">Artistic 1.0</skos:altLabel>
      <skos:altLabel xml:lang="cs">Artistic 1.0</skos:altLabel>
      <skos:altLabel xml:lang="da">Artistic 1.0</skos:altLabel>
      <skos:altLabel xml:lang="de">Artistic 1.0</skos:altLabel>
      <skos:altLabel xml:lang="el">Artistic 1.0</skos:altLabel>
      <skos:altLabel xml:lang="en">Artistic 1.0</skos:altLabel>
      <skos:altLabel xml:lang="es">Artistic 1.0</skos:altLabel>
      <skos:altLabel xml:lang="et">Artistic 1.0</skos:altLabel>
      <skos:altLabel xml:lang="fi">Artistic 1.0</skos:altLabel>
      <skos:altLabel xml:lang="fr">Artistic 1.0</skos:altLabel>
      <skos:altLabel xml:lang="ga">Artistic 1.0</skos:altLabel>
      <skos:altLabel xml:lang="hr">Artistic 1.0</skos:altLabel>
      <skos:altLabel xml:lang="hu">Artistic 1.0</skos:altLabel>
      <skos:altLabel xml:lang="it">Artistic 1.0</skos:altLabel>
      <skos:altLabel xml:lang="lt">Artistic 1.0</skos:altLabel>
      <skos:altLabel xml:lang="lv">Artistic 1.0</skos:altLabel>
      <skos:altLabel xml:lang="mt">Artistic 1.0</skos:altLabel>
      <skos:altLabel xml:lang="nl">Artistic 1.0</skos:altLabel>
      <skos:altLabel xml:lang="pl">Artistic 1.0</skos:altLabel>
      <skos:altLabel xml:lang="pt">Artistic 1.0</skos:altLabel>
      <skos:altLabel xml:lang="ro">Artistic 1.0</skos:altLabel>
      <skos:altLabel xml:lang="sk">Artistic 1.0</skos:altLabel>
      <skos:altLabel xml:lang="sl">Artistic 1.0</skos:altLabel>
      <skos:altLabel xml:lang="sv">Artistic 1.0</skos:altLabel>
      <skos:changeNote xml:lang="en">The source of the start-use date: https://wiki.vvlibri.org/index.php?title=Artistic_License_Version_2.0</skos:changeNote>
      <skos:definition xml:lang="en">Artistic-1.0 is a copyleft-style, free software licence approved by the Open Source Initiative. It is superseded by Artistic 2.0.</skos:definition>
      <skos:exactMatch rdf:resource="https://opensource.org/licenses/Artistic-1.0"/>
      <skos:inScheme rdf:resource="http://publications.europa.eu/resource/authority/licence"/>
      <skos:topConceptOf rdf:resource="http://publications.europa.eu/resource/authority/licence"/>
      <at:end.use>2000-06-30</at:end.use>
   </skos:Concept>
   <skos:Concept rdf:about="http://publications.europa.eu/resource/authority/licence/ARTISTIC_2_0"
                 at:deprecated="false">
      <skos:prefLabel xml:lang="en">Artistic License 2.0</skos:prefLabel>
      <at:authority-code>ARTISTIC_2_0</at:authority-code>
      <at:op-code>ARTISTIC_2_0</at:op-code>
      <at:start.use>2000-07-01</at:start.use>
      <atold:op-code>ARTISTIC_2_0</atold:op-code>
      <dc:identifier>ARTISTIC_2_0</dc:identifier>
      <skos:altLabel xml:lang="bg">Artistic 2.0</skos:altLabel>
      <skos:altLabel xml:lang="cs">Artistic 2.0</skos:altLabel>
      <skos:altLabel xml:lang="da">Artistic 2.0</skos:altLabel>
      <skos:altLabel xml:lang="de">Artistic 2.0</skos:altLabel>
      <skos:altLabel xml:lang="el">Artistic 2.0</skos:altLabel>
      <skos:altLabel xml:lang="en">Artistic 2.0</skos:altLabel>
      <skos:altLabel xml:lang="es">Artistic 2.0</skos:altLabel>
      <skos:altLabel xml:lang="et">Artistic 2.0</skos:altLabel>
      <skos:altLabel xml:lang="fi">Artistic 2.0</skos:altLabel>
      <skos:altLabel xml:lang="fr">Artistic 2.0</skos:altLabel>
      <skos:altLabel xml:lang="ga">Artistic 2.0</skos:altLabel>
      <skos:altLabel xml:lang="hr">Artistic 2.0</skos:altLabel>
      <skos:altLabel xml:lang="hu">Artistic 2.0</skos:altLabel>
      <skos:altLabel xml:lang="it">Artistic 2.0</skos:altLabel>
      <skos:altLabel xml:lang="lt">Artistic 2.0</skos:altLabel>
      <skos:altLabel xml:lang="lv">Artistic 2.0</skos:altLabel>
      <skos:altLabel xml:lang="mt">Artistic 2.0</skos:altLabel>
      <skos:altLabel xml:lang="nl">Artistic 2.0</skos:altLabel>
      <skos:altLabel xml:lang="pl">Artistic 2.0</skos:altLabel>
      <skos:altLabel xml:lang="pt">Artistic 2.0</skos:altLabel>
      <skos:altLabel xml:lang="ro">Artistic 2.0</skos:altLabel>
      <skos:altLabel xml:lang="sk">Artistic 2.0</skos:altLabel>
      <skos:altLabel xml:lang="sl">Artistic 2.0</skos:altLabel>
      <skos:altLabel xml:lang="sv">Artistic 2.0</skos:altLabel>
      <skos:changeNote xml:lang="en">The source of the start-use date: https://www.appropedia.org/Open_software_licenses; http://www.linfo.org/artistic.html</skos:changeNote>
      <skos:definition xml:lang="en">Artistic-2.0 is a copyleft-style, free software licence approved by the Open Source Initiative. It preserves control of the original copyright holder: recipient can use, modify and distribute the original versions but other modified versions must document how far they are different and be reported to the original author, or be distributed under a different name, or otherwise be available under the Artistic licence or any other licence granting similar rights.</skos:definition>
      <skos:exactMatch rdf:resource="https://opensource.org/licenses/Artistic-2.0"/>
      <skos:inScheme rdf:resource="http://publications.europa.eu/resource/authority/licence"/>
      <skos:topConceptOf rdf:resource="http://publications.europa.eu/resource/authority/licence"/>
   </skos:Concept>
   <skos:Concept rdf:about="http://publications.europa.eu/resource/authority/licence/BSD_2_CLAUSE"
                 at:deprecated="false">
      <skos:prefLabel xml:lang="en">2-Clause BSD License</skos:prefLabel>
      <at:authority-code>BSD_2_CLAUSE</at:authority-code>
      <at:op-code>BSD_2_CLAUSE</at:op-code>
      <at:start.use>1999-04-01</at:start.use>
      <atold:op-code>BSD_2_CLAUSE</atold:op-code>
      <dc:identifier>BSD_2_CLAUSE</dc:identifier>
      <skos:altLabel xml:lang="bg">BSD-2-Clause</skos:altLabel>
      <skos:altLabel xml:lang="cs">BSD-2-Clause</skos:altLabel>
      <skos:altLabel xml:lang="da">BSD-2-Clause</skos:altLabel>
      <skos:altLabel xml:lang="de">BSD-2-Clause</skos:altLabel>
      <skos:altLabel xml:lang="el">BSD-2-Clause</skos:altLabel>
      <skos:altLabel xml:lang="en">BSD-2-Clause</skos:altLabel>
      <skos:altLabel xml:lang="es">BSD-2-Clause</skos:altLabel>
      <skos:altLabel xml:lang="et">BSD-2-Clause</skos:altLabel>
      <skos:altLabel xml:lang="fi">BSD-2-Clause</skos:altLabel>
      <skos:altLabel xml:lang="fr">BSD-2-Clause</skos:altLabel>
      <skos:altLabel xml:lang="ga">BSD-2-Clause</skos:altLabel>
      <skos:altLabel xml:lang="hr">BSD-2-Clause</skos:altLabel>
      <skos:altLabel xml:lang="hu">BSD-2-Clause</skos:altLabel>
      <skos:altLabel xml:lang="it">BSD-2-Clause</skos:altLabel>
      <skos:altLabel xml:lang="lt">BSD-2-Clause</skos:altLabel>
      <skos:altLabel xml:lang="lv">BSD-2-Clause</skos:altLabel>
      <skos:altLabel xml:lang="mt">BSD-2-Clause</skos:altLabel>
      <skos:altLabel xml:lang="nl">BSD-2-Clause</skos:altLabel>
      <skos:altLabel xml:lang="pl">BSD-2-Clause</skos:altLabel>
      <skos:altLabel xml:lang="pt">BSD-2-Clause</skos:altLabel>
      <skos:altLabel xml:lang="ro">BSD-2-Clause</skos:altLabel>
      <skos:altLabel xml:lang="sk">BSD-2-Clause</skos:altLabel>
      <skos:altLabel xml:lang="sl">BSD-2-Clause</skos:altLabel>
      <skos:altLabel xml:lang="sv">BSD-2-Clause</skos:altLabel>
      <skos:changeNote xml:lang="en">The source of the start-use date: https://en.wikipedia.org/wiki/BSD_licenses</skos:changeNote>
      <skos:definition xml:lang="en">BSD-2-Clause permits redistribution and use in source and binary forms, with or without modification, provided that the certain conditions are met: redistributions of source code must retain the copyright notice, the specific list of conditions and the disclaimer.</skos:definition>
      <skos:exactMatch rdf:resource="https://opensource.org/licenses/BSD-2-Clause"/>
      <skos:inScheme rdf:resource="http://publications.europa.eu/resource/authority/licence"/>
      <skos:topConceptOf rdf:resource="http://publications.europa.eu/resource/authority/licence"/>
   </skos:Concept>
   <skos:Concept rdf:about="http://publications.europa.eu/resource/authority/licence/BSD_3_CLAUSE"
                 at:deprecated="false">
      <skos:prefLabel xml:lang="en">3-Clause BSD License</skos:prefLabel>
      <at:authority-code>BSD_3_CLAUSE</at:authority-code>
      <at:op-code>BSD_3_CLAUSE</at:op-code>
      <at:start.use>1999-07-22</at:start.use>
      <atold:op-code>BSD_3_CLAUSE</atold:op-code>
      <dc:identifier>BSD_3_CLAUSE</dc:identifier>
      <skos:altLabel xml:lang="bg">BSD-3-Clause</skos:altLabel>
      <skos:altLabel xml:lang="cs">BSD-3-Clause</skos:altLabel>
      <skos:altLabel xml:lang="da">BSD-3-Clause</skos:altLabel>
      <skos:altLabel xml:lang="de">BSD-3-Clause</skos:altLabel>
      <skos:altLabel xml:lang="el">BSD-3-Clause</skos:altLabel>
      <skos:altLabel xml:lang="en">BSD-3-Clause</skos:altLabel>
      <skos:altLabel xml:lang="es">BSD-3-Clause</skos:altLabel>
      <skos:altLabel xml:lang="et">BSD-3-Clause</skos:altLabel>
      <skos:altLabel xml:lang="fi">BSD-3-Clause</skos:altLabel>
      <skos:altLabel xml:lang="fr">BSD-3-Clause</skos:altLabel>
      <skos:altLabel xml:lang="ga">BSD-3-Clause</skos:altLabel>
      <skos:altLabel xml:lang="hr">BSD-3-Clause</skos:altLabel>
      <skos:altLabel xml:lang="hu">BSD-3-Clause</skos:altLabel>
      <skos:altLabel xml:lang="it">BSD-3-Clause</skos:altLabel>
      <skos:altLabel xml:lang="lt">BSD-3-Clause</skos:altLabel>
      <skos:altLabel xml:lang="lv">BSD-3-Clause</skos:altLabel>
      <skos:altLabel xml:lang="mt">BSD-3-Clause</skos:altLabel>
      <skos:altLabel xml:lang="nl">BSD-3-Clause</skos:altLabel>
      <skos:altLabel xml:lang="pl">BSD-3-Clause</skos:altLabel>
      <skos:altLabel xml:lang="pt">BSD-3-Clause</skos:altLabel>
      <skos:altLabel xml:lang="ro">BSD-3-Clause</skos:altLabel>
      <skos:altLabel xml:lang="sk">BSD-3-Clause</skos:altLabel>
      <skos:altLabel xml:lang="sl">BSD-3-Clause</skos:altLabel>
      <skos:altLabel xml:lang="sv">BSD-3-Clause</skos:altLabel>
      <skos:changeNote xml:lang="en">The source of the start-use date: https://en.wikipedia.org/wiki/BSD_licenses</skos:changeNote>
      <skos:definition xml:lang="en">BSD-3-Clause permits redistribution and use in source and binary forms, with or without modification, provided that the certain conditions are met: redistributions of source code and in binary forms must retain the copyright notice, the specific list of conditions and the disclaimer. Neither the name of the copyright holder nor of its contributors may be used to promote derived products without prior written permission.</skos:definition>
      <skos:exactMatch rdf:resource="https://opensource.org/licenses/BSD-3-Clause"/>
      <skos:inScheme rdf:resource="http://publications.europa.eu/resource/authority/licence"/>
      <skos:topConceptOf rdf:resource="http://publications.europa.eu/resource/authority/licence"/>
   </skos:Concept>
   <skos:Concept rdf:about="http://publications.europa.eu/resource/authority/licence/BSD_3_CLAUSE_LBNL"
                 at:deprecated="false">
      <skos:prefLabel xml:lang="en">Lawrence Berkeley National Labs BSD Variant License (BSD-3-Clause-LBNL)</skos:prefLabel>
      <at:authority-code>BSD_3_CLAUSE_LBNL</at:authority-code>
      <at:op-code>BSD_3_CLAUSE_LBNL</at:op-code>
      <at:start.use>2002-07-01</at:start.use>
      <atold:op-code>BSD_3_CLAUSE_LBNL</atold:op-code>
      <dc:identifier>BSD_3_CLAUSE_LBNL</dc:identifier>
      <skos:altLabel xml:lang="bg">BSD-3-Clause-LBNL</skos:altLabel>
      <skos:altLabel xml:lang="cs">BSD-3-Clause-LBNL</skos:altLabel>
      <skos:altLabel xml:lang="da">BSD-3-Clause-LBNL</skos:altLabel>
      <skos:altLabel xml:lang="de">BSD-3-Clause-LBNL</skos:altLabel>
      <skos:altLabel xml:lang="el">BSD-3-Clause-LBNL</skos:altLabel>
      <skos:altLabel xml:lang="en">BSD-3-Clause-LBNL</skos:altLabel>
      <skos:altLabel xml:lang="es">BSD-3-Clause-LBNL</skos:altLabel>
      <skos:altLabel xml:lang="et">BSD-3-Clause-LBNL</skos:altLabel>
      <skos:altLabel xml:lang="fi">BSD-3-Clause-LBNL</skos:altLabel>
      <skos:altLabel xml:lang="fr">BSD-3-Clause-LBNL</skos:altLabel>
      <skos:altLabel xml:lang="ga">BSD-3-Clause-LBNL</skos:altLabel>
      <skos:altLabel xml:lang="hr">BSD-3-Clause-LBNL</skos:altLabel>
      <skos:altLabel xml:lang="hu">BSD-3-Clause-LBNL</skos:altLabel>
      <skos:altLabel xml:lang="it">BSD-3-Clause-LBNL</skos:altLabel>
      <skos:altLabel xml:lang="lt">BSD-3-Clause-LBNL</skos:altLabel>
      <skos:altLabel xml:lang="lv">BSD-3-Clause-LBNL</skos:altLabel>
      <skos:altLabel xml:lang="mt">BSD-3-Clause-LBNL</skos:altLabel>
      <skos:altLabel xml:lang="nl">BSD-3-Clause-LBNL</skos:altLabel>
      <skos:altLabel xml:lang="pl">BSD-3-Clause-LBNL</skos:altLabel>
      <skos:altLabel xml:lang="pt">BSD-3-Clause-LBNL</skos:altLabel>
      <skos:altLabel xml:lang="ro">BSD-3-Clause-LBNL</skos:altLabel>
      <skos:altLabel xml:lang="sk">BSD-3-Clause-LBNL</skos:altLabel>
      <skos:altLabel xml:lang="sl">BSD-3-Clause-LBNL</skos:altLabel>
      <skos:altLabel xml:lang="sv">BSD-3-Clause-LBNL</skos:altLabel>
      <skos:changeNote xml:lang="en">The source of the start-use date: https://enterprise.dejacode.com/licenses/public/lbnl-bsd/?_list_filters=q%3Dbsd#essentials</skos:changeNote>
      <skos:definition xml:lang="en">BSD-3-Clause-LBNL is a BSD-style, permissive free software licence approved by the Open Source Initiative.</skos:definition>
      <skos:exactMatch rdf:resource="https://opensource.org/licenses/BSD-3-Clause-LBNL"/>
      <skos:inScheme rdf:resource="http://publications.europa.eu/resource/authority/licence"/>
      <skos:topConceptOf rdf:resource="http://publications.europa.eu/resource/authority/licence"/>
   </skos:Concept>
   <skos:Concept rdf:about="http://publications.europa.eu/resource/authority/licence/BSD_PLUS_PATENT"
                 at:deprecated="false">
      <skos:prefLabel xml:lang="en">BSD+Patent</skos:prefLabel>
      <at:authority-code>BSD_PLUS_PATENT</at:authority-code>
      <at:op-code>BSD_PLUS_PATENT</at:op-code>
      <at:start.use>2017-07-01</at:start.use>
      <atold:op-code>BSD_PLUS_PATENT</atold:op-code>
      <dc:identifier>BSD_PLUS_PATENT</dc:identifier>
      <skos:altLabel xml:lang="bg">BSD+Patent</skos:altLabel>
      <skos:altLabel xml:lang="cs">BSD+Patent</skos:altLabel>
      <skos:altLabel xml:lang="da">BSD+Patent</skos:altLabel>
      <skos:altLabel xml:lang="de">BSD+Patent</skos:altLabel>
      <skos:altLabel xml:lang="el">BSD+Patent</skos:altLabel>
      <skos:altLabel xml:lang="es">BSD+Patent</skos:altLabel>
      <skos:altLabel xml:lang="et">BSD+Patent</skos:altLabel>
      <skos:altLabel xml:lang="fi">BSD+Patent</skos:altLabel>
      <skos:altLabel xml:lang="fr">BSD+Patent</skos:altLabel>
      <skos:altLabel xml:lang="ga">BSD+Patent</skos:altLabel>
      <skos:altLabel xml:lang="hr">BSD+Patent</skos:altLabel>
      <skos:altLabel xml:lang="hu">BSD+Patent</skos:altLabel>
      <skos:altLabel xml:lang="it">BSD+Patent</skos:altLabel>
      <skos:altLabel xml:lang="lt">BSD+Patent</skos:altLabel>
      <skos:altLabel xml:lang="lv">BSD+Patent</skos:altLabel>
      <skos:altLabel xml:lang="mt">BSD+Patent</skos:altLabel>
      <skos:altLabel xml:lang="nl">BSD+Patent</skos:altLabel>
      <skos:altLabel xml:lang="pl">BSD+Patent</skos:altLabel>
      <skos:altLabel xml:lang="pt">BSD+Patent</skos:altLabel>
      <skos:altLabel xml:lang="ro">BSD+Patent</skos:altLabel>
      <skos:altLabel xml:lang="sk">BSD+Patent</skos:altLabel>
      <skos:altLabel xml:lang="sl">BSD+Patent</skos:altLabel>
      <skos:altLabel xml:lang="sv">BSD+Patent</skos:altLabel>
      <skos:changeNote xml:lang="en">The source of the start-use date: https://enterprise.dejacode.com/licenses/public/bsd-plus-patent/?_list_filters=q%3Dbsd#essentials</skos:changeNote>
      <skos:definition xml:lang="en">BSD+Patent is a free software licence approved by the Open Source Initiative. It is a 2-clause license in which nothing restricts redistribution under any other license, but it requests to retain copyright notices and restrict the use of the BSD licensor name to promote derivative products.</skos:definition>
      <skos:exactMatch rdf:resource="https://opensource.org/licenses/BSDplusPatent"/>
      <skos:inScheme rdf:resource="http://publications.europa.eu/resource/authority/licence"/>
      <skos:topConceptOf rdf:resource="http://publications.europa.eu/resource/authority/licence"/>
   </skos:Concept>
   <skos:Concept rdf:about="http://publications.europa.eu/resource/authority/licence/BSL_1_0"
                 at:deprecated="false">
      <skos:prefLabel xml:lang="en">Boost Software License 1.0</skos:prefLabel>
      <at:authority-code>BSL_1_0</at:authority-code>
      <at:op-code>BSL_1_0</at:op-code>
      <at:start.use>2003-08-17</at:start.use>
      <atold:op-code>BSL_1_0</atold:op-code>
      <dc:identifier>BSL_1_0</dc:identifier>
      <skos:altLabel xml:lang="bg">BSL-1.0</skos:altLabel>
      <skos:altLabel xml:lang="cs">BSL-1.0</skos:altLabel>
      <skos:altLabel xml:lang="da">BSL-1.0</skos:altLabel>
      <skos:altLabel xml:lang="de">BSL-1.0</skos:altLabel>
      <skos:altLabel xml:lang="el">BSL-1.0</skos:altLabel>
      <skos:altLabel xml:lang="en">BSL-1.0</skos:altLabel>
      <skos:altLabel xml:lang="es">BSL-1.0</skos:altLabel>
      <skos:altLabel xml:lang="et">BSL-1.0</skos:altLabel>
      <skos:altLabel xml:lang="fi">BSL-1.0</skos:altLabel>
      <skos:altLabel xml:lang="fr">BSL-1.0</skos:altLabel>
      <skos:altLabel xml:lang="ga">BSL-1.0</skos:altLabel>
      <skos:altLabel xml:lang="hr">BSL-1.0</skos:altLabel>
      <skos:altLabel xml:lang="hu">BSL-1.0</skos:altLabel>
      <skos:altLabel xml:lang="it">BSL-1.0</skos:altLabel>
      <skos:altLabel xml:lang="lt">BSL-1.0</skos:altLabel>
      <skos:altLabel xml:lang="lv">BSL-1.0</skos:altLabel>
      <skos:altLabel xml:lang="mt">BSL-1.0</skos:altLabel>
      <skos:altLabel xml:lang="nl">BSL-1.0</skos:altLabel>
      <skos:altLabel xml:lang="pl">BSL-1.0</skos:altLabel>
      <skos:altLabel xml:lang="pt">BSL-1.0</skos:altLabel>
      <skos:altLabel xml:lang="ro">BSL-1.0</skos:altLabel>
      <skos:altLabel xml:lang="sk">BSL-1.0</skos:altLabel>
      <skos:altLabel xml:lang="sl">BSL-1.0</skos:altLabel>
      <skos:altLabel xml:lang="sv">BSL-1.0</skos:altLabel>
      <skos:changeNote xml:lang="en">The source of the start-use date: https://en.wikipedia.org/wiki/Boost_(C%2B%2B_libraries)#License</skos:changeNote>
      <skos:definition xml:lang="en">BSL-1.0 is a simple permissive licence only requiring preservation of copyright and licence notices for source (and not binary) distribution. Licenced works, modifications, and larger works may be distributed under different terms and without source code.</skos:definition>
      <skos:exactMatch rdf:resource="https://opensource.org/licenses/BSL-1.0"/>
      <skos:inScheme rdf:resource="http://publications.europa.eu/resource/authority/licence"/>
      <skos:topConceptOf rdf:resource="http://publications.europa.eu/resource/authority/licence"/>
   </skos:Concept>
   <skos:Concept rdf:about="http://publications.europa.eu/resource/authority/licence/CATOSL_1_1"
                 at:deprecated="false">
      <skos:prefLabel xml:lang="en">Computer Associates Trusted Open Source License 1.1 (CATOSL-1.1)</skos:prefLabel>
      <at:authority-code>CATOSL_1_1</at:authority-code>
      <at:op-code>CATOSL_1_1</at:op-code>
      <at:start.use>2004-07-31</at:start.use>
      <atold:op-code>CATOSL_1_1</atold:op-code>
      <dc:identifier>CATOSL_1_1</dc:identifier>
      <skos:altLabel xml:lang="bg">CATOSL-1.1</skos:altLabel>
      <skos:altLabel xml:lang="cs">CATOSL-1.1</skos:altLabel>
      <skos:altLabel xml:lang="da">CATOSL-1.1</skos:altLabel>
      <skos:altLabel xml:lang="de">CATOSL-1.1</skos:altLabel>
      <skos:altLabel xml:lang="el">CATOSL-1.1</skos:altLabel>
      <skos:altLabel xml:lang="en">CATOSL-1.1</skos:altLabel>
      <skos:altLabel xml:lang="es">CATOSL-1.1</skos:altLabel>
      <skos:altLabel xml:lang="et">CATOSL-1.1</skos:altLabel>
      <skos:altLabel xml:lang="fi">CATOSL-1.1</skos:altLabel>
      <skos:altLabel xml:lang="fr">CATOSL-1.1</skos:altLabel>
      <skos:altLabel xml:lang="ga">CATOSL-1.1</skos:altLabel>
      <skos:altLabel xml:lang="hr">CATOSL-1.1</skos:altLabel>
      <skos:altLabel xml:lang="hu">CATOSL-1.1</skos:altLabel>
      <skos:altLabel xml:lang="it">CATOSL-1.1</skos:altLabel>
      <skos:altLabel xml:lang="lt">CATOSL-1.1</skos:altLabel>
      <skos:altLabel xml:lang="lv">CATOSL-1.1</skos:altLabel>
      <skos:altLabel xml:lang="mt">CATOSL-1.1</skos:altLabel>
      <skos:altLabel xml:lang="nl">CATOSL-1.1</skos:altLabel>
      <skos:altLabel xml:lang="pl">CATOSL-1.1</skos:altLabel>
      <skos:altLabel xml:lang="pt">CATOSL-1.1</skos:altLabel>
      <skos:altLabel xml:lang="ro">CATOSL-1.1</skos:altLabel>
      <skos:altLabel xml:lang="sk">CATOSL-1.1</skos:altLabel>
      <skos:altLabel xml:lang="sl">CATOSL-1.1</skos:altLabel>
      <skos:altLabel xml:lang="sv">CATOSL-1.1</skos:altLabel>
      <skos:changeNote xml:lang="en">The source of the start-use date: https://webcache.googleusercontent.com/search?q=cache:7pbd65y1OUYJ:https://www.theinquirer.net/inquirer/news/1022762/computer-associates-open-source-guru-speaks-out+&amp;cd=1&amp;hl=en&amp;ct=clnk&amp;gl=lu</skos:changeNote>
      <skos:definition xml:lang="en">CATOSL-1.1 is a copyleft-style, free software licence approved by the Open Source Initiative. Under this licence, it is possible to create a larger work by combining the program with other software code not governed by the terms of this licence, and distribute the larger work as a single product.</skos:definition>
      <skos:exactMatch rdf:resource="https://opensource.org/licenses/CATOSL-1.1"/>
      <skos:inScheme rdf:resource="http://publications.europa.eu/resource/authority/licence"/>
      <skos:topConceptOf rdf:resource="http://publications.europa.eu/resource/authority/licence"/>
   </skos:Concept>
   <skos:Concept rdf:about="http://publications.europa.eu/resource/authority/licence/CC0"
                 at:deprecated="false">
      <skos:prefLabel xml:lang="bg">Creative Commons CC0 1.0 Универсален</skos:prefLabel>
      <skos:prefLabel xml:lang="cs">Creative Commons CC0 1.0 Univerzální</skos:prefLabel>
      <skos:prefLabel xml:lang="da">Creative Commons CC0 1.0 Universel</skos:prefLabel>
      <skos:prefLabel xml:lang="de">Creative Commons CC0 1.0 Universell</skos:prefLabel>
      <skos:prefLabel xml:lang="el">Creative Commons CC0 1.0 Παγκόσμια</skos:prefLabel>
      <skos:prefLabel xml:lang="en">Creative Commons CC0 1.0 Universal</skos:prefLabel>
      <skos:prefLabel xml:lang="es">Creative Commons CC0 1.0 Universal</skos:prefLabel>
      <skos:prefLabel xml:lang="et">Creative Commons CC0 1.0 Üldine</skos:prefLabel>
      <skos:prefLabel xml:lang="fi">Creative Commons CC0 1.0 Yleismaailmallinen</skos:prefLabel>
      <skos:prefLabel xml:lang="fr">Creative Commons CC0 1.0 Universel</skos:prefLabel>
      <skos:prefLabel xml:lang="hr">Creative Commons CC0 1.0 Univerzalno</skos:prefLabel>
      <skos:prefLabel xml:lang="hu">Creative Commons CC0 1.0 Univerzális</skos:prefLabel>
      <skos:prefLabel xml:lang="it">Creative Commons CC0 1.0 Universal</skos:prefLabel>
      <skos:prefLabel xml:lang="lt">Creative Commons CC0 1.0 Universali</skos:prefLabel>
      <skos:prefLabel xml:lang="lv">Creative Commons CC0 1.0 Universāls</skos:prefLabel>
      <skos:prefLabel xml:lang="mt">Creative Commons CC0 1.0 Universali</skos:prefLabel>
      <skos:prefLabel xml:lang="nl">Creative Commons CC0 1.0 Universeel</skos:prefLabel>
      <skos:prefLabel xml:lang="pl">Creative Commons CC0 1.0 Universal</skos:prefLabel>
      <skos:prefLabel xml:lang="pt">Creative Commons CC0 1.0 Universal</skos:prefLabel>
      <skos:prefLabel xml:lang="ro">Creative Commons CC0 1.0 Universal</skos:prefLabel>
      <skos:prefLabel xml:lang="sk">Creative Commons CC0 1.0 Univerzálne</skos:prefLabel>
      <skos:prefLabel xml:lang="sl">Creative Commons CC0 1.0 Univerzalna</skos:prefLabel>
      <skos:prefLabel xml:lang="sv">Creative Commons CC0 1.0 universell</skos:prefLabel>
      <at:authority-code>CC0</at:authority-code>
      <at:op-code>CC0</at:op-code>
      <at:start.use>2009-03-11</at:start.use>
      <atold:op-code>CC0</atold:op-code>
      <dc:identifier>CC0</dc:identifier>
      <skos:altLabel xml:lang="bg">CC0 1.0</skos:altLabel>
      <skos:altLabel xml:lang="cs">CC0 1.0</skos:altLabel>
      <skos:altLabel xml:lang="da">CC0 1.0</skos:altLabel>
      <skos:altLabel xml:lang="de">CC0 1.0</skos:altLabel>
      <skos:altLabel xml:lang="el">CC0 1.0</skos:altLabel>
      <skos:altLabel xml:lang="en">CC0 1.0</skos:altLabel>
      <skos:altLabel xml:lang="es">CC0 1.0</skos:altLabel>
      <skos:altLabel xml:lang="et">CC0 1.0</skos:altLabel>
      <skos:altLabel xml:lang="fi">CC0 1.0</skos:altLabel>
      <skos:altLabel xml:lang="fr">CC0 1.0</skos:altLabel>
      <skos:altLabel xml:lang="ga">CC0 1.0</skos:altLabel>
      <skos:altLabel xml:lang="hr">CC0 1.0</skos:altLabel>
      <skos:altLabel xml:lang="hu">CC0 1.0</skos:altLabel>
      <skos:altLabel xml:lang="it">CC0 1.0</skos:altLabel>
      <skos:altLabel xml:lang="lt">CC0 1.0</skos:altLabel>
      <skos:altLabel xml:lang="lv">CC0 1.0</skos:altLabel>
      <skos:altLabel xml:lang="mt">CC0 1.0</skos:altLabel>
      <skos:altLabel xml:lang="nl">CC0 1.0</skos:altLabel>
      <skos:altLabel xml:lang="pl">CC0 1.0</skos:altLabel>
      <skos:altLabel xml:lang="pt">CC0 1.0</skos:altLabel>
      <skos:altLabel xml:lang="ro">CC0 1.0</skos:altLabel>
      <skos:altLabel xml:lang="sk">CC0 1.0</skos:altLabel>
      <skos:altLabel xml:lang="sl">CC0 1.0</skos:altLabel>
      <skos:altLabel xml:lang="sv">CC0 1.0</skos:altLabel>
      <skos:definition xml:lang="da">Personen, der har tilknyttet et værk disse betingelser, har dedikeret værket til offentligheden ved at give afkald på alle sine rettigheder til værket verden over, indenfor lovgivning om ophavsret, herunder alle relaterede og beslægtede rettigheder i det omfang, loven tillader. Du må kopiere, ændre, distribuere og fremføre værket, selv til kommercielle formål, alt sammen uden at spørge om tilladelse.</skos:definition>
      <skos:definition xml:lang="en">The person who associated a work with CC0 1.0 has dedicated the work to the public domain by waiving all of his or her rights to the work worldwide under copyright law, including all related and neighboring rights, to the extent allowed by law. One can copy, modify, distribute and perform the work, even for commercial purposes, all without asking permission.</skos:definition>
      <skos:definition xml:lang="fr">La personne qui a associé une œuvre à CC0 1.0 a dédié l’œuvre au domaine public en renonçant dans le monde entier à ses droits sur l’œuvre selon les lois sur le droit d’auteur, droit voisin et connexes, dans la mesure permise par la loi. On peut copier, modifier, distribuer et représenter l’œuvre, même à des fins commerciales, sans avoir besoin de demander l’autorisation.</skos:definition>
      <skos:exactMatch rdf:resource="http://creativecommons.org/publicdomain/zero/1.0/"/>
      <skos:inScheme rdf:resource="http://publications.europa.eu/resource/authority/licence"/>
      <skos:topConceptOf rdf:resource="http://publications.europa.eu/resource/authority/licence"/>
   </skos:Concept>
   <skos:Concept rdf:about="http://publications.europa.eu/resource/authority/licence/CC_BY"
                 at:deprecated="true">
      <skos:prefLabel xml:lang="cs">Creative Commons Uveďte původ 4.0 Mezinárodní</skos:prefLabel>
      <skos:prefLabel xml:lang="da">Creative Commons Navngivelse 4.0 International</skos:prefLabel>
      <skos:prefLabel xml:lang="de">Creative Commons Namensnennung 4.0 International</skos:prefLabel>
      <skos:prefLabel xml:lang="el">Creative Commons Αναφορά Δημιουργού 4.0 Διεθνές</skos:prefLabel>
      <skos:prefLabel xml:lang="en">Creative Commons Attribution 4.0 International</skos:prefLabel>
      <skos:prefLabel xml:lang="es">Creative Commons Atribución 4.0 Internacional</skos:prefLabel>
      <skos:prefLabel xml:lang="fi">Creative Commons Nimeä 4.0 Kansainvälinen</skos:prefLabel>
      <skos:prefLabel xml:lang="fr">Creative Commons Attribution 4.0 International</skos:prefLabel>
      <skos:prefLabel xml:lang="hr">Creative Commons Imenovanje 4.0 međunarodna</skos:prefLabel>
      <skos:prefLabel xml:lang="hu">Creative Commons Nevezd meg! 4.0 Nemzetközi</skos:prefLabel>
      <skos:prefLabel xml:lang="it">Creative Commons Attribuzione 4.0 Internazionale</skos:prefLabel>
      <skos:prefLabel xml:lang="lt">Creative Commons Priskyrimas 4.0 Tarptautinė</skos:prefLabel>
      <skos:prefLabel xml:lang="lv">Creative Commons Atsaucoties 4.0 Internacionāls</skos:prefLabel>
      <skos:prefLabel xml:lang="nl">Creative Commons Naamsvermelding 4.0 Internationaal</skos:prefLabel>
      <skos:prefLabel xml:lang="pl">Creative Commons Uznanie autorstwa 4.0 Międzynarodowe</skos:prefLabel>
      <skos:prefLabel xml:lang="pt">Creative Commons Atribuição 4.0 Internacional</skos:prefLabel>
      <skos:prefLabel xml:lang="ro">Creative Commons Atribuire 4.0 Internațional</skos:prefLabel>
      <skos:prefLabel xml:lang="sv">Creative Commons Erkännande 4.0 Internationell</skos:prefLabel>
      <at:authority-code>CC_BY</at:authority-code>
      <at:op-code>CC_BY</at:op-code>
      <at:start.use>2013-11-25</at:start.use>
      <atold:op-code>CC_BY</atold:op-code>
      <dc:identifier>CC_BY</dc:identifier>
      <skos:altLabel xml:lang="bg">CC BY 4.0</skos:altLabel>
      <skos:altLabel xml:lang="cs">CC BY 4.0</skos:altLabel>
      <skos:altLabel xml:lang="da">CC BY 4.0</skos:altLabel>
      <skos:altLabel xml:lang="de">CC BY 4.0</skos:altLabel>
      <skos:altLabel xml:lang="el">CC BY 4.0</skos:altLabel>
      <skos:altLabel xml:lang="en">CC BY 4.0</skos:altLabel>
      <skos:altLabel xml:lang="es">CC BY 4.0</skos:altLabel>
      <skos:altLabel xml:lang="et">CC BY 4.0</skos:altLabel>
      <skos:altLabel xml:lang="fi">CC BY 4.0</skos:altLabel>
      <skos:altLabel xml:lang="fr">CC BY 4.0</skos:altLabel>
      <skos:altLabel xml:lang="ga">CC BY 4.0</skos:altLabel>
      <skos:altLabel xml:lang="hr">CC BY 4.0</skos:altLabel>
      <skos:altLabel xml:lang="hu">CC BY 4.0</skos:altLabel>
      <skos:altLabel xml:lang="it">CC BY 4.0</skos:altLabel>
      <skos:altLabel xml:lang="lt">CC BY 4.0</skos:altLabel>
      <skos:altLabel xml:lang="lv">CC BY 4.0</skos:altLabel>
      <skos:altLabel xml:lang="mt">CC BY 4.0</skos:altLabel>
      <skos:altLabel xml:lang="nl">CC BY 4.0</skos:altLabel>
      <skos:altLabel xml:lang="pl">CC BY 4.0</skos:altLabel>
      <skos:altLabel xml:lang="pt">CC BY 4.0</skos:altLabel>
      <skos:altLabel xml:lang="ro">CC BY 4.0</skos:altLabel>
      <skos:altLabel xml:lang="sk">CC BY 4.0</skos:altLabel>
      <skos:altLabel xml:lang="sl">CC BY 4.0</skos:altLabel>
      <skos:altLabel xml:lang="sv">CC BY 4.0</skos:altLabel>
      <skos:definition xml:lang="en">This licence lets others distribute, remix, tweak, and build upon the author's work, even commercially, as long as they credit the author for the original creation. This is the most accommodating of licences offered. Recommended for maximum dissemination and use of licenced materials.</skos:definition>
      <skos:definition xml:lang="fr">Cette licence permet aux autres de distribuer, remixer, arranger, et adapter l’œuvre de l’auteur/autrice, même à des fins commerciales, tant qu’on accorde le mérite de la création originale à l’auteur/l’autrice en citant son nom. C’est le contrat le plus souple proposé. Recommandé pour la diffusion et l’utilisation maximales d’œuvres licenciées sous CC.</skos:definition>
      <skos:inScheme rdf:resource="http://publications.europa.eu/resource/authority/licence"/>
      <skos:topConceptOf rdf:resource="http://publications.europa.eu/resource/authority/licence"/>
      <at:end.use>2013-11-26</at:end.use>
   </skos:Concept>
   <skos:Concept rdf:about="http://publications.europa.eu/resource/authority/licence/CC_BYNC"
                 at:deprecated="true">
      <skos:prefLabel xml:lang="cs">Creative Commons Uveďte původ–Neužívejte komerčně 4.0 Mezinárodní</skos:prefLabel>
      <skos:prefLabel xml:lang="da">Creative Commons Navngivelse–IkkeKommerciel 4.0 International</skos:prefLabel>
      <skos:prefLabel xml:lang="de">Creative Commons Namensnennung – Nicht kommerziell 4.0 International</skos:prefLabel>
      <skos:prefLabel xml:lang="el">Creative Commons Αναφορά Δημιουργού – Μη Εμπορική Χρήση 4.0 Διεθνές</skos:prefLabel>
      <skos:prefLabel xml:lang="en">Creative Commons Attribution–NonCommercial 4.0 International</skos:prefLabel>
      <skos:prefLabel xml:lang="es">Creative Commons Atribución–NoComercial 4.0 Internacional</skos:prefLabel>
      <skos:prefLabel xml:lang="fi">Creative Commons Nimeä–EiKaupallinen 4.0 Kansainvälinen</skos:prefLabel>
      <skos:prefLabel xml:lang="fr">Creative Commons Attribution – Pas d’Utilisation Commerciale 4.0 International</skos:prefLabel>
      <skos:prefLabel xml:lang="hr">Creative Commons Imenovanje–Nekomercijalno 4.0 međunarodna</skos:prefLabel>
      <skos:prefLabel xml:lang="hu">Creative Commons Nevezd meg! – Ne add el! 4.0 Nemzetközi</skos:prefLabel>
      <skos:prefLabel xml:lang="it">Creative Commons Attribuzione – Non commerciale 4.0 Internazionale</skos:prefLabel>
      <skos:prefLabel xml:lang="lt">Creative Commons Priskyrimas – Nekomercinis platinimas 4.0 Tarptautinė</skos:prefLabel>
      <skos:prefLabel xml:lang="lv">Creative Commons Atsaucoties–Nekomerciāli 4.0 Internacionāls</skos:prefLabel>
      <skos:prefLabel xml:lang="nl">Creative Commons Naamsvermelding–NietCommercieel 4.0 Internationaal</skos:prefLabel>
      <skos:prefLabel xml:lang="pl">Creative Commons Uznanie autorstwa–Użycie niekomercyjne 4.0 Międzynarodowe</skos:prefLabel>
      <skos:prefLabel xml:lang="pt">Creative Commons Atribuição–NãoComercial 4.0 Internacional</skos:prefLabel>
      <skos:prefLabel xml:lang="ro">Creative Commons Atribuire–Necomercial 4.0 Internațional</skos:prefLabel>
      <skos:prefLabel xml:lang="sv">Creative Commons Erkännande–IckeKommersiell 4.0 Internationell</skos:prefLabel>
      <at:authority-code>CC_BYNC</at:authority-code>
      <at:op-code>CC_BYNC</at:op-code>
      <at:start.use>2013-11-25</at:start.use>
      <atold:op-code>CC_BYNC</atold:op-code>
      <dc:identifier>CC_BYNC</dc:identifier>
      <skos:altLabel xml:lang="bg">CC BY-NC 4.0</skos:altLabel>
      <skos:altLabel xml:lang="cs">CC BY-NC 4.0</skos:altLabel>
      <skos:altLabel xml:lang="da">CC BY-NC 4.0</skos:altLabel>
      <skos:altLabel xml:lang="de">CC BY-NC 4.0</skos:altLabel>
      <skos:altLabel xml:lang="el">CC BY-NC 4.0</skos:altLabel>
      <skos:altLabel xml:lang="en">CC BY-NC 4.0</skos:altLabel>
      <skos:altLabel xml:lang="es">CC BY-NC 4.0</skos:altLabel>
      <skos:altLabel xml:lang="et">CC BY-NC 4.0</skos:altLabel>
      <skos:altLabel xml:lang="fi">CC BY-NC 4.0</skos:altLabel>
      <skos:altLabel xml:lang="fr">CC BY-NC 4.0</skos:altLabel>
      <skos:altLabel xml:lang="ga">CC BY-NC 4.0</skos:altLabel>
      <skos:altLabel xml:lang="hr">CC BY-NC 4.0</skos:altLabel>
      <skos:altLabel xml:lang="hu">CC BY-NC 4.0</skos:altLabel>
      <skos:altLabel xml:lang="it">CC BY-NC 4.0</skos:altLabel>
      <skos:altLabel xml:lang="lt">CC BY-NC 4.0</skos:altLabel>
      <skos:altLabel xml:lang="lv">CC BY-NC 4.0</skos:altLabel>
      <skos:altLabel xml:lang="mt">CC BY-NC 4.0</skos:altLabel>
      <skos:altLabel xml:lang="nl">CC BY-NC 4.0</skos:altLabel>
      <skos:altLabel xml:lang="pl">CC BY-NC 4.0</skos:altLabel>
      <skos:altLabel xml:lang="pt">CC BY-NC 4.0</skos:altLabel>
      <skos:altLabel xml:lang="ro">CC BY-NC 4.0</skos:altLabel>
      <skos:altLabel xml:lang="sk">CC BY-NC 4.0</skos:altLabel>
      <skos:altLabel xml:lang="sl">CC BY-NC 4.0</skos:altLabel>
      <skos:altLabel xml:lang="sv">CC BY-NC 4.0</skos:altLabel>
      <skos:definition xml:lang="en">This licence lets others remix, tweak, and build upon the author's work non-commercially, and although their new works must also acknowledge the author and be non-commercial, they don’t have to licence their derivative works on the same terms.</skos:definition>
      <skos:definition xml:lang="fr">Cette licence permet aux autres de remixer, arranger, et adapter l’œuvre de l’auteur/autrice à des fins non commerciales et, bien que les nouvelles œuvres doivent créditer l’auteur/autrice en citant son nom et ne pas constituer une utilisation commerciale, elles n’ont pas à être diffusées selon les mêmes conditions.</skos:definition>
      <skos:inScheme rdf:resource="http://publications.europa.eu/resource/authority/licence"/>
      <skos:topConceptOf rdf:resource="http://publications.europa.eu/resource/authority/licence"/>
      <at:end.use>2013-11-26</at:end.use>
   </skos:Concept>
   <skos:Concept rdf:about="http://publications.europa.eu/resource/authority/licence/CC_BYNCND"
                 at:deprecated="true">
      <skos:prefLabel xml:lang="cs">Creative Commons Uveďte původ–Neužívejte komerčně–Nezpracovávejte 4.0 Mezinárodní</skos:prefLabel>
      <skos:prefLabel xml:lang="da">Creative Commons Navngivelse–IkkeKommerciel–IngenBearbejdelse 4.0 International</skos:prefLabel>
      <skos:prefLabel xml:lang="de">Creative Commons Namensnennung – Nicht kommerziell – Keine Bearbeitungen 4.0 International</skos:prefLabel>
      <skos:prefLabel xml:lang="el">Creative Commons Αναφορά Δημιουργού – Μη Εμπορική Χρήση – Όχι Παράγωγα Έργα 4.0 Διεθνές</skos:prefLabel>
      <skos:prefLabel xml:lang="en">Creative Commons Attribution–NonCommercial–NoDerivatives 4.0 International</skos:prefLabel>
      <skos:prefLabel xml:lang="es">Creative Commons Atribución–NoComercial–SinDerivar 4.0 Internacional</skos:prefLabel>
      <skos:prefLabel xml:lang="fi">Creative Commons Nimeä–EiKaupallinen–EiMuutoksia 4.0 Kansainvälinen</skos:prefLabel>
      <skos:prefLabel xml:lang="fr">Creative Commons Attribution – Pas d'Utilisation Commerciale – Pas de Modification 4.0 International</skos:prefLabel>
      <skos:prefLabel xml:lang="hr">Creative Commons Imenovanje–Nekomercijalno–Bez prerada 4.0 međunarodna</skos:prefLabel>
      <skos:prefLabel xml:lang="hu">Creative Commons Nevezd meg! – Ne add el! – Ne változtasd! 4.0 Nemzetközi</skos:prefLabel>
      <skos:prefLabel xml:lang="it">Creative Commons Attribuzione – Non commerciale – Non opere derivate 4.0 Internazionale</skos:prefLabel>
      <skos:prefLabel xml:lang="lt">Creative Commons Priskyrimas – Nekomercinis platinimas – Jokių išvestinių darbų 4.0 Tarptautinė</skos:prefLabel>
      <skos:prefLabel xml:lang="lv">Creative Commons Atsaucoties, nekomerciāli, nepārveidojot 4.0 Internacionāls</skos:prefLabel>
      <skos:prefLabel xml:lang="nl">Creative Commons Naamsvermelding–NietCommercieel–GeenAfgeleideWerken 4.0 Internationaal</skos:prefLabel>
      <skos:prefLabel xml:lang="pl">Creative Commons Uznanie autorstwa–Użycie niekomercyjne–Bez utworów zależnych 4.0 Międzynarodowe</skos:prefLabel>
      <skos:prefLabel xml:lang="pt">Creative Commons Atribuição–NãoComercial–SemDerivações 4.0 Internacional</skos:prefLabel>
      <skos:prefLabel xml:lang="ro">Creative Commons Atribuire–Necomercial–FărăDerivate 4.0 Internațional</skos:prefLabel>
      <skos:prefLabel xml:lang="sv">Creative Commons Erkännande–Ickekommersiell–IngaBearbetningar 4.0 Internationell</skos:prefLabel>
      <at:authority-code>CC_BYNCND</at:authority-code>
      <at:op-code>CC_BYNCND</at:op-code>
      <at:start.use>2013-11-25</at:start.use>
      <atold:op-code>CC_BYNCND</atold:op-code>
      <dc:identifier>CC_BYNCND</dc:identifier>
      <skos:altLabel xml:lang="bg">CC BY-NC-ND 4.0</skos:altLabel>
      <skos:altLabel xml:lang="cs">CC BY-NC-ND 4.0</skos:altLabel>
      <skos:altLabel xml:lang="da">CC BY-NC-ND 4.0</skos:altLabel>
      <skos:altLabel xml:lang="de">CC BY-NC-ND 4.0</skos:altLabel>
      <skos:altLabel xml:lang="el">CC BY-NC-ND 4.0</skos:altLabel>
      <skos:altLabel xml:lang="en">CC BY-NC-ND 4.0</skos:altLabel>
      <skos:altLabel xml:lang="es">CC BY-NC-ND 4.0</skos:altLabel>
      <skos:altLabel xml:lang="et">CC BY-NC-ND 4.0</skos:altLabel>
      <skos:altLabel xml:lang="fi">CC BY-NC-ND 4.0</skos:altLabel>
      <skos:altLabel xml:lang="fr">CC BY-NC-ND 4.0</skos:altLabel>
      <skos:altLabel xml:lang="ga">CC BY-NC-ND 4.0</skos:altLabel>
      <skos:altLabel xml:lang="hr">CC BY-NC-ND 4.0</skos:altLabel>
      <skos:altLabel xml:lang="hu">CC BY-NC-ND 4.0</skos:altLabel>
      <skos:altLabel xml:lang="it">CC BY-NC-ND 4.0</skos:altLabel>
      <skos:altLabel xml:lang="lt">CC BY-NC-ND 4.0</skos:altLabel>
      <skos:altLabel xml:lang="lv">CC BY-NC-ND 4.0</skos:altLabel>
      <skos:altLabel xml:lang="mt">CC BY-NC-ND 4.0</skos:altLabel>
      <skos:altLabel xml:lang="nl">CC BY-NC-ND 4.0</skos:altLabel>
      <skos:altLabel xml:lang="pl">CC BY-NC-ND 4.0</skos:altLabel>
      <skos:altLabel xml:lang="pt">CC BY-NC-ND 4.0</skos:altLabel>
      <skos:altLabel xml:lang="ro">CC BY-NC-ND 4.0</skos:altLabel>
      <skos:altLabel xml:lang="sk">CC BY-NC-ND 4.0</skos:altLabel>
      <skos:altLabel xml:lang="sl">CC BY-NC-ND 4.0</skos:altLabel>
      <skos:altLabel xml:lang="sv">CC BY-NC-ND 4.0</skos:altLabel>
      <skos:definition xml:lang="en">This licence is the most restrictive of the six main licences of Creative Commons, only allowing others to download the works and share them with others as long as they credit the author, but they can’t change them in any way or use them commercially.</skos:definition>
      <skos:definition xml:lang="fr">Cette licence est la plus restrictive des six licences principales de Creative Commons, n’autorisant les autres qu’à télécharger les œuvres de l’auteur/autrice et à les partager qu’on le/la crédite en citant son nom, mais on ne peut les modifier de quelque façon que ce soit ni les utiliser à des fins commerciales.</skos:definition>
      <skos:inScheme rdf:resource="http://publications.europa.eu/resource/authority/licence"/>
      <skos:topConceptOf rdf:resource="http://publications.europa.eu/resource/authority/licence"/>
      <at:end.use>2013-11-26</at:end.use>
   </skos:Concept>
   <skos:Concept rdf:about="http://publications.europa.eu/resource/authority/licence/CC_BYNCND_1_0"
                 at:deprecated="true">
      <skos:prefLabel xml:lang="bg">Creative Commons Признание-Без производни-Некомерсиално 1.0 Неадаптиран</skos:prefLabel>
      <skos:prefLabel xml:lang="cs">Creative Commons Uveďte původ–Nezpracovávejte–Neužívejte komerčně 1.0 Generic</skos:prefLabel>
      <skos:prefLabel xml:lang="da">Creative Commons Kreditering-Ingen afledninger-Ikkekommerciel 1.0 Generisk</skos:prefLabel>
      <skos:prefLabel xml:lang="de">Creative Commons Namensnennung – Keine Bearbeitungen – Nicht-kommerziell 1.0 Generic</skos:prefLabel>
      <skos:prefLabel xml:lang="el">Creative Commons Αναφορά Δημιουργού – Όχι Παράγωγα Έργα – Μη Εμπορική Χρήση 1.0 Γενικό</skos:prefLabel>
      <skos:prefLabel xml:lang="en">Creative Commons Attribution–NoDerivs–NonCommercial 1.0 Generic</skos:prefLabel>
      <skos:prefLabel xml:lang="es">Creative Commons Atribución–SinDerivadas–NoComercial 1.0 Genérica</skos:prefLabel>
      <skos:prefLabel xml:lang="et">Creative Commons Autorile viitamine–Tuletatud teoste keeld–Mitteäriline eesmärk 1.0 Üldine</skos:prefLabel>
      <skos:prefLabel xml:lang="fi">Creative Commons Nimeä–EiMuutoksia–EiKaupallinen 1.0 Yleinen</skos:prefLabel>
      <skos:prefLabel xml:lang="fr">Creative Commons Attribution – Pas de Modification – Pas d’Utilisation Commerciale 1.0 Générique</skos:prefLabel>
      <skos:prefLabel xml:lang="hr">Creative Commons Imenovanje–Bez prerada–Nekomercijalno 1.0 nelokalizirana licenca</skos:prefLabel>
      <skos:prefLabel xml:lang="hu">Creative Commons Nevezd meg! – Ne változtasd! – Ne add el! 1.0 Általános</skos:prefLabel>
      <skos:prefLabel xml:lang="it">Creative Commons Attribuzione – Non opere derivate – Non commerciale 1.0 Generico</skos:prefLabel>
      <skos:prefLabel xml:lang="lt">Creative Commons Priskyrimas – Jokių išvestinių darbų – Nekomercinis platinimas 1.0 Bendrasis</skos:prefLabel>
      <skos:prefLabel xml:lang="lv">Creative Commons Atsaucoties–Nepārveidojot–Nekomerciāli 1.0 Vispārīgs</skos:prefLabel>
      <skos:prefLabel xml:lang="mt">Creative Commons Attribuzzjoni-EbdaDerivattivi-MhuxKummerċjali 1.0 Generic</skos:prefLabel>
      <skos:prefLabel xml:lang="nl">Creative Commons Naamsvermelding–GeenAfgeleideWerken–NietCommercieel 1.0 Unported</skos:prefLabel>
      <skos:prefLabel xml:lang="pl">Creative Commons Uznanie autorstwa–Bez utworów zależnych–Użycie Niekomercyjne 1.0 Ogólny</skos:prefLabel>
      <skos:prefLabel xml:lang="pt">Creative Commons Atribuição–SemDerivações–NãoComercial 1.0 Genérica</skos:prefLabel>
      <skos:prefLabel xml:lang="ro">Creative Commons Atribuire–FărăModificări–Necomercial 1.0 Generică</skos:prefLabel>
      <skos:prefLabel xml:lang="sk">Creative Commons Uvedenie Autora-Bez Odvodeného Obsahu-Nekomerčné Použitie 1.0 Generic</skos:prefLabel>
      <skos:prefLabel xml:lang="sl">Creative Commons Priznanje avtorstva-Brez predelav-Nekomercialno 1.0 Generična</skos:prefLabel>
      <skos:prefLabel xml:lang="sv">Creative Commons Erkännande–IngaBearbetningar–IckeKommersiell 1.0 Generisk</skos:prefLabel>
      <at:authority-code>CC_BYNCND_1_0</at:authority-code>
      <at:op-code>CC_BYNCND_1_0</at:op-code>
      <at:start.use>2002-12-15</at:start.use>
      <atold:op-code>CC_BYNCND_1_0</atold:op-code>
      <dc:identifier>CC_BYNCND_1_0</dc:identifier>
      <skos:altLabel xml:lang="bg">CC BY-ND-NC 1.0</skos:altLabel>
      <skos:altLabel xml:lang="cs">CC BY-ND-NC 1.0</skos:altLabel>
      <skos:altLabel xml:lang="da">CC BY-ND-NC 1.0</skos:altLabel>
      <skos:altLabel xml:lang="de">CC BY-ND-NC 1.0</skos:altLabel>
      <skos:altLabel xml:lang="el">CC BY-ND-NC 1.0</skos:altLabel>
      <skos:altLabel xml:lang="en">CC BY-ND-NC 1.0</skos:altLabel>
      <skos:altLabel xml:lang="es">CC BY-ND-NC 1.0</skos:altLabel>
      <skos:altLabel xml:lang="et">CC BY-ND-NC 1.0</skos:altLabel>
      <skos:altLabel xml:lang="fi">CC BY-ND-NC 1.0</skos:altLabel>
      <skos:altLabel xml:lang="fr">CC BY-ND-NC 1.0</skos:altLabel>
      <skos:altLabel xml:lang="ga">CC BY-ND-NC 1.0</skos:altLabel>
      <skos:altLabel xml:lang="hr">CC BY-ND-NC 1.0</skos:altLabel>
      <skos:altLabel xml:lang="hu">CC BY-ND-NC 1.0</skos:altLabel>
      <skos:altLabel xml:lang="it">CC BY-ND-NC 1.0</skos:altLabel>
      <skos:altLabel xml:lang="lt">CC BY-ND-NC 1.0</skos:altLabel>
      <skos:altLabel xml:lang="lv">CC BY-ND-NC 1.0</skos:altLabel>
      <skos:altLabel xml:lang="mt">CC BY-ND-NC 1.0</skos:altLabel>
      <skos:altLabel xml:lang="nl">CC BY-ND-NC 1.0</skos:altLabel>
      <skos:altLabel xml:lang="pl">CC BY-ND-NC 1.0</skos:altLabel>
      <skos:altLabel xml:lang="pt">CC BY-ND-NC 1.0</skos:altLabel>
      <skos:altLabel xml:lang="ro">CC BY-ND-NC 1.0</skos:altLabel>
      <skos:altLabel xml:lang="sk">CC BY-ND-NC 1.0</skos:altLabel>
      <skos:altLabel xml:lang="sl">CC BY-ND-NC 1.0</skos:altLabel>
      <skos:altLabel xml:lang="sv">CC BY-ND-NC 1.0</skos:altLabel>
      <skos:definition xml:lang="en">CC BY-ND-NC 1.0 is the most restrictive of the six main licences of Creative Commons, only allowing others to download the works and share them with others as long as they credit the author, but they can’t change them in any way or use them commercially.</skos:definition>
      <skos:definition xml:lang="fr">CC BY-ND-NC 1.0 est la plus restrictive des six licences principales de Creative Commons, n’autorisant les autres qu’à télécharger les œuvres de l’auteur/autrice et à les partager tant qu’on le/la crédite en citant son nom, mais on ne peut les modifier de quelque façon que ce soit ni les utiliser à des fins commerciales.</skos:definition>
      <skos:exactMatch rdf:resource="http://creativecommons.org/licenses/by-nd-nc/1.0/"/>
      <skos:inScheme rdf:resource="http://publications.europa.eu/resource/authority/licence"/>
      <skos:topConceptOf rdf:resource="http://publications.europa.eu/resource/authority/licence"/>
      <at:end.use>2004-05-24</at:end.use>
   </skos:Concept>
   <skos:Concept rdf:about="http://publications.europa.eu/resource/authority/licence/CC_BYNCND_2_0"
                 at:deprecated="false">
      <skos:prefLabel xml:lang="bg">Creative Commons Признание-Без производни-Некомерсиално 2.0 Неадаптиран</skos:prefLabel>
      <skos:prefLabel xml:lang="cs">Creative Commons Uveďte původ–Neužívejte komerčně–Nezpracovávejte 2.0 Generic</skos:prefLabel>
      <skos:prefLabel xml:lang="da">Creative Commons Kreditering-Ikkekommerciel-Ingen afledninger 2.0 Generisk</skos:prefLabel>
      <skos:prefLabel xml:lang="de">Creative Commons Namensnennung – Nicht-kommerziell – Keine Bearbeitung 2.0 Generic</skos:prefLabel>
      <skos:prefLabel xml:lang="el">Creative Commons Αναφορά Δημιουργού – Μη Εμπορική Χρήση – Όχι Παράγωγα Έργα 2.0 Γενικό</skos:prefLabel>
      <skos:prefLabel xml:lang="en">Creative Commons Attribution–NonCommercial–NoDerivs 2.0 Generic</skos:prefLabel>
      <skos:prefLabel xml:lang="es">Creative Commons Atribución–NoComercial–SinDerivadas 2.0 Genérica</skos:prefLabel>
      <skos:prefLabel xml:lang="et">Creative Commons Autorile viitamine–Mitteäriline eesmärk–Tuletatud teoste keeld 2.0 Üldine</skos:prefLabel>
      <skos:prefLabel xml:lang="fi">Creative Commons Nimeä–EiKaupallinen–EiMuutoksia 2.0 Yleinen</skos:prefLabel>
      <skos:prefLabel xml:lang="fr">Creative Commons Attribution – Pas d’Utilisation Commerciale – Pas de Modification 2.0 Générique</skos:prefLabel>
      <skos:prefLabel xml:lang="hr">Creative Commons Imenovanje–Nekomercijalno–Bez prerada 2.0 nelokalizirana licenca</skos:prefLabel>
      <skos:prefLabel xml:lang="hu">Creative Commons Nevezd meg! – Ne add el! – Ne változtasd! 2.0 Általános</skos:prefLabel>
      <skos:prefLabel xml:lang="it">Creative Commons Attribuzione – Non commerciale – Non opere derivate 2.0 Generico</skos:prefLabel>
      <skos:prefLabel xml:lang="lt">Creative Commons Priskyrimas – Nekomercinis platinimas – Jokių išvestinių darbų 2.0 Bendrasis</skos:prefLabel>
      <skos:prefLabel xml:lang="lv">Creative Commons Atsaucoties–Nekomerciāli–Nepārveidojot 2.0 Vispārīgs</skos:prefLabel>
      <skos:prefLabel xml:lang="mt">Creative Commons Attribuzzjoni-MhuxKummerċjali-EbdaDerivattivi 2.0 Generic</skos:prefLabel>
      <skos:prefLabel xml:lang="nl">Creative Commons Naamsvermelding–NietCommercieel–GeenAfgeleideWerken 2.0 Unported</skos:prefLabel>
      <skos:prefLabel xml:lang="pl">Creative Commons Uznanie autorstwa–Użycie niekomercyjne–Bez utworów zależnych 2.0 Ogólny</skos:prefLabel>
      <skos:prefLabel xml:lang="pt">Creative Commons Atribuição–NãoComercial–SemDerivações 2.0 Genérica</skos:prefLabel>
      <skos:prefLabel xml:lang="ro">Creative Commons Atribuire–Necomercial–FărăModificări 2.0 Generică</skos:prefLabel>
      <skos:prefLabel xml:lang="sk">Creative Commons Uvedenie Autora-Nekomerčné Použitie-Bez Odvodeného Obsahu 2.0 Generic</skos:prefLabel>
      <skos:prefLabel xml:lang="sl">Creative Commons Priznanje avtorstva-Nekomercialno-Brez predelav 2.0 Generična</skos:prefLabel>
      <skos:prefLabel xml:lang="sv">Creative Commons Erkännande–Ickekommersiell–IngaBearbetningar 2.0 Generisk</skos:prefLabel>
      <at:authority-code>CC_BYNCND_2_0</at:authority-code>
      <at:op-code>CC_BYNCND_2_0</at:op-code>
      <at:start.use>2004-05-25</at:start.use>
      <atold:op-code>CC_BYNCND_2_0</atold:op-code>
      <dc:identifier>CC_BYNCND_2_0</dc:identifier>
      <skos:altLabel xml:lang="bg">CC BY-NC-ND 2.0</skos:altLabel>
      <skos:altLabel xml:lang="cs">CC BY-NC-ND 2.0</skos:altLabel>
      <skos:altLabel xml:lang="da">CC BY-NC-ND 2.0</skos:altLabel>
      <skos:altLabel xml:lang="de">CC BY-NC-ND 2.0</skos:altLabel>
      <skos:altLabel xml:lang="el">CC BY-NC-ND 2.0</skos:altLabel>
      <skos:altLabel xml:lang="en">CC BY-NC-ND 2.0</skos:altLabel>
      <skos:altLabel xml:lang="es">CC BY-NC-ND 2.0</skos:altLabel>
      <skos:altLabel xml:lang="et">CC BY-NC-ND 2.0</skos:altLabel>
      <skos:altLabel xml:lang="fi">CC BY-NC-ND 2.0</skos:altLabel>
      <skos:altLabel xml:lang="fr">CC BY-NC-ND 2.0</skos:altLabel>
      <skos:altLabel xml:lang="ga">CC BY-NC-ND 2.0</skos:altLabel>
      <skos:altLabel xml:lang="hr">CC BY-NC-ND 2.0</skos:altLabel>
      <skos:altLabel xml:lang="hu">CC BY-NC-ND 2.0</skos:altLabel>
      <skos:altLabel xml:lang="it">CC BY-NC-ND 2.0</skos:altLabel>
      <skos:altLabel xml:lang="lt">CC BY-NC-ND 2.0</skos:altLabel>
      <skos:altLabel xml:lang="lv">CC BY-NC-ND 2.0</skos:altLabel>
      <skos:altLabel xml:lang="mt">CC BY-NC-ND 2.0</skos:altLabel>
      <skos:altLabel xml:lang="nl">CC BY-NC-ND 2.0</skos:altLabel>
      <skos:altLabel xml:lang="pl">CC BY-NC-ND 2.0</skos:altLabel>
      <skos:altLabel xml:lang="pt">CC BY-NC-ND 2.0</skos:altLabel>
      <skos:altLabel xml:lang="ro">CC BY-NC-ND 2.0</skos:altLabel>
      <skos:altLabel xml:lang="sk">CC BY-NC-ND 2.0</skos:altLabel>
      <skos:altLabel xml:lang="sl">CC BY-NC-ND 2.0</skos:altLabel>
      <skos:altLabel xml:lang="sv">CC BY-NC-ND 2.0</skos:altLabel>
      <skos:definition xml:lang="en">CC BY-ND-NC 2.0 is the most restrictive of the six main licences of Creative Commons, only allowing others to download the works and share them with others as long as they credit the author, but they can’t change them in any way or use them commercially.</skos:definition>
      <skos:definition xml:lang="fr">CC BY-ND-NC 2.0 est la plus restrictive des six licences principales de Creative Commons, n’autorisant les autres qu’à télécharger les œuvres de l’auteur/autrice et à les partager tant qu’on le/la crédite en citant son nom, mais on ne peut les modifier de quelque façon que ce soit ni les utiliser à des fins commerciales.</skos:definition>
      <skos:exactMatch rdf:resource="http://creativecommons.org/licenses/by-nc-nd/2.0/"/>
      <skos:inScheme rdf:resource="http://publications.europa.eu/resource/authority/licence"/>
      <skos:topConceptOf rdf:resource="http://publications.europa.eu/resource/authority/licence"/>
   </skos:Concept>
   <skos:Concept rdf:about="http://publications.europa.eu/resource/authority/licence/CC_BYNCND_2_5"
                 at:deprecated="false">
      <skos:prefLabel xml:lang="bg">Creative Commons Признание-Без производни-Некомерсиално 2.5 Неадаптиран</skos:prefLabel>
      <skos:prefLabel xml:lang="cs">Creative Commons Uveďte původ–Neužívejte komerčně–Nezpracovávejte 2.5 Generic</skos:prefLabel>
      <skos:prefLabel xml:lang="da">Creative Commons Kreditering-Ikkekommerciel-Ingen afledninger 2.5 Generisk</skos:prefLabel>
      <skos:prefLabel xml:lang="de">Creative Commons Namensnennung – Nicht-kommerziell – Keine Bearbeitung 2.5 Generic</skos:prefLabel>
      <skos:prefLabel xml:lang="el">Creative Commons Αναφορά Δημιουργού – Μη Εμπορική Χρήση – Όχι Παράγωγα Έργα 2.5 Γενικό</skos:prefLabel>
      <skos:prefLabel xml:lang="en">Creative Commons Attribution–NonCommercial–NoDerivs 2.5 Generic</skos:prefLabel>
      <skos:prefLabel xml:lang="es">Creative Commons Atribución–NoComercial–SinDerivadas 2.5 Genérica</skos:prefLabel>
      <skos:prefLabel xml:lang="et">Creative Commons Autorile viitamine–Mitteäriline eesmärk–Tuletatud teoste keeld 2.5 Üldine</skos:prefLabel>
      <skos:prefLabel xml:lang="fi">Creative Commons Nimeä–EiKaupallinen–EiMuutoksia 2.5 Yleinen</skos:prefLabel>
      <skos:prefLabel xml:lang="fr">Creative Commons Attribution – Pas d’Utilisation Commerciale – Pas de Modification 2.5 Générique</skos:prefLabel>
      <skos:prefLabel xml:lang="hr">Creative Commons Imenovanje–Nekomercijalno–Bez prerada 2.5 nelokalizirana licenca</skos:prefLabel>
      <skos:prefLabel xml:lang="hu">Creative Commons Nevezd meg! – Ne add el! – Ne változtasd! 2.5 Általános</skos:prefLabel>
      <skos:prefLabel xml:lang="it">Creative Commons Attribuzione – Non commerciale – Non opere derivate 2.5 Generico</skos:prefLabel>
      <skos:prefLabel xml:lang="lt">Creative Commons Priskyrimas – Nekomercinis platinimas – Jokių išvestinių darbų 2.5 Bendrasis</skos:prefLabel>
      <skos:prefLabel xml:lang="lv">Creative Commons Atsaucoties–Nekomerciāli–Nepārveidojot 2.5 Vispārīgs</skos:prefLabel>
      <skos:prefLabel xml:lang="mt">Creative Commons Attribuzzjoni-MhuxKummerċjali-EbdaDerivattivi 2.5 Generic</skos:prefLabel>
      <skos:prefLabel xml:lang="nl">Creative Commons Naamsvermelding–NietCommercieel–GeenAfgeleideWerken 2.5 Unported</skos:prefLabel>
      <skos:prefLabel xml:lang="pl">Creative Commons Uznanie autorstwa–Użycie niekomercyjne–Bez utworów zależnych 2.5 Ogólny</skos:prefLabel>
      <skos:prefLabel xml:lang="pt">Creative Commons Atribuição–NãoComercial–SemDerivações 2.5 Genérica</skos:prefLabel>
      <skos:prefLabel xml:lang="ro">Creative Commons Atribuire–Necomercial–FărăModificări 2.5 Generică</skos:prefLabel>
      <skos:prefLabel xml:lang="sk">Creative Commons Uvedenie Autora-Nekomerčné Použitie-Bez Odvodeného Obsahu 2.5 Generic</skos:prefLabel>
      <skos:prefLabel xml:lang="sl">Creative Commons Priznanje avtorstva-Nekomercialno-Brez predelav 2.5 Generična</skos:prefLabel>
      <skos:prefLabel xml:lang="sv">Creative Commons Erkännande–Ickekommersiell–IngaBearbetningar 2.5 Generisk</skos:prefLabel>
      <at:authority-code>CC_BYNCND_2_5</at:authority-code>
      <at:op-code>CC_BYNCND_2_5</at:op-code>
      <at:start.use>2005-06-01</at:start.use>
      <atold:op-code>CC_BYNCND_2_5</atold:op-code>
      <dc:identifier>CC_BYNCND_2_5</dc:identifier>
      <skos:altLabel xml:lang="bg">CC BY-NC-ND 2.5</skos:altLabel>
      <skos:altLabel xml:lang="cs">CC BY-NC-ND 2.5</skos:altLabel>
      <skos:altLabel xml:lang="da">CC BY-NC-ND 2.5</skos:altLabel>
      <skos:altLabel xml:lang="de">CC BY-NC-ND 2.5</skos:altLabel>
      <skos:altLabel xml:lang="el">CC BY-NC-ND 2.5</skos:altLabel>
      <skos:altLabel xml:lang="en">CC BY-NC-ND 2.5</skos:altLabel>
      <skos:altLabel xml:lang="es">CC BY-NC-ND 2.5</skos:altLabel>
      <skos:altLabel xml:lang="et">CC BY-NC-ND 2.5</skos:altLabel>
      <skos:altLabel xml:lang="fi">CC BY-NC-ND 2.5</skos:altLabel>
      <skos:altLabel xml:lang="fr">CC BY-NC-ND 2.5</skos:altLabel>
      <skos:altLabel xml:lang="ga">CC BY-NC-ND 2.5</skos:altLabel>
      <skos:altLabel xml:lang="hr">CC BY-NC-ND 2.5</skos:altLabel>
      <skos:altLabel xml:lang="hu">CC BY-NC-ND 2.5</skos:altLabel>
      <skos:altLabel xml:lang="it">CC BY-NC-ND 2.5</skos:altLabel>
      <skos:altLabel xml:lang="lt">CC BY-NC-ND 2.5</skos:altLabel>
      <skos:altLabel xml:lang="lv">CC BY-NC-ND 2.5</skos:altLabel>
      <skos:altLabel xml:lang="mt">CC BY-NC-ND 2.5</skos:altLabel>
      <skos:altLabel xml:lang="nl">CC BY-NC-ND 2.5</skos:altLabel>
      <skos:altLabel xml:lang="pl">CC BY-NC-ND 2.5</skos:altLabel>
      <skos:altLabel xml:lang="pt">CC BY-NC-ND 2.5</skos:altLabel>
      <skos:altLabel xml:lang="ro">CC BY-NC-ND 2.5</skos:altLabel>
      <skos:altLabel xml:lang="sk">CC BY-NC-ND 2.5</skos:altLabel>
      <skos:altLabel xml:lang="sl">CC BY-NC-ND 2.5</skos:altLabel>
      <skos:altLabel xml:lang="sv">CC BY-NC-ND 2.5</skos:altLabel>
      <skos:definition xml:lang="en">CC BY-ND-NC 2.5 is the most restrictive of the six main licences of Creative Commons, only allowing others to download the works and share them with others as long as they credit the author, but they can’t change them in any way or use them commercially.</skos:definition>
      <skos:definition xml:lang="fr">CC BY-ND-NC 2.5 est la plus restrictive des six licences principales de Creative Commons, n’autorisant les autres qu’à télécharger les œuvres de l’auteur/autrice et à les partager tant qu’on le/la crédite en citant son nom, mais on ne peut les modifier de quelque façon que ce soit ni les utiliser à des fins commerciales.</skos:definition>
      <skos:exactMatch rdf:resource="http://creativecommons.org/licenses/by-nc-nd/2.5/"/>
      <skos:inScheme rdf:resource="http://publications.europa.eu/resource/authority/licence"/>
      <skos:topConceptOf rdf:resource="http://publications.europa.eu/resource/authority/licence"/>
   </skos:Concept>
   <skos:Concept rdf:about="http://publications.europa.eu/resource/authority/licence/CC_BYNCND_3_0"
                 at:deprecated="false">
      <skos:prefLabel xml:lang="bg">Creative Commons Признание-Некомерсиално-Без производни 3.0 Нелокализиран</skos:prefLabel>
      <skos:prefLabel xml:lang="cs">Creative Commons Uveďte původ–Neužívejte komerčně–Nezpracovávejte 3.0 Unported</skos:prefLabel>
      <skos:prefLabel xml:lang="da">Creative Commons Kreditering-Ikkekommerciel-Ingen afledninger 3.0 Ikke porteret</skos:prefLabel>
      <skos:prefLabel xml:lang="de">Creative Commons Namensnennung – Nicht-kommerziell – Keine Bearbeitung 3.0 Unported</skos:prefLabel>
      <skos:prefLabel xml:lang="el">Creative Commons Αναφορά Δημιουργού – Μη Εμπορική Χρήση – Όχι Παράγωγα Έργα 3.0 Μη εισαγόμενο</skos:prefLabel>
      <skos:prefLabel xml:lang="en">Creative Commons Attribution–NonCommercial–NoDerivs 3.0 Unported</skos:prefLabel>
      <skos:prefLabel xml:lang="es">Creative Commons Atribución–NoComercial–SinDerivadas 3.0 Unported</skos:prefLabel>
      <skos:prefLabel xml:lang="et">Creative Commons Autorile viitamine–Mitteäriline eesmärk–Tuletatud teoste keeld 3.0 Jurisdiktsiooniga sidumata</skos:prefLabel>
      <skos:prefLabel xml:lang="fi">Creative Commons Nimeä–EiKaupallinen–EiMuutoksia 3.0 Ei sovitettu</skos:prefLabel>
      <skos:prefLabel xml:lang="fr">Creative Commons Attribution – Pas d’Utilisation Commerciale – Pas de Modification 3.0 non transposé</skos:prefLabel>
      <skos:prefLabel xml:lang="hr">Creative Commons Imenovanje–Nekomercijalno–Bez prerada 3.0 nelokalizirana licenca</skos:prefLabel>
      <skos:prefLabel xml:lang="hu">Creative Commons Nevezd meg! – Ne add el! – Ne változtasd! 3.0 Unported</skos:prefLabel>
      <skos:prefLabel xml:lang="it">Creative Commons Attribuzione – Non commerciale – Non opere derivate 3.0 Unported</skos:prefLabel>
      <skos:prefLabel xml:lang="lt">Creative Commons Priskyrimas – Nekomercinis platinimas – Jokių išvestinių darbų 3.0 Nepritaikyta jurisdikcijai</skos:prefLabel>
      <skos:prefLabel xml:lang="lv">Creative Commons Atsaucoties–Nekomerciāli–Nepārveidojot 3.0 Nepārnesta</skos:prefLabel>
      <skos:prefLabel xml:lang="mt">Creative Commons Attribuzzjoni-MhuxKummerċjali-EbdaDerivattivi 3.0 Unported</skos:prefLabel>
      <skos:prefLabel xml:lang="nl">Creative Commons Naamsvermelding–NietCommercieel–GeenAfgeleideWerken 3.0 Unported</skos:prefLabel>
      <skos:prefLabel xml:lang="pl">Creative Commons Uznanie autorstwa–Użycie niekomercyjne–Bez utworów zależnych 3.0 Unported</skos:prefLabel>
      <skos:prefLabel xml:lang="pt">Creative Commons Atribuição–NãoComercial–SemDerivações 3.0 Não Adaptada</skos:prefLabel>
      <skos:prefLabel xml:lang="ro">Creative Commons Atribuire–Necomercial–FărăModificări 3.0 Ne-adaptată</skos:prefLabel>
      <skos:prefLabel xml:lang="sk">Creative Commons Uvedenie Autora-Nekomerčné Použitie-Bez Odvodeného Obsahu 3.0 Unported</skos:prefLabel>
      <skos:prefLabel xml:lang="sl">Creative Commons Priznanje avtorstva-Nekomercialno-Brez predelav 3.0 Nedoločena</skos:prefLabel>
      <skos:prefLabel xml:lang="sv">Creative Commons Erkännande–Ickekommersiell–IngaBearbetningar 3.0 Unported</skos:prefLabel>
      <at:authority-code>CC_BYNCND_3_0</at:authority-code>
      <at:op-code>CC_BYNCND_3_0</at:op-code>
      <at:start.use>2007-02-23</at:start.use>
      <atold:op-code>CC_BYNCND_3_0</atold:op-code>
      <dc:identifier>CC_BYNCND_3_0</dc:identifier>
      <skos:altLabel xml:lang="bg">CC BY-NC-ND 3.0</skos:altLabel>
      <skos:altLabel xml:lang="cs">CC BY-NC-ND 3.0</skos:altLabel>
      <skos:altLabel xml:lang="da">CC BY-NC-ND 3.0</skos:altLabel>
      <skos:altLabel xml:lang="de">CC BY-NC-ND 3.0</skos:altLabel>
      <skos:altLabel xml:lang="el">CC BY-NC-ND 3.0</skos:altLabel>
      <skos:altLabel xml:lang="en">CC BY-NC-ND 3.0</skos:altLabel>
      <skos:altLabel xml:lang="es">CC BY-NC-ND 3.0</skos:altLabel>
      <skos:altLabel xml:lang="et">CC BY-NC-ND 3.0</skos:altLabel>
      <skos:altLabel xml:lang="fi">CC BY-NC-ND 3.0</skos:altLabel>
      <skos:altLabel xml:lang="fr">CC BY-NC-ND 3.0</skos:altLabel>
      <skos:altLabel xml:lang="ga">CC BY-NC-ND 3.0</skos:altLabel>
      <skos:altLabel xml:lang="hr">CC BY-NC-ND 3.0</skos:altLabel>
      <skos:altLabel xml:lang="hu">CC BY-NC-ND 3.0</skos:altLabel>
      <skos:altLabel xml:lang="it">CC BY-NC-ND 3.0</skos:altLabel>
      <skos:altLabel xml:lang="lt">CC BY-NC-ND 3.0</skos:altLabel>
      <skos:altLabel xml:lang="lv">CC BY-NC-ND 3.0</skos:altLabel>
      <skos:altLabel xml:lang="mt">CC BY-NC-ND 3.0</skos:altLabel>
      <skos:altLabel xml:lang="nl">CC BY-NC-ND 3.0</skos:altLabel>
      <skos:altLabel xml:lang="pl">CC BY-NC-ND 3.0</skos:altLabel>
      <skos:altLabel xml:lang="pt">CC BY-NC-ND 3.0</skos:altLabel>
      <skos:altLabel xml:lang="ro">CC BY-NC-ND 3.0</skos:altLabel>
      <skos:altLabel xml:lang="sk">CC BY-NC-ND 3.0</skos:altLabel>
      <skos:altLabel xml:lang="sl">CC BY-NC-ND 3.0</skos:altLabel>
      <skos:altLabel xml:lang="sv">CC BY-NC-ND 3.0</skos:altLabel>
      <skos:definition xml:lang="en">CC BY-ND-NC 3.0 is the most restrictive of the six main licences of Creative Commons, only allowing others to download the works and share them with others as long as they credit the author, but they can’t change them in any way or use them commercially.</skos:definition>
      <skos:definition xml:lang="fr">CC BY-ND-NC 3.0 est la plus restrictive des six licences principales de Creative Commons, n’autorisant les autres qu’à télécharger les œuvres de l’auteur/autrice et à les partager tant qu’on le/la crédite en citant son nom, mais on ne peut les modifier de quelque façon que ce soit ni les utiliser à des fins commerciales.</skos:definition>
      <skos:exactMatch rdf:resource="http://creativecommons.org/licenses/by-nc-nd/3.0/"/>
      <skos:inScheme rdf:resource="http://publications.europa.eu/resource/authority/licence"/>
      <skos:topConceptOf rdf:resource="http://publications.europa.eu/resource/authority/licence"/>
      <skos:historyNote xml:lang="en">Unported licences are licences that are not associated with any specific jurisdiction, e.g. country.</skos:historyNote>
   </skos:Concept>
   <skos:Concept rdf:about="http://publications.europa.eu/resource/authority/licence/CC_BYNCND_4_0"
                 at:deprecated="false">
      <skos:prefLabel xml:lang="cs">Creative Commons Uveďte původ–Neužívejte komerčně–Nezpracovávejte 4.0 Mezinárodní</skos:prefLabel>
      <skos:prefLabel xml:lang="de">Creative Commons Namensnennung – Nicht kommerziell – Keine Bearbeitungen 4.0 International</skos:prefLabel>
      <skos:prefLabel xml:lang="el">Creative Commons Αναφορά Δημιουργού – Μη Εμπορική Χρήση – Όχι Παράγωγα Έργα 4.0 Διεθνές</skos:prefLabel>
      <skos:prefLabel xml:lang="en">Creative Commons Attribution–NonCommercial–NoDerivatives 4.0 International</skos:prefLabel>
      <skos:prefLabel xml:lang="es">Creative Commons Atribución–NoComercial–SinDerivar 4.0 Internacional</skos:prefLabel>
      <skos:prefLabel xml:lang="fi">Creative Commons Nimeä–EiKaupallinen–EiMuutoksia 4.0 Kansainvälinen</skos:prefLabel>
      <skos:prefLabel xml:lang="fr">Creative Commons Attribution – Pas d'Utilisation Commerciale – Pas de Modification 4.0 International</skos:prefLabel>
      <skos:prefLabel xml:lang="hr">Creative Commons Imenovanje–Nekomercijalno–Bez prerada 4.0 međunarodna</skos:prefLabel>
      <skos:prefLabel xml:lang="hu">Creative Commons Nevezd meg! – Ne add el! – Ne változtasd! 4.0 Nemzetközi</skos:prefLabel>
      <skos:prefLabel xml:lang="it">Creative Commons Attribuzione – Non commerciale – Non opere derivate 4.0 Internazionale</skos:prefLabel>
      <skos:prefLabel xml:lang="lt">Creative Commons Priskyrimas – Nekomercinis platinimas – Jokių išvestinių darbų 4.0 Tarptautinė</skos:prefLabel>
      <skos:prefLabel xml:lang="lv">Creative Commons Atsaucoties, nekomerciāli, nepārveidojot 4.0 Internacionāls</skos:prefLabel>
      <skos:prefLabel xml:lang="nl">Creative Commons Naamsvermelding–NietCommercieel–GeenAfgeleideWerken 4.0 Internationaal</skos:prefLabel>
      <skos:prefLabel xml:lang="pl">Creative Commons Uznanie autorstwa–Użycie niekomercyjne–Bez utworów zależnych 4.0 Międzynarodowe</skos:prefLabel>
      <skos:prefLabel xml:lang="pt">Creative Commons Atribuição–NãoComercial–SemDerivações 4.0 Internacional</skos:prefLabel>
      <skos:prefLabel xml:lang="ro">Creative Commons Atribuire–Necomercial–FărăDerivate 4.0 Internațional</skos:prefLabel>
      <skos:prefLabel xml:lang="sv">Creative Commons Erkännande–Ickekommersiell–IngaBearbetningar 4.0 Internationell</skos:prefLabel>
      <skos:prefLabel xml:lang="bg">Creative Commons Признание-Некомерсиално-Без производни 4.0 Международен</skos:prefLabel>
      <skos:prefLabel xml:lang="da">Creative Commons Kreditering-Ikkekommerciel-Ingen afledninger 4.0 International</skos:prefLabel>
      <skos:prefLabel xml:lang="et">Creative Commons Autorile viitamine–Mitteäriline eesmärk–Tuletatud teoste keeld 4.0 Rahvusvaheline</skos:prefLabel>
      <skos:prefLabel xml:lang="mt">Creative Commons Attribuzzjoni-MhuxKummerċjali-EbdaDerivattivi 4.0 Unported</skos:prefLabel>
      <skos:prefLabel xml:lang="sk">Creative Commons Uvedenie Autora-Nekomerčné Použitie-Žiadne Odvodené Diela 4.0 Medzinárodný</skos:prefLabel>
      <skos:prefLabel xml:lang="sl">Creative Commons Priznanje avtorstva-Nekomercialno-Brez predelav 4.0 Mednarodna</skos:prefLabel>
      <at:authority-code>CC_BYNCND_4_0</at:authority-code>
      <at:op-code>CC_BYNCND_4_0</at:op-code>
      <at:start.use>2013-11-26</at:start.use>
      <atold:op-code>CC_BYNCND_4_0</atold:op-code>
      <dc:identifier>CC_BYNCND_4_0</dc:identifier>
      <skos:altLabel xml:lang="bg">CC BY-NC-ND 4.0</skos:altLabel>
      <skos:altLabel xml:lang="cs">CC BY-NC-ND 4.0</skos:altLabel>
      <skos:altLabel xml:lang="da">CC BY-NC-ND 4.0</skos:altLabel>
      <skos:altLabel xml:lang="de">CC BY-NC-ND 4.0</skos:altLabel>
      <skos:altLabel xml:lang="el">CC BY-NC-ND 4.0</skos:altLabel>
      <skos:altLabel xml:lang="en">CC BY-NC-ND 4.0</skos:altLabel>
      <skos:altLabel xml:lang="es">CC BY-NC-ND 4.0</skos:altLabel>
      <skos:altLabel xml:lang="et">CC BY-NC-ND 4.0</skos:altLabel>
      <skos:altLabel xml:lang="fi">CC BY-NC-ND 4.0</skos:altLabel>
      <skos:altLabel xml:lang="fr">CC BY-NC-ND 4.0</skos:altLabel>
      <skos:altLabel xml:lang="ga">CC BY-NC-ND 4.0</skos:altLabel>
      <skos:altLabel xml:lang="hr">CC BY-NC-ND 4.0</skos:altLabel>
      <skos:altLabel xml:lang="hu">CC BY-NC-ND 4.0</skos:altLabel>
      <skos:altLabel xml:lang="it">CC BY-NC-ND 4.0</skos:altLabel>
      <skos:altLabel xml:lang="lt">CC BY-NC-ND 4.0</skos:altLabel>
      <skos:altLabel xml:lang="lv">CC BY-NC-ND 4.0</skos:altLabel>
      <skos:altLabel xml:lang="mt">CC BY-NC-ND 4.0</skos:altLabel>
      <skos:altLabel xml:lang="nl">CC BY-NC-ND 4.0</skos:altLabel>
      <skos:altLabel xml:lang="pl">CC BY-NC-ND 4.0</skos:altLabel>
      <skos:altLabel xml:lang="pt">CC BY-NC-ND 4.0</skos:altLabel>
      <skos:altLabel xml:lang="ro">CC BY-NC-ND 4.0</skos:altLabel>
      <skos:altLabel xml:lang="sk">CC BY-NC-ND 4.0</skos:altLabel>
      <skos:altLabel xml:lang="sl">CC BY-NC-ND 4.0</skos:altLabel>
      <skos:altLabel xml:lang="sv">CC BY-NC-ND 4.0</skos:altLabel>
      <skos:definition xml:lang="en">CC BY-ND-NC 4.0 is the most restrictive of the six main licences of Creative Commons, only allowing others to download the works and share them with others as long as they credit the author, but they can’t change them in any way or use them commercially.</skos:definition>
      <skos:definition xml:lang="fr">CC BY-ND-NC 4.0 est la plus restrictive des six licences principales de Creative Commons, n’autorisant les autres qu’à télécharger les œuvres de l’auteur/autrice et à les partager tant qu’on le/la crédite en citant son nom, mais on ne peut les modifier de quelque façon que ce soit ni les utiliser à des fins commerciales.</skos:definition>
      <skos:exactMatch rdf:resource="http://creativecommons.org/licenses/by-nc-nd/4.0/"/>
      <skos:inScheme rdf:resource="http://publications.europa.eu/resource/authority/licence"/>
      <skos:topConceptOf rdf:resource="http://publications.europa.eu/resource/authority/licence"/>
   </skos:Concept>
   <skos:Concept rdf:about="http://publications.europa.eu/resource/authority/licence/CC_BYNCSA"
                 at:deprecated="true">
      <skos:prefLabel xml:lang="cs">Creative Commons Uveďte původ–Neužívejte dílo komerčně–Zachovejte licenci 4.0 Mezinárodní</skos:prefLabel>
      <skos:prefLabel xml:lang="da">Creative Commons Navngivelse–IkkeKommerciel–DelPåSammeVilkår 4.0 International</skos:prefLabel>
      <skos:prefLabel xml:lang="de">Creative Commons Namensnennung – Nicht-kommerziell – Weitergabe unter gleichen Bedingungen 4.0 International</skos:prefLabel>
      <skos:prefLabel xml:lang="el">Creative Commons Αναφορά Δημιουργού – Μη Εμπορική Χρήση – Παρόμοια Διανομή 4.0 Διεθνές</skos:prefLabel>
      <skos:prefLabel xml:lang="en">Creative Commons Attribution–NonCommercial–ShareAlike 4.0 International</skos:prefLabel>
      <skos:prefLabel xml:lang="es">Creative Commons Atribución–NoComercial–CompartirIgual 4.0 Internacional</skos:prefLabel>
      <skos:prefLabel xml:lang="fi">Creative Commons Nimeä–EiKaupallinen–JaaSamoin 4.0 Kansainvälinen</skos:prefLabel>
      <skos:prefLabel xml:lang="fr">Creative Commons Attribution – Pas d’Utilisation Commerciale – Partage dans les Mêmes Conditions 4.0 International</skos:prefLabel>
      <skos:prefLabel xml:lang="hr">Creative Commons Imenovanje–Nekomercijalno–Dijeli pod istim uvjetima 4.0 međunarodna</skos:prefLabel>
      <skos:prefLabel xml:lang="hu">Creative Commons Nevezd meg! – Ne add el! – Így add tovább! 4.0 Nemzetközi</skos:prefLabel>
      <skos:prefLabel xml:lang="it">Creative Commons Attribuzione – Non commerciale – Condividi allo stesso modo 4.0 Internazionale</skos:prefLabel>
      <skos:prefLabel xml:lang="lt">Creative Commons Priskyrimas – Nekomercinis platinimas – Analogiškas platinimas 4.0 Tarptautinė</skos:prefLabel>
      <skos:prefLabel xml:lang="lv">Creative Commons Atsaucoties–Nekomerciāli–Nemainot licenci 4.0 Internacionāls</skos:prefLabel>
      <skos:prefLabel xml:lang="nl">Creative Commons Naamsvermelding–NietCommercieel–GelijkDelen 4.0 Internationaal</skos:prefLabel>
      <skos:prefLabel xml:lang="pl">Creative Commons Uznanie autorstwa–Użycie niekomercyjne–Na tych samych warunkach 4.0 Międzynarodowe</skos:prefLabel>
      <skos:prefLabel xml:lang="pt">Creative Commons Atribuição–NãoComercial–CompartilhaIgual 4.0 Internacional</skos:prefLabel>
      <skos:prefLabel xml:lang="ro">Creative Commons Atribuire–Necomercial–Distribuire în Condiţii Identice 4.0 Internațional</skos:prefLabel>
      <skos:prefLabel xml:lang="sv">Creative Commons Erkännande–IckeKommersiell–DelaLika 4.0 Internationell</skos:prefLabel>
      <at:authority-code>CC_BYNCSA</at:authority-code>
      <at:op-code>CC_BYNCSA</at:op-code>
      <at:start.use>2013-11-25</at:start.use>
      <atold:op-code>CC_BYNCSA</atold:op-code>
      <dc:identifier>CC_BYNCSA</dc:identifier>
      <skos:altLabel xml:lang="bg">CC BY-NC-SA 4.0</skos:altLabel>
      <skos:altLabel xml:lang="cs">CC BY-NC-SA 4.0</skos:altLabel>
      <skos:altLabel xml:lang="da">CC BY-NC-SA 4.0</skos:altLabel>
      <skos:altLabel xml:lang="de">CC BY-NC-SA 4.0</skos:altLabel>
      <skos:altLabel xml:lang="el">CC BY-NC-SA 4.0</skos:altLabel>
      <skos:altLabel xml:lang="en">CC BY-NC-SA 4.0</skos:altLabel>
      <skos:altLabel xml:lang="es">CC BY-NC-SA 4.0</skos:altLabel>
      <skos:altLabel xml:lang="et">CC BY-NC-SA 4.0</skos:altLabel>
      <skos:altLabel xml:lang="fi">CC BY-NC-SA 4.0</skos:altLabel>
      <skos:altLabel xml:lang="fr">CC BY-NC-SA 4.0</skos:altLabel>
      <skos:altLabel xml:lang="ga">CC BY-NC-SA 4.0</skos:altLabel>
      <skos:altLabel xml:lang="hr">CC BY-NC-SA 4.0</skos:altLabel>
      <skos:altLabel xml:lang="hu">CC BY-NC-SA 4.0</skos:altLabel>
      <skos:altLabel xml:lang="it">CC BY-NC-SA 4.0</skos:altLabel>
      <skos:altLabel xml:lang="lt">CC BY-NC-SA 4.0</skos:altLabel>
      <skos:altLabel xml:lang="lv">CC BY-NC-SA 4.0</skos:altLabel>
      <skos:altLabel xml:lang="mt">CC BY-NC-SA 4.0</skos:altLabel>
      <skos:altLabel xml:lang="nl">CC BY-NC-SA 4.0</skos:altLabel>
      <skos:altLabel xml:lang="pl">CC BY-NC-SA 4.0</skos:altLabel>
      <skos:altLabel xml:lang="pt">CC BY-NC-SA 4.0</skos:altLabel>
      <skos:altLabel xml:lang="ro">CC BY-NC-SA 4.0</skos:altLabel>
      <skos:altLabel xml:lang="sk">CC BY-NC-SA 4.0</skos:altLabel>
      <skos:altLabel xml:lang="sl">CC BY-NC-SA 4.0</skos:altLabel>
      <skos:altLabel xml:lang="sv">CC BY-NC-SA 4.0</skos:altLabel>
      <skos:definition xml:lang="en">This licence lets others remix, tweak, and build upon the author’s work non-commercially, as long as they credit the author and licence their new creations under the identical terms.</skos:definition>
      <skos:definition xml:lang="fr">Cette licence permet aux autres de remixer, arranger, et adapter l’œuvre de l’auteur/autrice à des fins non commerciales tant qu’on le/la crédite en citant son nom et que les nouvelles œuvres sont diffusées selon les mêmes conditions.</skos:definition>
      <skos:inScheme rdf:resource="http://publications.europa.eu/resource/authority/licence"/>
      <skos:topConceptOf rdf:resource="http://publications.europa.eu/resource/authority/licence"/>
      <at:end.use>2013-11-26</at:end.use>
   </skos:Concept>
   <skos:Concept rdf:about="http://publications.europa.eu/resource/authority/licence/CC_BYNCSA_1_0"
                 at:deprecated="true">
      <skos:prefLabel xml:lang="bg">Creative Commons Признание-Некомерсиално-Споделяне на споделеното 1.0 Неадаптиран</skos:prefLabel>
      <skos:prefLabel xml:lang="cs">Creative Commons Uveďte původ–Neužívejte dílo komerčně–Zachovejte licenci 1.0 Generic</skos:prefLabel>
      <skos:prefLabel xml:lang="da">Creative Commons Kreditering-Ikkekommerciel-Deling på samme vilkår 1.0 Generisk</skos:prefLabel>
      <skos:prefLabel xml:lang="de">Creative Commons Namensnennung – Nicht-kommerziell – Weitergabe unter gleichen Bedingungen 1.0 Generic</skos:prefLabel>
      <skos:prefLabel xml:lang="el">Creative Commons Αναφορά Δημιουργού – Μη Εμπορική Χρήση – Παρόμοια Διανομή 1.0 Γενικό</skos:prefLabel>
      <skos:prefLabel xml:lang="en">Creative Commons Attribution–NonCommercial–ShareAlike 1.0 Generic</skos:prefLabel>
      <skos:prefLabel xml:lang="es">Creative Commons Atribución–NoComercial–CompartirIgual 1.0 Genérica</skos:prefLabel>
      <skos:prefLabel xml:lang="et">Creative Commons Autorile viitamine–Mitteäriline eesmärk–Jagamine samadel tingimustel 1.0 Üldine</skos:prefLabel>
      <skos:prefLabel xml:lang="fi">Creative Commons Nimeä–EiKaupallinen–JaaSamoin 1.0 Yleinen</skos:prefLabel>
      <skos:prefLabel xml:lang="fr">Creative Commons Attribution – Pas d’Utilisation Commerciale – Partage dans les Mêmes Conditions 1.0 Générique</skos:prefLabel>
      <skos:prefLabel xml:lang="hr">Creative Commons Imenovanje–Nekomercijalno–Dijeli pod istim uvjetima 1.0 nelokalizirana licenca</skos:prefLabel>
      <skos:prefLabel xml:lang="hu">Creative Commons Nevezd meg! – Ne add el! – Így add tovább! 1.0 Általános</skos:prefLabel>
      <skos:prefLabel xml:lang="it">Creative Commons Attribuzione – Non commerciale – Condividi allo stesso modo 1.0 Generico</skos:prefLabel>
      <skos:prefLabel xml:lang="lt">Creative Commons Priskyrimas – Nekomercinis platinimas – Analogiškas platinimas 1.0 Bendrasis</skos:prefLabel>
      <skos:prefLabel xml:lang="lv">Creative Commons Atsaucoties–Nekomerciāli–Nemainot licenci 1.0 Vispārīgs</skos:prefLabel>
      <skos:prefLabel xml:lang="mt">Creative Commons Attribuzzjoni-MhuxKummerċjali-KondiviżjoniUgwali 1.0 Generic</skos:prefLabel>
      <skos:prefLabel xml:lang="nl">Creative Commons Naamsvermelding–NietCommercieel–GelijkDelen 1.0 Unported</skos:prefLabel>
      <skos:prefLabel xml:lang="pl">Creative Commons Uznanie autorstwa–Użycie niekomercyjne–Na tych samych warunkach 1.0 Ogólny</skos:prefLabel>
      <skos:prefLabel xml:lang="pt">Creative Commons Atribuição–NãoComercial–CompartilhaIgual 1.0 Genérica</skos:prefLabel>
      <skos:prefLabel xml:lang="ro">Creative Commons Atribuire–Necomercial–Distribuire în Condiţii Identice 1.0 Generică</skos:prefLabel>
      <skos:prefLabel xml:lang="sk">Creative Commons Uvedenie Autora-Nekomerčné Použitie-Rovnaké Šírenie 1.0 Generic</skos:prefLabel>
      <skos:prefLabel xml:lang="sl">Creative Commons Priznanje avtorstva-Nekomercialno-Deljenje pod enakimi pogoji 1.0 Generična</skos:prefLabel>
      <skos:prefLabel xml:lang="sv">Creative Commons Erkännande–IckeKommersiell–DelaLika 1.0 Generisk</skos:prefLabel>
      <at:authority-code>CC_BYNCSA_1_0</at:authority-code>
      <at:op-code>CC_BYNCSA_1_0</at:op-code>
      <at:start.use>2002-12-15</at:start.use>
      <atold:op-code>CC_BYNCSA_1_0</atold:op-code>
      <dc:identifier>CC_BYNCSA_1_0</dc:identifier>
      <skos:altLabel xml:lang="bg">CC BY-NC-SA 1.0</skos:altLabel>
      <skos:altLabel xml:lang="cs">CC BY-NC-SA 1.0</skos:altLabel>
      <skos:altLabel xml:lang="da">CC BY-NC-SA 1.0</skos:altLabel>
      <skos:altLabel xml:lang="de">CC BY-NC-SA 1.0</skos:altLabel>
      <skos:altLabel xml:lang="el">CC BY-NC-SA 1.0</skos:altLabel>
      <skos:altLabel xml:lang="en">CC BY-NC-SA 1.0</skos:altLabel>
      <skos:altLabel xml:lang="es">CC BY-NC-SA 1.0</skos:altLabel>
      <skos:altLabel xml:lang="et">CC BY-NC-SA 1.0</skos:altLabel>
      <skos:altLabel xml:lang="fi">CC BY-NC-SA 1.0</skos:altLabel>
      <skos:altLabel xml:lang="fr">CC BY-NC-SA 1.0</skos:altLabel>
      <skos:altLabel xml:lang="ga">CC BY-NC-SA 1.0</skos:altLabel>
      <skos:altLabel xml:lang="hr">CC BY-NC-SA 1.0</skos:altLabel>
      <skos:altLabel xml:lang="hu">CC BY-NC-SA 1.0</skos:altLabel>
      <skos:altLabel xml:lang="it">CC BY-NC-SA 1.0</skos:altLabel>
      <skos:altLabel xml:lang="lt">CC BY-NC-SA 1.0</skos:altLabel>
      <skos:altLabel xml:lang="lv">CC BY-NC-SA 1.0</skos:altLabel>
      <skos:altLabel xml:lang="mt">CC BY-NC-SA 1.0</skos:altLabel>
      <skos:altLabel xml:lang="nl">CC BY-NC-SA 1.0</skos:altLabel>
      <skos:altLabel xml:lang="pl">CC BY-NC-SA 1.0</skos:altLabel>
      <skos:altLabel xml:lang="pt">CC BY-NC-SA 1.0</skos:altLabel>
      <skos:altLabel xml:lang="ro">CC BY-NC-SA 1.0</skos:altLabel>
      <skos:altLabel xml:lang="sk">CC BY-NC-SA 1.0</skos:altLabel>
      <skos:altLabel xml:lang="sl">CC BY-NC-SA 1.0</skos:altLabel>
      <skos:altLabel xml:lang="sv">CC BY-NC-SA 1.0</skos:altLabel>
      <skos:definition xml:lang="en">CC BY-NC-SA 1.0 lets others remix, tweak, and build upon the author’s work non-commercially, as long as they credit the author and licence their new creations under the identical terms.</skos:definition>
      <skos:definition xml:lang="fr">CC BY-NC-SA 1.0 permet aux autres de remixer, arranger, et adapter l’œuvre de l’auteur/autrice à des fins non commerciales tant qu’on le/la crédite en citant son nom et que les nouvelles œuvres sont diffusées selon les mêmes conditions.</skos:definition>
      <skos:exactMatch rdf:resource="http://creativecommons.org/licenses/by-nc-sa/1.0/"/>
      <skos:inScheme rdf:resource="http://publications.europa.eu/resource/authority/licence"/>
      <skos:topConceptOf rdf:resource="http://publications.europa.eu/resource/authority/licence"/>
      <at:end.use>2004-05-24</at:end.use>
   </skos:Concept>
   <skos:Concept rdf:about="http://publications.europa.eu/resource/authority/licence/CC_BYNCSA_2_0"
                 at:deprecated="false">
      <skos:prefLabel xml:lang="bg">Creative Commons Признание-Некомерсиално-Споделяне на споделеното 2.0 Неадаптиран</skos:prefLabel>
      <skos:prefLabel xml:lang="cs">Creative Commons Uveďte původ–Neužívejte dílo komerčně–Zachovejte licenci 2.0 Generic</skos:prefLabel>
      <skos:prefLabel xml:lang="da">Creative Commons Kreditering-Ikkekommerciel-Deling på samme vilkår 2.0 Generisk</skos:prefLabel>
      <skos:prefLabel xml:lang="de">Creative Commons Namensnennung – Nicht-kommerziell – Weitergabe unter gleichen Bedingungen 2.0 Generic</skos:prefLabel>
      <skos:prefLabel xml:lang="el">Creative Commons Αναφορά Δημιουργού – Μη Εμπορική Χρήση – Παρόμοια Διανομή 2.0 Γενικό</skos:prefLabel>
      <skos:prefLabel xml:lang="en">Creative Commons Attribution–NonCommercial–ShareAlike 2.0 Generic</skos:prefLabel>
      <skos:prefLabel xml:lang="es">Creative Commons Atribución–NoComercial–CompartirIgual 2.0 Genérica</skos:prefLabel>
      <skos:prefLabel xml:lang="et">Creative Commons Autorile viitamine–Mitteäriline eesmärk–Jagamine samadel tingimustel 2.0 Üldine</skos:prefLabel>
      <skos:prefLabel xml:lang="fi">Creative Commons Nimeä–EiKaupallinen–JaaSamoin 2.0 Yleinen</skos:prefLabel>
      <skos:prefLabel xml:lang="fr">Creative Commons Attribution – Pas d’Utilisation Commerciale – Partage dans les Mêmes Conditions 2.0 Générique</skos:prefLabel>
      <skos:prefLabel xml:lang="hr">Creative Commons Imenovanje–Nekomercijalno–Dijeli pod istim uvjetima 2.0 nelokalizirana licenca</skos:prefLabel>
      <skos:prefLabel xml:lang="hu">Creative Commons Nevezd meg! – Ne add el! – Így add tovább! 2.0 Általános</skos:prefLabel>
      <skos:prefLabel xml:lang="it">Creative Commons Attribuzione – Non commerciale – Condividi allo stesso modo 2.0 Generico</skos:prefLabel>
      <skos:prefLabel xml:lang="lt">Creative Commons Priskyrimas – Nekomercinis platinimas – Analogiškas platinimas 2.0 Bendrasis</skos:prefLabel>
      <skos:prefLabel xml:lang="lv">Creative Commons Atsaucoties–Nekomerciāli–Nemainot licenci 2.0 Vispārīgs</skos:prefLabel>
      <skos:prefLabel xml:lang="mt">Creative Commons Attribuzzjoni-MhuxKummerċjali-KondiviżjoniUgwali 2.0 Generic</skos:prefLabel>
      <skos:prefLabel xml:lang="nl">Creative Commons Naamsvermelding–NietCommercieel–GelijkDelen 2.0 Unported</skos:prefLabel>
      <skos:prefLabel xml:lang="pl">Creative Commons Uznanie autorstwa–Użycie niekomercyjne–Na tych samych warunkach 2.0 Ogólny</skos:prefLabel>
      <skos:prefLabel xml:lang="pt">Creative Commons Atribuição–NãoComercial–CompartilhaIgual 2.0 Genérica</skos:prefLabel>
      <skos:prefLabel xml:lang="ro">Creative Commons Atribuire–Necomercial–Distribuire în Condiţii Identice 2.0 Generică</skos:prefLabel>
      <skos:prefLabel xml:lang="sk">Creative Commons Uvedenie Autora-Nekomerčné Použitie-Rovnaké Šírenie 2.0 Generic</skos:prefLabel>
      <skos:prefLabel xml:lang="sl">Creative Commons Priznanje avtorstva-Nekomercialno-Deljenje pod enakimi pogoji 2.0 Generična</skos:prefLabel>
      <skos:prefLabel xml:lang="sv">Creative Commons Erkännande–IckeKommersiell–DelaLika 2.0 Generisk</skos:prefLabel>
      <at:authority-code>CC_BYNCSA_2_0</at:authority-code>
      <at:op-code>CC_BYNCSA_2_0</at:op-code>
      <at:start.use>2004-05-25</at:start.use>
      <atold:op-code>CC_BYNCSA_2_0</atold:op-code>
      <dc:identifier>CC_BYNCSA_2_0</dc:identifier>
      <skos:altLabel xml:lang="bg">CC BY-NC-SA 2.0</skos:altLabel>
      <skos:altLabel xml:lang="cs">CC BY-NC-SA 2.0</skos:altLabel>
      <skos:altLabel xml:lang="da">CC BY-NC-SA 2.0</skos:altLabel>
      <skos:altLabel xml:lang="de">CC BY-NC-SA 2.0</skos:altLabel>
      <skos:altLabel xml:lang="el">CC BY-NC-SA 2.0</skos:altLabel>
      <skos:altLabel xml:lang="en">CC BY-NC-SA 2.0</skos:altLabel>
      <skos:altLabel xml:lang="es">CC BY-NC-SA 2.0</skos:altLabel>
      <skos:altLabel xml:lang="et">CC BY-NC-SA 2.0</skos:altLabel>
      <skos:altLabel xml:lang="fi">CC BY-NC-SA 2.0</skos:altLabel>
      <skos:altLabel xml:lang="fr">CC BY-NC-SA 2.0</skos:altLabel>
      <skos:altLabel xml:lang="ga">CC BY-NC-SA 2.0</skos:altLabel>
      <skos:altLabel xml:lang="hr">CC BY-NC-SA 2.0</skos:altLabel>
      <skos:altLabel xml:lang="hu">CC BY-NC-SA 2.0</skos:altLabel>
      <skos:altLabel xml:lang="it">CC BY-NC-SA 2.0</skos:altLabel>
      <skos:altLabel xml:lang="lt">CC BY-NC-SA 2.0</skos:altLabel>
      <skos:altLabel xml:lang="lv">CC BY-NC-SA 2.0</skos:altLabel>
      <skos:altLabel xml:lang="mt">CC BY-NC-SA 2.0</skos:altLabel>
      <skos:altLabel xml:lang="nl">CC BY-NC-SA 2.0</skos:altLabel>
      <skos:altLabel xml:lang="pl">CC BY-NC-SA 2.0</skos:altLabel>
      <skos:altLabel xml:lang="pt">CC BY-NC-SA 2.0</skos:altLabel>
      <skos:altLabel xml:lang="ro">CC BY-NC-SA 2.0</skos:altLabel>
      <skos:altLabel xml:lang="sk">CC BY-NC-SA 2.0</skos:altLabel>
      <skos:altLabel xml:lang="sl">CC BY-NC-SA 2.0</skos:altLabel>
      <skos:altLabel xml:lang="sv">CC BY-NC-SA 2.0</skos:altLabel>
      <skos:definition xml:lang="en">CC BY-NC-SA 2.0 lets others remix, tweak, and build upon the author’s work non-commercially, as long as they credit the author and licence their new creations under the identical terms.</skos:definition>
      <skos:definition xml:lang="fr">CC BY-NC-SA 2.0 permet aux autres de remixer, arranger, et adapter l’œuvre de l’auteur/autrice à des fins non commerciales tant qu’on le/la crédite en citant son nom et que les nouvelles œuvres sont diffusées selon les mêmes conditions.</skos:definition>
      <skos:exactMatch rdf:resource="http://creativecommons.org/licenses/by-nc-sa/2.0/"/>
      <skos:inScheme rdf:resource="http://publications.europa.eu/resource/authority/licence"/>
      <skos:topConceptOf rdf:resource="http://publications.europa.eu/resource/authority/licence"/>
   </skos:Concept>
   <skos:Concept rdf:about="http://publications.europa.eu/resource/authority/licence/CC_BYNCSA_2_5"
                 at:deprecated="false">
      <skos:prefLabel xml:lang="bg">Creative Commons Признание-Некомерсиално-Споделяне на споделеното 2.5 Неадаптиран</skos:prefLabel>
      <skos:prefLabel xml:lang="cs">Creative Commons Uveďte původ–Neužívejte dílo komerčně–Zachovejte licenci 2.5 Generic</skos:prefLabel>
      <skos:prefLabel xml:lang="da">Creative Commons Kreditering-Ikkekommerciel-Deling på samme vilkår 2.5 Generisk</skos:prefLabel>
      <skos:prefLabel xml:lang="de">Creative Commons Namensnennung – Nicht-kommerziell – Weitergabe unter gleichen Bedingungen 2.5 Generic</skos:prefLabel>
      <skos:prefLabel xml:lang="el">Creative Commons Αναφορά Δημιουργού – Μη Εμπορική Χρήση – Παρόμοια Διανομή 2.5 Γενικό</skos:prefLabel>
      <skos:prefLabel xml:lang="en">Creative Commons Attribution–NonCommercial–ShareAlike 2.5 Generic</skos:prefLabel>
      <skos:prefLabel xml:lang="es">Creative Commons Atribución–NoComercial–CompartirIgual 2.5 Genérica</skos:prefLabel>
      <skos:prefLabel xml:lang="et">Creative Commons Autorile viitamine–Mitteäriline eesmärk–Jagamine samadel tingimustel 2.5 Üldine</skos:prefLabel>
      <skos:prefLabel xml:lang="fi">Creative Commons Nimeä–EiKaupallinen–JaaSamoin 2.5 Yleinen</skos:prefLabel>
      <skos:prefLabel xml:lang="fr">Creative Commons Attribution – Pas d’Utilisation Commerciale – Partage dans les Mêmes Conditions 2.5 Générique</skos:prefLabel>
      <skos:prefLabel xml:lang="hr">Creative Commons Imenovanje–Nekomercijalno–Dijeli pod istim uvjetima 2.5 nelokalizirana licenca</skos:prefLabel>
      <skos:prefLabel xml:lang="hu">Creative Commons Nevezd meg! – Ne add el! – Így add tovább! 2.5 Általános</skos:prefLabel>
      <skos:prefLabel xml:lang="it">Creative Commons Attribuzione – Non commerciale – Condividi allo stesso modo 2.5 Generico</skos:prefLabel>
      <skos:prefLabel xml:lang="lt">Creative Commons Priskyrimas – Nekomercinis platinimas – Analogiškas platinimas 2.5 Bendrasis</skos:prefLabel>
      <skos:prefLabel xml:lang="lv">Creative Commons Atsaucoties–Nekomerciāli–Nemainot licenci 2.5 Vispārīgs</skos:prefLabel>
      <skos:prefLabel xml:lang="mt">Creative Commons Attribuzzjoni-MhuxKummerċjali-KondiviżjoniUgwali 2.5 Generic</skos:prefLabel>
      <skos:prefLabel xml:lang="nl">Creative Commons Naamsvermelding–NietCommercieel–GelijkDelen 2.5 Unported</skos:prefLabel>
      <skos:prefLabel xml:lang="pl">Creative Commons Uznanie autorstwa–Użycie niekomercyjne–Na tych samych warunkach 2.5 Ogólny</skos:prefLabel>
      <skos:prefLabel xml:lang="pt">Creative Commons Atribuição–NãoComercial–CompartilhaIgual 2.5 Genérica</skos:prefLabel>
      <skos:prefLabel xml:lang="ro">Creative Commons Atribuire–Necomercial–Distribuire în Condiţii Identice 2.5 Generică</skos:prefLabel>
      <skos:prefLabel xml:lang="sk">Creative Commons Uvedenie Autora-Nekomerčné Použitie-Rovnaké Šírenie 2.5 Generic</skos:prefLabel>
      <skos:prefLabel xml:lang="sl">Creative Commons Priznanje avtorstva-Nekomercialno-Deljenje pod enakimi pogoji 2.5 Generična</skos:prefLabel>
      <skos:prefLabel xml:lang="sv">Creative Commons Erkännande–IckeKommersiell–DelaLika 2.5 Generisk</skos:prefLabel>
      <at:authority-code>CC_BYNCSA_2_5</at:authority-code>
      <at:op-code>CC_BYNCSA_2_5</at:op-code>
      <at:start.use>2005-06-01</at:start.use>
      <atold:op-code>CC_BYNCSA_2_5</atold:op-code>
      <dc:identifier>CC_BYNCSA_2_5</dc:identifier>
      <skos:altLabel xml:lang="bg">CC BY-NC-SA 2.5</skos:altLabel>
      <skos:altLabel xml:lang="cs">CC BY-NC-SA 2.5</skos:altLabel>
      <skos:altLabel xml:lang="da">CC BY-NC-SA 2.5</skos:altLabel>
      <skos:altLabel xml:lang="de">CC BY-NC-SA 2.5</skos:altLabel>
      <skos:altLabel xml:lang="el">CC BY-NC-SA 2.5</skos:altLabel>
      <skos:altLabel xml:lang="en">CC BY-NC-SA 2.5</skos:altLabel>
      <skos:altLabel xml:lang="es">CC BY-NC-SA 2.5</skos:altLabel>
      <skos:altLabel xml:lang="et">CC BY-NC-SA 2.5</skos:altLabel>
      <skos:altLabel xml:lang="fi">CC BY-NC-SA 2.5</skos:altLabel>
      <skos:altLabel xml:lang="fr">CC BY-NC-SA 2.5</skos:altLabel>
      <skos:altLabel xml:lang="ga">CC BY-NC-SA 2.5</skos:altLabel>
      <skos:altLabel xml:lang="hr">CC BY-NC-SA 2.5</skos:altLabel>
      <skos:altLabel xml:lang="hu">CC BY-NC-SA 2.5</skos:altLabel>
      <skos:altLabel xml:lang="it">CC BY-NC-SA 2.5</skos:altLabel>
      <skos:altLabel xml:lang="lt">CC BY-NC-SA 2.5</skos:altLabel>
      <skos:altLabel xml:lang="lv">CC BY-NC-SA 2.5</skos:altLabel>
      <skos:altLabel xml:lang="mt">CC BY-NC-SA 2.5</skos:altLabel>
      <skos:altLabel xml:lang="nl">CC BY-NC-SA 2.5</skos:altLabel>
      <skos:altLabel xml:lang="pl">CC BY-NC-SA 2.5</skos:altLabel>
      <skos:altLabel xml:lang="pt">CC BY-NC-SA 2.5</skos:altLabel>
      <skos:altLabel xml:lang="ro">CC BY-NC-SA 2.5</skos:altLabel>
      <skos:altLabel xml:lang="sk">CC BY-NC-SA 2.5</skos:altLabel>
      <skos:altLabel xml:lang="sl">CC BY-NC-SA 2.5</skos:altLabel>
      <skos:altLabel xml:lang="sv">CC BY-NC-SA 2.5</skos:altLabel>
      <skos:definition xml:lang="en">CC BY-NC-SA 2.5 lets others remix, tweak, and build upon the author’s work non-commercially, as long as they credit the author and licence their new creations under the identical terms.</skos:definition>
      <skos:definition xml:lang="fr">CC BY-NC-SA 2.5 permet aux autres de remixer, arranger, et adapter l’œuvre de l’auteur/autrice à des fins non commerciales tant qu’on le/la crédite en citant son nom et que les nouvelles œuvres sont diffusées selon les mêmes conditions.</skos:definition>
      <skos:exactMatch rdf:resource="http://creativecommons.org/licenses/by-nc-sa/2.5/"/>
      <skos:inScheme rdf:resource="http://publications.europa.eu/resource/authority/licence"/>
      <skos:topConceptOf rdf:resource="http://publications.europa.eu/resource/authority/licence"/>
   </skos:Concept>
   <skos:Concept rdf:about="http://publications.europa.eu/resource/authority/licence/CC_BYNCSA_3_0"
                 at:deprecated="false">
      <skos:prefLabel xml:lang="bg">Creative Commons Признание-Некомерсиално-Споделяне на споделеното 3.0 Нелокализиран</skos:prefLabel>
      <skos:prefLabel xml:lang="cs">Creative Commons Uveďte původ–Neužívejte dílo komerčně–Zachovejte licenci 3.0 Unported</skos:prefLabel>
      <skos:prefLabel xml:lang="da">Creative Commons Kreditering-Ikkekommerciel-Deling på samme vilkår 3.0 Ikke porteret</skos:prefLabel>
      <skos:prefLabel xml:lang="de">Creative Commons Namensnennung – Nicht-kommerziell – Weitergabe unter gleichen Bedingungen 3.0 Unported</skos:prefLabel>
      <skos:prefLabel xml:lang="el">Creative Commons Αναφορά Δημιουργού – Μη Εμπορική Χρήση – Παρόμοια Διανομή 3.0 Μη εισαγόμενο</skos:prefLabel>
      <skos:prefLabel xml:lang="en">Creative Commons Attribution–NonCommercial–ShareAlike 3.0 Unported</skos:prefLabel>
      <skos:prefLabel xml:lang="es">Creative Commons Atribución–NoComercial–CompartirIgual 3.0 Unported</skos:prefLabel>
      <skos:prefLabel xml:lang="et">Creative Commons Autorile viitamine–Mitteäriline eesmärk–Jagamine samadel tingimustel 3.0 Jurisdiktsiooniga sidumata</skos:prefLabel>
      <skos:prefLabel xml:lang="fi">Creative Commons Nimeä–EiKaupallinen–JaaSamoin 3.0 Ei sovitettu</skos:prefLabel>
      <skos:prefLabel xml:lang="fr">Creative Commons Attribution – Pas d’Utilisation Commerciale – Partage dans les Mêmes Conditions 3.0 non transposé</skos:prefLabel>
      <skos:prefLabel xml:lang="hr">Creative Commons Imenovanje–Nekomercijalno–Dijeli pod istim uvjetima 3.0 nelokalizirana licenca</skos:prefLabel>
      <skos:prefLabel xml:lang="hu">Creative Commons Nevezd meg! – Ne add el! – Így add tovább! 3.0 Unported</skos:prefLabel>
      <skos:prefLabel xml:lang="it">Creative Commons Attribuzione – Non commerciale – Condividi allo stesso modo 3.0 Unported</skos:prefLabel>
      <skos:prefLabel xml:lang="lt">Creative Commons Priskyrimas – Nekomercinis platinimas – Analogiškas platinimas 3.0 Nepritaikyta jurisdikcijai</skos:prefLabel>
      <skos:prefLabel xml:lang="lv">Creative Commons Atsaucoties–Nekomerciāli–Nemainot licenci 3.0 Nepārnesta</skos:prefLabel>
      <skos:prefLabel xml:lang="mt">Creative Commons Attribuzzjoni-MhuxKummerċjali-KondiviżjoniUgwali 3.0 Unported</skos:prefLabel>
      <skos:prefLabel xml:lang="nl">Creative Commons Naamsvermelding–NietCommercieel–GelijkDelen 3.0 Unported</skos:prefLabel>
      <skos:prefLabel xml:lang="pl">Creative Commons Uznanie autorstwa–Użycie niekomercyjne–Na tych samych warunkach 3.0 Unported</skos:prefLabel>
      <skos:prefLabel xml:lang="pt">Creative Commons Atribuição–NãoComercial–CompartilhaIgual 3.0 Não Adaptada</skos:prefLabel>
      <skos:prefLabel xml:lang="ro">Creative Commons Atribuire–Necomercial–Distribuire în Condiţii Identice 3.0 Ne-adaptată</skos:prefLabel>
      <skos:prefLabel xml:lang="sk">Creative Commons Uvedenie Autora-Nekomerčné Použitie-Rovnaké Šírenie 3.0 Unported</skos:prefLabel>
      <skos:prefLabel xml:lang="sl">Creative Commons Priznanje avtorstva-Nekomercialno-Deljenje pod enakimi pogoji 3.0 Nedoločena</skos:prefLabel>
      <skos:prefLabel xml:lang="sv">Creative Commons Erkännande–IckeKommersiell–DelaLika 3.0 Unported</skos:prefLabel>
      <at:authority-code>CC_BYNCSA_3_0</at:authority-code>
      <at:op-code>CC_BYNCSA_3_0</at:op-code>
      <at:start.use>2007-02-23</at:start.use>
      <atold:op-code>CC_BYNCSA_3_0</atold:op-code>
      <dc:identifier>CC_BYNCSA_3_0</dc:identifier>
      <skos:altLabel xml:lang="bg">CC BY-NC-SA 3.0</skos:altLabel>
      <skos:altLabel xml:lang="cs">CC BY-NC-SA 3.0</skos:altLabel>
      <skos:altLabel xml:lang="da">CC BY-NC-SA 3.0</skos:altLabel>
      <skos:altLabel xml:lang="de">CC BY-NC-SA 3.0</skos:altLabel>
      <skos:altLabel xml:lang="el">CC BY-NC-SA 3.0</skos:altLabel>
      <skos:altLabel xml:lang="en">CC BY-NC-SA 3.0</skos:altLabel>
      <skos:altLabel xml:lang="es">CC BY-NC-SA 3.0</skos:altLabel>
      <skos:altLabel xml:lang="et">CC BY-NC-SA 3.0</skos:altLabel>
      <skos:altLabel xml:lang="fi">CC BY-NC-SA 3.0</skos:altLabel>
      <skos:altLabel xml:lang="fr">CC BY-NC-SA 3.0</skos:altLabel>
      <skos:altLabel xml:lang="ga">CC BY-NC-SA 3.0</skos:altLabel>
      <skos:altLabel xml:lang="hr">CC BY-NC-SA 3.0</skos:altLabel>
      <skos:altLabel xml:lang="hu">CC BY-NC-SA 3.0</skos:altLabel>
      <skos:altLabel xml:lang="it">CC BY-NC-SA 3.0</skos:altLabel>
      <skos:altLabel xml:lang="lt">CC BY-NC-SA 3.0</skos:altLabel>
      <skos:altLabel xml:lang="lv">CC BY-NC-SA 3.0</skos:altLabel>
      <skos:altLabel xml:lang="mt">CC BY-NC-SA 3.0</skos:altLabel>
      <skos:altLabel xml:lang="nl">CC BY-NC-SA 3.0</skos:altLabel>
      <skos:altLabel xml:lang="pl">CC BY-NC-SA 3.0</skos:altLabel>
      <skos:altLabel xml:lang="pt">CC BY-NC-SA 3.0</skos:altLabel>
      <skos:altLabel xml:lang="ro">CC BY-NC-SA 3.0</skos:altLabel>
      <skos:altLabel xml:lang="sk">CC BY-NC-SA 3.0</skos:altLabel>
      <skos:altLabel xml:lang="sl">CC BY-NC-SA 3.0</skos:altLabel>
      <skos:altLabel xml:lang="sv">CC BY-NC-SA 3.0</skos:altLabel>
      <skos:definition xml:lang="en">CC BY-NC-SA 3.0 lets others remix, tweak, and build upon the author’s work non-commercially, as long as they credit the author and licence their new creations under the identical terms.</skos:definition>
      <skos:definition xml:lang="fr">CC BY-NC-SA 3.0 permet aux autres de remixer, arranger, et adapter l’œuvre de l’auteur/autrice à des fins non commerciales tant qu’on le/la crédite en citant son nom et que les nouvelles œuvres sont diffusées selon les mêmes conditions.</skos:definition>
      <skos:exactMatch rdf:resource="http://creativecommons.org/licenses/by-nc-sa/3.0/"/>
      <skos:inScheme rdf:resource="http://publications.europa.eu/resource/authority/licence"/>
      <skos:topConceptOf rdf:resource="http://publications.europa.eu/resource/authority/licence"/>
      <skos:historyNote xml:lang="en">Unported licences are licences that are not associated with any specific jurisdiction, e.g. country.</skos:historyNote>
   </skos:Concept>
   <skos:Concept rdf:about="http://publications.europa.eu/resource/authority/licence/CC_BYNCSA_4_0"
                 at:deprecated="false">
      <skos:prefLabel xml:lang="cs">Creative Commons Uveďte původ–Neužívejte dílo komerčně–Zachovejte licenci 4.0 Mezinárodní</skos:prefLabel>
      <skos:prefLabel xml:lang="de">Creative Commons Namensnennung – Nicht-kommerziell – Weitergabe unter gleichen Bedingungen 4.0 International</skos:prefLabel>
      <skos:prefLabel xml:lang="el">Creative Commons Αναφορά Δημιουργού – Μη Εμπορική Χρήση – Παρόμοια Διανομή 4.0 Διεθνές</skos:prefLabel>
      <skos:prefLabel xml:lang="en">Creative Commons Attribution–NonCommercial–ShareAlike 4.0 International</skos:prefLabel>
      <skos:prefLabel xml:lang="es">Creative Commons Atribución–NoComercial–CompartirIgual 4.0 Internacional</skos:prefLabel>
      <skos:prefLabel xml:lang="fi">Creative Commons Nimeä–EiKaupallinen–JaaSamoin 4.0 Kansainvälinen</skos:prefLabel>
      <skos:prefLabel xml:lang="fr">Creative Commons Attribution – Pas d’Utilisation Commerciale – Partage dans les Mêmes Conditions 4.0 International</skos:prefLabel>
      <skos:prefLabel xml:lang="hr">Creative Commons Imenovanje–Nekomercijalno–Dijeli pod istim uvjetima 4.0 međunarodna</skos:prefLabel>
      <skos:prefLabel xml:lang="hu">Creative Commons Nevezd meg! – Ne add el! – Így add tovább! 4.0 Nemzetközi</skos:prefLabel>
      <skos:prefLabel xml:lang="it">Creative Commons Attribuzione – Non commerciale – Condividi allo stesso modo 4.0 Internazionale</skos:prefLabel>
      <skos:prefLabel xml:lang="lt">Creative Commons Priskyrimas – Nekomercinis platinimas – Analogiškas platinimas 4.0 Tarptautinė</skos:prefLabel>
      <skos:prefLabel xml:lang="lv">Creative Commons Atsaucoties–Nekomerciāli–Nemainot licenci 4.0 Internacionāls</skos:prefLabel>
      <skos:prefLabel xml:lang="nl">Creative Commons Naamsvermelding–NietCommercieel–GelijkDelen 4.0 Internationaal</skos:prefLabel>
      <skos:prefLabel xml:lang="pl">Creative Commons Uznanie autorstwa–Użycie niekomercyjne–Na tych samych warunkach 4.0 Międzynarodowe</skos:prefLabel>
      <skos:prefLabel xml:lang="pt">Creative Commons Atribuição–NãoComercial–CompartilhaIgual 4.0 Internacional</skos:prefLabel>
      <skos:prefLabel xml:lang="ro">Creative Commons Atribuire–Necomercial–Distribuire în Condiţii Identice 4.0 Internațional</skos:prefLabel>
      <skos:prefLabel xml:lang="sv">Creative Commons Erkännande–IckeKommersiell–DelaLika 4.0 Internationell</skos:prefLabel>
      <skos:prefLabel xml:lang="bg">Creative Commons Признание-Некомерсиално-Споделяне на споделеното 4.0 Международен</skos:prefLabel>
      <skos:prefLabel xml:lang="da">Creative Commons Kreditering-Ikkekommerciel-Deling på samme vilkår 4.0 International</skos:prefLabel>
      <skos:prefLabel xml:lang="et">Creative Commons Autorile viitamine–Mitteäriline eesmärk–Jagamine samadel tingimustel 4.0 Rahvusvaheline</skos:prefLabel>
      <skos:prefLabel xml:lang="mt">Creative Commons Attribuzzjoni-MhuxKummerċjali-KondiviżjoniUgwali 4.0 Internazzjonali</skos:prefLabel>
      <skos:prefLabel xml:lang="sk">Creative Commons Uvedenie Autora-Nekomerčné Použitie-Rovnaké Šírenie 4.0 Medzinárodný</skos:prefLabel>
      <skos:prefLabel xml:lang="sl">Creative Commons Priznanje avtorstva-Nekomercialno-Deljenje pod enakimi pogoji 4.0 Mednarodna</skos:prefLabel>
      <at:authority-code>CC_BYNCSA_4_0</at:authority-code>
      <at:op-code>CC_BYNCSA_4_0</at:op-code>
      <at:start.use>2013-11-26</at:start.use>
      <atold:op-code>CC_BYNCSA_4_0</atold:op-code>
      <dc:identifier>CC_BYNCSA_4_0</dc:identifier>
      <skos:altLabel xml:lang="bg">CC BY-NC-SA 4.0</skos:altLabel>
      <skos:altLabel xml:lang="cs">CC BY-NC-SA 4.0</skos:altLabel>
      <skos:altLabel xml:lang="da">CC BY-NC-SA 4.0</skos:altLabel>
      <skos:altLabel xml:lang="de">CC BY-NC-SA 4.0</skos:altLabel>
      <skos:altLabel xml:lang="el">CC BY-NC-SA 4.0</skos:altLabel>
      <skos:altLabel xml:lang="en">CC BY-NC-SA 4.0</skos:altLabel>
      <skos:altLabel xml:lang="es">CC BY-NC-SA 4.0</skos:altLabel>
      <skos:altLabel xml:lang="et">CC BY-NC-SA 4.0</skos:altLabel>
      <skos:altLabel xml:lang="fi">CC BY-NC-SA 4.0</skos:altLabel>
      <skos:altLabel xml:lang="fr">CC BY-NC-SA 4.0</skos:altLabel>
      <skos:altLabel xml:lang="ga">CC BY-NC-SA 4.0</skos:altLabel>
      <skos:altLabel xml:lang="hr">CC BY-NC-SA 4.0</skos:altLabel>
      <skos:altLabel xml:lang="hu">CC BY-NC-SA 4.0</skos:altLabel>
      <skos:altLabel xml:lang="it">CC BY-NC-SA 4.0</skos:altLabel>
      <skos:altLabel xml:lang="lt">CC BY-NC-SA 4.0</skos:altLabel>
      <skos:altLabel xml:lang="lv">CC BY-NC-SA 4.0</skos:altLabel>
      <skos:altLabel xml:lang="mt">CC BY-NC-SA 4.0</skos:altLabel>
      <skos:altLabel xml:lang="nl">CC BY-NC-SA 4.0</skos:altLabel>
      <skos:altLabel xml:lang="pl">CC BY-NC-SA 4.0</skos:altLabel>
      <skos:altLabel xml:lang="pt">CC BY-NC-SA 4.0</skos:altLabel>
      <skos:altLabel xml:lang="ro">CC BY-NC-SA 4.0</skos:altLabel>
      <skos:altLabel xml:lang="sk">CC BY-NC-SA 4.0</skos:altLabel>
      <skos:altLabel xml:lang="sl">CC BY-NC-SA 4.0</skos:altLabel>
      <skos:altLabel xml:lang="sv">CC BY-NC-SA 4.0</skos:altLabel>
      <skos:definition xml:lang="en">CC BY-NC-SA 4.0 lets others remix, tweak, and build upon the author’s work non-commercially, as long as they credit the author and licence their new creations under the identical terms.</skos:definition>
      <skos:definition xml:lang="fr">CC BY-NC-SA 4.0 permet aux autres de remixer, arranger, et adapter l’œuvre de l’auteur/autrice à des fins non commerciales tant qu’on le/la crédite en citant son nom et que les nouvelles œuvres sont diffusées selon les mêmes conditions.</skos:definition>
      <skos:exactMatch rdf:resource="http://creativecommons.org/licenses/by-nc-sa/4.0/"/>
      <skos:inScheme rdf:resource="http://publications.europa.eu/resource/authority/licence"/>
      <skos:topConceptOf rdf:resource="http://publications.europa.eu/resource/authority/licence"/>
   </skos:Concept>
   <skos:Concept rdf:about="http://publications.europa.eu/resource/authority/licence/CC_BYNC_1_0"
                 at:deprecated="true">
      <skos:prefLabel xml:lang="bg">Creative Commons Признание-Некомерсиално 1.0 Неадаптиран</skos:prefLabel>
      <skos:prefLabel xml:lang="cs">Creative Commons Uveďte původ–Neužívejte komerčně 1.0 Generic</skos:prefLabel>
      <skos:prefLabel xml:lang="da">Creative Commons Kreditering-Ikkekommerciel 1.0 Generisk</skos:prefLabel>
      <skos:prefLabel xml:lang="de">Creative Commons Namensnennung – Nicht kommerziell 1.0 Generic</skos:prefLabel>
      <skos:prefLabel xml:lang="el">Creative Commons Αναφορά Δημιουργού – Μη Εμπορική Χρήση 1.0 Γενικό</skos:prefLabel>
      <skos:prefLabel xml:lang="en">Creative Commons Attribution–NonCommercial 1.0 Generic</skos:prefLabel>
      <skos:prefLabel xml:lang="es">Creative Commons Atribución–NoComercial 1.0 Genérica</skos:prefLabel>
      <skos:prefLabel xml:lang="et">Creative Commons Autorile viitamine–Mitteäriline eesmärk 1.0 Üldine</skos:prefLabel>
      <skos:prefLabel xml:lang="fi">Creative Commons Nimeä–EiKaupallinen 1.0 Yleinen</skos:prefLabel>
      <skos:prefLabel xml:lang="fr">Creative Commons Attribution – Pas d’Utilisation Commerciale 1.0 Générique</skos:prefLabel>
      <skos:prefLabel xml:lang="hr">Creative Commons Imenovanje–Nekomercijalno 1.0 nelokalizirana licenca</skos:prefLabel>
      <skos:prefLabel xml:lang="hu">Creative Commons Nevezd meg! – Ne add el! 1.0 Általános</skos:prefLabel>
      <skos:prefLabel xml:lang="it">Creative Commons Attribuzione – Non commerciale 1.0 Generico</skos:prefLabel>
      <skos:prefLabel xml:lang="lt">Creative Commons Priskyrimas – Nekomercinis platinimas 1.0 Bendrasis</skos:prefLabel>
      <skos:prefLabel xml:lang="lv">Creative Commons Atsaucoties–Nekomerciāli 1.0 Vispārīgs</skos:prefLabel>
      <skos:prefLabel xml:lang="mt">Creative Commons Attribuzzjoni-MhuxKummerċjali 1.0 Generic</skos:prefLabel>
      <skos:prefLabel xml:lang="nl">Creative Commons Naamsvermelding–NietCommercieel 1.0 Unported</skos:prefLabel>
      <skos:prefLabel xml:lang="pl">Creative Commons Uznanie autorstwa–Użycie niekomercyjne 1.0 Ogólny</skos:prefLabel>
      <skos:prefLabel xml:lang="pt">Creative Commons Atribuição–NãoComercial 1.0 Genérica</skos:prefLabel>
      <skos:prefLabel xml:lang="ro">Creative Commons Atribuire–Necomercial 1.0 Generică</skos:prefLabel>
      <skos:prefLabel xml:lang="sk">Creative Commons Uvedenie Autora-Nekomerčné Použitie 1.0 Generic</skos:prefLabel>
      <skos:prefLabel xml:lang="sl">Creative Commons Priznanje avtorstva-Nekomercialno 1.0 Generična</skos:prefLabel>
      <skos:prefLabel xml:lang="sv">Creative Commons Erkännande–IckeKommersiell 1.0 Generisk</skos:prefLabel>
      <at:authority-code>CC_BYNC_1_0</at:authority-code>
      <at:op-code>CC_BYNC_1_0</at:op-code>
      <at:start.use>2002-12-15</at:start.use>
      <atold:op-code>CC_BYNC_1_0</atold:op-code>
      <dc:identifier>CC_BYNC_1_0</dc:identifier>
      <skos:altLabel xml:lang="bg">CC BY-NC 1.0</skos:altLabel>
      <skos:altLabel xml:lang="cs">CC BY-NC 1.0</skos:altLabel>
      <skos:altLabel xml:lang="da">CC BY-NC 1.0</skos:altLabel>
      <skos:altLabel xml:lang="de">CC BY-NC 1.0</skos:altLabel>
      <skos:altLabel xml:lang="el">CC BY-NC 1.0</skos:altLabel>
      <skos:altLabel xml:lang="en">CC BY-NC 1.0</skos:altLabel>
      <skos:altLabel xml:lang="es">CC BY-NC 1.0</skos:altLabel>
      <skos:altLabel xml:lang="et">CC BY-NC 1.0</skos:altLabel>
      <skos:altLabel xml:lang="fi">CC BY-NC 1.0</skos:altLabel>
      <skos:altLabel xml:lang="fr">CC BY-NC 1.0</skos:altLabel>
      <skos:altLabel xml:lang="ga">CC BY-NC 1.0</skos:altLabel>
      <skos:altLabel xml:lang="hr">CC BY-NC 1.0</skos:altLabel>
      <skos:altLabel xml:lang="hu">CC BY-NC 1.0</skos:altLabel>
      <skos:altLabel xml:lang="it">CC BY-NC 1.0</skos:altLabel>
      <skos:altLabel xml:lang="lt">CC BY-NC 1.0</skos:altLabel>
      <skos:altLabel xml:lang="lv">CC BY-NC 1.0</skos:altLabel>
      <skos:altLabel xml:lang="mt">CC BY-NC 1.0</skos:altLabel>
      <skos:altLabel xml:lang="nl">CC BY-NC 1.0</skos:altLabel>
      <skos:altLabel xml:lang="pl">CC BY-NC 1.0</skos:altLabel>
      <skos:altLabel xml:lang="pt">CC BY-NC 1.0</skos:altLabel>
      <skos:altLabel xml:lang="ro">CC BY-NC 1.0</skos:altLabel>
      <skos:altLabel xml:lang="sk">CC BY-NC 1.0</skos:altLabel>
      <skos:altLabel xml:lang="sl">CC BY-NC 1.0</skos:altLabel>
      <skos:altLabel xml:lang="sv">CC BY-NC 1.0</skos:altLabel>
      <skos:definition xml:lang="en">CC BY-NC 1.0 lets others remix, tweak, and build upon the author’s work non-commercially, and although their new works must also acknowledge the author and be non-commercial, they don’t have to licence their derivative works on the same terms.</skos:definition>
      <skos:definition xml:lang="fr">CC BY-NC 1.0 permet aux autres de remixer, arranger, et adapter l’œuvre de l’auteur/autrice à des fins non commerciales et, bien que les nouvelles œuvres doivent créditer l’auteur/autrice en citant son nom et ne pas constituer une utilisation commerciale, elles n’ont pas à être diffusées selon les mêmes conditions.</skos:definition>
      <skos:exactMatch rdf:resource="http://creativecommons.org/licenses/by-nc/1.0/"/>
      <skos:inScheme rdf:resource="http://publications.europa.eu/resource/authority/licence"/>
      <skos:topConceptOf rdf:resource="http://publications.europa.eu/resource/authority/licence"/>
      <at:end.use>2004-05-24</at:end.use>
   </skos:Concept>
   <skos:Concept rdf:about="http://publications.europa.eu/resource/authority/licence/CC_BYNC_2_0"
                 at:deprecated="false">
      <skos:prefLabel xml:lang="bg">Creative Commons Признание-Некомерсиално 2.0 Неадаптиран</skos:prefLabel>
      <skos:prefLabel xml:lang="cs">Creative Commons Uveďte původ–Neužívejte komerčně 2.0 Generic</skos:prefLabel>
      <skos:prefLabel xml:lang="da">Creative Commons Kreditering-Ikkekommerciel 2.0 Generisk</skos:prefLabel>
      <skos:prefLabel xml:lang="de">Creative Commons Namensnennung – Nicht kommerziell 2.0 Generic</skos:prefLabel>
      <skos:prefLabel xml:lang="el">Creative Commons Αναφορά Δημιουργού – Μη Εμπορική Χρήση 2.0 Γενικό</skos:prefLabel>
      <skos:prefLabel xml:lang="en">Creative Commons Attribution–NonCommercial 2.0 Generic</skos:prefLabel>
      <skos:prefLabel xml:lang="es">Creative Commons Atribución–NoComercial 2.0 Genérica</skos:prefLabel>
      <skos:prefLabel xml:lang="et">Creative Commons Autorile viitamine–Mitteäriline eesmärk 2.0 Üldine</skos:prefLabel>
      <skos:prefLabel xml:lang="fi">Creative Commons Nimeä–EiKaupallinen 2.0 Yleinen</skos:prefLabel>
      <skos:prefLabel xml:lang="fr">Creative Commons Attribution – Pas d’Utilisation Commerciale 2.0 Générique</skos:prefLabel>
      <skos:prefLabel xml:lang="hr">Creative Commons Imenovanje–Nekomercijalno 2.0 nelokalizirana licenca</skos:prefLabel>
      <skos:prefLabel xml:lang="hu">Creative Commons Nevezd meg! – Ne add el! 2.0 Általános</skos:prefLabel>
      <skos:prefLabel xml:lang="it">Creative Commons Attribuzione – Non commerciale 2.0 Generico</skos:prefLabel>
      <skos:prefLabel xml:lang="lt">Creative Commons Priskyrimas – Nekomercinis platinimas 2.0 Bendrasis</skos:prefLabel>
      <skos:prefLabel xml:lang="lv">Creative Commons Atsaucoties–Nekomerciāli 2.0 Vispārīgs</skos:prefLabel>
      <skos:prefLabel xml:lang="mt">Creative Commons Attribuzzjoni-MhuxKummerċjali 2.0 Generic</skos:prefLabel>
      <skos:prefLabel xml:lang="nl">Creative Commons Naamsvermelding–NietCommercieel 2.0 Unported</skos:prefLabel>
      <skos:prefLabel xml:lang="pl">Creative Commons Uznanie autorstwa–Użycie niekomercyjne 2.0 Ogólny</skos:prefLabel>
      <skos:prefLabel xml:lang="pt">Creative Commons Atribuição–NãoComercial 2.0 Genérica</skos:prefLabel>
      <skos:prefLabel xml:lang="ro">Creative Commons Atribuire–Necomercial 2.0 Generică</skos:prefLabel>
      <skos:prefLabel xml:lang="sk">Creative Commons Uvedenie Autora-Nekomerčné Použitie 2.0 Generic</skos:prefLabel>
      <skos:prefLabel xml:lang="sl">Creative Commons Priznanje avtorstva-Nekomercialno 2.0 Generična</skos:prefLabel>
      <skos:prefLabel xml:lang="sv">Creative Commons Erkännande–IckeKommersiell 2.0 Generisk</skos:prefLabel>
      <at:authority-code>CC_BYNC_2_0</at:authority-code>
      <at:op-code>CC_BYNC_2_0</at:op-code>
      <at:start.use>2004-05-25</at:start.use>
      <atold:op-code>CC_BYNC_2_0</atold:op-code>
      <dc:identifier>CC_BYNC_2_0</dc:identifier>
      <skos:altLabel xml:lang="bg">CC BY-NC 2.0</skos:altLabel>
      <skos:altLabel xml:lang="cs">CC BY-NC 2.0</skos:altLabel>
      <skos:altLabel xml:lang="da">CC BY-NC 2.0</skos:altLabel>
      <skos:altLabel xml:lang="de">CC BY-NC 2.0</skos:altLabel>
      <skos:altLabel xml:lang="el">CC BY-NC 2.0</skos:altLabel>
      <skos:altLabel xml:lang="en">CC BY-NC 2.0</skos:altLabel>
      <skos:altLabel xml:lang="es">CC BY-NC 2.0</skos:altLabel>
      <skos:altLabel xml:lang="et">CC BY-NC 2.0</skos:altLabel>
      <skos:altLabel xml:lang="fi">CC BY-NC 2.0</skos:altLabel>
      <skos:altLabel xml:lang="fr">CC BY-NC 2.0</skos:altLabel>
      <skos:altLabel xml:lang="ga">CC BY-NC 2.0</skos:altLabel>
      <skos:altLabel xml:lang="hr">CC BY-NC 2.0</skos:altLabel>
      <skos:altLabel xml:lang="hu">CC BY-NC 2.0</skos:altLabel>
      <skos:altLabel xml:lang="it">CC BY-NC 2.0</skos:altLabel>
      <skos:altLabel xml:lang="lt">CC BY-NC 2.0</skos:altLabel>
      <skos:altLabel xml:lang="lv">CC BY-NC 2.0</skos:altLabel>
      <skos:altLabel xml:lang="mt">CC BY-NC 2.0</skos:altLabel>
      <skos:altLabel xml:lang="nl">CC BY-NC 2.0</skos:altLabel>
      <skos:altLabel xml:lang="pl">CC BY-NC 2.0</skos:altLabel>
      <skos:altLabel xml:lang="pt">CC BY-NC 2.0</skos:altLabel>
      <skos:altLabel xml:lang="ro">CC BY-NC 2.0</skos:altLabel>
      <skos:altLabel xml:lang="sk">CC BY-NC 2.0</skos:altLabel>
      <skos:altLabel xml:lang="sl">CC BY-NC 2.0</skos:altLabel>
      <skos:altLabel xml:lang="sv">CC BY-NC 2.0</skos:altLabel>
      <skos:definition xml:lang="en">CC BY-NC 2.0 lets others remix, tweak, and build upon the author’s work non-commercially, and although their new works must also acknowledge the author and be non-commercial, they don’t have to licence their derivative works on the same terms.</skos:definition>
      <skos:definition xml:lang="fr">CC BY-NC 2.0 permet aux autres de remixer, arranger, et adapter l’œuvre de l’auteur/autrice à des fins non commerciales et, bien que les nouvelles œuvres doivent créditer l’auteur/autrice en citant son nom et ne pas constituer une utilisation commerciale, elles n’ont pas à être diffusées selon les mêmes conditions.</skos:definition>
      <skos:exactMatch rdf:resource="http://creativecommons.org/licenses/by-nc/2.0/"/>
      <skos:inScheme rdf:resource="http://publications.europa.eu/resource/authority/licence"/>
      <skos:topConceptOf rdf:resource="http://publications.europa.eu/resource/authority/licence"/>
   </skos:Concept>
   <skos:Concept rdf:about="http://publications.europa.eu/resource/authority/licence/CC_BYNC_2_5"
                 at:deprecated="false">
      <skos:prefLabel xml:lang="bg">Creative Commons Признание-Некомерсиално 2.5 Неадаптиран</skos:prefLabel>
      <skos:prefLabel xml:lang="cs">Creative Commons Uveďte původ–Neužívejte komerčně 2.5 Generic</skos:prefLabel>
      <skos:prefLabel xml:lang="da">Creative Commons Kreditering-Ikkekommerciel 2.5 Generisk</skos:prefLabel>
      <skos:prefLabel xml:lang="de">Creative Commons Namensnennung – Nicht kommerziell 2.5 Generic</skos:prefLabel>
      <skos:prefLabel xml:lang="el">Creative Commons Αναφορά Δημιουργού – Μη Εμπορική Χρήση 2.5 Γενικό</skos:prefLabel>
      <skos:prefLabel xml:lang="en">Creative Commons Attribution–NonCommercial 2.5 Generic</skos:prefLabel>
      <skos:prefLabel xml:lang="es">Creative Commons Atribución–NoComercial 2.5 Genérica</skos:prefLabel>
      <skos:prefLabel xml:lang="et">Creative Commons Autorile viitamine–Mitteäriline eesmärk 2.5 Üldine</skos:prefLabel>
      <skos:prefLabel xml:lang="fi">Creative Commons Nimeä–EiKaupallinen 2.5 Yleinen</skos:prefLabel>
      <skos:prefLabel xml:lang="fr">Creative Commons Attribution – Pas d’Utilisation Commerciale 2.5 Générique</skos:prefLabel>
      <skos:prefLabel xml:lang="hr">Creative Commons Imenovanje–Nekomercijalno 2.5 nelokalizirana licenca</skos:prefLabel>
      <skos:prefLabel xml:lang="hu">Creative Commons Nevezd meg! – Ne add el! 2.5 Általános</skos:prefLabel>
      <skos:prefLabel xml:lang="it">Creative Commons Attribuzione – Non commerciale 2.5 Generico</skos:prefLabel>
      <skos:prefLabel xml:lang="lt">Creative Commons Priskyrimas – Nekomercinis platinimas 2.5 Bendrasis</skos:prefLabel>
      <skos:prefLabel xml:lang="lv">Creative Commons Atsaucoties–Nekomerciāli 2.5 Vispārīgs</skos:prefLabel>
      <skos:prefLabel xml:lang="mt">Creative Commons Attribuzzjoni-MhuxKummerċjali 2.5 Generic</skos:prefLabel>
      <skos:prefLabel xml:lang="nl">Creative Commons Naamsvermelding–NietCommercieel 2.5 Unported</skos:prefLabel>
      <skos:prefLabel xml:lang="pl">Creative Commons Uznanie autorstwa–Użycie niekomercyjne 2.5 Ogólny</skos:prefLabel>
      <skos:prefLabel xml:lang="pt">Creative Commons Atribuição–NãoComercial 2.5 Genérica</skos:prefLabel>
      <skos:prefLabel xml:lang="ro">Creative Commons Atribuire–Necomercial 2.5 Generică</skos:prefLabel>
      <skos:prefLabel xml:lang="sk">Creative Commons Uvedenie Autora-Nekomerčné Použitie 2.5 Generic</skos:prefLabel>
      <skos:prefLabel xml:lang="sl">Creative Commons Priznanje avtorstva-Nekomercialno 2.5 Generična</skos:prefLabel>
      <skos:prefLabel xml:lang="sv">Creative Commons Erkännande–IckeKommersiell 2.5 Generisk</skos:prefLabel>
      <at:authority-code>CC_BYNC_2_5</at:authority-code>
      <at:op-code>CC_BYNC_2_5</at:op-code>
      <at:start.use>2005-06-01</at:start.use>
      <atold:op-code>CC_BYNC_2_5</atold:op-code>
      <dc:identifier>CC_BYNC_2_5</dc:identifier>
      <skos:altLabel xml:lang="bg">CC BY-NC 2.5</skos:altLabel>
      <skos:altLabel xml:lang="cs">CC BY-NC 2.5</skos:altLabel>
      <skos:altLabel xml:lang="da">CC BY-NC 2.5</skos:altLabel>
      <skos:altLabel xml:lang="de">CC BY-NC 2.5</skos:altLabel>
      <skos:altLabel xml:lang="el">CC BY-NC 2.5</skos:altLabel>
      <skos:altLabel xml:lang="en">CC BY-NC 2.5</skos:altLabel>
      <skos:altLabel xml:lang="es">CC BY-NC 2.5</skos:altLabel>
      <skos:altLabel xml:lang="et">CC BY-NC 2.5</skos:altLabel>
      <skos:altLabel xml:lang="fi">CC BY-NC 2.5</skos:altLabel>
      <skos:altLabel xml:lang="fr">CC BY-NC 2.5</skos:altLabel>
      <skos:altLabel xml:lang="ga">CC BY-NC 2.5</skos:altLabel>
      <skos:altLabel xml:lang="hr">CC BY-NC 2.5</skos:altLabel>
      <skos:altLabel xml:lang="hu">CC BY-NC 2.5</skos:altLabel>
      <skos:altLabel xml:lang="it">CC BY-NC 2.5</skos:altLabel>
      <skos:altLabel xml:lang="lt">CC BY-NC 2.5</skos:altLabel>
      <skos:altLabel xml:lang="lv">CC BY-NC 2.5</skos:altLabel>
      <skos:altLabel xml:lang="mt">CC BY-NC 2.5</skos:altLabel>
      <skos:altLabel xml:lang="nl">CC BY-NC 2.5</skos:altLabel>
      <skos:altLabel xml:lang="pl">CC BY-NC 2.5</skos:altLabel>
      <skos:altLabel xml:lang="pt">CC BY-NC 2.5</skos:altLabel>
      <skos:altLabel xml:lang="ro">CC BY-NC 2.5</skos:altLabel>
      <skos:altLabel xml:lang="sk">CC BY-NC 2.5</skos:altLabel>
      <skos:altLabel xml:lang="sl">CC BY-NC 2.5</skos:altLabel>
      <skos:altLabel xml:lang="sv">CC BY-NC 2.5</skos:altLabel>
      <skos:definition xml:lang="en">CC BY-NC 2.5 lets others remix, tweak, and build upon the author’s work non-commercially, and although their new works must also acknowledge the author and be non-commercial, they don’t have to licence their derivative works on the same terms.</skos:definition>
      <skos:definition xml:lang="fr">CC BY-NC 2.5 permet aux autres de remixer, arranger, et adapter l’œuvre de l’auteur/autrice à des fins non commerciales et, bien que les nouvelles œuvres doivent créditer l’auteur/autrice en citant son nom et ne pas constituer une utilisation commerciale, elles n’ont pas à être diffusées selon les mêmes conditions.</skos:definition>
      <skos:exactMatch rdf:resource="http://creativecommons.org/licenses/by-nc/2.5/"/>
      <skos:inScheme rdf:resource="http://publications.europa.eu/resource/authority/licence"/>
      <skos:topConceptOf rdf:resource="http://publications.europa.eu/resource/authority/licence"/>
   </skos:Concept>
   <skos:Concept rdf:about="http://publications.europa.eu/resource/authority/licence/CC_BYNC_3_0"
                 at:deprecated="false">
      <skos:prefLabel xml:lang="bg">Creative Commons Признание-Некомерсиално 3.0 Нелокализиран</skos:prefLabel>
      <skos:prefLabel xml:lang="cs">Creative Commons Uveďte původ–Neužívejte komerčně 3.0 Unported</skos:prefLabel>
      <skos:prefLabel xml:lang="da">Creative Commons Kreditering-Ikkekommerciel 3.0 Ikke porteret</skos:prefLabel>
      <skos:prefLabel xml:lang="de">Creative Commons Namensnennung – Nicht kommerziell 3.0 Unported</skos:prefLabel>
      <skos:prefLabel xml:lang="el">Creative Commons Αναφορά Δημιουργού – Μη Εμπορική Χρήση 3.0 Μη εισαγόμενο</skos:prefLabel>
      <skos:prefLabel xml:lang="en">Creative Commons Attribution–NonCommercial 3.0 Unported</skos:prefLabel>
      <skos:prefLabel xml:lang="es">Creative Commons Atribución–NoComercial 3.0 Unported</skos:prefLabel>
      <skos:prefLabel xml:lang="et">Creative Commons Autorile viitamine–Mitteäriline eesmärk 3.0 Jurisdiktsiooniga sidumata</skos:prefLabel>
      <skos:prefLabel xml:lang="fi">Creative Commons Nimeä–EiKaupallinen 3.0 Ei sovitettu</skos:prefLabel>
      <skos:prefLabel xml:lang="fr">Creative Commons Attribution – Pas d’Utilisation Commerciale 3.0 non transposé</skos:prefLabel>
      <skos:prefLabel xml:lang="hr">Creative Commons Imenovanje–Nekomercijalno 3.0 nelokalizirana licenca</skos:prefLabel>
      <skos:prefLabel xml:lang="hu">Creative Commons Nevezd meg! – Ne add el! 3.0 Unported</skos:prefLabel>
      <skos:prefLabel xml:lang="it">Creative Commons Attribuzione – Non commerciale 3.0 Unported</skos:prefLabel>
      <skos:prefLabel xml:lang="lt">Creative Commons Priskyrimas – Nekomercinis platinimas 3.0 Nepritaikyta jurisdikcijai</skos:prefLabel>
      <skos:prefLabel xml:lang="lv">Creative Commons Atsaucoties–Nekomerciāli 3.0 Nepārnesta</skos:prefLabel>
      <skos:prefLabel xml:lang="mt">Creative Commons Attribuzzjoni-MhuxKummerċjali 3.0 Unported</skos:prefLabel>
      <skos:prefLabel xml:lang="nl">Creative Commons Naamsvermelding–NietCommercieel 3.0 Unported</skos:prefLabel>
      <skos:prefLabel xml:lang="pl">Creative Commons Uznanie autorstwa–Użycie niekomercyjne 3.0 Unported</skos:prefLabel>
      <skos:prefLabel xml:lang="pt">Creative Commons Atribuição–NãoComercial 3.0 Não Adaptada</skos:prefLabel>
      <skos:prefLabel xml:lang="ro">Creative Commons Atribuire–Necomercial 3.0 Ne-adaptată</skos:prefLabel>
      <skos:prefLabel xml:lang="sk">Creative Commons Uvedenie Autora-Nekomerčné Použitie 3.0 Unported</skos:prefLabel>
      <skos:prefLabel xml:lang="sl">Creative Commons Priznanje avtorstva-Nekomercialno 3.0 Nedoločena</skos:prefLabel>
      <skos:prefLabel xml:lang="sv">Creative Commons Erkännande–IckeKommersiell 3.0 Unported</skos:prefLabel>
      <at:authority-code>CC_BYNC_3_0</at:authority-code>
      <at:op-code>CC_BYNC_3_0</at:op-code>
      <at:start.use>2007-02-23</at:start.use>
      <atold:op-code>CC_BYNC_3_0</atold:op-code>
      <dc:identifier>CC_BYNC_3_0</dc:identifier>
      <skos:altLabel xml:lang="bg">CC BY-NC 3.0</skos:altLabel>
      <skos:altLabel xml:lang="cs">CC BY-NC 3.0</skos:altLabel>
      <skos:altLabel xml:lang="da">CC BY-NC 3.0</skos:altLabel>
      <skos:altLabel xml:lang="de">CC BY-NC 3.0</skos:altLabel>
      <skos:altLabel xml:lang="el">CC BY-NC 3.0</skos:altLabel>
      <skos:altLabel xml:lang="en">CC BY-NC 3.0</skos:altLabel>
      <skos:altLabel xml:lang="es">CC BY-NC 3.0</skos:altLabel>
      <skos:altLabel xml:lang="et">CC BY-NC 3.0</skos:altLabel>
      <skos:altLabel xml:lang="fi">CC BY-NC 3.0</skos:altLabel>
      <skos:altLabel xml:lang="fr">CC BY-NC 3.0</skos:altLabel>
      <skos:altLabel xml:lang="ga">CC BY-NC 3.0</skos:altLabel>
      <skos:altLabel xml:lang="hr">CC BY-NC 3.0</skos:altLabel>
      <skos:altLabel xml:lang="hu">CC BY-NC 3.0</skos:altLabel>
      <skos:altLabel xml:lang="it">CC BY-NC 3.0</skos:altLabel>
      <skos:altLabel xml:lang="lt">CC BY-NC 3.0</skos:altLabel>
      <skos:altLabel xml:lang="lv">CC BY-NC 3.0</skos:altLabel>
      <skos:altLabel xml:lang="mt">CC BY-NC 3.0</skos:altLabel>
      <skos:altLabel xml:lang="nl">CC BY-NC 3.0</skos:altLabel>
      <skos:altLabel xml:lang="pl">CC BY-NC 3.0</skos:altLabel>
      <skos:altLabel xml:lang="pt">CC BY-NC 3.0</skos:altLabel>
      <skos:altLabel xml:lang="ro">CC BY-NC 3.0</skos:altLabel>
      <skos:altLabel xml:lang="sk">CC BY-NC 3.0</skos:altLabel>
      <skos:altLabel xml:lang="sl">CC BY-NC 3.0</skos:altLabel>
      <skos:altLabel xml:lang="sv">CC BY-NC 3.0</skos:altLabel>
      <skos:definition xml:lang="en">CC BY-NC 3.0 lets others remix, tweak, and build upon the author’s work non-commercially, and although their new works must also acknowledge the author and be non-commercial, they don’t have to licence their derivative works on the same terms.</skos:definition>
      <skos:definition xml:lang="fr">CC BY-NC 3.0 permet aux autres de remixer, arranger, et adapter l’œuvre de l’auteur/autrice à des fins non commerciales et, bien que les nouvelles œuvres doivent créditer l’auteur/autrice en citant son nom et ne pas constituer une utilisation commerciale, elles n’ont pas à être diffusées selon les mêmes conditions.</skos:definition>
      <skos:exactMatch rdf:resource="http://creativecommons.org/licenses/by-nc/3.0/"/>
      <skos:inScheme rdf:resource="http://publications.europa.eu/resource/authority/licence"/>
      <skos:topConceptOf rdf:resource="http://publications.europa.eu/resource/authority/licence"/>
      <skos:historyNote xml:lang="en">Unported licences are licences that are not associated with any specific jurisdiction, e.g. country.</skos:historyNote>
   </skos:Concept>
   <skos:Concept rdf:about="http://publications.europa.eu/resource/authority/licence/CC_BYNC_4_0"
                 at:deprecated="false">
      <skos:prefLabel xml:lang="cs">Creative Commons Uveďte původ–Neužívejte komerčně 4.0 Mezinárodní</skos:prefLabel>
      <skos:prefLabel xml:lang="de">Creative Commons Namensnennung – Nicht kommerziell 4.0 International</skos:prefLabel>
      <skos:prefLabel xml:lang="el">Creative Commons Αναφορά Δημιουργού – Μη Εμπορική Χρήση 4.0 Διεθνές</skos:prefLabel>
      <skos:prefLabel xml:lang="en">Creative Commons Attribution–NonCommercial 4.0 International</skos:prefLabel>
      <skos:prefLabel xml:lang="es">Creative Commons Atribución–NoComercial 4.0 Internacional</skos:prefLabel>
      <skos:prefLabel xml:lang="fi">Creative Commons Nimeä–EiKaupallinen 4.0 Kansainvälinen</skos:prefLabel>
      <skos:prefLabel xml:lang="fr">Creative Commons Attribution – Pas d’Utilisation Commerciale 4.0 International</skos:prefLabel>
      <skos:prefLabel xml:lang="hr">Creative Commons Imenovanje–Nekomercijalno 4.0 međunarodna</skos:prefLabel>
      <skos:prefLabel xml:lang="hu">Creative Commons Nevezd meg! – Ne add el! 4.0 Nemzetközi</skos:prefLabel>
      <skos:prefLabel xml:lang="it">Creative Commons Attribuzione – Non commerciale 4.0 Internazionale</skos:prefLabel>
      <skos:prefLabel xml:lang="lt">Creative Commons Priskyrimas – Nekomercinis platinimas 4.0 Tarptautinė</skos:prefLabel>
      <skos:prefLabel xml:lang="lv">Creative Commons Atsaucoties–Nekomerciāli 4.0 Internacionāls</skos:prefLabel>
      <skos:prefLabel xml:lang="nl">Creative Commons Naamsvermelding–NietCommercieel 4.0 Internationaal</skos:prefLabel>
      <skos:prefLabel xml:lang="pl">Creative Commons Uznanie autorstwa–Użycie niekomercyjne 4.0 Międzynarodowe</skos:prefLabel>
      <skos:prefLabel xml:lang="pt">Creative Commons Atribuição–NãoComercial 4.0 Internacional</skos:prefLabel>
      <skos:prefLabel xml:lang="ro">Creative Commons Atribuire–Necomercial 4.0 Internațional</skos:prefLabel>
      <skos:prefLabel xml:lang="sv">Creative Commons Erkännande–IckeKommersiell 4.0 Internationell</skos:prefLabel>
      <skos:prefLabel xml:lang="bg">Creative Commons Признание-Некомерсиално 4.0 Международен</skos:prefLabel>
      <skos:prefLabel xml:lang="da">Creative Commons Kreditering-Ikkekommerciel 4.0 International</skos:prefLabel>
      <skos:prefLabel xml:lang="et">Creative Commons Autorile viitamine–Mitteäriline eesmärk 4.0 Rahvusvaheline</skos:prefLabel>
      <skos:prefLabel xml:lang="mt">Creative Commons Attribuzzjoni-MhuxKummerċjali 4.0 Internazzjonali</skos:prefLabel>
      <skos:prefLabel xml:lang="sk">Creative Commons Uvedenie Autora-Nekomerčné Použitie 4.0 Medzinárodný</skos:prefLabel>
      <skos:prefLabel xml:lang="sl">Creative Commons Priznanje avtorstva-Nekomercialno 4.0 Mednarodna</skos:prefLabel>
      <at:authority-code>CC_BYNC_4_0</at:authority-code>
      <at:op-code>CC_BYNC_4_0</at:op-code>
      <at:start.use>2013-11-26</at:start.use>
      <atold:op-code>CC_BYNC_4_0</atold:op-code>
      <dc:identifier>CC_BYNC_4_0</dc:identifier>
      <skos:altLabel xml:lang="bg">CC BY-NC 4.0</skos:altLabel>
      <skos:altLabel xml:lang="cs">CC BY-NC 4.0</skos:altLabel>
      <skos:altLabel xml:lang="da">CC BY-NC 4.0</skos:altLabel>
      <skos:altLabel xml:lang="de">CC BY-NC 4.0</skos:altLabel>
      <skos:altLabel xml:lang="el">CC BY-NC 4.0</skos:altLabel>
      <skos:altLabel xml:lang="en">CC BY-NC 4.0</skos:altLabel>
      <skos:altLabel xml:lang="es">CC BY-NC 4.0</skos:altLabel>
      <skos:altLabel xml:lang="et">CC BY-NC 4.0</skos:altLabel>
      <skos:altLabel xml:lang="fi">CC BY-NC 4.0</skos:altLabel>
      <skos:altLabel xml:lang="fr">CC BY-NC 4.0</skos:altLabel>
      <skos:altLabel xml:lang="ga">CC BY-NC 4.0</skos:altLabel>
      <skos:altLabel xml:lang="hr">CC BY-NC 4.0</skos:altLabel>
      <skos:altLabel xml:lang="hu">CC BY-NC 4.0</skos:altLabel>
      <skos:altLabel xml:lang="it">CC BY-NC 4.0</skos:altLabel>
      <skos:altLabel xml:lang="lt">CC BY-NC 4.0</skos:altLabel>
      <skos:altLabel xml:lang="lv">CC BY-NC 4.0</skos:altLabel>
      <skos:altLabel xml:lang="mt">CC BY-NC 4.0</skos:altLabel>
      <skos:altLabel xml:lang="nl">CC BY-NC 4.0</skos:altLabel>
      <skos:altLabel xml:lang="pl">CC BY-NC 4.0</skos:altLabel>
      <skos:altLabel xml:lang="pt">CC BY-NC 4.0</skos:altLabel>
      <skos:altLabel xml:lang="ro">CC BY-NC 4.0</skos:altLabel>
      <skos:altLabel xml:lang="sk">CC BY-NC 4.0</skos:altLabel>
      <skos:altLabel xml:lang="sl">CC BY-NC 4.0</skos:altLabel>
      <skos:altLabel xml:lang="sv">CC BY-NC 4.0</skos:altLabel>
      <skos:definition xml:lang="en">CC BY-NC 4.0 lets others remix, tweak, and build upon the author’s work non-commercially, and although their new works must also acknowledge the author and be non-commercial, they don’t have to licence their derivative works on the same terms.</skos:definition>
      <skos:definition xml:lang="fr">CC BY-NC 4.0 permet aux autres de remixer, arranger, et adapter l’œuvre de l’auteur/autrice à des fins non commerciales et, bien que les nouvelles œuvres doivent créditer l’auteur/autrice en citant son nom et ne pas constituer une utilisation commerciale, elles n’ont pas à être diffusées selon les mêmes conditions.</skos:definition>
      <skos:exactMatch rdf:resource="http://creativecommons.org/licenses/by-nc/4.0/"/>
      <skos:inScheme rdf:resource="http://publications.europa.eu/resource/authority/licence"/>
      <skos:topConceptOf rdf:resource="http://publications.europa.eu/resource/authority/licence"/>
   </skos:Concept>
   <skos:Concept rdf:about="http://publications.europa.eu/resource/authority/licence/CC_BYND"
                 at:deprecated="true">
      <skos:prefLabel xml:lang="cs">Creative Commons Uveďte původ–Nezpracovávejte 4.0 Mezinárodní</skos:prefLabel>
      <skos:prefLabel xml:lang="da">Creative Commons Navngivelse–IngenBearbejdelse 4.0 International</skos:prefLabel>
      <skos:prefLabel xml:lang="de">Creative Commons Namensnennung – Keine Bearbeitungen 4.0 International</skos:prefLabel>
      <skos:prefLabel xml:lang="el">Creative Commons Αναφορά Δημιουργού – Όχι Παράγωγα Έργα 4.0 Διεθνές</skos:prefLabel>
      <skos:prefLabel xml:lang="en">Creative Commons Attribution–NoDerivatives 4.0 International</skos:prefLabel>
      <skos:prefLabel xml:lang="es">Creative Commons Atribución–SinDerivar 4.0 Internacional</skos:prefLabel>
      <skos:prefLabel xml:lang="fi">Creative Commons Nimeä–EiMuutoksia 4.0 Kansainvälinen</skos:prefLabel>
      <skos:prefLabel xml:lang="fr">Creative Commons Attribution – Pas de Modification 4.0 International</skos:prefLabel>
      <skos:prefLabel xml:lang="hr">Creative Commons Imenovanje–Bez prerada 4.0 međunarodna</skos:prefLabel>
      <skos:prefLabel xml:lang="hu">Creative Commons Nevezd meg! – Ne változtasd! 4.0 Nemzetközi</skos:prefLabel>
      <skos:prefLabel xml:lang="it">Creative Commons Attribuzione – Non opere derivate 4.0 Internazionale</skos:prefLabel>
      <skos:prefLabel xml:lang="lt">Creative Commons Priskyrimas – Jokių išvestinių darbų 4.0 Tarptautinė</skos:prefLabel>
      <skos:prefLabel xml:lang="lv">Creative Commons Atsaucoties, nepārveidojot 4.0 Internacionāls</skos:prefLabel>
      <skos:prefLabel xml:lang="nl">Creative Commons Naamsvermelding–GeenAfgeleideWerken 4.0 Internationaal</skos:prefLabel>
      <skos:prefLabel xml:lang="pl">Creative Commons Uznanie autorstwa – Bez utworów zależnych 4.0 Międzynarodowe</skos:prefLabel>
      <skos:prefLabel xml:lang="pt">Creative Commons Atribuição–SemDerivações 4.0 Internacional</skos:prefLabel>
      <skos:prefLabel xml:lang="ro">Creative Commons Atribuire–FărăDerivate 4.0 Internațional</skos:prefLabel>
      <skos:prefLabel xml:lang="sv">Creative Commons Erkännande–IngaBearbetningar 4.0 Internationell</skos:prefLabel>
      <at:authority-code>CC_BYND</at:authority-code>
      <at:op-code>CC_BYND</at:op-code>
      <at:start.use>2013-11-25</at:start.use>
      <atold:op-code>CC_BYND</atold:op-code>
      <dc:identifier>CC_BYND</dc:identifier>
      <skos:altLabel xml:lang="bg">CC BY-ND 4.0</skos:altLabel>
      <skos:altLabel xml:lang="cs">CC BY-ND 4.0</skos:altLabel>
      <skos:altLabel xml:lang="da">CC BY-ND 4.0</skos:altLabel>
      <skos:altLabel xml:lang="de">CC BY-ND 4.0</skos:altLabel>
      <skos:altLabel xml:lang="el">CC BY-ND 4.0</skos:altLabel>
      <skos:altLabel xml:lang="en">CC BY-ND 4.0</skos:altLabel>
      <skos:altLabel xml:lang="es">CC BY-ND 4.0</skos:altLabel>
      <skos:altLabel xml:lang="et">CC BY-ND 4.0</skos:altLabel>
      <skos:altLabel xml:lang="fi">CC BY-ND 4.0</skos:altLabel>
      <skos:altLabel xml:lang="fr">CC BY-ND 4.0</skos:altLabel>
      <skos:altLabel xml:lang="ga">CC BY-ND 4.0</skos:altLabel>
      <skos:altLabel xml:lang="hr">CC BY-ND 4.0</skos:altLabel>
      <skos:altLabel xml:lang="hu">CC BY-ND 4.0</skos:altLabel>
      <skos:altLabel xml:lang="it">CC BY-ND 4.0</skos:altLabel>
      <skos:altLabel xml:lang="lt">CC BY-ND 4.0</skos:altLabel>
      <skos:altLabel xml:lang="lv">CC BY-ND 4.0</skos:altLabel>
      <skos:altLabel xml:lang="mt">CC BY-ND 4.0</skos:altLabel>
      <skos:altLabel xml:lang="nl">CC BY-ND 4.0</skos:altLabel>
      <skos:altLabel xml:lang="pl">CC BY-ND 4.0</skos:altLabel>
      <skos:altLabel xml:lang="pt">CC BY-ND 4.0</skos:altLabel>
      <skos:altLabel xml:lang="ro">CC BY-ND 4.0</skos:altLabel>
      <skos:altLabel xml:lang="sk">CC BY-ND 4.0</skos:altLabel>
      <skos:altLabel xml:lang="sl">CC BY-ND 4.0</skos:altLabel>
      <skos:altLabel xml:lang="sv">CC BY-ND 4.0</skos:altLabel>
      <skos:definition xml:lang="en">This licence allows for redistribution, commercial and non-commercial, as long as it is passed along unchanged and in whole, with credit to the author.</skos:definition>
      <skos:definition xml:lang="fr">Cette licence autorise la redistribution, à des fins commerciales ou non, tant que l’œuvre est diffusée sans modification et dans son intégralité, avec attribution et citation du nom de l’auteur/autrice.</skos:definition>
      <skos:inScheme rdf:resource="http://publications.europa.eu/resource/authority/licence"/>
      <skos:topConceptOf rdf:resource="http://publications.europa.eu/resource/authority/licence"/>
      <at:end.use>2013-11-26</at:end.use>
   </skos:Concept>
   <skos:Concept rdf:about="http://publications.europa.eu/resource/authority/licence/CC_BYND_1_0"
                 at:deprecated="true">
      <skos:prefLabel xml:lang="bg">Creative Commons Признание-Без производни 1.0 Неадаптиран</skos:prefLabel>
      <skos:prefLabel xml:lang="cs">Creative Commons Uveďte původ–Nezpracovávejte 1.0 Generic</skos:prefLabel>
      <skos:prefLabel xml:lang="da">Creative Commons Kreditering-Ingen afledninger 1.0 Generisk</skos:prefLabel>
      <skos:prefLabel xml:lang="de">Creative Commons Namensnennung – Keine Bearbeitung 1.0 Generic</skos:prefLabel>
      <skos:prefLabel xml:lang="el">Creative Commons Αναφορά Δημιουργού – Όχι Παράγωγα Έργα 1.0 Γενικό</skos:prefLabel>
      <skos:prefLabel xml:lang="en">Creative Commons Attribution–NoDerivs 1.0 Generic</skos:prefLabel>
      <skos:prefLabel xml:lang="es">Creative Commons Atribución–SinDerivadas 1.0 Genérica</skos:prefLabel>
      <skos:prefLabel xml:lang="et">Creative Commons Autorile viitamine–Tuletatud teoste keeld 1.0 Üldine</skos:prefLabel>
      <skos:prefLabel xml:lang="fi">Creative Commons Nimeä–EiMuutoksia 1.0 Yleinen</skos:prefLabel>
      <skos:prefLabel xml:lang="fr">Creative Commons Attribution – Pas de Modification 1.0 Générique</skos:prefLabel>
      <skos:prefLabel xml:lang="hr">Creative Commons Imenovanje–Bez prerada 1.0 nelokalizirana licenca</skos:prefLabel>
      <skos:prefLabel xml:lang="hu">Creative Commons Nevezd meg! – Ne változtasd! 1.0 Általános</skos:prefLabel>
      <skos:prefLabel xml:lang="it">Creative Commons Attribuzione – Non opere derivate 1.0 Generico</skos:prefLabel>
      <skos:prefLabel xml:lang="lt">Creative Commons Priskyrimas – Jokių išvestinių darbų 1.0 Bendrasis</skos:prefLabel>
      <skos:prefLabel xml:lang="lv">Creative Commons Atsaucoties–Nepārveidojot 1.0 Vispārīgs</skos:prefLabel>
      <skos:prefLabel xml:lang="mt">Creative Commons Attribuzzjoni-EbdaDerivattivi 1.0 Generic</skos:prefLabel>
      <skos:prefLabel xml:lang="nl">Creative Commons Naamsvermelding–GeenAfgeleideWerken 1.0 Unported</skos:prefLabel>
      <skos:prefLabel xml:lang="pl">Creative Commons Uznanie autorstwa–Bez utworów zależnych 1.0 Ogólny</skos:prefLabel>
      <skos:prefLabel xml:lang="pt">Creative Commons Atribuição–SemDerivações 1.0 Genérica</skos:prefLabel>
      <skos:prefLabel xml:lang="ro">Creative Commons Atribuire–FărăModificări 1.0 Generică</skos:prefLabel>
      <skos:prefLabel xml:lang="sk">Creative Commons Uvedenie Autora-Bez Odvodeného Obsahu 1.0 Generic</skos:prefLabel>
      <skos:prefLabel xml:lang="sl">Creative Commons Priznanje avtorstva-Brez predelav 1.0 Generična</skos:prefLabel>
      <skos:prefLabel xml:lang="sv">Creative Commons Erkännande–IngaBearbetningar 1.0 Generisk</skos:prefLabel>
      <at:authority-code>CC_BYND_1_0</at:authority-code>
      <at:op-code>CC_BYND_1_0</at:op-code>
      <at:start.use>2002-12-15</at:start.use>
      <atold:op-code>CC_BYND_1_0</atold:op-code>
      <dc:identifier>CC_BYND_1_0</dc:identifier>
      <skos:altLabel xml:lang="bg">CC BY-ND 1.0</skos:altLabel>
      <skos:altLabel xml:lang="cs">CC BY-ND 1.0</skos:altLabel>
      <skos:altLabel xml:lang="da">CC BY-ND 1.0</skos:altLabel>
      <skos:altLabel xml:lang="de">CC BY-ND 1.0</skos:altLabel>
      <skos:altLabel xml:lang="el">CC BY-ND 1.0</skos:altLabel>
      <skos:altLabel xml:lang="en">CC BY-ND 1.0</skos:altLabel>
      <skos:altLabel xml:lang="es">CC BY-ND 1.0</skos:altLabel>
      <skos:altLabel xml:lang="et">CC BY-ND 1.0</skos:altLabel>
      <skos:altLabel xml:lang="fi">CC BY-ND 1.0</skos:altLabel>
      <skos:altLabel xml:lang="fr">CC BY-ND 1.0</skos:altLabel>
      <skos:altLabel xml:lang="ga">CC BY-ND 1.0</skos:altLabel>
      <skos:altLabel xml:lang="hr">CC BY-ND 1.0</skos:altLabel>
      <skos:altLabel xml:lang="hu">CC BY-ND 1.0</skos:altLabel>
      <skos:altLabel xml:lang="it">CC BY-ND 1.0</skos:altLabel>
      <skos:altLabel xml:lang="lt">CC BY-ND 1.0</skos:altLabel>
      <skos:altLabel xml:lang="lv">CC BY-ND 1.0</skos:altLabel>
      <skos:altLabel xml:lang="mt">CC BY-ND 1.0</skos:altLabel>
      <skos:altLabel xml:lang="nl">CC BY-ND 1.0</skos:altLabel>
      <skos:altLabel xml:lang="pl">CC BY-ND 1.0</skos:altLabel>
      <skos:altLabel xml:lang="pt">CC BY-ND 1.0</skos:altLabel>
      <skos:altLabel xml:lang="ro">CC BY-ND 1.0</skos:altLabel>
      <skos:altLabel xml:lang="sk">CC BY-ND 1.0</skos:altLabel>
      <skos:altLabel xml:lang="sl">CC BY-ND 1.0</skos:altLabel>
      <skos:altLabel xml:lang="sv">CC BY-ND 1.0</skos:altLabel>
      <skos:definition xml:lang="en">CC BY-ND 1.0 allows for redistribution, commercial and non-commercial, as long as it is passed along unchanged and in whole, with credit to the author.</skos:definition>
      <skos:definition xml:lang="fr">CC BY-ND 1.0 autorise la redistribution, à des fins commerciales ou non, tant que l’œuvre est diffusée sans modification et dans son intégralité, avec attribution et citation du nom de l’auteur/autrice.</skos:definition>
      <skos:exactMatch rdf:resource="http://creativecommons.org/licenses/by-nd/1.0/"/>
      <skos:inScheme rdf:resource="http://publications.europa.eu/resource/authority/licence"/>
      <skos:topConceptOf rdf:resource="http://publications.europa.eu/resource/authority/licence"/>
      <at:end.use>2004-05-24</at:end.use>
   </skos:Concept>
   <skos:Concept rdf:about="http://publications.europa.eu/resource/authority/licence/CC_BYND_2_0"
                 at:deprecated="false">
      <skos:prefLabel xml:lang="bg">Creative Commons Признание-Без производни 2.0 Неадаптиран</skos:prefLabel>
      <skos:prefLabel xml:lang="cs">Creative Commons Uveďte původ–Nezpracovávejte 2.0 Generic</skos:prefLabel>
      <skos:prefLabel xml:lang="da">Creative Commons Kreditering-Ingen afledninger 2.0 Generisk</skos:prefLabel>
      <skos:prefLabel xml:lang="de">Creative Commons Namensnennung – Keine Bearbeitung 2.0 Generic</skos:prefLabel>
      <skos:prefLabel xml:lang="el">Creative Commons Αναφορά Δημιουργού – Όχι Παράγωγα Έργα 2.0 Γενικό</skos:prefLabel>
      <skos:prefLabel xml:lang="en">Creative Commons Attribution–NoDerivs 2.0 Generic</skos:prefLabel>
      <skos:prefLabel xml:lang="es">Creative Commons Atribución–SinDerivadas 2.0 Genérica</skos:prefLabel>
      <skos:prefLabel xml:lang="et">Creative Commons Autorile viitamine–Tuletatud teoste keeld 2.0 Üldine</skos:prefLabel>
      <skos:prefLabel xml:lang="fi">Creative Commons Nimeä–EiMuutoksia 2.0 Yleinen</skos:prefLabel>
      <skos:prefLabel xml:lang="fr">Creative Commons Attribution – Pas de Modification 2.0 Générique</skos:prefLabel>
      <skos:prefLabel xml:lang="hr">Creative Commons Imenovanje–Bez prerada 2.0 nelokalizirana licenca</skos:prefLabel>
      <skos:prefLabel xml:lang="hu">Creative Commons Nevezd meg! – Ne változtasd! 2.0 Általános</skos:prefLabel>
      <skos:prefLabel xml:lang="it">Creative Commons Attribuzione – Non opere derivate 2.0 Generico</skos:prefLabel>
      <skos:prefLabel xml:lang="lt">Creative Commons Priskyrimas – Jokių išvestinių darbų 2.0 Bendrasis</skos:prefLabel>
      <skos:prefLabel xml:lang="lv">Creative Commons Atsaucoties–Nepārveidojot 2.0 Vispārīgs</skos:prefLabel>
      <skos:prefLabel xml:lang="mt">Creative Commons Attribuzzjoni-EbdaDerivattivi 2.0 Generic</skos:prefLabel>
      <skos:prefLabel xml:lang="nl">Creative Commons Naamsvermelding–GeenAfgeleideWerken 2.0 Unported</skos:prefLabel>
      <skos:prefLabel xml:lang="pl">Creative Commons Uznanie autorstwa–Bez utworów zależnych 2.0 Ogólny</skos:prefLabel>
      <skos:prefLabel xml:lang="pt">Creative Commons Atribuição–SemDerivações 2.0 Genérica</skos:prefLabel>
      <skos:prefLabel xml:lang="ro">Creative Commons Atribuire–FărăModificări 2.0 Generică</skos:prefLabel>
      <skos:prefLabel xml:lang="sk">Creative Commons Uvedenie Autora-Bez Odvodeného Obsahu 2.0 Generic</skos:prefLabel>
      <skos:prefLabel xml:lang="sl">Creative Commons Priznanje avtorstva-Brez predelav 2.0 Generična</skos:prefLabel>
      <skos:prefLabel xml:lang="sv">Creative Commons Erkännande–IngaBearbetningar 2.0 Generisk</skos:prefLabel>
      <at:authority-code>CC_BYND_2_0</at:authority-code>
      <at:op-code>CC_BYND_2_0</at:op-code>
      <at:start.use>2004-05-25</at:start.use>
      <atold:op-code>CC_BYND_2_0</atold:op-code>
      <dc:identifier>CC_BYND_2_0</dc:identifier>
      <skos:altLabel xml:lang="bg">CC BY-ND 2.0</skos:altLabel>
      <skos:altLabel xml:lang="cs">CC BY-ND 2.0</skos:altLabel>
      <skos:altLabel xml:lang="da">CC BY-ND 2.0</skos:altLabel>
      <skos:altLabel xml:lang="de">CC BY-ND 2.0</skos:altLabel>
      <skos:altLabel xml:lang="el">CC BY-ND 2.0</skos:altLabel>
      <skos:altLabel xml:lang="en">CC BY-ND 2.0</skos:altLabel>
      <skos:altLabel xml:lang="es">CC BY-ND 2.0</skos:altLabel>
      <skos:altLabel xml:lang="et">CC BY-ND 2.0</skos:altLabel>
      <skos:altLabel xml:lang="fi">CC BY-ND 2.0</skos:altLabel>
      <skos:altLabel xml:lang="fr">CC BY-ND 2.0</skos:altLabel>
      <skos:altLabel xml:lang="ga">CC BY-ND 2.0</skos:altLabel>
      <skos:altLabel xml:lang="hr">CC BY-ND 2.0</skos:altLabel>
      <skos:altLabel xml:lang="hu">CC BY-ND 2.0</skos:altLabel>
      <skos:altLabel xml:lang="it">CC BY-ND 2.0</skos:altLabel>
      <skos:altLabel xml:lang="lt">CC BY-ND 2.0</skos:altLabel>
      <skos:altLabel xml:lang="lv">CC BY-ND 2.0</skos:altLabel>
      <skos:altLabel xml:lang="mt">CC BY-ND 2.0</skos:altLabel>
      <skos:altLabel xml:lang="nl">CC BY-ND 2.0</skos:altLabel>
      <skos:altLabel xml:lang="pl">CC BY-ND 2.0</skos:altLabel>
      <skos:altLabel xml:lang="pt">CC BY-ND 2.0</skos:altLabel>
      <skos:altLabel xml:lang="ro">CC BY-ND 2.0</skos:altLabel>
      <skos:altLabel xml:lang="sk">CC BY-ND 2.0</skos:altLabel>
      <skos:altLabel xml:lang="sl">CC BY-ND 2.0</skos:altLabel>
      <skos:altLabel xml:lang="sv">CC BY-ND 2.0</skos:altLabel>
      <skos:definition xml:lang="en">CC BY-ND 2.0 allows for redistribution, commercial and non-commercial, as long as it is passed along unchanged and in whole, with credit to the author.</skos:definition>
      <skos:definition xml:lang="fr">CC BY-ND 2.0 autorise la redistribution, à des fins commerciales ou non, tant que l’œuvre est diffusée sans modification et dans son intégralité, avec attribution et citation du nom de l’auteur.</skos:definition>
      <skos:exactMatch rdf:resource="http://creativecommons.org/licenses/by-nd/2.0/"/>
      <skos:inScheme rdf:resource="http://publications.europa.eu/resource/authority/licence"/>
      <skos:topConceptOf rdf:resource="http://publications.europa.eu/resource/authority/licence"/>
   </skos:Concept>
   <skos:Concept rdf:about="http://publications.europa.eu/resource/authority/licence/CC_BYND_2_5"
                 at:deprecated="false">
      <skos:prefLabel xml:lang="bg">Creative Commons Признание-Без производни 2.5 Неадаптиран</skos:prefLabel>
      <skos:prefLabel xml:lang="cs">Creative Commons Uveďte původ–Nezpracovávejte 2.5 Generic</skos:prefLabel>
      <skos:prefLabel xml:lang="da">Creative Commons Kreditering-Ingen afledninger 2.5 Generisk</skos:prefLabel>
      <skos:prefLabel xml:lang="de">Creative Commons Namensnennung – Keine Bearbeitung 2.5 Generic</skos:prefLabel>
      <skos:prefLabel xml:lang="el">Creative Commons Αναφορά Δημιουργού – Όχι Παράγωγα Έργα 2.5 Γενικό</skos:prefLabel>
      <skos:prefLabel xml:lang="en">Creative Commons Attribution–NoDerivs 2.5 Generic</skos:prefLabel>
      <skos:prefLabel xml:lang="es">Creative Commons Atribución–SinDerivadas 2.5 Genérica</skos:prefLabel>
      <skos:prefLabel xml:lang="et">Creative Commons Autorile viitamine–Tuletatud teoste keeld 2.5 Üldine</skos:prefLabel>
      <skos:prefLabel xml:lang="fi">Creative Commons Nimeä–EiMuutoksia 2.5 Yleinen</skos:prefLabel>
      <skos:prefLabel xml:lang="fr">Creative Commons Attribution – Pas de Modification 2.5 Générique</skos:prefLabel>
      <skos:prefLabel xml:lang="hr">Creative Commons Imenovanje–Bez prerada 2.5 nelokalizirana licenca</skos:prefLabel>
      <skos:prefLabel xml:lang="hu">Creative Commons Nevezd meg! – Ne változtasd! 2.5 Általános</skos:prefLabel>
      <skos:prefLabel xml:lang="it">Creative Commons Attribuzione – Non opere derivate 2.5 Generico</skos:prefLabel>
      <skos:prefLabel xml:lang="lt">Creative Commons Priskyrimas – Jokių išvestinių darbų 2.5 Bendrasis</skos:prefLabel>
      <skos:prefLabel xml:lang="lv">Creative Commons Atsaucoties–Nepārveidojot 2.5 Vispārīgs</skos:prefLabel>
      <skos:prefLabel xml:lang="mt">Creative Commons Attribuzzjoni-EbdaDerivattivi 2.5 Generic</skos:prefLabel>
      <skos:prefLabel xml:lang="nl">Creative Commons Naamsvermelding–GeenAfgeleideWerken 2.5 Unported</skos:prefLabel>
      <skos:prefLabel xml:lang="pl">Creative Commons Uznanie autorstwa–Bez utworów zależnych 2.5 Ogólny</skos:prefLabel>
      <skos:prefLabel xml:lang="pt">Creative Commons Atribuição–SemDerivações 2.5 Genérica</skos:prefLabel>
      <skos:prefLabel xml:lang="ro">Creative Commons Atribuire–FărăModificări 2.5 Generică</skos:prefLabel>
      <skos:prefLabel xml:lang="sk">Creative Commons Uvedenie Autora-Bez Odvodeného Obsahu 2.5 Generic</skos:prefLabel>
      <skos:prefLabel xml:lang="sl">Creative Commons Priznanje avtorstva-Brez predelav 2.5 Generična</skos:prefLabel>
      <skos:prefLabel xml:lang="sv">Creative Commons Erkännande–IngaBearbetningar 2.5 Generisk</skos:prefLabel>
      <at:authority-code>CC_BYND_2_5</at:authority-code>
      <at:op-code>CC_BYND_2_5</at:op-code>
      <at:start.use>2005-06-01</at:start.use>
      <atold:op-code>CC_BYND_2_5</atold:op-code>
      <dc:identifier>CC_BYND_2_5</dc:identifier>
      <skos:altLabel xml:lang="bg">CC BY-ND 2.5</skos:altLabel>
      <skos:altLabel xml:lang="cs">CC BY-ND 2.5</skos:altLabel>
      <skos:altLabel xml:lang="da">CC BY-ND 2.5</skos:altLabel>
      <skos:altLabel xml:lang="de">CC BY-ND 2.5</skos:altLabel>
      <skos:altLabel xml:lang="el">CC BY-ND 2.5</skos:altLabel>
      <skos:altLabel xml:lang="en">CC BY-ND 2.5</skos:altLabel>
      <skos:altLabel xml:lang="es">CC BY-ND 2.5</skos:altLabel>
      <skos:altLabel xml:lang="et">CC BY-ND 2.5</skos:altLabel>
      <skos:altLabel xml:lang="fi">CC BY-ND 2.5</skos:altLabel>
      <skos:altLabel xml:lang="fr">CC BY-ND 2.5</skos:altLabel>
      <skos:altLabel xml:lang="ga">CC BY-ND 2.5</skos:altLabel>
      <skos:altLabel xml:lang="hr">CC BY-ND 2.5</skos:altLabel>
      <skos:altLabel xml:lang="hu">CC BY-ND 2.5</skos:altLabel>
      <skos:altLabel xml:lang="it">CC BY-ND 2.5</skos:altLabel>
      <skos:altLabel xml:lang="lt">CC BY-ND 2.5</skos:altLabel>
      <skos:altLabel xml:lang="lv">CC BY-ND 2.5</skos:altLabel>
      <skos:altLabel xml:lang="mt">CC BY-ND 2.5</skos:altLabel>
      <skos:altLabel xml:lang="nl">CC BY-ND 2.5</skos:altLabel>
      <skos:altLabel xml:lang="pl">CC BY-ND 2.5</skos:altLabel>
      <skos:altLabel xml:lang="pt">CC BY-ND 2.5</skos:altLabel>
      <skos:altLabel xml:lang="ro">CC BY-ND 2.5</skos:altLabel>
      <skos:altLabel xml:lang="sk">CC BY-ND 2.5</skos:altLabel>
      <skos:altLabel xml:lang="sl">CC BY-ND 2.5</skos:altLabel>
      <skos:altLabel xml:lang="sv">CC BY-ND 2.5</skos:altLabel>
      <skos:definition xml:lang="en">CC BY-ND 2.5 allows for redistribution, commercial and non-commercial, as long as it is passed along unchanged and in whole, with credit to the author.</skos:definition>
      <skos:definition xml:lang="fr">CC BY-ND 2.5 autorise la redistribution, à des fins commerciales ou non, tant que l’œuvre est diffusée sans modification et dans son intégralité, avec attribution et citation du nom de l’auteur/autrice.</skos:definition>
      <skos:exactMatch rdf:resource="http://creativecommons.org/licenses/by-nd/2.5/"/>
      <skos:inScheme rdf:resource="http://publications.europa.eu/resource/authority/licence"/>
      <skos:topConceptOf rdf:resource="http://publications.europa.eu/resource/authority/licence"/>
   </skos:Concept>
   <skos:Concept rdf:about="http://publications.europa.eu/resource/authority/licence/CC_BYND_3_0"
                 at:deprecated="false">
      <skos:prefLabel xml:lang="bg">Creative Commons Признание-Без производни 3.0 Нелокализиран</skos:prefLabel>
      <skos:prefLabel xml:lang="cs">Creative Commons Uveďte původ–Nezpracovávejte 3.0 Unported</skos:prefLabel>
      <skos:prefLabel xml:lang="da">Creative Commons Kreditering-Ingen afledninger 3.0 Ikke porteret</skos:prefLabel>
      <skos:prefLabel xml:lang="de">Creative Commons Namensnennung – Keine Bearbeitung 3.0 Unported</skos:prefLabel>
      <skos:prefLabel xml:lang="el">Creative Commons Αναφορά Δημιουργού – Όχι Παράγωγα Έργα 3.0 Μη εισαγόμενο</skos:prefLabel>
      <skos:prefLabel xml:lang="en">Creative Commons Attribution–NoDerivs 3.0 Unported</skos:prefLabel>
      <skos:prefLabel xml:lang="es">Creative Commons Atribución–SinDerivadas 3.0 Unported</skos:prefLabel>
      <skos:prefLabel xml:lang="et">Creative Commons Autorile viitamine–Tuletatud teoste keeld 3.0 Jurisdiktsiooniga sidumata</skos:prefLabel>
      <skos:prefLabel xml:lang="fi">Creative Commons Nimeä–EiMuutoksia 3.0 Ei sovitettu</skos:prefLabel>
      <skos:prefLabel xml:lang="fr">Creative Commons Attribution – Pas de Modification 3.0 non transposé</skos:prefLabel>
      <skos:prefLabel xml:lang="hr">Creative Commons Imenovanje–Bez prerada 3.0 nelokalizirana licenca</skos:prefLabel>
      <skos:prefLabel xml:lang="hu">Creative Commons Nevezd meg! – Ne változtasd! 3.0 Unported</skos:prefLabel>
      <skos:prefLabel xml:lang="it">Creative Commons Attribuzione – Non opere derivate 3.0 Unported</skos:prefLabel>
      <skos:prefLabel xml:lang="lt">Creative Commons Priskyrimas – Jokių išvestinių darbų 3.0 Nepritaikyta jurisdikcijai</skos:prefLabel>
      <skos:prefLabel xml:lang="lv">Creative Commons Atsaucoties–Nepārveidojot 3.0 Nepārnesta</skos:prefLabel>
      <skos:prefLabel xml:lang="mt">Creative Commons Attribuzzjoni-EbdaDerivattivi 3.0 Unported</skos:prefLabel>
      <skos:prefLabel xml:lang="nl">Creative Commons Naamsvermelding–GeenAfgeleideWerken 3.0 Unported</skos:prefLabel>
      <skos:prefLabel xml:lang="pl">Creative Commons Uznanie autorstwa–Bez utworów zależnych 3.0 Unported</skos:prefLabel>
      <skos:prefLabel xml:lang="pt">Creative Commons Atribuição–SemDerivações 3.0 Não Adaptada</skos:prefLabel>
      <skos:prefLabel xml:lang="ro">Creative Commons Atribuire-FărăModificări 3.0 Ne-adaptată</skos:prefLabel>
      <skos:prefLabel xml:lang="sk">Creative Commons Uvedenie Autora-Bez Odvodeného Obsahu 3.0 Unported</skos:prefLabel>
      <skos:prefLabel xml:lang="sl">Creative Commons Priznanje avtorstva-Brez predelav 3.0 Nedoločena</skos:prefLabel>
      <skos:prefLabel xml:lang="sv">Creative Commons Erkännande–IngaBearbetningar 3.0 Unported</skos:prefLabel>
      <at:authority-code>CC_BYND_3_0</at:authority-code>
      <at:op-code>CC_BYND_3_0</at:op-code>
      <at:start.use>2007-02-23</at:start.use>
      <atold:op-code>CC_BYND_3_0</atold:op-code>
      <dc:identifier>CC_BYND_3_0</dc:identifier>
      <skos:altLabel xml:lang="bg">CC BY-ND 3.0</skos:altLabel>
      <skos:altLabel xml:lang="cs">CC BY-ND 3.0</skos:altLabel>
      <skos:altLabel xml:lang="da">CC BY-ND 3.0</skos:altLabel>
      <skos:altLabel xml:lang="de">CC BY-ND 3.0</skos:altLabel>
      <skos:altLabel xml:lang="el">CC BY-ND 3.0</skos:altLabel>
      <skos:altLabel xml:lang="en">CC BY-ND 3.0</skos:altLabel>
      <skos:altLabel xml:lang="es">CC BY-ND 3.0</skos:altLabel>
      <skos:altLabel xml:lang="et">CC BY-ND 3.0</skos:altLabel>
      <skos:altLabel xml:lang="fi">CC BY-ND 3.0</skos:altLabel>
      <skos:altLabel xml:lang="fr">CC BY-ND 3.0</skos:altLabel>
      <skos:altLabel xml:lang="ga">CC BY-ND 3.0</skos:altLabel>
      <skos:altLabel xml:lang="hr">CC BY-ND 3.0</skos:altLabel>
      <skos:altLabel xml:lang="hu">CC BY-ND 3.0</skos:altLabel>
      <skos:altLabel xml:lang="it">CC BY-ND 3.0</skos:altLabel>
      <skos:altLabel xml:lang="lt">CC BY-ND 3.0</skos:altLabel>
      <skos:altLabel xml:lang="lv">CC BY-ND 3.0</skos:altLabel>
      <skos:altLabel xml:lang="mt">CC BY-ND 3.0</skos:altLabel>
      <skos:altLabel xml:lang="nl">CC BY-ND 3.0</skos:altLabel>
      <skos:altLabel xml:lang="pl">CC BY-ND 3.0</skos:altLabel>
      <skos:altLabel xml:lang="pt">CC BY-ND 3.0</skos:altLabel>
      <skos:altLabel xml:lang="ro">CC BY-ND 3.0</skos:altLabel>
      <skos:altLabel xml:lang="sk">CC BY-ND 3.0</skos:altLabel>
      <skos:altLabel xml:lang="sl">CC BY-ND 3.0</skos:altLabel>
      <skos:altLabel xml:lang="sv">CC BY-ND 3.0</skos:altLabel>
      <skos:definition xml:lang="en">CC BY-ND 3.0 allows for redistribution, commercial and non-commercial, as long as it is passed along unchanged and in whole, with credit to the author.</skos:definition>
      <skos:definition xml:lang="fr">CC BY-ND 3.0 autorise la redistribution, à des fins commerciales ou non, tant que l’œuvre est diffusée sans modification et dans son intégralité, avec attribution et citation du nom de l’auteur/autrice.</skos:definition>
      <skos:exactMatch rdf:resource="http://creativecommons.org/licenses/by-nd/3.0/"/>
      <skos:inScheme rdf:resource="http://publications.europa.eu/resource/authority/licence"/>
      <skos:topConceptOf rdf:resource="http://publications.europa.eu/resource/authority/licence"/>
      <skos:historyNote xml:lang="en">Unported licences are licences that are not associated with any specific jurisdiction, e.g. country.</skos:historyNote>
   </skos:Concept>
   <skos:Concept rdf:about="http://publications.europa.eu/resource/authority/licence/CC_BYND_4_0"
                 at:deprecated="false">
      <skos:prefLabel xml:lang="cs">Creative Commons Uveďte původ–Nezpracovávejte 4.0 Mezinárodní</skos:prefLabel>
      <skos:prefLabel xml:lang="de">Creative Commons Namensnennung – Keine Bearbeitungen 4.0 International</skos:prefLabel>
      <skos:prefLabel xml:lang="el">Creative Commons Αναφορά Δημιουργού – Όχι Παράγωγα Έργα 4.0 Διεθνές</skos:prefLabel>
      <skos:prefLabel xml:lang="en">Creative Commons Attribution–NoDerivatives 4.0 International</skos:prefLabel>
      <skos:prefLabel xml:lang="es">Creative Commons Atribución–SinDerivar 4.0 Internacional</skos:prefLabel>
      <skos:prefLabel xml:lang="fi">Creative Commons Nimeä–EiMuutoksia 4.0 Kansainvälinen</skos:prefLabel>
      <skos:prefLabel xml:lang="fr">Creative Commons Attribution – Pas de Modification 4.0 International</skos:prefLabel>
      <skos:prefLabel xml:lang="hr">Creative Commons Imenovanje–Bez prerada 4.0 međunarodna</skos:prefLabel>
      <skos:prefLabel xml:lang="hu">Creative Commons Nevezd meg! – Ne változtasd! 4.0 Nemzetközi</skos:prefLabel>
      <skos:prefLabel xml:lang="it">Creative Commons Attribuzione – Non opere derivate 4.0 Internazionale</skos:prefLabel>
      <skos:prefLabel xml:lang="lt">Creative Commons Priskyrimas – Jokių išvestinių darbų 4.0 Tarptautinė</skos:prefLabel>
      <skos:prefLabel xml:lang="lv">Creative Commons Atsaucoties, nepārveidojot 4.0 Internacionāls</skos:prefLabel>
      <skos:prefLabel xml:lang="nl">Creative Commons Naamsvermelding–GeenAfgeleideWerken 4.0 Internationaal</skos:prefLabel>
      <skos:prefLabel xml:lang="pl">Creative Commons Uznanie autorstwa – Bez utworów zależnych 4.0 Międzynarodowe</skos:prefLabel>
      <skos:prefLabel xml:lang="pt">Creative Commons Atribuição–SemDerivações 4.0 Internacional</skos:prefLabel>
      <skos:prefLabel xml:lang="ro">Creative Commons Atribuire–FărăDerivate 4.0 Internațional</skos:prefLabel>
      <skos:prefLabel xml:lang="sv">Creative Commons Erkännande–IngaBearbetningar 4.0 Internationell</skos:prefLabel>
      <skos:prefLabel xml:lang="bg">Creative Commons Признание-Без производни 4.0 Международен</skos:prefLabel>
      <skos:prefLabel xml:lang="da">Creative Commons Kreditering-Ingen afledninger 4.0 International</skos:prefLabel>
      <skos:prefLabel xml:lang="et">Creative Commons Autorile viitamine–Tuletatud teoste keeld 4.0 Rahvusvaheline</skos:prefLabel>
      <skos:prefLabel xml:lang="mt">Creative Commons Attribuzzjoni-EbdaDerivattivi 4.0 Internazzjonali</skos:prefLabel>
      <skos:prefLabel xml:lang="sk">Creative Commons Uvedenie Autora-Žiadne Odvodené Diela 4.0 Medzinárodný</skos:prefLabel>
      <skos:prefLabel xml:lang="sl">Creative Commons Priznanje avtorstva-Brez predelav 4.0 Mednarodna</skos:prefLabel>
      <at:authority-code>CC_BYND_4_0</at:authority-code>
      <at:op-code>CC_BYND_4_0</at:op-code>
      <at:start.use>2013-11-26</at:start.use>
      <atold:op-code>CC_BYND_4_0</atold:op-code>
      <dc:identifier>CC_BYND_4_0</dc:identifier>
      <skos:altLabel xml:lang="bg">CC BY-ND 4.0</skos:altLabel>
      <skos:altLabel xml:lang="cs">CC BY-ND 4.0</skos:altLabel>
      <skos:altLabel xml:lang="da">CC BY-ND 4.0</skos:altLabel>
      <skos:altLabel xml:lang="de">CC BY-ND 4.0</skos:altLabel>
      <skos:altLabel xml:lang="el">CC BY-ND 4.0</skos:altLabel>
      <skos:altLabel xml:lang="en">CC BY-ND 4.0</skos:altLabel>
      <skos:altLabel xml:lang="es">CC BY-ND 4.0</skos:altLabel>
      <skos:altLabel xml:lang="et">CC BY-ND 4.0</skos:altLabel>
      <skos:altLabel xml:lang="fi">CC BY-ND 4.0</skos:altLabel>
      <skos:altLabel xml:lang="fr">CC BY-ND 4.0</skos:altLabel>
      <skos:altLabel xml:lang="ga">CC BY-ND 4.0</skos:altLabel>
      <skos:altLabel xml:lang="hr">CC BY-ND 4.0</skos:altLabel>
      <skos:altLabel xml:lang="hu">CC BY-ND 4.0</skos:altLabel>
      <skos:altLabel xml:lang="it">CC BY-ND 4.0</skos:altLabel>
      <skos:altLabel xml:lang="lt">CC BY-ND 4.0</skos:altLabel>
      <skos:altLabel xml:lang="lv">CC BY-ND 4.0</skos:altLabel>
      <skos:altLabel xml:lang="mt">CC BY-ND 4.0</skos:altLabel>
      <skos:altLabel xml:lang="nl">CC BY-ND 4.0</skos:altLabel>
      <skos:altLabel xml:lang="pl">CC BY-ND 4.0</skos:altLabel>
      <skos:altLabel xml:lang="pt">CC BY-ND 4.0</skos:altLabel>
      <skos:altLabel xml:lang="ro">CC BY-ND 4.0</skos:altLabel>
      <skos:altLabel xml:lang="sk">CC BY-ND 4.0</skos:altLabel>
      <skos:altLabel xml:lang="sl">CC BY-ND 4.0</skos:altLabel>
      <skos:altLabel xml:lang="sv">CC BY-ND 4.0</skos:altLabel>
      <skos:definition xml:lang="en">CC BY-ND 4.0 allows for redistribution, commercial and non-commercial, as long as it is passed along unchanged and in whole, with credit to the author.</skos:definition>
      <skos:definition xml:lang="fr">CC BY-ND 4.0 autorise la redistribution, à des fins commerciales ou non, tant que l’œuvre est diffusée sans modification et dans son intégralité, avec attribution et citation du nom de l’auteur/autrice.</skos:definition>
      <skos:exactMatch rdf:resource="http://creativecommons.org/licenses/by-nd/4.0/"/>
      <skos:inScheme rdf:resource="http://publications.europa.eu/resource/authority/licence"/>
      <skos:topConceptOf rdf:resource="http://publications.europa.eu/resource/authority/licence"/>
   </skos:Concept>
   <skos:Concept rdf:about="http://publications.europa.eu/resource/authority/licence/CC_BYSA"
                 at:deprecated="true">
      <skos:prefLabel xml:lang="cs">Creative Commons Uveďte původ–Zachovejte licenci 4.0 Mezinárodní</skos:prefLabel>
      <skos:prefLabel xml:lang="da">Creative Commons Navngivelse–DelPåSammeVilkår 4.0 International</skos:prefLabel>
      <skos:prefLabel xml:lang="de">Creative Commons Namensnennung – Weitergabe unter gleichen Bedingungen 4.0 International</skos:prefLabel>
      <skos:prefLabel xml:lang="el">Creative Commons Αναφορά Δημιουργού – Παρόμοια Διανομή 4.0 Διεθνές</skos:prefLabel>
      <skos:prefLabel xml:lang="en">Creative Commons Attribution–ShareAlike 4.0 International</skos:prefLabel>
      <skos:prefLabel xml:lang="es">Creative Commons Atribución–CompartirIgual 4.0 Internacional</skos:prefLabel>
      <skos:prefLabel xml:lang="fi">Creative Commons Nimeä–JaaSamoin 4.0 Kansainvälinen</skos:prefLabel>
      <skos:prefLabel xml:lang="fr">Creative Commons Attribution – Partage dans les Mêmes Conditions 4.0 International</skos:prefLabel>
      <skos:prefLabel xml:lang="hr">Creative Commons Imenovanje–Dijeli pod istim uvjetima 4.0 međunarodna</skos:prefLabel>
      <skos:prefLabel xml:lang="hu">Creative Commons Nevezd meg! – Így add tovább! 4.0 Nemzetközi</skos:prefLabel>
      <skos:prefLabel xml:lang="it">Creative Commons Attribuzione – Condividi allo stesso modo 4.0 Internazionale</skos:prefLabel>
      <skos:prefLabel xml:lang="lt">Creative Commons Priskyrimas – Analogiškas platinimas 4.0 Tarptautinė</skos:prefLabel>
      <skos:prefLabel xml:lang="lv">Creative Commons Atsaucoties–Nemainot licenci 4.0 Internacionāls</skos:prefLabel>
      <skos:prefLabel xml:lang="nl">Creative Commons Naamsvermelding–GelijkDelen 4.0 Internationaal</skos:prefLabel>
      <skos:prefLabel xml:lang="pl">Creative Commons Uznanie autorstwa–Na tych samych warunkach 4.0 Międzynarodowe</skos:prefLabel>
      <skos:prefLabel xml:lang="pt">Creative Commons Atribuição–CompartilhaIgual 4.0 Internacional</skos:prefLabel>
      <skos:prefLabel xml:lang="ro">Creative Commons Atribuire–Distribuire în condiţii identice 4.0 Internațional</skos:prefLabel>
      <skos:prefLabel xml:lang="sv">Creative Commons Erkännande–DelaLika 4.0 Internationell</skos:prefLabel>
      <at:authority-code>CC_BYSA</at:authority-code>
      <at:op-code>CC_BYSA</at:op-code>
      <at:start.use>2013-11-25</at:start.use>
      <atold:op-code>CC_BYSA</atold:op-code>
      <dc:identifier>CC_BYSA</dc:identifier>
      <skos:altLabel xml:lang="bg">CC BY-SA 4.0</skos:altLabel>
      <skos:altLabel xml:lang="cs">CC BY-SA 4.0</skos:altLabel>
      <skos:altLabel xml:lang="da">CC BY-SA 4.0</skos:altLabel>
      <skos:altLabel xml:lang="de">CC BY-SA 4.0</skos:altLabel>
      <skos:altLabel xml:lang="el">CC BY-SA 4.0</skos:altLabel>
      <skos:altLabel xml:lang="en">CC BY-SA 4.0</skos:altLabel>
      <skos:altLabel xml:lang="es">CC BY-SA 4.0</skos:altLabel>
      <skos:altLabel xml:lang="et">CC BY-SA 4.0</skos:altLabel>
      <skos:altLabel xml:lang="fi">CC BY-SA 4.0</skos:altLabel>
      <skos:altLabel xml:lang="fr">CC BY-SA 4.0</skos:altLabel>
      <skos:altLabel xml:lang="ga">CC BY-SA 4.0</skos:altLabel>
      <skos:altLabel xml:lang="hr">CC BY-SA 4.0</skos:altLabel>
      <skos:altLabel xml:lang="hu">CC BY-SA 4.0</skos:altLabel>
      <skos:altLabel xml:lang="it">CC BY-SA 4.0</skos:altLabel>
      <skos:altLabel xml:lang="lt">CC BY-SA 4.0</skos:altLabel>
      <skos:altLabel xml:lang="lv">CC BY-SA 4.0</skos:altLabel>
      <skos:altLabel xml:lang="mt">CC BY-SA 4.0</skos:altLabel>
      <skos:altLabel xml:lang="nl">CC BY-SA 4.0</skos:altLabel>
      <skos:altLabel xml:lang="pl">CC BY-SA 4.0</skos:altLabel>
      <skos:altLabel xml:lang="pt">CC BY-SA 4.0</skos:altLabel>
      <skos:altLabel xml:lang="ro">CC BY-SA 4.0</skos:altLabel>
      <skos:altLabel xml:lang="sk">CC BY-SA 4.0</skos:altLabel>
      <skos:altLabel xml:lang="sl">CC BY-SA 4.0</skos:altLabel>
      <skos:altLabel xml:lang="sv">CC BY-SA 4.0</skos:altLabel>
      <skos:definition xml:lang="en">This licence lets others remix, tweak, and build upon the author's work even for commercial purposes, as long as they credit the author and licence their new creations under the identical terms. This licence is often compared to “copyleft” free and open source software licences. All new works based on the original work will carry the same licence, so any derivatives will also allow commercial use. This is the licence used by Wikipedia, and is recommended for materials that would benefit from incorporating content from Wikipedia and similarly licenced projects.</skos:definition>
      <skos:definition xml:lang="fr">Cette licence permet aux autres de remixer, arranger, et adapter l’œuvre de l’auteur/l’autrice, même à des fins commerciales, tant qu’on accorde le mérite de la création originale à l’auteur/l’autrice en citant son nom et qu’on diffuse les nouvelles créations selon des conditions identiques. Cette licence est souvent comparée aux licences de logiciels libres, «open source» ou «copyleft». Toutes les nouvelles œuvres basées sur celles de l’auteur/autrice auront la même licence, et toute œuvre dérivée pourra être utilisée même à des fins commerciales. C’est la licence utilisée par Wikipédia; elle est recommandée pour des œuvres qui pourraient bénéficier de l’incorporation de contenu depuis Wikipédia et d’autres projets sous licence similaire.</skos:definition>
      <skos:inScheme rdf:resource="http://publications.europa.eu/resource/authority/licence"/>
      <skos:topConceptOf rdf:resource="http://publications.europa.eu/resource/authority/licence"/>
      <at:end.use>2013-11-26</at:end.use>
   </skos:Concept>
   <skos:Concept rdf:about="http://publications.europa.eu/resource/authority/licence/CC_BYSA_1_0"
                 at:deprecated="true">
      <skos:prefLabel xml:lang="bg">Creative Commons Признание-Споделяне на споделеното 1.0 Неадаптира</skos:prefLabel>
      <skos:prefLabel xml:lang="cs">Creative Commons Uveďte původ–Zachovejte licenci 1.0 Generic</skos:prefLabel>
      <skos:prefLabel xml:lang="da">Creative Commons Kreditering-Deling på samme vilkår 1.0 Generisk</skos:prefLabel>
      <skos:prefLabel xml:lang="de">Creative Commons Namensnennung – Weitergabe unter gleichen Bedingungen 1.0 Generic</skos:prefLabel>
      <skos:prefLabel xml:lang="el">Creative Commons Αναφορά Δημιουργού – Παρόμοια Διανομή 1.0 Μη εισαγόμενο</skos:prefLabel>
      <skos:prefLabel xml:lang="en">Creative Commons Attribution–ShareAlike 1.0 Generic</skos:prefLabel>
      <skos:prefLabel xml:lang="es">Creative Commons Atribución–CompartirIgual 1.0 Genérica</skos:prefLabel>
      <skos:prefLabel xml:lang="et">Creative Commons Autorile viitamine–Jagamine samadel tingimustel 1.0 Üldine</skos:prefLabel>
      <skos:prefLabel xml:lang="fi">Creative Commons Nimeä–JaaSamoin 1.0 Yleinen</skos:prefLabel>
      <skos:prefLabel xml:lang="fr">Creative Commons Attribution – Partage dans les Mêmes Conditions 1.0 Générique</skos:prefLabel>
      <skos:prefLabel xml:lang="hr">Creative Commons Imenovanje–Dijeli pod istim uvjetima 1.0 nelokalizirana licenca</skos:prefLabel>
      <skos:prefLabel xml:lang="hu">Creative Commons Nevezd meg! – Így add tovább! 1.0 Általános</skos:prefLabel>
      <skos:prefLabel xml:lang="it">Creative Commons Attribuzione – Condividi allo stesso modo 1.0 Generico</skos:prefLabel>
      <skos:prefLabel xml:lang="lt">Creative Commons Priskyrimas – Analogiškas platinimas 1.0 Bendrasis</skos:prefLabel>
      <skos:prefLabel xml:lang="lv">Creative Commons Atsaucoties–Nemainot licenci 1.0 Vispārīgs</skos:prefLabel>
      <skos:prefLabel xml:lang="mt">Creative Commons Attribuzzjoni-KondiviżjoniUgwali 1.0 Generic</skos:prefLabel>
      <skos:prefLabel xml:lang="nl">Creative Commons Naamsvermelding–GelijkDelen 1.0 Unported</skos:prefLabel>
      <skos:prefLabel xml:lang="pl">Creative Commons Uznanie autorstwa–Na tych samych warunkach 1.0 Ogólny</skos:prefLabel>
      <skos:prefLabel xml:lang="pt">Creative Commons Atribuição–CompartilhaIgual 1.0 Genérica</skos:prefLabel>
      <skos:prefLabel xml:lang="ro">Creative Commons Atribuire–Distribuire în condiţii identice 1.0 Generică</skos:prefLabel>
      <skos:prefLabel xml:lang="sk">Creative Commons Uvedenie Autora-Rovnaké Šírenie 1.0 Generic</skos:prefLabel>
      <skos:prefLabel xml:lang="sl">Creative Commons Priznanje avtorstva-Deljenje pod enakimi pogoji 1.0 Generična</skos:prefLabel>
      <skos:prefLabel xml:lang="sv">Creative Commons Erkännande–DelaLika 1.0 Generisk</skos:prefLabel>
      <at:authority-code>CC_BYSA_1_0</at:authority-code>
      <at:op-code>CC_BYSA_1_0</at:op-code>
      <at:start.use>2002-12-15</at:start.use>
      <atold:op-code>CC_BYSA_1_0</atold:op-code>
      <dc:identifier>CC_BYSA_1_0</dc:identifier>
      <skos:altLabel xml:lang="bg">CC BY-SA 1.0</skos:altLabel>
      <skos:altLabel xml:lang="cs">CC BY-SA 1.0</skos:altLabel>
      <skos:altLabel xml:lang="da">CC BY-SA 1.0</skos:altLabel>
      <skos:altLabel xml:lang="de">CC BY-SA 1.0</skos:altLabel>
      <skos:altLabel xml:lang="el">CC BY-SA 1.0</skos:altLabel>
      <skos:altLabel xml:lang="en">CC BY-SA 1.0</skos:altLabel>
      <skos:altLabel xml:lang="es">CC BY-SA 1.0</skos:altLabel>
      <skos:altLabel xml:lang="et">CC BY-SA 1.0</skos:altLabel>
      <skos:altLabel xml:lang="fi">CC BY-SA 1.0</skos:altLabel>
      <skos:altLabel xml:lang="fr">CC BY-SA 1.0</skos:altLabel>
      <skos:altLabel xml:lang="ga">CC BY-SA 1.0</skos:altLabel>
      <skos:altLabel xml:lang="hr">CC BY-SA 1.0</skos:altLabel>
      <skos:altLabel xml:lang="hu">CC BY-SA 1.0</skos:altLabel>
      <skos:altLabel xml:lang="it">CC BY-SA 1.0</skos:altLabel>
      <skos:altLabel xml:lang="lt">CC BY-SA 1.0</skos:altLabel>
      <skos:altLabel xml:lang="lv">CC BY-SA 1.0</skos:altLabel>
      <skos:altLabel xml:lang="mt">CC BY-SA 1.0</skos:altLabel>
      <skos:altLabel xml:lang="nl">CC BY-SA 1.0</skos:altLabel>
      <skos:altLabel xml:lang="pl">CC BY-SA 1.0</skos:altLabel>
      <skos:altLabel xml:lang="pt">CC BY-SA 1.0</skos:altLabel>
      <skos:altLabel xml:lang="ro">CC BY-SA 1.0</skos:altLabel>
      <skos:altLabel xml:lang="sk">CC BY-SA 1.0</skos:altLabel>
      <skos:altLabel xml:lang="sl">CC BY-SA 1.0</skos:altLabel>
      <skos:altLabel xml:lang="sv">CC BY-SA 1.0</skos:altLabel>
      <skos:definition xml:lang="en">CC BY-SA 1.0 lets others remix, tweak, and build upon the author’s work even for commercial purposes, as long as they credit the author and licence their new creations under the identical terms. This licence is often compared to “copyleft” free and open source software licences. All new works based on the original work will carry the same licence, so any derivatives will also allow commercial use. This is the licence used by Wikipedia, and is recommended for materials that would benefit from incorporating content from Wikipedia and similarly licenced projects.</skos:definition>
      <skos:definition xml:lang="fr">CC BY-SA 1.0 permet aux autres de remixer, arranger, et adapter l’œuvre de l’auteur/autrice, même à des fins commerciales, tant qu’on accorde le mérite de la création originale à l’auteur/autrice en citant son nom et qu’on diffuse les nouvelles créations selon des conditions identiques. Cette licence est souvent comparée aux licences de logiciels libres, «open source» ou «copyleft». Toutes les nouvelles œuvres basées sur celles de l’auteur/autrice auront la même licence, et toute œuvre dérivée pourra être utilisée même à des fins commerciales. C’est la licence utilisée par Wikipédia; elle est recommandée pour des œuvres qui pourraient bénéficier de l’incorporation de contenu depuis Wikipédia et d’autres projets sous licence similaire.</skos:definition>
      <skos:exactMatch rdf:resource="http://creativecommons.org/licenses/by-sa/1.0/"/>
      <skos:inScheme rdf:resource="http://publications.europa.eu/resource/authority/licence"/>
      <skos:topConceptOf rdf:resource="http://publications.europa.eu/resource/authority/licence"/>
      <at:end.use>2004-05-24</at:end.use>
   </skos:Concept>
   <skos:Concept rdf:about="http://publications.europa.eu/resource/authority/licence/CC_BYSA_2_0"
                 at:deprecated="false">
      <skos:prefLabel xml:lang="bg">Creative Commons Признание-Споделяне на споделеното 2.0 Неадаптиран</skos:prefLabel>
      <skos:prefLabel xml:lang="cs">Creative Commons Uveďte původ–Zachovejte licenci 2.0 Generic</skos:prefLabel>
      <skos:prefLabel xml:lang="da">Creative Commons Kreditering-Deling på samme vilkår 2.0 Generisk</skos:prefLabel>
      <skos:prefLabel xml:lang="de">Creative Commons Namensnennung – Weitergabe unter gleichen Bedingungen 2.0 Generic</skos:prefLabel>
      <skos:prefLabel xml:lang="el">Creative Commons Αναφορά Δημιουργού – Παρόμοια Διανομή 2.0 Μη εισαγόμενο</skos:prefLabel>
      <skos:prefLabel xml:lang="en">Creative Commons Attribution–ShareAlike 2.0 Generic</skos:prefLabel>
      <skos:prefLabel xml:lang="es">Creative Commons Atribución–CompartirIgual 2.0 Genérica</skos:prefLabel>
      <skos:prefLabel xml:lang="et">Creative Commons Autorile viitamine–Jagamine samadel tingimustel 2.0 Üldine</skos:prefLabel>
      <skos:prefLabel xml:lang="fi">Creative Commons Nimeä–JaaSamoin 2.0 Yleinen</skos:prefLabel>
      <skos:prefLabel xml:lang="fr">Creative Commons Attribution – Partage dans les Mêmes Conditions 2.0 Générique</skos:prefLabel>
      <skos:prefLabel xml:lang="hr">Creative Commons Imenovanje–Dijeli pod istim uvjetima 2.0 nelokalizirana licenca</skos:prefLabel>
      <skos:prefLabel xml:lang="hu">Creative Commons Nevezd meg! – Így add tovább! 2.0 Általános</skos:prefLabel>
      <skos:prefLabel xml:lang="it">Creative Commons Attribuzione – Condividi allo stesso modo 2.0 Generico</skos:prefLabel>
      <skos:prefLabel xml:lang="lt">Creative Commons Priskyrimas – Analogiškas platinimas 2.0 Bendrasis</skos:prefLabel>
      <skos:prefLabel xml:lang="lv">Creative Commons Atsaucoties–Nemainot licenci 2.0 Vispārīgs</skos:prefLabel>
      <skos:prefLabel xml:lang="mt">Creative Commons Attribuzzjoni-KondiviżjoniUgwali 2.0 Generic</skos:prefLabel>
      <skos:prefLabel xml:lang="nl">Creative Commons Naamsvermelding–GelijkDelen 2.0 Unported</skos:prefLabel>
      <skos:prefLabel xml:lang="pl">Creative Commons Uznanie autorstwa–Na tych samych warunkach 2.0 Ogólny</skos:prefLabel>
      <skos:prefLabel xml:lang="pt">Creative Commons Atribuição–CompartilhaIgual 2.0 Genérica</skos:prefLabel>
      <skos:prefLabel xml:lang="ro">Creative Commons Atribuire–Distribuire în condiţii identice 2.0 Generică</skos:prefLabel>
      <skos:prefLabel xml:lang="sk">Creative Commons Uvedenie Autora-Rovnaké Šírenie 2.0 Generic</skos:prefLabel>
      <skos:prefLabel xml:lang="sl">Creative Commons Priznanje avtorstva-Deljenje pod enakimi pogoji 2.0 Generična</skos:prefLabel>
      <skos:prefLabel xml:lang="sv">Creative Commons Erkännande–DelaLika 2.0 Generisk</skos:prefLabel>
      <at:authority-code>CC_BYSA_2_0</at:authority-code>
      <at:op-code>CC_BYSA_2_0</at:op-code>
      <at:start.use>2004-05-25</at:start.use>
      <atold:op-code>CC_BYSA_2_0</atold:op-code>
      <dc:identifier>CC_BYSA_2_0</dc:identifier>
      <skos:altLabel xml:lang="bg">CC BY-SA 2.0</skos:altLabel>
      <skos:altLabel xml:lang="cs">CC BY-SA 2.0</skos:altLabel>
      <skos:altLabel xml:lang="da">CC BY-SA 2.0</skos:altLabel>
      <skos:altLabel xml:lang="de">CC BY-SA 2.0</skos:altLabel>
      <skos:altLabel xml:lang="el">CC BY-SA 2.0</skos:altLabel>
      <skos:altLabel xml:lang="en">CC BY-SA 2.0</skos:altLabel>
      <skos:altLabel xml:lang="es">CC BY-SA 2.0</skos:altLabel>
      <skos:altLabel xml:lang="et">CC BY-SA 2.0</skos:altLabel>
      <skos:altLabel xml:lang="fi">CC BY-SA 2.0</skos:altLabel>
      <skos:altLabel xml:lang="fr">CC BY-SA 2.0</skos:altLabel>
      <skos:altLabel xml:lang="ga">CC BY-SA 2.0</skos:altLabel>
      <skos:altLabel xml:lang="hr">CC BY-SA 2.0</skos:altLabel>
      <skos:altLabel xml:lang="hu">CC BY-SA 2.0</skos:altLabel>
      <skos:altLabel xml:lang="it">CC BY-SA 2.0</skos:altLabel>
      <skos:altLabel xml:lang="lt">CC BY-SA 2.0</skos:altLabel>
      <skos:altLabel xml:lang="lv">CC BY-SA 2.0</skos:altLabel>
      <skos:altLabel xml:lang="mt">CC BY-SA 2.0</skos:altLabel>
      <skos:altLabel xml:lang="nl">CC BY-SA 2.0</skos:altLabel>
      <skos:altLabel xml:lang="pl">CC BY-SA 2.0</skos:altLabel>
      <skos:altLabel xml:lang="pt">CC BY-SA 2.0</skos:altLabel>
      <skos:altLabel xml:lang="ro">CC BY-SA 2.0</skos:altLabel>
      <skos:altLabel xml:lang="sk">CC BY-SA 2.0</skos:altLabel>
      <skos:altLabel xml:lang="sl">CC BY-SA 2.0</skos:altLabel>
      <skos:altLabel xml:lang="sv">CC BY-SA 2.0</skos:altLabel>
      <skos:definition xml:lang="en">CC BY-SA 2.0 lets others remix, tweak, and build upon the author’s work even for commercial purposes, as long as they credit the author and licence their new creations under the identical terms. This licence is often compared to “copyleft” free and open source software licences. All new works based on the original work will carry the same licence, so any derivatives will also allow commercial use. This is the licence used by Wikipedia, and is recommended for materials that would benefit from incorporating content from Wikipedia and similarly licenced projects.</skos:definition>
      <skos:definition xml:lang="fr">CC BY-SA 2.0 permet aux autres de remixer, arranger, et adapter l’œuvre de l’auteur/autrice, même à des fins commerciales, tant qu’on accorde le mérite de la création originale à l’auteur/autrice en citant son nom et qu’on diffuse les nouvelles créations selon des conditions identiques. Cette licence est souvent comparée aux licences de logiciels libres, «open source» ou «copyleft». Toutes les nouvelles œuvres basées sur celles de l’auteur/autrice auront la même licence, et toute œuvre dérivée pourra être utilisée même à des fins commerciales. C’est la licence utilisée par Wikipédia; elle est recommandée pour des œuvres qui pourraient bénéficier de l’incorporation de contenu depuis Wikipédia et d’autres projets sous licence similaire.</skos:definition>
      <skos:exactMatch rdf:resource="http://creativecommons.org/licenses/by-sa/2.0/"/>
      <skos:inScheme rdf:resource="http://publications.europa.eu/resource/authority/licence"/>
      <skos:topConceptOf rdf:resource="http://publications.europa.eu/resource/authority/licence"/>
   </skos:Concept>
   <skos:Concept rdf:about="http://publications.europa.eu/resource/authority/licence/CC_BYSA_2_5"
                 at:deprecated="false">
      <skos:prefLabel xml:lang="bg">Creative Commons Признание-Споделяне на споделеното 2.5 Неадаптиран</skos:prefLabel>
      <skos:prefLabel xml:lang="cs">Creative Commons Uveďte původ–Zachovejte licenci 2.5 Generic</skos:prefLabel>
      <skos:prefLabel xml:lang="da">Creative Commons Kreditering-Deling på samme vilkår 2.5 Generisk</skos:prefLabel>
      <skos:prefLabel xml:lang="de">Creative Commons Namensnennung – Weitergabe unter gleichen Bedingungen 2.5 Generic</skos:prefLabel>
      <skos:prefLabel xml:lang="el">Creative Commons Αναφορά Δημιουργού – Παρόμοια Διανομή 2.5 Μη εισαγόμενο</skos:prefLabel>
      <skos:prefLabel xml:lang="en">Creative Commons Attribution–ShareAlike 2.5 Generic</skos:prefLabel>
      <skos:prefLabel xml:lang="es">Creative Commons Atribución–CompartirIgual 2.5 Genérica</skos:prefLabel>
      <skos:prefLabel xml:lang="et">Creative Commons Autorile viitamine–Jagamine samadel tingimustel 2.5 Üldine</skos:prefLabel>
      <skos:prefLabel xml:lang="fi">Creative Commons Nimeä–JaaSamoin 2.5 Yleinen</skos:prefLabel>
      <skos:prefLabel xml:lang="fr">Creative Commons Attribution – Partage dans les Mêmes Conditions 2.5 Générique</skos:prefLabel>
      <skos:prefLabel xml:lang="hr">Creative Commons Imenovanje–Dijeli pod istim uvjetima 2.5 nelokalizirana licenca</skos:prefLabel>
      <skos:prefLabel xml:lang="hu">Creative Commons Nevezd meg! – Így add tovább! 2.5 Általános</skos:prefLabel>
      <skos:prefLabel xml:lang="it">Creative Commons Attribuzione – Condividi allo stesso modo 2.5 Generico</skos:prefLabel>
      <skos:prefLabel xml:lang="lt">Creative Commons Priskyrimas – Analogiškas platinimas 2.5 Bendrasis</skos:prefLabel>
      <skos:prefLabel xml:lang="lv">Creative Commons Atsaucoties–Nemainot licenci 2.5 Vispārīgs</skos:prefLabel>
      <skos:prefLabel xml:lang="mt">Creative Commons Attribuzzjoni-KondiviżjoniUgwali 2.5 Generic</skos:prefLabel>
      <skos:prefLabel xml:lang="nl">Creative Commons Naamsvermelding–GelijkDelen 2.5 Unported</skos:prefLabel>
      <skos:prefLabel xml:lang="pl">Creative Commons Uznanie autorstwa–Na tych samych warunkach 2.5 Ogólny</skos:prefLabel>
      <skos:prefLabel xml:lang="pt">Creative Commons Atribuição–CompartilhaIgual 2.5 Genérica</skos:prefLabel>
      <skos:prefLabel xml:lang="ro">Creative Commons Atribuire–Distribuire în condiţii identice 2.5 Generică</skos:prefLabel>
      <skos:prefLabel xml:lang="sk">Creative Commons Uvedenie Autora-Rovnaké Šírenie 2.5 Generic</skos:prefLabel>
      <skos:prefLabel xml:lang="sl">Creative Commons Priznanje avtorstva-Deljenje pod enakimi pogoji 2.5 Generična</skos:prefLabel>
      <skos:prefLabel xml:lang="sv">Creative Commons Erkännande–DelaLika 2.5 Generisk</skos:prefLabel>
      <at:authority-code>CC_BYSA_2_5</at:authority-code>
      <at:op-code>CC_BYSA_2_5</at:op-code>
      <at:start.use>2005-06-01</at:start.use>
      <atold:op-code>CC_BYSA_2_5</atold:op-code>
      <dc:identifier>CC_BYSA_2_5</dc:identifier>
      <skos:altLabel xml:lang="bg">CC BY-SA 2.5</skos:altLabel>
      <skos:altLabel xml:lang="cs">CC BY-SA 2.5</skos:altLabel>
      <skos:altLabel xml:lang="da">CC BY-SA 2.5</skos:altLabel>
      <skos:altLabel xml:lang="de">CC BY-SA 2.5</skos:altLabel>
      <skos:altLabel xml:lang="el">CC BY-SA 2.5</skos:altLabel>
      <skos:altLabel xml:lang="en">CC BY-SA 2.5</skos:altLabel>
      <skos:altLabel xml:lang="es">CC BY-SA 2.5</skos:altLabel>
      <skos:altLabel xml:lang="et">CC BY-SA 2.5</skos:altLabel>
      <skos:altLabel xml:lang="fi">CC BY-SA 2.5</skos:altLabel>
      <skos:altLabel xml:lang="fr">CC BY-SA 2.5</skos:altLabel>
      <skos:altLabel xml:lang="ga">CC BY-SA 2.5</skos:altLabel>
      <skos:altLabel xml:lang="hr">CC BY-SA 2.5</skos:altLabel>
      <skos:altLabel xml:lang="hu">CC BY-SA 2.5</skos:altLabel>
      <skos:altLabel xml:lang="it">CC BY-SA 2.5</skos:altLabel>
      <skos:altLabel xml:lang="lt">CC BY-SA 2.5</skos:altLabel>
      <skos:altLabel xml:lang="lv">CC BY-SA 2.5</skos:altLabel>
      <skos:altLabel xml:lang="mt">CC BY-SA 2.5</skos:altLabel>
      <skos:altLabel xml:lang="nl">CC BY-SA 2.5</skos:altLabel>
      <skos:altLabel xml:lang="pl">CC BY-SA 2.5</skos:altLabel>
      <skos:altLabel xml:lang="pt">CC BY-SA 2.5</skos:altLabel>
      <skos:altLabel xml:lang="ro">CC BY-SA 2.5</skos:altLabel>
      <skos:altLabel xml:lang="sk">CC BY-SA 2.5</skos:altLabel>
      <skos:altLabel xml:lang="sl">CC BY-SA 2.5</skos:altLabel>
      <skos:altLabel xml:lang="sv">CC BY-SA 2.5</skos:altLabel>
      <skos:definition xml:lang="en">CC BY-SA 2.5 lets others remix, tweak, and build upon the author’s work even for commercial purposes, as long as they credit the author and licence their new creations under the identical terms. This licence is often compared to “copyleft” free and open source software licences. All new works based on the original work will carry the same licence, so any derivatives will also allow commercial use. This is the licence used by Wikipedia, and is recommended for materials that would benefit from incorporating content from Wikipedia and similarly licenced projects.</skos:definition>
      <skos:definition xml:lang="fr">CC BY-SA 2.5 permet aux autres de remixer, arranger, et adapter l’œuvre de l’auteur/autrice, même à des fins commerciales, tant qu’on accorde le mérite de la création originale à l’auteur/autrice en citant son nom et qu’on diffuse les nouvelles créations selon des conditions identiques. Cette licence est souvent comparée aux licences de logiciels libres, «open source» ou «copyleft». Toutes les nouvelles œuvres basées sur celles de l’auteur/autrice auront la même licence, et toute œuvre dérivée pourra être utilisée même à des fins commerciales. C’est la licence utilisée par Wikipédia; elle est recommandée pour des œuvres qui pourraient bénéficier de l’incorporation de contenu depuis Wikipédia et d’autres projets sous licence similaire.</skos:definition>
      <skos:exactMatch rdf:resource="http://creativecommons.org/licenses/by-sa/2.5/"/>
      <skos:inScheme rdf:resource="http://publications.europa.eu/resource/authority/licence"/>
      <skos:topConceptOf rdf:resource="http://publications.europa.eu/resource/authority/licence"/>
   </skos:Concept>
   <skos:Concept rdf:about="http://publications.europa.eu/resource/authority/licence/CC_BYSA_3_0"
                 at:deprecated="false">
      <skos:prefLabel xml:lang="bg">Creative Commons Признание-Споделяне на споделеното 3.0 Нелокализиран</skos:prefLabel>
      <skos:prefLabel xml:lang="cs">Creative Commons Uveďte původ–Zachovejte licenci 3.0 Unported</skos:prefLabel>
      <skos:prefLabel xml:lang="da">Creative Commons Kreditering-Deling på samme vilkår 3.0 Ikke porteret</skos:prefLabel>
      <skos:prefLabel xml:lang="de">Creative Commons Namensnennung – Weitergabe unter gleichen Bedingungen 3.0 Unported</skos:prefLabel>
      <skos:prefLabel xml:lang="el">Creative Commons Αναφορά Δημιουργού – Παρόμοια Διανομή 3.0 Μη εισαγόμενο</skos:prefLabel>
      <skos:prefLabel xml:lang="en">Creative Commons Attribution–ShareAlike 3.0 Unported</skos:prefLabel>
      <skos:prefLabel xml:lang="es">Creative Commons Atribución–CompartirIgual 3.0 Unported</skos:prefLabel>
      <skos:prefLabel xml:lang="et">Creative Commons Autorile viitamine–Jagamine samadel tingimustel 3.0 Jurisdiktsiooniga sidumata</skos:prefLabel>
      <skos:prefLabel xml:lang="fi">Creative Commons Nimeä–JaaSamoin 3.0 Ei sovitettu</skos:prefLabel>
      <skos:prefLabel xml:lang="fr">Creative Commons Attribution – Partage dans les Mêmes Conditions 3.0 non transposé</skos:prefLabel>
      <skos:prefLabel xml:lang="hr">Creative Commons Imenovanje–Dijeli pod istim uvjetima 3.0 nelokalizirana licenca</skos:prefLabel>
      <skos:prefLabel xml:lang="hu">Creative Commons Nevezd meg! – Így add tovább! 3.0 Unported</skos:prefLabel>
      <skos:prefLabel xml:lang="it">Creative Commons Attribuzione – Condividi allo stesso modo 3.0 Unported</skos:prefLabel>
      <skos:prefLabel xml:lang="lt">Creative Commons Priskyrimas – Analogiškas platinimas 3.0 Nepritaikyta jurisdikcijai</skos:prefLabel>
      <skos:prefLabel xml:lang="lv">Creative Commons Atsaucoties–Nemainot licenci 3.0 Nepārnesta</skos:prefLabel>
      <skos:prefLabel xml:lang="mt">Creative Commons Attribuzzjoni-KondiviżjoniUgwali 3.0 Unported</skos:prefLabel>
      <skos:prefLabel xml:lang="nl">Creative Commons Naamsvermelding–GelijkDelen 3.0 Unported</skos:prefLabel>
      <skos:prefLabel xml:lang="pl">Creative Commons Uznanie autorstwa–Na tych samych warunkach 3.0 Unported</skos:prefLabel>
      <skos:prefLabel xml:lang="pt">Creative Commons Atribuição–CompartilhaIgual 3.0 Não Adaptada</skos:prefLabel>
      <skos:prefLabel xml:lang="ro">Creative Commons Atribuire–Distribuire în condiţii identice 3.0 Ne-adaptată</skos:prefLabel>
      <skos:prefLabel xml:lang="sk">Creative Commons Uvedenie Autora-Rovnaké Šírenie 3.0 Unported</skos:prefLabel>
      <skos:prefLabel xml:lang="sl">Creative Commons Priznanje avtorstva-Deljenje pod enakimi pogoji 3.0 Nedoločena</skos:prefLabel>
      <skos:prefLabel xml:lang="sv">Creative Commons Erkännande–DelaLika 3.0 Unported</skos:prefLabel>
      <at:authority-code>CC_BYSA_3_0</at:authority-code>
      <at:op-code>CC_BYSA_3_0</at:op-code>
      <at:start.use>2007-02-23</at:start.use>
      <atold:op-code>CC_BYSA_3_0</atold:op-code>
      <dc:identifier>CC_BYSA_3_0</dc:identifier>
      <skos:altLabel xml:lang="bg">CC BY-SA 3.0</skos:altLabel>
      <skos:altLabel xml:lang="cs">CC BY-SA 3.0</skos:altLabel>
      <skos:altLabel xml:lang="da">CC BY-SA 3.0</skos:altLabel>
      <skos:altLabel xml:lang="de">CC BY-SA 3.0</skos:altLabel>
      <skos:altLabel xml:lang="el">CC BY-SA 3.0</skos:altLabel>
      <skos:altLabel xml:lang="en">CC BY-SA 3.0</skos:altLabel>
      <skos:altLabel xml:lang="es">CC BY-SA 3.0</skos:altLabel>
      <skos:altLabel xml:lang="et">CC BY-SA 3.0</skos:altLabel>
      <skos:altLabel xml:lang="fi">CC BY-SA 3.0</skos:altLabel>
      <skos:altLabel xml:lang="fr">CC BY-SA 3.0</skos:altLabel>
      <skos:altLabel xml:lang="ga">CC BY-SA 3.0</skos:altLabel>
      <skos:altLabel xml:lang="hr">CC BY-SA 3.0</skos:altLabel>
      <skos:altLabel xml:lang="hu">CC BY-SA 3.0</skos:altLabel>
      <skos:altLabel xml:lang="it">CC BY-SA 3.0</skos:altLabel>
      <skos:altLabel xml:lang="lt">CC BY-SA 3.0</skos:altLabel>
      <skos:altLabel xml:lang="lv">CC BY-SA 3.0</skos:altLabel>
      <skos:altLabel xml:lang="mt">CC BY-SA 3.0</skos:altLabel>
      <skos:altLabel xml:lang="nl">CC BY-SA 3.0</skos:altLabel>
      <skos:altLabel xml:lang="pl">CC BY-SA 3.0</skos:altLabel>
      <skos:altLabel xml:lang="pt">CC BY-SA 3.0</skos:altLabel>
      <skos:altLabel xml:lang="ro">CC BY-SA 3.0</skos:altLabel>
      <skos:altLabel xml:lang="sk">CC BY-SA 3.0</skos:altLabel>
      <skos:altLabel xml:lang="sl">CC BY-SA 3.0</skos:altLabel>
      <skos:altLabel xml:lang="sv">CC BY-SA 3.0</skos:altLabel>
      <skos:definition xml:lang="en">CC BY-SA 3.0 lets others remix, tweak, and build upon the author’s work even for commercial purposes, as long as they credit the author and licence their new creations under the identical terms. This licence is often compared to “copyleft” free and open source software licences. All new works based on the original work will carry the same licence, so any derivatives will also allow commercial use. This is the licence used by Wikipedia, and is recommended for materials that would benefit from incorporating content from Wikipedia and similarly licenced projects.</skos:definition>
      <skos:definition xml:lang="fr">CC BY-SA 3.0 permet aux autres de remixer, arranger, et adapter l’œuvre de l’auteur/autrice, même à des fins commerciales, tant qu’on accorde le mérite de la création originale à l’auteur/autrice en citant son nom et qu’on diffuse les nouvelles créations selon des conditions identiques. Cette licence est souvent comparée aux licences de logiciels libres, «open source» ou «copyleft». Toutes les nouvelles œuvres basées sur les œuvres de l’auteur/autrice auront la même licence, et toute œuvre dérivée pourra être utilisée même à des fins commerciales. C’est la licence utilisée par Wikipédia; elle est recommandée pour des œuvres qui pourraient bénéficier de l’incorporation de contenu depuis Wikipédia et d’autres projets sous licence similaire.</skos:definition>
      <skos:exactMatch rdf:resource="http://creativecommons.org/licenses/by-sa/3.0/"/>
      <skos:inScheme rdf:resource="http://publications.europa.eu/resource/authority/licence"/>
      <skos:topConceptOf rdf:resource="http://publications.europa.eu/resource/authority/licence"/>
      <skos:historyNote xml:lang="en">Unported licences are licences that are not associated with any specific jurisdiction, e.g. country.</skos:historyNote>
   </skos:Concept>
   <skos:Concept rdf:about="http://publications.europa.eu/resource/authority/licence/CC_BYSA_3_0_NL"
                 at:deprecated="false">
      <skos:prefLabel xml:lang="bg">Признание-Споделяне на споделеното 3.0 Холандия</skos:prefLabel>
      <skos:prefLabel xml:lang="cs">Uveďte původ–Zachovejte licenci 3.0 Nizozemí</skos:prefLabel>
      <skos:prefLabel xml:lang="da">Kreditering-Deling på samme vilkår 3.0 Holland</skos:prefLabel>
      <skos:prefLabel xml:lang="de">Namensnennung – Weitergabe unter gleichen Bedingungen 3.0 Niederlande</skos:prefLabel>
      <skos:prefLabel xml:lang="el">Αναφορά Δημιουργού – Παρόμοια Διανομή 3.0 Ολλανδία</skos:prefLabel>
      <skos:prefLabel xml:lang="en">Attribution-ShareAlike 3.0 Netherlands </skos:prefLabel>
      <skos:prefLabel xml:lang="es">Reconocimiento–CompartirIgual 3.0 Países Bajos</skos:prefLabel>
      <skos:prefLabel xml:lang="et">Autorile viitamine–Jagamine samadel tingimustel 3.0 Holland</skos:prefLabel>
      <skos:prefLabel xml:lang="fi">Nimeä–JaaSamoin 3.0 Hollanti</skos:prefLabel>
      <skos:prefLabel xml:lang="fr">Attribution – Partage dans les Mêmes Conditions 3.0 Pays-Bas</skos:prefLabel>
      <skos:prefLabel xml:lang="hr">Imenovanje–Dijeli pod istim uvjetima 3.0 Nizozemska</skos:prefLabel>
      <skos:prefLabel xml:lang="hu">Nevezd meg! – Így add tovább! 3.0 Hollandia</skos:prefLabel>
      <skos:prefLabel xml:lang="it">Attribuzione – Condividi allo stesso modo 3.0 Olanda</skos:prefLabel>
      <skos:prefLabel xml:lang="lt">Priskyrimas – Analogiškas platinimas 3.0 Nyderlandai</skos:prefLabel>
      <skos:prefLabel xml:lang="lv">Attiecinājums–Dalīties līdzīgi 3.0 Nīderlande</skos:prefLabel>
      <skos:prefLabel xml:lang="mt">Attribuzzjoni-KondiviżjoniUgwali 3.0 Pajjiżi l-Baxxi</skos:prefLabel>
      <skos:prefLabel xml:lang="nl">Naamsvermelding–GelijkDelen 3.0 Nederland</skos:prefLabel>
      <skos:prefLabel xml:lang="pl">Uznanie autorstwa–Na tych samych warunkach 3.0 Holandia</skos:prefLabel>
      <skos:prefLabel xml:lang="pt">Atribuição–CompartilhaIgual 3.0 Holanda</skos:prefLabel>
      <skos:prefLabel xml:lang="ro">Atribuire – Distribuire în condiţii identice 3.0 Olanda</skos:prefLabel>
      <skos:prefLabel xml:lang="sk">Uvedenie Autora-Rovnaké Šírenie 3.0 Holandsko</skos:prefLabel>
      <skos:prefLabel xml:lang="sl">Priznanje avtorstva-Deljenje pod enakimi pogoji 3.0 Nizozemska</skos:prefLabel>
      <skos:prefLabel xml:lang="sv">Erkännande–DelaLika 3.0 Nederländerna</skos:prefLabel>
      <at:authority-code>CC_BYSA_3_0_NL</at:authority-code>
      <at:op-code>CC_BYSA_3_0_NL</at:op-code>
      <at:start.use>2007-02-23</at:start.use>
      <atold:op-code>CC_BYSA_3_0_NL</atold:op-code>
      <dc:identifier>CC_BYSA_3_0_NL</dc:identifier>
      <skos:altLabel xml:lang="bg">CC BY-SA 3.0 NL</skos:altLabel>
      <skos:altLabel xml:lang="cs">CC BY-SA 3.0 NL</skos:altLabel>
      <skos:altLabel xml:lang="da">CC BY-SA 3.0 NL</skos:altLabel>
      <skos:altLabel xml:lang="de">CC BY-SA 3.0 NL</skos:altLabel>
      <skos:altLabel xml:lang="el">CC BY-SA 3.0 NL</skos:altLabel>
      <skos:altLabel xml:lang="en">CC BY-SA 3.0 NL</skos:altLabel>
      <skos:altLabel xml:lang="es">CC BY-SA 3.0 NL</skos:altLabel>
      <skos:altLabel xml:lang="et">CC BY-SA 3.0 NL</skos:altLabel>
      <skos:altLabel xml:lang="fi">CC BY-SA 3.0 NL</skos:altLabel>
      <skos:altLabel xml:lang="fr">CC BY-SA 3.0 NL</skos:altLabel>
      <skos:altLabel xml:lang="ga">CC BY-SA 3.0 NL</skos:altLabel>
      <skos:altLabel xml:lang="hr">CC BY-SA 3.0 NL</skos:altLabel>
      <skos:altLabel xml:lang="hu">CC BY-SA 3.0 NL</skos:altLabel>
      <skos:altLabel xml:lang="it">CC BY-SA 3.0 NL</skos:altLabel>
      <skos:altLabel xml:lang="lt">CC BY-SA 3.0 NL</skos:altLabel>
      <skos:altLabel xml:lang="lv">CC BY-SA 3.0 NL</skos:altLabel>
      <skos:altLabel xml:lang="mt">CC BY-SA 3.0 NL</skos:altLabel>
      <skos:altLabel xml:lang="nl">CC BY-SA 3.0 NL</skos:altLabel>
      <skos:altLabel xml:lang="pl">CC BY-SA 3.0 NL</skos:altLabel>
      <skos:altLabel xml:lang="pt">CC BY-SA 3.0 NL</skos:altLabel>
      <skos:altLabel xml:lang="ro">CC BY-SA 3.0 NL</skos:altLabel>
      <skos:altLabel xml:lang="sk">CC BY-SA 3.0 NL</skos:altLabel>
      <skos:altLabel xml:lang="sl">CC BY-SA 3.0 NL</skos:altLabel>
      <skos:altLabel xml:lang="sv">CC BY-SA 3.0 NL</skos:altLabel>
      <skos:definition xml:lang="en">Published by Creative Commons for Netherlands, Naamsvermelding-GelijkDelen 3.0 Nederland (CC BY-SA 3.0 NL) is a licence permitting any commercial and non-commercial use, as long as credit is given to the author for the original creation and new creations are licenced under the identical terms. All new works based on the original work will carry the same licence, so any derivatives will also allow commercial use.</skos:definition>
      <skos:exactMatch rdf:resource="http://creativecommons.org/licenses/by-sa/3.0/nl/legalcode/"/>
      <skos:inScheme rdf:resource="http://publications.europa.eu/resource/authority/licence"/>
      <skos:topConceptOf rdf:resource="http://publications.europa.eu/resource/authority/licence"/>
   </skos:Concept>
   <skos:Concept rdf:about="http://publications.europa.eu/resource/authority/licence/CC_BYSA_4_0"
                 at:deprecated="false">
      <skos:prefLabel xml:lang="cs">Creative Commons Uveďte původ–Zachovejte licenci 4.0 Mezinárodní</skos:prefLabel>
      <skos:prefLabel xml:lang="de">Creative Commons Namensnennung – Weitergabe unter gleichen Bedingungen 4.0 International</skos:prefLabel>
      <skos:prefLabel xml:lang="el">Creative Commons Αναφορά Δημιουργού – Παρόμοια Διανομή 4.0 Διεθνές</skos:prefLabel>
      <skos:prefLabel xml:lang="en">Creative Commons Attribution–ShareAlike 4.0 International</skos:prefLabel>
      <skos:prefLabel xml:lang="es">Creative Commons Atribución–CompartirIgual 4.0 Internacional</skos:prefLabel>
      <skos:prefLabel xml:lang="fi">Creative Commons Nimeä–JaaSamoin 4.0 Kansainvälinen</skos:prefLabel>
      <skos:prefLabel xml:lang="fr">Creative Commons Attribution – Partage dans les Mêmes Conditions 4.0 International</skos:prefLabel>
      <skos:prefLabel xml:lang="hr">Creative Commons Imenovanje–Dijeli pod istim uvjetima 4.0 međunarodna</skos:prefLabel>
      <skos:prefLabel xml:lang="hu">Creative Commons Nevezd meg! – Így add tovább! 4.0 Nemzetközi</skos:prefLabel>
      <skos:prefLabel xml:lang="it">Creative Commons Attribuzione – Condividi allo stesso modo 4.0 Internazionale</skos:prefLabel>
      <skos:prefLabel xml:lang="lt">Creative Commons Priskyrimas – Analogiškas platinimas 4.0 Tarptautinė</skos:prefLabel>
      <skos:prefLabel xml:lang="lv">Creative Commons Atsaucoties–Nemainot licenci 4.0 Internacionāls</skos:prefLabel>
      <skos:prefLabel xml:lang="nl">Creative Commons Naamsvermelding–GelijkDelen 4.0 Internationaal</skos:prefLabel>
      <skos:prefLabel xml:lang="pl">Creative Commons Uznanie autorstwa–Na tych samych warunkach 4.0 Międzynarodowe</skos:prefLabel>
      <skos:prefLabel xml:lang="pt">Creative Commons Atribuição–CompartilhaIgual 4.0 Internacional</skos:prefLabel>
      <skos:prefLabel xml:lang="ro">Creative Commons Atribuire–Distribuire în condiţii identice 4.0 Internațional</skos:prefLabel>
      <skos:prefLabel xml:lang="sv">Creative Commons Erkännande–DelaLika 4.0 Internationell</skos:prefLabel>
      <skos:prefLabel xml:lang="bg">Creative Commons Признание-Споделяне на споделеното 4.0 Международен</skos:prefLabel>
      <skos:prefLabel xml:lang="da">Creative Commons Kreditering-Deling på samme vilkår 4.0 International</skos:prefLabel>
      <skos:prefLabel xml:lang="et">Creative Commons Autorile viitamine–Jagamine samadel tingimustel 4.0 Rahvusvaheline</skos:prefLabel>
      <skos:prefLabel xml:lang="mt">Creative Commons Attribuzzjoni-KondiviżjoniUgwali 4.0 Internazzjonali</skos:prefLabel>
      <skos:prefLabel xml:lang="sk">Creative Commons Uvedenie Autora-Rovnaké Šírenie 4.0 Medzinárodný</skos:prefLabel>
      <skos:prefLabel xml:lang="sl">Creative Commons Priznanje avtorstva-Deljenje pod enakimi pogoji 4.0 Mednarodna</skos:prefLabel>
      <at:authority-code>CC_BYSA_4_0</at:authority-code>
      <at:op-code>CC_BYSA_4_0</at:op-code>
      <at:start.use>2013-11-26</at:start.use>
      <atold:op-code>CC_BYSA_4_0</atold:op-code>
      <dc:identifier>CC_BYSA_4_0</dc:identifier>
      <skos:altLabel xml:lang="bg">CC BY-SA 4.0</skos:altLabel>
      <skos:altLabel xml:lang="cs">CC BY-SA 4.0</skos:altLabel>
      <skos:altLabel xml:lang="da">CC BY-SA 4.0</skos:altLabel>
      <skos:altLabel xml:lang="de">CC BY-SA 4.0</skos:altLabel>
      <skos:altLabel xml:lang="el">CC BY-SA 4.0</skos:altLabel>
      <skos:altLabel xml:lang="en">CC BY-SA 4.0</skos:altLabel>
      <skos:altLabel xml:lang="es">CC BY-SA 4.0</skos:altLabel>
      <skos:altLabel xml:lang="et">CC BY-SA 4.0</skos:altLabel>
      <skos:altLabel xml:lang="fi">CC BY-SA 4.0</skos:altLabel>
      <skos:altLabel xml:lang="fr">CC BY-SA 4.0</skos:altLabel>
      <skos:altLabel xml:lang="ga">CC BY-SA 4.0</skos:altLabel>
      <skos:altLabel xml:lang="hr">CC BY-SA 4.0</skos:altLabel>
      <skos:altLabel xml:lang="hu">CC BY-SA 4.0</skos:altLabel>
      <skos:altLabel xml:lang="it">CC BY-SA 4.0</skos:altLabel>
      <skos:altLabel xml:lang="lt">CC BY-SA 4.0</skos:altLabel>
      <skos:altLabel xml:lang="lv">CC BY-SA 4.0</skos:altLabel>
      <skos:altLabel xml:lang="mt">CC BY-SA 4.0</skos:altLabel>
      <skos:altLabel xml:lang="nl">CC BY-SA 4.0</skos:altLabel>
      <skos:altLabel xml:lang="pl">CC BY-SA 4.0</skos:altLabel>
      <skos:altLabel xml:lang="pt">CC BY-SA 4.0</skos:altLabel>
      <skos:altLabel xml:lang="ro">CC BY-SA 4.0</skos:altLabel>
      <skos:altLabel xml:lang="sk">CC BY-SA 4.0</skos:altLabel>
      <skos:altLabel xml:lang="sl">CC BY-SA 4.0</skos:altLabel>
      <skos:altLabel xml:lang="sv">CC BY-SA 4.0</skos:altLabel>
      <skos:definition xml:lang="en">CC BY-SA 4.0 lets others remix, tweak, and build upon the author’s work even for commercial purposes, as long as they credit the author and licence their new creations under the identical terms. This licence is often compared to “copyleft” free and open source software licences. All new works based on the original work will carry the same licence, so any derivatives will also allow commercial use. This is the licence used by Wikipedia, and is recommended for materials that would benefit from incorporating content from Wikipedia and similarly licenced projects.</skos:definition>
      <skos:definition xml:lang="fr">CC BY-SA 4.0 permet aux autres de remixer, arranger, et adapter l’œuvre de l’auteur/autrice, même à des fins commerciales, tant qu’on accorde le mérite de la création originale à l’auteur/autrice en citant son nom et qu’on diffuse les nouvelles créations selon des conditions identiques. Cette licence est souvent comparée aux licences de logiciels libres, «open source» ou «copyleft». Toutes les nouvelles œuvres basées sur celles de l’auteur/autrice auront la même licence, et toute œuvre dérivée pourra être utilisée même à des fins commerciales. C’est la licence utilisée par Wikipédia; elle est recommandée pour des œuvres qui pourraient bénéficier de l’incorporation de contenu depuis Wikipédia et d’autres projets sous licence similaire.</skos:definition>
      <skos:exactMatch rdf:resource="http://creativecommons.org/licenses/by-sa/4.0/"/>
      <skos:inScheme rdf:resource="http://publications.europa.eu/resource/authority/licence"/>
      <skos:topConceptOf rdf:resource="http://publications.europa.eu/resource/authority/licence"/>
   </skos:Concept>
   <skos:Concept rdf:about="http://publications.europa.eu/resource/authority/licence/CC_BY_1_0"
                 at:deprecated="true">
      <skos:prefLabel xml:lang="bg">Creative Commons Признание 1.0 Неадаптиран</skos:prefLabel>
      <skos:prefLabel xml:lang="cs">Creative Commons Uveďte původ 1.0 Generic</skos:prefLabel>
      <skos:prefLabel xml:lang="da">Creative Commons Kreditering 1.0 Generisk</skos:prefLabel>
      <skos:prefLabel xml:lang="de">Creative Commons Namensnennung 1.0 Generic</skos:prefLabel>
      <skos:prefLabel xml:lang="el">Creative Commons Αναφορά Δημιουργού 1.0 Γενικό</skos:prefLabel>
      <skos:prefLabel xml:lang="en">Creative Commons Attribution 1.0 Generic</skos:prefLabel>
      <skos:prefLabel xml:lang="es">Creative Commons Atribución 1.0 Genérica</skos:prefLabel>
      <skos:prefLabel xml:lang="et">Creative Commons Autorile viitamine 1.0 Üldine</skos:prefLabel>
      <skos:prefLabel xml:lang="fi">Creative Commons Nimeä 1.0 Yleinen</skos:prefLabel>
      <skos:prefLabel xml:lang="fr">Creative Commons Attribution 1.0 Générique</skos:prefLabel>
      <skos:prefLabel xml:lang="hr">Creative Commons Imenovanje 1.0 nelokalizirana licenca</skos:prefLabel>
      <skos:prefLabel xml:lang="hu">Creative Commons Nevezd meg! 1.0 Általános</skos:prefLabel>
      <skos:prefLabel xml:lang="it">Creative Commons Attribuzione 1.0 Generico</skos:prefLabel>
      <skos:prefLabel xml:lang="lt">Creative Commons Priskyrimas 1.0 Bendrasis</skos:prefLabel>
      <skos:prefLabel xml:lang="lv">Creative Commons Atsaucoties 1.0 Vispārīgs</skos:prefLabel>
      <skos:prefLabel xml:lang="mt">Creative Commons Attribuzzjoni 1.0 Generic</skos:prefLabel>
      <skos:prefLabel xml:lang="nl">Creative Commons Naamsvermelding 1.0 Unported</skos:prefLabel>
      <skos:prefLabel xml:lang="pl">Creative Commons Uznanie autorstwa 1.0 Ogólny</skos:prefLabel>
      <skos:prefLabel xml:lang="pt">Creative Commons Atribuição 1.0 Genérica</skos:prefLabel>
      <skos:prefLabel xml:lang="ro">Creative Commons Atribuire 1.0 Generică</skos:prefLabel>
      <skos:prefLabel xml:lang="sk">Creative Commons Uvedenie Autora 1.0 Generic</skos:prefLabel>
      <skos:prefLabel xml:lang="sl">Creative Commons Priznanje avtorstva 1.0 Generična</skos:prefLabel>
      <skos:prefLabel xml:lang="sv">Creative Commons Erkännande 1.0 Generisk</skos:prefLabel>
      <at:authority-code>CC_BY_1_0</at:authority-code>
      <at:op-code>CC_BY_1_0</at:op-code>
      <at:start.use>2002-12-15</at:start.use>
      <atold:op-code>CC_BY_1_0</atold:op-code>
      <dc:identifier>CC_BY_1_0</dc:identifier>
      <skos:altLabel xml:lang="bg">CC BY 1.0</skos:altLabel>
      <skos:altLabel xml:lang="cs">CC BY 1.0</skos:altLabel>
      <skos:altLabel xml:lang="da">CC BY 1.0</skos:altLabel>
      <skos:altLabel xml:lang="de">CC BY 1.0</skos:altLabel>
      <skos:altLabel xml:lang="el">CC BY 1.0</skos:altLabel>
      <skos:altLabel xml:lang="en">CC BY 1.0</skos:altLabel>
      <skos:altLabel xml:lang="es">CC BY 1.0</skos:altLabel>
      <skos:altLabel xml:lang="et">CC BY 1.0</skos:altLabel>
      <skos:altLabel xml:lang="fi">CC BY 1.0</skos:altLabel>
      <skos:altLabel xml:lang="fr">CC BY 1.0</skos:altLabel>
      <skos:altLabel xml:lang="ga">CC BY 1.0</skos:altLabel>
      <skos:altLabel xml:lang="hr">CC BY 1.0</skos:altLabel>
      <skos:altLabel xml:lang="hu">CC BY 1.0</skos:altLabel>
      <skos:altLabel xml:lang="it">CC BY 1.0</skos:altLabel>
      <skos:altLabel xml:lang="lt">CC BY 1.0</skos:altLabel>
      <skos:altLabel xml:lang="lv">CC BY 1.0</skos:altLabel>
      <skos:altLabel xml:lang="mt">CC BY 1.0</skos:altLabel>
      <skos:altLabel xml:lang="nl">CC BY 1.0</skos:altLabel>
      <skos:altLabel xml:lang="pl">CC BY 1.0</skos:altLabel>
      <skos:altLabel xml:lang="pt">CC BY 1.0</skos:altLabel>
      <skos:altLabel xml:lang="ro">CC BY 1.0</skos:altLabel>
      <skos:altLabel xml:lang="sk">CC BY 1.0</skos:altLabel>
      <skos:altLabel xml:lang="sl">CC BY 1.0</skos:altLabel>
      <skos:altLabel xml:lang="sv">CC BY 1.0</skos:altLabel>
      <skos:definition xml:lang="en">CC BY 1.0 lets others distribute, remix, tweak, and build upon the author’s work, even commercially, as long as they credit the author for the original creation. This is the most accommodating of licences offered. Recommended for maximum dissemination and use of licenced materials.</skos:definition>
      <skos:definition xml:lang="fr">CC BY 1.0 permet aux autres de distribuer, remixer, arranger, et adapter l’œuvre de l’auteur/autrice, même à des fins commerciales, tant qu’on accorde le mérite de la création originale à l’auteur/autrice en citant son nom. C’est le contrat le plus souple proposé. Recommandé pour la diffusion et l’utilisation maximales d’œuvres licenciées sous CC.</skos:definition>
      <skos:exactMatch rdf:resource="http://creativecommons.org/licenses/by/1.0/"/>
      <skos:inScheme rdf:resource="http://publications.europa.eu/resource/authority/licence"/>
      <skos:topConceptOf rdf:resource="http://publications.europa.eu/resource/authority/licence"/>
      <at:end.use>2004-05-24</at:end.use>
   </skos:Concept>
   <skos:Concept rdf:about="http://publications.europa.eu/resource/authority/licence/CC_BY_2_0"
                 at:deprecated="false">
      <skos:prefLabel xml:lang="bg">Creative Commons Признание 2.0 Неадаптиран</skos:prefLabel>
      <skos:prefLabel xml:lang="cs">Creative Commons Uveďte původ 2.0 Generic</skos:prefLabel>
      <skos:prefLabel xml:lang="da">Creative Commons Kreditering 2.0 Generisk</skos:prefLabel>
      <skos:prefLabel xml:lang="de">Creative Commons Namensnennung 2.0 Generic</skos:prefLabel>
      <skos:prefLabel xml:lang="el">Creative Commons Αναφορά Δημιουργού 2.0 Γενικό</skos:prefLabel>
      <skos:prefLabel xml:lang="en">Creative Commons Attribution 2.0 Generic</skos:prefLabel>
      <skos:prefLabel xml:lang="es">Creative Commons Atribución 2.0 Genérica</skos:prefLabel>
      <skos:prefLabel xml:lang="et">Creative Commons Autorile viitamine 2.0 Üldine</skos:prefLabel>
      <skos:prefLabel xml:lang="fi">Creative Commons Nimeä 2.0 Yleinen</skos:prefLabel>
      <skos:prefLabel xml:lang="fr">Creative Commons Attribution 2.0 Générique</skos:prefLabel>
      <skos:prefLabel xml:lang="hr">Creative Commons Imenovanje 2.0 nelokalizirana licenca</skos:prefLabel>
      <skos:prefLabel xml:lang="hu">Creative Commons Nevezd meg! 2.0 Általános</skos:prefLabel>
      <skos:prefLabel xml:lang="it">Creative Commons Attribuzione 2.0 Generico</skos:prefLabel>
      <skos:prefLabel xml:lang="lt">Creative Commons Priskyrimas 2.0 Bendrasis</skos:prefLabel>
      <skos:prefLabel xml:lang="lv">Creative Commons Atsaucoties 2.0 Vispārīgs</skos:prefLabel>
      <skos:prefLabel xml:lang="mt">Creative Commons Attribuzzjoni 2.0 Generic</skos:prefLabel>
      <skos:prefLabel xml:lang="nl">Creative Commons Naamsvermelding 2.0 Unported</skos:prefLabel>
      <skos:prefLabel xml:lang="pl">Creative Commons Uznanie autorstwa 2.0 Ogólny</skos:prefLabel>
      <skos:prefLabel xml:lang="pt">Creative Commons Atribuição 2.0 Genérica</skos:prefLabel>
      <skos:prefLabel xml:lang="ro">Creative Commons Atribuire 2.0 Generică</skos:prefLabel>
      <skos:prefLabel xml:lang="sk">Creative Commons Uvedenie Autora 2.0 Generic</skos:prefLabel>
      <skos:prefLabel xml:lang="sl">Creative Commons Priznanje avtorstva 2.0 Generična</skos:prefLabel>
      <skos:prefLabel xml:lang="sv">Creative Commons Erkännande 2.0 Generisk</skos:prefLabel>
      <at:authority-code>CC_BY_2_0</at:authority-code>
      <at:op-code>CC_BY_2_0</at:op-code>
      <at:start.use>2004-05-25</at:start.use>
      <atold:op-code>CC_BY_2_0</atold:op-code>
      <dc:identifier>CC_BY_2_0</dc:identifier>
      <skos:altLabel xml:lang="bg">CC BY 2.0</skos:altLabel>
      <skos:altLabel xml:lang="cs">CC BY 2.0</skos:altLabel>
      <skos:altLabel xml:lang="da">CC BY 2.0</skos:altLabel>
      <skos:altLabel xml:lang="de">CC BY 2.0</skos:altLabel>
      <skos:altLabel xml:lang="el">CC BY 2.0</skos:altLabel>
      <skos:altLabel xml:lang="en">CC BY 2.0</skos:altLabel>
      <skos:altLabel xml:lang="es">CC BY 2.0</skos:altLabel>
      <skos:altLabel xml:lang="et">CC BY 2.0</skos:altLabel>
      <skos:altLabel xml:lang="fi">CC BY 2.0</skos:altLabel>
      <skos:altLabel xml:lang="fr">CC BY 2.0</skos:altLabel>
      <skos:altLabel xml:lang="ga">CC BY 2.0</skos:altLabel>
      <skos:altLabel xml:lang="hr">CC BY 2.0</skos:altLabel>
      <skos:altLabel xml:lang="hu">CC BY 2.0</skos:altLabel>
      <skos:altLabel xml:lang="it">CC BY 2.0</skos:altLabel>
      <skos:altLabel xml:lang="lt">CC BY 2.0</skos:altLabel>
      <skos:altLabel xml:lang="lv">CC BY 2.0</skos:altLabel>
      <skos:altLabel xml:lang="mt">CC BY 2.0</skos:altLabel>
      <skos:altLabel xml:lang="nl">CC BY 2.0</skos:altLabel>
      <skos:altLabel xml:lang="pl">CC BY 2.0</skos:altLabel>
      <skos:altLabel xml:lang="pt">CC BY 2.0</skos:altLabel>
      <skos:altLabel xml:lang="ro">CC BY 2.0</skos:altLabel>
      <skos:altLabel xml:lang="sk">CC BY 2.0</skos:altLabel>
      <skos:altLabel xml:lang="sl">CC BY 2.0</skos:altLabel>
      <skos:altLabel xml:lang="sv">CC BY 2.0</skos:altLabel>
      <skos:definition xml:lang="en">CC BY 2.0 lets others distribute, remix, tweak, and build upon the author’s work, even commercially, as long as they credit the author for the original creation. This is the most accommodating of licences offered. Recommended for maximum dissemination and use of licenced materials.</skos:definition>
      <skos:definition xml:lang="fr">CC BY 2.0 permet aux autres de distribuer, remixer, arranger, et adapter l’œuvre de l’auteur/autrice, même à des fins commerciales, tant qu’on accorde le mérite de la création originale à l’auteur/autrice en citant son nom. C’est le contrat le plus souple proposé. Recommandé pour la diffusion et l’utilisation maximales d’œuvres licenciées sous CC.</skos:definition>
      <skos:exactMatch rdf:resource="http://creativecommons.org/licenses/by/2.0/"/>
      <skos:inScheme rdf:resource="http://publications.europa.eu/resource/authority/licence"/>
      <skos:topConceptOf rdf:resource="http://publications.europa.eu/resource/authority/licence"/>
   </skos:Concept>
   <skos:Concept rdf:about="http://publications.europa.eu/resource/authority/licence/CC_BY_2_5"
                 at:deprecated="false">
      <skos:prefLabel xml:lang="de">Creative Commons Namensnennung – Weitergabe unter gleichen Bedingungen 2.5 Generic</skos:prefLabel>
      <skos:prefLabel xml:lang="bg">Creative Commons Признание 2.5 Неадаптиран</skos:prefLabel>
      <skos:prefLabel xml:lang="cs">Creative Commons Uveďte původ 2.5 Generic</skos:prefLabel>
      <skos:prefLabel xml:lang="da">Creative Commons Kreditering 2.5 Generisk</skos:prefLabel>
      <skos:prefLabel xml:lang="el">Creative Commons Αναφορά Δημιουργού 2.5 Γενικό</skos:prefLabel>
      <skos:prefLabel xml:lang="en">Creative Commons Attribution 2.5 Generic</skos:prefLabel>
      <skos:prefLabel xml:lang="es">Creative Commons Atribución 2.5 Genérica</skos:prefLabel>
      <skos:prefLabel xml:lang="et">Creative Commons Autorile viitamine 2.5 Üldine</skos:prefLabel>
      <skos:prefLabel xml:lang="fi">Creative Commons Nimeä 2.5 Yleinen</skos:prefLabel>
      <skos:prefLabel xml:lang="fr">Creative Commons Attribution 2.5 Générique</skos:prefLabel>
      <skos:prefLabel xml:lang="hr">Creative Commons Imenovanje 2.5 nelokalizirana licenca</skos:prefLabel>
      <skos:prefLabel xml:lang="hu">Creative Commons Nevezd meg! 2.5 Általános</skos:prefLabel>
      <skos:prefLabel xml:lang="it">Creative Commons Attribuzione 2.5 Generico</skos:prefLabel>
      <skos:prefLabel xml:lang="lt">Creative Commons Priskyrimas 2.5 Bendrasis</skos:prefLabel>
      <skos:prefLabel xml:lang="lv">Creative Commons Atsaucoties 2.5 Vispārīgs</skos:prefLabel>
      <skos:prefLabel xml:lang="mt">Creative Commons Attribuzzjoni 2.5 Generic</skos:prefLabel>
      <skos:prefLabel xml:lang="nl">Creative Commons Naamsvermelding 2.5 Unported</skos:prefLabel>
      <skos:prefLabel xml:lang="pl">Creative Commons Uznanie autorstwa 2.5 Ogólny</skos:prefLabel>
      <skos:prefLabel xml:lang="pt">Creative Commons Atribuição 2.5 Genérica</skos:prefLabel>
      <skos:prefLabel xml:lang="ro">Creative Commons Atribuire 2.5 Generică</skos:prefLabel>
      <skos:prefLabel xml:lang="sk">Creative Commons Uvedenie Autora 2.5 Generic</skos:prefLabel>
      <skos:prefLabel xml:lang="sl">Creative Commons Priznanje avtorstva 2.5 Generična</skos:prefLabel>
      <skos:prefLabel xml:lang="sv">Creative Commons Erkännande 2.5 Generisk</skos:prefLabel>
      <at:authority-code>CC_BY_2_5</at:authority-code>
      <at:op-code>CC_BY_2_5</at:op-code>
      <at:start.use>2005-06-01</at:start.use>
      <atold:op-code>CC_BY_2_5</atold:op-code>
      <dc:identifier>CC_BY_2_5</dc:identifier>
      <skos:altLabel xml:lang="bg">CC BY 2.5</skos:altLabel>
      <skos:altLabel xml:lang="cs">CC BY 2.5</skos:altLabel>
      <skos:altLabel xml:lang="da">CC BY 2.5</skos:altLabel>
      <skos:altLabel xml:lang="de">CC BY 2.5</skos:altLabel>
      <skos:altLabel xml:lang="el">CC BY 2.5</skos:altLabel>
      <skos:altLabel xml:lang="en">CC BY 2.5</skos:altLabel>
      <skos:altLabel xml:lang="es">CC BY 2.5</skos:altLabel>
      <skos:altLabel xml:lang="et">CC BY 2.5</skos:altLabel>
      <skos:altLabel xml:lang="fi">CC BY 2.5</skos:altLabel>
      <skos:altLabel xml:lang="fr">CC BY 2.5</skos:altLabel>
      <skos:altLabel xml:lang="ga">CC BY 2.5</skos:altLabel>
      <skos:altLabel xml:lang="hr">CC BY 2.5</skos:altLabel>
      <skos:altLabel xml:lang="hu">CC BY 2.5</skos:altLabel>
      <skos:altLabel xml:lang="it">CC BY 2.5</skos:altLabel>
      <skos:altLabel xml:lang="lt">CC BY 2.5</skos:altLabel>
      <skos:altLabel xml:lang="lv">CC BY 2.5</skos:altLabel>
      <skos:altLabel xml:lang="mt">CC BY 2.5</skos:altLabel>
      <skos:altLabel xml:lang="nl">CC BY 2.5</skos:altLabel>
      <skos:altLabel xml:lang="pl">CC BY 2.5</skos:altLabel>
      <skos:altLabel xml:lang="pt">CC BY 2.5</skos:altLabel>
      <skos:altLabel xml:lang="ro">CC BY 2.5</skos:altLabel>
      <skos:altLabel xml:lang="sk">CC BY 2.5</skos:altLabel>
      <skos:altLabel xml:lang="sl">CC BY 2.5</skos:altLabel>
      <skos:altLabel xml:lang="sv">CC BY 2.5</skos:altLabel>
      <skos:definition xml:lang="en">CC BY 2.5 lets others distribute, remix, tweak, and build upon the author’s work, even commercially, as long as they credit the author for the original creation. This is the most accommodating of licences offered. Recommended for maximum dissemination and use of licenced materials.</skos:definition>
      <skos:definition xml:lang="fr">CC BY 2.5 permet aux autres de distribuer, remixer, arranger, et adapter l’œuvre de l’auteur/autrice, même à des fins commerciales, tant qu’on accorde le mérite de la création originale à l’auteur/autrice en citant son nom. C’est le contrat le plus souple proposé. Recommandé pour la diffusion et l’utilisation maximales d’œuvres licenciées sous CC.</skos:definition>
      <skos:exactMatch rdf:resource="http://creativecommons.org/licenses/by/2.5/"/>
      <skos:inScheme rdf:resource="http://publications.europa.eu/resource/authority/licence"/>
      <skos:topConceptOf rdf:resource="http://publications.europa.eu/resource/authority/licence"/>
   </skos:Concept>
   <skos:Concept rdf:about="http://publications.europa.eu/resource/authority/licence/CC_BY_3_0"
                 at:deprecated="false">
      <skos:prefLabel xml:lang="bg">Creative Commons Признание 3.0 Нелокализиран</skos:prefLabel>
      <skos:prefLabel xml:lang="cs">Creative Commons Uveďte původ 3.0 Unported</skos:prefLabel>
      <skos:prefLabel xml:lang="da">Creative Commons Kreditering 3.0 Ikke porteret</skos:prefLabel>
      <skos:prefLabel xml:lang="de">Creative Commons Namensnennung 3.0 Unported</skos:prefLabel>
      <skos:prefLabel xml:lang="el">Creative Commons Αναφορά Δημιουργού 3.0 Μη εισαγόμενο</skos:prefLabel>
      <skos:prefLabel xml:lang="en">Creative Commons Attribution 3.0 Unported</skos:prefLabel>
      <skos:prefLabel xml:lang="es">Creative Commons Atribución 3.0 Unported</skos:prefLabel>
      <skos:prefLabel xml:lang="et">Creative Commons Autorile viitamine 3.0 Jurisdiktsiooniga sidumata</skos:prefLabel>
      <skos:prefLabel xml:lang="fi">Creative Commons Nimeä 3.0 Ei sovitettu</skos:prefLabel>
      <skos:prefLabel xml:lang="fr">Creative Commons Attribution 3.0 non transposé</skos:prefLabel>
      <skos:prefLabel xml:lang="hr">Creative Commons Imenovanje 3.0 nelokalizirana licenca</skos:prefLabel>
      <skos:prefLabel xml:lang="hu">Creative Commons Nevezd meg! 3.0 Unported</skos:prefLabel>
      <skos:prefLabel xml:lang="it">Creative Commons Attribuzione 3.0 Unported</skos:prefLabel>
      <skos:prefLabel xml:lang="lt">Creative Commons Priskyrimas 3.0 Nepritaikyta jurisdikcijai</skos:prefLabel>
      <skos:prefLabel xml:lang="lv">Creative Commons Atsaucoties 3.0 Nepārnesta</skos:prefLabel>
      <skos:prefLabel xml:lang="mt">Creative Commons Attribuzzjoni 3.0 Unported</skos:prefLabel>
      <skos:prefLabel xml:lang="nl">Creative Commons Naamsvermelding 3.0 Unported</skos:prefLabel>
      <skos:prefLabel xml:lang="pl">Creative Commons Uznanie autorstwa 3.0 Unported</skos:prefLabel>
      <skos:prefLabel xml:lang="pt">Creative Commons Atribuição 3.0 Não Adaptada</skos:prefLabel>
      <skos:prefLabel xml:lang="ro">Creative Commons Atribuire 3.0 Ne-adaptată</skos:prefLabel>
      <skos:prefLabel xml:lang="sk">Creative Commons Uvedenie Autora 3.0 Unported</skos:prefLabel>
      <skos:prefLabel xml:lang="sl">Creative Commons Priznanje avtorstva 3.0 Nedoločena</skos:prefLabel>
      <skos:prefLabel xml:lang="sv">Creative Commons Erkännande 3.0 Unported</skos:prefLabel>
      <at:authority-code>CC_BY_3_0</at:authority-code>
      <at:op-code>CC_BY_3_0</at:op-code>
      <at:start.use>2007-02-23</at:start.use>
      <atold:op-code>CC_BY_3_0</atold:op-code>
      <dc:identifier>CC_BY_3_0</dc:identifier>
      <skos:altLabel xml:lang="bg">CC BY 3.0</skos:altLabel>
      <skos:altLabel xml:lang="cs">CC BY 3.0</skos:altLabel>
      <skos:altLabel xml:lang="da">CC BY 3.0</skos:altLabel>
      <skos:altLabel xml:lang="de">CC BY 3.0</skos:altLabel>
      <skos:altLabel xml:lang="el">CC BY 3.0</skos:altLabel>
      <skos:altLabel xml:lang="en">CC BY 3.0</skos:altLabel>
      <skos:altLabel xml:lang="es">CC BY 3.0</skos:altLabel>
      <skos:altLabel xml:lang="et">CC BY 3.0</skos:altLabel>
      <skos:altLabel xml:lang="fi">CC BY 3.0</skos:altLabel>
      <skos:altLabel xml:lang="fr">CC BY 3.0</skos:altLabel>
      <skos:altLabel xml:lang="ga">CC BY 3.0</skos:altLabel>
      <skos:altLabel xml:lang="hr">CC BY 3.0</skos:altLabel>
      <skos:altLabel xml:lang="hu">CC BY 3.0</skos:altLabel>
      <skos:altLabel xml:lang="it">CC BY 3.0</skos:altLabel>
      <skos:altLabel xml:lang="lt">CC BY 3.0</skos:altLabel>
      <skos:altLabel xml:lang="lv">CC BY 3.0</skos:altLabel>
      <skos:altLabel xml:lang="mt">CC BY 3.0</skos:altLabel>
      <skos:altLabel xml:lang="nl">CC BY 3.0</skos:altLabel>
      <skos:altLabel xml:lang="pl">CC BY 3.0</skos:altLabel>
      <skos:altLabel xml:lang="pt">CC BY 3.0</skos:altLabel>
      <skos:altLabel xml:lang="ro">CC BY 3.0</skos:altLabel>
      <skos:altLabel xml:lang="sk">CC BY 3.0</skos:altLabel>
      <skos:altLabel xml:lang="sl">CC BY 3.0</skos:altLabel>
      <skos:altLabel xml:lang="sv">CC BY 3.0</skos:altLabel>
      <skos:definition xml:lang="en">CC BY 3.0 lets others distribute, remix, tweak, and build upon the author’s work, even commercially, as long as they credit the author for the original creation. This is the most accommodating of licences offered. Recommended for maximum dissemination and use of licenced materials.</skos:definition>
      <skos:definition xml:lang="fr">CC BY 3.0 permet aux autres de distribuer, remixer, arranger, et adapter l’œuvre de l’auteur/autrice, même à des fins commerciales, tant qu’on accorde le mérite de la création originale à l’auteur/autrice en citant son nom. C’est le contrat le plus souple proposé. Recommandé pour la diffusion et l’utilisation maximales d’œuvres licenciées sous CC.</skos:definition>
      <skos:exactMatch rdf:resource="http://creativecommons.org/licenses/by/3.0/"/>
      <skos:inScheme rdf:resource="http://publications.europa.eu/resource/authority/licence"/>
      <skos:topConceptOf rdf:resource="http://publications.europa.eu/resource/authority/licence"/>
      <skos:historyNote xml:lang="en">Unported licences are licences that are not associated with any specific jurisdiction, e.g. country.</skos:historyNote>
   </skos:Concept>
   <skos:Concept rdf:about="http://publications.europa.eu/resource/authority/licence/CC_BY_3_0_AT"
                 at:deprecated="false">
      <skos:prefLabel xml:lang="bg">Признание 3.0 Австрия</skos:prefLabel>
      <skos:prefLabel xml:lang="cs">Uveďte původ 3.0 Rakousko</skos:prefLabel>
      <skos:prefLabel xml:lang="da">Kreditering 3.0 Østrig</skos:prefLabel>
      <skos:prefLabel xml:lang="de">Namensnennung 3.0 Österreich</skos:prefLabel>
      <skos:prefLabel xml:lang="el">Αναφορά Δημιουργού 3.0</skos:prefLabel>
      <skos:prefLabel xml:lang="en">Attribution 3.0 Austria</skos:prefLabel>
      <skos:prefLabel xml:lang="es">Atribución 3.0 Austria</skos:prefLabel>
      <skos:prefLabel xml:lang="et">Autorile viitamine 3.0 Austria</skos:prefLabel>
      <skos:prefLabel xml:lang="fi">Nimeä 3.0 Itävalta</skos:prefLabel>
      <skos:prefLabel xml:lang="fr">Attribution 3.0 Autriche</skos:prefLabel>
      <skos:prefLabel xml:lang="hr">Imenovanje 3.0 Austrija</skos:prefLabel>
      <skos:prefLabel xml:lang="hu">Nevezd meg! 3.0 Ausztria</skos:prefLabel>
      <skos:prefLabel xml:lang="it">Attribuzione 3.0 Austria</skos:prefLabel>
      <skos:prefLabel xml:lang="lt">Priskyrimas 3.0 Austrija</skos:prefLabel>
      <skos:prefLabel xml:lang="lv">Attiecinājums 3.0 Austrija</skos:prefLabel>
      <skos:prefLabel xml:lang="mt">Attribuzzjoni 3.0 Awstrija</skos:prefLabel>
      <skos:prefLabel xml:lang="nl">Naamsvermelding 3.0 Oostenrijk</skos:prefLabel>
      <skos:prefLabel xml:lang="pl">Uznanie autorstwa 3.0 Austria</skos:prefLabel>
      <skos:prefLabel xml:lang="pt">Atribuição 3.0 Áustria</skos:prefLabel>
      <skos:prefLabel xml:lang="ro">Atribuire 3.0 Austria</skos:prefLabel>
      <skos:prefLabel xml:lang="sk">Uvedenie Autora 3.0 Rakúsko</skos:prefLabel>
      <skos:prefLabel xml:lang="sl">Priznanje avtorstva 3.0 Avstrija</skos:prefLabel>
      <skos:prefLabel xml:lang="sv">Erkännande 3.0 Österrike</skos:prefLabel>
      <at:authority-code>CC_BY_3_0_AT</at:authority-code>
      <at:op-code>CC_BY_3_0_AT</at:op-code>
      <at:start.use>2007-02-23</at:start.use>
      <atold:op-code>CC_BY_3_0_AT</atold:op-code>
      <dc:identifier>CC_BY_3_0_AT</dc:identifier>
      <skos:altLabel xml:lang="bg">CC BY 3.0 AT</skos:altLabel>
      <skos:altLabel xml:lang="cs">CC BY 3.0 AT</skos:altLabel>
      <skos:altLabel xml:lang="da">CC BY 3.0 AT</skos:altLabel>
      <skos:altLabel xml:lang="de">CC BY 3.0 AT</skos:altLabel>
      <skos:altLabel xml:lang="el">CC BY 3.0 AT</skos:altLabel>
      <skos:altLabel xml:lang="en">CC BY 3.0 AT</skos:altLabel>
      <skos:altLabel xml:lang="es">CC BY 3.0 NL</skos:altLabel>
      <skos:altLabel xml:lang="et">CC BY 3.0 AT</skos:altLabel>
      <skos:altLabel xml:lang="fi">CC BY 3.0 AT</skos:altLabel>
      <skos:altLabel xml:lang="fr">CC BY 3.0 AT</skos:altLabel>
      <skos:altLabel xml:lang="ga">CC BY 3.0 AT</skos:altLabel>
      <skos:altLabel xml:lang="hr">CC BY 3.0 AT</skos:altLabel>
      <skos:altLabel xml:lang="hu">CC BY 3.0 AT</skos:altLabel>
      <skos:altLabel xml:lang="it">CC BY 3.0 AT</skos:altLabel>
      <skos:altLabel xml:lang="lt">CC BY 3.0 AT</skos:altLabel>
      <skos:altLabel xml:lang="lv">CC BY 3.0 AT</skos:altLabel>
      <skos:altLabel xml:lang="mt">CC BY 3.0 AT</skos:altLabel>
      <skos:altLabel xml:lang="nl">CC BY 3.0 AT</skos:altLabel>
      <skos:altLabel xml:lang="pl">CC BY 3.0 AT</skos:altLabel>
      <skos:altLabel xml:lang="pt">CC BY 3.0 AT</skos:altLabel>
      <skos:altLabel xml:lang="ro">CC BY 3.0 AT</skos:altLabel>
      <skos:altLabel xml:lang="sk">CC BY 3.0 AT</skos:altLabel>
      <skos:altLabel xml:lang="sl">CC BY 3.0 AT</skos:altLabel>
      <skos:altLabel xml:lang="sv">CC BY 3.0 AT</skos:altLabel>
      <skos:definition xml:lang="en">Published by Creative Commons for Austria, Namensnennung 3.0 Österreich (CC BY 3.0 AT) is a licence permitting any commercial and non-commercial use as long as credit is given to the author for the original creation.</skos:definition>
      <skos:exactMatch rdf:resource="https://creativecommons.org/licenses/by/3.0/at/legalcode"/>
      <skos:inScheme rdf:resource="http://publications.europa.eu/resource/authority/licence"/>
      <skos:topConceptOf rdf:resource="http://publications.europa.eu/resource/authority/licence"/>
   </skos:Concept>
   <skos:Concept rdf:about="http://publications.europa.eu/resource/authority/licence/CC_BY_3_0_NL"
                 at:deprecated="false">
      <skos:prefLabel xml:lang="bg">Признание 3.0 Холандия</skos:prefLabel>
      <skos:prefLabel xml:lang="cs">Uveďte původ 3.0 Nizozemí</skos:prefLabel>
      <skos:prefLabel xml:lang="da">Kreditering 3.0 Holland</skos:prefLabel>
      <skos:prefLabel xml:lang="de">Namensnennung 3.0 Niederlande</skos:prefLabel>
      <skos:prefLabel xml:lang="el">Αναφορά Δημιουργού 3.0 Ολλανδία</skos:prefLabel>
      <skos:prefLabel xml:lang="en">Attribution 3.0 Netherlands</skos:prefLabel>
      <skos:prefLabel xml:lang="es">Atribución 3.0 Países Bajos</skos:prefLabel>
      <skos:prefLabel xml:lang="et">Autorile viitamine 3.0 Holland</skos:prefLabel>
      <skos:prefLabel xml:lang="fi">Nimeä 3.0 Hollanti</skos:prefLabel>
      <skos:prefLabel xml:lang="fr">Attribution 3.0 Pays-Bas</skos:prefLabel>
      <skos:prefLabel xml:lang="hr">Imenovanje 3.0 Nizozemska</skos:prefLabel>
      <skos:prefLabel xml:lang="hu">Nevezd meg! 3.0 Hollandia</skos:prefLabel>
      <skos:prefLabel xml:lang="it">Attribuzione 3.0 Olanda</skos:prefLabel>
      <skos:prefLabel xml:lang="lt">Priskyrimas 3.0 Nyderlandai</skos:prefLabel>
      <skos:prefLabel xml:lang="lv">Attiecinājums 3.0 Nīderlande</skos:prefLabel>
      <skos:prefLabel xml:lang="mt">Attribuzzjoni 3.0 Pajjiżi l-Baxxi</skos:prefLabel>
      <skos:prefLabel xml:lang="nl">Naamsvermelding 3.0 Nederland</skos:prefLabel>
      <skos:prefLabel xml:lang="pl">Uznanie autorstwa 3.0 Holandia</skos:prefLabel>
      <skos:prefLabel xml:lang="pt">Atribuição 3.0 Holanda</skos:prefLabel>
      <skos:prefLabel xml:lang="ro">Atribuire 3.0 Olanda</skos:prefLabel>
      <skos:prefLabel xml:lang="sk">Uvedenie Autora 3.0 Holandsko</skos:prefLabel>
      <skos:prefLabel xml:lang="sl">Priznanje avtorstva 3.0 Nizozemska</skos:prefLabel>
      <skos:prefLabel xml:lang="sv">Erkännande 3.0 Nederländerna</skos:prefLabel>
      <at:authority-code>CC_BY_3_0_NL</at:authority-code>
      <at:op-code>CC_BY_3_0_NL</at:op-code>
      <at:start.use>2007-02-23</at:start.use>
      <atold:op-code>CC_BY_3_0_NL</atold:op-code>
      <dc:identifier>CC_BY_3_0_NL</dc:identifier>
      <skos:altLabel xml:lang="es">CC BY 3.0 NL</skos:altLabel>
      <skos:altLabel xml:lang="bg">CC BY 3.0 NL</skos:altLabel>
      <skos:altLabel xml:lang="cs">CC BY 3.0 NL</skos:altLabel>
      <skos:altLabel xml:lang="da">CC BY 3.0 NL</skos:altLabel>
      <skos:altLabel xml:lang="de">CC BY 3.0 NL</skos:altLabel>
      <skos:altLabel xml:lang="el">CC BY 3.0 NL</skos:altLabel>
      <skos:altLabel xml:lang="en">CC BY 3.0 NL</skos:altLabel>
      <skos:altLabel xml:lang="et">CC BY 3.0 NL</skos:altLabel>
      <skos:altLabel xml:lang="fi">CC BY 3.0 NL</skos:altLabel>
      <skos:altLabel xml:lang="fr">CC BY 3.0 NL</skos:altLabel>
      <skos:altLabel xml:lang="ga">CC BY 3.0 NL</skos:altLabel>
      <skos:altLabel xml:lang="hr">CC BY 3.0 NL</skos:altLabel>
      <skos:altLabel xml:lang="hu">CC BY 3.0 NL</skos:altLabel>
      <skos:altLabel xml:lang="it">CC BY 3.0 NL</skos:altLabel>
      <skos:altLabel xml:lang="lt">CC BY 3.0 NL</skos:altLabel>
      <skos:altLabel xml:lang="lv">CC BY 3.0 NL</skos:altLabel>
      <skos:altLabel xml:lang="mt">CC BY 3.0 NL</skos:altLabel>
      <skos:altLabel xml:lang="nl">CC BY 3.0 NL</skos:altLabel>
      <skos:altLabel xml:lang="pl">CC BY 3.0 NL</skos:altLabel>
      <skos:altLabel xml:lang="pt">CC BY 3.0 NL</skos:altLabel>
      <skos:altLabel xml:lang="ro">CC BY 3.0 NL</skos:altLabel>
      <skos:altLabel xml:lang="sk">CC BY 3.0 NL</skos:altLabel>
      <skos:altLabel xml:lang="sl">CC BY 3.0 NL</skos:altLabel>
      <skos:altLabel xml:lang="sv">CC BY 3.0 NL</skos:altLabel>
      <skos:definition xml:lang="en">Published by Creative Commons for Netherlands, Naamsvermelding 3.0 Nederland (CC BY 3.0 NL) is a licence permitting any commercial and non-commercial use as long as credit is given to the author for the original creation.</skos:definition>
      <skos:exactMatch rdf:resource="http://creativecommons.org/licenses/by/3.0/nl/legalcode"/>
      <skos:inScheme rdf:resource="http://publications.europa.eu/resource/authority/licence"/>
      <skos:topConceptOf rdf:resource="http://publications.europa.eu/resource/authority/licence"/>
   </skos:Concept>
   <skos:Concept rdf:about="http://publications.europa.eu/resource/authority/licence/CC_BY_4_0"
                 at:deprecated="false">
      <skos:prefLabel xml:lang="cs">Creative Commons Uveďte původ 4.0 Mezinárodní</skos:prefLabel>
      <skos:prefLabel xml:lang="de">Creative Commons Namensnennung 4.0 International</skos:prefLabel>
      <skos:prefLabel xml:lang="el">Creative Commons Αναφορά Δημιουργού 4.0 Διεθνές</skos:prefLabel>
      <skos:prefLabel xml:lang="en">Creative Commons Attribution 4.0 International</skos:prefLabel>
      <skos:prefLabel xml:lang="es">Creative Commons Atribución 4.0 Internacional</skos:prefLabel>
      <skos:prefLabel xml:lang="fi">Creative Commons Nimeä 4.0 Kansainvälinen</skos:prefLabel>
      <skos:prefLabel xml:lang="fr">Creative Commons Attribution 4.0 International</skos:prefLabel>
      <skos:prefLabel xml:lang="hr">Creative Commons Imenovanje 4.0 međunarodna</skos:prefLabel>
      <skos:prefLabel xml:lang="hu">Creative Commons Nevezd meg! 4.0 Nemzetközi</skos:prefLabel>
      <skos:prefLabel xml:lang="it">Creative Commons Attribuzione 4.0 Internazionale</skos:prefLabel>
      <skos:prefLabel xml:lang="lt">Creative Commons Priskyrimas 4.0 Tarptautinė</skos:prefLabel>
      <skos:prefLabel xml:lang="lv">Creative Commons Atsaucoties 4.0 Internacionāls</skos:prefLabel>
      <skos:prefLabel xml:lang="nl">Creative Commons Naamsvermelding 4.0 Internationaal</skos:prefLabel>
      <skos:prefLabel xml:lang="pl">Creative Commons Uznanie autorstwa 4.0 Międzynarodowe</skos:prefLabel>
      <skos:prefLabel xml:lang="pt">Creative Commons Atribuição 4.0 Internacional</skos:prefLabel>
      <skos:prefLabel xml:lang="ro">Creative Commons Atribuire 4.0 Internațional</skos:prefLabel>
      <skos:prefLabel xml:lang="sv">Creative Commons Erkännande 4.0 Internationell</skos:prefLabel>
      <skos:prefLabel xml:lang="bg">Creative Commons Признание 4.0 Международен</skos:prefLabel>
      <skos:prefLabel xml:lang="da">Creative Commons Kreditering 4.0 International</skos:prefLabel>
      <skos:prefLabel xml:lang="et">Creative Commons Autorile viitamine 4.0 Rahvusvaheline</skos:prefLabel>
      <skos:prefLabel xml:lang="mt">Creative Commons Attribuzzjoni 4.0 Internazzjonali</skos:prefLabel>
      <skos:prefLabel xml:lang="sk">Creative Commons Uvedenie Autora 4.0 Medzinárodný</skos:prefLabel>
      <skos:prefLabel xml:lang="sl">Creative Commons Priznanje avtorstva 4.0 Mednarodna</skos:prefLabel>
      <at:authority-code>CC_BY_4_0</at:authority-code>
      <at:op-code>CC_BY_4_0</at:op-code>
      <at:start.use>2013-11-26</at:start.use>
      <atold:op-code>CC_BY_4_0</atold:op-code>
      <dc:identifier>CC_BY_4_0</dc:identifier>
      <skos:altLabel xml:lang="bg">CC BY 4.0</skos:altLabel>
      <skos:altLabel xml:lang="cs">CC BY 4.0</skos:altLabel>
      <skos:altLabel xml:lang="da">CC BY 4.0</skos:altLabel>
      <skos:altLabel xml:lang="de">CC BY 4.0</skos:altLabel>
      <skos:altLabel xml:lang="el">CC BY 4.0</skos:altLabel>
      <skos:altLabel xml:lang="en">CC BY 4.0</skos:altLabel>
      <skos:altLabel xml:lang="es">CC BY 4.0</skos:altLabel>
      <skos:altLabel xml:lang="et">CC BY 4.0</skos:altLabel>
      <skos:altLabel xml:lang="fi">CC BY 4.0</skos:altLabel>
      <skos:altLabel xml:lang="fr">CC BY 4.0</skos:altLabel>
      <skos:altLabel xml:lang="ga">CC BY 4.0</skos:altLabel>
      <skos:altLabel xml:lang="hr">CC BY 4.0</skos:altLabel>
      <skos:altLabel xml:lang="hu">CC BY 4.0</skos:altLabel>
      <skos:altLabel xml:lang="it">CC BY 4.0</skos:altLabel>
      <skos:altLabel xml:lang="lt">CC BY 4.0</skos:altLabel>
      <skos:altLabel xml:lang="lv">CC BY 4.0</skos:altLabel>
      <skos:altLabel xml:lang="mt">CC BY 4.0</skos:altLabel>
      <skos:altLabel xml:lang="nl">CC BY 4.0</skos:altLabel>
      <skos:altLabel xml:lang="pl">CC BY 4.0</skos:altLabel>
      <skos:altLabel xml:lang="pt">CC BY 4.0</skos:altLabel>
      <skos:altLabel xml:lang="ro">CC BY 4.0</skos:altLabel>
      <skos:altLabel xml:lang="sk">CC BY 4.0</skos:altLabel>
      <skos:altLabel xml:lang="sl">CC BY 4.0</skos:altLabel>
      <skos:altLabel xml:lang="sv">CC BY 4.0</skos:altLabel>
      <skos:definition xml:lang="da">Denne licens tillader andre at videredistribuere, omarbejde, tilpasse og bygge videre på materialet, også kommercielt, så længe de krediterer skaberen af det oprindelige materiale. Dette er den mindst restriktive licens, creative commons udbyder. Anbefalet hvis man ønsker mest mulig videreformidling og brug af det licenserede materiale.</skos:definition>
      <skos:definition xml:lang="en">CC BY 4.0 lets others distribute, remix, tweak, and build upon the author’s work, even commercially, as long as they credit the author for the original creation. This is the most accommodating of licences offered. Recommended for maximum dissemination and use of licenced materials.</skos:definition>
      <skos:definition xml:lang="fr">CC BY 4.0 permet aux autres de distribuer, remixer, arranger, et adapter l’œuvre de l’auteur/autrice, même à des fins commerciales, tant qu’on accorde le mérite de la création originale à l’auteur/autrice en citant son nom. C’est le contrat le plus souple proposé. Recommandé pour la diffusion et l’utilisation maximales d’œuvres licenciées sous CC.</skos:definition>
      <skos:exactMatch rdf:resource="http://creativecommons.org/licenses/by/4.0/"/>
      <skos:inScheme rdf:resource="http://publications.europa.eu/resource/authority/licence"/>
      <skos:topConceptOf rdf:resource="http://publications.europa.eu/resource/authority/licence"/>
   </skos:Concept>
   <skos:Concept rdf:about="http://publications.europa.eu/resource/authority/licence/CC_PDM_1_0"
                 at:deprecated="false">
      <skos:prefLabel xml:lang="bg">Public Domain Mark 1.0</skos:prefLabel>
      <skos:prefLabel xml:lang="cs">Označení volného díla 1.0</skos:prefLabel>
      <skos:prefLabel xml:lang="da">Public domain-mærke 1.0</skos:prefLabel>
      <skos:prefLabel xml:lang="de">Public Domain Mark 1.0</skos:prefLabel>
      <skos:prefLabel xml:lang="el">Σήμα Δημόσιου Τομέα 1.0</skos:prefLabel>
      <skos:prefLabel xml:lang="en">Public Domain Mark 1.0</skos:prefLabel>
      <skos:prefLabel xml:lang="es">Etiqueta de Dominio Público 1.0</skos:prefLabel>
      <skos:prefLabel xml:lang="et">Avaliku omandi märge 1.0</skos:prefLabel>
      <skos:prefLabel xml:lang="fi">Public Domain -merkintä 1.0</skos:prefLabel>
      <skos:prefLabel xml:lang="fr">Marque du Domaine Public 1.0</skos:prefLabel>
      <skos:prefLabel xml:lang="hr">Oznaka javnog dobra 1.0</skos:prefLabel>
      <skos:prefLabel xml:lang="hu">Közkincs megjelölés 1.0</skos:prefLabel>
      <skos:prefLabel xml:lang="it">Marchio di pubblico dominio 1.0</skos:prefLabel>
      <skos:prefLabel xml:lang="lt">Viešosios srities žymuo 1.0</skos:prefLabel>
      <skos:prefLabel xml:lang="lv">Sabiedrības īpašuma iezīme 1.0</skos:prefLabel>
      <skos:prefLabel xml:lang="mt">Public Domain Mark 1.0</skos:prefLabel>
      <skos:prefLabel xml:lang="nl">Public Domain Mark 1.0</skos:prefLabel>
      <skos:prefLabel xml:lang="pl">Znak domeny publicznej 1.0</skos:prefLabel>
      <skos:prefLabel xml:lang="pt">Marca de Domínio Público 1.0</skos:prefLabel>
      <skos:prefLabel xml:lang="ro">Marca Domeniului Public 1.0</skos:prefLabel>
      <skos:prefLabel xml:lang="sk">Public Domain Mark 1.0</skos:prefLabel>
      <skos:prefLabel xml:lang="sl">Oznaka javne domene 1.0</skos:prefLabel>
      <skos:prefLabel xml:lang="sv">Public domain-märke 1.0</skos:prefLabel>
      <at:authority-code>CC_PDM_1_0</at:authority-code>
      <at:op-code>CC_PDM_1_0</at:op-code>
      <at:start.use>2010-10-01</at:start.use>
      <atold:op-code>CC_PDM_1_0</atold:op-code>
      <dc:identifier>CC_PDM_1_0</dc:identifier>
      <skos:altLabel xml:lang="bg">CC PDM 1.0</skos:altLabel>
      <skos:altLabel xml:lang="cs">CC PDM 1.0</skos:altLabel>
      <skos:altLabel xml:lang="da">CC PDM 1.0</skos:altLabel>
      <skos:altLabel xml:lang="de">CC PDM 1.0</skos:altLabel>
      <skos:altLabel xml:lang="el">CC PDM 1.0</skos:altLabel>
      <skos:altLabel xml:lang="en">CC PDM 1.0</skos:altLabel>
      <skos:altLabel xml:lang="es">CC PDM 1.0</skos:altLabel>
      <skos:altLabel xml:lang="et">CC PDM 1.0</skos:altLabel>
      <skos:altLabel xml:lang="fi">CC PDM 1.0</skos:altLabel>
      <skos:altLabel xml:lang="fr">CC PDM 1.0</skos:altLabel>
      <skos:altLabel xml:lang="ga">CC PDM 1.0</skos:altLabel>
      <skos:altLabel xml:lang="hr">CC PDM 1.0</skos:altLabel>
      <skos:altLabel xml:lang="hu">CC PDM 1.0</skos:altLabel>
      <skos:altLabel xml:lang="it">CC PDM 1.0</skos:altLabel>
      <skos:altLabel xml:lang="lt">CC PDM 1.0</skos:altLabel>
      <skos:altLabel xml:lang="lv">CC PDM 1.0</skos:altLabel>
      <skos:altLabel xml:lang="mt">CC PDM 1.0</skos:altLabel>
      <skos:altLabel xml:lang="nl">CC PDM 1.0</skos:altLabel>
      <skos:altLabel xml:lang="pl">CC PDM 1.0</skos:altLabel>
      <skos:altLabel xml:lang="pt">CC PDM 1.0</skos:altLabel>
      <skos:altLabel xml:lang="ro">CC PDM 1.0</skos:altLabel>
      <skos:altLabel xml:lang="sk">CC PDM 1.0</skos:altLabel>
      <skos:altLabel xml:lang="sl">CC PDM 1.0</skos:altLabel>
      <skos:altLabel xml:lang="sv">CC PDM 1.0</skos:altLabel>
      <skos:changeNote xml:lang="en">The source of the start-use date: https://wiki.openmod-initiative.org/images/6/63/Jens-opendata_govdata.de_FraunhoferFokus.pdf</skos:changeNote>
      <skos:definition xml:lang="en">Published by Creative Commons, Public Domain Mark (CC PDM 1.0) identifies a work as being free of known restrictions under copyright law, including all related and neighboring rights. The user can copy, modify, distribute and perform the work, even for commercial purposes, all without asking permission.</skos:definition>
      <skos:exactMatch rdf:resource="http://creativecommons.org/publicdomain/mark/1.0/"/>
      <skos:inScheme rdf:resource="http://publications.europa.eu/resource/authority/licence"/>
      <skos:topConceptOf rdf:resource="http://publications.europa.eu/resource/authority/licence"/>
   </skos:Concept>
   <skos:Concept rdf:about="http://publications.europa.eu/resource/authority/licence/CDDL_1_0"
                 at:deprecated="false">
      <skos:prefLabel xml:lang="en">Common Development and Distribution License 1.0</skos:prefLabel>
      <at:authority-code>CDDL_1_0</at:authority-code>
      <at:op-code>CDDL_1_0</at:op-code>
      <at:start.use>2004-01-24</at:start.use>
      <atold:op-code>CDDL_1_0</atold:op-code>
      <dc:identifier>CDDL_1_0</dc:identifier>
      <skos:altLabel xml:lang="bg">CDDL-1.0</skos:altLabel>
      <skos:altLabel xml:lang="cs">CDDL-1.0</skos:altLabel>
      <skos:altLabel xml:lang="da">CDDL-1.0</skos:altLabel>
      <skos:altLabel xml:lang="de">CDDL-1.0</skos:altLabel>
      <skos:altLabel xml:lang="el">CDDL-1.0</skos:altLabel>
      <skos:altLabel xml:lang="en">CDDL-1.0</skos:altLabel>
      <skos:altLabel xml:lang="es">CDDL-1.0</skos:altLabel>
      <skos:altLabel xml:lang="et">CDDL-1.0</skos:altLabel>
      <skos:altLabel xml:lang="fi">CDDL-1.0</skos:altLabel>
      <skos:altLabel xml:lang="fr">CDDL-1.0</skos:altLabel>
      <skos:altLabel xml:lang="ga">CDDL-1.0</skos:altLabel>
      <skos:altLabel xml:lang="hr">CDDL-1.0</skos:altLabel>
      <skos:altLabel xml:lang="hu">CDDL-1.0</skos:altLabel>
      <skos:altLabel xml:lang="it">CDDL-1.0</skos:altLabel>
      <skos:altLabel xml:lang="lt">CDDL-1.0</skos:altLabel>
      <skos:altLabel xml:lang="lv">CDDL-1.0</skos:altLabel>
      <skos:altLabel xml:lang="mt">CDDL-1.0</skos:altLabel>
      <skos:altLabel xml:lang="nl">CDDL-1.0</skos:altLabel>
      <skos:altLabel xml:lang="pl">CDDL-1.0</skos:altLabel>
      <skos:altLabel xml:lang="pt">CDDL-1.0</skos:altLabel>
      <skos:altLabel xml:lang="ro">CDDL-1.0</skos:altLabel>
      <skos:altLabel xml:lang="sk">CDDL-1.0</skos:altLabel>
      <skos:altLabel xml:lang="sl">CDDL-1.0</skos:altLabel>
      <skos:altLabel xml:lang="sv">CDDL-1.0</skos:altLabel>
      <skos:changeNote xml:lang="en">The source of the start-use date: https://spdx.org/licenses/CDDL-1.0.html</skos:changeNote>
      <skos:definition xml:lang="en">CDDL-1.0 is a free software licence approved by the Open Source Initiative. A moderated (or weak) copyleft licence used by SUN, including explicit patent grants, it is similar to MPL and EPL. Compiled object code can be distributed under any licence, but the original source code (and modified derivatives) must be made available, under the CDDL.</skos:definition>
      <skos:exactMatch rdf:resource="https://opensource.org/licenses/CDDL-1.0"/>
      <skos:inScheme rdf:resource="http://publications.europa.eu/resource/authority/licence"/>
      <skos:topConceptOf rdf:resource="http://publications.europa.eu/resource/authority/licence"/>
   </skos:Concept>
   <skos:Concept rdf:about="http://publications.europa.eu/resource/authority/licence/CECILL_2_1"
                 at:deprecated="false">
      <skos:prefLabel xml:lang="en">CEA CNRS Inria Free Software License Agreement, v2.1 (CECILL-2.1)</skos:prefLabel>
      <skos:prefLabel xml:lang="fr">CEA CNRS Inria Logiciel Libre License, version 2.1 (CECILL-2.1)</skos:prefLabel>
      <at:authority-code>CECILL_2_1</at:authority-code>
      <at:op-code>CECILL_2_1</at:op-code>
      <at:start.use>2013-06-21</at:start.use>
      <atold:op-code>CECILL_2_1</atold:op-code>
      <dc:identifier>CECILL_2_1</dc:identifier>
      <skos:altLabel xml:lang="bg">CECILL-2.1</skos:altLabel>
      <skos:altLabel xml:lang="cs">CECILL-2.1</skos:altLabel>
      <skos:altLabel xml:lang="da">CECILL-2.1</skos:altLabel>
      <skos:altLabel xml:lang="de">CECILL-2.1</skos:altLabel>
      <skos:altLabel xml:lang="el">CECILL-2.1</skos:altLabel>
      <skos:altLabel xml:lang="en">CECILL-2.1</skos:altLabel>
      <skos:altLabel xml:lang="es">CECILL-2.1</skos:altLabel>
      <skos:altLabel xml:lang="et">CECILL-2.1</skos:altLabel>
      <skos:altLabel xml:lang="fi">CECILL-2.1</skos:altLabel>
      <skos:altLabel xml:lang="fr">CECILL-2.1</skos:altLabel>
      <skos:altLabel xml:lang="ga">CECILL-2.1</skos:altLabel>
      <skos:altLabel xml:lang="hr">CECILL-2.1</skos:altLabel>
      <skos:altLabel xml:lang="hu">CECILL-2.1</skos:altLabel>
      <skos:altLabel xml:lang="it">CECILL-2.1</skos:altLabel>
      <skos:altLabel xml:lang="lt">CECILL-2.1</skos:altLabel>
      <skos:altLabel xml:lang="lv">CECILL-2.1</skos:altLabel>
      <skos:altLabel xml:lang="mt">CECILL-2.1</skos:altLabel>
      <skos:altLabel xml:lang="nl">CECILL-2.1</skos:altLabel>
      <skos:altLabel xml:lang="pl">CECILL-2.1</skos:altLabel>
      <skos:altLabel xml:lang="pt">CECILL-2.1</skos:altLabel>
      <skos:altLabel xml:lang="ro">CECILL-2.1</skos:altLabel>
      <skos:altLabel xml:lang="sk">CECILL-2.1</skos:altLabel>
      <skos:altLabel xml:lang="sl">CECILL-2.1</skos:altLabel>
      <skos:altLabel xml:lang="sv">CECILL-2.1</skos:altLabel>
      <skos:changeNote xml:lang="en">The source of the start-use date: https://en.wikipedia.org/wiki/CeCILL</skos:changeNote>
      <skos:definition xml:lang="en">CECILL-2.1 is a moderate copyleft licence initiated in France by CEA, CNRS and Inria and approved by the Open Source Initiative. It has a working value in English/French. It is widely compatible, since only the specific files source code must stay covered, and not the other files or components of a solution. It is therefore designed for components or libraries. Governed by French law.</skos:definition>
      <skos:exactMatch rdf:resource="https://opensource.org/licenses/CECILL-2.1"/>
      <skos:inScheme rdf:resource="http://publications.europa.eu/resource/authority/licence"/>
      <skos:topConceptOf rdf:resource="http://publications.europa.eu/resource/authority/licence"/>
   </skos:Concept>
   <skos:Concept rdf:about="http://publications.europa.eu/resource/authority/licence/CLARIN_ACA_1_0"
                 at:deprecated="false">
      <skos:prefLabel xml:lang="en">Clarin Academic End-User Licence (ACA) 1.0</skos:prefLabel>
      <skos:prefLabel xml:lang="et">Clarin akadeemiline lõppkasutaja litsents (ACA) 1.0</skos:prefLabel>
      <at:authority-code>CLARIN_ACA_1_0</at:authority-code>
      <at:op-code>CLARIN_ACA_1_0</at:op-code>
      <at:start.use>2014-12-12</at:start.use>
      <atold:op-code>CLARIN_ACA_1_0</atold:op-code>
      <dc:identifier>CLARIN_ACA_1_0</dc:identifier>
      <skos:altLabel xml:lang="bg">CLARIN-EULA-ACA-v1.0</skos:altLabel>
      <skos:altLabel xml:lang="cs">CLARIN-EULA-ACA-v1.0</skos:altLabel>
      <skos:altLabel xml:lang="da">CLARIN-EULA-ACA-v1.0</skos:altLabel>
      <skos:altLabel xml:lang="de">CLARIN-EULA-ACA-v1.0</skos:altLabel>
      <skos:altLabel xml:lang="el">CLARIN-EULA-ACA-v1.0</skos:altLabel>
      <skos:altLabel xml:lang="en">CLARIN-EULA-ACA-v1.0</skos:altLabel>
      <skos:altLabel xml:lang="es">CLARIN-EULA-ACA-v1.0</skos:altLabel>
      <skos:altLabel xml:lang="et">CLARIN-EULA-ACA-v1.0</skos:altLabel>
      <skos:altLabel xml:lang="fi">CLARIN-EULA-ACA-v1.0</skos:altLabel>
      <skos:altLabel xml:lang="fr">CLARIN-EULA-ACA-v1.0</skos:altLabel>
      <skos:altLabel xml:lang="ga">CLARIN-EULA-ACA-v1.0</skos:altLabel>
      <skos:altLabel xml:lang="hr">CLARIN-EULA-ACA-v1.0</skos:altLabel>
      <skos:altLabel xml:lang="hu">CLARIN-EULA-ACA-v1.0</skos:altLabel>
      <skos:altLabel xml:lang="it">CLARIN-EULA-ACA-v1.0</skos:altLabel>
      <skos:altLabel xml:lang="lt">CLARIN-EULA-ACA-v1.0</skos:altLabel>
      <skos:altLabel xml:lang="lv">CLARIN-EULA-ACA-v1.0</skos:altLabel>
      <skos:altLabel xml:lang="mt">CLARIN-EULA-ACA-v1.0</skos:altLabel>
      <skos:altLabel xml:lang="nl">CLARIN-EULA-ACA-v1.0</skos:altLabel>
      <skos:altLabel xml:lang="pl">CLARIN-EULA-ACA-v1.0</skos:altLabel>
      <skos:altLabel xml:lang="pt">CLARIN-EULA-ACA-v1.0</skos:altLabel>
      <skos:altLabel xml:lang="ro">CLARIN-EULA-ACA-v1.0</skos:altLabel>
      <skos:altLabel xml:lang="sk">CLARIN-EULA-ACA-v1.0</skos:altLabel>
      <skos:altLabel xml:lang="sl">CLARIN-EULA-ACA-v1.0</skos:altLabel>
      <skos:altLabel xml:lang="sv">CLARIN-EULA-ACA-v1.0</skos:altLabel>
      <skos:definition xml:lang="en">The copyright holder grants the end-user a free, non-exclusive and perpetual (for the duration of the copyright) right to use and make copies of the resource for educational, teaching or research purposes as such, as modified, or as part of a compilation or derived work.</skos:definition>
      <skos:exactMatch rdf:resource="https://www.clarin.eu/content/licenses-and-clarin-categories"/>
      <skos:inScheme rdf:resource="http://publications.europa.eu/resource/authority/licence"/>
      <skos:topConceptOf rdf:resource="http://publications.europa.eu/resource/authority/licence"/>
   </skos:Concept>
   <skos:Concept rdf:about="http://publications.europa.eu/resource/authority/licence/CNRI_PYTHON"
                 at:deprecated="false">
      <skos:prefLabel xml:lang="en">The CNRI portion of the multi-part Python License (CNRI-Python)</skos:prefLabel>
      <at:authority-code>CNRI_PYTHON</at:authority-code>
      <at:op-code>CNRI_PYTHON</at:op-code>
      <at:start.use>2001-03-06</at:start.use>
      <atold:op-code>CNRI_PYTHON</atold:op-code>
      <dc:identifier>CNRI_PYTHON</dc:identifier>
      <skos:altLabel xml:lang="bg">CNRI-Python</skos:altLabel>
      <skos:altLabel xml:lang="cs">CNRI-Python</skos:altLabel>
      <skos:altLabel xml:lang="da">CNRI-Python</skos:altLabel>
      <skos:altLabel xml:lang="de">CNRI-Python</skos:altLabel>
      <skos:altLabel xml:lang="el">CNRI-Python</skos:altLabel>
      <skos:altLabel xml:lang="en">CNRI-Python</skos:altLabel>
      <skos:altLabel xml:lang="es">CNRI-Python</skos:altLabel>
      <skos:altLabel xml:lang="et">CNRI-Python</skos:altLabel>
      <skos:altLabel xml:lang="fi">CNRI-Python</skos:altLabel>
      <skos:altLabel xml:lang="fr">CNRI-Python</skos:altLabel>
      <skos:altLabel xml:lang="ga">CNRI-Python</skos:altLabel>
      <skos:altLabel xml:lang="hr">CNRI-Python</skos:altLabel>
      <skos:altLabel xml:lang="hu">CNRI-Python</skos:altLabel>
      <skos:altLabel xml:lang="it">CNRI-Python</skos:altLabel>
      <skos:altLabel xml:lang="lt">CNRI-Python</skos:altLabel>
      <skos:altLabel xml:lang="lv">CNRI-Python</skos:altLabel>
      <skos:altLabel xml:lang="mt">CNRI-Python</skos:altLabel>
      <skos:altLabel xml:lang="nl">CNRI-Python</skos:altLabel>
      <skos:altLabel xml:lang="pl">CNRI-Python</skos:altLabel>
      <skos:altLabel xml:lang="pt">CNRI-Python</skos:altLabel>
      <skos:altLabel xml:lang="ro">CNRI-Python</skos:altLabel>
      <skos:altLabel xml:lang="sk">CNRI-Python</skos:altLabel>
      <skos:altLabel xml:lang="sl">CNRI-Python</skos:altLabel>
      <skos:altLabel xml:lang="sv">CNRI-Python</skos:altLabel>
      <skos:changeNote xml:lang="en">The source of the start-use date: https://en.wikipedia.org/wiki/Python_Software_Foundation</skos:changeNote>
      <skos:definition xml:lang="en">CNRI-Python is a permissive free software licence approved by the Open Source Initiative.</skos:definition>
      <skos:exactMatch rdf:resource="https://opensource.org/licenses/CNRI-Python"/>
      <skos:inScheme rdf:resource="http://publications.europa.eu/resource/authority/licence"/>
      <skos:topConceptOf rdf:resource="http://publications.europa.eu/resource/authority/licence"/>
   </skos:Concept>
   <skos:Concept rdf:about="http://publications.europa.eu/resource/authority/licence/COM_REUSE"
                 at:deprecated="false">
      <skos:prefLabel xml:lang="en">European Commission reuse notice</skos:prefLabel>
      <at:authority-code>COM_REUSE</at:authority-code>
      <at:op-code>COM_REUSE</at:op-code>
      <at:start.use>2011-12-14</at:start.use>
      <atold:op-code>COM_REUSE</atold:op-code>
      <dc:identifier>COM_REUSE</dc:identifier>
      <skos:definition xml:lang="en">According to the European Commission reuse notice, reuse is authorised, provided the source is acknowledged. The reuse policy of the European Commission is implemented by the Decision of 12 December 2011. The general principle of reuse can be subject to conditions which may be specified in individual copyright notices. Therefore users are advised to refer to the copyright notices of the individual websites maintained under Europa and of the individual documents. Reuse is not applicable to documents subject to intellectual property rights of third parties.</skos:definition>
      <skos:exactMatch rdf:resource="http://data.europa.eu/eli/dec/2011/833/oj"/>
      <skos:inScheme rdf:resource="http://publications.europa.eu/resource/authority/licence"/>
      <skos:topConceptOf rdf:resource="http://publications.europa.eu/resource/authority/licence"/>
   </skos:Concept>
   <skos:Concept rdf:about="http://publications.europa.eu/resource/authority/licence/CPAL_1_0"
                 at:deprecated="false">
      <skos:prefLabel xml:lang="en">Common Public Attribution License Version 1.0 (CPAL-1.0)</skos:prefLabel>
      <at:authority-code>CPAL_1_0</at:authority-code>
      <at:op-code>CPAL_1_0</at:op-code>
      <at:start.use>2007-07-26</at:start.use>
      <atold:op-code>CPAL_1_0</atold:op-code>
      <dc:identifier>CPAL_1_0</dc:identifier>
      <skos:altLabel xml:lang="bg">CPAL-1.0</skos:altLabel>
      <skos:altLabel xml:lang="cs">CPAL-1.0</skos:altLabel>
      <skos:altLabel xml:lang="da">CPAL-1.0</skos:altLabel>
      <skos:altLabel xml:lang="de">CPAL-1.0</skos:altLabel>
      <skos:altLabel xml:lang="el">CPAL-1.0</skos:altLabel>
      <skos:altLabel xml:lang="en">CPAL-1.0</skos:altLabel>
      <skos:altLabel xml:lang="es">CPAL-1.0</skos:altLabel>
      <skos:altLabel xml:lang="et">CPAL-1.0</skos:altLabel>
      <skos:altLabel xml:lang="fi">CPAL-1.0</skos:altLabel>
      <skos:altLabel xml:lang="fr">CPAL-1.0</skos:altLabel>
      <skos:altLabel xml:lang="ga">CPAL-1.0</skos:altLabel>
      <skos:altLabel xml:lang="hr">CPAL-1.0</skos:altLabel>
      <skos:altLabel xml:lang="hu">CPAL-1.0</skos:altLabel>
      <skos:altLabel xml:lang="it">CPAL-1.0</skos:altLabel>
      <skos:altLabel xml:lang="lt">CPAL-1.0</skos:altLabel>
      <skos:altLabel xml:lang="lv">CPAL-1.0</skos:altLabel>
      <skos:altLabel xml:lang="mt">CPAL-1.0</skos:altLabel>
      <skos:altLabel xml:lang="nl">CPAL-1.0</skos:altLabel>
      <skos:altLabel xml:lang="pl">CPAL-1.0</skos:altLabel>
      <skos:altLabel xml:lang="pt">CPAL-1.0</skos:altLabel>
      <skos:altLabel xml:lang="ro">CPAL-1.0</skos:altLabel>
      <skos:altLabel xml:lang="sk">CPAL-1.0</skos:altLabel>
      <skos:altLabel xml:lang="sl">CPAL-1.0</skos:altLabel>
      <skos:altLabel xml:lang="sv">CPAL-1.0</skos:altLabel>
      <skos:changeNote xml:lang="en">The source of the start-use date: https://en.wikipedia.org/wiki/Common_Public_Attribution_License; https://www.socialtext.net/open/cpal</skos:changeNote>
      <skos:definition xml:lang="en">CPAL-1.0 is a copyleft-style, free software licence approved by the Open Source Initiative. Under this licence, it is possible to create a larger work by combining the program with other software code not governed by the terms of this licence, and distribute the larger work as a single product.</skos:definition>
      <skos:exactMatch rdf:resource="https://opensource.org/licenses/CPAL-1.0"/>
      <skos:inScheme rdf:resource="http://publications.europa.eu/resource/authority/licence"/>
      <skos:topConceptOf rdf:resource="http://publications.europa.eu/resource/authority/licence"/>
   </skos:Concept>
   <skos:Concept rdf:about="http://publications.europa.eu/resource/authority/licence/CPL_1_0"
                 at:deprecated="true">
      <skos:prefLabel xml:lang="en">Common Public License, version 1.0 (CPL-1.0)</skos:prefLabel>
      <at:authority-code>CPL_1_0</at:authority-code>
      <at:op-code>CPL_1_0</at:op-code>
      <at:start.use>2001-05-01</at:start.use>
      <atold:op-code>CPL_1_0</atold:op-code>
      <dc:identifier>CPL_1_0</dc:identifier>
      <skos:altLabel xml:lang="bg">CPL-1.0</skos:altLabel>
      <skos:altLabel xml:lang="cs">CPL-1.0</skos:altLabel>
      <skos:altLabel xml:lang="da">CPL-1.0</skos:altLabel>
      <skos:altLabel xml:lang="de">CPL-1.0</skos:altLabel>
      <skos:altLabel xml:lang="el">CPL-1.0</skos:altLabel>
      <skos:altLabel xml:lang="en">CPL-1.0</skos:altLabel>
      <skos:altLabel xml:lang="es">CPL-1.0</skos:altLabel>
      <skos:altLabel xml:lang="et">CPL-1.0</skos:altLabel>
      <skos:altLabel xml:lang="fi">CPL-1.0</skos:altLabel>
      <skos:altLabel xml:lang="fr">CPL-1.0</skos:altLabel>
      <skos:altLabel xml:lang="ga">CPL-1.0</skos:altLabel>
      <skos:altLabel xml:lang="hr">CPL-1.0</skos:altLabel>
      <skos:altLabel xml:lang="hu">CPL-1.0</skos:altLabel>
      <skos:altLabel xml:lang="it">CPL-1.0</skos:altLabel>
      <skos:altLabel xml:lang="lt">CPL-1.0</skos:altLabel>
      <skos:altLabel xml:lang="lv">CPL-1.0</skos:altLabel>
      <skos:altLabel xml:lang="mt">CPL-1.0</skos:altLabel>
      <skos:altLabel xml:lang="nl">CPL-1.0</skos:altLabel>
      <skos:altLabel xml:lang="pl">CPL-1.0</skos:altLabel>
      <skos:altLabel xml:lang="pt">CPL-1.0</skos:altLabel>
      <skos:altLabel xml:lang="ro">CPL-1.0</skos:altLabel>
      <skos:altLabel xml:lang="sk">CPL-1.0</skos:altLabel>
      <skos:altLabel xml:lang="sl">CPL-1.0</skos:altLabel>
      <skos:altLabel xml:lang="sv">CPL-1.0</skos:altLabel>
      <skos:changeNote xml:lang="en">The source of the start-use date: https://en.wikipedia.org/wiki/Common_Public_License</skos:changeNote>
      <skos:definition xml:lang="en">CPL-1.0 is a copyleft-style, free software licence approved by the Open Source Initiative. It is superseded by EPL-1.0.</skos:definition>
      <skos:exactMatch rdf:resource="https://opensource.org/licenses/CPL-1.0"/>
      <skos:inScheme rdf:resource="http://publications.europa.eu/resource/authority/licence"/>
      <skos:topConceptOf rdf:resource="http://publications.europa.eu/resource/authority/licence"/>
      <at:end.use>2005-06-27</at:end.use>
   </skos:Concept>
   <skos:Concept rdf:about="http://publications.europa.eu/resource/authority/licence/DLDE_BYNC_1_0"
                 at:deprecated="false">
      <skos:prefLabel xml:lang="de">Datenlizenz Deutschland – Namensnennung – Version 1.0</skos:prefLabel>
      <skos:prefLabel xml:lang="en">Data licence Germany – attribution – non-commercial – Version 1.0</skos:prefLabel>
      <at:authority-code>DLDE_BYNC_1_0</at:authority-code>
      <at:op-code>DLDE_BYNC_1_0</at:op-code>
      <at:start.use>2012-01-01</at:start.use>
      <atold:op-code>DLDE_BYNC_1_0</atold:op-code>
      <dc:identifier>DLDE_BYNC_1_0</dc:identifier>
      <skos:altLabel xml:lang="bg">DL-DE BY-NC 1.0</skos:altLabel>
      <skos:altLabel xml:lang="cs">DL-DE BY-NC 1.0</skos:altLabel>
      <skos:altLabel xml:lang="da">DL-DE BY-NC 1.0</skos:altLabel>
      <skos:altLabel xml:lang="de">DL-DE BY-NC 1.0</skos:altLabel>
      <skos:altLabel xml:lang="el">DL-DE BY-NC 1.0</skos:altLabel>
      <skos:altLabel xml:lang="en">DL-DE BY-NC 1.0</skos:altLabel>
      <skos:altLabel xml:lang="es">DL-DE BY-NC 1.0</skos:altLabel>
      <skos:altLabel xml:lang="et">DL-DE BY-NC 1.0</skos:altLabel>
      <skos:altLabel xml:lang="fi">DL-DE BY-NC 1.0</skos:altLabel>
      <skos:altLabel xml:lang="fr">DL-DE BY-NC 1.0</skos:altLabel>
      <skos:altLabel xml:lang="ga">DL-DE BY-NC 1.0</skos:altLabel>
      <skos:altLabel xml:lang="hr">DL-DE BY-NC 1.0</skos:altLabel>
      <skos:altLabel xml:lang="hu">DL-DE BY-NC 1.0</skos:altLabel>
      <skos:altLabel xml:lang="it">DL-DE BY-NC 1.0</skos:altLabel>
      <skos:altLabel xml:lang="lt">DL-DE BY-NC 1.0</skos:altLabel>
      <skos:altLabel xml:lang="lv">DL-DE BY-NC 1.0</skos:altLabel>
      <skos:altLabel xml:lang="mt">DL-DE BY-NC 1.0</skos:altLabel>
      <skos:altLabel xml:lang="nl">DL-DE BY-NC 1.0</skos:altLabel>
      <skos:altLabel xml:lang="pl">DL-DE BY-NC 1.0</skos:altLabel>
      <skos:altLabel xml:lang="pt">DL-DE BY-NC 1.0</skos:altLabel>
      <skos:altLabel xml:lang="ro">DL-DE BY-NC 1.0</skos:altLabel>
      <skos:altLabel xml:lang="sk">DL-DE BY-NC 1.0</skos:altLabel>
      <skos:altLabel xml:lang="sl">DL-DE BY-NC 1.0</skos:altLabel>
      <skos:altLabel xml:lang="sv">DL-DE BY-NC 1.0</skos:altLabel>
      <skos:changeNote xml:lang="en">The source of the start-use date: https://wiki.openmod-initiative.org/images/6/63/Jens-opendata_govdata.de_FraunhoferFokus.pdf</skos:changeNote>
      <skos:definition xml:lang="en">Published by Germany, DL-DE BY-NC 1.0 is a data licence permitting any non-commercial use, as long as credit is given to the author for the original creation. Changes must be marked as such in the source note. The provider mus make available the data, contents and services with the diligence necessary for the discharge of its public tasks.</skos:definition>
      <skos:exactMatch rdf:resource="https://www.govdata.de/dl-de/by-nc-1-0"/>
      <skos:inScheme rdf:resource="http://publications.europa.eu/resource/authority/licence"/>
      <skos:topConceptOf rdf:resource="http://publications.europa.eu/resource/authority/licence"/>
   </skos:Concept>
   <skos:Concept rdf:about="http://publications.europa.eu/resource/authority/licence/DLDE_BY_1_0"
                 at:deprecated="false">
      <skos:prefLabel xml:lang="de">Datenlizenz Deutschland – Namensnennung – Version 1.0</skos:prefLabel>
      <skos:prefLabel xml:lang="en">Data licence Germany – attribution – Version 1.0</skos:prefLabel>
      <at:authority-code>DLDE_BY_1_0</at:authority-code>
      <at:op-code>DLDE_BY_1_0</at:op-code>
      <at:start.use>2013-01-31</at:start.use>
      <atold:op-code>DLDE_BY_1_0</atold:op-code>
      <dc:identifier>DLDE_BY_1_0</dc:identifier>
      <skos:altLabel xml:lang="bg">DL-DE BY 1.0</skos:altLabel>
      <skos:altLabel xml:lang="cs">DL-DE BY 1.0</skos:altLabel>
      <skos:altLabel xml:lang="da">DL-DE BY 1.0</skos:altLabel>
      <skos:altLabel xml:lang="de">DL-DE BY 1.0</skos:altLabel>
      <skos:altLabel xml:lang="el">DL-DE BY 1.0</skos:altLabel>
      <skos:altLabel xml:lang="en">DL-DE BY 1.0</skos:altLabel>
      <skos:altLabel xml:lang="es">DL-DE BY 1.0</skos:altLabel>
      <skos:altLabel xml:lang="et">DL-DE BY 1.0</skos:altLabel>
      <skos:altLabel xml:lang="fi">DL-DE BY 1.0</skos:altLabel>
      <skos:altLabel xml:lang="fr">DL-DE BY 1.0</skos:altLabel>
      <skos:altLabel xml:lang="ga">DL-DE BY 1.0</skos:altLabel>
      <skos:altLabel xml:lang="hr">DL-DE BY 1.0</skos:altLabel>
      <skos:altLabel xml:lang="hu">DL-DE BY 1.0</skos:altLabel>
      <skos:altLabel xml:lang="it">DL-DE BY 1.0</skos:altLabel>
      <skos:altLabel xml:lang="lt">DL-DE BY 1.0</skos:altLabel>
      <skos:altLabel xml:lang="lv">DL-DE BY 1.0</skos:altLabel>
      <skos:altLabel xml:lang="mt">DL-DE BY 1.0</skos:altLabel>
      <skos:altLabel xml:lang="nl">DL-DE BY 1.0</skos:altLabel>
      <skos:altLabel xml:lang="pl">DL-DE BY 1.0</skos:altLabel>
      <skos:altLabel xml:lang="pt">DL-DE BY 1.0</skos:altLabel>
      <skos:altLabel xml:lang="ro">DL-DE BY 1.0</skos:altLabel>
      <skos:altLabel xml:lang="sk">DL-DE BY 1.0</skos:altLabel>
      <skos:altLabel xml:lang="sl">DL-DE BY 1.0</skos:altLabel>
      <skos:altLabel xml:lang="sv">DL-DE BY 1.0</skos:altLabel>
      <skos:changeNote xml:lang="en">The source of the start-use date: https://wiki.openmod-initiative.org/images/6/63/Jens-opendata_govdata.de_FraunhoferFokus.pdf</skos:changeNote>
      <skos:definition xml:lang="en">Published by Germany, DL-DE BY 1.0 is a data licence permitting any use commercially and non-commercially, as long as credit is given to the author for the original creation. Changes must be marked as such in the source note. The provider mus make available the data, contents and services with the diligence necessary for the discharge of its public tasks.</skos:definition>
      <skos:exactMatch rdf:resource="https://www.govdata.de/dl-de/by-1-0"/>
      <skos:inScheme rdf:resource="http://publications.europa.eu/resource/authority/licence"/>
      <skos:topConceptOf rdf:resource="http://publications.europa.eu/resource/authority/licence"/>
   </skos:Concept>
   <skos:Concept rdf:about="http://publications.europa.eu/resource/authority/licence/DLDE_BY_2_0"
                 at:deprecated="false">
      <skos:prefLabel xml:lang="de">Datenlizenz Deutschland – Namensnennung – Version 2.0</skos:prefLabel>
      <skos:prefLabel xml:lang="en">Data licence Germany – attribution – Version 2.0</skos:prefLabel>
      <at:authority-code>DLDE_BY_2_0</at:authority-code>
      <at:op-code>DLDE_BY_2_0</at:op-code>
      <at:start.use>2014-07-01</at:start.use>
      <atold:op-code>DLDE_BY_2_0</atold:op-code>
      <dc:identifier>DLDE_BY_2_0</dc:identifier>
      <skos:altLabel xml:lang="bg">DL-DE BY 2.0</skos:altLabel>
      <skos:altLabel xml:lang="cs">DL-DE BY 2.0</skos:altLabel>
      <skos:altLabel xml:lang="da">DL-DE BY 2.0</skos:altLabel>
      <skos:altLabel xml:lang="de">DL-DE BY 2.0</skos:altLabel>
      <skos:altLabel xml:lang="el">DL-DE BY 2.0</skos:altLabel>
      <skos:altLabel xml:lang="en">DL-DE BY 2.0</skos:altLabel>
      <skos:altLabel xml:lang="es">DL-DE BY 2.0</skos:altLabel>
      <skos:altLabel xml:lang="et">DL-DE BY 2.0</skos:altLabel>
      <skos:altLabel xml:lang="fi">DL-DE BY 2.0</skos:altLabel>
      <skos:altLabel xml:lang="fr">DL-DE BY 2.0</skos:altLabel>
      <skos:altLabel xml:lang="ga">DL-DE BY 2.0</skos:altLabel>
      <skos:altLabel xml:lang="hr">DL-DE BY 2.0</skos:altLabel>
      <skos:altLabel xml:lang="hu">DL-DE BY 2.0</skos:altLabel>
      <skos:altLabel xml:lang="it">DL-DE BY 2.0</skos:altLabel>
      <skos:altLabel xml:lang="lt">DL-DE BY 2.0</skos:altLabel>
      <skos:altLabel xml:lang="lv">DL-DE BY 2.0</skos:altLabel>
      <skos:altLabel xml:lang="mt">DL-DE BY 2.0</skos:altLabel>
      <skos:altLabel xml:lang="nl">DL-DE BY 2.0</skos:altLabel>
      <skos:altLabel xml:lang="pl">DL-DE BY 2.0</skos:altLabel>
      <skos:altLabel xml:lang="pt">DL-DE BY 2.0</skos:altLabel>
      <skos:altLabel xml:lang="ro">DL-DE BY 2.0</skos:altLabel>
      <skos:altLabel xml:lang="sk">DL-DE BY 2.0</skos:altLabel>
      <skos:altLabel xml:lang="sl">DL-DE BY 2.0</skos:altLabel>
      <skos:altLabel xml:lang="sv">DL-DE BY 2.0</skos:altLabel>
      <skos:changeNote xml:lang="en">The source of the start-use date: https://wiki.openmod-initiative.org/images/6/63/Jens-opendata_govdata.de_FraunhoferFokus.pdf</skos:changeNote>
      <skos:definition xml:lang="en">Published by Germany, DL-DE BY 2.0 is a data licence permitting any use commercially and non-commercially, as long as credit is given to the author for the original creation. Changes must be marked as such in the source note.</skos:definition>
      <skos:exactMatch rdf:resource="https://www.govdata.de/dl-de/by-2-0"/>
      <skos:inScheme rdf:resource="http://publications.europa.eu/resource/authority/licence"/>
      <skos:topConceptOf rdf:resource="http://publications.europa.eu/resource/authority/licence"/>
   </skos:Concept>
   <skos:Concept rdf:about="http://publications.europa.eu/resource/authority/licence/DLDE_ZERO_2_0"
                 at:deprecated="false">
      <skos:prefLabel xml:lang="de">Datenlizenz Deutschland – Zero – Version 2.0</skos:prefLabel>
      <skos:prefLabel xml:lang="en">Data licence Germany – Zero – Version 2.0</skos:prefLabel>
      <at:authority-code>DLDE_ZERO_2_0</at:authority-code>
      <at:op-code>DLDE_ZERO_2_0</at:op-code>
      <at:start.use>2014-07-01</at:start.use>
      <atold:op-code>DLDE_ZERO_2_0</atold:op-code>
      <dc:identifier>DLDE_ZERO_2_0</dc:identifier>
      <skos:altLabel xml:lang="bg">DL-DE ZERO 2.0</skos:altLabel>
      <skos:altLabel xml:lang="cs">DL-DE ZERO 2.0</skos:altLabel>
      <skos:altLabel xml:lang="da">DL-DE ZERO 2.0</skos:altLabel>
      <skos:altLabel xml:lang="de">DL-DE ZERO 2.0</skos:altLabel>
      <skos:altLabel xml:lang="el">DL-DE ZERO 2.0</skos:altLabel>
      <skos:altLabel xml:lang="en">DL-DE ZERO 2.0</skos:altLabel>
      <skos:altLabel xml:lang="es">DL-DE ZERO 2.0</skos:altLabel>
      <skos:altLabel xml:lang="et">DL-DE ZERO 2.0</skos:altLabel>
      <skos:altLabel xml:lang="fi">DL-DE ZERO 2.0</skos:altLabel>
      <skos:altLabel xml:lang="fr">DL-DE ZERO 2.0</skos:altLabel>
      <skos:altLabel xml:lang="ga">DL-DE ZERO 2.0</skos:altLabel>
      <skos:altLabel xml:lang="hr">DL-DE ZERO 2.0</skos:altLabel>
      <skos:altLabel xml:lang="hu">DL-DE ZERO 2.0</skos:altLabel>
      <skos:altLabel xml:lang="it">DL-DE ZERO 2.0</skos:altLabel>
      <skos:altLabel xml:lang="lt">DL-DE ZERO 2.0</skos:altLabel>
      <skos:altLabel xml:lang="lv">DL-DE ZERO 2.0</skos:altLabel>
      <skos:altLabel xml:lang="mt">DL-DE ZERO 2.0</skos:altLabel>
      <skos:altLabel xml:lang="nl">DL-DE ZERO 2.0</skos:altLabel>
      <skos:altLabel xml:lang="pl">DL-DE ZERO 2.0</skos:altLabel>
      <skos:altLabel xml:lang="pt">DL-DE ZERO 2.0</skos:altLabel>
      <skos:altLabel xml:lang="ro">DL-DE ZERO 2.0</skos:altLabel>
      <skos:altLabel xml:lang="sk">DL-DE ZERO 2.0</skos:altLabel>
      <skos:altLabel xml:lang="sl">DL-DE ZERO 2.0</skos:altLabel>
      <skos:altLabel xml:lang="sv">DL-DE ZERO 2.0</skos:altLabel>
      <skos:changeNote xml:lang="en">The source of the start-use date: https://wiki.openmod-initiative.org/images/6/63/Jens-opendata_govdata.de_FraunhoferFokus.pdf</skos:changeNote>
      <skos:definition xml:lang="en">Published by Germany, DL-DE ZERO 2.0 is a data licence permitting any use without restrictions or conditions. The data and meta-data provided may be for commercial and non-commercial use.</skos:definition>
      <skos:exactMatch rdf:resource="https://www.govdata.de/dl-de/by-2-0"/>
      <skos:inScheme rdf:resource="http://publications.europa.eu/resource/authority/licence"/>
      <skos:topConceptOf rdf:resource="http://publications.europa.eu/resource/authority/licence"/>
   </skos:Concept>
   <skos:Concept rdf:about="http://publications.europa.eu/resource/authority/licence/ECL_1_0"
                 at:deprecated="true">
      <skos:prefLabel xml:lang="en">Educational Community License version 1.0 (ECL-1.0)</skos:prefLabel>
      <at:authority-code>ECL_1_0</at:authority-code>
      <at:op-code>ECL_1_0</at:op-code>
      <at:start.use>2005-03-15</at:start.use>
      <atold:op-code>ECL_1_0</atold:op-code>
      <dc:identifier>ECL_1_0</dc:identifier>
      <skos:altLabel xml:lang="bg">ECL-1.0</skos:altLabel>
      <skos:altLabel xml:lang="cs">ECL-1.0</skos:altLabel>
      <skos:altLabel xml:lang="da">ECL-1.0</skos:altLabel>
      <skos:altLabel xml:lang="de">ECL-1.0</skos:altLabel>
      <skos:altLabel xml:lang="el">ECL-1.0</skos:altLabel>
      <skos:altLabel xml:lang="en">ECL-1.0</skos:altLabel>
      <skos:altLabel xml:lang="es">ECL-1.0</skos:altLabel>
      <skos:altLabel xml:lang="et">ECL-1.0</skos:altLabel>
      <skos:altLabel xml:lang="fi">ECL-1.0</skos:altLabel>
      <skos:altLabel xml:lang="fr">ECL-1.0</skos:altLabel>
      <skos:altLabel xml:lang="ga">ECL-1.0</skos:altLabel>
      <skos:altLabel xml:lang="hr">ECL-1.0</skos:altLabel>
      <skos:altLabel xml:lang="hu">ECL-1.0</skos:altLabel>
      <skos:altLabel xml:lang="it">ECL-1.0</skos:altLabel>
      <skos:altLabel xml:lang="lt">ECL-1.0</skos:altLabel>
      <skos:altLabel xml:lang="lv">ECL-1.0</skos:altLabel>
      <skos:altLabel xml:lang="mt">ECL-1.0</skos:altLabel>
      <skos:altLabel xml:lang="nl">ECL-1.0</skos:altLabel>
      <skos:altLabel xml:lang="pl">ECL-1.0</skos:altLabel>
      <skos:altLabel xml:lang="pt">ECL-1.0</skos:altLabel>
      <skos:altLabel xml:lang="ro">ECL-1.0</skos:altLabel>
      <skos:altLabel xml:lang="sk">ECL-1.0</skos:altLabel>
      <skos:altLabel xml:lang="sl">ECL-1.0</skos:altLabel>
      <skos:altLabel xml:lang="sv">ECL-1.0</skos:altLabel>
      <skos:changeNote xml:lang="en">The source of the start-use date: https://en.wikipedia.org/wiki/Sakai_(software</skos:changeNote>
      <skos:definition xml:lang="en">ECL-1.0 is a permissive free software licence approved by the Open Source Initiative. It is similar to the Apache 1.2. It is superseded by ECL-2.0.</skos:definition>
      <skos:exactMatch rdf:resource="https://opensource.org/licenses/ECL-1.0"/>
      <skos:inScheme rdf:resource="http://publications.europa.eu/resource/authority/licence"/>
      <skos:topConceptOf rdf:resource="http://publications.europa.eu/resource/authority/licence"/>
      <at:end.use>2007-04-14</at:end.use>
   </skos:Concept>
   <skos:Concept rdf:about="http://publications.europa.eu/resource/authority/licence/ECL_2_0"
                 at:deprecated="false">
      <skos:prefLabel xml:lang="en">Educational Community License version 2.0 (ECL-2.0)</skos:prefLabel>
      <at:authority-code>ECL_2_0</at:authority-code>
      <at:op-code>ECL_2_0</at:op-code>
      <at:start.use>2007-04-15</at:start.use>
      <atold:op-code>ECL_2_0</atold:op-code>
      <dc:identifier>ECL_2_0</dc:identifier>
      <skos:altLabel xml:lang="bg">ECL-2.0</skos:altLabel>
      <skos:altLabel xml:lang="cs">ECL-2.0</skos:altLabel>
      <skos:altLabel xml:lang="da">ECL-2.0</skos:altLabel>
      <skos:altLabel xml:lang="de">ECL-2.0</skos:altLabel>
      <skos:altLabel xml:lang="el">ECL-2.0</skos:altLabel>
      <skos:altLabel xml:lang="en">ECL-2.0</skos:altLabel>
      <skos:altLabel xml:lang="es">ECL-2.0</skos:altLabel>
      <skos:altLabel xml:lang="et">ECL-2.0</skos:altLabel>
      <skos:altLabel xml:lang="fi">ECL-2.0</skos:altLabel>
      <skos:altLabel xml:lang="fr">ECL-2.0</skos:altLabel>
      <skos:altLabel xml:lang="ga">ECL-2.0</skos:altLabel>
      <skos:altLabel xml:lang="hr">ECL-2.0</skos:altLabel>
      <skos:altLabel xml:lang="hu">ECL-2.0</skos:altLabel>
      <skos:altLabel xml:lang="it">ECL-2.0</skos:altLabel>
      <skos:altLabel xml:lang="lt">ECL-2.0</skos:altLabel>
      <skos:altLabel xml:lang="lv">ECL-2.0</skos:altLabel>
      <skos:altLabel xml:lang="mt">ECL-2.0</skos:altLabel>
      <skos:altLabel xml:lang="nl">ECL-2.0</skos:altLabel>
      <skos:altLabel xml:lang="pl">ECL-2.0</skos:altLabel>
      <skos:altLabel xml:lang="pt">ECL-2.0</skos:altLabel>
      <skos:altLabel xml:lang="ro">ECL-2.0</skos:altLabel>
      <skos:altLabel xml:lang="sk">ECL-2.0</skos:altLabel>
      <skos:altLabel xml:lang="sl">ECL-2.0</skos:altLabel>
      <skos:altLabel xml:lang="sv">ECL-2.0</skos:altLabel>
      <skos:changeNote xml:lang="en">The source of the start-use date: https://tldrlegal.com/license/educational-community-license,-version-2.0-(ecl-2.0)#fulltext</skos:changeNote>
      <skos:definition xml:lang="en">ECL-2.0 is a permissive free software licence approved by the Open Source Initiative. It is similar to the Apache 1.2. Nothing in the licence prohibits re-licencing of a larger work under the EUPL.</skos:definition>
      <skos:exactMatch rdf:resource="https://opensource.org/licenses/ECL-2.0"/>
      <skos:inScheme rdf:resource="http://publications.europa.eu/resource/authority/licence"/>
      <skos:topConceptOf rdf:resource="http://publications.europa.eu/resource/authority/licence"/>
   </skos:Concept>
   <skos:Concept rdf:about="http://publications.europa.eu/resource/authority/licence/ECOS_2_0"
                 at:deprecated="false">
      <skos:prefLabel xml:lang="en">eCos License version 2.0</skos:prefLabel>
      <at:authority-code>ECOS_2_0</at:authority-code>
      <at:op-code>ECOS_2_0</at:op-code>
      <at:start.use>2002-05-15</at:start.use>
      <atold:op-code>ECOS_2_0</atold:op-code>
      <dc:identifier>ECOS_2_0</dc:identifier>
      <skos:altLabel xml:lang="bg">eCos-2.0</skos:altLabel>
      <skos:altLabel xml:lang="cs">eCos-2.0</skos:altLabel>
      <skos:altLabel xml:lang="da">eCos-2.0</skos:altLabel>
      <skos:altLabel xml:lang="de">eCos-2.0</skos:altLabel>
      <skos:altLabel xml:lang="el">eCos-2.0</skos:altLabel>
      <skos:altLabel xml:lang="en">eCos-2.0</skos:altLabel>
      <skos:altLabel xml:lang="es">eCos-2.0</skos:altLabel>
      <skos:altLabel xml:lang="et">eCos-2.0</skos:altLabel>
      <skos:altLabel xml:lang="fi">eCos-2.0</skos:altLabel>
      <skos:altLabel xml:lang="fr">eCos-2.0</skos:altLabel>
      <skos:altLabel xml:lang="ga">eCos-2.0</skos:altLabel>
      <skos:altLabel xml:lang="hr">eCos-2.0</skos:altLabel>
      <skos:altLabel xml:lang="hu">eCos-2.0</skos:altLabel>
      <skos:altLabel xml:lang="it">eCos-2.0</skos:altLabel>
      <skos:altLabel xml:lang="lt">eCos-2.0</skos:altLabel>
      <skos:altLabel xml:lang="lv">eCos-2.0</skos:altLabel>
      <skos:altLabel xml:lang="mt">eCos-2.0</skos:altLabel>
      <skos:altLabel xml:lang="nl">eCos-2.0</skos:altLabel>
      <skos:altLabel xml:lang="pl">eCos-2.0</skos:altLabel>
      <skos:altLabel xml:lang="pt">eCos-2.0</skos:altLabel>
      <skos:altLabel xml:lang="ro">eCos-2.0</skos:altLabel>
      <skos:altLabel xml:lang="sk">eCos-2.0</skos:altLabel>
      <skos:altLabel xml:lang="sl">eCos-2.0</skos:altLabel>
      <skos:altLabel xml:lang="sv">eCos-2.0</skos:altLabel>
      <skos:changeNote xml:lang="en">The source of the start-use date: http://ecos.sourceware.org/license-overview.html</skos:changeNote>
      <skos:definition xml:lang="en">Owned by the Free Software Foundation, eCos-2.0 is a copyleft-style, free software licence approved by the Open Source Initiative.</skos:definition>
      <skos:exactMatch rdf:resource="https://opensource.org/licenses/eCos-2.0"/>
      <skos:inScheme rdf:resource="http://publications.europa.eu/resource/authority/licence"/>
      <skos:topConceptOf rdf:resource="http://publications.europa.eu/resource/authority/licence"/>
   </skos:Concept>
   <skos:Concept rdf:about="http://publications.europa.eu/resource/authority/licence/EFL_1_0"
                 at:deprecated="true">
      <skos:prefLabel xml:lang="en">The Eiffel Forum License, version 1 (EFL-1.0)</skos:prefLabel>
      <at:authority-code>EFL_1_0</at:authority-code>
      <at:op-code>EFL_1_0</at:op-code>
      <at:start.use>2002-07-01</at:start.use>
      <atold:op-code>EFL_1_0</atold:op-code>
      <dc:identifier>EFL_1_0</dc:identifier>
      <skos:altLabel xml:lang="bg">EFL-1.0</skos:altLabel>
      <skos:altLabel xml:lang="cs">EFL-1.0</skos:altLabel>
      <skos:altLabel xml:lang="da">EFL-1.0</skos:altLabel>
      <skos:altLabel xml:lang="de">EFL-1.0</skos:altLabel>
      <skos:altLabel xml:lang="el">EFL-1.0</skos:altLabel>
      <skos:altLabel xml:lang="en">EFL-1.0</skos:altLabel>
      <skos:altLabel xml:lang="es">EFL-1.0</skos:altLabel>
      <skos:altLabel xml:lang="et">EFL-1.0</skos:altLabel>
      <skos:altLabel xml:lang="fi">EFL-1.0</skos:altLabel>
      <skos:altLabel xml:lang="fr">EFL-1.0</skos:altLabel>
      <skos:altLabel xml:lang="ga">EFL-1.0</skos:altLabel>
      <skos:altLabel xml:lang="hr">EFL-1.0</skos:altLabel>
      <skos:altLabel xml:lang="hu">EFL-1.0</skos:altLabel>
      <skos:altLabel xml:lang="it">EFL-1.0</skos:altLabel>
      <skos:altLabel xml:lang="lt">EFL-1.0</skos:altLabel>
      <skos:altLabel xml:lang="lv">EFL-1.0</skos:altLabel>
      <skos:altLabel xml:lang="mt">EFL-1.0</skos:altLabel>
      <skos:altLabel xml:lang="nl">EFL-1.0</skos:altLabel>
      <skos:altLabel xml:lang="pl">EFL-1.0</skos:altLabel>
      <skos:altLabel xml:lang="pt">EFL-1.0</skos:altLabel>
      <skos:altLabel xml:lang="ro">EFL-1.0</skos:altLabel>
      <skos:altLabel xml:lang="sk">EFL-1.0</skos:altLabel>
      <skos:altLabel xml:lang="sl">EFL-1.0</skos:altLabel>
      <skos:altLabel xml:lang="sv">EFL-1.0</skos:altLabel>
      <skos:changeNote xml:lang="en">The source of the start-use date: https://en.wikipedia.org/wiki/Eiffel_Forum_License</skos:changeNote>
      <skos:definition xml:lang="en">EFL-1.0 is a BSD-style, permissive free software licence approved by the Open Source Initiative. It is superseded by 2.0.</skos:definition>
      <skos:exactMatch rdf:resource="https://opensource.org/licenses/EFL-1.0"/>
      <skos:inScheme rdf:resource="http://publications.europa.eu/resource/authority/licence"/>
      <skos:topConceptOf rdf:resource="http://publications.europa.eu/resource/authority/licence"/>
      <at:end.use>2008-01-01</at:end.use>
   </skos:Concept>
   <skos:Concept rdf:about="http://publications.europa.eu/resource/authority/licence/EFL_2"
                 at:deprecated="false">
      <skos:prefLabel xml:lang="en">Eiffel Forum License, version 2</skos:prefLabel>
      <at:authority-code>EFL_2</at:authority-code>
      <at:op-code>EFL_2</at:op-code>
      <at:start.use>2008-01-02</at:start.use>
      <atold:op-code>EFL_2</atold:op-code>
      <dc:identifier>EFL_2</dc:identifier>
      <skos:altLabel xml:lang="bg">EFL-2.0</skos:altLabel>
      <skos:altLabel xml:lang="cs">EFL-2.0</skos:altLabel>
      <skos:altLabel xml:lang="da">EFL-2.0</skos:altLabel>
      <skos:altLabel xml:lang="de">EFL-2.0</skos:altLabel>
      <skos:altLabel xml:lang="el">EFL-2.0</skos:altLabel>
      <skos:altLabel xml:lang="en">EFL-2.0</skos:altLabel>
      <skos:altLabel xml:lang="es">EFL-2.0</skos:altLabel>
      <skos:altLabel xml:lang="et">EFL-2.0</skos:altLabel>
      <skos:altLabel xml:lang="fi">EFL-2.0</skos:altLabel>
      <skos:altLabel xml:lang="fr">EFL-2.0</skos:altLabel>
      <skos:altLabel xml:lang="ga">EFL-2.0</skos:altLabel>
      <skos:altLabel xml:lang="hr">EFL-2.0</skos:altLabel>
      <skos:altLabel xml:lang="hu">EFL-2.0</skos:altLabel>
      <skos:altLabel xml:lang="it">EFL-2.0</skos:altLabel>
      <skos:altLabel xml:lang="lt">EFL-2.0</skos:altLabel>
      <skos:altLabel xml:lang="lv">EFL-2.0</skos:altLabel>
      <skos:altLabel xml:lang="mt">EFL-2.0</skos:altLabel>
      <skos:altLabel xml:lang="nl">EFL-2.0</skos:altLabel>
      <skos:altLabel xml:lang="pl">EFL-2.0</skos:altLabel>
      <skos:altLabel xml:lang="pt">EFL-2.0</skos:altLabel>
      <skos:altLabel xml:lang="ro">EFL-2.0</skos:altLabel>
      <skos:altLabel xml:lang="sk">EFL-2.0</skos:altLabel>
      <skos:altLabel xml:lang="sl">EFL-2.0</skos:altLabel>
      <skos:altLabel xml:lang="sv">EFL-2.0</skos:altLabel>
      <skos:changeNote xml:lang="en">The source of the start-use date: https://en.wikipedia.org/wiki/Eiffel_Forum_License</skos:changeNote>
      <skos:definition xml:lang="en">EFL-2.0 is a BSD-style, permissive free software licence approved by the Open Source Initiative.</skos:definition>
      <skos:exactMatch rdf:resource="https://opensource.org/licenses/EFL-2.0"/>
      <skos:inScheme rdf:resource="http://publications.europa.eu/resource/authority/licence"/>
      <skos:topConceptOf rdf:resource="http://publications.europa.eu/resource/authority/licence"/>
   </skos:Concept>
   <skos:Concept rdf:about="http://publications.europa.eu/resource/authority/licence/ENTESSA"
                 at:deprecated="false">
      <skos:prefLabel xml:lang="en">Entessa Public License Version 1.0 (Entessa)</skos:prefLabel>
      <at:authority-code>ENTESSA</at:authority-code>
      <at:op-code>ENTESSA</at:op-code>
      <at:start.use>2003-07-01</at:start.use>
      <atold:op-code>ENTESSA</atold:op-code>
      <dc:identifier>ENTESSA</dc:identifier>
      <skos:altLabel xml:lang="bg">Entessa</skos:altLabel>
      <skos:altLabel xml:lang="cs">Entessa</skos:altLabel>
      <skos:altLabel xml:lang="da">Entessa</skos:altLabel>
      <skos:altLabel xml:lang="de">Entessa</skos:altLabel>
      <skos:altLabel xml:lang="el">Entessa</skos:altLabel>
      <skos:altLabel xml:lang="en">Entessa</skos:altLabel>
      <skos:altLabel xml:lang="es">Entessa</skos:altLabel>
      <skos:altLabel xml:lang="et">Entessa</skos:altLabel>
      <skos:altLabel xml:lang="fi">Entessa</skos:altLabel>
      <skos:altLabel xml:lang="fr">Entessa</skos:altLabel>
      <skos:altLabel xml:lang="ga">Entessa</skos:altLabel>
      <skos:altLabel xml:lang="hr">Entessa</skos:altLabel>
      <skos:altLabel xml:lang="hu">Entessa</skos:altLabel>
      <skos:altLabel xml:lang="it">Entessa</skos:altLabel>
      <skos:altLabel xml:lang="lt">Entessa</skos:altLabel>
      <skos:altLabel xml:lang="lv">Entessa</skos:altLabel>
      <skos:altLabel xml:lang="mt">Entessa</skos:altLabel>
      <skos:altLabel xml:lang="nl">Entessa</skos:altLabel>
      <skos:altLabel xml:lang="pl">Entessa</skos:altLabel>
      <skos:altLabel xml:lang="pt">Entessa</skos:altLabel>
      <skos:altLabel xml:lang="ro">Entessa</skos:altLabel>
      <skos:altLabel xml:lang="sk">Entessa</skos:altLabel>
      <skos:altLabel xml:lang="sl">Entessa</skos:altLabel>
      <skos:altLabel xml:lang="sv">Entessa</skos:altLabel>
      <skos:changeNote xml:lang="en">The source of the start-use date: https://enterprise.dejacode.com/licenses/public/entessa-1.0/</skos:changeNote>
      <skos:definition xml:lang="en">Entessa 1.0 is a BSD-style, permissive free software licence approved by the Open Source Initiative. It imposes copyright acknowledgements that are compatible with the EUPL.</skos:definition>
      <skos:exactMatch rdf:resource="https://opensource.org/licenses/Entessa"/>
      <skos:inScheme rdf:resource="http://publications.europa.eu/resource/authority/licence"/>
      <skos:topConceptOf rdf:resource="http://publications.europa.eu/resource/authority/licence"/>
   </skos:Concept>
   <skos:Concept rdf:about="http://publications.europa.eu/resource/authority/licence/EPL_1_0"
                 at:deprecated="true">
      <skos:prefLabel xml:lang="en">Eclipse Public License 1.0 (EPL-1.0)</skos:prefLabel>
      <at:authority-code>EPL_1_0</at:authority-code>
      <at:op-code>EPL_1_0</at:op-code>
      <at:start.use>2005-06-28</at:start.use>
      <atold:op-code>EPL_1_0</atold:op-code>
      <dc:identifier>EPL_1_0</dc:identifier>
      <skos:altLabel xml:lang="bg">EPL-1.0</skos:altLabel>
      <skos:altLabel xml:lang="cs">EPL-1.0</skos:altLabel>
      <skos:altLabel xml:lang="da">EPL-1.0</skos:altLabel>
      <skos:altLabel xml:lang="de">EPL-1.0</skos:altLabel>
      <skos:altLabel xml:lang="el">EPL-1.0</skos:altLabel>
      <skos:altLabel xml:lang="en">EPL-1.0</skos:altLabel>
      <skos:altLabel xml:lang="es">EPL-1.0</skos:altLabel>
      <skos:altLabel xml:lang="et">EPL-1.0</skos:altLabel>
      <skos:altLabel xml:lang="fi">EPL-1.0</skos:altLabel>
      <skos:altLabel xml:lang="fr">EPL-1.0</skos:altLabel>
      <skos:altLabel xml:lang="ga">EPL-1.0</skos:altLabel>
      <skos:altLabel xml:lang="hr">EPL-1.0</skos:altLabel>
      <skos:altLabel xml:lang="hu">EPL-1.0</skos:altLabel>
      <skos:altLabel xml:lang="it">EPL-1.0</skos:altLabel>
      <skos:altLabel xml:lang="lt">EPL-1.0</skos:altLabel>
      <skos:altLabel xml:lang="lv">EPL-1.0</skos:altLabel>
      <skos:altLabel xml:lang="mt">EPL-1.0</skos:altLabel>
      <skos:altLabel xml:lang="nl">EPL-1.0</skos:altLabel>
      <skos:altLabel xml:lang="pl">EPL-1.0</skos:altLabel>
      <skos:altLabel xml:lang="pt">EPL-1.0</skos:altLabel>
      <skos:altLabel xml:lang="ro">EPL-1.0</skos:altLabel>
      <skos:altLabel xml:lang="sk">EPL-1.0</skos:altLabel>
      <skos:altLabel xml:lang="sl">EPL-1.0</skos:altLabel>
      <skos:altLabel xml:lang="sv">EPL-1.0</skos:altLabel>
      <skos:changeNote xml:lang="en">The source of the start-use date: https://spdx.org/licenses/EPL-1.0.html</skos:changeNote>
      <skos:definition xml:lang="en">EPL 1.0 is a copyleft-style, free software licence approved by the Open Source Initiative. Made and mainly used by the Eclipse Foundation, it is similar to GPL but does not submit linking of the covered code to conditions or ”viral” extension of licence coverage to the other linked software. It is superseded by EPL 2.0.</skos:definition>
      <skos:exactMatch rdf:resource="https://opensource.org/licenses/EPL-1.0"/>
      <skos:inScheme rdf:resource="http://publications.europa.eu/resource/authority/licence"/>
      <skos:topConceptOf rdf:resource="http://publications.europa.eu/resource/authority/licence"/>
      <at:end.use>2017-08-23</at:end.use>
   </skos:Concept>
   <skos:Concept rdf:about="http://publications.europa.eu/resource/authority/licence/EPL_2_0"
                 at:deprecated="false">
      <skos:prefLabel xml:lang="en">Eclipse Public License version 2.0</skos:prefLabel>
      <at:authority-code>EPL_2_0</at:authority-code>
      <at:op-code>EPL_2_0</at:op-code>
      <at:start.use>2017-08-24</at:start.use>
      <atold:op-code>EPL_2_0</atold:op-code>
      <dc:identifier>EPL_2_0</dc:identifier>
      <skos:altLabel xml:lang="bg">EPL-2.0</skos:altLabel>
      <skos:altLabel xml:lang="cs">EPL-2.0</skos:altLabel>
      <skos:altLabel xml:lang="da">EPL-2.0</skos:altLabel>
      <skos:altLabel xml:lang="de">EPL-2.0</skos:altLabel>
      <skos:altLabel xml:lang="el">EPL-2.0</skos:altLabel>
      <skos:altLabel xml:lang="en">EPL-2.0</skos:altLabel>
      <skos:altLabel xml:lang="es">EPL-2.0</skos:altLabel>
      <skos:altLabel xml:lang="et">EPL-2.0</skos:altLabel>
      <skos:altLabel xml:lang="fi">EPL-2.0</skos:altLabel>
      <skos:altLabel xml:lang="fr">EPL-2.0</skos:altLabel>
      <skos:altLabel xml:lang="ga">EPL-2.0</skos:altLabel>
      <skos:altLabel xml:lang="hr">EPL-2.0</skos:altLabel>
      <skos:altLabel xml:lang="hu">EPL-2.0</skos:altLabel>
      <skos:altLabel xml:lang="it">EPL-2.0</skos:altLabel>
      <skos:altLabel xml:lang="lt">EPL-2.0</skos:altLabel>
      <skos:altLabel xml:lang="lv">EPL-2.0</skos:altLabel>
      <skos:altLabel xml:lang="mt">EPL-2.0</skos:altLabel>
      <skos:altLabel xml:lang="nl">EPL-2.0</skos:altLabel>
      <skos:altLabel xml:lang="pl">EPL-2.0</skos:altLabel>
      <skos:altLabel xml:lang="pt">EPL-2.0</skos:altLabel>
      <skos:altLabel xml:lang="ro">EPL-2.0</skos:altLabel>
      <skos:altLabel xml:lang="sk">EPL-2.0</skos:altLabel>
      <skos:altLabel xml:lang="sl">EPL-2.0</skos:altLabel>
      <skos:altLabel xml:lang="sv">EPL-2.0</skos:altLabel>
      <skos:changeNote xml:lang="en">The source of the start-use date: https://en.wikipedia.org/wiki/Eclipse_Public_License</skos:changeNote>
      <skos:definition xml:lang="en">EPL 2.0 is a copyleft-style, free software licence approved by the Open Source Initiative. Made and mainly used by the Eclipse Foundation, it is similar to GPL but does not submit linking of the covered code to conditions or ”viral” extension of licence coverage to the other linked software.</skos:definition>
      <skos:exactMatch rdf:resource="https://opensource.org/licenses/EPL-2.0"/>
      <skos:inScheme rdf:resource="http://publications.europa.eu/resource/authority/licence"/>
      <skos:topConceptOf rdf:resource="http://publications.europa.eu/resource/authority/licence"/>
   </skos:Concept>
   <skos:Concept rdf:about="http://publications.europa.eu/resource/authority/licence/ETALAB_2_0"
                 at:deprecated="false">
      <skos:prefLabel xml:lang="en">Etalab Open Licence V 2.0</skos:prefLabel>
      <skos:prefLabel xml:lang="fr">Licence Ouverte Etalab V 2.0 </skos:prefLabel>
      <at:authority-code>ETALAB_2_0</at:authority-code>
      <at:op-code>ETALAB_2_0</at:op-code>
      <at:start.use>2011-10-18</at:start.use>
      <atold:op-code>ETALAB_2_0</atold:op-code>
      <dc:identifier>ETALAB_2_0</dc:identifier>
      <skos:altLabel xml:lang="bg">Etalab-2.0</skos:altLabel>
      <skos:altLabel xml:lang="cs">Etalab-2.0</skos:altLabel>
      <skos:altLabel xml:lang="da">Etalab-2.0</skos:altLabel>
      <skos:altLabel xml:lang="de">Etalab-2.0</skos:altLabel>
      <skos:altLabel xml:lang="el">Etalab-2.0</skos:altLabel>
      <skos:altLabel xml:lang="en">Etalab-2.0</skos:altLabel>
      <skos:altLabel xml:lang="es">Etalab-2.0</skos:altLabel>
      <skos:altLabel xml:lang="et">Etalab-2.0</skos:altLabel>
      <skos:altLabel xml:lang="fi">Etalab-2.0</skos:altLabel>
      <skos:altLabel xml:lang="fr">Etalab-2.0</skos:altLabel>
      <skos:altLabel xml:lang="ga">Etalab-2.0</skos:altLabel>
      <skos:altLabel xml:lang="hr">Etalab-2.0</skos:altLabel>
      <skos:altLabel xml:lang="hu">Etalab-2.0</skos:altLabel>
      <skos:altLabel xml:lang="it">Etalab-2.0</skos:altLabel>
      <skos:altLabel xml:lang="lt">Etalab-2.0</skos:altLabel>
      <skos:altLabel xml:lang="lv">Etalab-2.0</skos:altLabel>
      <skos:altLabel xml:lang="mt">Etalab-2.0</skos:altLabel>
      <skos:altLabel xml:lang="nl">Etalab-2.0</skos:altLabel>
      <skos:altLabel xml:lang="pl">Etalab-2.0</skos:altLabel>
      <skos:altLabel xml:lang="pt">Etalab-2.0</skos:altLabel>
      <skos:altLabel xml:lang="ro">Etalab-2.0</skos:altLabel>
      <skos:altLabel xml:lang="sk">Etalab-2.0</skos:altLabel>
      <skos:altLabel xml:lang="sl">Etalab-2.0</skos:altLabel>
      <skos:altLabel xml:lang="sv">Etalab-2.0</skos:altLabel>
      <skos:definition xml:lang="en">The Licence Ouverte / Open Licence is a French open licence published by Etalab for open data from the State of France. The licence was designed to be compatible with Creative Commons Licences, Open Government Licence and the Open Data Commons Attribution License.</skos:definition>
      <skos:definition xml:lang="fr">La Licence ouverte / Open Licence, aussi appelée Licence Ouverte Etalab, est une licence libre française créée par la mission Etalab afin d’encadrer l’ouverture des données de l’État français. Cette licence a été voulue comme une licence compatible avec les licences Open Government Licence du Royaume-Uni, Open Data Commons Attribution de l’Open Knowledge Foundation et Creative Commons Attribution 2.0 de Creative Commons.</skos:definition>
      <skos:exactMatch rdf:resource="https://www.etalab.gouv.fr/licence-ouverte-open-licence/"/>
      <skos:inScheme rdf:resource="http://publications.europa.eu/resource/authority/licence"/>
      <skos:topConceptOf rdf:resource="http://publications.europa.eu/resource/authority/licence"/>
   </skos:Concept>
   <skos:Concept rdf:about="http://publications.europa.eu/resource/authority/licence/EUPL_1_0"
                 at:deprecated="false">
      <skos:prefLabel xml:lang="bg">Публичен лиценз на Европейския съюз версия v.1.0</skos:prefLabel>
      <skos:prefLabel xml:lang="cs">Veřejná Licence Evropské Unie v.1.0</skos:prefLabel>
      <skos:prefLabel xml:lang="da">Europæiske Unions Offentlige Licens v.1.0</skos:prefLabel>
      <skos:prefLabel xml:lang="de">Open-Source-Lizenz für die Europäische Union v.1.0</skos:prefLabel>
      <skos:prefLabel xml:lang="el">Άδεια δημόσιας χρήσης για την Ευρωπαϊκή Ένωση v.1.0</skos:prefLabel>
      <skos:prefLabel xml:lang="en">European Union Public Licence v.1.0</skos:prefLabel>
      <skos:prefLabel xml:lang="es">Licencia Pública de la Unión Europea v.1.0</skos:prefLabel>
      <skos:prefLabel xml:lang="et">Euroopa Liidu tarkvara vaba kasutuse litsents v.1.0</skos:prefLabel>
      <skos:prefLabel xml:lang="fi">Euroopan unionin yleinen lisenssi v.1.0</skos:prefLabel>
      <skos:prefLabel xml:lang="fr">Licence Publique de l’Union européenne v.1.0</skos:prefLabel>
      <skos:prefLabel xml:lang="hr">Javna licencija Europske unije v. 1.0</skos:prefLabel>
      <skos:prefLabel xml:lang="hu">Európai Uniós Nyílt Forráskódú Licenc v.1.0</skos:prefLabel>
      <skos:prefLabel xml:lang="it">Licenza Pubblica dell'Unione europea v.1.0</skos:prefLabel>
      <skos:prefLabel xml:lang="lt">Europos Sąjungos viešoji licencija V.1.0</skos:prefLabel>
      <skos:prefLabel xml:lang="lv">Eiropas Savienības sabiedriskā licence V.1.0</skos:prefLabel>
      <skos:prefLabel xml:lang="mt">Liċenzja Pubblika ta' l-Unjoni Ewropea V.1.0</skos:prefLabel>
      <skos:prefLabel xml:lang="nl">Openbare licentie van de Europese Unie V.1.0</skos:prefLabel>
      <skos:prefLabel xml:lang="pl">Licencja publiczna UE wersja 1.0</skos:prefLabel>
      <skos:prefLabel xml:lang="pt">Licença Pública da União Europeia V.1.0</skos:prefLabel>
      <skos:prefLabel xml:lang="ro">Licenţa publică a Uniunii Europene v.1.0</skos:prefLabel>
      <skos:prefLabel xml:lang="sk">Verejná licencia Európskej únie V.1.0</skos:prefLabel>
      <skos:prefLabel xml:lang="sl">Javna licenca Evropske unije V.1.0</skos:prefLabel>
      <skos:prefLabel xml:lang="sv">Licens till öppen källkod från Europeiska Unionen V.1.0</skos:prefLabel>
      <at:authority-code>EUPL_1_0</at:authority-code>
      <at:op-code>EUPL_1_0</at:op-code>
      <at:start.use>2007-01-09</at:start.use>
      <atold:op-code>EUPL_1_0</atold:op-code>
      <dc:identifier>EUPL_1_0</dc:identifier>
      <skos:altLabel xml:lang="bg">EUPL v.1.0</skos:altLabel>
      <skos:altLabel xml:lang="cs">EUPL v.1.0</skos:altLabel>
      <skos:altLabel xml:lang="da">EUPL v.1.0</skos:altLabel>
      <skos:altLabel xml:lang="de">EUPL v.1.0</skos:altLabel>
      <skos:altLabel xml:lang="el">EUPL v.1.0</skos:altLabel>
      <skos:altLabel xml:lang="en">EUPL v.1.0</skos:altLabel>
      <skos:altLabel xml:lang="es">EUPL v.1.0</skos:altLabel>
      <skos:altLabel xml:lang="et">EUPL v.1.0</skos:altLabel>
      <skos:altLabel xml:lang="fi">EUPL v.1.0</skos:altLabel>
      <skos:altLabel xml:lang="fr">EUPL v.1.0</skos:altLabel>
      <skos:altLabel xml:lang="ga">EUPL v.1.0</skos:altLabel>
      <skos:altLabel xml:lang="hr">EUPL v.1.0</skos:altLabel>
      <skos:altLabel xml:lang="hu">EUPL v.1.0</skos:altLabel>
      <skos:altLabel xml:lang="it">EUPL v.1.0</skos:altLabel>
      <skos:altLabel xml:lang="lt">EUPL v.1.0</skos:altLabel>
      <skos:altLabel xml:lang="lv">EUPL v.1.0</skos:altLabel>
      <skos:altLabel xml:lang="mt">EUPL v.1.0</skos:altLabel>
      <skos:altLabel xml:lang="nl">EUPL v.1.0</skos:altLabel>
      <skos:altLabel xml:lang="pl">EUPL v.1.0</skos:altLabel>
      <skos:altLabel xml:lang="pt">EUPL v.1.0</skos:altLabel>
      <skos:altLabel xml:lang="ro">EUPL v.1.0</skos:altLabel>
      <skos:altLabel xml:lang="sk">EUPL v.1.0</skos:altLabel>
      <skos:altLabel xml:lang="sl">EUPL v.1.0</skos:altLabel>
      <skos:altLabel xml:lang="sv">EUPL v.1.0</skos:altLabel>
      <skos:definition xml:lang="en">Created as a tool for publishing any copyrighted work as open source on the initiative of the European Commission, EUPL v.1.0 is the first European Free/Open Source Software (F/OSS) licence. The final version (v.1.0) was officially approved on 9 January 2007 in three linguistic versions. By a second Decision of 9 January 2008, the European Commission validated the EUPL in all the official languages of the European Union.</skos:definition>
      <skos:exactMatch rdf:resource="http://ec.europa.eu/idabc/en/document/7330.html"/>
      <skos:inScheme rdf:resource="http://publications.europa.eu/resource/authority/licence"/>
      <skos:topConceptOf rdf:resource="http://publications.europa.eu/resource/authority/licence"/>
   </skos:Concept>
   <skos:Concept rdf:about="http://publications.europa.eu/resource/authority/licence/EUPL_1_1"
                 at:deprecated="false">
      <skos:prefLabel xml:lang="bg">Публичен лиценз на Европейския съюз версия v.1.1</skos:prefLabel>
      <skos:prefLabel xml:lang="cs">Veřejná Licence Evropské Unie v.1.1</skos:prefLabel>
      <skos:prefLabel xml:lang="da">Europæiske Unions Offentlige Licens v.1.1</skos:prefLabel>
      <skos:prefLabel xml:lang="de">Open-Source-Lizenz für die Europäische Union v.1.1</skos:prefLabel>
      <skos:prefLabel xml:lang="el">Άδεια δηµόσιας χρήσης για την Ευρωπαϊκή Ένωση V.1.1</skos:prefLabel>
      <skos:prefLabel xml:lang="en">European Union Public Licence v. 1.1</skos:prefLabel>
      <skos:prefLabel xml:lang="es">Licencia Pública de la Unión Europea v.1.1</skos:prefLabel>
      <skos:prefLabel xml:lang="et">Euroopa Liidu tarkvara vaba kasutuse litsents v.1.1</skos:prefLabel>
      <skos:prefLabel xml:lang="fi">Euroopan unionin yleinen lisenssi v.1.1</skos:prefLabel>
      <skos:prefLabel xml:lang="fr">Licence publique de l'Union européenne v. 1.1</skos:prefLabel>
      <skos:prefLabel xml:lang="hr">Javna licencija Europske unije v. 1.1</skos:prefLabel>
      <skos:prefLabel xml:lang="hu">Európai Uniós Nyílt Forráskódú Licenc V.1.1</skos:prefLabel>
      <skos:prefLabel xml:lang="it">Licenza Pubblica dell'Unione europea v. 1.1</skos:prefLabel>
      <skos:prefLabel xml:lang="lt">Europos Sąjungos viešoji licencija V.1.1</skos:prefLabel>
      <skos:prefLabel xml:lang="lv">Eiropas Savienības sabiedriskā licence V.1.1</skos:prefLabel>
      <skos:prefLabel xml:lang="mt">Liċenzja Pubblika tal-Unjoni Ewropea V.1.1</skos:prefLabel>
      <skos:prefLabel xml:lang="nl">Openbare licentie van de Europese Unie V.1.1</skos:prefLabel>
      <skos:prefLabel xml:lang="pl">Licencja publiczna Unii Europejskiej v.1.1</skos:prefLabel>
      <skos:prefLabel xml:lang="pt">Licença Pública da União Europeia V.1.1</skos:prefLabel>
      <skos:prefLabel xml:lang="ro">Licenţa publică a Uniunii Europene V.1.1</skos:prefLabel>
      <skos:prefLabel xml:lang="sk">Verejná licencia Európskej únie V.1.1</skos:prefLabel>
      <skos:prefLabel xml:lang="sl">Javna licenca Evropske unije V.1.1</skos:prefLabel>
      <skos:prefLabel xml:lang="sv">Licens till öppen källkod från Europeiska unionen v.1.1</skos:prefLabel>
      <at:authority-code>EUPL_1_1</at:authority-code>
      <at:op-code>EUPL_1_1</at:op-code>
      <at:start.use>2009-01-09</at:start.use>
      <atold:op-code>EUPL_1_1</atold:op-code>
      <dc:identifier>EUPL_1_1</dc:identifier>
      <skos:altLabel xml:lang="bg">EUPL v.1.1</skos:altLabel>
      <skos:altLabel xml:lang="cs">EUPL v.1.1</skos:altLabel>
      <skos:altLabel xml:lang="da">EUPL v.1.1</skos:altLabel>
      <skos:altLabel xml:lang="de">EUPL v.1.1</skos:altLabel>
      <skos:altLabel xml:lang="el">EUPL v.1.1</skos:altLabel>
      <skos:altLabel xml:lang="en">EUPL v.1.1</skos:altLabel>
      <skos:altLabel xml:lang="es">EUPL v.1.1</skos:altLabel>
      <skos:altLabel xml:lang="et">EUPL v.1.1</skos:altLabel>
      <skos:altLabel xml:lang="fi">EUPL v.1.1</skos:altLabel>
      <skos:altLabel xml:lang="fr">EUPL v.1.1</skos:altLabel>
      <skos:altLabel xml:lang="ga">EUPL v.1.1</skos:altLabel>
      <skos:altLabel xml:lang="hr">EUPL v.1.1</skos:altLabel>
      <skos:altLabel xml:lang="hu">EUPL v.1.1</skos:altLabel>
      <skos:altLabel xml:lang="it">EUPL v.1.1</skos:altLabel>
      <skos:altLabel xml:lang="lt">EUPL v.1.1</skos:altLabel>
      <skos:altLabel xml:lang="lv">EUPL v.1.1</skos:altLabel>
      <skos:altLabel xml:lang="mt">EUPL v.1.1</skos:altLabel>
      <skos:altLabel xml:lang="nl">EUPL v.1.1</skos:altLabel>
      <skos:altLabel xml:lang="pl">EUPL v.1.1</skos:altLabel>
      <skos:altLabel xml:lang="pt">EUPL v.1.1</skos:altLabel>
      <skos:altLabel xml:lang="ro">EUPL v.1.1</skos:altLabel>
      <skos:altLabel xml:lang="sk">EUPL v.1.1</skos:altLabel>
      <skos:altLabel xml:lang="sl">EUPL v.1.1</skos:altLabel>
      <skos:altLabel xml:lang="sv">EUPL v.1.1</skos:altLabel>
      <skos:definition xml:lang="en">Created as a tool for publishing any copyrighted work as open source on the initiative of the European Commission, EUPL v.1.1 is the first European Free/Open Source Software (F/OSS) licence. The European Commission published the version 1.1 in all the official languages of the European Union by the Decision of 9 January 2009.</skos:definition>
      <skos:exactMatch rdf:resource="https://joinup.ec.europa.eu/collection/eupl/eupl-text-11-12"/>
      <skos:inScheme rdf:resource="http://publications.europa.eu/resource/authority/licence"/>
      <skos:topConceptOf rdf:resource="http://publications.europa.eu/resource/authority/licence"/>
   </skos:Concept>
   <skos:Concept rdf:about="http://publications.europa.eu/resource/authority/licence/EUPL_1_2"
                 at:deprecated="false">
      <skos:prefLabel xml:lang="bg">Публичен лиценз на Европейския съюз версия v.1.2</skos:prefLabel>
      <skos:prefLabel xml:lang="cs">Veřejná Licence Evropské Unie v.1.2</skos:prefLabel>
      <skos:prefLabel xml:lang="da">Europæiske Unions Offentlige Licens v.1.2</skos:prefLabel>
      <skos:prefLabel xml:lang="de">Open-Source-Lizenz für die Europäische Union v.1.2</skos:prefLabel>
      <skos:prefLabel xml:lang="el">Άδεια δημόσιας χρήσης για την Ευρωπαϊκή Ένωση v. 1.2</skos:prefLabel>
      <skos:prefLabel xml:lang="en">European Union Public Licence v. 1.2</skos:prefLabel>
      <skos:prefLabel xml:lang="es">Licencia Pública de la Unión Europea v.1.2</skos:prefLabel>
      <skos:prefLabel xml:lang="et">Euroopa Liidu tarkvara vaba kasutuse litsents v.1.2</skos:prefLabel>
      <skos:prefLabel xml:lang="fi">Euroopan unionin yleisen lisenssi v. 1.2</skos:prefLabel>
      <skos:prefLabel xml:lang="fr">Licence publique de l'Union européenne v. 1.2</skos:prefLabel>
      <skos:prefLabel xml:lang="hr">Javna licencija Europske unije v. 1.2</skos:prefLabel>
      <skos:prefLabel xml:lang="hu">Európai Uniós Nyilvános Licenc 1.2. verzió</skos:prefLabel>
      <skos:prefLabel xml:lang="it">Licenza Pubblica dell'Unione europea v 1.2</skos:prefLabel>
      <skos:prefLabel xml:lang="lt">Europos Sąjungos viešoji licencija v. 1.2</skos:prefLabel>
      <skos:prefLabel xml:lang="lv">Eiropas Savienības sabiedriskā licence 1.2. redakcija</skos:prefLabel>
      <skos:prefLabel xml:lang="mt">Liċenzja Pubblika tal-Unjoni Ewropea v. 1.2</skos:prefLabel>
      <skos:prefLabel xml:lang="nl">Openbare licentie van de Europese Unie v. 1.2</skos:prefLabel>
      <skos:prefLabel xml:lang="pl">Licencja publiczna Unii Europejskiej wersja 1.2</skos:prefLabel>
      <skos:prefLabel xml:lang="pt">Licença Pública da União Europeia v. 1.2</skos:prefLabel>
      <skos:prefLabel xml:lang="ro">Licență publică a Uniunii Europene V. 1.2</skos:prefLabel>
      <skos:prefLabel xml:lang="sk">Verejná licencia Európskej únie v. 1.2</skos:prefLabel>
      <skos:prefLabel xml:lang="sl">Javna licenca Evropske unije v. 1.2</skos:prefLabel>
      <skos:prefLabel xml:lang="sv">Licens till öppen källkod från Europeiska unionen v. 1.2</skos:prefLabel>
      <at:authority-code>EUPL_1_2</at:authority-code>
      <at:op-code>EUPL_1_2</at:op-code>
      <at:start.use>2017-05-19</at:start.use>
      <atold:op-code>EUPL_1_2</atold:op-code>
      <dc:identifier>EUPL_1_2</dc:identifier>
      <skos:altLabel xml:lang="bg">EUPL v1.2</skos:altLabel>
      <skos:altLabel xml:lang="cs">EUPL v1.2</skos:altLabel>
      <skos:altLabel xml:lang="da">EUPL v1.2</skos:altLabel>
      <skos:altLabel xml:lang="de">EUPL v1.2</skos:altLabel>
      <skos:altLabel xml:lang="el">EUPL v1.2</skos:altLabel>
      <skos:altLabel xml:lang="en">EUPL v1.2</skos:altLabel>
      <skos:altLabel xml:lang="es">EUPL v1.2</skos:altLabel>
      <skos:altLabel xml:lang="et">EUPL v1.2</skos:altLabel>
      <skos:altLabel xml:lang="fi">EUPL v1.2</skos:altLabel>
      <skos:altLabel xml:lang="fr">EUPL v1.2</skos:altLabel>
      <skos:altLabel xml:lang="ga">EUPL v1.2</skos:altLabel>
      <skos:altLabel xml:lang="hr">EUPL v1.2</skos:altLabel>
      <skos:altLabel xml:lang="hu">EUPL v1.2</skos:altLabel>
      <skos:altLabel xml:lang="it">EUPL v1.2</skos:altLabel>
      <skos:altLabel xml:lang="lt">EUPL v1.2</skos:altLabel>
      <skos:altLabel xml:lang="lv">EUPL v1.2</skos:altLabel>
      <skos:altLabel xml:lang="mt">EUPL v1.2</skos:altLabel>
      <skos:altLabel xml:lang="nl">EUPL v1.2</skos:altLabel>
      <skos:altLabel xml:lang="pl">EUPL v1.2</skos:altLabel>
      <skos:altLabel xml:lang="pt">EUPL v1.2</skos:altLabel>
      <skos:altLabel xml:lang="ro">EUPL v1.2</skos:altLabel>
      <skos:altLabel xml:lang="sk">EUPL v1.2</skos:altLabel>
      <skos:altLabel xml:lang="sl">EUPL v1.2</skos:altLabel>
      <skos:altLabel xml:lang="sv">EUPL v1.2</skos:altLabel>
      <skos:definition xml:lang="en">Created as a tool for publishing any copyrighted work as open source, EUPL v.1.2 is legally consistent with the copyright law of all EU countries and is especially well-suited for public administrations sharing IT solutions. It is also widely used by the private sector. The text of the EUPL version 1.2 was published on 19 May 2017.</skos:definition>
      <skos:definition xml:lang="fr">EUPL v.1.2 a été créée par la Commission en 2007. Elle a pour but de constituer une licence libre valable dans toutes les langues de l’Union, en tenant compte de ses spécificités juridiques et des questions de compatibilité entre licences libres. Il s’agit d’une licence dite «copyleft» dont le but est de garantir la nature «open source» des dérivés des logiciels.</skos:definition>
      <skos:exactMatch rdf:resource="https://joinup.ec.europa.eu/collection/eupl/eupl-text-11-12"/>
      <skos:inScheme rdf:resource="http://publications.europa.eu/resource/authority/licence"/>
      <skos:topConceptOf rdf:resource="http://publications.europa.eu/resource/authority/licence"/>
   </skos:Concept>
   <skos:Concept rdf:about="http://publications.europa.eu/resource/authority/licence/EUROGEO_2022"
                 at:deprecated="false">
      <skos:prefLabel xml:lang="en">EuroGeographics Open Data Licence v.2022</skos:prefLabel>
      <at:authority-code>EUROGEO_2022</at:authority-code>
      <at:op-code>EUROGEO_2022</at:op-code>
      <at:start.use>2013-01-01</at:start.use>
      <atold:op-code>EUROGEO_2022</atold:op-code>
      <dc:identifier>EUROGEO_2022</dc:identifier>
      <skos:altLabel xml:lang="bg">EuroGeographicsODL v.2022</skos:altLabel>
      <skos:altLabel xml:lang="cs">EuroGeographicsODL v.2022</skos:altLabel>
      <skos:altLabel xml:lang="da">EuroGeographicsODL v.2022</skos:altLabel>
      <skos:altLabel xml:lang="de">EuroGeographicsODL v.2022</skos:altLabel>
      <skos:altLabel xml:lang="el">EuroGeographicsODL v.2022</skos:altLabel>
      <skos:altLabel xml:lang="en">EuroGeographicsODL v.2022</skos:altLabel>
      <skos:altLabel xml:lang="es">EuroGeographicsODL v.2022</skos:altLabel>
      <skos:altLabel xml:lang="et">EuroGeographicsODL v.2022</skos:altLabel>
      <skos:altLabel xml:lang="fi">EuroGeographicsODL v.2022</skos:altLabel>
      <skos:altLabel xml:lang="fr">EuroGeographicsODL v.2022</skos:altLabel>
      <skos:altLabel xml:lang="ga">EuroGeographicsODL v.2022</skos:altLabel>
      <skos:altLabel xml:lang="hr">EuroGeographicsODL v.2022</skos:altLabel>
      <skos:altLabel xml:lang="hu">EuroGeographicsODL v.2022</skos:altLabel>
      <skos:altLabel xml:lang="it">EuroGeographicsODL v.2022</skos:altLabel>
      <skos:altLabel xml:lang="lt">EuroGeographicsODL v.2022</skos:altLabel>
      <skos:altLabel xml:lang="lv">EuroGeographicsODL v.2022</skos:altLabel>
      <skos:altLabel xml:lang="mt">EuroGeographicsODL v.2022</skos:altLabel>
      <skos:altLabel xml:lang="nl">EuroGeographicsODL v.2022</skos:altLabel>
      <skos:altLabel xml:lang="pl">EuroGeographicsODL v.2022</skos:altLabel>
      <skos:altLabel xml:lang="pt">EuroGeographicsODL v.2022</skos:altLabel>
      <skos:altLabel xml:lang="ro">EuroGeographicsODL v.2022</skos:altLabel>
      <skos:altLabel xml:lang="sk">EuroGeographicsODL v.2022</skos:altLabel>
      <skos:altLabel xml:lang="sl">EuroGeographicsODL v.2022</skos:altLabel>
      <skos:altLabel xml:lang="sv">EuroGeographicsODL v.2022</skos:altLabel>
      <skos:definition xml:lang="en">free software licence approved by the EuroGeographics AISBL, letting others to reuse the work as long as credit is given to the author and new creations are licenced under the identical terms</skos:definition>
      <skos:exactMatch rdf:resource="https://www.mapsforeurope.org/licence"/>
      <skos:inScheme rdf:resource="http://publications.europa.eu/resource/authority/licence"/>
      <skos:topConceptOf rdf:resource="http://publications.europa.eu/resource/authority/licence"/>
   </skos:Concept>
   <skos:Concept rdf:about="http://publications.europa.eu/resource/authority/licence/EU_DATAGRID"
                 at:deprecated="false">
      <skos:prefLabel xml:lang="en">EU DataGrid Software License (EUDatagrid)</skos:prefLabel>
      <at:authority-code>EU_DATAGRID</at:authority-code>
      <at:op-code>EU_DATAGRID</at:op-code>
      <at:start.use>2001-06-30</at:start.use>
      <atold:op-code>EU_DATAGRID</atold:op-code>
      <dc:identifier>EU_DATAGRID</dc:identifier>
      <skos:altLabel xml:lang="bg">EUDatagrid</skos:altLabel>
      <skos:altLabel xml:lang="cs">EUDatagrid</skos:altLabel>
      <skos:altLabel xml:lang="da">EUDatagrid</skos:altLabel>
      <skos:altLabel xml:lang="de">EUDatagrid</skos:altLabel>
      <skos:altLabel xml:lang="el">EUDatagrid</skos:altLabel>
      <skos:altLabel xml:lang="en">EUDatagrid</skos:altLabel>
      <skos:altLabel xml:lang="es">EUDatagrid</skos:altLabel>
      <skos:altLabel xml:lang="et">EUDatagrid</skos:altLabel>
      <skos:altLabel xml:lang="fi">EUDatagrid</skos:altLabel>
      <skos:altLabel xml:lang="fr">EUDatagrid</skos:altLabel>
      <skos:altLabel xml:lang="ga">EUDatagrid</skos:altLabel>
      <skos:altLabel xml:lang="hr">EUDatagrid</skos:altLabel>
      <skos:altLabel xml:lang="hu">EUDatagrid</skos:altLabel>
      <skos:altLabel xml:lang="it">EUDatagrid</skos:altLabel>
      <skos:altLabel xml:lang="lt">EUDatagrid</skos:altLabel>
      <skos:altLabel xml:lang="lv">EUDatagrid</skos:altLabel>
      <skos:altLabel xml:lang="mt">EUDatagrid</skos:altLabel>
      <skos:altLabel xml:lang="nl">EUDatagrid</skos:altLabel>
      <skos:altLabel xml:lang="pl">EUDatagrid</skos:altLabel>
      <skos:altLabel xml:lang="pt">EUDatagrid</skos:altLabel>
      <skos:altLabel xml:lang="ro">EUDatagrid</skos:altLabel>
      <skos:altLabel xml:lang="sk">EUDatagrid</skos:altLabel>
      <skos:altLabel xml:lang="sl">EUDatagrid</skos:altLabel>
      <skos:altLabel xml:lang="sv">EUDatagrid</skos:altLabel>
      <skos:changeNote xml:lang="en">The source of the start-use date: https://enterprise.dejacode.com/licenses/public/eu-datagrid/</skos:changeNote>
      <skos:definition xml:lang="en">EUDatagrid is a permissive free software licence approved by the Open Source Initiative. It is a classic 3-clause licence. Nothing in this licence restricts redistribution of larger works under the EUPL.</skos:definition>
      <skos:exactMatch rdf:resource="https://opensource.org/licenses/EUDatagrid"/>
      <skos:inScheme rdf:resource="http://publications.europa.eu/resource/authority/licence"/>
      <skos:topConceptOf rdf:resource="http://publications.europa.eu/resource/authority/licence"/>
   </skos:Concept>
   <skos:Concept rdf:about="http://publications.europa.eu/resource/authority/licence/FAIR"
                 at:deprecated="false">
      <skos:prefLabel xml:lang="en">Fair License (Fair)</skos:prefLabel>
      <at:authority-code>FAIR</at:authority-code>
      <at:op-code>FAIR</at:op-code>
      <at:start.use>2004-01-31</at:start.use>
      <atold:op-code>FAIR</atold:op-code>
      <dc:identifier>FAIR</dc:identifier>
      <skos:altLabel xml:lang="bg">Fair</skos:altLabel>
      <skos:altLabel xml:lang="cs">Fair</skos:altLabel>
      <skos:altLabel xml:lang="da">Fair</skos:altLabel>
      <skos:altLabel xml:lang="de">Fair</skos:altLabel>
      <skos:altLabel xml:lang="el">Fair</skos:altLabel>
      <skos:altLabel xml:lang="en">Fair</skos:altLabel>
      <skos:altLabel xml:lang="es">Fair</skos:altLabel>
      <skos:altLabel xml:lang="et">Fair</skos:altLabel>
      <skos:altLabel xml:lang="fi">Fair</skos:altLabel>
      <skos:altLabel xml:lang="fr">Fair</skos:altLabel>
      <skos:altLabel xml:lang="ga">Fair</skos:altLabel>
      <skos:altLabel xml:lang="hr">Fair</skos:altLabel>
      <skos:altLabel xml:lang="hu">Fair</skos:altLabel>
      <skos:altLabel xml:lang="it">Fair</skos:altLabel>
      <skos:altLabel xml:lang="lt">Fair</skos:altLabel>
      <skos:altLabel xml:lang="lv">Fair</skos:altLabel>
      <skos:altLabel xml:lang="mt">Fair</skos:altLabel>
      <skos:altLabel xml:lang="nl">Fair</skos:altLabel>
      <skos:altLabel xml:lang="pl">Fair</skos:altLabel>
      <skos:altLabel xml:lang="pt">Fair</skos:altLabel>
      <skos:altLabel xml:lang="ro">Fair</skos:altLabel>
      <skos:altLabel xml:lang="sk">Fair</skos:altLabel>
      <skos:altLabel xml:lang="sl">Fair</skos:altLabel>
      <skos:altLabel xml:lang="sv">Fair</skos:altLabel>
      <skos:changeNote xml:lang="en">The source of the start-use date: https://en.wikipedia.org/wiki/Fair_License</skos:changeNote>
      <skos:definition xml:lang="en">Fair is a permissive free software licence approved by the Open Source Initiative. It gives complete freedom to use the given works, as long as this licence is included and a warranty is not placed.</skos:definition>
      <skos:exactMatch rdf:resource="https://opensource.org/licenses/Fair"/>
      <skos:inScheme rdf:resource="http://publications.europa.eu/resource/authority/licence"/>
      <skos:topConceptOf rdf:resource="http://publications.europa.eu/resource/authority/licence"/>
   </skos:Concept>
   <skos:Concept rdf:about="http://publications.europa.eu/resource/authority/licence/FRAMEWORX_1_0"
                 at:deprecated="false">
      <skos:prefLabel xml:lang="en">Frameworx License 1.0 (Frameworx-1.0)</skos:prefLabel>
      <at:authority-code>FRAMEWORX_1_0</at:authority-code>
      <at:op-code>FRAMEWORX_1_0</at:op-code>
      <at:start.use>2003-07-01</at:start.use>
      <atold:op-code>FRAMEWORX_1_0</atold:op-code>
      <dc:identifier>FRAMEWORX_1_0</dc:identifier>
      <skos:altLabel xml:lang="bg">Frameworx-1.0</skos:altLabel>
      <skos:altLabel xml:lang="cs">Frameworx-1.0</skos:altLabel>
      <skos:altLabel xml:lang="da">Frameworx-1.0</skos:altLabel>
      <skos:altLabel xml:lang="de">Frameworx-1.0</skos:altLabel>
      <skos:altLabel xml:lang="el">Frameworx-1.0</skos:altLabel>
      <skos:altLabel xml:lang="en">Frameworx-1.0</skos:altLabel>
      <skos:altLabel xml:lang="es">Frameworx-1.0</skos:altLabel>
      <skos:altLabel xml:lang="et">Frameworx-1.0</skos:altLabel>
      <skos:altLabel xml:lang="fi">Frameworx-1.0</skos:altLabel>
      <skos:altLabel xml:lang="fr">Frameworx-1.0</skos:altLabel>
      <skos:altLabel xml:lang="ga">Frameworx-1.0</skos:altLabel>
      <skos:altLabel xml:lang="hr">Frameworx-1.0</skos:altLabel>
      <skos:altLabel xml:lang="hu">Frameworx-1.0</skos:altLabel>
      <skos:altLabel xml:lang="it">Frameworx-1.0</skos:altLabel>
      <skos:altLabel xml:lang="lt">Frameworx-1.0</skos:altLabel>
      <skos:altLabel xml:lang="lv">Frameworx-1.0</skos:altLabel>
      <skos:altLabel xml:lang="mt">Frameworx-1.0</skos:altLabel>
      <skos:altLabel xml:lang="nl">Frameworx-1.0</skos:altLabel>
      <skos:altLabel xml:lang="pl">Frameworx-1.0</skos:altLabel>
      <skos:altLabel xml:lang="pt">Frameworx-1.0</skos:altLabel>
      <skos:altLabel xml:lang="ro">Frameworx-1.0</skos:altLabel>
      <skos:altLabel xml:lang="sk">Frameworx-1.0</skos:altLabel>
      <skos:altLabel xml:lang="sl">Frameworx-1.0</skos:altLabel>
      <skos:altLabel xml:lang="sv">Frameworx-1.0</skos:altLabel>
      <skos:changeNote xml:lang="en">The source of the start-use date: https://enterprise.dejacode.com/licenses/public/frameworx-1.0/?_list_filters=q%3Dframeworx#essentials</skos:changeNote>
      <skos:definition xml:lang="en">Frameworx-1.0 is a copyleft-style, free software licence approved by the Open Source Initiative.</skos:definition>
      <skos:exactMatch rdf:resource="https://opensource.org/licenses/Frameworx-1.0"/>
      <skos:inScheme rdf:resource="http://publications.europa.eu/resource/authority/licence"/>
      <skos:topConceptOf rdf:resource="http://publications.europa.eu/resource/authority/licence"/>
   </skos:Concept>
   <skos:Concept rdf:about="http://publications.europa.eu/resource/authority/licence/GNU_FDL"
                 at:deprecated="true">
      <skos:prefLabel xml:lang="en">GNU Free Documentation License</skos:prefLabel>
      <at:authority-code>GNU_FDL</at:authority-code>
      <at:op-code>GNU_FDL</at:op-code>
      <at:start.use>2008-11-03</at:start.use>
      <atold:op-code>GNU_FDL</atold:op-code>
      <dc:identifier>GNU_FDL</dc:identifier>
      <skos:altLabel xml:lang="bg">GFDL</skos:altLabel>
      <skos:altLabel xml:lang="cs">GFDL</skos:altLabel>
      <skos:altLabel xml:lang="da">GFDL</skos:altLabel>
      <skos:altLabel xml:lang="de">GFDL</skos:altLabel>
      <skos:altLabel xml:lang="el">GFDL</skos:altLabel>
      <skos:altLabel xml:lang="en">GFDL</skos:altLabel>
      <skos:altLabel xml:lang="es">GFDL</skos:altLabel>
      <skos:altLabel xml:lang="et">GFDL</skos:altLabel>
      <skos:altLabel xml:lang="fi">GFDL</skos:altLabel>
      <skos:altLabel xml:lang="fr">GFDL</skos:altLabel>
      <skos:altLabel xml:lang="ga">GFDL</skos:altLabel>
      <skos:altLabel xml:lang="hr">GFDL</skos:altLabel>
      <skos:altLabel xml:lang="hu">GFDL</skos:altLabel>
      <skos:altLabel xml:lang="it">GFDL</skos:altLabel>
      <skos:altLabel xml:lang="lt">GFDL</skos:altLabel>
      <skos:altLabel xml:lang="lv">GFDL</skos:altLabel>
      <skos:altLabel xml:lang="mt">GFDL</skos:altLabel>
      <skos:altLabel xml:lang="nl">GFDL</skos:altLabel>
      <skos:altLabel xml:lang="pl">GFDL</skos:altLabel>
      <skos:altLabel xml:lang="pt">GFDL</skos:altLabel>
      <skos:altLabel xml:lang="ro">GFDL</skos:altLabel>
      <skos:altLabel xml:lang="sk">GFDL</skos:altLabel>
      <skos:altLabel xml:lang="sl">GFDL</skos:altLabel>
      <skos:altLabel xml:lang="sv">GFDL</skos:altLabel>
      <skos:definition xml:lang="en">GNU Free Documentation License is a form of copyleft intended for use on a manual, textbook or other document to assure everyone the effective freedom to copy and redistribute it, with or without modifications, either commercially or non-commercially.</skos:definition>
      <skos:definition xml:lang="fr">GNU Free Documentation License est une forme de copyleft destinée aux manuels, aux livres scolaires et autres documents. Son objectif est de garantir à tous la possibilité effective de copier et de redistribuer librement le document avec ou sans modification, et que ce soit ou non dans un but commercial.</skos:definition>
      <skos:exactMatch rdf:resource="http://www.gnu.org/licenses/licenses.html"/>
      <skos:inScheme rdf:resource="http://publications.europa.eu/resource/authority/licence"/>
      <skos:topConceptOf rdf:resource="http://publications.europa.eu/resource/authority/licence"/>
      <at:end.use>2008-11-04</at:end.use>
   </skos:Concept>
   <skos:Concept rdf:about="http://publications.europa.eu/resource/authority/licence/GNU_FDL_1_1"
                 at:deprecated="true">
      <skos:prefLabel xml:lang="en">GNU Free Documentation License 1.1</skos:prefLabel>
      <at:authority-code>GNU_FDL_1_1</at:authority-code>
      <at:op-code>GNU_FDL_1_1</at:op-code>
      <at:start.use>2000-03-01</at:start.use>
      <atold:op-code>GNU_FDL_1_1</atold:op-code>
      <dc:identifier>GNU_FDL_1_1</dc:identifier>
      <skos:altLabel xml:lang="bg">GNU FDL 1.1</skos:altLabel>
      <skos:altLabel xml:lang="cs">GNU FDL 1.1</skos:altLabel>
      <skos:altLabel xml:lang="da">GNU FDL 1.1</skos:altLabel>
      <skos:altLabel xml:lang="de">GNU FDL 1.1</skos:altLabel>
      <skos:altLabel xml:lang="el">GNU FDL 1.1</skos:altLabel>
      <skos:altLabel xml:lang="en">GNU FDL 1.1</skos:altLabel>
      <skos:altLabel xml:lang="es">GNU FDL 1.1</skos:altLabel>
      <skos:altLabel xml:lang="et">GNU FDL 1.1</skos:altLabel>
      <skos:altLabel xml:lang="fi">GNU FDL 1.1</skos:altLabel>
      <skos:altLabel xml:lang="fr">GNU FDL 1.1</skos:altLabel>
      <skos:altLabel xml:lang="ga">GNU FDL 1.1</skos:altLabel>
      <skos:altLabel xml:lang="hr">GNU FDL 1.1</skos:altLabel>
      <skos:altLabel xml:lang="hu">GNU FDL 1.1</skos:altLabel>
      <skos:altLabel xml:lang="it">GNU FDL 1.1</skos:altLabel>
      <skos:altLabel xml:lang="lt">GNU FDL 1.1</skos:altLabel>
      <skos:altLabel xml:lang="lv">GNU FDL 1.1</skos:altLabel>
      <skos:altLabel xml:lang="mt">GNU FDL 1.1</skos:altLabel>
      <skos:altLabel xml:lang="nl">GNU FDL 1.1</skos:altLabel>
      <skos:altLabel xml:lang="pl">GNU FDL 1.1</skos:altLabel>
      <skos:altLabel xml:lang="pt">GNU FDL 1.1</skos:altLabel>
      <skos:altLabel xml:lang="ro">GNU FDL 1.1</skos:altLabel>
      <skos:altLabel xml:lang="sk">GNU FDL 1.1</skos:altLabel>
      <skos:altLabel xml:lang="sl">GNU FDL 1.1</skos:altLabel>
      <skos:altLabel xml:lang="sv">GNU FDL 1.1</skos:altLabel>
      <skos:changeNote xml:lang="en">The source of the start-use date: https://www.gnu.org/licenses/old-licenses/fdl-1.1</skos:changeNote>
      <skos:definition xml:lang="en">GNU FDL 1.1 is a form of copyleft intended for use on a manual, textbook or other document to assure everyone the effective freedom to copy and redistribute it, with or without modifications, either commercially or non-commercially.</skos:definition>
      <skos:exactMatch rdf:resource="https://gnu.org/licenses/old-licenses/fdl-1.1"/>
      <skos:inScheme rdf:resource="http://publications.europa.eu/resource/authority/licence"/>
      <skos:topConceptOf rdf:resource="http://publications.europa.eu/resource/authority/licence"/>
      <at:end.use>2007-06-28</at:end.use>
   </skos:Concept>
   <skos:Concept rdf:about="http://publications.europa.eu/resource/authority/licence/GNU_FDL_1_2"
                 at:deprecated="true">
      <skos:prefLabel xml:lang="en">GNU Free Documentation License 1.2</skos:prefLabel>
      <at:authority-code>GNU_FDL_1_2</at:authority-code>
      <at:op-code>GNU_FDL_1_2</at:op-code>
      <at:start.use>2002-11-01</at:start.use>
      <atold:op-code>GNU_FDL_1_2</atold:op-code>
      <dc:identifier>GNU_FDL_1_2</dc:identifier>
      <skos:altLabel xml:lang="bg">GNU FDL 1.2</skos:altLabel>
      <skos:altLabel xml:lang="cs">GNU FDL 1.2</skos:altLabel>
      <skos:altLabel xml:lang="da">GNU FDL 1.2</skos:altLabel>
      <skos:altLabel xml:lang="de">GNU FDL 1.2</skos:altLabel>
      <skos:altLabel xml:lang="el">GNU FDL 1.2</skos:altLabel>
      <skos:altLabel xml:lang="en">GNU FDL 1.2</skos:altLabel>
      <skos:altLabel xml:lang="es">GNU FDL 1.2</skos:altLabel>
      <skos:altLabel xml:lang="et">GNU FDL 1.2</skos:altLabel>
      <skos:altLabel xml:lang="fi">GNU FDL 1.2</skos:altLabel>
      <skos:altLabel xml:lang="fr">GNU FDL 1.2</skos:altLabel>
      <skos:altLabel xml:lang="ga">GNU FDL 1.2</skos:altLabel>
      <skos:altLabel xml:lang="hr">GNU FDL 1.2</skos:altLabel>
      <skos:altLabel xml:lang="hu">GNU FDL 1.2</skos:altLabel>
      <skos:altLabel xml:lang="it">GNU FDL 1.2</skos:altLabel>
      <skos:altLabel xml:lang="lt">GNU FDL 1.2</skos:altLabel>
      <skos:altLabel xml:lang="lv">GNU FDL 1.2</skos:altLabel>
      <skos:altLabel xml:lang="mt">GNU FDL 1.2</skos:altLabel>
      <skos:altLabel xml:lang="nl">GNU FDL 1.2</skos:altLabel>
      <skos:altLabel xml:lang="pl">GNU FDL 1.2</skos:altLabel>
      <skos:altLabel xml:lang="pt">GNU FDL 1.2</skos:altLabel>
      <skos:altLabel xml:lang="ro">GNU FDL 1.2</skos:altLabel>
      <skos:altLabel xml:lang="sk">GNU FDL 1.2</skos:altLabel>
      <skos:altLabel xml:lang="sl">GNU FDL 1.2</skos:altLabel>
      <skos:altLabel xml:lang="sv">GNU FDL 1.2</skos:altLabel>
      <skos:changeNote xml:lang="en">The source of the start-use date: https://www.gnu.org/licenses/old-licenses/fdl-1.2</skos:changeNote>
      <skos:definition xml:lang="en">GNU FDL 1.2 is a form of copyleft intended for use on a manual, textbook or other document to assure everyone the effective freedom to copy and redistribute it, with or without modifications, either commercially or non-commercially.</skos:definition>
      <skos:exactMatch rdf:resource="ttps://gnu.org/licenses/old-licenses/fdl-1.2"/>
      <skos:inScheme rdf:resource="http://publications.europa.eu/resource/authority/licence"/>
      <skos:topConceptOf rdf:resource="http://publications.europa.eu/resource/authority/licence"/>
      <at:end.use>2007-06-28</at:end.use>
   </skos:Concept>
   <skos:Concept rdf:about="http://publications.europa.eu/resource/authority/licence/GNU_FDL_1_3"
                 at:deprecated="false">
      <skos:prefLabel xml:lang="en">GNU Free Documentation License 1.3</skos:prefLabel>
      <at:authority-code>GNU_FDL_1_3</at:authority-code>
      <at:op-code>GNU_FDL_1_3</at:op-code>
      <at:start.use>2008-11-04</at:start.use>
      <atold:op-code>GNU_FDL_1_3</atold:op-code>
      <dc:identifier>GNU_FDL_1_3</dc:identifier>
      <skos:altLabel xml:lang="bg">GFDL-1.3</skos:altLabel>
      <skos:altLabel xml:lang="bg">GNU FDL 1.3</skos:altLabel>
      <skos:altLabel xml:lang="cs">GFDL-1.3</skos:altLabel>
      <skos:altLabel xml:lang="cs">GNU FDL 1.3</skos:altLabel>
      <skos:altLabel xml:lang="da">GFDL-1.3</skos:altLabel>
      <skos:altLabel xml:lang="da">GNU FDL 1.3</skos:altLabel>
      <skos:altLabel xml:lang="de">GFDL-1.3</skos:altLabel>
      <skos:altLabel xml:lang="de">GNU FDL 1.3</skos:altLabel>
      <skos:altLabel xml:lang="el">GFDL-1.3</skos:altLabel>
      <skos:altLabel xml:lang="el">GNU FDL 1.3</skos:altLabel>
      <skos:altLabel xml:lang="en">GFDL-1.3</skos:altLabel>
      <skos:altLabel xml:lang="en">GNU FDL 1.3</skos:altLabel>
      <skos:altLabel xml:lang="es">GFDL-1.3</skos:altLabel>
      <skos:altLabel xml:lang="es">GNU FDL 1.3</skos:altLabel>
      <skos:altLabel xml:lang="et">GFDL-1.3</skos:altLabel>
      <skos:altLabel xml:lang="et">GNU FDL 1.3</skos:altLabel>
      <skos:altLabel xml:lang="fi">GFDL-1.3</skos:altLabel>
      <skos:altLabel xml:lang="fi">GNU FDL 1.3</skos:altLabel>
      <skos:altLabel xml:lang="fr">GFDL-1.3</skos:altLabel>
      <skos:altLabel xml:lang="fr">GNU FDL 1.3</skos:altLabel>
      <skos:altLabel xml:lang="ga">GFDL-1.3</skos:altLabel>
      <skos:altLabel xml:lang="ga">GNU FDL 1.3</skos:altLabel>
      <skos:altLabel xml:lang="hr">GFDL-1.3</skos:altLabel>
      <skos:altLabel xml:lang="hr">GNU FDL 1.3</skos:altLabel>
      <skos:altLabel xml:lang="hu">GFDL-1.3</skos:altLabel>
      <skos:altLabel xml:lang="hu">GNU FDL 1.3</skos:altLabel>
      <skos:altLabel xml:lang="it">GFDL-1.3</skos:altLabel>
      <skos:altLabel xml:lang="it">GNU FDL 1.3</skos:altLabel>
      <skos:altLabel xml:lang="lt">GFDL-1.3</skos:altLabel>
      <skos:altLabel xml:lang="lt">GNU FDL 1.3</skos:altLabel>
      <skos:altLabel xml:lang="lv">GFDL-1.3</skos:altLabel>
      <skos:altLabel xml:lang="lv">GNU FDL 1.3</skos:altLabel>
      <skos:altLabel xml:lang="mt">GFDL-1.3</skos:altLabel>
      <skos:altLabel xml:lang="mt">GNU FDL 1.3</skos:altLabel>
      <skos:altLabel xml:lang="nl">GFDL-1.3</skos:altLabel>
      <skos:altLabel xml:lang="nl">GNU FDL 1.3</skos:altLabel>
      <skos:altLabel xml:lang="pl">GFDL-1.3</skos:altLabel>
      <skos:altLabel xml:lang="pl">GNU FDL 1.3</skos:altLabel>
      <skos:altLabel xml:lang="pt">GFDL-1.3</skos:altLabel>
      <skos:altLabel xml:lang="pt">GNU FDL 1.3</skos:altLabel>
      <skos:altLabel xml:lang="ro">GFDL-1.3</skos:altLabel>
      <skos:altLabel xml:lang="ro">GNU FDL 1.3</skos:altLabel>
      <skos:altLabel xml:lang="sk">GFDL-1.3</skos:altLabel>
      <skos:altLabel xml:lang="sk">GNU FDL 1.3</skos:altLabel>
      <skos:altLabel xml:lang="sl">GFDL-1.3</skos:altLabel>
      <skos:altLabel xml:lang="sl">GNU FDL 1.3</skos:altLabel>
      <skos:altLabel xml:lang="sv">GFDL-1.3</skos:altLabel>
      <skos:altLabel xml:lang="sv">GNU FDL 1.3</skos:altLabel>
      <skos:changeNote xml:lang="en">The source of the start-use date: https://www.gnu.org/licenses/fdl-1.3.html</skos:changeNote>
      <skos:definition xml:lang="en">GNU FDL 1.3 is a form of copyleft intended for use on a manual, textbook or other document to assure everyone the effective freedom to copy and redistribute it, with or without modifications, either commercially or non-commercially.</skos:definition>
      <skos:exactMatch rdf:resource="http://www.gnu.org/licenses/licenses.html"/>
      <skos:inScheme rdf:resource="http://publications.europa.eu/resource/authority/licence"/>
      <skos:topConceptOf rdf:resource="http://publications.europa.eu/resource/authority/licence"/>
   </skos:Concept>
   <skos:Concept rdf:about="http://publications.europa.eu/resource/authority/licence/GPL_2_0"
                 at:deprecated="false">
      <skos:prefLabel xml:lang="en">GNU General Public License version 2</skos:prefLabel>
      <skos:prefLabel xml:lang="et">GNU üldine vaba kasutuse litsents versioon 2</skos:prefLabel>
      <at:authority-code>GPL_2_0</at:authority-code>
      <at:op-code>GPL_2_0</at:op-code>
      <at:start.use>1991-06-02</at:start.use>
      <atold:op-code>GPL_2_0</atold:op-code>
      <dc:identifier>GPL_2_0</dc:identifier>
      <skos:altLabel xml:lang="bg">GPL-2.0</skos:altLabel>
      <skos:altLabel xml:lang="cs">GPL-2.0</skos:altLabel>
      <skos:altLabel xml:lang="da">GPL-2.0</skos:altLabel>
      <skos:altLabel xml:lang="de">GPL-2.0</skos:altLabel>
      <skos:altLabel xml:lang="el">GPL-2.0</skos:altLabel>
      <skos:altLabel xml:lang="en">GPL-2.0</skos:altLabel>
      <skos:altLabel xml:lang="es">GPL-2.0</skos:altLabel>
      <skos:altLabel xml:lang="et">GPL-2.0</skos:altLabel>
      <skos:altLabel xml:lang="fi">GPL-2.0</skos:altLabel>
      <skos:altLabel xml:lang="fr">GPL-2.0</skos:altLabel>
      <skos:altLabel xml:lang="ga">GPL-2.0</skos:altLabel>
      <skos:altLabel xml:lang="hr">GPL-2.0</skos:altLabel>
      <skos:altLabel xml:lang="hu">GPL-2.0</skos:altLabel>
      <skos:altLabel xml:lang="it">GPL-2.0</skos:altLabel>
      <skos:altLabel xml:lang="lt">GPL-2.0</skos:altLabel>
      <skos:altLabel xml:lang="lv">GPL-2.0</skos:altLabel>
      <skos:altLabel xml:lang="mt">GPL-2.0</skos:altLabel>
      <skos:altLabel xml:lang="nl">GPL-2.0</skos:altLabel>
      <skos:altLabel xml:lang="pl">GPL-2.0</skos:altLabel>
      <skos:altLabel xml:lang="pt">GPL-2.0</skos:altLabel>
      <skos:altLabel xml:lang="ro">GPL-2.0</skos:altLabel>
      <skos:altLabel xml:lang="sk">GPL-2.0</skos:altLabel>
      <skos:altLabel xml:lang="sl">GPL-2.0</skos:altLabel>
      <skos:altLabel xml:lang="sv">GPL-2.0</skos:altLabel>
      <skos:changeNote xml:lang="en">The source of the start-use date: https://spdx.org/licenses/GPL-2.0-only.html#licenseText</skos:changeNote>
      <skos:definition xml:lang="en">GPL-2.0 is the ”historical” free software licence. It is supported by the Free Software Foundation. Copy, modification and distribution are authorised, changes/dates must be traced in source files. Any derivative must also be made available under the GPL along with build and install instructions. Lack of compatibility is a known GPL-2.0 issue when a project combines multiple sources and stakeholders.</skos:definition>
      <skos:exactMatch rdf:resource="https://opensource.org/licenses/GPL-2.0"/>
      <skos:inScheme rdf:resource="http://publications.europa.eu/resource/authority/licence"/>
      <skos:topConceptOf rdf:resource="http://publications.europa.eu/resource/authority/licence"/>
   </skos:Concept>
   <skos:Concept rdf:about="http://publications.europa.eu/resource/authority/licence/GPL_3_0"
                 at:deprecated="false">
      <skos:prefLabel xml:lang="en">GNU General Public License version 3</skos:prefLabel>
      <skos:prefLabel xml:lang="et">GNU üldine vaba kasutuse litsents versioon 3</skos:prefLabel>
      <at:authority-code>GPL_3_0</at:authority-code>
      <at:op-code>GPL_3_0</at:op-code>
      <at:start.use>2007-06-29</at:start.use>
      <atold:op-code>GPL_3_0</atold:op-code>
      <dc:identifier>GPL_3_0</dc:identifier>
      <skos:altLabel xml:lang="bg">GPL-3.0</skos:altLabel>
      <skos:altLabel xml:lang="cs">GPL-3.0</skos:altLabel>
      <skos:altLabel xml:lang="da">GPL-3.0</skos:altLabel>
      <skos:altLabel xml:lang="de">GPL-3.0</skos:altLabel>
      <skos:altLabel xml:lang="el">GPL-3.0</skos:altLabel>
      <skos:altLabel xml:lang="en">GPL-3.0</skos:altLabel>
      <skos:altLabel xml:lang="es">GPL-3.0</skos:altLabel>
      <skos:altLabel xml:lang="et">GPL-3.0</skos:altLabel>
      <skos:altLabel xml:lang="fi">GPL-3.0</skos:altLabel>
      <skos:altLabel xml:lang="fr">GPL-3.0</skos:altLabel>
      <skos:altLabel xml:lang="ga">GPL-3.0</skos:altLabel>
      <skos:altLabel xml:lang="hr">GPL-3.0</skos:altLabel>
      <skos:altLabel xml:lang="hu">GPL-3.0</skos:altLabel>
      <skos:altLabel xml:lang="it">GPL-3.0</skos:altLabel>
      <skos:altLabel xml:lang="lt">GPL-3.0</skos:altLabel>
      <skos:altLabel xml:lang="lv">GPL-3.0</skos:altLabel>
      <skos:altLabel xml:lang="mt">GPL-3.0</skos:altLabel>
      <skos:altLabel xml:lang="nl">GPL-3.0</skos:altLabel>
      <skos:altLabel xml:lang="pl">GPL-3.0</skos:altLabel>
      <skos:altLabel xml:lang="pt">GPL-3.0</skos:altLabel>
      <skos:altLabel xml:lang="ro">GPL-3.0</skos:altLabel>
      <skos:altLabel xml:lang="sk">GPL-3.0</skos:altLabel>
      <skos:altLabel xml:lang="sl">GPL-3.0</skos:altLabel>
      <skos:altLabel xml:lang="sv">GPL-3.0</skos:altLabel>
      <skos:changeNote xml:lang="en">The source of the start-use date: https://www.tatanka.com/administrative/licenses/fsf_gpl_3.0_license.html</skos:changeNote>
      <skos:definition xml:lang="en">GPL-3.0 is supported by the Free Software Foundation. Under this licence, software can be copied, distributed and modified as long as changes/dates are tracked in source files. Any derivative including (i.e. via compiler) GPL-licenced code must also be made available under the GPL-3.0 along with build and install instructions.</skos:definition>
      <skos:exactMatch rdf:resource="https://opensource.org/licenses/GPL-3.0"/>
      <skos:inScheme rdf:resource="http://publications.europa.eu/resource/authority/licence"/>
      <skos:topConceptOf rdf:resource="http://publications.europa.eu/resource/authority/licence"/>
   </skos:Concept>
   <skos:Concept rdf:about="http://publications.europa.eu/resource/authority/licence/HPND"
                 at:deprecated="true">
      <skos:prefLabel xml:lang="en">Historical Permission Notice and Disclaimer (HPND)</skos:prefLabel>
      <at:authority-code>HPND</at:authority-code>
      <at:op-code>HPND</at:op-code>
      <at:start.use>2002-11-29</at:start.use>
      <atold:op-code>HPND</atold:op-code>
      <dc:identifier>HPND</dc:identifier>
      <skos:altLabel xml:lang="bg">HPND</skos:altLabel>
      <skos:altLabel xml:lang="cs">HPND</skos:altLabel>
      <skos:altLabel xml:lang="da">HPND</skos:altLabel>
      <skos:altLabel xml:lang="de">HPND</skos:altLabel>
      <skos:altLabel xml:lang="el">HPND</skos:altLabel>
      <skos:altLabel xml:lang="en">HPND</skos:altLabel>
      <skos:altLabel xml:lang="es">HPND</skos:altLabel>
      <skos:altLabel xml:lang="et">HPND</skos:altLabel>
      <skos:altLabel xml:lang="fi">HPND</skos:altLabel>
      <skos:altLabel xml:lang="fr">HPND</skos:altLabel>
      <skos:altLabel xml:lang="ga">HPND</skos:altLabel>
      <skos:altLabel xml:lang="hr">HPND</skos:altLabel>
      <skos:altLabel xml:lang="hu">HPND</skos:altLabel>
      <skos:altLabel xml:lang="it">HPND</skos:altLabel>
      <skos:altLabel xml:lang="lt">HPND</skos:altLabel>
      <skos:altLabel xml:lang="lv">HPND</skos:altLabel>
      <skos:altLabel xml:lang="mt">HPND</skos:altLabel>
      <skos:altLabel xml:lang="nl">HPND</skos:altLabel>
      <skos:altLabel xml:lang="pl">HPND</skos:altLabel>
      <skos:altLabel xml:lang="pt">HPND</skos:altLabel>
      <skos:altLabel xml:lang="ro">HPND</skos:altLabel>
      <skos:altLabel xml:lang="sk">HPND</skos:altLabel>
      <skos:altLabel xml:lang="sl">HPND</skos:altLabel>
      <skos:altLabel xml:lang="sv">HPND</skos:altLabel>
      <skos:changeNote xml:lang="en">The source of the start-use date: https://en.wikipedia.org/wiki/Historical_Permission_Notice_and_Disclaimer</skos:changeNote>
      <skos:definition xml:lang="en">Deprecated by the author, HPND is a template that provides some protection for the author. The work itself is not restricted by the permissive licence.</skos:definition>
      <skos:exactMatch rdf:resource="https://opensource.org/licenses/HPND"/>
      <skos:inScheme rdf:resource="http://publications.europa.eu/resource/authority/licence"/>
      <skos:topConceptOf rdf:resource="http://publications.europa.eu/resource/authority/licence"/>
      <at:end.use>2015-01-01</at:end.use>
      <skos:historyNote xml:lang="en">The source of the deprecation date: https://www.fsf.org/blogs/licensing/historical-permission-notice-and-disclaimer-added-to-license-list</skos:historyNote>
   </skos:Concept>
   <skos:Concept rdf:about="http://publications.europa.eu/resource/authority/licence/HROD"
                 at:deprecated="false">
      <skos:prefLabel xml:lang="en">Open Licence – The Republic of Croatia</skos:prefLabel>
      <skos:prefLabel xml:lang="hr">Objavljena hrvatska dozvola (licenca)</skos:prefLabel>
      <at:authority-code>HROD</at:authority-code>
      <at:op-code>HROD</at:op-code>
      <at:start.use>2017-07-01</at:start.use>
      <atold:op-code>HROD</atold:op-code>
      <dc:identifier>HROD</dc:identifier>
      <skos:altLabel xml:lang="bg">HR-OD</skos:altLabel>
      <skos:altLabel xml:lang="cs">HR-OD</skos:altLabel>
      <skos:altLabel xml:lang="da">HR-OD</skos:altLabel>
      <skos:altLabel xml:lang="de">HR-OD</skos:altLabel>
      <skos:altLabel xml:lang="el">HR-OD</skos:altLabel>
      <skos:altLabel xml:lang="en">HR-OD</skos:altLabel>
      <skos:altLabel xml:lang="es">HR-OD</skos:altLabel>
      <skos:altLabel xml:lang="et">HR-OD</skos:altLabel>
      <skos:altLabel xml:lang="fi">HR-OD</skos:altLabel>
      <skos:altLabel xml:lang="fr">HR-OD</skos:altLabel>
      <skos:altLabel xml:lang="ga">HR-OD</skos:altLabel>
      <skos:altLabel xml:lang="hr">HR-OD</skos:altLabel>
      <skos:altLabel xml:lang="hu">HR-OD</skos:altLabel>
      <skos:altLabel xml:lang="it">HR-OD</skos:altLabel>
      <skos:altLabel xml:lang="lt">HR-OD</skos:altLabel>
      <skos:altLabel xml:lang="lv">HR-OD</skos:altLabel>
      <skos:altLabel xml:lang="mt">HR-OD</skos:altLabel>
      <skos:altLabel xml:lang="nl">HR-OD</skos:altLabel>
      <skos:altLabel xml:lang="pl">HR-OD</skos:altLabel>
      <skos:altLabel xml:lang="pt">HR-OD</skos:altLabel>
      <skos:altLabel xml:lang="ro">HR-OD</skos:altLabel>
      <skos:altLabel xml:lang="sk">HR-OD</skos:altLabel>
      <skos:altLabel xml:lang="sl">HR-OD</skos:altLabel>
      <skos:altLabel xml:lang="sv">HR-OD</skos:altLabel>
      <skos:changeNote xml:lang="en">The source of the start-use date: https://www.pristupinfo.hr/objavljena-hrvatska-dozvola-licenca-za-otvorene-podatke/</skos:changeNote>
      <skos:definition xml:lang="en">Published by the Republic of Croatia, HR-OD grants the re-user any re-use of the Information subject to the licence, including a spatially and temporally unrestricted, free-of-charge, non-exclusive and personal right to re-use the Information under this licence.</skos:definition>
      <skos:exactMatch rdf:resource="http://data.gov.hr/open-licence-republic-croatia"/>
      <skos:inScheme rdf:resource="http://publications.europa.eu/resource/authority/licence"/>
      <skos:topConceptOf rdf:resource="http://publications.europa.eu/resource/authority/licence"/>
   </skos:Concept>
   <skos:Concept rdf:about="http://publications.europa.eu/resource/authority/licence/IODL_1_0"
                 at:deprecated="false">
      <skos:prefLabel xml:lang="en">Italian Open Data License v1.0</skos:prefLabel>
      <at:authority-code>IODL_1_0</at:authority-code>
      <at:op-code>IODL_1_0</at:op-code>
      <at:start.use>2010-10-01</at:start.use>
      <atold:op-code>IODL_1_0</atold:op-code>
      <dc:identifier>IODL_1_0</dc:identifier>
      <skos:altLabel xml:lang="bg">IODL 1.0</skos:altLabel>
      <skos:altLabel xml:lang="cs">IODL 1.0</skos:altLabel>
      <skos:altLabel xml:lang="da">IODL 1.0</skos:altLabel>
      <skos:altLabel xml:lang="de">IODL 1.0</skos:altLabel>
      <skos:altLabel xml:lang="el">IODL 1.0</skos:altLabel>
      <skos:altLabel xml:lang="en">IODL 1.0</skos:altLabel>
      <skos:altLabel xml:lang="es">IODL 1.0</skos:altLabel>
      <skos:altLabel xml:lang="et">IODL 1.0</skos:altLabel>
      <skos:altLabel xml:lang="fi">IODL 1.0</skos:altLabel>
      <skos:altLabel xml:lang="fr">IODL 1.0</skos:altLabel>
      <skos:altLabel xml:lang="ga">IODL 1.0</skos:altLabel>
      <skos:altLabel xml:lang="hr">IODL 1.0</skos:altLabel>
      <skos:altLabel xml:lang="hu">IODL 1.0</skos:altLabel>
      <skos:altLabel xml:lang="it">IODL 1.0</skos:altLabel>
      <skos:altLabel xml:lang="lt">IODL 1.0</skos:altLabel>
      <skos:altLabel xml:lang="lv">IODL 1.0</skos:altLabel>
      <skos:altLabel xml:lang="mt">IODL 1.0</skos:altLabel>
      <skos:altLabel xml:lang="nl">IODL 1.0</skos:altLabel>
      <skos:altLabel xml:lang="pl">IODL 1.0</skos:altLabel>
      <skos:altLabel xml:lang="pt">IODL 1.0</skos:altLabel>
      <skos:altLabel xml:lang="ro">IODL 1.0</skos:altLabel>
      <skos:altLabel xml:lang="sk">IODL 1.0</skos:altLabel>
      <skos:altLabel xml:lang="sl">IODL 1.0</skos:altLabel>
      <skos:altLabel xml:lang="sv">IODL 1.0</skos:altLabel>
      <skos:changeNote xml:lang="en">The source of the start-use date: https://it.wikipedia.org/wiki/Italian_Open_Data_License</skos:changeNote>
      <skos:definition xml:lang="en">Published by Italy, IODL 1.0 aims at providing the Italian public sector with a licence facilitating the re-use of public sector information. Even commercial reuse of data is allowed, as long as credit is given to the author and new creations are licenced under the identical terms. All new works based on the original work will carry the same licence, so any derivatives will also allow commercial use.</skos:definition>
      <skos:exactMatch rdf:resource="http://www.formez.it/iodl/"/>
      <skos:inScheme rdf:resource="http://publications.europa.eu/resource/authority/licence"/>
      <skos:topConceptOf rdf:resource="http://publications.europa.eu/resource/authority/licence"/>
   </skos:Concept>
   <skos:Concept rdf:about="http://publications.europa.eu/resource/authority/licence/IODL_2_0"
                 at:deprecated="false">
      <skos:prefLabel xml:lang="en">Italian Open Data License v2.0</skos:prefLabel>
      <at:authority-code>IODL_2_0</at:authority-code>
      <at:op-code>IODL_2_0</at:op-code>
      <at:start.use>2012-03-02</at:start.use>
      <atold:op-code>IODL_2_0</atold:op-code>
      <dc:identifier>IODL_2_0</dc:identifier>
      <skos:altLabel xml:lang="bg">IODL 2.0</skos:altLabel>
      <skos:altLabel xml:lang="cs">IODL 2.0</skos:altLabel>
      <skos:altLabel xml:lang="da">IODL 2.0</skos:altLabel>
      <skos:altLabel xml:lang="de">IODL 2.0</skos:altLabel>
      <skos:altLabel xml:lang="el">IODL 2.0</skos:altLabel>
      <skos:altLabel xml:lang="en">IODL 2.0</skos:altLabel>
      <skos:altLabel xml:lang="es">IODL 2.0</skos:altLabel>
      <skos:altLabel xml:lang="et">IODL 2.0</skos:altLabel>
      <skos:altLabel xml:lang="fi">IODL 2.0</skos:altLabel>
      <skos:altLabel xml:lang="fr">IODL 2.0</skos:altLabel>
      <skos:altLabel xml:lang="ga">IODL 2.0</skos:altLabel>
      <skos:altLabel xml:lang="hr">IODL 2.0</skos:altLabel>
      <skos:altLabel xml:lang="hu">IODL 2.0</skos:altLabel>
      <skos:altLabel xml:lang="it">IODL 2.0</skos:altLabel>
      <skos:altLabel xml:lang="lt">IODL 2.0</skos:altLabel>
      <skos:altLabel xml:lang="lv">IODL 2.0</skos:altLabel>
      <skos:altLabel xml:lang="mt">IODL 2.0</skos:altLabel>
      <skos:altLabel xml:lang="nl">IODL 2.0</skos:altLabel>
      <skos:altLabel xml:lang="pl">IODL 2.0</skos:altLabel>
      <skos:altLabel xml:lang="pt">IODL 2.0</skos:altLabel>
      <skos:altLabel xml:lang="ro">IODL 2.0</skos:altLabel>
      <skos:altLabel xml:lang="sk">IODL 2.0</skos:altLabel>
      <skos:altLabel xml:lang="sl">IODL 2.0</skos:altLabel>
      <skos:altLabel xml:lang="sv">IODL 2.0</skos:altLabel>
      <skos:changeNote xml:lang="en">The source of the start-use date: https://it.wikipedia.org/wiki/Italian_Open_Data_License</skos:changeNote>
      <skos:definition xml:lang="en">Published by Italy, IODL 2.0 aims at providing the Italian public sector with a licence facilitating the re-use of public sector information. It allows distribution and building upon the author’s work, even commercially, as long as credit is given to the author for the original creation.</skos:definition>
      <skos:exactMatch rdf:resource="https://www.dati.gov.it/content/italian-open-data-license-v20"/>
      <skos:inScheme rdf:resource="http://publications.europa.eu/resource/authority/licence"/>
      <skos:topConceptOf rdf:resource="http://publications.europa.eu/resource/authority/licence"/>
   </skos:Concept>
   <skos:Concept rdf:about="http://publications.europa.eu/resource/authority/licence/IPA"
                 at:deprecated="false">
      <skos:prefLabel xml:lang="en">IPA Font License (IPA)</skos:prefLabel>
      <at:authority-code>IPA</at:authority-code>
      <at:op-code>IPA</at:op-code>
      <at:start.use>2014-09-30</at:start.use>
      <atold:op-code>IPA</atold:op-code>
      <dc:identifier>IPA</dc:identifier>
      <skos:altLabel xml:lang="bg">IPA</skos:altLabel>
      <skos:altLabel xml:lang="cs">IPA</skos:altLabel>
      <skos:altLabel xml:lang="da">IPA</skos:altLabel>
      <skos:altLabel xml:lang="de">IPA</skos:altLabel>
      <skos:altLabel xml:lang="el">IPA</skos:altLabel>
      <skos:altLabel xml:lang="en">IPA</skos:altLabel>
      <skos:altLabel xml:lang="es">IPA</skos:altLabel>
      <skos:altLabel xml:lang="et">IPA</skos:altLabel>
      <skos:altLabel xml:lang="fi">IPA</skos:altLabel>
      <skos:altLabel xml:lang="fr">IPA</skos:altLabel>
      <skos:altLabel xml:lang="ga">IPA</skos:altLabel>
      <skos:altLabel xml:lang="hr">IPA</skos:altLabel>
      <skos:altLabel xml:lang="hu">IPA</skos:altLabel>
      <skos:altLabel xml:lang="it">IPA</skos:altLabel>
      <skos:altLabel xml:lang="lt">IPA</skos:altLabel>
      <skos:altLabel xml:lang="lv">IPA</skos:altLabel>
      <skos:altLabel xml:lang="mt">IPA</skos:altLabel>
      <skos:altLabel xml:lang="nl">IPA</skos:altLabel>
      <skos:altLabel xml:lang="pl">IPA</skos:altLabel>
      <skos:altLabel xml:lang="pt">IPA</skos:altLabel>
      <skos:altLabel xml:lang="ro">IPA</skos:altLabel>
      <skos:altLabel xml:lang="sk">IPA</skos:altLabel>
      <skos:altLabel xml:lang="sl">IPA</skos:altLabel>
      <skos:altLabel xml:lang="sv">IPA</skos:altLabel>
      <skos:changeNote xml:lang="en">The source of the start-use date: https://www.fsf.org/blogs/licensing/ipa-font-license-added-to-license-list</skos:changeNote>
      <skos:definition xml:lang="en">The IPA licence applies only to font programs and allows for a great deal of freedom in distributing them, both commercially and non-commercially. The name of redistributed versions of the original software cannot be changed and must include a copy of the license.</skos:definition>
      <skos:exactMatch rdf:resource="https://opensource.org/licenses/IPA"/>
      <skos:inScheme rdf:resource="http://publications.europa.eu/resource/authority/licence"/>
      <skos:topConceptOf rdf:resource="http://publications.europa.eu/resource/authority/licence"/>
   </skos:Concept>
   <skos:Concept rdf:about="http://publications.europa.eu/resource/authority/licence/IPL_1_0"
                 at:deprecated="false">
      <skos:prefLabel xml:lang="en">IBM Public License Version 1.0 (IPL-1.0)</skos:prefLabel>
      <at:authority-code>IPL_1_0</at:authority-code>
      <at:op-code>IPL_1_0</at:op-code>
      <at:start.use>1999-08-31</at:start.use>
      <atold:op-code>IPL_1_0</atold:op-code>
      <dc:identifier>IPL_1_0</dc:identifier>
      <skos:altLabel xml:lang="bg">IPL-1.0</skos:altLabel>
      <skos:altLabel xml:lang="cs">IPL-1.0</skos:altLabel>
      <skos:altLabel xml:lang="da">IPL-1.0</skos:altLabel>
      <skos:altLabel xml:lang="de">IPL-1.0</skos:altLabel>
      <skos:altLabel xml:lang="el">IPL-1.0</skos:altLabel>
      <skos:altLabel xml:lang="en">IPL-1.0</skos:altLabel>
      <skos:altLabel xml:lang="es">IPL-1.0</skos:altLabel>
      <skos:altLabel xml:lang="et">IPL-1.0</skos:altLabel>
      <skos:altLabel xml:lang="fi">IPL-1.0</skos:altLabel>
      <skos:altLabel xml:lang="fr">IPL-1.0</skos:altLabel>
      <skos:altLabel xml:lang="ga">IPL-1.0</skos:altLabel>
      <skos:altLabel xml:lang="hr">IPL-1.0</skos:altLabel>
      <skos:altLabel xml:lang="hu">IPL-1.0</skos:altLabel>
      <skos:altLabel xml:lang="it">IPL-1.0</skos:altLabel>
      <skos:altLabel xml:lang="lt">IPL-1.0</skos:altLabel>
      <skos:altLabel xml:lang="lv">IPL-1.0</skos:altLabel>
      <skos:altLabel xml:lang="mt">IPL-1.0</skos:altLabel>
      <skos:altLabel xml:lang="nl">IPL-1.0</skos:altLabel>
      <skos:altLabel xml:lang="pl">IPL-1.0</skos:altLabel>
      <skos:altLabel xml:lang="pt">IPL-1.0</skos:altLabel>
      <skos:altLabel xml:lang="ro">IPL-1.0</skos:altLabel>
      <skos:altLabel xml:lang="sk">IPL-1.0</skos:altLabel>
      <skos:altLabel xml:lang="sl">IPL-1.0</skos:altLabel>
      <skos:altLabel xml:lang="sv">IPL-1.0</skos:altLabel>
      <skos:changeNote xml:lang="en">The source of the start-use date: https://en.wikipedia.org/wiki/IBM_Public_License</skos:changeNote>
      <skos:definition xml:lang="en">The IPL-1.0 is the open-source licence IBM uses for some of its software. Supposed to facilitate commercial use of said software, is very clear on the specifics of liability. It also grants explicit patent rights.</skos:definition>
      <skos:exactMatch rdf:resource="https://opensource.org/licenses/IPL-1.0"/>
      <skos:inScheme rdf:resource="http://publications.europa.eu/resource/authority/licence"/>
      <skos:topConceptOf rdf:resource="http://publications.europa.eu/resource/authority/licence"/>
   </skos:Concept>
   <skos:Concept rdf:about="http://publications.europa.eu/resource/authority/licence/ISA_OML"
                 at:deprecated="true">
      <skos:prefLabel xml:lang="en">ISA Open Metadata Licence 1.1</skos:prefLabel>
      <at:authority-code>ISA_OML</at:authority-code>
      <at:op-code>ISA_OML</at:op-code>
      <at:start.use>2011-01-01</at:start.use>
      <atold:op-code>ISA_OML</atold:op-code>
      <dc:identifier>ISA_OML</dc:identifier>
      <skos:altLabel xml:lang="bg">ISA OMdL 1.1</skos:altLabel>
      <skos:altLabel xml:lang="cs">ISA OMdL 1.1</skos:altLabel>
      <skos:altLabel xml:lang="da">ISA OMdL 1.1</skos:altLabel>
      <skos:altLabel xml:lang="de">ISA OMdL 1.1</skos:altLabel>
      <skos:altLabel xml:lang="el">ISA OMdL 1.1</skos:altLabel>
      <skos:altLabel xml:lang="en">ISA OMdL 1.1</skos:altLabel>
      <skos:altLabel xml:lang="en">ISA Open Metadata Licence 1.0</skos:altLabel>
      <skos:altLabel xml:lang="es">ISA OMdL 1.1</skos:altLabel>
      <skos:altLabel xml:lang="et">ISA OMdL 1.1</skos:altLabel>
      <skos:altLabel xml:lang="fi">ISA OMdL 1.1</skos:altLabel>
      <skos:altLabel xml:lang="fr">ISA OMdL 1.1</skos:altLabel>
      <skos:altLabel xml:lang="ga">ISA OMdL 1.1</skos:altLabel>
      <skos:altLabel xml:lang="hr">ISA OMdL 1.1</skos:altLabel>
      <skos:altLabel xml:lang="hu">ISA OMdL 1.1</skos:altLabel>
      <skos:altLabel xml:lang="it">ISA OMdL 1.1</skos:altLabel>
      <skos:altLabel xml:lang="lt">ISA OMdL 1.1</skos:altLabel>
      <skos:altLabel xml:lang="lv">ISA OMdL 1.1</skos:altLabel>
      <skos:altLabel xml:lang="mt">ISA OMdL 1.1</skos:altLabel>
      <skos:altLabel xml:lang="nl">ISA OMdL 1.1</skos:altLabel>
      <skos:altLabel xml:lang="pl">ISA OMdL 1.1</skos:altLabel>
      <skos:altLabel xml:lang="pt">ISA OMdL 1.1</skos:altLabel>
      <skos:altLabel xml:lang="ro">ISA OMdL 1.1</skos:altLabel>
      <skos:altLabel xml:lang="sk">ISA OMdL 1.1</skos:altLabel>
      <skos:altLabel xml:lang="sl">ISA OMdL 1.1</skos:altLabel>
      <skos:altLabel xml:lang="sv">ISA OMdL 1.1</skos:altLabel>
      <skos:definition xml:lang="en">The ISA Open metadata licence 1.1 is a permissive open licence created by the European Commission to support the publication of technical and semantic specifications. Users are allowed to distribute, copy, adapt or modify the licenced work for any commercial and non-commercial purpose with only a limited set of conditions.</skos:definition>
      <skos:exactMatch rdf:resource="https://joinup.ec.europa.eu/licence/isa-open-metadata-licence-v11"/>
      <skos:inScheme rdf:resource="http://publications.europa.eu/resource/authority/licence"/>
      <skos:topConceptOf rdf:resource="http://publications.europa.eu/resource/authority/licence"/>
      <at:end.use>2012-04-19</at:end.use>
   </skos:Concept>
   <skos:Concept rdf:about="http://publications.europa.eu/resource/authority/licence/ISA_OML_1_1"
                 at:deprecated="false">
      <skos:prefLabel xml:lang="en">ISA Open Metadata Licence 1.1</skos:prefLabel>
      <at:authority-code>ISA_OML_1_1</at:authority-code>
      <at:op-code>ISA_OML_1_1</at:op-code>
      <at:start.use>2012-04-18</at:start.use>
      <atold:op-code>ISA_OML_1_1</atold:op-code>
      <dc:identifier>ISA_OML_1_1</dc:identifier>
      <skos:altLabel xml:lang="bg">ISA OMdL 1.1</skos:altLabel>
      <skos:altLabel xml:lang="cs">ISA OMdL 1.1</skos:altLabel>
      <skos:altLabel xml:lang="da">ISA OMdL 1.1</skos:altLabel>
      <skos:altLabel xml:lang="de">ISA OMdL 1.1</skos:altLabel>
      <skos:altLabel xml:lang="el">ISA OMdL 1.1</skos:altLabel>
      <skos:altLabel xml:lang="en">ISA OMdL 1.1</skos:altLabel>
      <skos:altLabel xml:lang="es">ISA OMdL 1.1</skos:altLabel>
      <skos:altLabel xml:lang="et">ISA OMdL 1.1</skos:altLabel>
      <skos:altLabel xml:lang="fi">ISA OMdL 1.1</skos:altLabel>
      <skos:altLabel xml:lang="fr">ISA OMdL 1.1</skos:altLabel>
      <skos:altLabel xml:lang="ga">ISA OMdL 1.1</skos:altLabel>
      <skos:altLabel xml:lang="hr">ISA OMdL 1.1</skos:altLabel>
      <skos:altLabel xml:lang="hu">ISA OMdL 1.1</skos:altLabel>
      <skos:altLabel xml:lang="it">ISA OMdL 1.1</skos:altLabel>
      <skos:altLabel xml:lang="lt">ISA OMdL 1.1</skos:altLabel>
      <skos:altLabel xml:lang="lv">ISA OMdL 1.1</skos:altLabel>
      <skos:altLabel xml:lang="mt">ISA OMdL 1.1</skos:altLabel>
      <skos:altLabel xml:lang="nl">ISA OMdL 1.1</skos:altLabel>
      <skos:altLabel xml:lang="pl">ISA OMdL 1.1</skos:altLabel>
      <skos:altLabel xml:lang="pt">ISA OMdL 1.1</skos:altLabel>
      <skos:altLabel xml:lang="ro">ISA OMdL 1.1</skos:altLabel>
      <skos:altLabel xml:lang="sk">ISA OMdL 1.1</skos:altLabel>
      <skos:altLabel xml:lang="sl">ISA OMdL 1.1</skos:altLabel>
      <skos:altLabel xml:lang="sv">ISA OMdL 1.1</skos:altLabel>
      <skos:definition xml:lang="en">The ISA Open metadata licence 1.1 is a permissive open licence created by the European Commission to support the publication of technical and semantic specifications. Users are allowed to distribute, copy, adapt or modify the licenced work for any commercial and non-commercial purpose with only a limited set of conditions.</skos:definition>
      <skos:exactMatch rdf:resource="https://joinup.ec.europa.eu/licence/isa-open-metadata-licence-v11"/>
      <skos:inScheme rdf:resource="http://publications.europa.eu/resource/authority/licence"/>
      <skos:topConceptOf rdf:resource="http://publications.europa.eu/resource/authority/licence"/>
   </skos:Concept>
   <skos:Concept rdf:about="http://publications.europa.eu/resource/authority/licence/ISC"
                 at:deprecated="false">
      <skos:prefLabel xml:lang="en">ISC License (ISC)</skos:prefLabel>
      <at:authority-code>ISC</at:authority-code>
      <at:op-code>ISC</at:op-code>
      <at:start.use>1995-06-30</at:start.use>
      <atold:op-code>ISC</atold:op-code>
      <dc:identifier>ISC</dc:identifier>
      <skos:altLabel xml:lang="bg">ISC</skos:altLabel>
      <skos:altLabel xml:lang="cs">ISC</skos:altLabel>
      <skos:altLabel xml:lang="da">ISC</skos:altLabel>
      <skos:altLabel xml:lang="de">ISC</skos:altLabel>
      <skos:altLabel xml:lang="el">ISC</skos:altLabel>
      <skos:altLabel xml:lang="en">ISC</skos:altLabel>
      <skos:altLabel xml:lang="es">ISC</skos:altLabel>
      <skos:altLabel xml:lang="et">ISC</skos:altLabel>
      <skos:altLabel xml:lang="fi">ISC</skos:altLabel>
      <skos:altLabel xml:lang="fr">ISC</skos:altLabel>
      <skos:altLabel xml:lang="ga">ISC</skos:altLabel>
      <skos:altLabel xml:lang="hr">ISC</skos:altLabel>
      <skos:altLabel xml:lang="hu">ISC</skos:altLabel>
      <skos:altLabel xml:lang="it">ISC</skos:altLabel>
      <skos:altLabel xml:lang="lt">ISC</skos:altLabel>
      <skos:altLabel xml:lang="lv">ISC</skos:altLabel>
      <skos:altLabel xml:lang="mt">ISC</skos:altLabel>
      <skos:altLabel xml:lang="nl">ISC</skos:altLabel>
      <skos:altLabel xml:lang="pl">ISC</skos:altLabel>
      <skos:altLabel xml:lang="pt">ISC</skos:altLabel>
      <skos:altLabel xml:lang="ro">ISC</skos:altLabel>
      <skos:altLabel xml:lang="sk">ISC</skos:altLabel>
      <skos:altLabel xml:lang="sl">ISC</skos:altLabel>
      <skos:altLabel xml:lang="sv">ISC</skos:altLabel>
      <skos:changeNote xml:lang="en">The source of the start-use date: https://enterprise.dejacode.com/licenses/public/isc/?_list_filters=q%3Disc; https://en.wikipedia.org/wiki/ISC_license</skos:changeNote>
      <skos:definition xml:lang="en">ISC is a short and permissive software permissive licence (like MIT and BSD). Main obligation is to include the original copyright notice. For reducing licence proliferation, it is advised to use the MIT licence instead.</skos:definition>
      <skos:exactMatch rdf:resource="https://opensource.org/licenses/ISC"/>
      <skos:inScheme rdf:resource="http://publications.europa.eu/resource/authority/licence"/>
      <skos:topConceptOf rdf:resource="http://publications.europa.eu/resource/authority/licence"/>
   </skos:Concept>
   <skos:Concept rdf:about="http://publications.europa.eu/resource/authority/licence/LGPL_2_1"
                 at:deprecated="false">
      <skos:prefLabel xml:lang="en">GNU Lesser General Public License version 2.1</skos:prefLabel>
      <at:authority-code>LGPL_2_1</at:authority-code>
      <at:op-code>LGPL_2_1</at:op-code>
      <at:start.use>1999-02-15</at:start.use>
      <atold:op-code>LGPL_2_1</atold:op-code>
      <dc:identifier>LGPL_2_1</dc:identifier>
      <skos:altLabel xml:lang="bg">LGPL-2.1</skos:altLabel>
      <skos:altLabel xml:lang="cs">LGPL-2.1</skos:altLabel>
      <skos:altLabel xml:lang="da">LGPL-2.1</skos:altLabel>
      <skos:altLabel xml:lang="de">LGPL-2.1</skos:altLabel>
      <skos:altLabel xml:lang="el">LGPL-2.1</skos:altLabel>
      <skos:altLabel xml:lang="en">LGPL-2.1</skos:altLabel>
      <skos:altLabel xml:lang="es">LGPL-2.1</skos:altLabel>
      <skos:altLabel xml:lang="et">LGPL-2.1</skos:altLabel>
      <skos:altLabel xml:lang="fi">LGPL-2.1</skos:altLabel>
      <skos:altLabel xml:lang="fr">LGPL-2.1</skos:altLabel>
      <skos:altLabel xml:lang="ga">LGPL-2.1</skos:altLabel>
      <skos:altLabel xml:lang="hr">LGPL-2.1</skos:altLabel>
      <skos:altLabel xml:lang="hu">LGPL-2.1</skos:altLabel>
      <skos:altLabel xml:lang="it">LGPL-2.1</skos:altLabel>
      <skos:altLabel xml:lang="lt">LGPL-2.1</skos:altLabel>
      <skos:altLabel xml:lang="lv">LGPL-2.1</skos:altLabel>
      <skos:altLabel xml:lang="mt">LGPL-2.1</skos:altLabel>
      <skos:altLabel xml:lang="nl">LGPL-2.1</skos:altLabel>
      <skos:altLabel xml:lang="pl">LGPL-2.1</skos:altLabel>
      <skos:altLabel xml:lang="pt">LGPL-2.1</skos:altLabel>
      <skos:altLabel xml:lang="ro">LGPL-2.1</skos:altLabel>
      <skos:altLabel xml:lang="sk">LGPL-2.1</skos:altLabel>
      <skos:altLabel xml:lang="sl">LGPL-2.1</skos:altLabel>
      <skos:altLabel xml:lang="sv">LGPL-2.1</skos:altLabel>
      <skos:changeNote xml:lang="en">The source of the start-use date: https://opensource.org/licenses/LGPL-2.1</skos:changeNote>
      <skos:definition xml:lang="en">LGPL 2.1 is supported by the Free Software Foundation for libraries. Works made by using the covered software could be distributed under any licence. Distribution of derivatives (code modifications) must be done under LGPL. Reverse engineering must be allowed.</skos:definition>
      <skos:exactMatch rdf:resource="https://opensource.org/licenses/LGPL-2.1"/>
      <skos:inScheme rdf:resource="http://publications.europa.eu/resource/authority/licence"/>
      <skos:topConceptOf rdf:resource="http://publications.europa.eu/resource/authority/licence"/>
   </skos:Concept>
   <skos:Concept rdf:about="http://publications.europa.eu/resource/authority/licence/LGPL_3_0"
                 at:deprecated="false">
      <skos:prefLabel xml:lang="en">GNU Lesser General Public License version 3</skos:prefLabel>
      <at:authority-code>LGPL_3_0</at:authority-code>
      <at:op-code>LGPL_3_0</at:op-code>
      <at:start.use>2007-06-29</at:start.use>
      <atold:op-code>LGPL_3_0</atold:op-code>
      <dc:identifier>LGPL_3_0</dc:identifier>
      <skos:altLabel xml:lang="bg">LGPL-3.0</skos:altLabel>
      <skos:altLabel xml:lang="cs">LGPL-3.0</skos:altLabel>
      <skos:altLabel xml:lang="da">LGPL-3.0</skos:altLabel>
      <skos:altLabel xml:lang="de">LGPL-3.0</skos:altLabel>
      <skos:altLabel xml:lang="el">LGPL-3.0</skos:altLabel>
      <skos:altLabel xml:lang="en">LGPL-3.0</skos:altLabel>
      <skos:altLabel xml:lang="es">LGPL-3.0</skos:altLabel>
      <skos:altLabel xml:lang="et">LGPL-3.0</skos:altLabel>
      <skos:altLabel xml:lang="fi">LGPL-3.0</skos:altLabel>
      <skos:altLabel xml:lang="fr">LGPL-3.0</skos:altLabel>
      <skos:altLabel xml:lang="ga">LGPL-3.0</skos:altLabel>
      <skos:altLabel xml:lang="hr">LGPL-3.0</skos:altLabel>
      <skos:altLabel xml:lang="hu">LGPL-3.0</skos:altLabel>
      <skos:altLabel xml:lang="it">LGPL-3.0</skos:altLabel>
      <skos:altLabel xml:lang="lt">LGPL-3.0</skos:altLabel>
      <skos:altLabel xml:lang="lv">LGPL-3.0</skos:altLabel>
      <skos:altLabel xml:lang="mt">LGPL-3.0</skos:altLabel>
      <skos:altLabel xml:lang="nl">LGPL-3.0</skos:altLabel>
      <skos:altLabel xml:lang="pl">LGPL-3.0</skos:altLabel>
      <skos:altLabel xml:lang="pt">LGPL-3.0</skos:altLabel>
      <skos:altLabel xml:lang="ro">LGPL-3.0</skos:altLabel>
      <skos:altLabel xml:lang="sk">LGPL-3.0</skos:altLabel>
      <skos:altLabel xml:lang="sl">LGPL-3.0</skos:altLabel>
      <skos:altLabel xml:lang="sv">LGPL-3.0</skos:altLabel>
      <skos:changeNote xml:lang="en">The source of the start-use date: https://opensource.org/licenses/LGPL-3.0</skos:changeNote>
      <skos:definition xml:lang="en">LGPL-3.0 was produced by the Free Software Foundation for libraries. Works made by using the covered software could be distributed under any licence. Distribution of derivatives (code modifications) must be done under LGPL. Reverse engineering must be allowed.</skos:definition>
      <skos:exactMatch rdf:resource="https://opensource.org/licenses/LGPL-3.0"/>
      <skos:inScheme rdf:resource="http://publications.europa.eu/resource/authority/licence"/>
      <skos:topConceptOf rdf:resource="http://publications.europa.eu/resource/authority/licence"/>
   </skos:Concept>
   <skos:Concept rdf:about="http://publications.europa.eu/resource/authority/licence/LILIQ_P_1_1"
                 at:deprecated="false">
      <skos:prefLabel xml:lang="en">Québec Free and Open-Source Licence – Permissive (LiLiQ-P) version 1.1</skos:prefLabel>
      <skos:prefLabel xml:lang="fr">Licence Libre du Québec – Permissive (LiLiQ-P) version 1.1</skos:prefLabel>
      <at:authority-code>LILIQ_P_1_1</at:authority-code>
      <at:op-code>LILIQ_P_1_1</at:op-code>
      <at:start.use>2016-01-31</at:start.use>
      <atold:op-code>LILIQ_P_1_1</atold:op-code>
      <dc:identifier>LILIQ_P_1_1</dc:identifier>
      <skos:altLabel xml:lang="bg">LiLiQ-P-1.1</skos:altLabel>
      <skos:altLabel xml:lang="cs">LiLiQ-P-1.1</skos:altLabel>
      <skos:altLabel xml:lang="da">LiLiQ-P-1.1</skos:altLabel>
      <skos:altLabel xml:lang="de">LiLiQ-P-1.1</skos:altLabel>
      <skos:altLabel xml:lang="el">LiLiQ-P-1.1</skos:altLabel>
      <skos:altLabel xml:lang="en">LiLiQ-P-1.1</skos:altLabel>
      <skos:altLabel xml:lang="es">LiLiQ-P-1.1</skos:altLabel>
      <skos:altLabel xml:lang="et">LiLiQ-P-1.1</skos:altLabel>
      <skos:altLabel xml:lang="fi">LiLiQ-P-1.1</skos:altLabel>
      <skos:altLabel xml:lang="fr">LiLiQ-P-1.1</skos:altLabel>
      <skos:altLabel xml:lang="ga">LiLiQ-P-1.1</skos:altLabel>
      <skos:altLabel xml:lang="hr">LiLiQ-P-1.1</skos:altLabel>
      <skos:altLabel xml:lang="hu">LiLiQ-P-1.1</skos:altLabel>
      <skos:altLabel xml:lang="it">LiLiQ-P-1.1</skos:altLabel>
      <skos:altLabel xml:lang="lt">LiLiQ-P-1.1</skos:altLabel>
      <skos:altLabel xml:lang="lv">LiLiQ-P-1.1</skos:altLabel>
      <skos:altLabel xml:lang="mt">LiLiQ-P-1.1</skos:altLabel>
      <skos:altLabel xml:lang="nl">LiLiQ-P-1.1</skos:altLabel>
      <skos:altLabel xml:lang="pl">LiLiQ-P-1.1</skos:altLabel>
      <skos:altLabel xml:lang="pt">LiLiQ-P-1.1</skos:altLabel>
      <skos:altLabel xml:lang="ro">LiLiQ-P-1.1</skos:altLabel>
      <skos:altLabel xml:lang="sk">LiLiQ-P-1.1</skos:altLabel>
      <skos:altLabel xml:lang="sl">LiLiQ-P-1.1</skos:altLabel>
      <skos:altLabel xml:lang="sv">LiLiQ-P-1.1</skos:altLabel>
      <skos:changeNote xml:lang="en">The source of the start-use date: https://forge.gouv.qc.ca/licence/</skos:changeNote>
      <skos:definition xml:lang="en">Approved by the Open Source Initiative, LiLiQ-P-1.1 is a permissive licence produced by the State of Quebec (Canada).</skos:definition>
      <skos:exactMatch rdf:resource="https://opensource.org/licenses/LiLiQ-P-1.1"/>
      <skos:inScheme rdf:resource="http://publications.europa.eu/resource/authority/licence"/>
      <skos:topConceptOf rdf:resource="http://publications.europa.eu/resource/authority/licence"/>
   </skos:Concept>
   <skos:Concept rdf:about="http://publications.europa.eu/resource/authority/licence/LILIQ_RPLUS_1_1"
                 at:deprecated="false">
      <skos:prefLabel xml:lang="en">Québec Free and Open-Source Licence – Strong Reciprocity (LiLiQ-R+) version 1.1</skos:prefLabel>
      <skos:prefLabel xml:lang="fr">Licence Libre du Québec – Réciprocité forte (LiLiQ-R+) version 1.1</skos:prefLabel>
      <at:authority-code>LILIQ_RPLUS_1_1</at:authority-code>
      <at:op-code>LILIQ_RPLUS_1_1</at:op-code>
      <at:start.use>2016-01-31</at:start.use>
      <atold:op-code>LILIQ_RPLUS_1_1</atold:op-code>
      <dc:identifier>LILIQ_RPLUS_1_1</dc:identifier>
      <skos:altLabel xml:lang="bg">LiLiQ-Rplus-1.1</skos:altLabel>
      <skos:altLabel xml:lang="cs">LiLiQ-Rplus-1.1</skos:altLabel>
      <skos:altLabel xml:lang="da">LiLiQ-Rplus-1.1</skos:altLabel>
      <skos:altLabel xml:lang="de">LiLiQ-Rplus-1.1</skos:altLabel>
      <skos:altLabel xml:lang="el">LiLiQ-Rplus-1.1</skos:altLabel>
      <skos:altLabel xml:lang="en">LiLiQ-Rplus-1.1</skos:altLabel>
      <skos:altLabel xml:lang="es">LiLiQ-Rplus-1.1</skos:altLabel>
      <skos:altLabel xml:lang="et">LiLiQ-Rplus-1.1</skos:altLabel>
      <skos:altLabel xml:lang="fi">LiLiQ-Rplus-1.1</skos:altLabel>
      <skos:altLabel xml:lang="fr">LiLiQ-Rplus-1.1</skos:altLabel>
      <skos:altLabel xml:lang="ga">LiLiQ-Rplus-1.1</skos:altLabel>
      <skos:altLabel xml:lang="hr">LiLiQ-Rplus-1.1</skos:altLabel>
      <skos:altLabel xml:lang="hu">LiLiQ-Rplus-1.1</skos:altLabel>
      <skos:altLabel xml:lang="it">LiLiQ-Rplus-1.1</skos:altLabel>
      <skos:altLabel xml:lang="lt">LiLiQ-Rplus-1.1</skos:altLabel>
      <skos:altLabel xml:lang="lv">LiLiQ-Rplus-1.1</skos:altLabel>
      <skos:altLabel xml:lang="mt">LiLiQ-Rplus-1.1</skos:altLabel>
      <skos:altLabel xml:lang="nl">LiLiQ-Rplus-1.1</skos:altLabel>
      <skos:altLabel xml:lang="pl">LiLiQ-Rplus-1.1</skos:altLabel>
      <skos:altLabel xml:lang="pt">LiLiQ-Rplus-1.1</skos:altLabel>
      <skos:altLabel xml:lang="ro">LiLiQ-Rplus-1.1</skos:altLabel>
      <skos:altLabel xml:lang="sk">LiLiQ-Rplus-1.1</skos:altLabel>
      <skos:altLabel xml:lang="sl">LiLiQ-Rplus-1.1</skos:altLabel>
      <skos:altLabel xml:lang="sv">LiLiQ-Rplus-1.1</skos:altLabel>
      <skos:changeNote xml:lang="en">The source of the start-use date: https://forge.gouv.qc.ca/licence/</skos:changeNote>
      <skos:definition xml:lang="en">LiLiQ-Rplus-1.1 is a reciprocate (copyleft) licence produced by the State of Quebec (Canada). Other reciprocal licences GPL-2.0-or-later and the EUPL are expressly listed as compatible, meaning that the covered code can be reused in other projects covered by these licences. It is approved by the Open Source Initiative.</skos:definition>
      <skos:exactMatch rdf:resource="https://opensource.org/licenses/LiLiQ-Rplus-1.1"/>
      <skos:inScheme rdf:resource="http://publications.europa.eu/resource/authority/licence"/>
      <skos:topConceptOf rdf:resource="http://publications.europa.eu/resource/authority/licence"/>
   </skos:Concept>
   <skos:Concept rdf:about="http://publications.europa.eu/resource/authority/licence/LILIQ_R_1_1"
                 at:deprecated="false">
      <skos:prefLabel xml:lang="en">Québec Free and Open-Source Licence – Reciprocity (LiLiQ-R) version 1.1</skos:prefLabel>
      <skos:prefLabel xml:lang="fr">Licence Libre du Québec – Réciprocité (LiLiQ-R) version 1.1</skos:prefLabel>
      <at:authority-code>LILIQ_R_1_1</at:authority-code>
      <at:op-code>LILIQ_R_1_1</at:op-code>
      <at:start.use>2016-01-31</at:start.use>
      <atold:op-code>LILIQ_R_1_1</atold:op-code>
      <dc:identifier>LILIQ_R_1_1</dc:identifier>
      <skos:altLabel xml:lang="bg">LiLiQ-R-1.1</skos:altLabel>
      <skos:altLabel xml:lang="cs">LiLiQ-R-1.1</skos:altLabel>
      <skos:altLabel xml:lang="da">LiLiQ-R-1.1</skos:altLabel>
      <skos:altLabel xml:lang="de">LiLiQ-R-1.1</skos:altLabel>
      <skos:altLabel xml:lang="el">LiLiQ-R-1.1</skos:altLabel>
      <skos:altLabel xml:lang="en">LiLiQ-R-1.1</skos:altLabel>
      <skos:altLabel xml:lang="es">LiLiQ-R-1.1</skos:altLabel>
      <skos:altLabel xml:lang="et">LiLiQ-R-1.1</skos:altLabel>
      <skos:altLabel xml:lang="fi">LiLiQ-R-1.1</skos:altLabel>
      <skos:altLabel xml:lang="fr">LiLiQ-R-1.1</skos:altLabel>
      <skos:altLabel xml:lang="ga">LiLiQ-R-1.1</skos:altLabel>
      <skos:altLabel xml:lang="hr">LiLiQ-R-1.1</skos:altLabel>
      <skos:altLabel xml:lang="hu">LiLiQ-R-1.1</skos:altLabel>
      <skos:altLabel xml:lang="it">LiLiQ-R-1.1</skos:altLabel>
      <skos:altLabel xml:lang="lt">LiLiQ-R-1.1</skos:altLabel>
      <skos:altLabel xml:lang="lv">LiLiQ-R-1.1</skos:altLabel>
      <skos:altLabel xml:lang="mt">LiLiQ-R-1.1</skos:altLabel>
      <skos:altLabel xml:lang="nl">LiLiQ-R-1.1</skos:altLabel>
      <skos:altLabel xml:lang="pl">LiLiQ-R-1.1</skos:altLabel>
      <skos:altLabel xml:lang="pt">LiLiQ-R-1.1</skos:altLabel>
      <skos:altLabel xml:lang="ro">LiLiQ-R-1.1</skos:altLabel>
      <skos:altLabel xml:lang="sk">LiLiQ-R-1.1</skos:altLabel>
      <skos:altLabel xml:lang="sl">LiLiQ-R-1.1</skos:altLabel>
      <skos:altLabel xml:lang="sv">LiLiQ-R-1.1</skos:altLabel>
      <skos:changeNote xml:lang="en">The source of the start-use date: https://forge.gouv.qc.ca/licence/</skos:changeNote>
      <skos:definition xml:lang="en">LiLiQ-R 1.1 is a moderately reciprocate licence produced by the State of Quebec (Canada). A list of liences with similar level of reciprocity is declared compatible, including GPL, EUPL, MPL, LGPL etc., meaning that the covered code can be reused in other projects covered by these licences. It is approved by the Open Source Initiative.</skos:definition>
      <skos:exactMatch rdf:resource="https://opensource.org/licenses/LiLiQ-R-1.1"/>
      <skos:inScheme rdf:resource="http://publications.europa.eu/resource/authority/licence"/>
      <skos:topConceptOf rdf:resource="http://publications.europa.eu/resource/authority/licence"/>
   </skos:Concept>
   <skos:Concept rdf:about="http://publications.europa.eu/resource/authority/licence/LPL_1_0"
                 at:deprecated="true">
      <skos:prefLabel xml:lang="en">Lucent Public License, Plan 9, version 1.0 (LPL-1.0)</skos:prefLabel>
      <at:authority-code>LPL_1_0</at:authority-code>
      <at:op-code>LPL_1_0</at:op-code>
      <at:start.use>2003-01-01</at:start.use>
      <atold:op-code>LPL_1_0</atold:op-code>
      <dc:identifier>LPL_1_0</dc:identifier>
      <skos:altLabel xml:lang="bg">LPL-1.0</skos:altLabel>
      <skos:altLabel xml:lang="cs">LPL-1.0</skos:altLabel>
      <skos:altLabel xml:lang="da">LPL-1.0</skos:altLabel>
      <skos:altLabel xml:lang="de">LPL-1.0</skos:altLabel>
      <skos:altLabel xml:lang="el">LPL-1.0</skos:altLabel>
      <skos:altLabel xml:lang="en">LPL-1.0</skos:altLabel>
      <skos:altLabel xml:lang="es">LPL-1.0</skos:altLabel>
      <skos:altLabel xml:lang="et">LPL-1.0</skos:altLabel>
      <skos:altLabel xml:lang="fi">LPL-1.0</skos:altLabel>
      <skos:altLabel xml:lang="fr">LPL-1.0</skos:altLabel>
      <skos:altLabel xml:lang="ga">LPL-1.0</skos:altLabel>
      <skos:altLabel xml:lang="hr">LPL-1.0</skos:altLabel>
      <skos:altLabel xml:lang="hu">LPL-1.0</skos:altLabel>
      <skos:altLabel xml:lang="it">LPL-1.0</skos:altLabel>
      <skos:altLabel xml:lang="lt">LPL-1.0</skos:altLabel>
      <skos:altLabel xml:lang="lv">LPL-1.0</skos:altLabel>
      <skos:altLabel xml:lang="mt">LPL-1.0</skos:altLabel>
      <skos:altLabel xml:lang="nl">LPL-1.0</skos:altLabel>
      <skos:altLabel xml:lang="pl">LPL-1.0</skos:altLabel>
      <skos:altLabel xml:lang="pt">LPL-1.0</skos:altLabel>
      <skos:altLabel xml:lang="ro">LPL-1.0</skos:altLabel>
      <skos:altLabel xml:lang="sk">LPL-1.0</skos:altLabel>
      <skos:altLabel xml:lang="sl">LPL-1.0</skos:altLabel>
      <skos:altLabel xml:lang="sv">LPL-1.0</skos:altLabel>
      <skos:changeNote xml:lang="en">The source of the start-use date: https://enterprise.dejacode.com/licenses/public/lucent-pl-1.0/?_list_filters=q%3Dlucent</skos:changeNote>
      <skos:definition xml:lang="en">LPL-1.0 is a copyleft-style, free software licence approved by the Open Source Initiative. It is superseded by LPL-1.02.</skos:definition>
      <skos:exactMatch rdf:resource="https://opensource.org/licenses/LPL-1.0"/>
      <skos:inScheme rdf:resource="http://publications.europa.eu/resource/authority/licence"/>
      <skos:topConceptOf rdf:resource="http://publications.europa.eu/resource/authority/licence"/>
      <at:end.use>2003-06-30</at:end.use>
   </skos:Concept>
   <skos:Concept rdf:about="http://publications.europa.eu/resource/authority/licence/LPL_1_02"
                 at:deprecated="false">
      <skos:prefLabel xml:lang="en">Lucent Public License Version 1.02 (LPL-1.02)</skos:prefLabel>
      <at:authority-code>LPL_1_02</at:authority-code>
      <at:op-code>LPL_1_02</at:op-code>
      <at:start.use>2003-07-01</at:start.use>
      <atold:op-code>LPL_1_02</atold:op-code>
      <dc:identifier>LPL_1_02</dc:identifier>
      <skos:altLabel xml:lang="bg">LPL-1.02</skos:altLabel>
      <skos:altLabel xml:lang="cs">LPL-1.02</skos:altLabel>
      <skos:altLabel xml:lang="da">LPL-1.02</skos:altLabel>
      <skos:altLabel xml:lang="de">LPL-1.02</skos:altLabel>
      <skos:altLabel xml:lang="el">LPL-1.02</skos:altLabel>
      <skos:altLabel xml:lang="en">LPL-1.02</skos:altLabel>
      <skos:altLabel xml:lang="es">LPL-1.02</skos:altLabel>
      <skos:altLabel xml:lang="et">LPL-1.02</skos:altLabel>
      <skos:altLabel xml:lang="fi">LPL-1.02</skos:altLabel>
      <skos:altLabel xml:lang="fr">LPL-1.02</skos:altLabel>
      <skos:altLabel xml:lang="ga">LPL-1.02</skos:altLabel>
      <skos:altLabel xml:lang="hr">LPL-1.02</skos:altLabel>
      <skos:altLabel xml:lang="hu">LPL-1.02</skos:altLabel>
      <skos:altLabel xml:lang="it">LPL-1.02</skos:altLabel>
      <skos:altLabel xml:lang="lt">LPL-1.02</skos:altLabel>
      <skos:altLabel xml:lang="lv">LPL-1.02</skos:altLabel>
      <skos:altLabel xml:lang="mt">LPL-1.02</skos:altLabel>
      <skos:altLabel xml:lang="nl">LPL-1.02</skos:altLabel>
      <skos:altLabel xml:lang="pl">LPL-1.02</skos:altLabel>
      <skos:altLabel xml:lang="pt">LPL-1.02</skos:altLabel>
      <skos:altLabel xml:lang="ro">LPL-1.02</skos:altLabel>
      <skos:altLabel xml:lang="sk">LPL-1.02</skos:altLabel>
      <skos:altLabel xml:lang="sl">LPL-1.02</skos:altLabel>
      <skos:altLabel xml:lang="sv">LPL-1.02</skos:altLabel>
      <skos:changeNote xml:lang="en">The source of the start-use date: https://enterprise.dejacode.com/licenses/public/lucent-pl-1.02/?_list_filters=q%3Dlucent</skos:changeNote>
      <skos:definition xml:lang="en">LPL-1.02 is a copyleft-style, free software licence approved by the Open Source Initiative. Similar to the Common Public License, this licence makes liability rules very clear.</skos:definition>
      <skos:exactMatch rdf:resource="https://opensource.org/licenses/LPL-1.02"/>
      <skos:inScheme rdf:resource="http://publications.europa.eu/resource/authority/licence"/>
      <skos:topConceptOf rdf:resource="http://publications.europa.eu/resource/authority/licence"/>
   </skos:Concept>
   <skos:Concept rdf:about="http://publications.europa.eu/resource/authority/licence/LPPL_1_3C"
                 at:deprecated="false">
      <skos:prefLabel xml:lang="en">LaTeX Project Public License v1.3c (LPPL-1.3c)</skos:prefLabel>
      <at:authority-code>LPPL_1_3C</at:authority-code>
      <at:op-code>LPPL_1_3C</at:op-code>
      <at:start.use>2008-05-04</at:start.use>
      <atold:op-code>LPPL_1_3C</atold:op-code>
      <dc:identifier>LPPL_1_3C</dc:identifier>
      <skos:altLabel xml:lang="bg">LPPL-1.3c</skos:altLabel>
      <skos:altLabel xml:lang="cs">LPPL-1.3c</skos:altLabel>
      <skos:altLabel xml:lang="da">LPPL-1.3c</skos:altLabel>
      <skos:altLabel xml:lang="de">LPPL-1.3c</skos:altLabel>
      <skos:altLabel xml:lang="el">LPPL-1.3c</skos:altLabel>
      <skos:altLabel xml:lang="en">LPPL-1.3c</skos:altLabel>
      <skos:altLabel xml:lang="es">LPPL-1.3c</skos:altLabel>
      <skos:altLabel xml:lang="et">LPPL-1.3c</skos:altLabel>
      <skos:altLabel xml:lang="fi">LPPL-1.3c</skos:altLabel>
      <skos:altLabel xml:lang="fr">LPPL-1.3c</skos:altLabel>
      <skos:altLabel xml:lang="ga">LPPL-1.3c</skos:altLabel>
      <skos:altLabel xml:lang="hr">LPPL-1.3c</skos:altLabel>
      <skos:altLabel xml:lang="hu">LPPL-1.3c</skos:altLabel>
      <skos:altLabel xml:lang="it">LPPL-1.3c</skos:altLabel>
      <skos:altLabel xml:lang="lt">LPPL-1.3c</skos:altLabel>
      <skos:altLabel xml:lang="lv">LPPL-1.3c</skos:altLabel>
      <skos:altLabel xml:lang="mt">LPPL-1.3c</skos:altLabel>
      <skos:altLabel xml:lang="nl">LPPL-1.3c</skos:altLabel>
      <skos:altLabel xml:lang="pl">LPPL-1.3c</skos:altLabel>
      <skos:altLabel xml:lang="pt">LPPL-1.3c</skos:altLabel>
      <skos:altLabel xml:lang="ro">LPPL-1.3c</skos:altLabel>
      <skos:altLabel xml:lang="sk">LPPL-1.3c</skos:altLabel>
      <skos:altLabel xml:lang="sl">LPPL-1.3c</skos:altLabel>
      <skos:altLabel xml:lang="sv">LPPL-1.3c</skos:altLabel>
      <skos:changeNote xml:lang="en">The source of the start-use date: https://en.wikipedia.org/wiki/LaTeX_Project_Public_License</skos:changeNote>
      <skos:definition xml:lang="en">LPPL-1.3c is a very specific, non-copyleft licence. It organises rights of the ”maintainer” of a work V/S other distributors who have to comply with documentation requirements and to communicate the original code (or report where it can be available).</skos:definition>
      <skos:exactMatch rdf:resource="https://opensource.org/licenses/LPPL-1.3c"/>
      <skos:inScheme rdf:resource="http://publications.europa.eu/resource/authority/licence"/>
      <skos:topConceptOf rdf:resource="http://publications.europa.eu/resource/authority/licence"/>
   </skos:Concept>
   <skos:Concept rdf:about="http://publications.europa.eu/resource/authority/licence/MIROS"
                 at:deprecated="false">
      <skos:prefLabel xml:lang="en">MirOS License (MirOS)</skos:prefLabel>
      <at:authority-code>MIROS</at:authority-code>
      <at:op-code>MIROS</at:op-code>
      <at:start.use>2006-12-11</at:start.use>
      <atold:op-code>MIROS</atold:op-code>
      <dc:identifier>MIROS</dc:identifier>
      <skos:altLabel xml:lang="bg">MirOS</skos:altLabel>
      <skos:altLabel xml:lang="cs">MirOS</skos:altLabel>
      <skos:altLabel xml:lang="da">MirOS</skos:altLabel>
      <skos:altLabel xml:lang="de">MirOS</skos:altLabel>
      <skos:altLabel xml:lang="el">MirOS</skos:altLabel>
      <skos:altLabel xml:lang="en">MirOS</skos:altLabel>
      <skos:altLabel xml:lang="es">MirOS</skos:altLabel>
      <skos:altLabel xml:lang="et">MirOS</skos:altLabel>
      <skos:altLabel xml:lang="fi">MirOS</skos:altLabel>
      <skos:altLabel xml:lang="fr">MirOS</skos:altLabel>
      <skos:altLabel xml:lang="ga">MirOS</skos:altLabel>
      <skos:altLabel xml:lang="hr">MirOS</skos:altLabel>
      <skos:altLabel xml:lang="hu">MirOS</skos:altLabel>
      <skos:altLabel xml:lang="it">MirOS</skos:altLabel>
      <skos:altLabel xml:lang="lt">MirOS</skos:altLabel>
      <skos:altLabel xml:lang="lv">MirOS</skos:altLabel>
      <skos:altLabel xml:lang="mt">MirOS</skos:altLabel>
      <skos:altLabel xml:lang="nl">MirOS</skos:altLabel>
      <skos:altLabel xml:lang="pl">MirOS</skos:altLabel>
      <skos:altLabel xml:lang="pt">MirOS</skos:altLabel>
      <skos:altLabel xml:lang="ro">MirOS</skos:altLabel>
      <skos:altLabel xml:lang="sk">MirOS</skos:altLabel>
      <skos:altLabel xml:lang="sl">MirOS</skos:altLabel>
      <skos:altLabel xml:lang="sv">MirOS</skos:altLabel>
      <skos:changeNote xml:lang="en">The source of the start-use date: https://en.wikipedia.org/wiki/MirOS_Licence</skos:changeNote>
      <skos:definition xml:lang="en">MirOS is a BSD-style, permissive free software licence approved by the Open Source Initiative.</skos:definition>
      <skos:exactMatch rdf:resource="https://opensource.org/licenses/MS-RL"/>
      <skos:inScheme rdf:resource="http://publications.europa.eu/resource/authority/licence"/>
      <skos:topConceptOf rdf:resource="http://publications.europa.eu/resource/authority/licence"/>
   </skos:Concept>
   <skos:Concept rdf:about="http://publications.europa.eu/resource/authority/licence/MIT"
                 at:deprecated="false">
      <skos:prefLabel xml:lang="en">The MIT License</skos:prefLabel>
      <skos:prefLabel xml:lang="et">MIT litsents</skos:prefLabel>
      <at:authority-code>MIT</at:authority-code>
      <at:op-code>MIT</at:op-code>
      <at:start.use>1988-08-14</at:start.use>
      <atold:op-code>MIT</atold:op-code>
      <dc:identifier>MIT</dc:identifier>
      <skos:altLabel xml:lang="bg">MIT</skos:altLabel>
      <skos:altLabel xml:lang="cs">MIT</skos:altLabel>
      <skos:altLabel xml:lang="da">MIT</skos:altLabel>
      <skos:altLabel xml:lang="de">MIT</skos:altLabel>
      <skos:altLabel xml:lang="el">MIT</skos:altLabel>
      <skos:altLabel xml:lang="en">MIT</skos:altLabel>
      <skos:altLabel xml:lang="es">MIT</skos:altLabel>
      <skos:altLabel xml:lang="et">MIT</skos:altLabel>
      <skos:altLabel xml:lang="fi">MIT</skos:altLabel>
      <skos:altLabel xml:lang="fr">MIT</skos:altLabel>
      <skos:altLabel xml:lang="ga">MIT</skos:altLabel>
      <skos:altLabel xml:lang="hr">MIT</skos:altLabel>
      <skos:altLabel xml:lang="hu">MIT</skos:altLabel>
      <skos:altLabel xml:lang="it">MIT</skos:altLabel>
      <skos:altLabel xml:lang="lt">MIT</skos:altLabel>
      <skos:altLabel xml:lang="lv">MIT</skos:altLabel>
      <skos:altLabel xml:lang="mt">MIT</skos:altLabel>
      <skos:altLabel xml:lang="nl">MIT</skos:altLabel>
      <skos:altLabel xml:lang="pl">MIT</skos:altLabel>
      <skos:altLabel xml:lang="pt">MIT</skos:altLabel>
      <skos:altLabel xml:lang="ro">MIT</skos:altLabel>
      <skos:altLabel xml:lang="sk">MIT</skos:altLabel>
      <skos:altLabel xml:lang="sl">MIT</skos:altLabel>
      <skos:altLabel xml:lang="sv">MIT</skos:altLabel>
      <skos:changeNote xml:lang="en">The source of the start-use date: https://opensource.com/article/19/4/history-mit-license; https://webcache.googleusercontent.com/search?q=cache:GAPzrOqxGoMJ:https://libexpat.github.io/doc/news/+&amp;cd=3&amp;hl=en&amp;ct=clnk&amp;gl=lu</skos:changeNote>
      <skos:definition xml:lang="en">Approved by the Open Source Initiative, MIT is the most recommended permissive licence: short and very popular. Everything is allowed as long as the original copyright and licence notice is included in any copy of the software/source.</skos:definition>
      <skos:exactMatch rdf:resource="https://opensource.org/licenses/MIT"/>
      <skos:inScheme rdf:resource="http://publications.europa.eu/resource/authority/licence"/>
      <skos:topConceptOf rdf:resource="http://publications.europa.eu/resource/authority/licence"/>
   </skos:Concept>
   <skos:Concept rdf:about="http://publications.europa.eu/resource/authority/licence/MOTOSOTO"
                 at:deprecated="false">
      <skos:prefLabel xml:lang="en">Motosoto Open Source License – Version 0.9.1 (Motosoto)</skos:prefLabel>
      <at:authority-code>MOTOSOTO</at:authority-code>
      <at:op-code>MOTOSOTO</at:op-code>
      <at:start.use>1995-01-01</at:start.use>
      <atold:op-code>MOTOSOTO</atold:op-code>
      <dc:identifier>MOTOSOTO</dc:identifier>
      <skos:altLabel xml:lang="bg">Motosoto</skos:altLabel>
      <skos:altLabel xml:lang="cs">Motosoto</skos:altLabel>
      <skos:altLabel xml:lang="da">Motosoto</skos:altLabel>
      <skos:altLabel xml:lang="de">Motosoto</skos:altLabel>
      <skos:altLabel xml:lang="el">Motosoto</skos:altLabel>
      <skos:altLabel xml:lang="en">Motosoto</skos:altLabel>
      <skos:altLabel xml:lang="es">Motosoto</skos:altLabel>
      <skos:altLabel xml:lang="et">Motosoto</skos:altLabel>
      <skos:altLabel xml:lang="fi">Motosoto</skos:altLabel>
      <skos:altLabel xml:lang="fr">Motosoto</skos:altLabel>
      <skos:altLabel xml:lang="ga">Motosoto</skos:altLabel>
      <skos:altLabel xml:lang="hr">Motosoto</skos:altLabel>
      <skos:altLabel xml:lang="hu">Motosoto</skos:altLabel>
      <skos:altLabel xml:lang="it">Motosoto</skos:altLabel>
      <skos:altLabel xml:lang="lt">Motosoto</skos:altLabel>
      <skos:altLabel xml:lang="lv">Motosoto</skos:altLabel>
      <skos:altLabel xml:lang="mt">Motosoto</skos:altLabel>
      <skos:altLabel xml:lang="nl">Motosoto</skos:altLabel>
      <skos:altLabel xml:lang="pl">Motosoto</skos:altLabel>
      <skos:altLabel xml:lang="pt">Motosoto</skos:altLabel>
      <skos:altLabel xml:lang="ro">Motosoto</skos:altLabel>
      <skos:altLabel xml:lang="sk">Motosoto</skos:altLabel>
      <skos:altLabel xml:lang="sl">Motosoto</skos:altLabel>
      <skos:altLabel xml:lang="sv">Motosoto</skos:altLabel>
      <skos:changeNote xml:lang="en">The source of the start-use date: http://www.worldlii.org/int/other/PubRL/1995/8.html</skos:changeNote>
      <skos:definition xml:lang="en">Motosoto is a copyleft-style, free software licence approved by the Open Source Initiative.</skos:definition>
      <skos:exactMatch rdf:resource="https://opensource.org/licenses/Motosoto"/>
      <skos:inScheme rdf:resource="http://publications.europa.eu/resource/authority/licence"/>
      <skos:topConceptOf rdf:resource="http://publications.europa.eu/resource/authority/licence"/>
   </skos:Concept>
   <skos:Concept rdf:about="http://publications.europa.eu/resource/authority/licence/MPL_1_0"
                 at:deprecated="true">
      <skos:prefLabel xml:lang="en">The Mozilla Public License (MPL), version 1.0 (MPL-1.0)</skos:prefLabel>
      <at:authority-code>MPL_1_0</at:authority-code>
      <at:op-code>MPL_1_0</at:op-code>
      <at:start.use>1998-01-01</at:start.use>
      <atold:op-code>MPL_1_0</atold:op-code>
      <dc:identifier>MPL_1_0</dc:identifier>
      <skos:altLabel xml:lang="bg">MPL-1.0</skos:altLabel>
      <skos:altLabel xml:lang="cs">MPL-1.0</skos:altLabel>
      <skos:altLabel xml:lang="da">MPL-1.0</skos:altLabel>
      <skos:altLabel xml:lang="de">MPL-1.0</skos:altLabel>
      <skos:altLabel xml:lang="el">MPL-1.0</skos:altLabel>
      <skos:altLabel xml:lang="en">MPL-1.0</skos:altLabel>
      <skos:altLabel xml:lang="es">MPL-1.0</skos:altLabel>
      <skos:altLabel xml:lang="et">MPL-1.0</skos:altLabel>
      <skos:altLabel xml:lang="fi">MPL-1.0</skos:altLabel>
      <skos:altLabel xml:lang="fr">MPL-1.0</skos:altLabel>
      <skos:altLabel xml:lang="ga">MPL-1.0</skos:altLabel>
      <skos:altLabel xml:lang="hr">MPL-1.0</skos:altLabel>
      <skos:altLabel xml:lang="hu">MPL-1.0</skos:altLabel>
      <skos:altLabel xml:lang="it">MPL-1.0</skos:altLabel>
      <skos:altLabel xml:lang="lt">MPL-1.0</skos:altLabel>
      <skos:altLabel xml:lang="lv">MPL-1.0</skos:altLabel>
      <skos:altLabel xml:lang="mt">MPL-1.0</skos:altLabel>
      <skos:altLabel xml:lang="nl">MPL-1.0</skos:altLabel>
      <skos:altLabel xml:lang="pl">MPL-1.0</skos:altLabel>
      <skos:altLabel xml:lang="pt">MPL-1.0</skos:altLabel>
      <skos:altLabel xml:lang="ro">MPL-1.0</skos:altLabel>
      <skos:altLabel xml:lang="sk">MPL-1.0</skos:altLabel>
      <skos:altLabel xml:lang="sl">MPL-1.0</skos:altLabel>
      <skos:altLabel xml:lang="sv">MPL-1.0</skos:altLabel>
      <skos:changeNote xml:lang="en">The source of the start-use date: https://en.wikipedia.org/wiki/Mozilla_Public_License</skos:changeNote>
      <skos:definition xml:lang="en">MPL-1.0 is a weak copyleft licence, characterised as a middle ground between permissive free software licences and the GNU General Public License that seeks to balance the concerns of proprietary and open source developers. As such, it allows re-licencing. It is approved by the Open Source Initiative. It has been superseded by v2.0.</skos:definition>
      <skos:exactMatch rdf:resource="https://opensource.org/licenses/MPL-1.0"/>
      <skos:inScheme rdf:resource="http://publications.europa.eu/resource/authority/licence"/>
      <skos:topConceptOf rdf:resource="http://publications.europa.eu/resource/authority/licence"/>
      <at:end.use>2012-01-02</at:end.use>
   </skos:Concept>
   <skos:Concept rdf:about="http://publications.europa.eu/resource/authority/licence/MPL_1_1"
                 at:deprecated="true">
      <skos:prefLabel xml:lang="en">Mozilla Public License (MPL), version 1.1 (MPL-1.1)</skos:prefLabel>
      <at:authority-code>MPL_1_1</at:authority-code>
      <at:op-code>MPL_1_1</at:op-code>
      <at:start.use>1999-01-01</at:start.use>
      <atold:op-code>MPL_1_1</atold:op-code>
      <dc:identifier>MPL_1_1</dc:identifier>
      <skos:altLabel xml:lang="bg">MPL-1.1</skos:altLabel>
      <skos:altLabel xml:lang="cs">MPL-1.1</skos:altLabel>
      <skos:altLabel xml:lang="da">MPL-1.1</skos:altLabel>
      <skos:altLabel xml:lang="de">MPL-1.1</skos:altLabel>
      <skos:altLabel xml:lang="el">MPL-1.1</skos:altLabel>
      <skos:altLabel xml:lang="en">MPL-1.1</skos:altLabel>
      <skos:altLabel xml:lang="es">MPL-1.1</skos:altLabel>
      <skos:altLabel xml:lang="et">MPL-1.1</skos:altLabel>
      <skos:altLabel xml:lang="fi">MPL-1.1</skos:altLabel>
      <skos:altLabel xml:lang="fr">MPL-1.1</skos:altLabel>
      <skos:altLabel xml:lang="ga">MPL-1.1</skos:altLabel>
      <skos:altLabel xml:lang="hr">MPL-1.1</skos:altLabel>
      <skos:altLabel xml:lang="hu">MPL-1.1</skos:altLabel>
      <skos:altLabel xml:lang="it">MPL-1.1</skos:altLabel>
      <skos:altLabel xml:lang="lt">MPL-1.1</skos:altLabel>
      <skos:altLabel xml:lang="lv">MPL-1.1</skos:altLabel>
      <skos:altLabel xml:lang="mt">MPL-1.1</skos:altLabel>
      <skos:altLabel xml:lang="nl">MPL-1.1</skos:altLabel>
      <skos:altLabel xml:lang="pl">MPL-1.1</skos:altLabel>
      <skos:altLabel xml:lang="pt">MPL-1.1</skos:altLabel>
      <skos:altLabel xml:lang="ro">MPL-1.1</skos:altLabel>
      <skos:altLabel xml:lang="sk">MPL-1.1</skos:altLabel>
      <skos:altLabel xml:lang="sl">MPL-1.1</skos:altLabel>
      <skos:altLabel xml:lang="sv">MPL-1.1</skos:altLabel>
      <skos:changeNote xml:lang="en">The source of the start-use date: https://en.wikisource.org/wiki/Mozilla_Public_License</skos:changeNote>
      <skos:definition xml:lang="en">MPL-1.1 is a weak copyleft licence, characterised as a middle ground between permissive free software licences and the GNU General Public License that seeks to balance the concerns of proprietary and open source developers. As such, it allows re-licencing. It is approved by the Open Source Initiative. It has been superseded by v2.0.</skos:definition>
      <skos:exactMatch rdf:resource="https://opensource.org/licenses/MPL-1.1"/>
      <skos:inScheme rdf:resource="http://publications.europa.eu/resource/authority/licence"/>
      <skos:topConceptOf rdf:resource="http://publications.europa.eu/resource/authority/licence"/>
      <at:end.use>2012-01-02</at:end.use>
   </skos:Concept>
   <skos:Concept rdf:about="http://publications.europa.eu/resource/authority/licence/MPL_2_0"
                 at:deprecated="false">
      <skos:prefLabel xml:lang="en">Mozilla Public License (MPL), version 2.0 (MPL-2.0)</skos:prefLabel>
      <at:authority-code>MPL_2_0</at:authority-code>
      <at:op-code>MPL_2_0</at:op-code>
      <at:start.use>2012-01-03</at:start.use>
      <atold:op-code>MPL_2_0</atold:op-code>
      <dc:identifier>MPL_2_0</dc:identifier>
      <skos:altLabel xml:lang="bg">MPL-2.0</skos:altLabel>
      <skos:altLabel xml:lang="cs">MPL-2.0</skos:altLabel>
      <skos:altLabel xml:lang="da">MPL-2.0</skos:altLabel>
      <skos:altLabel xml:lang="de">MPL-2.0</skos:altLabel>
      <skos:altLabel xml:lang="el">MPL-2.0</skos:altLabel>
      <skos:altLabel xml:lang="en">MPL-2.0</skos:altLabel>
      <skos:altLabel xml:lang="es">MPL-2.0</skos:altLabel>
      <skos:altLabel xml:lang="et">MPL-2.0</skos:altLabel>
      <skos:altLabel xml:lang="fi">MPL-2.0</skos:altLabel>
      <skos:altLabel xml:lang="fr">MPL-2.0</skos:altLabel>
      <skos:altLabel xml:lang="ga">MPL-2.0</skos:altLabel>
      <skos:altLabel xml:lang="hr">MPL-2.0</skos:altLabel>
      <skos:altLabel xml:lang="hu">MPL-2.0</skos:altLabel>
      <skos:altLabel xml:lang="it">MPL-2.0</skos:altLabel>
      <skos:altLabel xml:lang="lt">MPL-2.0</skos:altLabel>
      <skos:altLabel xml:lang="lv">MPL-2.0</skos:altLabel>
      <skos:altLabel xml:lang="mt">MPL-2.0</skos:altLabel>
      <skos:altLabel xml:lang="nl">MPL-2.0</skos:altLabel>
      <skos:altLabel xml:lang="pl">MPL-2.0</skos:altLabel>
      <skos:altLabel xml:lang="pt">MPL-2.0</skos:altLabel>
      <skos:altLabel xml:lang="ro">MPL-2.0</skos:altLabel>
      <skos:altLabel xml:lang="sk">MPL-2.0</skos:altLabel>
      <skos:altLabel xml:lang="sl">MPL-2.0</skos:altLabel>
      <skos:altLabel xml:lang="sv">MPL-2.0</skos:altLabel>
      <skos:changeNote xml:lang="en">The source of the start-use date: https://en.wikipedia.org/wiki/Mozilla_Public_License#cite_note-17</skos:changeNote>
      <skos:definition xml:lang="en">MPL-2.0 is a weak copyleft licence, characterised as a middle ground between permissive free software licences and the GNU General Public License that seeks to balance the concerns of proprietary and open source developers. As such, it allows re-licencing. It is approved by the Open Source Initiative.</skos:definition>
      <skos:exactMatch rdf:resource="https://opensource.org/licenses/MPL-2.0"/>
      <skos:inScheme rdf:resource="http://publications.europa.eu/resource/authority/licence"/>
      <skos:topConceptOf rdf:resource="http://publications.europa.eu/resource/authority/licence"/>
   </skos:Concept>
   <skos:Concept rdf:about="http://publications.europa.eu/resource/authority/licence/MS_PL"
                 at:deprecated="false">
      <skos:prefLabel xml:lang="en">Microsoft Public License (MS-PL)</skos:prefLabel>
      <at:authority-code>MS_PL</at:authority-code>
      <at:op-code>MS_PL</at:op-code>
      <at:start.use>2007-10-12</at:start.use>
      <atold:op-code>MS_PL</atold:op-code>
      <dc:identifier>MS_PL</dc:identifier>
      <skos:altLabel xml:lang="bg">MS-PL</skos:altLabel>
      <skos:altLabel xml:lang="cs">MS-PL</skos:altLabel>
      <skos:altLabel xml:lang="da">MS-PL</skos:altLabel>
      <skos:altLabel xml:lang="de">MS-PL</skos:altLabel>
      <skos:altLabel xml:lang="el">MS-PL</skos:altLabel>
      <skos:altLabel xml:lang="en">MS-PL</skos:altLabel>
      <skos:altLabel xml:lang="es">MS-PL</skos:altLabel>
      <skos:altLabel xml:lang="et">MS-PL</skos:altLabel>
      <skos:altLabel xml:lang="fi">MS-PL</skos:altLabel>
      <skos:altLabel xml:lang="fr">MS-PL</skos:altLabel>
      <skos:altLabel xml:lang="ga">MS-PL</skos:altLabel>
      <skos:altLabel xml:lang="hr">MS-PL</skos:altLabel>
      <skos:altLabel xml:lang="hu">MS-PL</skos:altLabel>
      <skos:altLabel xml:lang="it">MS-PL</skos:altLabel>
      <skos:altLabel xml:lang="lt">MS-PL</skos:altLabel>
      <skos:altLabel xml:lang="lv">MS-PL</skos:altLabel>
      <skos:altLabel xml:lang="mt">MS-PL</skos:altLabel>
      <skos:altLabel xml:lang="nl">MS-PL</skos:altLabel>
      <skos:altLabel xml:lang="pl">MS-PL</skos:altLabel>
      <skos:altLabel xml:lang="pt">MS-PL</skos:altLabel>
      <skos:altLabel xml:lang="ro">MS-PL</skos:altLabel>
      <skos:altLabel xml:lang="sk">MS-PL</skos:altLabel>
      <skos:altLabel xml:lang="sl">MS-PL</skos:altLabel>
      <skos:altLabel xml:lang="sv">MS-PL</skos:altLabel>
      <skos:changeNote xml:lang="en">The source of the start-use date: https://en.wikipedia.org/wiki/Shared_Source_Initiative#Microsoft_Public_License_(Ms-PL)</skos:changeNote>
      <skos:definition xml:lang="en">MS-PL is a BSD-style, permissive free software licence approved by the Open Source Initiative.</skos:definition>
      <skos:exactMatch rdf:resource="https://opensource.org/licenses/MS-PL"/>
      <skos:inScheme rdf:resource="http://publications.europa.eu/resource/authority/licence"/>
      <skos:topConceptOf rdf:resource="http://publications.europa.eu/resource/authority/licence"/>
   </skos:Concept>
   <skos:Concept rdf:about="http://publications.europa.eu/resource/authority/licence/MS_RL"
                 at:deprecated="false">
      <skos:prefLabel xml:lang="en">Microsoft Reciprocal License (MS-RL)</skos:prefLabel>
      <at:authority-code>MS_RL</at:authority-code>
      <at:op-code>MS_RL</at:op-code>
      <at:start.use>2007-08-10</at:start.use>
      <atold:op-code>MS_RL</atold:op-code>
      <dc:identifier>MS_RL</dc:identifier>
      <skos:altLabel xml:lang="bg">MS-RL</skos:altLabel>
      <skos:altLabel xml:lang="cs">MS-RL</skos:altLabel>
      <skos:altLabel xml:lang="da">MS-RL</skos:altLabel>
      <skos:altLabel xml:lang="de">MS-RL</skos:altLabel>
      <skos:altLabel xml:lang="el">MS-RL</skos:altLabel>
      <skos:altLabel xml:lang="en">MS-RL</skos:altLabel>
      <skos:altLabel xml:lang="es">MS-RL</skos:altLabel>
      <skos:altLabel xml:lang="et">MS-RL</skos:altLabel>
      <skos:altLabel xml:lang="fi">MS-RL</skos:altLabel>
      <skos:altLabel xml:lang="fr">MS-RL</skos:altLabel>
      <skos:altLabel xml:lang="ga">MS-RL</skos:altLabel>
      <skos:altLabel xml:lang="hr">MS-RL</skos:altLabel>
      <skos:altLabel xml:lang="hu">MS-RL</skos:altLabel>
      <skos:altLabel xml:lang="it">MS-RL</skos:altLabel>
      <skos:altLabel xml:lang="lt">MS-RL</skos:altLabel>
      <skos:altLabel xml:lang="lv">MS-RL</skos:altLabel>
      <skos:altLabel xml:lang="mt">MS-RL</skos:altLabel>
      <skos:altLabel xml:lang="nl">MS-RL</skos:altLabel>
      <skos:altLabel xml:lang="pl">MS-RL</skos:altLabel>
      <skos:altLabel xml:lang="pt">MS-RL</skos:altLabel>
      <skos:altLabel xml:lang="ro">MS-RL</skos:altLabel>
      <skos:altLabel xml:lang="sk">MS-RL</skos:altLabel>
      <skos:altLabel xml:lang="sl">MS-RL</skos:altLabel>
      <skos:altLabel xml:lang="sv">MS-RL</skos:altLabel>
      <skos:changeNote xml:lang="en">The source of the start-use date: https://de.wikipedia.org/wiki/Microsoft_Reciprocal_License</skos:changeNote>
      <skos:definition xml:lang="en">MS-RL is a copyleft-style, free software licence approved by the Open Source Initiative.</skos:definition>
      <skos:exactMatch rdf:resource="https://opensource.org/licenses/MS-RL"/>
      <skos:inScheme rdf:resource="http://publications.europa.eu/resource/authority/licence"/>
      <skos:topConceptOf rdf:resource="http://publications.europa.eu/resource/authority/licence"/>
   </skos:Concept>
   <skos:Concept rdf:about="http://publications.europa.eu/resource/authority/licence/MULTICS"
                 at:deprecated="false">
      <skos:prefLabel xml:lang="en">Multics License (Multics)</skos:prefLabel>
      <at:authority-code>MULTICS</at:authority-code>
      <at:op-code>MULTICS</at:op-code>
      <at:start.use>2006-07-01</at:start.use>
      <atold:op-code>MULTICS</atold:op-code>
      <dc:identifier>MULTICS</dc:identifier>
      <skos:altLabel xml:lang="bg">Multics</skos:altLabel>
      <skos:altLabel xml:lang="cs">Multics</skos:altLabel>
      <skos:altLabel xml:lang="da">Multics</skos:altLabel>
      <skos:altLabel xml:lang="de">Multics</skos:altLabel>
      <skos:altLabel xml:lang="el">Multics</skos:altLabel>
      <skos:altLabel xml:lang="en">Multics</skos:altLabel>
      <skos:altLabel xml:lang="es">Multics</skos:altLabel>
      <skos:altLabel xml:lang="et">Multics</skos:altLabel>
      <skos:altLabel xml:lang="fi">Multics</skos:altLabel>
      <skos:altLabel xml:lang="fr">Multics</skos:altLabel>
      <skos:altLabel xml:lang="ga">Multics</skos:altLabel>
      <skos:altLabel xml:lang="hr">Multics</skos:altLabel>
      <skos:altLabel xml:lang="hu">Multics</skos:altLabel>
      <skos:altLabel xml:lang="it">Multics</skos:altLabel>
      <skos:altLabel xml:lang="lt">Multics</skos:altLabel>
      <skos:altLabel xml:lang="lv">Multics</skos:altLabel>
      <skos:altLabel xml:lang="mt">Multics</skos:altLabel>
      <skos:altLabel xml:lang="nl">Multics</skos:altLabel>
      <skos:altLabel xml:lang="pl">Multics</skos:altLabel>
      <skos:altLabel xml:lang="pt">Multics</skos:altLabel>
      <skos:altLabel xml:lang="ro">Multics</skos:altLabel>
      <skos:altLabel xml:lang="sk">Multics</skos:altLabel>
      <skos:altLabel xml:lang="sl">Multics</skos:altLabel>
      <skos:altLabel xml:lang="sv">Multics</skos:altLabel>
      <skos:changeNote xml:lang="en">The source of the start-use date: https://enterprise.dejacode.com/licenses/public/multics/?_list_filters=q%3Dmultics</skos:changeNote>
      <skos:definition xml:lang="en">Multics is a permissive free software licence approved by the Open Source Initiative. The legal text of this licence is only a paragraph long and both protects the authors' trademarks and requires users to include this licence.</skos:definition>
      <skos:exactMatch rdf:resource="https://opensource.org/licenses/Multics"/>
      <skos:inScheme rdf:resource="http://publications.europa.eu/resource/authority/licence"/>
      <skos:topConceptOf rdf:resource="http://publications.europa.eu/resource/authority/licence"/>
   </skos:Concept>
   <skos:Concept rdf:about="http://publications.europa.eu/resource/authority/licence/NASA_1_3"
                 at:deprecated="false">
      <skos:prefLabel xml:lang="en">NASA Open Source Agreement v1.3 (NASA-1.3)</skos:prefLabel>
      <at:authority-code>NASA_1_3</at:authority-code>
      <at:op-code>NASA_1_3</at:op-code>
      <at:start.use>2012-01-01</at:start.use>
      <atold:op-code>NASA_1_3</atold:op-code>
      <dc:identifier>NASA_1_3</dc:identifier>
      <skos:altLabel xml:lang="bg">NASA-1.3</skos:altLabel>
      <skos:altLabel xml:lang="cs">NASA-1.3</skos:altLabel>
      <skos:altLabel xml:lang="da">NASA-1.3</skos:altLabel>
      <skos:altLabel xml:lang="de">NASA-1.3</skos:altLabel>
      <skos:altLabel xml:lang="el">NASA-1.3</skos:altLabel>
      <skos:altLabel xml:lang="en">NASA-1.3</skos:altLabel>
      <skos:altLabel xml:lang="es">NASA-1.3</skos:altLabel>
      <skos:altLabel xml:lang="et">NASA-1.3</skos:altLabel>
      <skos:altLabel xml:lang="fi">NASA-1.3</skos:altLabel>
      <skos:altLabel xml:lang="fr">NASA-1.3</skos:altLabel>
      <skos:altLabel xml:lang="ga">NASA-1.3</skos:altLabel>
      <skos:altLabel xml:lang="hr">NASA-1.3</skos:altLabel>
      <skos:altLabel xml:lang="hu">NASA-1.3</skos:altLabel>
      <skos:altLabel xml:lang="it">NASA-1.3</skos:altLabel>
      <skos:altLabel xml:lang="lt">NASA-1.3</skos:altLabel>
      <skos:altLabel xml:lang="lv">NASA-1.3</skos:altLabel>
      <skos:altLabel xml:lang="mt">NASA-1.3</skos:altLabel>
      <skos:altLabel xml:lang="nl">NASA-1.3</skos:altLabel>
      <skos:altLabel xml:lang="pl">NASA-1.3</skos:altLabel>
      <skos:altLabel xml:lang="pt">NASA-1.3</skos:altLabel>
      <skos:altLabel xml:lang="ro">NASA-1.3</skos:altLabel>
      <skos:altLabel xml:lang="sk">NASA-1.3</skos:altLabel>
      <skos:altLabel xml:lang="sl">NASA-1.3</skos:altLabel>
      <skos:altLabel xml:lang="sv">NASA-1.3</skos:altLabel>
      <skos:changeNote xml:lang="en">The source of the start-use date: https://en.wikipedia.org/wiki/NASA_Open_Source_Agreement; http://openvsp.org/learn.shtml</skos:changeNote>
      <skos:definition xml:lang="en">Approved by the Open Source Initiative, NASA-1.3 is a licence used by NASA containing an obligation to register with the government when receiving the software and to tell a specified agency how the modifications are used.</skos:definition>
      <skos:exactMatch rdf:resource="https://opensource.org/licenses/NASA-1.3"/>
      <skos:inScheme rdf:resource="http://publications.europa.eu/resource/authority/licence"/>
      <skos:topConceptOf rdf:resource="http://publications.europa.eu/resource/authority/licence"/>
   </skos:Concept>
   <skos:Concept rdf:about="http://publications.europa.eu/resource/authority/licence/NAUMEN"
                 at:deprecated="false">
      <skos:prefLabel xml:lang="en">NAUMEN Public License (Naumen)</skos:prefLabel>
      <at:authority-code>NAUMEN</at:authority-code>
      <at:op-code>NAUMEN</at:op-code>
      <at:start.use>2001-12-01</at:start.use>
      <atold:op-code>NAUMEN</atold:op-code>
      <dc:identifier>NAUMEN</dc:identifier>
      <skos:altLabel xml:lang="bg">Naumen</skos:altLabel>
      <skos:altLabel xml:lang="cs">Naumen</skos:altLabel>
      <skos:altLabel xml:lang="da">Naumen</skos:altLabel>
      <skos:altLabel xml:lang="de">Naumen</skos:altLabel>
      <skos:altLabel xml:lang="el">Naumen</skos:altLabel>
      <skos:altLabel xml:lang="en">Naumen</skos:altLabel>
      <skos:altLabel xml:lang="es">Naumen</skos:altLabel>
      <skos:altLabel xml:lang="et">Naumen</skos:altLabel>
      <skos:altLabel xml:lang="fi">Naumen</skos:altLabel>
      <skos:altLabel xml:lang="fr">Naumen</skos:altLabel>
      <skos:altLabel xml:lang="ga">Naumen</skos:altLabel>
      <skos:altLabel xml:lang="hr">Naumen</skos:altLabel>
      <skos:altLabel xml:lang="hu">Naumen</skos:altLabel>
      <skos:altLabel xml:lang="it">Naumen</skos:altLabel>
      <skos:altLabel xml:lang="lt">Naumen</skos:altLabel>
      <skos:altLabel xml:lang="lv">Naumen</skos:altLabel>
      <skos:altLabel xml:lang="mt">Naumen</skos:altLabel>
      <skos:altLabel xml:lang="nl">Naumen</skos:altLabel>
      <skos:altLabel xml:lang="pl">Naumen</skos:altLabel>
      <skos:altLabel xml:lang="pt">Naumen</skos:altLabel>
      <skos:altLabel xml:lang="ro">Naumen</skos:altLabel>
      <skos:altLabel xml:lang="sk">Naumen</skos:altLabel>
      <skos:altLabel xml:lang="sl">Naumen</skos:altLabel>
      <skos:altLabel xml:lang="sv">Naumen</skos:altLabel>
      <skos:changeNote xml:lang="en">The source of the start-use date: https://ru.wikipedia.org/wiki/Naumen; http://licenseit.ru/wiki/index.php/Naumen_Public_License</skos:changeNote>
      <skos:definition xml:lang="en">Approved by the Open Source Initiative, Naumen is a fairly restrictive free software licence, but provides good protection for the author of the software.</skos:definition>
      <skos:exactMatch rdf:resource="https://opensource.org/licenses/Naumen"/>
      <skos:inScheme rdf:resource="http://publications.europa.eu/resource/authority/licence"/>
      <skos:topConceptOf rdf:resource="http://publications.europa.eu/resource/authority/licence"/>
   </skos:Concept>
   <skos:Concept rdf:about="http://publications.europa.eu/resource/authority/licence/NCSA"
                 at:deprecated="false">
      <skos:prefLabel xml:lang="en">The University of Illinois/NCSA Open Source License (NCSA)</skos:prefLabel>
      <at:authority-code>NCSA</at:authority-code>
      <at:op-code>NCSA</at:op-code>
      <at:start.use>2002-03-28</at:start.use>
      <atold:op-code>NCSA</atold:op-code>
      <dc:identifier>NCSA</dc:identifier>
      <skos:altLabel xml:lang="bg">NCSA</skos:altLabel>
      <skos:altLabel xml:lang="cs">NCSA</skos:altLabel>
      <skos:altLabel xml:lang="da">NCSA</skos:altLabel>
      <skos:altLabel xml:lang="de">NCSA</skos:altLabel>
      <skos:altLabel xml:lang="el">NCSA</skos:altLabel>
      <skos:altLabel xml:lang="en">NCSA</skos:altLabel>
      <skos:altLabel xml:lang="es">NCSA</skos:altLabel>
      <skos:altLabel xml:lang="et">NCSA</skos:altLabel>
      <skos:altLabel xml:lang="fi">NCSA</skos:altLabel>
      <skos:altLabel xml:lang="fr">NCSA</skos:altLabel>
      <skos:altLabel xml:lang="ga">NCSA</skos:altLabel>
      <skos:altLabel xml:lang="hr">NCSA</skos:altLabel>
      <skos:altLabel xml:lang="hu">NCSA</skos:altLabel>
      <skos:altLabel xml:lang="it">NCSA</skos:altLabel>
      <skos:altLabel xml:lang="lt">NCSA</skos:altLabel>
      <skos:altLabel xml:lang="lv">NCSA</skos:altLabel>
      <skos:altLabel xml:lang="mt">NCSA</skos:altLabel>
      <skos:altLabel xml:lang="nl">NCSA</skos:altLabel>
      <skos:altLabel xml:lang="pl">NCSA</skos:altLabel>
      <skos:altLabel xml:lang="pt">NCSA</skos:altLabel>
      <skos:altLabel xml:lang="ro">NCSA</skos:altLabel>
      <skos:altLabel xml:lang="sk">NCSA</skos:altLabel>
      <skos:altLabel xml:lang="sl">NCSA</skos:altLabel>
      <skos:altLabel xml:lang="sv">NCSA</skos:altLabel>
      <skos:changeNote xml:lang="en">The source of the start-use date: https://en.wikipedia.org/wiki/University_of_Illinois/NCSA_Open_Source_License</skos:changeNote>
      <skos:definition xml:lang="en">NCSA Open Source License is a BSD-style, permissive free software licence approved by the Open Source Initiative.</skos:definition>
      <skos:exactMatch rdf:resource="https://opensource.org/licenses/NCSA"/>
      <skos:inScheme rdf:resource="http://publications.europa.eu/resource/authority/licence"/>
      <skos:topConceptOf rdf:resource="http://publications.europa.eu/resource/authority/licence"/>
   </skos:Concept>
   <skos:Concept rdf:about="http://publications.europa.eu/resource/authority/licence/NGPL"
                 at:deprecated="false">
      <skos:prefLabel xml:lang="en">The Nethack General Public License (NGPL)</skos:prefLabel>
      <at:authority-code>NGPL</at:authority-code>
      <at:op-code>NGPL</at:op-code>
      <at:start.use>1989-07-31</at:start.use>
      <atold:op-code>NGPL</atold:op-code>
      <dc:identifier>NGPL</dc:identifier>
      <skos:altLabel xml:lang="bg">NGPL</skos:altLabel>
      <skos:altLabel xml:lang="cs">NGPL</skos:altLabel>
      <skos:altLabel xml:lang="da">NGPL</skos:altLabel>
      <skos:altLabel xml:lang="de">NGPL</skos:altLabel>
      <skos:altLabel xml:lang="el">NGPL</skos:altLabel>
      <skos:altLabel xml:lang="en">NGPL</skos:altLabel>
      <skos:altLabel xml:lang="es">NGPL</skos:altLabel>
      <skos:altLabel xml:lang="et">NGPL</skos:altLabel>
      <skos:altLabel xml:lang="fi">NGPL</skos:altLabel>
      <skos:altLabel xml:lang="fr">NGPL</skos:altLabel>
      <skos:altLabel xml:lang="ga">NGPL</skos:altLabel>
      <skos:altLabel xml:lang="hr">NGPL</skos:altLabel>
      <skos:altLabel xml:lang="hu">NGPL</skos:altLabel>
      <skos:altLabel xml:lang="it">NGPL</skos:altLabel>
      <skos:altLabel xml:lang="lt">NGPL</skos:altLabel>
      <skos:altLabel xml:lang="lv">NGPL</skos:altLabel>
      <skos:altLabel xml:lang="mt">NGPL</skos:altLabel>
      <skos:altLabel xml:lang="nl">NGPL</skos:altLabel>
      <skos:altLabel xml:lang="pl">NGPL</skos:altLabel>
      <skos:altLabel xml:lang="pt">NGPL</skos:altLabel>
      <skos:altLabel xml:lang="ro">NGPL</skos:altLabel>
      <skos:altLabel xml:lang="sk">NGPL</skos:altLabel>
      <skos:altLabel xml:lang="sl">NGPL</skos:altLabel>
      <skos:altLabel xml:lang="sv">NGPL</skos:altLabel>
      <skos:changeNote xml:lang="en">The source of the start-use date: https://en.wikipedia.org/wiki/NetHack</skos:changeNote>
      <skos:definition xml:lang="en">Approved by the Open Source Initiative, NGPL is a very old licence used for the game NetHack. It allows users to freely share their modifications, in exchange for several restrictions and little protection for the authors.</skos:definition>
      <skos:exactMatch rdf:resource="https://opensource.org/licenses/NGPL"/>
      <skos:inScheme rdf:resource="http://publications.europa.eu/resource/authority/licence"/>
      <skos:topConceptOf rdf:resource="http://publications.europa.eu/resource/authority/licence"/>
   </skos:Concept>
   <skos:Concept rdf:about="http://publications.europa.eu/resource/authority/licence/NLOD_1_0"
                 at:deprecated="false">
      <skos:prefLabel xml:lang="en">Norwegian Licence for Open Government Data 1.0</skos:prefLabel>
      <at:authority-code>NLOD_1_0</at:authority-code>
      <at:op-code>NLOD_1_0</at:op-code>
      <at:start.use>2012-01-01</at:start.use>
      <atold:op-code>NLOD_1_0</atold:op-code>
      <dc:identifier>NLOD_1_0</dc:identifier>
      <skos:altLabel xml:lang="bg">NLOD 1.0</skos:altLabel>
      <skos:altLabel xml:lang="cs">NLOD 1.0</skos:altLabel>
      <skos:altLabel xml:lang="da">NLOD 1.0</skos:altLabel>
      <skos:altLabel xml:lang="de">NLOD 1.0</skos:altLabel>
      <skos:altLabel xml:lang="el">NLOD 1.0</skos:altLabel>
      <skos:altLabel xml:lang="en">NLOD 1.0</skos:altLabel>
      <skos:altLabel xml:lang="es">NLOD 1.0</skos:altLabel>
      <skos:altLabel xml:lang="et">NLOD 1.0</skos:altLabel>
      <skos:altLabel xml:lang="fi">NLOD 1.0</skos:altLabel>
      <skos:altLabel xml:lang="fr">NLOD 1.0</skos:altLabel>
      <skos:altLabel xml:lang="ga">NLOD 1.0</skos:altLabel>
      <skos:altLabel xml:lang="hr">NLOD 1.0</skos:altLabel>
      <skos:altLabel xml:lang="hu">NLOD 1.0</skos:altLabel>
      <skos:altLabel xml:lang="it">NLOD 1.0</skos:altLabel>
      <skos:altLabel xml:lang="lt">NLOD 1.0</skos:altLabel>
      <skos:altLabel xml:lang="lv">NLOD 1.0</skos:altLabel>
      <skos:altLabel xml:lang="mt">NLOD 1.0</skos:altLabel>
      <skos:altLabel xml:lang="nl">NLOD 1.0</skos:altLabel>
      <skos:altLabel xml:lang="pl">NLOD 1.0</skos:altLabel>
      <skos:altLabel xml:lang="pt">NLOD 1.0</skos:altLabel>
      <skos:altLabel xml:lang="ro">NLOD 1.0</skos:altLabel>
      <skos:altLabel xml:lang="sk">NLOD 1.0</skos:altLabel>
      <skos:altLabel xml:lang="sl">NLOD 1.0</skos:altLabel>
      <skos:altLabel xml:lang="sv">NLOD 1.0</skos:altLabel>
      <skos:changeNote xml:lang="en">The source of the start-use date: https://github.com/difi/veileder-opnedata/blob/master/build/html/en/_sources/Hvordan-aapne-opp-data/index.txt</skos:changeNote>
      <skos:definition xml:lang="en">Published by Norway, NLOD 1.0 grants the user the right to copy, use and distribute information, provided the user acknowledges the contributors and complies with the terms and conditions stipulated in this licence.</skos:definition>
      <skos:exactMatch rdf:resource="http://data.norge.no/nlod/en/1.0"/>
      <skos:inScheme rdf:resource="http://publications.europa.eu/resource/authority/licence"/>
      <skos:topConceptOf rdf:resource="http://publications.europa.eu/resource/authority/licence"/>
   </skos:Concept>
   <skos:Concept rdf:about="http://publications.europa.eu/resource/authority/licence/NLOD_2_0"
                 at:deprecated="false">
      <skos:prefLabel xml:lang="en">Norwegian Licence for Open Government Data (NLOD) 2.0</skos:prefLabel>
      <at:authority-code>NLOD_2_0</at:authority-code>
      <at:op-code>NLOD_2_0</at:op-code>
      <at:start.use>2016-09-01</at:start.use>
      <atold:op-code>NLOD_2_0</atold:op-code>
      <dc:identifier>NLOD_2_0</dc:identifier>
      <skos:altLabel xml:lang="bg">NLOD 2.0</skos:altLabel>
      <skos:altLabel xml:lang="cs">NLOD 2.0</skos:altLabel>
      <skos:altLabel xml:lang="da">NLOD 2.0</skos:altLabel>
      <skos:altLabel xml:lang="de">NLOD 2.0</skos:altLabel>
      <skos:altLabel xml:lang="el">NLOD 2.0</skos:altLabel>
      <skos:altLabel xml:lang="en">NLOD 2.0</skos:altLabel>
      <skos:altLabel xml:lang="es">NLOD 2.0</skos:altLabel>
      <skos:altLabel xml:lang="et">NLOD 2.0</skos:altLabel>
      <skos:altLabel xml:lang="fi">NLOD 2.0</skos:altLabel>
      <skos:altLabel xml:lang="fr">NLOD 2.0</skos:altLabel>
      <skos:altLabel xml:lang="ga">NLOD 2.0</skos:altLabel>
      <skos:altLabel xml:lang="hr">NLOD 2.0</skos:altLabel>
      <skos:altLabel xml:lang="hu">NLOD 2.0</skos:altLabel>
      <skos:altLabel xml:lang="it">NLOD 2.0</skos:altLabel>
      <skos:altLabel xml:lang="lt">NLOD 2.0</skos:altLabel>
      <skos:altLabel xml:lang="lv">NLOD 2.0</skos:altLabel>
      <skos:altLabel xml:lang="mt">NLOD 2.0</skos:altLabel>
      <skos:altLabel xml:lang="nl">NLOD 2.0</skos:altLabel>
      <skos:altLabel xml:lang="pl">NLOD 2.0</skos:altLabel>
      <skos:altLabel xml:lang="pt">NLOD 2.0</skos:altLabel>
      <skos:altLabel xml:lang="ro">NLOD 2.0</skos:altLabel>
      <skos:altLabel xml:lang="sk">NLOD 2.0</skos:altLabel>
      <skos:altLabel xml:lang="sl">NLOD 2.0</skos:altLabel>
      <skos:altLabel xml:lang="sv">NLOD 2.0</skos:altLabel>
      <skos:definition xml:lang="en">Published by Norway, NLOD 2.0 grants the user the right to copy, use and distribute information, provided the user acknowledges the contributors and complies with the terms and conditions stipulated in this licence.</skos:definition>
      <skos:exactMatch rdf:resource="https://data.norge.no/nlod/en/2.0/"/>
      <skos:inScheme rdf:resource="http://publications.europa.eu/resource/authority/licence"/>
      <skos:topConceptOf rdf:resource="http://publications.europa.eu/resource/authority/licence"/>
   </skos:Concept>
   <skos:Concept rdf:about="http://publications.europa.eu/resource/authority/licence/NOKIA"
                 at:deprecated="false">
      <skos:prefLabel xml:lang="en">Nokia Open Source License Version 1.0a (NOKIA)</skos:prefLabel>
      <at:authority-code>NOKIA</at:authority-code>
      <at:op-code>NOKIA</at:op-code>
      <at:start.use>2006-01-01</at:start.use>
      <atold:op-code>NOKIA</atold:op-code>
      <dc:identifier>NOKIA</dc:identifier>
      <skos:altLabel xml:lang="bg">NOKIA</skos:altLabel>
      <skos:altLabel xml:lang="cs">NOKIA</skos:altLabel>
      <skos:altLabel xml:lang="da">NOKIA</skos:altLabel>
      <skos:altLabel xml:lang="de">NOKIA</skos:altLabel>
      <skos:altLabel xml:lang="el">NOKIA</skos:altLabel>
      <skos:altLabel xml:lang="en">NOKIA</skos:altLabel>
      <skos:altLabel xml:lang="es">NOKIA</skos:altLabel>
      <skos:altLabel xml:lang="et">NOKIA</skos:altLabel>
      <skos:altLabel xml:lang="fi">NOKIA</skos:altLabel>
      <skos:altLabel xml:lang="fr">NOKIA</skos:altLabel>
      <skos:altLabel xml:lang="ga">NOKIA</skos:altLabel>
      <skos:altLabel xml:lang="hr">NOKIA</skos:altLabel>
      <skos:altLabel xml:lang="hu">NOKIA</skos:altLabel>
      <skos:altLabel xml:lang="it">NOKIA</skos:altLabel>
      <skos:altLabel xml:lang="lt">NOKIA</skos:altLabel>
      <skos:altLabel xml:lang="lv">NOKIA</skos:altLabel>
      <skos:altLabel xml:lang="mt">NOKIA</skos:altLabel>
      <skos:altLabel xml:lang="nl">NOKIA</skos:altLabel>
      <skos:altLabel xml:lang="pl">NOKIA</skos:altLabel>
      <skos:altLabel xml:lang="pt">NOKIA</skos:altLabel>
      <skos:altLabel xml:lang="ro">NOKIA</skos:altLabel>
      <skos:altLabel xml:lang="sk">NOKIA</skos:altLabel>
      <skos:altLabel xml:lang="sl">NOKIA</skos:altLabel>
      <skos:altLabel xml:lang="sv">NOKIA</skos:altLabel>
      <skos:changeNote xml:lang="en">The source of the start-use date: http://www.kansai-u.ac.jp/riss/rcss/conf/confdocs/3rdRCSS_ueda.pdf; https://opensource.org/minutes20060208</skos:changeNote>
      <skos:definition xml:lang="en">Approved by the Open Source Initiative, NOKIA is a slightly altered variant on the Mozilla Public License specified for Nokia. It requires including a notice in each source file. Disputes must be settled through a Finnish arbitration process.</skos:definition>
      <skos:exactMatch rdf:resource="https://opensource.org/licenses/NOKIA"/>
      <skos:inScheme rdf:resource="http://publications.europa.eu/resource/authority/licence"/>
      <skos:topConceptOf rdf:resource="http://publications.europa.eu/resource/authority/licence"/>
   </skos:Concept>
   <skos:Concept rdf:about="http://publications.europa.eu/resource/authority/licence/NPOSL_3_0"
                 at:deprecated="false">
      <skos:prefLabel xml:lang="en">The Non-Profit Open Software License version 3.0 (NPOSL-3.0)</skos:prefLabel>
      <at:authority-code>NPOSL_3_0</at:authority-code>
      <at:op-code>NPOSL_3_0</at:op-code>
      <at:start.use>2007-09-20</at:start.use>
      <atold:op-code>NPOSL_3_0</atold:op-code>
      <dc:identifier>NPOSL_3_0</dc:identifier>
      <skos:altLabel xml:lang="bg">NPOSL-3.0</skos:altLabel>
      <skos:altLabel xml:lang="cs">NPOSL-3.0</skos:altLabel>
      <skos:altLabel xml:lang="da">NPOSL-3.0</skos:altLabel>
      <skos:altLabel xml:lang="de">NPOSL-3.0</skos:altLabel>
      <skos:altLabel xml:lang="el">NPOSL-3.0</skos:altLabel>
      <skos:altLabel xml:lang="en">NPOSL-3.0</skos:altLabel>
      <skos:altLabel xml:lang="es">NPOSL-3.0</skos:altLabel>
      <skos:altLabel xml:lang="et">NPOSL-3.0</skos:altLabel>
      <skos:altLabel xml:lang="fi">NPOSL-3.0</skos:altLabel>
      <skos:altLabel xml:lang="fr">NPOSL-3.0</skos:altLabel>
      <skos:altLabel xml:lang="ga">NPOSL-3.0</skos:altLabel>
      <skos:altLabel xml:lang="hr">NPOSL-3.0</skos:altLabel>
      <skos:altLabel xml:lang="hu">NPOSL-3.0</skos:altLabel>
      <skos:altLabel xml:lang="it">NPOSL-3.0</skos:altLabel>
      <skos:altLabel xml:lang="lt">NPOSL-3.0</skos:altLabel>
      <skos:altLabel xml:lang="lv">NPOSL-3.0</skos:altLabel>
      <skos:altLabel xml:lang="mt">NPOSL-3.0</skos:altLabel>
      <skos:altLabel xml:lang="nl">NPOSL-3.0</skos:altLabel>
      <skos:altLabel xml:lang="pl">NPOSL-3.0</skos:altLabel>
      <skos:altLabel xml:lang="pt">NPOSL-3.0</skos:altLabel>
      <skos:altLabel xml:lang="ro">NPOSL-3.0</skos:altLabel>
      <skos:altLabel xml:lang="sk">NPOSL-3.0</skos:altLabel>
      <skos:altLabel xml:lang="sl">NPOSL-3.0</skos:altLabel>
      <skos:altLabel xml:lang="sv">NPOSL-3.0</skos:altLabel>
      <skos:changeNote xml:lang="en">The source of the start-use date: https://lists.debian.org/debian-legal/2008/04/msg00055.html; https://trustee.ietf.org/licenses.html</skos:changeNote>
      <skos:definition xml:lang="en">A variant of the Open Software License 3.0, NPOSL-3.0 requires that the organisation using it is a non-profit and that no revenue is generated from sale of the software, support or services. It is approved by the Open Source Initiative.</skos:definition>
      <skos:exactMatch rdf:resource="https://opensource.org/licenses/NPOSL-3.0"/>
      <skos:inScheme rdf:resource="http://publications.europa.eu/resource/authority/licence"/>
      <skos:topConceptOf rdf:resource="http://publications.europa.eu/resource/authority/licence"/>
   </skos:Concept>
   <skos:Concept rdf:about="http://publications.europa.eu/resource/authority/licence/NTP"
                 at:deprecated="false">
      <skos:prefLabel xml:lang="en">NTP License (NTP)</skos:prefLabel>
      <at:authority-code>NTP</at:authority-code>
      <at:op-code>NTP</at:op-code>
      <at:start.use>2008-08-01</at:start.use>
      <atold:op-code>NTP</atold:op-code>
      <dc:identifier>NTP</dc:identifier>
      <skos:altLabel xml:lang="bg">NTP</skos:altLabel>
      <skos:altLabel xml:lang="cs">NTP</skos:altLabel>
      <skos:altLabel xml:lang="da">NTP</skos:altLabel>
      <skos:altLabel xml:lang="de">NTP</skos:altLabel>
      <skos:altLabel xml:lang="el">NTP</skos:altLabel>
      <skos:altLabel xml:lang="en">NTP</skos:altLabel>
      <skos:altLabel xml:lang="es">NTP</skos:altLabel>
      <skos:altLabel xml:lang="et">NTP</skos:altLabel>
      <skos:altLabel xml:lang="fi">NTP</skos:altLabel>
      <skos:altLabel xml:lang="fr">NTP</skos:altLabel>
      <skos:altLabel xml:lang="ga">NTP</skos:altLabel>
      <skos:altLabel xml:lang="hr">NTP</skos:altLabel>
      <skos:altLabel xml:lang="hu">NTP</skos:altLabel>
      <skos:altLabel xml:lang="it">NTP</skos:altLabel>
      <skos:altLabel xml:lang="lt">NTP</skos:altLabel>
      <skos:altLabel xml:lang="lv">NTP</skos:altLabel>
      <skos:altLabel xml:lang="mt">NTP</skos:altLabel>
      <skos:altLabel xml:lang="nl">NTP</skos:altLabel>
      <skos:altLabel xml:lang="pl">NTP</skos:altLabel>
      <skos:altLabel xml:lang="pt">NTP</skos:altLabel>
      <skos:altLabel xml:lang="ro">NTP</skos:altLabel>
      <skos:altLabel xml:lang="sk">NTP</skos:altLabel>
      <skos:altLabel xml:lang="sl">NTP</skos:altLabel>
      <skos:altLabel xml:lang="sv">NTP</skos:altLabel>
      <skos:changeNote xml:lang="en">The source of the start-use date: http://lists.opensource.org/pipermail/license-review_lists.opensource.org/2008-March/000099.html; https://opensource.org/node/1015</skos:changeNote>
      <skos:definition xml:lang="en">Approved by the Open Source Initiative, NTP is a simple licence, written as a template, that provides protection for the author while giving users full rights to the software.</skos:definition>
      <skos:exactMatch rdf:resource="https://opensource.org/licenses/NTP"/>
      <skos:inScheme rdf:resource="http://publications.europa.eu/resource/authority/licence"/>
      <skos:topConceptOf rdf:resource="http://publications.europa.eu/resource/authority/licence"/>
   </skos:Concept>
   <skos:Concept rdf:about="http://publications.europa.eu/resource/authority/licence/OCLC_2_0"
                 at:deprecated="false">
      <skos:prefLabel xml:lang="en">The OCLC Research Public License 2.0 License (OCLC-2.0)</skos:prefLabel>
      <at:authority-code>OCLC_2_0</at:authority-code>
      <at:op-code>OCLC_2_0</at:op-code>
      <at:start.use>2002-05-31</at:start.use>
      <atold:op-code>OCLC_2_0</atold:op-code>
      <dc:identifier>OCLC_2_0</dc:identifier>
      <skos:altLabel xml:lang="bg">OCLC-2.0</skos:altLabel>
      <skos:altLabel xml:lang="cs">OCLC-2.0</skos:altLabel>
      <skos:altLabel xml:lang="da">OCLC-2.0</skos:altLabel>
      <skos:altLabel xml:lang="de">OCLC-2.0</skos:altLabel>
      <skos:altLabel xml:lang="el">OCLC-2.0</skos:altLabel>
      <skos:altLabel xml:lang="en">OCLC-2.0</skos:altLabel>
      <skos:altLabel xml:lang="es">OCLC-2.0</skos:altLabel>
      <skos:altLabel xml:lang="et">OCLC-2.0</skos:altLabel>
      <skos:altLabel xml:lang="fi">OCLC-2.0</skos:altLabel>
      <skos:altLabel xml:lang="fr">OCLC-2.0</skos:altLabel>
      <skos:altLabel xml:lang="ga">OCLC-2.0</skos:altLabel>
      <skos:altLabel xml:lang="hr">OCLC-2.0</skos:altLabel>
      <skos:altLabel xml:lang="hu">OCLC-2.0</skos:altLabel>
      <skos:altLabel xml:lang="it">OCLC-2.0</skos:altLabel>
      <skos:altLabel xml:lang="lt">OCLC-2.0</skos:altLabel>
      <skos:altLabel xml:lang="lv">OCLC-2.0</skos:altLabel>
      <skos:altLabel xml:lang="mt">OCLC-2.0</skos:altLabel>
      <skos:altLabel xml:lang="nl">OCLC-2.0</skos:altLabel>
      <skos:altLabel xml:lang="pl">OCLC-2.0</skos:altLabel>
      <skos:altLabel xml:lang="pt">OCLC-2.0</skos:altLabel>
      <skos:altLabel xml:lang="ro">OCLC-2.0</skos:altLabel>
      <skos:altLabel xml:lang="sk">OCLC-2.0</skos:altLabel>
      <skos:altLabel xml:lang="sl">OCLC-2.0</skos:altLabel>
      <skos:altLabel xml:lang="sv">OCLC-2.0</skos:altLabel>
      <skos:changeNote xml:lang="en">The source of the start-use date: https://opensource.org/licenses/OCLC-2.0</skos:changeNote>
      <skos:definition xml:lang="en">While OCLC Research now uses the Apache 2.0 licence, OCLC-2.0 is a relatively strong copyleft licence with fairly lenient restrictions and built-in protection for the author. It is approved by the Open Source Initiative.</skos:definition>
      <skos:exactMatch rdf:resource="https://opensource.org/licenses/OCLC-2.0"/>
      <skos:inScheme rdf:resource="http://publications.europa.eu/resource/authority/licence"/>
      <skos:topConceptOf rdf:resource="http://publications.europa.eu/resource/authority/licence"/>
   </skos:Concept>
   <skos:Concept rdf:about="http://publications.europa.eu/resource/authority/licence/ODC_BL"
                 at:deprecated="false">
      <skos:prefLabel xml:lang="en">Open Data Commons Open Database License v1.0</skos:prefLabel>
      <at:authority-code>ODC_BL</at:authority-code>
      <at:op-code>ODC_BL</at:op-code>
      <at:start.use>2009-01-01</at:start.use>
      <atold:op-code>ODC_BL</atold:op-code>
      <dc:identifier>ODC_BL</dc:identifier>
      <skos:altLabel xml:lang="bg">ODbL</skos:altLabel>
      <skos:altLabel xml:lang="cs">ODbL</skos:altLabel>
      <skos:altLabel xml:lang="da">ODbL</skos:altLabel>
      <skos:altLabel xml:lang="de">ODbL</skos:altLabel>
      <skos:altLabel xml:lang="el">ODbL</skos:altLabel>
      <skos:altLabel xml:lang="en">ODbL</skos:altLabel>
      <skos:altLabel xml:lang="es">ODbL</skos:altLabel>
      <skos:altLabel xml:lang="et">ODbL</skos:altLabel>
      <skos:altLabel xml:lang="fi">ODbL</skos:altLabel>
      <skos:altLabel xml:lang="fr">ODbL</skos:altLabel>
      <skos:altLabel xml:lang="ga">ODbL</skos:altLabel>
      <skos:altLabel xml:lang="hr">ODbL</skos:altLabel>
      <skos:altLabel xml:lang="hu">ODbL</skos:altLabel>
      <skos:altLabel xml:lang="it">ODbL</skos:altLabel>
      <skos:altLabel xml:lang="lt">ODbL</skos:altLabel>
      <skos:altLabel xml:lang="lv">ODbL</skos:altLabel>
      <skos:altLabel xml:lang="mt">ODbL</skos:altLabel>
      <skos:altLabel xml:lang="nl">ODbL</skos:altLabel>
      <skos:altLabel xml:lang="pl">ODbL</skos:altLabel>
      <skos:altLabel xml:lang="pt">ODbL</skos:altLabel>
      <skos:altLabel xml:lang="ro">ODbL</skos:altLabel>
      <skos:altLabel xml:lang="sk">ODbL</skos:altLabel>
      <skos:altLabel xml:lang="sl">ODbL</skos:altLabel>
      <skos:altLabel xml:lang="sv">ODbL</skos:altLabel>
      <skos:definition xml:lang="en">ODbL is a licence agreement intended to allow users to freely share, modify, and use the database concerned while maintaining this same freedom for others. Some jurisdictions, mainly in the European Union, have specific rights that cover databases, and so this licence addresses these rights, too. This licence is also an agreement in contract for users of this database to act in certain ways in return for accessing the database concerned.</skos:definition>
      <skos:definition xml:lang="fr">ODbL est un contrat de licence ayant pour objet d’autoriser les utilisateurs à partager, modifier et utiliser librement la base de données initiale tout en maintenant ces mêmes libertés pour les autres. De nombreuses bases de données étant protégées par des droits d’auteur, les présentes règles ont pour objet de céder ces droits. Certains États, principalement au sein de l’Union européenne, prévoient des droits spécifiques régissant les bases de données, de ce fait ces droits sont également concernés par cette licence. Cette licence est aussi un contrat en ce que les utilisateurs de la base de données initiale s’engagent à respecter certaines obligations en contrepartie de l’autorisation d’accéder à ladite base de données initiale.</skos:definition>
      <skos:exactMatch rdf:resource="http://opendatacommons.org/licenses/odbl/1.0/"/>
      <skos:inScheme rdf:resource="http://publications.europa.eu/resource/authority/licence"/>
      <skos:topConceptOf rdf:resource="http://publications.europa.eu/resource/authority/licence"/>
   </skos:Concept>
   <skos:Concept rdf:about="http://publications.europa.eu/resource/authority/licence/ODC_BY"
                 at:deprecated="false">
      <skos:prefLabel xml:lang="en">Open Data Commons Attribution License v1.0</skos:prefLabel>
      <at:authority-code>ODC_BY</at:authority-code>
      <at:op-code>ODC_BY</at:op-code>
      <at:start.use>2010-10-24</at:start.use>
      <atold:op-code>ODC_BY</atold:op-code>
      <dc:identifier>ODC_BY</dc:identifier>
      <skos:altLabel xml:lang="bg">ODC-By-1.0</skos:altLabel>
      <skos:altLabel xml:lang="cs">ODC-By-1.0</skos:altLabel>
      <skos:altLabel xml:lang="da">ODC-By-1.0</skos:altLabel>
      <skos:altLabel xml:lang="de">ODC-By-1.0</skos:altLabel>
      <skos:altLabel xml:lang="el">ODC-By-1.0</skos:altLabel>
      <skos:altLabel xml:lang="en">ODC-By-1.0</skos:altLabel>
      <skos:altLabel xml:lang="es">ODC-By-1.0</skos:altLabel>
      <skos:altLabel xml:lang="et">ODC-By-1.0</skos:altLabel>
      <skos:altLabel xml:lang="fi">ODC-By-1.0</skos:altLabel>
      <skos:altLabel xml:lang="fr">ODC-By-1.0</skos:altLabel>
      <skos:altLabel xml:lang="ga">ODC-By-1.0</skos:altLabel>
      <skos:altLabel xml:lang="hr">ODC-By-1.0</skos:altLabel>
      <skos:altLabel xml:lang="hu">ODC-By-1.0</skos:altLabel>
      <skos:altLabel xml:lang="it">ODC-By-1.0</skos:altLabel>
      <skos:altLabel xml:lang="lt">ODC-By-1.0</skos:altLabel>
      <skos:altLabel xml:lang="lv">ODC-By-1.0</skos:altLabel>
      <skos:altLabel xml:lang="mt">ODC-By-1.0</skos:altLabel>
      <skos:altLabel xml:lang="nl">ODC-By-1.0</skos:altLabel>
      <skos:altLabel xml:lang="pl">ODC-By-1.0</skos:altLabel>
      <skos:altLabel xml:lang="pt">ODC-By-1.0</skos:altLabel>
      <skos:altLabel xml:lang="ro">ODC-By-1.0</skos:altLabel>
      <skos:altLabel xml:lang="sk">ODC-By-1.0</skos:altLabel>
      <skos:altLabel xml:lang="sl">ODC-By-1.0</skos:altLabel>
      <skos:altLabel xml:lang="sv">ODC-By-1.0</skos:altLabel>
      <skos:definition xml:lang="en">ODC-By-1.0 is a licence agreement intended to allow users to freely share, modify, and use the database concerned subject only to the attribution requirements set out in Section 4 (notices, no sublicensing). Databases can contain a wide variety of types of content, and so this licence only governs the rights over the database, and not the contents of the database individually.</skos:definition>
      <skos:exactMatch rdf:resource="http://opendatacommons.org/licenses/by/1.0/"/>
      <skos:inScheme rdf:resource="http://publications.europa.eu/resource/authority/licence"/>
      <skos:topConceptOf rdf:resource="http://publications.europa.eu/resource/authority/licence"/>
   </skos:Concept>
   <skos:Concept rdf:about="http://publications.europa.eu/resource/authority/licence/ODC_PDDL"
                 at:deprecated="false">
      <skos:prefLabel xml:lang="en">Open Data Commons Public Domain Dedication and License 1.0</skos:prefLabel>
      <at:authority-code>ODC_PDDL</at:authority-code>
      <at:op-code>ODC_PDDL</at:op-code>
      <at:start.use>2008-03-01</at:start.use>
      <atold:op-code>ODC_PDDL</atold:op-code>
      <dc:identifier>ODC_PDDL</dc:identifier>
      <skos:altLabel xml:lang="bg">PDDL</skos:altLabel>
      <skos:altLabel xml:lang="cs">PDDL</skos:altLabel>
      <skos:altLabel xml:lang="da">PDDL</skos:altLabel>
      <skos:altLabel xml:lang="de">PDDL</skos:altLabel>
      <skos:altLabel xml:lang="el">PDDL</skos:altLabel>
      <skos:altLabel xml:lang="en">PDDL</skos:altLabel>
      <skos:altLabel xml:lang="es">PDDL</skos:altLabel>
      <skos:altLabel xml:lang="et">PDDL</skos:altLabel>
      <skos:altLabel xml:lang="fi">PDDL</skos:altLabel>
      <skos:altLabel xml:lang="fr">PDDL</skos:altLabel>
      <skos:altLabel xml:lang="ga">PDDL</skos:altLabel>
      <skos:altLabel xml:lang="hr">PDDL</skos:altLabel>
      <skos:altLabel xml:lang="hu">PDDL</skos:altLabel>
      <skos:altLabel xml:lang="it">PDDL</skos:altLabel>
      <skos:altLabel xml:lang="lt">PDDL</skos:altLabel>
      <skos:altLabel xml:lang="lv">PDDL</skos:altLabel>
      <skos:altLabel xml:lang="mt">PDDL</skos:altLabel>
      <skos:altLabel xml:lang="nl">PDDL</skos:altLabel>
      <skos:altLabel xml:lang="pl">PDDL</skos:altLabel>
      <skos:altLabel xml:lang="pt">PDDL</skos:altLabel>
      <skos:altLabel xml:lang="ro">PDDL</skos:altLabel>
      <skos:altLabel xml:lang="sk">PDDL</skos:altLabel>
      <skos:altLabel xml:lang="sl">PDDL</skos:altLabel>
      <skos:altLabel xml:lang="sv">PDDL</skos:altLabel>
      <skos:changeNote xml:lang="en">https://www.geeklawblog.com/2010/10/creative-commons-releases-public-domain.html</skos:changeNote>
      <skos:definition xml:lang="en">ODC PDDL is a document intended to allow the user to freely share, modify, and use this work for any purpose and without any restrictions. It is intended for use on databases or their contents (“data”), either together or individually.</skos:definition>
      <skos:exactMatch rdf:resource="http://opendatacommons.org/licenses/pddl/1.0/"/>
      <skos:inScheme rdf:resource="http://publications.europa.eu/resource/authority/licence"/>
      <skos:topConceptOf rdf:resource="http://publications.europa.eu/resource/authority/licence"/>
   </skos:Concept>
   <skos:Concept rdf:about="http://publications.europa.eu/resource/authority/licence/OFL_1_1"
                 at:deprecated="false">
      <skos:prefLabel xml:lang="en">SIL Open Font License (OFL-1.1)</skos:prefLabel>
      <at:authority-code>OFL_1_1</at:authority-code>
      <at:op-code>OFL_1_1</at:op-code>
      <at:start.use>2007-02-26</at:start.use>
      <atold:op-code>OFL_1_1</atold:op-code>
      <dc:identifier>OFL_1_1</dc:identifier>
      <skos:altLabel xml:lang="bg">OFL-1.1</skos:altLabel>
      <skos:altLabel xml:lang="cs">OFL-1.1</skos:altLabel>
      <skos:altLabel xml:lang="da">OFL-1.1</skos:altLabel>
      <skos:altLabel xml:lang="de">OFL-1.1</skos:altLabel>
      <skos:altLabel xml:lang="el">OFL-1.1</skos:altLabel>
      <skos:altLabel xml:lang="en">OFL-1.1</skos:altLabel>
      <skos:altLabel xml:lang="es">OFL-1.1</skos:altLabel>
      <skos:altLabel xml:lang="et">OFL-1.1</skos:altLabel>
      <skos:altLabel xml:lang="fi">OFL-1.1</skos:altLabel>
      <skos:altLabel xml:lang="fr">OFL-1.1</skos:altLabel>
      <skos:altLabel xml:lang="ga">OFL-1.1</skos:altLabel>
      <skos:altLabel xml:lang="hr">OFL-1.1</skos:altLabel>
      <skos:altLabel xml:lang="hu">OFL-1.1</skos:altLabel>
      <skos:altLabel xml:lang="it">OFL-1.1</skos:altLabel>
      <skos:altLabel xml:lang="lt">OFL-1.1</skos:altLabel>
      <skos:altLabel xml:lang="lv">OFL-1.1</skos:altLabel>
      <skos:altLabel xml:lang="mt">OFL-1.1</skos:altLabel>
      <skos:altLabel xml:lang="nl">OFL-1.1</skos:altLabel>
      <skos:altLabel xml:lang="pl">OFL-1.1</skos:altLabel>
      <skos:altLabel xml:lang="pt">OFL-1.1</skos:altLabel>
      <skos:altLabel xml:lang="ro">OFL-1.1</skos:altLabel>
      <skos:altLabel xml:lang="sk">OFL-1.1</skos:altLabel>
      <skos:altLabel xml:lang="sl">OFL-1.1</skos:altLabel>
      <skos:altLabel xml:lang="sv">OFL-1.1</skos:altLabel>
      <skos:changeNote xml:lang="en">The source of the start-use date: https://scripts.sil.org/cms/scripts/page.php?site_id=nrsi&amp;id=OFL</skos:changeNote>
      <skos:definition xml:lang="en">The SIL Open Font License 1.1 is one of the major open font licences, which allows embedding of the font in commercially sold products. It is a free and open source licence approved by the Open Source Initiative.</skos:definition>
      <skos:exactMatch rdf:resource="https://opensource.org/licenses/OFL-1.1"/>
      <skos:inScheme rdf:resource="http://publications.europa.eu/resource/authority/licence"/>
      <skos:topConceptOf rdf:resource="http://publications.europa.eu/resource/authority/licence"/>
   </skos:Concept>
   <skos:Concept rdf:about="http://publications.europa.eu/resource/authority/licence/OGL_1_0"
                 at:deprecated="false">
      <skos:prefLabel xml:lang="en">Open Government Licence 1.0</skos:prefLabel>
      <at:authority-code>OGL_1_0</at:authority-code>
      <at:op-code>OGL_1_0</at:op-code>
      <at:start.use>2010-09-01</at:start.use>
      <atold:op-code>OGL_1_0</atold:op-code>
      <dc:identifier>OGL_1_0</dc:identifier>
      <skos:altLabel xml:lang="bg">OGL 1.0</skos:altLabel>
      <skos:altLabel xml:lang="cs">OGL 1.0</skos:altLabel>
      <skos:altLabel xml:lang="da">OGL 1.0</skos:altLabel>
      <skos:altLabel xml:lang="de">OGL 1.0</skos:altLabel>
      <skos:altLabel xml:lang="el">OGL 1.0</skos:altLabel>
      <skos:altLabel xml:lang="en">OGL 1.0</skos:altLabel>
      <skos:altLabel xml:lang="es">OGL 1.0</skos:altLabel>
      <skos:altLabel xml:lang="et">OGL 1.0</skos:altLabel>
      <skos:altLabel xml:lang="fi">OGL 1.0</skos:altLabel>
      <skos:altLabel xml:lang="fr">OGL 1.0</skos:altLabel>
      <skos:altLabel xml:lang="ga">OGL 1.0</skos:altLabel>
      <skos:altLabel xml:lang="hr">OGL 1.0</skos:altLabel>
      <skos:altLabel xml:lang="hu">OGL 1.0</skos:altLabel>
      <skos:altLabel xml:lang="it">OGL 1.0</skos:altLabel>
      <skos:altLabel xml:lang="lt">OGL 1.0</skos:altLabel>
      <skos:altLabel xml:lang="lv">OGL 1.0</skos:altLabel>
      <skos:altLabel xml:lang="mt">OGL 1.0</skos:altLabel>
      <skos:altLabel xml:lang="nl">OGL 1.0</skos:altLabel>
      <skos:altLabel xml:lang="pl">OGL 1.0</skos:altLabel>
      <skos:altLabel xml:lang="pt">OGL 1.0</skos:altLabel>
      <skos:altLabel xml:lang="ro">OGL 1.0</skos:altLabel>
      <skos:altLabel xml:lang="sk">OGL 1.0</skos:altLabel>
      <skos:altLabel xml:lang="sl">OGL 1.0</skos:altLabel>
      <skos:altLabel xml:lang="sv">OGL 1.0</skos:altLabel>
      <skos:changeNote xml:lang="en">The source of the start-use date: https://en.wikipedia.org/wiki/Open_Government_Licence</skos:changeNote>
      <skos:definition xml:lang="en">Developed and maintained by the National Archives, OGL-1.0 is a copyright licence for Crown Copyright works published by the UK government consisting of a simple set of terms and conditions facilitating the re-use of a wide range of public sector information free of charge. The OGL terms are compatible with the latest versions of the Creative Commons Attribution Licence and the Open Data Commons Attribution Licence. The OGL is a perpetual licence so any past and continuing use of information authorised under v1.0 or v2.0 may continue.</skos:definition>
      <skos:exactMatch rdf:resource="http://www.nationalarchives.gov.uk/doc/open-government-licence/version/1/"/>
      <skos:inScheme rdf:resource="http://publications.europa.eu/resource/authority/licence"/>
      <skos:topConceptOf rdf:resource="http://publications.europa.eu/resource/authority/licence"/>
   </skos:Concept>
   <skos:Concept rdf:about="http://publications.europa.eu/resource/authority/licence/OGL_2_0"
                 at:deprecated="false">
      <skos:prefLabel xml:lang="en">Open Government Licence 2.0</skos:prefLabel>
      <at:authority-code>OGL_2_0</at:authority-code>
      <at:op-code>OGL_2_0</at:op-code>
      <at:start.use>2013-06-28</at:start.use>
      <atold:op-code>OGL_2_0</atold:op-code>
      <dc:identifier>OGL_2_0</dc:identifier>
      <skos:altLabel xml:lang="bg">OGL 2.0</skos:altLabel>
      <skos:altLabel xml:lang="cs">OGL 2.0</skos:altLabel>
      <skos:altLabel xml:lang="da">OGL 2.0</skos:altLabel>
      <skos:altLabel xml:lang="de">OGL 2.0</skos:altLabel>
      <skos:altLabel xml:lang="el">OGL 2.0</skos:altLabel>
      <skos:altLabel xml:lang="en">OGL 2.0</skos:altLabel>
      <skos:altLabel xml:lang="es">OGL 2.0</skos:altLabel>
      <skos:altLabel xml:lang="et">OGL 2.0</skos:altLabel>
      <skos:altLabel xml:lang="fi">OGL 2.0</skos:altLabel>
      <skos:altLabel xml:lang="fr">OGL 2.0</skos:altLabel>
      <skos:altLabel xml:lang="ga">OGL 2.0</skos:altLabel>
      <skos:altLabel xml:lang="hr">OGL 2.0</skos:altLabel>
      <skos:altLabel xml:lang="hu">OGL 2.0</skos:altLabel>
      <skos:altLabel xml:lang="it">OGL 2.0</skos:altLabel>
      <skos:altLabel xml:lang="lt">OGL 2.0</skos:altLabel>
      <skos:altLabel xml:lang="lv">OGL 2.0</skos:altLabel>
      <skos:altLabel xml:lang="mt">OGL 2.0</skos:altLabel>
      <skos:altLabel xml:lang="nl">OGL 2.0</skos:altLabel>
      <skos:altLabel xml:lang="pl">OGL 2.0</skos:altLabel>
      <skos:altLabel xml:lang="pt">OGL 2.0</skos:altLabel>
      <skos:altLabel xml:lang="ro">OGL 2.0</skos:altLabel>
      <skos:altLabel xml:lang="sk">OGL 2.0</skos:altLabel>
      <skos:altLabel xml:lang="sl">OGL 2.0</skos:altLabel>
      <skos:altLabel xml:lang="sv">OGL 2.0</skos:altLabel>
      <skos:changeNote xml:lang="en">The source of the start-use date: https://en.wikipedia.org/wiki/Open_Government_Licence</skos:changeNote>
      <skos:definition xml:lang="en">Developed and maintained by the National Archives, OGL-2.0 is a copyright licence for Crown Copyright works published by the UK government consisting of a simple set of terms and conditions facilitating the re-use of a wide range of public sector information free of charge. The OGL terms are compatible with the latest versions of the Creative Commons Attribution Licence and the Open Data Commons Attribution Licence. The OGL is a perpetual licence so any past and continuing use of information authorised under v1.0 or v2.0 may continue.</skos:definition>
      <skos:exactMatch rdf:resource="http://www.nationalarchives.gov.uk/doc/open-government-licence/version/2/"/>
      <skos:inScheme rdf:resource="http://publications.europa.eu/resource/authority/licence"/>
      <skos:topConceptOf rdf:resource="http://publications.europa.eu/resource/authority/licence"/>
   </skos:Concept>
   <skos:Concept rdf:about="http://publications.europa.eu/resource/authority/licence/OGL_3_0"
                 at:deprecated="false">
      <skos:prefLabel xml:lang="en">Open Government Licence 3.0</skos:prefLabel>
      <at:authority-code>OGL_3_0</at:authority-code>
      <at:op-code>OGL_3_0</at:op-code>
      <at:start.use>2014-10-31</at:start.use>
      <atold:op-code>OGL_3_0</atold:op-code>
      <dc:identifier>OGL_3_0</dc:identifier>
      <skos:altLabel xml:lang="bg">OGL 3.0</skos:altLabel>
      <skos:altLabel xml:lang="cs">OGL 3.0</skos:altLabel>
      <skos:altLabel xml:lang="da">OGL 3.0</skos:altLabel>
      <skos:altLabel xml:lang="de">OGL 3.0</skos:altLabel>
      <skos:altLabel xml:lang="el">OGL 3.0</skos:altLabel>
      <skos:altLabel xml:lang="en">OGL 3.0</skos:altLabel>
      <skos:altLabel xml:lang="es">OGL 3.0</skos:altLabel>
      <skos:altLabel xml:lang="et">OGL 3.0</skos:altLabel>
      <skos:altLabel xml:lang="fi">OGL 3.0</skos:altLabel>
      <skos:altLabel xml:lang="fr">OGL 3.0</skos:altLabel>
      <skos:altLabel xml:lang="ga">OGL 3.0</skos:altLabel>
      <skos:altLabel xml:lang="hr">OGL 3.0</skos:altLabel>
      <skos:altLabel xml:lang="hu">OGL 3.0</skos:altLabel>
      <skos:altLabel xml:lang="it">OGL 3.0</skos:altLabel>
      <skos:altLabel xml:lang="lt">OGL 3.0</skos:altLabel>
      <skos:altLabel xml:lang="lv">OGL 3.0</skos:altLabel>
      <skos:altLabel xml:lang="mt">OGL 3.0</skos:altLabel>
      <skos:altLabel xml:lang="nl">OGL 3.0</skos:altLabel>
      <skos:altLabel xml:lang="pl">OGL 3.0</skos:altLabel>
      <skos:altLabel xml:lang="pt">OGL 3.0</skos:altLabel>
      <skos:altLabel xml:lang="ro">OGL 3.0</skos:altLabel>
      <skos:altLabel xml:lang="sk">OGL 3.0</skos:altLabel>
      <skos:altLabel xml:lang="sl">OGL 3.0</skos:altLabel>
      <skos:altLabel xml:lang="sv">OGL 3.0</skos:altLabel>
      <skos:changeNote xml:lang="en">The source of the start-use date: https://en.wikipedia.org/wiki/Open_Government_Licence</skos:changeNote>
      <skos:definition xml:lang="en">Developed and maintained by the National Archives, OGL-3.0 is a copyright licence for Crown Copyright works published by the UK government consisting of a simple set of terms and conditions facilitating the re-use of a wide range of public sector information free of charge. The OGL terms are compatible with the latest versions of the Creative Commons Attribution Licence and the Open Data Commons Attribution Licence. The OGL is a perpetual licence so any past and continuing use of information authorised under v1.0 or v2.0 may continue.</skos:definition>
      <skos:exactMatch rdf:resource="http://www.nationalarchives.gov.uk/doc/open-government-licence/version/3/"/>
      <skos:inScheme rdf:resource="http://publications.europa.eu/resource/authority/licence"/>
      <skos:topConceptOf rdf:resource="http://publications.europa.eu/resource/authority/licence"/>
   </skos:Concept>
   <skos:Concept rdf:about="http://publications.europa.eu/resource/authority/licence/OGL_NC"
                 at:deprecated="false">
      <skos:prefLabel xml:lang="en">Non-Commercial Government Licence</skos:prefLabel>
      <at:authority-code>OGL_NC</at:authority-code>
      <at:op-code>OGL_NC</at:op-code>
      <at:start.use>2013-06-28</at:start.use>
      <atold:op-code>OGL_NC</atold:op-code>
      <dc:identifier>OGL_NC</dc:identifier>
      <skos:altLabel xml:lang="bg">OGL-NC</skos:altLabel>
      <skos:altLabel xml:lang="cs">OGL-NC</skos:altLabel>
      <skos:altLabel xml:lang="da">OGL-NC</skos:altLabel>
      <skos:altLabel xml:lang="de">OGL-NC</skos:altLabel>
      <skos:altLabel xml:lang="el">OGL-NC</skos:altLabel>
      <skos:altLabel xml:lang="en">OGL-NC</skos:altLabel>
      <skos:altLabel xml:lang="es">OGL-NC</skos:altLabel>
      <skos:altLabel xml:lang="et">OGL-NC</skos:altLabel>
      <skos:altLabel xml:lang="fi">OGL-NC</skos:altLabel>
      <skos:altLabel xml:lang="fr">OGL-NC</skos:altLabel>
      <skos:altLabel xml:lang="ga">OGL-NC</skos:altLabel>
      <skos:altLabel xml:lang="hr">OGL-NC</skos:altLabel>
      <skos:altLabel xml:lang="hu">OGL-NC</skos:altLabel>
      <skos:altLabel xml:lang="it">OGL-NC</skos:altLabel>
      <skos:altLabel xml:lang="lt">OGL-NC</skos:altLabel>
      <skos:altLabel xml:lang="lv">OGL-NC</skos:altLabel>
      <skos:altLabel xml:lang="mt">OGL-NC</skos:altLabel>
      <skos:altLabel xml:lang="nl">OGL-NC</skos:altLabel>
      <skos:altLabel xml:lang="pl">OGL-NC</skos:altLabel>
      <skos:altLabel xml:lang="pt">OGL-NC</skos:altLabel>
      <skos:altLabel xml:lang="ro">OGL-NC</skos:altLabel>
      <skos:altLabel xml:lang="sk">OGL-NC</skos:altLabel>
      <skos:altLabel xml:lang="sl">OGL-NC</skos:altLabel>
      <skos:altLabel xml:lang="sv">OGL-NC</skos:altLabel>
      <skos:changeNote xml:lang="en">The source of the start-use date: https://en.wikipedia.org/wiki/Open_Government_Licence</skos:changeNote>
      <skos:definition xml:lang="en">Developed and maintained by the National Archives, the Non-Commercial Government Licence (OGL-NC) may be used by public sector bodies that have a Delegation of Authority to licence Crown copyright material non-commercially. It may also be used by public sector bodies holding non-Crown copyright information in accordance with the PSI Regulations 2015.</skos:definition>
      <skos:exactMatch rdf:resource="http://www.nationalarchives.gov.uk/doc/non-commercial-government-licence/non-commercial-government-licence.htm"/>
      <skos:inScheme rdf:resource="http://publications.europa.eu/resource/authority/licence"/>
      <skos:topConceptOf rdf:resource="http://publications.europa.eu/resource/authority/licence"/>
   </skos:Concept>
   <skos:Concept rdf:about="http://publications.europa.eu/resource/authority/licence/OGL_ROU_1_0"
                 at:deprecated="false">
      <skos:prefLabel xml:lang="en">Non-Commercial Government Licence 1.0</skos:prefLabel>
      <at:authority-code>OGL_ROU_1_0</at:authority-code>
      <at:op-code>OGL_ROU_1_0</at:op-code>
      <at:start.use>2010-09-01</at:start.use>
      <atold:op-code>OGL_ROU_1_0</atold:op-code>
      <dc:identifier>OGL_ROU_1_0</dc:identifier>
      <skos:altLabel xml:lang="bg">OGL-ROU 1.0</skos:altLabel>
      <skos:altLabel xml:lang="cs">OGL-ROU 1.0</skos:altLabel>
      <skos:altLabel xml:lang="da">OGL-ROU 1.0</skos:altLabel>
      <skos:altLabel xml:lang="de">OGL-ROU 1.0</skos:altLabel>
      <skos:altLabel xml:lang="el">OGL-ROU 1.0</skos:altLabel>
      <skos:altLabel xml:lang="en">OGL-ROU 1.0</skos:altLabel>
      <skos:altLabel xml:lang="es">OGL-ROU 1.0</skos:altLabel>
      <skos:altLabel xml:lang="et">OGL-ROU 1.0</skos:altLabel>
      <skos:altLabel xml:lang="fi">OGL-ROU 1.0</skos:altLabel>
      <skos:altLabel xml:lang="fr">OGL-ROU 1.0</skos:altLabel>
      <skos:altLabel xml:lang="ga">OGL-ROU 1.0</skos:altLabel>
      <skos:altLabel xml:lang="hr">OGL-ROU 1.0</skos:altLabel>
      <skos:altLabel xml:lang="hu">OGL-ROU 1.0</skos:altLabel>
      <skos:altLabel xml:lang="it">OGL-ROU 1.0</skos:altLabel>
      <skos:altLabel xml:lang="lt">OGL-ROU 1.0</skos:altLabel>
      <skos:altLabel xml:lang="lv">OGL-ROU 1.0</skos:altLabel>
      <skos:altLabel xml:lang="mt">OGL-ROU 1.0</skos:altLabel>
      <skos:altLabel xml:lang="nl">OGL-ROU 1.0</skos:altLabel>
      <skos:altLabel xml:lang="pl">OGL-ROU 1.0</skos:altLabel>
      <skos:altLabel xml:lang="pt">OGL-ROU 1.0</skos:altLabel>
      <skos:altLabel xml:lang="ro">OGL-ROU 1.0</skos:altLabel>
      <skos:altLabel xml:lang="sk">OGL-ROU 1.0</skos:altLabel>
      <skos:altLabel xml:lang="sl">OGL-ROU 1.0</skos:altLabel>
      <skos:altLabel xml:lang="sv">OGL-ROU 1.0</skos:altLabel>
      <skos:changeNote xml:lang="en">The source of the start-use date: https://en.wikipedia.org/wiki/Open_Government_Licence</skos:changeNote>
      <skos:definition xml:lang="en">Having a working value in Romanian, the Non-Commercial Government Licence 1.0 (OGL-ROU 1.0) consists of a simple set of terms and conditions facilitating the re-use of a wide range of public sector information free of charge. The OGL terms are compatible with the latest versions of the Creative Commons Attribution Licence and the Open Data Commons Attribution Licence.</skos:definition>
      <skos:exactMatch rdf:resource="http://data.gov.ro/base/images/logoinst/OGL-ROU-1.0.pdf"/>
      <skos:inScheme rdf:resource="http://publications.europa.eu/resource/authority/licence"/>
      <skos:topConceptOf rdf:resource="http://publications.europa.eu/resource/authority/licence"/>
   </skos:Concept>
   <skos:Concept rdf:about="http://publications.europa.eu/resource/authority/licence/OGTSL"
                 at:deprecated="false">
      <skos:prefLabel xml:lang="en">The Open Group Test Suite License (OGTSL)</skos:prefLabel>
      <at:authority-code>OGTSL</at:authority-code>
      <at:op-code>OGTSL</at:op-code>
      <at:start.use>2007-04-01</at:start.use>
      <atold:op-code>OGTSL</atold:op-code>
      <dc:identifier>OGTSL</dc:identifier>
      <skos:altLabel xml:lang="bg">OGTSL</skos:altLabel>
      <skos:altLabel xml:lang="cs">OGTSL</skos:altLabel>
      <skos:altLabel xml:lang="da">OGTSL</skos:altLabel>
      <skos:altLabel xml:lang="de">OGTSL</skos:altLabel>
      <skos:altLabel xml:lang="el">OGTSL</skos:altLabel>
      <skos:altLabel xml:lang="en">OGTSL</skos:altLabel>
      <skos:altLabel xml:lang="es">OGTSL</skos:altLabel>
      <skos:altLabel xml:lang="et">OGTSL</skos:altLabel>
      <skos:altLabel xml:lang="fi">OGTSL</skos:altLabel>
      <skos:altLabel xml:lang="fr">OGTSL</skos:altLabel>
      <skos:altLabel xml:lang="ga">OGTSL</skos:altLabel>
      <skos:altLabel xml:lang="hr">OGTSL</skos:altLabel>
      <skos:altLabel xml:lang="hu">OGTSL</skos:altLabel>
      <skos:altLabel xml:lang="it">OGTSL</skos:altLabel>
      <skos:altLabel xml:lang="lt">OGTSL</skos:altLabel>
      <skos:altLabel xml:lang="lv">OGTSL</skos:altLabel>
      <skos:altLabel xml:lang="mt">OGTSL</skos:altLabel>
      <skos:altLabel xml:lang="nl">OGTSL</skos:altLabel>
      <skos:altLabel xml:lang="pl">OGTSL</skos:altLabel>
      <skos:altLabel xml:lang="pt">OGTSL</skos:altLabel>
      <skos:altLabel xml:lang="ro">OGTSL</skos:altLabel>
      <skos:altLabel xml:lang="sk">OGTSL</skos:altLabel>
      <skos:altLabel xml:lang="sl">OGTSL</skos:altLabel>
      <skos:altLabel xml:lang="sv">OGTSL</skos:altLabel>
      <skos:changeNote xml:lang="en">The source of the start-use date: https://appaji.livejournal.com/53826.html</skos:changeNote>
      <skos:definition xml:lang="en">OGTSL was meant to facilitate software testing, without placing severe restrictions on use of the software except in terms of including original versions of the software. It is approved by the Open Source Initiative.</skos:definition>
      <skos:exactMatch rdf:resource="https://opensource.org/licenses/OGTSL"/>
      <skos:inScheme rdf:resource="http://publications.europa.eu/resource/authority/licence"/>
      <skos:topConceptOf rdf:resource="http://publications.europa.eu/resource/authority/licence"/>
   </skos:Concept>
   <skos:Concept rdf:about="http://publications.europa.eu/resource/authority/licence/OPL_2_1"
                 at:deprecated="false">
      <skos:prefLabel xml:lang="en">OSET Public License version 2.1</skos:prefLabel>
      <at:authority-code>OPL_2_1</at:authority-code>
      <at:op-code>OPL_2_1</at:op-code>
      <at:start.use>2015-08-31</at:start.use>
      <atold:op-code>OPL_2_1</atold:op-code>
      <dc:identifier>OPL_2_1</dc:identifier>
      <skos:altLabel xml:lang="bg">OPL-2.1</skos:altLabel>
      <skos:altLabel xml:lang="cs">OPL-2.1</skos:altLabel>
      <skos:altLabel xml:lang="da">OPL-2.1</skos:altLabel>
      <skos:altLabel xml:lang="de">OPL-2.1</skos:altLabel>
      <skos:altLabel xml:lang="el">OPL-2.1</skos:altLabel>
      <skos:altLabel xml:lang="en">OPL-2.1</skos:altLabel>
      <skos:altLabel xml:lang="es">OPL-2.1</skos:altLabel>
      <skos:altLabel xml:lang="et">OPL-2.1</skos:altLabel>
      <skos:altLabel xml:lang="fi">OPL-2.1</skos:altLabel>
      <skos:altLabel xml:lang="fr">OPL-2.1</skos:altLabel>
      <skos:altLabel xml:lang="ga">OPL-2.1</skos:altLabel>
      <skos:altLabel xml:lang="hr">OPL-2.1</skos:altLabel>
      <skos:altLabel xml:lang="hu">OPL-2.1</skos:altLabel>
      <skos:altLabel xml:lang="it">OPL-2.1</skos:altLabel>
      <skos:altLabel xml:lang="lt">OPL-2.1</skos:altLabel>
      <skos:altLabel xml:lang="lv">OPL-2.1</skos:altLabel>
      <skos:altLabel xml:lang="mt">OPL-2.1</skos:altLabel>
      <skos:altLabel xml:lang="nl">OPL-2.1</skos:altLabel>
      <skos:altLabel xml:lang="pl">OPL-2.1</skos:altLabel>
      <skos:altLabel xml:lang="pt">OPL-2.1</skos:altLabel>
      <skos:altLabel xml:lang="ro">OPL-2.1</skos:altLabel>
      <skos:altLabel xml:lang="sk">OPL-2.1</skos:altLabel>
      <skos:altLabel xml:lang="sl">OPL-2.1</skos:altLabel>
      <skos:altLabel xml:lang="sv">OPL-2.1</skos:altLabel>
      <skos:changeNote xml:lang="en">The source of the start-use date: https://libraries.io/search?licenses=OSET-PL-2.1&amp;order=desc&amp;page=4&amp;sort=latest_release_published_at</skos:changeNote>
      <skos:definition xml:lang="en">OSET Public License 2.1 is a copyleft-style, free software licence approved by the Open Source Initiative.</skos:definition>
      <skos:exactMatch rdf:resource="https://opensource.org/licenses/OPL-2.1"/>
      <skos:inScheme rdf:resource="http://publications.europa.eu/resource/authority/licence"/>
      <skos:topConceptOf rdf:resource="http://publications.europa.eu/resource/authority/licence"/>
   </skos:Concept>
   <skos:Concept rdf:about="http://publications.europa.eu/resource/authority/licence/OP_DATPRO"
                 at:deprecated="false">
      <skos:prefLabel xml:lang="bg">Неокончателни данни</skos:prefLabel>
      <skos:prefLabel xml:lang="cs">Předběžné údaje</skos:prefLabel>
      <skos:prefLabel xml:lang="da">Midlertidige data</skos:prefLabel>
      <skos:prefLabel xml:lang="de">Vorläufige Daten</skos:prefLabel>
      <skos:prefLabel xml:lang="el">Προσωρινά δεδομένα</skos:prefLabel>
      <skos:prefLabel xml:lang="en">Provisional data</skos:prefLabel>
      <skos:prefLabel xml:lang="es">Datos provisionales</skos:prefLabel>
      <skos:prefLabel xml:lang="et">Esialgsed andmed</skos:prefLabel>
      <skos:prefLabel xml:lang="fi">Alustavat tiedot</skos:prefLabel>
      <skos:prefLabel xml:lang="fr">Données provisoires</skos:prefLabel>
      <skos:prefLabel xml:lang="ga">Sonraí sealadacha</skos:prefLabel>
      <skos:prefLabel xml:lang="hr">Privremeni podaci</skos:prefLabel>
      <skos:prefLabel xml:lang="hu">Ideiglenes adatok</skos:prefLabel>
      <skos:prefLabel xml:lang="it">Dati provvisori</skos:prefLabel>
      <skos:prefLabel xml:lang="lt">Laikinieji duomenys</skos:prefLabel>
      <skos:prefLabel xml:lang="lv">Provizoriski dati</skos:prefLabel>
      <skos:prefLabel xml:lang="mt">Dejta provviżorja</skos:prefLabel>
      <skos:prefLabel xml:lang="nl">Voorlopige gegevens</skos:prefLabel>
      <skos:prefLabel xml:lang="pl">Dane tymczasowe</skos:prefLabel>
      <skos:prefLabel xml:lang="pt">Dados provisórios</skos:prefLabel>
      <skos:prefLabel xml:lang="ro">Date provizorii</skos:prefLabel>
      <skos:prefLabel xml:lang="sk">Predbežné údaje</skos:prefLabel>
      <skos:prefLabel xml:lang="sl">Začasni podatki</skos:prefLabel>
      <skos:prefLabel xml:lang="sv">Tillfälliga uppgifter</skos:prefLabel>
      <at:authority-code>OP_DATPRO</at:authority-code>
      <at:op-code>OP_DATPRO</at:op-code>
      <at:start.use>1952-07-23</at:start.use>
      <atold:op-code>OP_DATPRO</atold:op-code>
      <dc:identifier>OP_DATPRO</dc:identifier>
      <skos:inScheme rdf:resource="http://publications.europa.eu/resource/authority/licence"/>
      <skos:topConceptOf rdf:resource="http://publications.europa.eu/resource/authority/licence"/>
   </skos:Concept>
   <skos:Concept rdf:about="http://publications.europa.eu/resource/authority/licence/OSL_1_0"
                 at:deprecated="true">
      <skos:prefLabel xml:lang="en">Open Software License, version 1.0 (OSL-1.0)</skos:prefLabel>
      <at:authority-code>OSL_1_0</at:authority-code>
      <at:op-code>OSL_1_0</at:op-code>
      <at:start.use>2002-08-31</at:start.use>
      <atold:op-code>OSL_1_0</atold:op-code>
      <dc:identifier>OSL_1_0</dc:identifier>
      <skos:altLabel xml:lang="bg">OSL-1.0</skos:altLabel>
      <skos:altLabel xml:lang="cs">OSL-1.0</skos:altLabel>
      <skos:altLabel xml:lang="da">OSL-1.0</skos:altLabel>
      <skos:altLabel xml:lang="de">OSL-1.0</skos:altLabel>
      <skos:altLabel xml:lang="el">OSL-1.0</skos:altLabel>
      <skos:altLabel xml:lang="en">OSL-1.0</skos:altLabel>
      <skos:altLabel xml:lang="es">OSL-1.0</skos:altLabel>
      <skos:altLabel xml:lang="et">OSL-1.0</skos:altLabel>
      <skos:altLabel xml:lang="fi">OSL-1.0</skos:altLabel>
      <skos:altLabel xml:lang="fr">OSL-1.0</skos:altLabel>
      <skos:altLabel xml:lang="ga">OSL-1.0</skos:altLabel>
      <skos:altLabel xml:lang="hr">OSL-1.0</skos:altLabel>
      <skos:altLabel xml:lang="hu">OSL-1.0</skos:altLabel>
      <skos:altLabel xml:lang="it">OSL-1.0</skos:altLabel>
      <skos:altLabel xml:lang="lt">OSL-1.0</skos:altLabel>
      <skos:altLabel xml:lang="lv">OSL-1.0</skos:altLabel>
      <skos:altLabel xml:lang="mt">OSL-1.0</skos:altLabel>
      <skos:altLabel xml:lang="nl">OSL-1.0</skos:altLabel>
      <skos:altLabel xml:lang="pl">OSL-1.0</skos:altLabel>
      <skos:altLabel xml:lang="pt">OSL-1.0</skos:altLabel>
      <skos:altLabel xml:lang="ro">OSL-1.0</skos:altLabel>
      <skos:altLabel xml:lang="sk">OSL-1.0</skos:altLabel>
      <skos:altLabel xml:lang="sl">OSL-1.0</skos:altLabel>
      <skos:altLabel xml:lang="sv">OSL-1.0</skos:altLabel>
      <skos:changeNote xml:lang="en">The source of the start-use date: https://old.computerra.ru/2002/466/200189/</skos:changeNote>
      <skos:definition xml:lang="en">Open Software License 1.0 is a copyleft-style, free software licence approved by the Open Source Initiative.</skos:definition>
      <skos:exactMatch rdf:resource="https://opensource.org/licenses/OSL-1.0"/>
      <skos:inScheme rdf:resource="http://publications.europa.eu/resource/authority/licence"/>
      <skos:topConceptOf rdf:resource="http://publications.europa.eu/resource/authority/licence"/>
      <at:end.use>2005-11-30</at:end.use>
   </skos:Concept>
   <skos:Concept rdf:about="http://publications.europa.eu/resource/authority/licence/OSL_2_1"
                 at:deprecated="true">
      <skos:prefLabel xml:lang="en">The Open Software License, version 2.1 (OSL-2.1)</skos:prefLabel>
      <at:authority-code>OSL_2_1</at:authority-code>
      <at:op-code>OSL_2_1</at:op-code>
      <at:start.use>2003-10-31</at:start.use>
      <atold:op-code>OSL_2_1</atold:op-code>
      <dc:identifier>OSL_2_1</dc:identifier>
      <skos:altLabel xml:lang="bg">OSL-2.1</skos:altLabel>
      <skos:altLabel xml:lang="cs">OSL-2.1</skos:altLabel>
      <skos:altLabel xml:lang="da">OSL-2.1</skos:altLabel>
      <skos:altLabel xml:lang="de">OSL-2.1</skos:altLabel>
      <skos:altLabel xml:lang="el">OSL-2.1</skos:altLabel>
      <skos:altLabel xml:lang="en">OSL-2.1</skos:altLabel>
      <skos:altLabel xml:lang="es">OSL-2.1</skos:altLabel>
      <skos:altLabel xml:lang="et">OSL-2.1</skos:altLabel>
      <skos:altLabel xml:lang="fi">OSL-2.1</skos:altLabel>
      <skos:altLabel xml:lang="fr">OSL-2.1</skos:altLabel>
      <skos:altLabel xml:lang="ga">OSL-2.1</skos:altLabel>
      <skos:altLabel xml:lang="hr">OSL-2.1</skos:altLabel>
      <skos:altLabel xml:lang="hu">OSL-2.1</skos:altLabel>
      <skos:altLabel xml:lang="it">OSL-2.1</skos:altLabel>
      <skos:altLabel xml:lang="lt">OSL-2.1</skos:altLabel>
      <skos:altLabel xml:lang="lv">OSL-2.1</skos:altLabel>
      <skos:altLabel xml:lang="mt">OSL-2.1</skos:altLabel>
      <skos:altLabel xml:lang="nl">OSL-2.1</skos:altLabel>
      <skos:altLabel xml:lang="pl">OSL-2.1</skos:altLabel>
      <skos:altLabel xml:lang="pt">OSL-2.1</skos:altLabel>
      <skos:altLabel xml:lang="ro">OSL-2.1</skos:altLabel>
      <skos:altLabel xml:lang="sk">OSL-2.1</skos:altLabel>
      <skos:altLabel xml:lang="sl">OSL-2.1</skos:altLabel>
      <skos:altLabel xml:lang="sv">OSL-2.1</skos:altLabel>
      <skos:changeNote xml:lang="en">The source of the start-use date: https://lists.debian.org/debian-legal/2003/11/msg00181.html</skos:changeNote>
      <skos:definition xml:lang="en">Open Software License 2.1 is a copyleft-style, free software licence approved by the Open Source Initiative.</skos:definition>
      <skos:exactMatch rdf:resource="https://opensource.org/licenses/OSL-2.1"/>
      <skos:inScheme rdf:resource="http://publications.europa.eu/resource/authority/licence"/>
      <skos:topConceptOf rdf:resource="http://publications.europa.eu/resource/authority/licence"/>
      <at:end.use>2005-11-30</at:end.use>
   </skos:Concept>
   <skos:Concept rdf:about="http://publications.europa.eu/resource/authority/licence/OSL_3_0"
                 at:deprecated="false">
      <skos:prefLabel xml:lang="en">Open Software License, version 3.0 (OSL-3.0)</skos:prefLabel>
      <at:authority-code>OSL_3_0</at:authority-code>
      <at:op-code>OSL_3_0</at:op-code>
      <at:start.use>2005-12-01</at:start.use>
      <atold:op-code>OSL_3_0</atold:op-code>
      <dc:identifier>OSL_3_0</dc:identifier>
      <skos:altLabel xml:lang="bg">OSL-3.0</skos:altLabel>
      <skos:altLabel xml:lang="cs">OSL-3.0</skos:altLabel>
      <skos:altLabel xml:lang="da">OSL-3.0</skos:altLabel>
      <skos:altLabel xml:lang="de">OSL-3.0</skos:altLabel>
      <skos:altLabel xml:lang="el">OSL-3.0</skos:altLabel>
      <skos:altLabel xml:lang="en">OSL-3.0</skos:altLabel>
      <skos:altLabel xml:lang="es">OSL-3.0</skos:altLabel>
      <skos:altLabel xml:lang="et">OSL-3.0</skos:altLabel>
      <skos:altLabel xml:lang="fi">OSL-3.0</skos:altLabel>
      <skos:altLabel xml:lang="fr">OSL-3.0</skos:altLabel>
      <skos:altLabel xml:lang="ga">OSL-3.0</skos:altLabel>
      <skos:altLabel xml:lang="hr">OSL-3.0</skos:altLabel>
      <skos:altLabel xml:lang="hu">OSL-3.0</skos:altLabel>
      <skos:altLabel xml:lang="it">OSL-3.0</skos:altLabel>
      <skos:altLabel xml:lang="lt">OSL-3.0</skos:altLabel>
      <skos:altLabel xml:lang="lv">OSL-3.0</skos:altLabel>
      <skos:altLabel xml:lang="mt">OSL-3.0</skos:altLabel>
      <skos:altLabel xml:lang="nl">OSL-3.0</skos:altLabel>
      <skos:altLabel xml:lang="pl">OSL-3.0</skos:altLabel>
      <skos:altLabel xml:lang="pt">OSL-3.0</skos:altLabel>
      <skos:altLabel xml:lang="ro">OSL-3.0</skos:altLabel>
      <skos:altLabel xml:lang="sk">OSL-3.0</skos:altLabel>
      <skos:altLabel xml:lang="sl">OSL-3.0</skos:altLabel>
      <skos:altLabel xml:lang="sv">OSL-3.0</skos:altLabel>
      <skos:changeNote xml:lang="en">The source of the start-use date: http://rosenlaw.com/OSL3.0-explained.htm; https://lwn.net/Articles/147660/</skos:changeNote>
      <skos:definition xml:lang="en">Open Software License 3.0 is a copyleft-style, free software licence approved by the Open Source Initiative. Similar to the AGPL, the OSL requires the user to disclose the source code when communicating software.</skos:definition>
      <skos:exactMatch rdf:resource="https://opensource.org/licenses/OSL-3.0"/>
      <skos:inScheme rdf:resource="http://publications.europa.eu/resource/authority/licence"/>
      <skos:topConceptOf rdf:resource="http://publications.europa.eu/resource/authority/licence"/>
   </skos:Concept>
   <skos:Concept rdf:about="http://publications.europa.eu/resource/authority/licence/PHP_3_0"
                 at:deprecated="false">
      <skos:prefLabel xml:lang="en">The PHP License 3.0 (PHP-3.0)</skos:prefLabel>
      <at:authority-code>PHP_3_0</at:authority-code>
      <at:op-code>PHP_3_0</at:op-code>
      <at:start.use>2002-07-21</at:start.use>
      <atold:op-code>PHP_3_0</atold:op-code>
      <dc:identifier>PHP_3_0</dc:identifier>
      <skos:altLabel xml:lang="bg">PHP-3.0</skos:altLabel>
      <skos:altLabel xml:lang="cs">PHP-3.0</skos:altLabel>
      <skos:altLabel xml:lang="da">PHP-3.0</skos:altLabel>
      <skos:altLabel xml:lang="de">PHP-3.0</skos:altLabel>
      <skos:altLabel xml:lang="el">PHP-3.0</skos:altLabel>
      <skos:altLabel xml:lang="en">PHP-3.0</skos:altLabel>
      <skos:altLabel xml:lang="es">PHP-3.0</skos:altLabel>
      <skos:altLabel xml:lang="et">PHP-3.0</skos:altLabel>
      <skos:altLabel xml:lang="fi">PHP-3.0</skos:altLabel>
      <skos:altLabel xml:lang="fr">PHP-3.0</skos:altLabel>
      <skos:altLabel xml:lang="ga">PHP-3.0</skos:altLabel>
      <skos:altLabel xml:lang="hr">PHP-3.0</skos:altLabel>
      <skos:altLabel xml:lang="hu">PHP-3.0</skos:altLabel>
      <skos:altLabel xml:lang="it">PHP-3.0</skos:altLabel>
      <skos:altLabel xml:lang="lt">PHP-3.0</skos:altLabel>
      <skos:altLabel xml:lang="lv">PHP-3.0</skos:altLabel>
      <skos:altLabel xml:lang="mt">PHP-3.0</skos:altLabel>
      <skos:altLabel xml:lang="nl">PHP-3.0</skos:altLabel>
      <skos:altLabel xml:lang="pl">PHP-3.0</skos:altLabel>
      <skos:altLabel xml:lang="pt">PHP-3.0</skos:altLabel>
      <skos:altLabel xml:lang="ro">PHP-3.0</skos:altLabel>
      <skos:altLabel xml:lang="sk">PHP-3.0</skos:altLabel>
      <skos:altLabel xml:lang="sl">PHP-3.0</skos:altLabel>
      <skos:altLabel xml:lang="sv">PHP-3.0</skos:altLabel>
      <skos:changeNote xml:lang="en">The source of the start-use date: http://lists.opensource.org/pipermail/license-review_lists.opensource.org/2020-March/004716.html</skos:changeNote>
      <skos:definition xml:lang="en">The PHP License 3.0 is a permissive free software licence approved by the Open Source Initiative. It has minimal, clear requirements, and explicitly bars the use of the PHP name to endorse the software.</skos:definition>
      <skos:exactMatch rdf:resource="https://opensource.org/licenses/PHP-3.0"/>
      <skos:inScheme rdf:resource="http://publications.europa.eu/resource/authority/licence"/>
      <skos:topConceptOf rdf:resource="http://publications.europa.eu/resource/authority/licence"/>
   </skos:Concept>
   <skos:Concept rdf:about="http://publications.europa.eu/resource/authority/licence/POSTGRE_SQL"
                 at:deprecated="false">
      <skos:prefLabel xml:lang="en">The PostgreSQL Licence (PostgreSQL)</skos:prefLabel>
      <at:authority-code>POSTGRE_SQL</at:authority-code>
      <at:op-code>POSTGRE_SQL</at:op-code>
      <at:start.use>1996-07-08</at:start.use>
      <atold:op-code>POSTGRE_SQL</atold:op-code>
      <dc:identifier>POSTGRE_SQL</dc:identifier>
      <skos:altLabel xml:lang="bg">PostgreSQL</skos:altLabel>
      <skos:altLabel xml:lang="cs">PostgreSQL</skos:altLabel>
      <skos:altLabel xml:lang="da">PostgreSQL</skos:altLabel>
      <skos:altLabel xml:lang="de">PostgreSQL</skos:altLabel>
      <skos:altLabel xml:lang="el">PostgreSQL</skos:altLabel>
      <skos:altLabel xml:lang="en">PostgreSQL</skos:altLabel>
      <skos:altLabel xml:lang="es">PostgreSQL</skos:altLabel>
      <skos:altLabel xml:lang="et">PostgreSQL</skos:altLabel>
      <skos:altLabel xml:lang="fi">PostgreSQL</skos:altLabel>
      <skos:altLabel xml:lang="fr">PostgreSQL</skos:altLabel>
      <skos:altLabel xml:lang="ga">PostgreSQL</skos:altLabel>
      <skos:altLabel xml:lang="hr">PostgreSQL</skos:altLabel>
      <skos:altLabel xml:lang="hu">PostgreSQL</skos:altLabel>
      <skos:altLabel xml:lang="it">PostgreSQL</skos:altLabel>
      <skos:altLabel xml:lang="lt">PostgreSQL</skos:altLabel>
      <skos:altLabel xml:lang="lv">PostgreSQL</skos:altLabel>
      <skos:altLabel xml:lang="mt">PostgreSQL</skos:altLabel>
      <skos:altLabel xml:lang="nl">PostgreSQL</skos:altLabel>
      <skos:altLabel xml:lang="pl">PostgreSQL</skos:altLabel>
      <skos:altLabel xml:lang="pt">PostgreSQL</skos:altLabel>
      <skos:altLabel xml:lang="ro">PostgreSQL</skos:altLabel>
      <skos:altLabel xml:lang="sk">PostgreSQL</skos:altLabel>
      <skos:altLabel xml:lang="sl">PostgreSQL</skos:altLabel>
      <skos:altLabel xml:lang="sv">PostgreSQL</skos:altLabel>
      <skos:changeNote xml:lang="en">The source of the start-use date: https://en.wikipedia.org/wiki/PostgreSQL</skos:changeNote>
      <skos:definition xml:lang="en">PostgreSQL is a BSD-style permissive free software licence approved by the Open Source Initiative.</skos:definition>
      <skos:exactMatch rdf:resource="https://opensource.org/licenses/PostgreSQL"/>
      <skos:inScheme rdf:resource="http://publications.europa.eu/resource/authority/licence"/>
      <skos:topConceptOf rdf:resource="http://publications.europa.eu/resource/authority/licence"/>
   </skos:Concept>
   <skos:Concept rdf:about="http://publications.europa.eu/resource/authority/licence/PSEUL"
                 at:deprecated="false">
      <skos:prefLabel xml:lang="en">INSPIRE End User Licence</skos:prefLabel>
      <at:authority-code>PSEUL</at:authority-code>
      <at:op-code>PSEUL</at:op-code>
      <at:start.use>2013-08-01</at:start.use>
      <atold:op-code>PSEUL</atold:op-code>
      <dc:identifier>PSEUL</dc:identifier>
      <skos:altLabel xml:lang="bg">PSEUL</skos:altLabel>
      <skos:altLabel xml:lang="cs">PSEUL</skos:altLabel>
      <skos:altLabel xml:lang="da">PSEUL</skos:altLabel>
      <skos:altLabel xml:lang="de">PSEUL</skos:altLabel>
      <skos:altLabel xml:lang="el">PSEUL</skos:altLabel>
      <skos:altLabel xml:lang="en">PSEUL</skos:altLabel>
      <skos:altLabel xml:lang="es">PSEUL</skos:altLabel>
      <skos:altLabel xml:lang="et">PSEUL</skos:altLabel>
      <skos:altLabel xml:lang="fi">PSEUL</skos:altLabel>
      <skos:altLabel xml:lang="fr">PSEUL</skos:altLabel>
      <skos:altLabel xml:lang="ga">PSEUL</skos:altLabel>
      <skos:altLabel xml:lang="hr">PSEUL</skos:altLabel>
      <skos:altLabel xml:lang="hu">PSEUL</skos:altLabel>
      <skos:altLabel xml:lang="it">PSEUL</skos:altLabel>
      <skos:altLabel xml:lang="lt">PSEUL</skos:altLabel>
      <skos:altLabel xml:lang="lv">PSEUL</skos:altLabel>
      <skos:altLabel xml:lang="mt">PSEUL</skos:altLabel>
      <skos:altLabel xml:lang="nl">PSEUL</skos:altLabel>
      <skos:altLabel xml:lang="pl">PSEUL</skos:altLabel>
      <skos:altLabel xml:lang="pt">PSEUL</skos:altLabel>
      <skos:altLabel xml:lang="ro">PSEUL</skos:altLabel>
      <skos:altLabel xml:lang="sk">PSEUL</skos:altLabel>
      <skos:altLabel xml:lang="sl">PSEUL</skos:altLabel>
      <skos:altLabel xml:lang="sv">PSEUL</skos:altLabel>
      <skos:changeNote xml:lang="en">The source of the start-use date: https://data.blog.gov.uk/2013/08/23/new-psma-end-user-licences-for-inspire/</skos:changeNote>
      <skos:definition xml:lang="en">The INSPIRE End User Licence (PSEUL) aims to enable the sharing of environmental spatial information amongst public sector organisations. Licenced data under PSEUL is limited to data created (derived) by the user using Ordnance Survey (OS) licenced data.</skos:definition>
      <skos:exactMatch rdf:resource="https://www.ordnancesurvey.co.uk/documents/licensing/inspire-end-user-licence.pdf"/>
      <skos:inScheme rdf:resource="http://publications.europa.eu/resource/authority/licence"/>
      <skos:topConceptOf rdf:resource="http://publications.europa.eu/resource/authority/licence"/>
   </skos:Concept>
   <skos:Concept rdf:about="http://publications.europa.eu/resource/authority/licence/PYTHON_2_0"
                 at:deprecated="false">
      <skos:prefLabel xml:lang="en">Python License (Python-2.0)</skos:prefLabel>
      <at:authority-code>PYTHON_2_0</at:authority-code>
      <at:op-code>PYTHON_2_0</at:op-code>
      <at:start.use>2000-09-01</at:start.use>
      <atold:op-code>PYTHON_2_0</atold:op-code>
      <dc:identifier>PYTHON_2_0</dc:identifier>
      <skos:altLabel xml:lang="bg">Python-2.0</skos:altLabel>
      <skos:altLabel xml:lang="cs">Python-2.0</skos:altLabel>
      <skos:altLabel xml:lang="da">Python-2.0</skos:altLabel>
      <skos:altLabel xml:lang="de">Python-2.0</skos:altLabel>
      <skos:altLabel xml:lang="el">Python-2.0</skos:altLabel>
      <skos:altLabel xml:lang="en">Python-2.0</skos:altLabel>
      <skos:altLabel xml:lang="es">Python-2.0</skos:altLabel>
      <skos:altLabel xml:lang="et">Python-2.0</skos:altLabel>
      <skos:altLabel xml:lang="fi">Python-2.0</skos:altLabel>
      <skos:altLabel xml:lang="fr">Python-2.0</skos:altLabel>
      <skos:altLabel xml:lang="ga">Python-2.0</skos:altLabel>
      <skos:altLabel xml:lang="hr">Python-2.0</skos:altLabel>
      <skos:altLabel xml:lang="hu">Python-2.0</skos:altLabel>
      <skos:altLabel xml:lang="it">Python-2.0</skos:altLabel>
      <skos:altLabel xml:lang="lt">Python-2.0</skos:altLabel>
      <skos:altLabel xml:lang="lv">Python-2.0</skos:altLabel>
      <skos:altLabel xml:lang="mt">Python-2.0</skos:altLabel>
      <skos:altLabel xml:lang="nl">Python-2.0</skos:altLabel>
      <skos:altLabel xml:lang="pl">Python-2.0</skos:altLabel>
      <skos:altLabel xml:lang="pt">Python-2.0</skos:altLabel>
      <skos:altLabel xml:lang="ro">Python-2.0</skos:altLabel>
      <skos:altLabel xml:lang="sk">Python-2.0</skos:altLabel>
      <skos:altLabel xml:lang="sl">Python-2.0</skos:altLabel>
      <skos:altLabel xml:lang="sv">Python-2.0</skos:altLabel>
      <skos:changeNote xml:lang="en">The source of the start-use date: https://www.slideshare.net/kanchilug/python-quick-guide1; https://en.wikipedia.org/wiki/Python_License</skos:changeNote>
      <skos:definition xml:lang="en">Python 2.0 is a permissive free software licence approved by the Open Source Initiative.</skos:definition>
      <skos:exactMatch rdf:resource="https://opensource.org/licenses/Python-2.0"/>
      <skos:inScheme rdf:resource="http://publications.europa.eu/resource/authority/licence"/>
      <skos:topConceptOf rdf:resource="http://publications.europa.eu/resource/authority/licence"/>
   </skos:Concept>
   <skos:Concept rdf:about="http://publications.europa.eu/resource/authority/licence/QPL_1_0"
                 at:deprecated="false">
      <skos:prefLabel xml:lang="en">The Q Public License Version (QPL-1.0)</skos:prefLabel>
      <at:authority-code>QPL_1_0</at:authority-code>
      <at:op-code>QPL_1_0</at:op-code>
      <at:start.use>1999-03-04</at:start.use>
      <atold:op-code>QPL_1_0</atold:op-code>
      <dc:identifier>QPL_1_0</dc:identifier>
      <skos:altLabel xml:lang="bg">QPL-1.0</skos:altLabel>
      <skos:altLabel xml:lang="cs">QPL-1.0</skos:altLabel>
      <skos:altLabel xml:lang="da">QPL-1.0</skos:altLabel>
      <skos:altLabel xml:lang="de">QPL-1.0</skos:altLabel>
      <skos:altLabel xml:lang="el">QPL-1.0</skos:altLabel>
      <skos:altLabel xml:lang="en">QPL-1.0</skos:altLabel>
      <skos:altLabel xml:lang="es">QPL-1.0</skos:altLabel>
      <skos:altLabel xml:lang="et">QPL-1.0</skos:altLabel>
      <skos:altLabel xml:lang="fi">QPL-1.0</skos:altLabel>
      <skos:altLabel xml:lang="fr">QPL-1.0</skos:altLabel>
      <skos:altLabel xml:lang="ga">QPL-1.0</skos:altLabel>
      <skos:altLabel xml:lang="hr">QPL-1.0</skos:altLabel>
      <skos:altLabel xml:lang="hu">QPL-1.0</skos:altLabel>
      <skos:altLabel xml:lang="it">QPL-1.0</skos:altLabel>
      <skos:altLabel xml:lang="lt">QPL-1.0</skos:altLabel>
      <skos:altLabel xml:lang="lv">QPL-1.0</skos:altLabel>
      <skos:altLabel xml:lang="mt">QPL-1.0</skos:altLabel>
      <skos:altLabel xml:lang="nl">QPL-1.0</skos:altLabel>
      <skos:altLabel xml:lang="pl">QPL-1.0</skos:altLabel>
      <skos:altLabel xml:lang="pt">QPL-1.0</skos:altLabel>
      <skos:altLabel xml:lang="ro">QPL-1.0</skos:altLabel>
      <skos:altLabel xml:lang="sk">QPL-1.0</skos:altLabel>
      <skos:altLabel xml:lang="sl">QPL-1.0</skos:altLabel>
      <skos:altLabel xml:lang="sv">QPL-1.0</skos:altLabel>
      <skos:changeNote xml:lang="en">The source of the start-use date: http://blog.hermit4.info/2013/01/qt-news-title.html</skos:changeNote>
      <skos:definition xml:lang="en">The Q Public License Version 1.0 is a copyleft-style, free software licence approved by the Open Source Initiative. It was designed by the Norwegian firm Trolltech to govern the distribution of its software, the Qt Toolkit.</skos:definition>
      <skos:exactMatch rdf:resource="https://opensource.org/licenses/QPL-1.0"/>
      <skos:inScheme rdf:resource="http://publications.europa.eu/resource/authority/licence"/>
      <skos:topConceptOf rdf:resource="http://publications.europa.eu/resource/authority/licence"/>
   </skos:Concept>
   <skos:Concept rdf:about="http://publications.europa.eu/resource/authority/licence/RPL_1_1"
                 at:deprecated="true">
      <skos:prefLabel xml:lang="en">Reciprocal Public License, version 1.1</skos:prefLabel>
      <at:authority-code>RPL_1_1</at:authority-code>
      <at:op-code>RPL_1_1</at:op-code>
      <at:start.use>2002-11-01</at:start.use>
      <atold:op-code>RPL_1_1</atold:op-code>
      <dc:identifier>RPL_1_1</dc:identifier>
      <skos:altLabel xml:lang="bg">RPL-1.1</skos:altLabel>
      <skos:altLabel xml:lang="cs">RPL-1.1</skos:altLabel>
      <skos:altLabel xml:lang="da">RPL-1.1</skos:altLabel>
      <skos:altLabel xml:lang="de">RPL-1.1</skos:altLabel>
      <skos:altLabel xml:lang="el">RPL-1.1</skos:altLabel>
      <skos:altLabel xml:lang="en">RPL-1.1</skos:altLabel>
      <skos:altLabel xml:lang="es">RPL-1.1</skos:altLabel>
      <skos:altLabel xml:lang="et">RPL-1.1</skos:altLabel>
      <skos:altLabel xml:lang="fi">RPL-1.1</skos:altLabel>
      <skos:altLabel xml:lang="fr">RPL-1.1</skos:altLabel>
      <skos:altLabel xml:lang="ga">RPL-1.1</skos:altLabel>
      <skos:altLabel xml:lang="hr">RPL-1.1</skos:altLabel>
      <skos:altLabel xml:lang="hu">RPL-1.1</skos:altLabel>
      <skos:altLabel xml:lang="it">RPL-1.1</skos:altLabel>
      <skos:altLabel xml:lang="lt">RPL-1.1</skos:altLabel>
      <skos:altLabel xml:lang="lv">RPL-1.1</skos:altLabel>
      <skos:altLabel xml:lang="mt">RPL-1.1</skos:altLabel>
      <skos:altLabel xml:lang="nl">RPL-1.1</skos:altLabel>
      <skos:altLabel xml:lang="pl">RPL-1.1</skos:altLabel>
      <skos:altLabel xml:lang="pt">RPL-1.1</skos:altLabel>
      <skos:altLabel xml:lang="ro">RPL-1.1</skos:altLabel>
      <skos:altLabel xml:lang="sk">RPL-1.1</skos:altLabel>
      <skos:altLabel xml:lang="sl">RPL-1.1</skos:altLabel>
      <skos:altLabel xml:lang="sv">RPL-1.1</skos:altLabel>
      <skos:changeNote xml:lang="en">The source of the start-use date: https://cc.com.au/files/acquisition_of_open-source_software_-_text.pdf</skos:changeNote>
      <skos:definition xml:lang="en">The Reciprocal Public License, version 1.1 is a copyleft-style, free software licence approved by the Open Source Initiative. It contains rules on redistribution.</skos:definition>
      <skos:exactMatch rdf:resource="https://opensource.org/licenses/RPL-1.1"/>
      <skos:inScheme rdf:resource="http://publications.europa.eu/resource/authority/licence"/>
      <skos:topConceptOf rdf:resource="http://publications.europa.eu/resource/authority/licence"/>
      <at:end.use>2007-07-14</at:end.use>
   </skos:Concept>
   <skos:Concept rdf:about="http://publications.europa.eu/resource/authority/licence/RPL_1_5"
                 at:deprecated="false">
      <skos:prefLabel xml:lang="en">Reciprocal Public License 1.5 (RPL-1.5)</skos:prefLabel>
      <at:authority-code>RPL_1_5</at:authority-code>
      <at:op-code>RPL_1_5</at:op-code>
      <at:start.use>2007-07-15</at:start.use>
      <atold:op-code>RPL_1_5</atold:op-code>
      <dc:identifier>RPL_1_5</dc:identifier>
      <skos:altLabel xml:lang="bg">RPL-1.5</skos:altLabel>
      <skos:altLabel xml:lang="cs">RPL-1.5</skos:altLabel>
      <skos:altLabel xml:lang="da">RPL-1.5</skos:altLabel>
      <skos:altLabel xml:lang="de">RPL-1.5</skos:altLabel>
      <skos:altLabel xml:lang="el">RPL-1.5</skos:altLabel>
      <skos:altLabel xml:lang="en">RPL-1.5</skos:altLabel>
      <skos:altLabel xml:lang="es">RPL-1.5</skos:altLabel>
      <skos:altLabel xml:lang="et">RPL-1.5</skos:altLabel>
      <skos:altLabel xml:lang="fi">RPL-1.5</skos:altLabel>
      <skos:altLabel xml:lang="fr">RPL-1.5</skos:altLabel>
      <skos:altLabel xml:lang="ga">RPL-1.5</skos:altLabel>
      <skos:altLabel xml:lang="hr">RPL-1.5</skos:altLabel>
      <skos:altLabel xml:lang="hu">RPL-1.5</skos:altLabel>
      <skos:altLabel xml:lang="it">RPL-1.5</skos:altLabel>
      <skos:altLabel xml:lang="lt">RPL-1.5</skos:altLabel>
      <skos:altLabel xml:lang="lv">RPL-1.5</skos:altLabel>
      <skos:altLabel xml:lang="mt">RPL-1.5</skos:altLabel>
      <skos:altLabel xml:lang="nl">RPL-1.5</skos:altLabel>
      <skos:altLabel xml:lang="pl">RPL-1.5</skos:altLabel>
      <skos:altLabel xml:lang="pt">RPL-1.5</skos:altLabel>
      <skos:altLabel xml:lang="ro">RPL-1.5</skos:altLabel>
      <skos:altLabel xml:lang="sk">RPL-1.5</skos:altLabel>
      <skos:altLabel xml:lang="sl">RPL-1.5</skos:altLabel>
      <skos:altLabel xml:lang="sv">RPL-1.5</skos:altLabel>
      <skos:changeNote xml:lang="en">The source of the start-use date: https://spdx.org/licenses/RPL-1.5.html</skos:changeNote>
      <skos:definition xml:lang="en">The Reciprocal Public License 1.5 is a copyleft-style, free software licence approved by the Open Source Initiative with detailed liability protection and numerous requirements, created to close a loophole in the GPL which let users sell modified software without ”fairly” distributing it.</skos:definition>
      <skos:exactMatch rdf:resource="https://opensource.org/licenses/RPL-1.5"/>
      <skos:inScheme rdf:resource="http://publications.europa.eu/resource/authority/licence"/>
      <skos:topConceptOf rdf:resource="http://publications.europa.eu/resource/authority/licence"/>
   </skos:Concept>
   <skos:Concept rdf:about="http://publications.europa.eu/resource/authority/licence/RPSL_1_0"
                 at:deprecated="false">
      <skos:prefLabel xml:lang="en">RealNetworks Public Source License Version 1.0 (RPSL-1.0)</skos:prefLabel>
      <at:authority-code>RPSL_1_0</at:authority-code>
      <at:op-code>RPSL_1_0</at:op-code>
      <at:start.use>2002-10-28</at:start.use>
      <atold:op-code>RPSL_1_0</atold:op-code>
      <dc:identifier>RPSL_1_0</dc:identifier>
      <skos:altLabel xml:lang="bg">RPSL-1.0</skos:altLabel>
      <skos:altLabel xml:lang="cs">RPSL-1.0</skos:altLabel>
      <skos:altLabel xml:lang="da">RPSL-1.0</skos:altLabel>
      <skos:altLabel xml:lang="de">RPSL-1.0</skos:altLabel>
      <skos:altLabel xml:lang="el">RPSL-1.0</skos:altLabel>
      <skos:altLabel xml:lang="en">RPSL-1.0</skos:altLabel>
      <skos:altLabel xml:lang="es">RPSL-1.0</skos:altLabel>
      <skos:altLabel xml:lang="et">RPSL-1.0</skos:altLabel>
      <skos:altLabel xml:lang="fi">RPSL-1.0</skos:altLabel>
      <skos:altLabel xml:lang="fr">RPSL-1.0</skos:altLabel>
      <skos:altLabel xml:lang="ga">RPSL-1.0</skos:altLabel>
      <skos:altLabel xml:lang="hr">RPSL-1.0</skos:altLabel>
      <skos:altLabel xml:lang="hu">RPSL-1.0</skos:altLabel>
      <skos:altLabel xml:lang="it">RPSL-1.0</skos:altLabel>
      <skos:altLabel xml:lang="lt">RPSL-1.0</skos:altLabel>
      <skos:altLabel xml:lang="lv">RPSL-1.0</skos:altLabel>
      <skos:altLabel xml:lang="mt">RPSL-1.0</skos:altLabel>
      <skos:altLabel xml:lang="nl">RPSL-1.0</skos:altLabel>
      <skos:altLabel xml:lang="pl">RPSL-1.0</skos:altLabel>
      <skos:altLabel xml:lang="pt">RPSL-1.0</skos:altLabel>
      <skos:altLabel xml:lang="ro">RPSL-1.0</skos:altLabel>
      <skos:altLabel xml:lang="sk">RPSL-1.0</skos:altLabel>
      <skos:altLabel xml:lang="sl">RPSL-1.0</skos:altLabel>
      <skos:altLabel xml:lang="sv">RPSL-1.0</skos:altLabel>
      <skos:changeNote xml:lang="en">The source of the start-use date: https://spdx.org/licenses/RPSL-1.0.html</skos:changeNote>
      <skos:definition xml:lang="en">Published by RealNetworks, RPSL-1.0 is a copyleft-style, free software licence approved by the Open Source Initiative.</skos:definition>
      <skos:exactMatch rdf:resource="https://opensource.org/licenses/RPSL-1.0"/>
      <skos:inScheme rdf:resource="http://publications.europa.eu/resource/authority/licence"/>
      <skos:topConceptOf rdf:resource="http://publications.europa.eu/resource/authority/licence"/>
   </skos:Concept>
   <skos:Concept rdf:about="http://publications.europa.eu/resource/authority/licence/RSCPL"
                 at:deprecated="false">
      <skos:prefLabel xml:lang="en">The Ricoh Source Code Public License (RSCPL)</skos:prefLabel>
      <at:authority-code>RSCPL</at:authority-code>
      <at:op-code>RSCPL</at:op-code>
      <at:start.use>1995-12-01</at:start.use>
      <atold:op-code>RSCPL</atold:op-code>
      <dc:identifier>RSCPL</dc:identifier>
      <skos:altLabel xml:lang="bg">RSCPL</skos:altLabel>
      <skos:altLabel xml:lang="cs">RSCPL</skos:altLabel>
      <skos:altLabel xml:lang="da">RSCPL</skos:altLabel>
      <skos:altLabel xml:lang="de">RSCPL</skos:altLabel>
      <skos:altLabel xml:lang="el">RSCPL</skos:altLabel>
      <skos:altLabel xml:lang="en">RSCPL</skos:altLabel>
      <skos:altLabel xml:lang="es">RSCPL</skos:altLabel>
      <skos:altLabel xml:lang="et">RSCPL</skos:altLabel>
      <skos:altLabel xml:lang="fi">RSCPL</skos:altLabel>
      <skos:altLabel xml:lang="fr">RSCPL</skos:altLabel>
      <skos:altLabel xml:lang="ga">RSCPL</skos:altLabel>
      <skos:altLabel xml:lang="hr">RSCPL</skos:altLabel>
      <skos:altLabel xml:lang="hu">RSCPL</skos:altLabel>
      <skos:altLabel xml:lang="it">RSCPL</skos:altLabel>
      <skos:altLabel xml:lang="lt">RSCPL</skos:altLabel>
      <skos:altLabel xml:lang="lv">RSCPL</skos:altLabel>
      <skos:altLabel xml:lang="mt">RSCPL</skos:altLabel>
      <skos:altLabel xml:lang="nl">RSCPL</skos:altLabel>
      <skos:altLabel xml:lang="pl">RSCPL</skos:altLabel>
      <skos:altLabel xml:lang="pt">RSCPL</skos:altLabel>
      <skos:altLabel xml:lang="ro">RSCPL</skos:altLabel>
      <skos:altLabel xml:lang="sk">RSCPL</skos:altLabel>
      <skos:altLabel xml:lang="sl">RSCPL</skos:altLabel>
      <skos:altLabel xml:lang="sv">RSCPL</skos:altLabel>
      <skos:changeNote xml:lang="en">The source of the start-use date: http://ploug22.free.fr/doc/oss-market-structure-urope.pdf; https://spdx.org/licenses/RSCPL.html</skos:changeNote>
      <skos:definition xml:lang="en">The Ricoh Source Code Public License (RSCPL) is a copyleft-style, free software licence approved by the Open Source Initiative with much built-in protection for the author.</skos:definition>
      <skos:exactMatch rdf:resource="https://opensource.org/licenses/RSCPL"/>
      <skos:inScheme rdf:resource="http://publications.europa.eu/resource/authority/licence"/>
      <skos:topConceptOf rdf:resource="http://publications.europa.eu/resource/authority/licence"/>
   </skos:Concept>
   <skos:Concept rdf:about="http://publications.europa.eu/resource/authority/licence/SIMPL_2_0"
                 at:deprecated="false">
      <skos:prefLabel xml:lang="en">Simple Public License (SimPL-2.0)</skos:prefLabel>
      <at:authority-code>SIMPL_2_0</at:authority-code>
      <at:op-code>SIMPL_2_0</at:op-code>
      <at:start.use>2007-11-01</at:start.use>
      <atold:op-code>SIMPL_2_0</atold:op-code>
      <dc:identifier>SIMPL_2_0</dc:identifier>
      <skos:altLabel xml:lang="bg">SimPL-2.0</skos:altLabel>
      <skos:altLabel xml:lang="cs">SimPL-2.0</skos:altLabel>
      <skos:altLabel xml:lang="da">SimPL-2.0</skos:altLabel>
      <skos:altLabel xml:lang="de">SimPL-2.0</skos:altLabel>
      <skos:altLabel xml:lang="el">SimPL-2.0</skos:altLabel>
      <skos:altLabel xml:lang="en">SimPL-2.0</skos:altLabel>
      <skos:altLabel xml:lang="es">SimPL-2.0</skos:altLabel>
      <skos:altLabel xml:lang="et">SimPL-2.0</skos:altLabel>
      <skos:altLabel xml:lang="fi">SimPL-2.0</skos:altLabel>
      <skos:altLabel xml:lang="fr">SimPL-2.0</skos:altLabel>
      <skos:altLabel xml:lang="ga">SimPL-2.0</skos:altLabel>
      <skos:altLabel xml:lang="hr">SimPL-2.0</skos:altLabel>
      <skos:altLabel xml:lang="hu">SimPL-2.0</skos:altLabel>
      <skos:altLabel xml:lang="it">SimPL-2.0</skos:altLabel>
      <skos:altLabel xml:lang="lt">SimPL-2.0</skos:altLabel>
      <skos:altLabel xml:lang="lv">SimPL-2.0</skos:altLabel>
      <skos:altLabel xml:lang="mt">SimPL-2.0</skos:altLabel>
      <skos:altLabel xml:lang="nl">SimPL-2.0</skos:altLabel>
      <skos:altLabel xml:lang="pl">SimPL-2.0</skos:altLabel>
      <skos:altLabel xml:lang="pt">SimPL-2.0</skos:altLabel>
      <skos:altLabel xml:lang="ro">SimPL-2.0</skos:altLabel>
      <skos:altLabel xml:lang="sk">SimPL-2.0</skos:altLabel>
      <skos:altLabel xml:lang="sl">SimPL-2.0</skos:altLabel>
      <skos:altLabel xml:lang="sv">SimPL-2.0</skos:altLabel>
      <skos:changeNote xml:lang="en">The source of the start-use date: https://opensource.org/node/228</skos:changeNote>
      <skos:definition xml:lang="en">Simple Public License 2.0 is a copyleft-style, free software licence approved by the Open Source Initiative.</skos:definition>
      <skos:exactMatch rdf:resource="https://opensource.org/licenses/SimPL-2.0"/>
      <skos:inScheme rdf:resource="http://publications.europa.eu/resource/authority/licence"/>
      <skos:topConceptOf rdf:resource="http://publications.europa.eu/resource/authority/licence"/>
   </skos:Concept>
   <skos:Concept rdf:about="http://publications.europa.eu/resource/authority/licence/SLEEPYCAT"
                 at:deprecated="false">
      <skos:prefLabel xml:lang="en">The Sleepycat License (Sleepycat)</skos:prefLabel>
      <at:authority-code>SLEEPYCAT</at:authority-code>
      <at:op-code>SLEEPYCAT</at:op-code>
      <at:start.use>1990-01-01</at:start.use>
      <atold:op-code>SLEEPYCAT</atold:op-code>
      <dc:identifier>SLEEPYCAT</dc:identifier>
      <skos:altLabel xml:lang="bg">Sleepycat</skos:altLabel>
      <skos:altLabel xml:lang="cs">Sleepycat</skos:altLabel>
      <skos:altLabel xml:lang="da">Sleepycat</skos:altLabel>
      <skos:altLabel xml:lang="de">Sleepycat</skos:altLabel>
      <skos:altLabel xml:lang="el">Sleepycat</skos:altLabel>
      <skos:altLabel xml:lang="en">Sleepycat</skos:altLabel>
      <skos:altLabel xml:lang="es">Sleepycat</skos:altLabel>
      <skos:altLabel xml:lang="et">Sleepycat</skos:altLabel>
      <skos:altLabel xml:lang="fi">Sleepycat</skos:altLabel>
      <skos:altLabel xml:lang="fr">Sleepycat</skos:altLabel>
      <skos:altLabel xml:lang="ga">Sleepycat</skos:altLabel>
      <skos:altLabel xml:lang="hr">Sleepycat</skos:altLabel>
      <skos:altLabel xml:lang="hu">Sleepycat</skos:altLabel>
      <skos:altLabel xml:lang="it">Sleepycat</skos:altLabel>
      <skos:altLabel xml:lang="lt">Sleepycat</skos:altLabel>
      <skos:altLabel xml:lang="lv">Sleepycat</skos:altLabel>
      <skos:altLabel xml:lang="mt">Sleepycat</skos:altLabel>
      <skos:altLabel xml:lang="nl">Sleepycat</skos:altLabel>
      <skos:altLabel xml:lang="pl">Sleepycat</skos:altLabel>
      <skos:altLabel xml:lang="pt">Sleepycat</skos:altLabel>
      <skos:altLabel xml:lang="ro">Sleepycat</skos:altLabel>
      <skos:altLabel xml:lang="sk">Sleepycat</skos:altLabel>
      <skos:altLabel xml:lang="sl">Sleepycat</skos:altLabel>
      <skos:altLabel xml:lang="sv">Sleepycat</skos:altLabel>
      <skos:changeNote xml:lang="en">The source of the start-use date: https://en.wikipedia.org/wiki/Talk%3ASleepycat_License</skos:changeNote>
      <skos:definition xml:lang="en">The Sleepycat License is a BSD plus-style, permissive free software licence approved by the Open Source Initiative.</skos:definition>
      <skos:exactMatch rdf:resource="https://opensource.org/licenses/Sleepycat"/>
      <skos:inScheme rdf:resource="http://publications.europa.eu/resource/authority/licence"/>
      <skos:topConceptOf rdf:resource="http://publications.europa.eu/resource/authority/licence"/>
   </skos:Concept>
   <skos:Concept rdf:about="http://publications.europa.eu/resource/authority/licence/SPL_1_0"
                 at:deprecated="false">
      <skos:prefLabel xml:lang="en">Sun Public License Version 1.0 (SPL-1.0)</skos:prefLabel>
      <at:authority-code>SPL_1_0</at:authority-code>
      <at:op-code>SPL_1_0</at:op-code>
      <at:start.use>1995-01-01</at:start.use>
      <atold:op-code>SPL_1_0</atold:op-code>
      <dc:identifier>SPL_1_0</dc:identifier>
      <skos:altLabel xml:lang="bg">SPL-1.0</skos:altLabel>
      <skos:altLabel xml:lang="cs">SPL-1.0</skos:altLabel>
      <skos:altLabel xml:lang="da">SPL-1.0</skos:altLabel>
      <skos:altLabel xml:lang="de">SPL-1.0</skos:altLabel>
      <skos:altLabel xml:lang="el">SPL-1.0</skos:altLabel>
      <skos:altLabel xml:lang="en">SPL-1.0</skos:altLabel>
      <skos:altLabel xml:lang="es">SPL-1.0</skos:altLabel>
      <skos:altLabel xml:lang="et">SPL-1.0</skos:altLabel>
      <skos:altLabel xml:lang="fi">SPL-1.0</skos:altLabel>
      <skos:altLabel xml:lang="fr">SPL-1.0</skos:altLabel>
      <skos:altLabel xml:lang="ga">SPL-1.0</skos:altLabel>
      <skos:altLabel xml:lang="hr">SPL-1.0</skos:altLabel>
      <skos:altLabel xml:lang="hu">SPL-1.0</skos:altLabel>
      <skos:altLabel xml:lang="it">SPL-1.0</skos:altLabel>
      <skos:altLabel xml:lang="lt">SPL-1.0</skos:altLabel>
      <skos:altLabel xml:lang="lv">SPL-1.0</skos:altLabel>
      <skos:altLabel xml:lang="mt">SPL-1.0</skos:altLabel>
      <skos:altLabel xml:lang="nl">SPL-1.0</skos:altLabel>
      <skos:altLabel xml:lang="pl">SPL-1.0</skos:altLabel>
      <skos:altLabel xml:lang="pt">SPL-1.0</skos:altLabel>
      <skos:altLabel xml:lang="ro">SPL-1.0</skos:altLabel>
      <skos:altLabel xml:lang="sk">SPL-1.0</skos:altLabel>
      <skos:altLabel xml:lang="sl">SPL-1.0</skos:altLabel>
      <skos:altLabel xml:lang="sv">SPL-1.0</skos:altLabel>
      <skos:changeNote xml:lang="en">The source of the start-use date: https://enterprise.dejacode.com/licenses/public/spl-1.0/?_list_filters=q%3DSun%2BPublic%2BLicense</skos:changeNote>
      <skos:definition xml:lang="en">Sun Public License 1.0 is a copyleft-style, free software licence approved by the Open Source Initiative.</skos:definition>
      <skos:exactMatch rdf:resource="https://opensource.org/licenses/SPL-1.0"/>
      <skos:inScheme rdf:resource="http://publications.europa.eu/resource/authority/licence"/>
      <skos:topConceptOf rdf:resource="http://publications.europa.eu/resource/authority/licence"/>
   </skos:Concept>
   <skos:Concept rdf:about="http://publications.europa.eu/resource/authority/licence/UCL_1_0"
                 at:deprecated="false">
      <skos:prefLabel xml:lang="en">Upstream Compatibility License v1.0</skos:prefLabel>
      <at:authority-code>UCL_1_0</at:authority-code>
      <at:op-code>UCL_1_0</at:op-code>
      <at:start.use>2017-02-01</at:start.use>
      <atold:op-code>UCL_1_0</atold:op-code>
      <dc:identifier>UCL_1_0</dc:identifier>
      <skos:altLabel xml:lang="bg">UCL-1.0</skos:altLabel>
      <skos:altLabel xml:lang="cs">UCL-1.0</skos:altLabel>
      <skos:altLabel xml:lang="da">UCL-1.0</skos:altLabel>
      <skos:altLabel xml:lang="de">UCL-1.0</skos:altLabel>
      <skos:altLabel xml:lang="el">UCL-1.0</skos:altLabel>
      <skos:altLabel xml:lang="en">UCL-1.0</skos:altLabel>
      <skos:altLabel xml:lang="es">UCL-1.0</skos:altLabel>
      <skos:altLabel xml:lang="et">UCL-1.0</skos:altLabel>
      <skos:altLabel xml:lang="fi">UCL-1.0</skos:altLabel>
      <skos:altLabel xml:lang="fr">UCL-1.0</skos:altLabel>
      <skos:altLabel xml:lang="ga">UCL-1.0</skos:altLabel>
      <skos:altLabel xml:lang="hr">UCL-1.0</skos:altLabel>
      <skos:altLabel xml:lang="hu">UCL-1.0</skos:altLabel>
      <skos:altLabel xml:lang="it">UCL-1.0</skos:altLabel>
      <skos:altLabel xml:lang="lt">UCL-1.0</skos:altLabel>
      <skos:altLabel xml:lang="lv">UCL-1.0</skos:altLabel>
      <skos:altLabel xml:lang="mt">UCL-1.0</skos:altLabel>
      <skos:altLabel xml:lang="nl">UCL-1.0</skos:altLabel>
      <skos:altLabel xml:lang="pl">UCL-1.0</skos:altLabel>
      <skos:altLabel xml:lang="pt">UCL-1.0</skos:altLabel>
      <skos:altLabel xml:lang="ro">UCL-1.0</skos:altLabel>
      <skos:altLabel xml:lang="sk">UCL-1.0</skos:altLabel>
      <skos:altLabel xml:lang="sl">UCL-1.0</skos:altLabel>
      <skos:altLabel xml:lang="sv">UCL-1.0</skos:altLabel>
      <skos:changeNote xml:lang="en">The source of the start-use date: http://lists.opensource.org/pipermail/license-review_lists.opensource.org/2017-February/002983.html</skos:changeNote>
      <skos:definition xml:lang="en">Upstream Compatibility License v1.0 is a copyleft-style, free software licence approved by the Open Source Initiative.</skos:definition>
      <skos:exactMatch rdf:resource="https://opensource.org/licenses/UCL-1.0"/>
      <skos:inScheme rdf:resource="http://publications.europa.eu/resource/authority/licence"/>
      <skos:topConceptOf rdf:resource="http://publications.europa.eu/resource/authority/licence"/>
   </skos:Concept>
   <skos:Concept rdf:about="http://publications.europa.eu/resource/authority/licence/UPL_1_0"
                 at:deprecated="false">
      <skos:prefLabel xml:lang="en">The Universal Permissive License (UPL), Version 1.0</skos:prefLabel>
      <at:authority-code>UPL_1_0</at:authority-code>
      <at:op-code>UPL_1_0</at:op-code>
      <at:start.use>2015-02-01</at:start.use>
      <atold:op-code>UPL_1_0</atold:op-code>
      <dc:identifier>UPL_1_0</dc:identifier>
      <skos:altLabel xml:lang="bg">UPL</skos:altLabel>
      <skos:altLabel xml:lang="cs">UPL</skos:altLabel>
      <skos:altLabel xml:lang="da">UPL</skos:altLabel>
      <skos:altLabel xml:lang="de">UPL</skos:altLabel>
      <skos:altLabel xml:lang="el">UPL</skos:altLabel>
      <skos:altLabel xml:lang="en">UPL</skos:altLabel>
      <skos:altLabel xml:lang="es">UPL</skos:altLabel>
      <skos:altLabel xml:lang="et">UPL</skos:altLabel>
      <skos:altLabel xml:lang="fi">UPL</skos:altLabel>
      <skos:altLabel xml:lang="fr">UPL</skos:altLabel>
      <skos:altLabel xml:lang="ga">UPL</skos:altLabel>
      <skos:altLabel xml:lang="hr">UPL</skos:altLabel>
      <skos:altLabel xml:lang="hu">UPL</skos:altLabel>
      <skos:altLabel xml:lang="it">UPL</skos:altLabel>
      <skos:altLabel xml:lang="lt">UPL</skos:altLabel>
      <skos:altLabel xml:lang="lv">UPL</skos:altLabel>
      <skos:altLabel xml:lang="mt">UPL</skos:altLabel>
      <skos:altLabel xml:lang="nl">UPL</skos:altLabel>
      <skos:altLabel xml:lang="pl">UPL</skos:altLabel>
      <skos:altLabel xml:lang="pt">UPL</skos:altLabel>
      <skos:altLabel xml:lang="ro">UPL</skos:altLabel>
      <skos:altLabel xml:lang="sk">UPL</skos:altLabel>
      <skos:altLabel xml:lang="sl">UPL</skos:altLabel>
      <skos:altLabel xml:lang="sv">UPL</skos:altLabel>
      <skos:changeNote xml:lang="en">The source of the start-use date: https://oss.oracle.com/licenses/upl/</skos:changeNote>
      <skos:definition xml:lang="en">The Universal Permissive License 1.0 is an attribution+patent-style, permissive free software licence issued by Oracle and approved by the Open Source Initiative.</skos:definition>
      <skos:exactMatch rdf:resource="https://opensource.org/licenses/UPL"/>
      <skos:inScheme rdf:resource="http://publications.europa.eu/resource/authority/licence"/>
      <skos:topConceptOf rdf:resource="http://publications.europa.eu/resource/authority/licence"/>
   </skos:Concept>
   <skos:Concept rdf:about="http://publications.europa.eu/resource/authority/licence/VSL_1_0"
                 at:deprecated="false">
      <skos:prefLabel xml:lang="en">The Vovida Software License v. 1.0 (VSL-1.0)</skos:prefLabel>
      <at:authority-code>VSL_1_0</at:authority-code>
      <at:op-code>VSL_1_0</at:op-code>
      <at:start.use>2000-01-01</at:start.use>
      <atold:op-code>VSL_1_0</atold:op-code>
      <dc:identifier>VSL_1_0</dc:identifier>
      <skos:altLabel xml:lang="bg">VSL-1.0</skos:altLabel>
      <skos:altLabel xml:lang="cs">VSL-1.0</skos:altLabel>
      <skos:altLabel xml:lang="da">VSL-1.0</skos:altLabel>
      <skos:altLabel xml:lang="de">VSL-1.0</skos:altLabel>
      <skos:altLabel xml:lang="el">VSL-1.0</skos:altLabel>
      <skos:altLabel xml:lang="en">VSL-1.0</skos:altLabel>
      <skos:altLabel xml:lang="es">VSL-1.0</skos:altLabel>
      <skos:altLabel xml:lang="et">VSL-1.0</skos:altLabel>
      <skos:altLabel xml:lang="fi">VSL-1.0</skos:altLabel>
      <skos:altLabel xml:lang="fr">VSL-1.0</skos:altLabel>
      <skos:altLabel xml:lang="ga">VSL-1.0</skos:altLabel>
      <skos:altLabel xml:lang="hr">VSL-1.0</skos:altLabel>
      <skos:altLabel xml:lang="hu">VSL-1.0</skos:altLabel>
      <skos:altLabel xml:lang="it">VSL-1.0</skos:altLabel>
      <skos:altLabel xml:lang="lt">VSL-1.0</skos:altLabel>
      <skos:altLabel xml:lang="lv">VSL-1.0</skos:altLabel>
      <skos:altLabel xml:lang="mt">VSL-1.0</skos:altLabel>
      <skos:altLabel xml:lang="nl">VSL-1.0</skos:altLabel>
      <skos:altLabel xml:lang="pl">VSL-1.0</skos:altLabel>
      <skos:altLabel xml:lang="pt">VSL-1.0</skos:altLabel>
      <skos:altLabel xml:lang="ro">VSL-1.0</skos:altLabel>
      <skos:altLabel xml:lang="sk">VSL-1.0</skos:altLabel>
      <skos:altLabel xml:lang="sl">VSL-1.0</skos:altLabel>
      <skos:altLabel xml:lang="sv">VSL-1.0</skos:altLabel>
      <skos:changeNote xml:lang="en">The source of the start-use date: https://spdx.org/licenses/VSL-1.0.html#licenseText</skos:changeNote>
      <skos:definition xml:lang="en">The Vovida Software License v. 1.0 is a BSD plus-style, permissive free software licence approved by the Open Source Initiative.</skos:definition>
      <skos:exactMatch rdf:resource="https://opensource.org/licenses/VSL-1.0"/>
      <skos:inScheme rdf:resource="http://publications.europa.eu/resource/authority/licence"/>
      <skos:topConceptOf rdf:resource="http://publications.europa.eu/resource/authority/licence"/>
   </skos:Concept>
   <skos:Concept rdf:about="http://publications.europa.eu/resource/authority/licence/W3C"
                 at:deprecated="false">
      <skos:prefLabel xml:lang="en">The W3C Software Notice and License (W3C)</skos:prefLabel>
      <at:authority-code>W3C</at:authority-code>
      <at:op-code>W3C</at:op-code>
      <at:start.use>2002-12-31</at:start.use>
      <atold:op-code>W3C</atold:op-code>
      <dc:identifier>W3C</dc:identifier>
      <skos:altLabel xml:lang="bg">W3C</skos:altLabel>
      <skos:altLabel xml:lang="cs">W3C</skos:altLabel>
      <skos:altLabel xml:lang="da">W3C</skos:altLabel>
      <skos:altLabel xml:lang="de">W3C</skos:altLabel>
      <skos:altLabel xml:lang="el">W3C</skos:altLabel>
      <skos:altLabel xml:lang="en">W3C</skos:altLabel>
      <skos:altLabel xml:lang="es">W3C</skos:altLabel>
      <skos:altLabel xml:lang="et">W3C</skos:altLabel>
      <skos:altLabel xml:lang="fi">W3C</skos:altLabel>
      <skos:altLabel xml:lang="fr">W3C</skos:altLabel>
      <skos:altLabel xml:lang="ga">W3C</skos:altLabel>
      <skos:altLabel xml:lang="hr">W3C</skos:altLabel>
      <skos:altLabel xml:lang="hu">W3C</skos:altLabel>
      <skos:altLabel xml:lang="it">W3C</skos:altLabel>
      <skos:altLabel xml:lang="lt">W3C</skos:altLabel>
      <skos:altLabel xml:lang="lv">W3C</skos:altLabel>
      <skos:altLabel xml:lang="mt">W3C</skos:altLabel>
      <skos:altLabel xml:lang="nl">W3C</skos:altLabel>
      <skos:altLabel xml:lang="pl">W3C</skos:altLabel>
      <skos:altLabel xml:lang="pt">W3C</skos:altLabel>
      <skos:altLabel xml:lang="ro">W3C</skos:altLabel>
      <skos:altLabel xml:lang="sk">W3C</skos:altLabel>
      <skos:altLabel xml:lang="sl">W3C</skos:altLabel>
      <skos:altLabel xml:lang="sv">W3C</skos:altLabel>
      <skos:changeNote xml:lang="en">The source of the start-use date: https://en.wikipedia.org/wiki/W3C_Software_Notice_and_License</skos:changeNote>
      <skos:definition xml:lang="en">The W3C Software Notice and License is a permissive free software licence used by software released by the World Wide Web Consortium. It is a permissive licence, compatible with the GNU General Public License and approved by the Open Source Initiative.</skos:definition>
      <skos:exactMatch rdf:resource="https://opensource.org/licenses/W3C"/>
      <skos:inScheme rdf:resource="http://publications.europa.eu/resource/authority/licence"/>
      <skos:topConceptOf rdf:resource="http://publications.europa.eu/resource/authority/licence"/>
   </skos:Concept>
   <skos:Concept rdf:about="http://publications.europa.eu/resource/authority/licence/WATCOM_1_0"
                 at:deprecated="false">
      <skos:prefLabel xml:lang="en">The Sybase Open Source Licence (Watcom-1.0)</skos:prefLabel>
      <at:authority-code>WATCOM_1_0</at:authority-code>
      <at:op-code>WATCOM_1_0</at:op-code>
      <at:start.use>2002-05-19</at:start.use>
      <atold:op-code>WATCOM_1_0</atold:op-code>
      <dc:identifier>WATCOM_1_0</dc:identifier>
      <skos:altLabel xml:lang="bg">Watcom-1.0</skos:altLabel>
      <skos:altLabel xml:lang="cs">Watcom-1.0</skos:altLabel>
      <skos:altLabel xml:lang="da">Watcom-1.0</skos:altLabel>
      <skos:altLabel xml:lang="de">Watcom-1.0</skos:altLabel>
      <skos:altLabel xml:lang="el">Watcom-1.0</skos:altLabel>
      <skos:altLabel xml:lang="en">Watcom-1.0</skos:altLabel>
      <skos:altLabel xml:lang="es">Watcom-1.0</skos:altLabel>
      <skos:altLabel xml:lang="et">Watcom-1.0</skos:altLabel>
      <skos:altLabel xml:lang="fi">Watcom-1.0</skos:altLabel>
      <skos:altLabel xml:lang="fr">Watcom-1.0</skos:altLabel>
      <skos:altLabel xml:lang="ga">Watcom-1.0</skos:altLabel>
      <skos:altLabel xml:lang="hr">Watcom-1.0</skos:altLabel>
      <skos:altLabel xml:lang="hu">Watcom-1.0</skos:altLabel>
      <skos:altLabel xml:lang="it">Watcom-1.0</skos:altLabel>
      <skos:altLabel xml:lang="lt">Watcom-1.0</skos:altLabel>
      <skos:altLabel xml:lang="lv">Watcom-1.0</skos:altLabel>
      <skos:altLabel xml:lang="mt">Watcom-1.0</skos:altLabel>
      <skos:altLabel xml:lang="nl">Watcom-1.0</skos:altLabel>
      <skos:altLabel xml:lang="pl">Watcom-1.0</skos:altLabel>
      <skos:altLabel xml:lang="pt">Watcom-1.0</skos:altLabel>
      <skos:altLabel xml:lang="ro">Watcom-1.0</skos:altLabel>
      <skos:altLabel xml:lang="sk">Watcom-1.0</skos:altLabel>
      <skos:altLabel xml:lang="sl">Watcom-1.0</skos:altLabel>
      <skos:altLabel xml:lang="sv">Watcom-1.0</skos:altLabel>
      <skos:changeNote xml:lang="en">The source of the start-use date: http://howlingmad.gmxhome.de/watcom_new_en.html</skos:changeNote>
      <skos:definition xml:lang="en">Watcom-1.0 is a proprietary+patent-style, strong copyleft software licence approved by the Open Source Initiative.</skos:definition>
      <skos:exactMatch rdf:resource="https://opensource.org/licenses/Watcom-1.0"/>
      <skos:inScheme rdf:resource="http://publications.europa.eu/resource/authority/licence"/>
      <skos:topConceptOf rdf:resource="http://publications.europa.eu/resource/authority/licence"/>
   </skos:Concept>
   <skos:Concept rdf:about="http://publications.europa.eu/resource/authority/licence/WXWINDOWS"
                 at:deprecated="true">
      <skos:prefLabel xml:lang="en">The wxWindows Library Licence (wxWindows)</skos:prefLabel>
      <at:authority-code>WXWINDOWS</at:authority-code>
      <at:op-code>WXWINDOWS</at:op-code>
      <at:start.use>1998-07-01</at:start.use>
      <atold:op-code>WXWINDOWS</atold:op-code>
      <dc:identifier>WXWINDOWS</dc:identifier>
      <skos:altLabel xml:lang="bg">wxWindows</skos:altLabel>
      <skos:altLabel xml:lang="cs">wxWindows</skos:altLabel>
      <skos:altLabel xml:lang="da">wxWindows</skos:altLabel>
      <skos:altLabel xml:lang="de">wxWindows</skos:altLabel>
      <skos:altLabel xml:lang="el">wxWindows</skos:altLabel>
      <skos:altLabel xml:lang="en">wxWindows</skos:altLabel>
      <skos:altLabel xml:lang="es">wxWindows</skos:altLabel>
      <skos:altLabel xml:lang="et">wxWindows</skos:altLabel>
      <skos:altLabel xml:lang="fi">wxWindows</skos:altLabel>
      <skos:altLabel xml:lang="fr">wxWindows</skos:altLabel>
      <skos:altLabel xml:lang="ga">wxWindows</skos:altLabel>
      <skos:altLabel xml:lang="hr">wxWindows</skos:altLabel>
      <skos:altLabel xml:lang="hu">wxWindows</skos:altLabel>
      <skos:altLabel xml:lang="it">wxWindows</skos:altLabel>
      <skos:altLabel xml:lang="lt">wxWindows</skos:altLabel>
      <skos:altLabel xml:lang="lv">wxWindows</skos:altLabel>
      <skos:altLabel xml:lang="mt">wxWindows</skos:altLabel>
      <skos:altLabel xml:lang="nl">wxWindows</skos:altLabel>
      <skos:altLabel xml:lang="pl">wxWindows</skos:altLabel>
      <skos:altLabel xml:lang="pt">wxWindows</skos:altLabel>
      <skos:altLabel xml:lang="ro">wxWindows</skos:altLabel>
      <skos:altLabel xml:lang="sk">wxWindows</skos:altLabel>
      <skos:altLabel xml:lang="sl">wxWindows</skos:altLabel>
      <skos:altLabel xml:lang="sv">wxWindows</skos:altLabel>
      <skos:changeNote xml:lang="en">The source of the start-use date: https://opensource.org/licenses/WXwindows</skos:changeNote>
      <skos:definition xml:lang="en">Approved by the Open Source Initiative, wxWindows is a copyleft-style, free software licence created for wxWidgets.</skos:definition>
      <skos:exactMatch rdf:resource="https://opensource.org/licenses/WXwindows"/>
      <skos:inScheme rdf:resource="http://publications.europa.eu/resource/authority/licence"/>
      <skos:topConceptOf rdf:resource="http://publications.europa.eu/resource/authority/licence"/>
      <at:end.use>2007-06-28</at:end.use>
   </skos:Concept>
   <skos:Concept rdf:about="http://publications.europa.eu/resource/authority/licence/XNET"
                 at:deprecated="true">
      <skos:prefLabel xml:lang="en">The X.Net, Inc. License (Xnet)</skos:prefLabel>
      <at:authority-code>XNET</at:authority-code>
      <at:op-code>XNET</at:op-code>
      <at:start.use>2000-07-01</at:start.use>
      <atold:op-code>XNET</atold:op-code>
      <dc:identifier>XNET</dc:identifier>
      <skos:altLabel xml:lang="bg">Xnet</skos:altLabel>
      <skos:altLabel xml:lang="cs">Xnet</skos:altLabel>
      <skos:altLabel xml:lang="da">Xnet</skos:altLabel>
      <skos:altLabel xml:lang="de">Xnet</skos:altLabel>
      <skos:altLabel xml:lang="el">Xnet</skos:altLabel>
      <skos:altLabel xml:lang="en">Xnet</skos:altLabel>
      <skos:altLabel xml:lang="es">Xnet</skos:altLabel>
      <skos:altLabel xml:lang="et">Xnet</skos:altLabel>
      <skos:altLabel xml:lang="fi">Xnet</skos:altLabel>
      <skos:altLabel xml:lang="fr">Xnet</skos:altLabel>
      <skos:altLabel xml:lang="ga">Xnet</skos:altLabel>
      <skos:altLabel xml:lang="hr">Xnet</skos:altLabel>
      <skos:altLabel xml:lang="hu">Xnet</skos:altLabel>
      <skos:altLabel xml:lang="it">Xnet</skos:altLabel>
      <skos:altLabel xml:lang="lt">Xnet</skos:altLabel>
      <skos:altLabel xml:lang="lv">Xnet</skos:altLabel>
      <skos:altLabel xml:lang="mt">Xnet</skos:altLabel>
      <skos:altLabel xml:lang="nl">Xnet</skos:altLabel>
      <skos:altLabel xml:lang="pl">Xnet</skos:altLabel>
      <skos:altLabel xml:lang="pt">Xnet</skos:altLabel>
      <skos:altLabel xml:lang="ro">Xnet</skos:altLabel>
      <skos:altLabel xml:lang="sk">Xnet</skos:altLabel>
      <skos:altLabel xml:lang="sl">Xnet</skos:altLabel>
      <skos:altLabel xml:lang="sv">Xnet</skos:altLabel>
      <skos:changeNote xml:lang="en">The source of the start-use date: https://opensource.org/licenses/Xnet</skos:changeNote>
      <skos:definition xml:lang="en">Xnet is a MIT-style, permissive free software licence approved by the Open Source Initiative.</skos:definition>
      <skos:exactMatch rdf:resource="https://opensource.org/licenses/Xnet"/>
      <skos:inScheme rdf:resource="http://publications.europa.eu/resource/authority/licence"/>
      <skos:topConceptOf rdf:resource="http://publications.europa.eu/resource/authority/licence"/>
      <at:end.use>2020-01-01</at:end.use>
   </skos:Concept>
   <skos:Concept rdf:about="http://publications.europa.eu/resource/authority/licence/ZLIB"
                 at:deprecated="false">
      <skos:prefLabel xml:lang="en">The zlib/libpng License (Zlib)</skos:prefLabel>
      <at:authority-code>ZLIB</at:authority-code>
      <at:op-code>ZLIB</at:op-code>
      <at:start.use>1995-05-01</at:start.use>
      <atold:op-code>ZLIB</atold:op-code>
      <dc:identifier>ZLIB</dc:identifier>
      <skos:altLabel xml:lang="bg">Zlib</skos:altLabel>
      <skos:altLabel xml:lang="cs">Zlib</skos:altLabel>
      <skos:altLabel xml:lang="da">Zlib</skos:altLabel>
      <skos:altLabel xml:lang="de">Zlib</skos:altLabel>
      <skos:altLabel xml:lang="el">Zlib</skos:altLabel>
      <skos:altLabel xml:lang="en">Zlib</skos:altLabel>
      <skos:altLabel xml:lang="es">Zlib</skos:altLabel>
      <skos:altLabel xml:lang="et">Zlib</skos:altLabel>
      <skos:altLabel xml:lang="fi">Zlib</skos:altLabel>
      <skos:altLabel xml:lang="fr">Zlib</skos:altLabel>
      <skos:altLabel xml:lang="ga">Zlib</skos:altLabel>
      <skos:altLabel xml:lang="hr">Zlib</skos:altLabel>
      <skos:altLabel xml:lang="hu">Zlib</skos:altLabel>
      <skos:altLabel xml:lang="it">Zlib</skos:altLabel>
      <skos:altLabel xml:lang="lt">Zlib</skos:altLabel>
      <skos:altLabel xml:lang="lv">Zlib</skos:altLabel>
      <skos:altLabel xml:lang="mt">Zlib</skos:altLabel>
      <skos:altLabel xml:lang="nl">Zlib</skos:altLabel>
      <skos:altLabel xml:lang="pl">Zlib</skos:altLabel>
      <skos:altLabel xml:lang="pt">Zlib</skos:altLabel>
      <skos:altLabel xml:lang="ro">Zlib</skos:altLabel>
      <skos:altLabel xml:lang="sk">Zlib</skos:altLabel>
      <skos:altLabel xml:lang="sl">Zlib</skos:altLabel>
      <skos:altLabel xml:lang="sv">Zlib</skos:altLabel>
      <skos:changeNote xml:lang="en">The source of the start-use date: https://en.wikipedia.org/wiki/Zlib</skos:changeNote>
      <skos:definition xml:lang="en">Zlib is designed to be a free, general-purpose, legally unencumbered – not covered by any patents – lossless data-compression library for use on virtually any computer hardware and operating system. It is approved by the Open Source Initiative.</skos:definition>
      <skos:exactMatch rdf:resource="https://opensource.org/licenses/Zlib"/>
      <skos:inScheme rdf:resource="http://publications.europa.eu/resource/authority/licence"/>
      <skos:topConceptOf rdf:resource="http://publications.europa.eu/resource/authority/licence"/>
   </skos:Concept>
   <skos:Concept rdf:about="http://publications.europa.eu/resource/authority/licence/ZPL_2_0"
                 at:deprecated="false">
      <skos:prefLabel xml:lang="en">The Zope Public License Version 2.0 (ZPL-2.0)</skos:prefLabel>
      <at:authority-code>ZPL_2_0</at:authority-code>
      <at:op-code>ZPL_2_0</at:op-code>
      <at:start.use>2002-02-01</at:start.use>
      <atold:op-code>ZPL_2_0</atold:op-code>
      <dc:identifier>ZPL_2_0</dc:identifier>
      <skos:altLabel xml:lang="bg">ZPL-2.0</skos:altLabel>
      <skos:altLabel xml:lang="cs">ZPL-2.0</skos:altLabel>
      <skos:altLabel xml:lang="da">ZPL-2.0</skos:altLabel>
      <skos:altLabel xml:lang="de">ZPL-2.0</skos:altLabel>
      <skos:altLabel xml:lang="el">ZPL-2.0</skos:altLabel>
      <skos:altLabel xml:lang="en">ZPL-2.0</skos:altLabel>
      <skos:altLabel xml:lang="es">ZPL-2.0</skos:altLabel>
      <skos:altLabel xml:lang="et">ZPL-2.0</skos:altLabel>
      <skos:altLabel xml:lang="fi">ZPL-2.0</skos:altLabel>
      <skos:altLabel xml:lang="fr">ZPL-2.0</skos:altLabel>
      <skos:altLabel xml:lang="ga">ZPL-2.0</skos:altLabel>
      <skos:altLabel xml:lang="hr">ZPL-2.0</skos:altLabel>
      <skos:altLabel xml:lang="hu">ZPL-2.0</skos:altLabel>
      <skos:altLabel xml:lang="it">ZPL-2.0</skos:altLabel>
      <skos:altLabel xml:lang="lt">ZPL-2.0</skos:altLabel>
      <skos:altLabel xml:lang="lv">ZPL-2.0</skos:altLabel>
      <skos:altLabel xml:lang="mt">ZPL-2.0</skos:altLabel>
      <skos:altLabel xml:lang="nl">ZPL-2.0</skos:altLabel>
      <skos:altLabel xml:lang="pl">ZPL-2.0</skos:altLabel>
      <skos:altLabel xml:lang="pt">ZPL-2.0</skos:altLabel>
      <skos:altLabel xml:lang="ro">ZPL-2.0</skos:altLabel>
      <skos:altLabel xml:lang="sk">ZPL-2.0</skos:altLabel>
      <skos:altLabel xml:lang="sl">ZPL-2.0</skos:altLabel>
      <skos:altLabel xml:lang="sv">ZPL-2.0</skos:altLabel>
      <skos:changeNote xml:lang="en">The source of the start-use date: Open Source Software: From Open Science to New Marketing Model, p. 116</skos:changeNote>
      <skos:definition xml:lang="en">The Zope Public License Version 2.0 is a free software licence approved by the Open Source Initiative, used primarily for the Zope application server software. It is similar to the well-known BSD license, however the ZPL also adds clauses prohibiting trademark use and requiring documentation of all changes.</skos:definition>
      <skos:exactMatch rdf:resource="https://opensource.org/licenses/ZPL-2.0"/>
      <skos:inScheme rdf:resource="http://publications.europa.eu/resource/authority/licence"/>
      <skos:topConceptOf rdf:resource="http://publications.europa.eu/resource/authority/licence"/>
   </skos:Concept>
</rdf:RDF>
